{"@context":{"rdf":"http://www.w3.org/1999/02/22-rdf-syntax-ns#","owl":"http://www.w3.org/2002/07/owl#","rdfs":"http://www.w3.org/2000/01/rdf-schema#","schema":"https://schema.org/","unece":"https://vocabulary.uncefact.org/"},"@graph":[{"@id":"unece:AgriculturalCertificate","@type":"rdfs:Class","rdfs:label":"AgriculturalCertificate","schema:source":{"@id":"https://vocabulary.uncefact.org/AgriculturalCertificate"},"rdfs:comment":"A legal proof of ownership, worthiness or qualification to operate an agricultural item."},{"@id":"unece:AgriculturalProcess","@type":"rdfs:Class","rdfs:label":"AgriculturalProcess","schema:source":{"@id":"https://vocabulary.uncefact.org/AgriculturalProcess"},"rdfs:comment":"A practice of cultivating land, raising crops, or treatment of the agricultural produce."},{"@id":"unece:Area","@type":"rdfs:Class","rdfs:label":"Area","schema:source":{"@id":"https://vocabulary.uncefact.org/Area"},"rdfs:comment":"A named, delimited and identified part of a land and or water surface of the globe subject to dedicated uniform agricultural treatment."},{"@id":"unece:FieldCrop","@type":"rdfs:Class","rdfs:label":"FieldCrop","schema:source":{"@id":"https://vocabulary.uncefact.org/FieldCrop"},"rdfs:comment":"A field with one or more cultivated plants or produce from one or more botanical species or varieties."},{"@id":"unece:Plot","@type":"rdfs:Class","rdfs:label":"Plot","schema:source":{"@id":"https://vocabulary.uncefact.org/Plot"},"rdfs:comment":"A small piece of land or water used for a crop such as an agricultural or aquacultural crop."},{"@id":"unece:AnimalCertificate","@type":"rdfs:Class","rdfs:label":"AnimalCertificate","schema:source":{"@id":"https://vocabulary.uncefact.org/AnimalCertificate"},"rdfs:comment":"A collection of data for a piece of written, printed or electronic matter that provides information or evidence about the identity of an animal or a batch of animals."},{"@id":"unece:CropProtectionTreatment","@type":"rdfs:Class","rdfs:label":"CropProtectionTreatment","schema:source":{"@id":"https://vocabulary.uncefact.org/CropProtectionTreatment"},"rdfs:comment":"A method or substance, such as chemical fertilizers and crop protection products, applied to plant growth whilst managing and controlling diseases and pests."},{"@id":"unece:AgriculturalApplication","@type":"rdfs:Class","rdfs:label":"AgriculturalApplication","schema:source":{"@id":"https://vocabulary.uncefact.org/AgriculturalApplication"},"rdfs:comment":"Any substance such as seed, fertilizer, water, gas or chemical applied to an agricultural field, substrate, construction, plant, animal or product."},{"@id":"unece:CropProduceBatch","@type":"rdfs:Class","rdfs:label":"CropProduceBatch","schema:source":{"@id":"https://vocabulary.uncefact.org/CropProduceBatch"},"rdfs:comment":"A group of crop produce considered or dealt with together."},{"@id":"unece:AnimalCertification","@type":"rdfs:Class","rdfs:label":"AnimalCertification","schema:source":{"@id":"https://vocabulary.uncefact.org/AnimalCertification"},"rdfs:comment":"The process of certifying that a certain animal has met performance and quality assurance requirements, or qualification requirements as stipulated in regulations."},{"@id":"unece:IndividualTTAnimal","@type":"rdfs:Class","rdfs:label":"IndividualTTAnimal","schema:source":{"@id":"https://vocabulary.uncefact.org/IndividualTTAnimal"},"rdfs:comment":"A Track and Trace (TT) animal, such as one kept or raised on a farm, ranch."},{"@id":"unece:BotanicalCrop","@type":"rdfs:Class","rdfs:label":"BotanicalCrop","schema:source":{"@id":"https://vocabulary.uncefact.org/BotanicalCrop"},"rdfs:comment":"Plants or produce cultivated from a single botanical species or variety."},{"@id":"unece:AnimalBatch","@type":"rdfs:Class","rdfs:label":"AnimalBatch","schema:source":{"@id":"https://vocabulary.uncefact.org/AnimalBatch"},"rdfs:comment":"A group of animals dealt with together."},{"@id":"unece:Produce","@type":"rdfs:Class","rdfs:label":"Produce","schema:source":{"@id":"https://vocabulary.uncefact.org/Produce"},"rdfs:comment":"Agricultural plants or plant products grown and harvested, such as grain, fruit, vegetables, silage."},{"@id":"unece:CropMixtureConstituent","@type":"rdfs:Class","rdfs:label":"CropMixtureConstituent","schema:source":{"@id":"https://vocabulary.uncefact.org/CropMixtureConstituent"},"rdfs:comment":"A plant species or variety constituting part of a field crop mixture."},{"@id":"unece:AgriculturalCharacteristic","@type":"rdfs:Class","rdfs:label":"AgriculturalCharacteristic","schema:source":{"@id":"https://vocabulary.uncefact.org/AgriculturalCharacteristic"},"rdfs:comment":"A prominent attribute or aspect of an agricultural object."},{"@id":"unece:AnimalIdentity","@type":"rdfs:Class","rdfs:label":"AnimalIdentity","schema:source":{"@id":"https://vocabulary.uncefact.org/AnimalIdentity"},"rdfs:comment":"Information about an animal which uniquely identifies it."},{"@id":"unece:AnimalHoldingEvent","@type":"rdfs:Class","rdfs:label":"AnimalHoldingEvent","schema:source":{"@id":"https://vocabulary.uncefact.org/AnimalHoldingEvent"},"rdfs:comment":"The keeping of an animal in a particular location."},{"@id":"unece:SpeciesTTAnimal","@type":"rdfs:Class","rdfs:label":"SpeciesTTAnimal","schema:source":{"@id":"https://vocabulary.uncefact.org/SpeciesTTAnimal"},"rdfs:comment":"The species of a Track and Trace (TT) animal or batch of animals."},{"@id":"unece:actualEffectiveDateTime","@type":["rdf:Property","owl:DatatypeProperty"],"rdfs:label":"actualEffectiveDateTime","schema:rangeIncludes":{"@id":"schema:Text"},"schema:domainIncludes":[{"@id":"unece:AgriculturalCertificate"},{"@id":"unece:OrganizationalCertificate"},{"@id":"unece:ProcessCertificate"},{"@id":"unece:ProductBatchCertificate"},{"@id":"unece:ProductCertificate"},{"@id":"unece:SpecifiedCertificate"}],"rdfs:comment":"The actual effective date, time, date time or other date time value for this agricultural certificate."},{"@id":"unece:applicableAssertion","@type":["rdf:Property","owl:ObjectProperty"],"rdfs:label":"applicableAssertion","schema:rangeIncludes":{"@id":"unece:Assertion"},"schema:domainIncludes":[{"@id":"unece:AgriculturalCertificate"},{"@id":"unece:AnimalCertificate"},{"@id":"unece:OrganizationalCertificate"},{"@id":"unece:ProcessCertificate"},{"@id":"unece:ProductBatchCertificate"},{"@id":"unece:ProductCertificate"}],"rdfs:comment":"A statement that user needs of the present are met without compromising the needs of future generations."},{"@id":"unece:applicableObjectCode","@type":["rdf:Property","owl:DatatypeProperty"],"rdfs:label":"applicableObjectCode","schema:rangeIncludes":{"@id":"schema:Text"},"schema:domainIncludes":[{"@id":"unece:AgriculturalCertificate"},{"@id":"unece:OrganizationalCertificate"},{"@id":"unece:ProcessCertificate"},{"@id":"unece:ProductBatchCertificate"},{"@id":"unece:ProductCertificate"}],"rdfs:comment":"A code specifying an applicable object, such as item, animal, person or organization, for this agricultural certificate."},{"@id":"unece:applicableStandard","@type":["rdf:Property","owl:ObjectProperty"],"rdfs:label":"applicableStandard","schema:rangeIncludes":{"@id":"unece:Standard"},"schema:domainIncludes":[{"@id":"unece:AgriculturalCertificate"},{"@id":"unece:AnimalCertificate"},{"@id":"unece:OrganizationalCertificate"},{"@id":"unece:ProcessCertificate"},{"@id":"unece:ProductBatchCertificate"},{"@id":"unece:ProductCertificate"},{"@id":"unece:SpecifiedCertificate"},{"@id":"unece:ProductCharacteristic"},{"@id":"unece:ProductBatchCharacteristic"},{"@id":"unece:SustainabilityCharacteristic"},{"@id":"unece:SustainabilityInspection"},{"@id":"unece:Assertion"},{"@id":"unece:Assessment"},{"@id":"unece:OrganizationalCertification"},{"@id":"unece:Policy"},{"@id":"unece:ProcessCertification"},{"@id":"unece:ProcessCharacteristic"},{"@id":"unece:ProductBatchCertification"},{"@id":"unece:TechnicalCharacteristic"},{"@id":"unece:OrganizationCharacteristic"},{"@id":"unece:TradeProductCertification"}],"rdfs:comment":"A referenced norm or requirement that establishes uniform criteria, methods, processes and practices, such as in engineering or technical areas."},{"@id":"unece:applicableSustainabilityCharacteristic","@type":["rdf:Property","owl:ObjectProperty"],"rdfs:label":"applicableSustainabilityCharacteristic","schema:rangeIncludes":{"@id":"unece:SustainabilityCharacteristic"},"schema:domainIncludes":[{"@id":"unece:AgriculturalCertificate"},{"@id":"unece:AnimalCertificate"},{"@id":"unece:CropProtectionTreatment"},{"@id":"unece:AgriculturalApplication"},{"@id":"unece:OrganizationalCertificate"},{"@id":"unece:ProcessCertificate"},{"@id":"unece:ProductBatchCertificate"},{"@id":"unece:ProductCertificate"},{"@id":"unece:SpecifiedCertificate"},{"@id":"unece:ProductCharacteristic"},{"@id":"unece:Chemical"},{"@id":"unece:SustainabilityInspection"},{"@id":"unece:HazardousMaterial"},{"@id":"unece:Assessment"},{"@id":"unece:ProcessCharacteristic"},{"@id":"unece:OrganizationCharacteristic"},{"@id":"unece:SpecifiedMaterial"},{"@id":"unece:ProductionWasteMaterial"},{"@id":"unece:ProductionWasteMaterialComponent"}],"rdfs:comment":"A prominent attribute or aspect of an object, such as recyclability of a product, which can meet customer needs without compromising the ability of future generations to meet their own needs."},{"@id":"unece:attachedBinaryFile","@type":["rdf:Property","owl:ObjectProperty"],"rdfs:label":"attachedBinaryFile","schema:rangeIncludes":{"@id":"unece:BinaryFile"},"schema:domainIncludes":[{"@id":"unece:AgriculturalCertificate"},{"@id":"unece:Document"},{"@id":"unece:ExchangedDocument"},{"@id":"unece:Picture"},{"@id":"unece:OrganizationalCertificate"},{"@id":"unece:ProcessCertificate"},{"@id":"unece:ProductBatchCertificate"},{"@id":"unece:ProductCertificate"},{"@id":"unece:SpecifiedCertificate"},{"@id":"unece:Standard"},{"@id":"unece:InspectionResult"},{"@id":"unece:SustainabilityInspection"},{"@id":"unece:SpecifiedInspection"}],"rdfs:comment":"A specified computer file or program stored in a binary format."},{"@id":"unece:certificateTypeCode","@type":["rdf:Property","owl:DatatypeProperty"],"rdfs:label":"certificateTypeCode","schema:rangeIncludes":{"@id":"unece:CertificateTypeCodeList"},"schema:domainIncludes":[{"@id":"unece:AgriculturalCertificate"},{"@id":"unece:AnimalCertificate"},{"@id":"unece:OrganizationalCertificate"},{"@id":"unece:ProcessCertificate"},{"@id":"unece:ProductBatchCertificate"},{"@id":"unece:ProductCertificate"},{"@id":"unece:SpecifiedCertificate"},{"@id":"unece:ConformanceCertificate"}],"rdfs:comment":"A code specifying a type of specified certificate."},{"@id":"unece:description","@type":["rdf:Property","owl:DatatypeProperty"],"rdfs:label":"description","schema:rangeIncludes":{"@id":"schema:Text"},"schema:domainIncludes":[{"@id":"unece:AgriculturalCertificate"},{"@id":"unece:AgriculturalProcess"},{"@id":"unece:FieldCrop"},{"@id":"unece:CropProtectionTreatment"},{"@id":"unece:AgriculturalCharacteristic"},{"@id":"unece:Document"},{"@id":"unece:ExchangedDocument"},{"@id":"unece:BinaryFile"},{"@id":"unece:SpecifiedAction"},{"@id":"unece:Measurement"},{"@id":"unece:QuantityAnalysis"},{"@id":"unece:SpecifiedFault"},{"@id":"unece:Picture"},{"@id":"unece:UsageCondition"},{"@id":"unece:Location"},{"@id":"unece:CommunicationEvent"},{"@id":"unece:CustomerClass"},{"@id":"unece:InformationSource"},{"@id":"unece:GeographicalFeature"},{"@id":"unece:Communication"},{"@id":"unece:SpecifiedPeriod"},{"@id":"unece:WorkItemDimension"},{"@id":"unece:DocumentStatus"},{"@id":"unece:Project"},{"@id":"unece:SpecifiedNote"},{"@id":"unece:MetricCharacteristic"},{"@id":"unece:AvailablePeriod"},{"@id":"unece:DocumentCharacteristic"},{"@id":"unece:GeographicalObjectCharacteristic"},{"@id":"unece:IdentifiedFault"},{"@id":"unece:Membership"},{"@id":"unece:Schedule"},{"@id":"unece:SpatialDimension"},{"@id":"unece:SpecifiedFeature"},{"@id":"unece:SpecifiedLocation"},{"@id":"unece:SpecifiedParameter"},{"@id":"unece:Address"},{"@id":"unece:Event"},{"@id":"unece:InspectionReference"},{"@id":"unece:LaboratoryObservationReference"},{"@id":"unece:ProtectionMeans"},{"@id":"unece:Accreditation"},{"@id":"unece:CorrectiveAction"},{"@id":"unece:PreventiveAction"},{"@id":"unece:OrganizationalCertificate"},{"@id":"unece:ProcessCertificate"},{"@id":"unece:ProductBatchCertificate"},{"@id":"unece:ProductCertificate"},{"@id":"unece:SpecifiedCertificate"},{"@id":"unece:Standard"},{"@id":"unece:ProcessWorkItem"},{"@id":"unece:ProductCharacteristic"},{"@id":"unece:ProductBatchCharacteristic"},{"@id":"unece:SustainabilityCharacteristic"},{"@id":"unece:SustainabilityInspection"},{"@id":"unece:Observation"},{"@id":"unece:HazardousMaterial"},{"@id":"unece:Assertion"},{"@id":"unece:Policy"},{"@id":"unece:ProcessCharacteristic"},{"@id":"unece:TechnicalCharacteristic"},{"@id":"unece:Licence"},{"@id":"unece:SpecifiedDeclaration"},{"@id":"unece:SpecifiedInspection"},{"@id":"unece:Source"},{"@id":"unece:RiskAnalysisResult"},{"@id":"unece:ControlSettingParameter"},{"@id":"unece:OperationalParameter"},{"@id":"unece:InspectionStatus"},{"@id":"unece:DisposalInstructions"},{"@id":"unece:InspectionEvent"},{"@id":"unece:InspectionInstructions"},{"@id":"unece:LaboratoryObservationInstructions"},{"@id":"unece:ObservationObjectiveParameter"},{"@id":"unece:QuarantineInstructions"},{"@id":"unece:Requirement"},{"@id":"unece:TemperatureSettingInstructions"},{"@id":"unece:OrganizationCharacteristic"},{"@id":"unece:GoodsCharacteristic"},{"@id":"unece:SpecifiedMaterial"},{"@id":"unece:WasteMaterialRecoveryDisposalProcess"},{"@id":"unece:TransportInstructions"},{"@id":"unece:IngredientRangeMeasurement"},{"@id":"unece:ProductionWasteMaterialComponent"},{"@id":"unece:ProductionWasteRecoveryDisposalProcess"}],"rdfs:comment":"A textual description for the type of transportation waste recovery disposal process."},{"@id":"unece:expiryDateTime","@type":["rdf:Property","owl:DatatypeProperty"],"rdfs:label":"expiryDateTime","schema:rangeIncludes":{"@id":"schema:Text"},"schema:domainIncludes":[{"@id":"unece:AgriculturalCertificate"},{"@id":"unece:Accreditation"},{"@id":"unece:OrganizationalCertificate"},{"@id":"unece:ProcessCertificate"},{"@id":"unece:ProductBatchCertificate"},{"@id":"unece:ProductCertificate"},{"@id":"unece:SpecifiedCertificate"},{"@id":"unece:Licence"}],"rdfs:comment":"An expiry date, time, date time or other date time value for this specified licence."},{"@id":"unece:identifier","@type":["rdf:Property","owl:DatatypeProperty"],"rdfs:label":"identifier","schema:rangeIncludes":{"@id":"schema:Text"},"schema:domainIncludes":[{"@id":"unece:AgriculturalCertificate"},{"@id":"unece:Area"},{"@id":"unece:Plot"},{"@id":"unece:AnimalCertificate"},{"@id":"unece:CropProtectionTreatment"},{"@id":"unece:AgriculturalApplication"},{"@id":"unece:CropProduceBatch"},{"@id":"unece:IndividualTTAnimal"},{"@id":"unece:AnimalBatch"},{"@id":"unece:Produce"},{"@id":"unece:AgriculturalCharacteristic"},{"@id":"unece:AnimalIdentity"},{"@id":"unece:Document"},{"@id":"unece:ExchangedDocument"},{"@id":"unece:BinaryFile"},{"@id":"unece:GeographicalCoordinate"},{"@id":"unece:CountrySubDivision"},{"@id":"unece:QuantityAnalysis"},{"@id":"unece:Picture"},{"@id":"unece:SpecifiedMethod"},{"@id":"unece:Location"},{"@id":"unece:CommunicationEvent"},{"@id":"unece:GeographicalGrid"},{"@id":"unece:LegalOrganization"},{"@id":"unece:Object"},{"@id":"unece:GeographicalFeature"},{"@id":"unece:SpecifiedPeriod"},{"@id":"unece:WorkItemDimension"},{"@id":"unece:Project"},{"@id":"unece:Note"},{"@id":"unece:Response"},{"@id":"unece:SpecialQuery"},{"@id":"unece:SpecifiedNote"},{"@id":"unece:MetricCharacteristic"},{"@id":"unece:LegalRegistration"},{"@id":"unece:DocumentCharacteristic"},{"@id":"unece:GeographicalObjectCharacteristic"},{"@id":"unece:Membership"},{"@id":"unece:Schedule"},{"@id":"unece:SpatialDimension"},{"@id":"unece:SpecifiedParameter"},{"@id":"unece:ProprietaryIdentity"},{"@id":"unece:CoordinateReferenceSystem"},{"@id":"unece:CoordinateSourceSystem"},{"@id":"unece:DocumentContextParameter"},{"@id":"unece:EmployerIdentity"},{"@id":"unece:GeopoliticalRegion"},{"@id":"unece:Issue"},{"@id":"unece:Radionuclide"},{"@id":"unece:Section"},{"@id":"unece:Segment"},{"@id":"unece:SubordinateLocation"},{"@id":"unece:SubordinateSubordinateLocation"},{"@id":"unece:Version"},{"@id":"unece:WorkflowObject"},{"@id":"unece:Party"},{"@id":"unece:Authentication"},{"@id":"unece:Clause"},{"@id":"unece:Address"},{"@id":"unece:Event"},{"@id":"unece:SpecificationQuery"},{"@id":"unece:Person"},{"@id":"unece:InspectionReference"},{"@id":"unece:LaboratoryObservationReference"},{"@id":"unece:Accreditation"},{"@id":"unece:OrganizationalCertificate"},{"@id":"unece:ProcessCertificate"},{"@id":"unece:ProductBatchCertificate"},{"@id":"unece:ProductCertificate"},{"@id":"unece:SpecifiedCertificate"},{"@id":"unece:ObservationResult"},{"@id":"unece:Standard"},{"@id":"unece:ProcessWorkItem"},{"@id":"unece:ProductCharacteristic"},{"@id":"unece:InspectionResult"},{"@id":"unece:ProductBatchCharacteristic"},{"@id":"unece:Chemical"},{"@id":"unece:SustainabilityCharacteristic"},{"@id":"unece:SustainabilityInspection"},{"@id":"unece:Observation"},{"@id":"unece:Assertion"},{"@id":"unece:Policy"},{"@id":"unece:ProcessCharacteristic"},{"@id":"unece:TechnicalCharacteristic"},{"@id":"unece:SpecifiedCertification"},{"@id":"unece:Licence"},{"@id":"unece:SpecifiedDeclaration"},{"@id":"unece:TaxRegistration"},{"@id":"unece:SpecifiedInspection"},{"@id":"unece:Source"},{"@id":"unece:GovernmentRegistration"},{"@id":"unece:ConformanceCertificate"},{"@id":"unece:LaboratoryObservationAnalysisMethod"},{"@id":"unece:ControlSettingParameter"},{"@id":"unece:OperationalParameter"},{"@id":"unece:LaboratoryObservationContact"},{"@id":"unece:InspectionInstructions"},{"@id":"unece:LaboratoryObservationInstructions"},{"@id":"unece:ObservationObjectiveParameter"},{"@id":"unece:CalibratedMeasurement"},{"@id":"unece:CorrectiveEvent"},{"@id":"unece:LaboratoryObservationParty"},{"@id":"unece:OrganizationCharacteristic"},{"@id":"unece:SpecifiedMaterial"},{"@id":"unece:Seal"}],"rdfs:comment":"A proprietary identifier."},{"@id":"unece:issueDateTime","@type":["rdf:Property","owl:DatatypeProperty"],"rdfs:label":"issueDateTime","schema:rangeIncludes":{"@id":"schema:Text"},"schema:domainIncludes":[{"@id":"unece:AgriculturalCertificate"},{"@id":"unece:Document"},{"@id":"unece:ExchangedDocument"},{"@id":"unece:Error"},{"@id":"unece:Version"},{"@id":"unece:OrganizationalCertificate"},{"@id":"unece:ProcessCertificate"},{"@id":"unece:ProductBatchCertificate"},{"@id":"unece:ProductCertificate"},{"@id":"unece:SpecifiedCertificate"},{"@id":"unece:Licence"},{"@id":"unece:SpecifiedDeclaration"},{"@id":"unece:ConformanceCertificate"}],"rdfs:comment":"An issue date, time, date time or other date time value for this declared error."},{"@id":"unece:issueReasonCode","@type":["rdf:Property","owl:DatatypeProperty"],"rdfs:label":"issueReasonCode","schema:rangeIncludes":{"@id":"schema:Text"},"schema:domainIncludes":[{"@id":"unece:AgriculturalCertificate"},{"@id":"unece:OrganizationalCertificate"},{"@id":"unece:ProcessCertificate"},{"@id":"unece:ProductBatchCertificate"},{"@id":"unece:ProductCertificate"},{"@id":"unece:SpecifiedCertificate"}],"rdfs:comment":"The code specifying the reason for the issue of this process certificate."},{"@id":"unece:issuingPartyId","@type":["rdf:Property","owl:DatatypeProperty"],"rdfs:label":"issuingPartyId","schema:rangeIncludes":{"@id":"schema:Text"},"schema:domainIncludes":[{"@id":"unece:AgriculturalCertificate"},{"@id":"unece:OrganizationalCertificate"},{"@id":"unece:ProcessCertificate"},{"@id":"unece:ProductBatchCertificate"},{"@id":"unece:ProductCertificate"},{"@id":"unece:Assertion"},{"@id":"unece:ConformanceCertificate"}],"rdfs:comment":"An identifier of a party issuing this sustainability assertion."},{"@id":"unece:purposeCode","@type":["rdf:Property","owl:DatatypeProperty"],"rdfs:label":"purposeCode","schema:rangeIncludes":{"@id":"schema:Text"},"schema:domainIncludes":[{"@id":"unece:AgriculturalCertificate"},{"@id":"unece:FieldCrop"},{"@id":"unece:SpecifiedPeriod"},{"@id":"unece:OrganizationalCertificate"},{"@id":"unece:ProcessCertificate"},{"@id":"unece:ProductBatchCertificate"},{"@id":"unece:ProductCertificate"},{"@id":"unece:SpecifiedCertificate"}],"rdfs:comment":"A code specifying a purpose for this field crop."},{"@id":"unece:requestedEffectiveDateTime","@type":["rdf:Property","owl:DatatypeProperty"],"rdfs:label":"requestedEffectiveDateTime","schema:rangeIncludes":{"@id":"schema:Text"},"schema:domainIncludes":[{"@id":"unece:AgriculturalCertificate"},{"@id":"unece:OrganizationalCertificate"},{"@id":"unece:ProcessCertificate"},{"@id":"unece:ProductBatchCertificate"},{"@id":"unece:ProductCertificate"},{"@id":"unece:SpecifiedCertificate"}],"rdfs:comment":"The requested effective date, time, date time or other date time value for this agricultural certificate."},{"@id":"unece:actualEndDateTime","@type":["rdf:Property","owl:DatatypeProperty"],"rdfs:label":"actualEndDateTime","schema:rangeIncludes":{"@id":"schema:Text"},"schema:domainIncludes":{"@id":"unece:AgriculturalProcess"},"rdfs:comment":"The date, time, date time or other date time value of the actual end for the crop production in this agricultural process."},{"@id":"unece:actualStartDateTime","@type":["rdf:Property","owl:DatatypeProperty"],"rdfs:label":"actualStartDateTime","schema:rangeIncludes":{"@id":"schema:Text"},"schema:domainIncludes":{"@id":"unece:AgriculturalProcess"},"rdfs:comment":"The date, time, date time or other date time value for the actual start of the crop production in this agricultural process."},{"@id":"unece:appliedAgriculturalApplication","@type":["rdf:Property","owl:ObjectProperty"],"rdfs:label":"appliedAgriculturalApplication","schema:rangeIncludes":{"@id":"unece:AgriculturalApplication"},"schema:domainIncludes":[{"@id":"unece:AgriculturalProcess"},{"@id":"unece:Area"},{"@id":"unece:FieldCrop"},{"@id":"unece:Plot"}],"rdfs:comment":"A specified agricultural application applied to this agricultural zone area."},{"@id":"unece:earliestStartDateTime","@type":["rdf:Property","owl:DatatypeProperty"],"rdfs:label":"earliestStartDateTime","schema:rangeIncludes":{"@id":"schema:Text"},"schema:domainIncludes":{"@id":"unece:AgriculturalProcess"},"rdfs:comment":"The date, time, date time or other date time value for the earliest start of the crop production in this agricultural process."},{"@id":"unece:harvestedBatch","@type":["rdf:Property","owl:ObjectProperty"],"rdfs:label":"harvestedBatch","schema:rangeIncludes":{"@id":"unece:CropProduceBatch"},"schema:domainIncludes":{"@id":"unece:AgriculturalProcess"},"rdfs:comment":"A crop produce batch harvested in the crop production for this agricultural process."},{"@id":"unece:latestEndDateTime","@type":["rdf:Property","owl:DatatypeProperty"],"rdfs:label":"latestEndDateTime","schema:rangeIncludes":{"@id":"schema:Text"},"schema:domainIncludes":{"@id":"unece:AgriculturalProcess"},"rdfs:comment":"The date, time, date time or other date time value of the latest end for the crop production in this agricultural process."},{"@id":"unece:productionWasteInstructions","@type":["rdf:Property","owl:ObjectProperty"],"rdfs:label":"productionWasteInstructions","schema:rangeIncludes":{"@id":"unece:DisposalInstructions"},"schema:domainIncludes":{"@id":"unece:AgriculturalProcess"},"rdfs:comment":"A set of instructions detailing how to properly dispose of a material."},{"@id":"unece:reportedProductionWasteMaterial","@type":["rdf:Property","owl:ObjectProperty"],"rdfs:label":"reportedProductionWasteMaterial","schema:rangeIncludes":{"@id":"unece:ProductionWasteMaterial"},"schema:domainIncludes":{"@id":"unece:AgriculturalProcess"},"rdfs:comment":"Any materials unused and rejected as unwanted during a production process."},{"@id":"unece:specifiedFieldCrop","@type":["rdf:Property","owl:ObjectProperty"],"rdfs:label":"specifiedFieldCrop","schema:rangeIncludes":{"@id":"unece:FieldCrop"},"schema:domainIncludes":{"@id":"unece:AgriculturalProcess"},"rdfs:comment":"A field crop specified for this crop production agricultural process."},{"@id":"unece:statusCode","@type":["rdf:Property","owl:DatatypeProperty"],"rdfs:label":"statusCode","schema:rangeIncludes":{"@id":"schema:Text"},"schema:domainIncludes":[{"@id":"unece:AgriculturalProcess"},{"@id":"unece:Schedule"},{"@id":"unece:SpecifiedParameter"},{"@id":"unece:SpecifiedCertificate"},{"@id":"unece:InspectionResult"},{"@id":"unece:Assertion"},{"@id":"unece:Assessment"},{"@id":"unece:ControlSettingParameter"},{"@id":"unece:OperationalParameter"},{"@id":"unece:InspectionInstructions"},{"@id":"unece:LaboratoryObservationInstructions"},{"@id":"unece:ObservationObjectiveParameter"},{"@id":"unece:SpecifiedMaterial"}],"rdfs:comment":"A code specifying a status for this trade product."},{"@id":"unece:subordinateTypeCode","@type":["rdf:Property","owl:DatatypeProperty"],"rdfs:label":"subordinateTypeCode","schema:rangeIncludes":{"@id":"schema:Text"},"schema:domainIncludes":[{"@id":"unece:AgriculturalProcess"},{"@id":"unece:Produce"},{"@id":"unece:SustainabilityCharacteristic"},{"@id":"unece:TechnicalCharacteristic"}],"rdfs:comment":"The code specifying the subordinate type for this production device."},{"@id":"unece:typeCode","@type":["rdf:Property","owl:DatatypeProperty"],"rdfs:label":"typeCode","schema:rangeIncludes":{"@id":"schema:Text"},"schema:domainIncludes":[{"@id":"unece:AgriculturalProcess"},{"@id":"unece:CropProtectionTreatment"},{"@id":"unece:CropProduceBatch"},{"@id":"unece:Produce"},{"@id":"unece:AgriculturalCharacteristic"},{"@id":"unece:AnimalHoldingEvent"},{"@id":"unece:SpecifiedAction"},{"@id":"unece:CountrySubDivision"},{"@id":"unece:Measurement"},{"@id":"unece:QuantityAnalysis"},{"@id":"unece:SpecifiedFault"},{"@id":"unece:RadioactiveMaterial"},{"@id":"unece:CommunicationEvent"},{"@id":"unece:LegalOrganization"},{"@id":"unece:Object"},{"@id":"unece:SpecifiedPeriod"},{"@id":"unece:Project"},{"@id":"unece:MetricCharacteristic"},{"@id":"unece:LegalRegistration"},{"@id":"unece:DocumentCharacteristic"},{"@id":"unece:Schedule"},{"@id":"unece:SpecifiedFeature"},{"@id":"unece:SpecifiedParameter"},{"@id":"unece:Range"},{"@id":"unece:GeopoliticalRegion"},{"@id":"unece:Issue"},{"@id":"unece:Segment"},{"@id":"unece:SecurityTag"},{"@id":"unece:SpecificationQuery"},{"@id":"unece:Accreditation"},{"@id":"unece:CorrectiveAction"},{"@id":"unece:PreventiveAction"},{"@id":"unece:Standard"},{"@id":"unece:ProcessWorkItem"},{"@id":"unece:ProductCharacteristic"},{"@id":"unece:ProductBatchCharacteristic"},{"@id":"unece:Chemical"},{"@id":"unece:SustainabilityCharacteristic"},{"@id":"unece:SustainabilityInspection"},{"@id":"unece:Assessment"},{"@id":"unece:TechnicalCharacteristic"},{"@id":"unece:Licence"},{"@id":"unece:SpecifiedDeclaration"},{"@id":"unece:SpecifiedInspection"},{"@id":"unece:GovernmentRegistration"},{"@id":"unece:ControlSettingParameter"},{"@id":"unece:OperationalParameter"},{"@id":"unece:InspectionEvent"},{"@id":"unece:ObservationObjectiveParameter"},{"@id":"unece:Requirement"},{"@id":"unece:ProductCharacteristicCondition"},{"@id":"unece:OrganizationCharacteristic"},{"@id":"unece:GoodsCharacteristic"},{"@id":"unece:SpecifiedMaterial"},{"@id":"unece:WasteMaterialRecoveryDisposalProcess"},{"@id":"unece:ProductionWasteMaterial"},{"@id":"unece:ProductionWasteMaterialComponent"},{"@id":"unece:ProductionWasteRecoveryDisposalProcess"}],"rdfs:comment":"A code specifying a type of MDH health indication."},{"@id":"unece:applicableAgriculturalCharacteristic","@type":["rdf:Property","owl:ObjectProperty"],"rdfs:label":"applicableAgriculturalCharacteristic","schema:rangeIncludes":{"@id":"unece:AgriculturalCharacteristic"},"schema:domainIncludes":{"@id":"unece:Area"},"rdfs:comment":"An agricultural characteristic applicable to this agricultural zone area."},{"@id":"unece:designatedSection","@type":["rdf:Property","owl:DatatypeProperty"],"rdfs:label":"designatedSection","schema:rangeIncludes":{"@id":"schema:Text"},"schema:domainIncludes":{"@id":"unece:Area"},"rdfs:comment":"The designated section, expressed as text, of this agricultural zone area."},{"@id":"unece:harvestedProduce","@type":["rdf:Property","owl:ObjectProperty"],"rdfs:label":"harvestedProduce","schema:rangeIncludes":{"@id":"unece:Produce"},"schema:domainIncludes":[{"@id":"unece:Area"},{"@id":"unece:FieldCrop"}],"rdfs:comment":"Crop produce harvested from this agricultural zone area."},{"@id":"unece:multiSurfaceTypeCode","@type":["rdf:Property","owl:DatatypeProperty"],"rdfs:label":"multiSurfaceTypeCode","schema:rangeIncludes":{"@id":"schema:Text"},"schema:domainIncludes":{"@id":"unece:Area"},"rdfs:comment":"The code specifying the multi-surface type for this agricultural zone area."},{"@id":"unece:name","@type":["rdf:Property","owl:DatatypeProperty"],"rdfs:label":"name","schema:rangeIncludes":{"@id":"schema:Text"},"schema:domainIncludes":[{"@id":"unece:Area"},{"@id":"unece:Produce"},{"@id":"unece:Document"},{"@id":"unece:ExchangedDocument"},{"@id":"unece:CountrySubDivision"},{"@id":"unece:RadioactiveIsotope"},{"@id":"unece:SpecifiedMethod"},{"@id":"unece:Location"},{"@id":"unece:LegalOrganization"},{"@id":"unece:DirectPosition"},{"@id":"unece:DirectPositionList"},{"@id":"unece:InformationSource"},{"@id":"unece:GeographicalFeature"},{"@id":"unece:SpecifiedPeriod"},{"@id":"unece:Project"},{"@id":"unece:SpecifiedNote"},{"@id":"unece:Country"},{"@id":"unece:DocumentCharacteristic"},{"@id":"unece:GeographicalObjectCharacteristic"},{"@id":"unece:Membership"},{"@id":"unece:SpecifiedLocation"},{"@id":"unece:SpecifiedParameter"},{"@id":"unece:CoordinateReferenceSystem"},{"@id":"unece:GeopoliticalRegion"},{"@id":"unece:Radionuclide"},{"@id":"unece:SubordinateLocation"},{"@id":"unece:SubordinateSubordinateLocation"},{"@id":"unece:Version"},{"@id":"unece:CooperatingOrganization"},{"@id":"unece:Keyword"},{"@id":"unece:AcademicQualification"},{"@id":"unece:SpecifiedCertificate"},{"@id":"unece:Standard"},{"@id":"unece:SustainabilityInspection"},{"@id":"unece:AppliedChemicalTreatment"},{"@id":"unece:Assessment"},{"@id":"unece:Licence"},{"@id":"unece:SpecifiedDeclaration"},{"@id":"unece:SpecifiedInspection"},{"@id":"unece:AuthoritativeSignatoryPerson"},{"@id":"unece:Source"},{"@id":"unece:LaboratoryObservationAnalysisMethod"},{"@id":"unece:ControlSettingParameter"},{"@id":"unece:OperationalParameter"},{"@id":"unece:ObservationObjectiveParameter"},{"@id":"unece:LaboratoryObservationParty"},{"@id":"unece:ProductCharacteristicCondition"},{"@id":"unece:SpecifiedQualification"},{"@id":"unece:SpecifiedMaterial"}],"rdfs:comment":"A name or symbol, expressed as text, of a radioactive radionuclide."},{"@id":"unece:specifiedLocation","@type":["rdf:Property","owl:ObjectProperty"],"rdfs:label":"specifiedLocation","schema:rangeIncludes":{"@id":"unece:Location"},"schema:domainIncludes":[{"@id":"unece:Area"},{"@id":"unece:Plot"},{"@id":"unece:AgriculturalApplication"},{"@id":"unece:SpecifiedMaterial"}],"rdfs:comment":"A reference to a physical location or place."},{"@id":"unece:specifiedPlot","@type":["rdf:Property","owl:ObjectProperty"],"rdfs:label":"specifiedPlot","schema:rangeIncludes":{"@id":"unece:Plot"},"schema:domainIncludes":[{"@id":"unece:Area"},{"@id":"unece:AgriculturalApplication"}],"rdfs:comment":"A crop plot specified for this agricultural application."},{"@id":"unece:subordinateArea","@type":["rdf:Property","owl:ObjectProperty"],"rdfs:label":"subordinateArea","schema:rangeIncludes":{"@id":"unece:Area"},"schema:domainIncludes":{"@id":"unece:Area"},"rdfs:comment":"An agricultural zone area subordinate to this agricultural zone area."},{"@id":"unece:thirdPartyIssuedId","@type":["rdf:Property","owl:DatatypeProperty"],"rdfs:label":"thirdPartyIssuedId","schema:rangeIncludes":{"@id":"schema:Text"},"schema:domainIncludes":[{"@id":"unece:Area"},{"@id":"unece:LaboratoryObservationParty"}],"rdfs:comment":"An alternate identifier issued by a third party for this laboratory observation party."},{"@id":"unece:applicableAgriculturalProcess","@type":["rdf:Property","owl:ObjectProperty"],"rdfs:label":"applicableAgriculturalProcess","schema:rangeIncludes":{"@id":"unece:AgriculturalProcess"},"schema:domainIncludes":[{"@id":"unece:FieldCrop"},{"@id":"unece:Plot"}],"rdfs:comment":"An agricultural process crop production applicable for this field crop."},{"@id":"unece:className","@type":["rdf:Property","owl:DatatypeProperty"],"rdfs:label":"className","schema:rangeIncludes":{"@id":"schema:Text"},"schema:domainIncludes":{"@id":"unece:FieldCrop"},"rdfs:comment":"A class name, expressed as text, for this product classification."},{"@id":"unece:classificationCode","@type":["rdf:Property","owl:DatatypeProperty"],"rdfs:label":"classificationCode","schema:rangeIncludes":{"@id":"schema:Text"},"schema:domainIncludes":[{"@id":"unece:FieldCrop"},{"@id":"unece:SpecifiedFault"}],"rdfs:comment":"A code specifying a classification for this field crop."},{"@id":"unece:cultivationContainerCode","@type":["rdf:Property","owl:DatatypeProperty"],"rdfs:label":"cultivationContainerCode","schema:rangeIncludes":{"@id":"schema:Text"},"schema:domainIncludes":{"@id":"unece:FieldCrop"},"rdfs:comment":"The code specifying the type of cultivation container, such as a pot or an iron cabinet, for this field crop."},{"@id":"unece:cultivationCoverageCode","@type":["rdf:Property","owl:DatatypeProperty"],"rdfs:label":"cultivationCoverageCode","schema:rangeIncludes":{"@id":"schema:Text"},"schema:domainIncludes":{"@id":"unece:FieldCrop"},"rdfs:comment":"A code specifying a type of cultivation coverage, such as glass, for this field crop."},{"@id":"unece:cultivationMediumCode","@type":["rdf:Property","owl:DatatypeProperty"],"rdfs:label":"cultivationMediumCode","schema:rangeIncludes":{"@id":"schema:Text"},"schema:domainIncludes":{"@id":"unece:FieldCrop"},"rdfs:comment":"The code specifying the type of cultivation medium, such as substrate, for this field crop."},{"@id":"unece:cultivationTypeCode","@type":["rdf:Property","owl:DatatypeProperty"],"rdfs:label":"cultivationTypeCode","schema:rangeIncludes":{"@id":"schema:Text"},"schema:domainIncludes":{"@id":"unece:FieldCrop"},"rdfs:comment":"The code specifying the type of cultivation for this field crop."},{"@id":"unece:grownPlot","@type":["rdf:Property","owl:ObjectProperty"],"rdfs:label":"grownPlot","schema:rangeIncludes":{"@id":"unece:Plot"},"schema:domainIncludes":{"@id":"unece:FieldCrop"},"rdfs:comment":"The plot where this field crop is grown."},{"@id":"unece:harvestDateTime","@type":["rdf:Property","owl:DatatypeProperty"],"rdfs:label":"harvestDateTime","schema:rangeIncludes":{"@id":"schema:Text"},"schema:domainIncludes":{"@id":"unece:FieldCrop"},"rdfs:comment":"The date, time, date time, or other date time value for the harvest of this field crop."},{"@id":"unece:plantingReasonCode","@type":["rdf:Property","owl:DatatypeProperty"],"rdfs:label":"plantingReasonCode","schema:rangeIncludes":{"@id":"schema:Text"},"schema:domainIncludes":{"@id":"unece:FieldCrop"},"rdfs:comment":"A code specifying a reason for planting this field crop."},{"@id":"unece:productionEnvironmentCode","@type":["rdf:Property","owl:DatatypeProperty"],"rdfs:label":"productionEnvironmentCode","schema:rangeIncludes":{"@id":"schema:Text"},"schema:domainIncludes":{"@id":"unece:FieldCrop"},"rdfs:comment":"The code specifying the production environment for this field crop."},{"@id":"unece:productionPeriodCode","@type":["rdf:Property","owl:DatatypeProperty"],"rdfs:label":"productionPeriodCode","schema:rangeIncludes":{"@id":"schema:Text"},"schema:domainIncludes":{"@id":"unece:FieldCrop"},"rdfs:comment":"The code specifying the production period for this field crop."},{"@id":"unece:propagationMaterialIndicator","@type":["rdf:Property","owl:DatatypeProperty"],"rdfs:label":"propagationMaterialIndicator","schema:rangeIncludes":{"@id":"schema:Boolean"},"schema:domainIncludes":{"@id":"unece:FieldCrop"},"rdfs:comment":"The indication of whether or not a field crop is to be used as propagation material."},{"@id":"unece:sowingPeriodCode","@type":["rdf:Property","owl:DatatypeProperty"],"rdfs:label":"sowingPeriodCode","schema:rangeIncludes":{"@id":"schema:Text"},"schema:domainIncludes":{"@id":"unece:FieldCrop"},"rdfs:comment":"The code specifying the sowing period for this field crop, such as spring or winter."},{"@id":"unece:specifiedAgriculturalCharacteristic","@type":["rdf:Property","owl:ObjectProperty"],"rdfs:label":"specifiedAgriculturalCharacteristic","schema:rangeIncludes":{"@id":"unece:AgriculturalCharacteristic"},"schema:domainIncludes":[{"@id":"unece:FieldCrop"},{"@id":"unece:Plot"},{"@id":"unece:CropProduceBatch"}],"rdfs:comment":"An agricultural characteristic specified for this crop plot."},{"@id":"unece:specifiedCropMixtureConstituent","@type":["rdf:Property","owl:ObjectProperty"],"rdfs:label":"specifiedCropMixtureConstituent","schema:rangeIncludes":{"@id":"unece:CropMixtureConstituent"},"schema:domainIncludes":{"@id":"unece:FieldCrop"},"rdfs:comment":"A field crop mixture constituent specified for this field crop."},{"@id":"unece:areaMeasure","@type":["rdf:Property","owl:ObjectProperty"],"rdfs:label":"areaMeasure","schema:rangeIncludes":{"@id":"unece:MeasureType"},"schema:domainIncludes":{"@id":"unece:Plot"},"rdfs:comment":""},{"@id":"unece:endDateTime","@type":["rdf:Property","owl:DatatypeProperty"],"rdfs:label":"endDateTime","schema:rangeIncludes":{"@id":"schema:Text"},"schema:domainIncludes":[{"@id":"unece:Plot"},{"@id":"unece:SpecifiedPeriod"},{"@id":"unece:AvailablePeriod"},{"@id":"unece:Membership"},{"@id":"unece:DelimitedPeriod"},{"@id":"unece:Assessment"},{"@id":"unece:SpecifiedCertification"}],"rdfs:comment":"The date, time, date time or other date time value for the end of this available period of time."},{"@id":"unece:grownCrop","@type":["rdf:Property","owl:ObjectProperty"],"rdfs:label":"grownCrop","schema:rangeIncludes":{"@id":"unece:FieldCrop"},"schema:domainIncludes":{"@id":"unece:Plot"},"rdfs:comment":"A field crop grown on this crop plot."},{"@id":"unece:regulatoryOrganicIndicator","@type":["rdf:Property","owl:DatatypeProperty"],"rdfs:label":"regulatoryOrganicIndicator","schema:rangeIncludes":{"@id":"schema:Boolean"},"schema:domainIncludes":{"@id":"unece:Plot"},"rdfs:comment":"The indication of whether or not this crop plot is certified as regulatory organic."},{"@id":"unece:regulatorySoilTypeCode","@type":["rdf:Property","owl:DatatypeProperty"],"rdfs:label":"regulatorySoilTypeCode","schema:rangeIncludes":{"@id":"schema:Text"},"schema:domainIncludes":{"@id":"unece:Plot"},"rdfs:comment":"The code specifying the type of regulatory soil for this crop plot."},{"@id":"unece:specifiedAgriculturalCertificate","@type":["rdf:Property","owl:ObjectProperty"],"rdfs:label":"specifiedAgriculturalCertificate","schema:rangeIncludes":{"@id":"unece:AgriculturalCertificate"},"schema:domainIncludes":[{"@id":"unece:Plot"},{"@id":"unece:CropProduceBatch"}],"rdfs:comment":"An agricultural certificate specified for this crop plot."},{"@id":"unece:specifiedArea","@type":["rdf:Property","owl:ObjectProperty"],"rdfs:label":"specifiedArea","schema:rangeIncludes":{"@id":"unece:Area"},"schema:domainIncludes":{"@id":"unece:Plot"},"rdfs:comment":"An agricultural zone area specified for this crop plot."},{"@id":"unece:startDateTime","@type":["rdf:Property","owl:DatatypeProperty"],"rdfs:label":"startDateTime","schema:rangeIncludes":{"@id":"schema:Text"},"schema:domainIncludes":[{"@id":"unece:Plot"},{"@id":"unece:SpecifiedPeriod"},{"@id":"unece:AvailablePeriod"},{"@id":"unece:Membership"},{"@id":"unece:DelimitedPeriod"},{"@id":"unece:Assessment"},{"@id":"unece:SpecifiedCertification"}],"rdfs:comment":"The date, time, date time or other date time value for the start of this available period of time."},{"@id":"unece:applicableAnimalCertification","@type":["rdf:Property","owl:ObjectProperty"],"rdfs:label":"applicableAnimalCertification","schema:rangeIncludes":{"@id":"unece:AnimalCertification"},"schema:domainIncludes":{"@id":"unece:AnimalCertificate"},"rdfs:comment":"An animal certification applicable to this animal certificate."},{"@id":"unece:applicableProcessCertificate","@type":["rdf:Property","owl:ObjectProperty"],"rdfs:label":"applicableProcessCertificate","schema:rangeIncludes":{"@id":"unece:ProcessCertificate"},"schema:domainIncludes":[{"@id":"unece:CropProtectionTreatment"},{"@id":"unece:WasteMaterialRecoveryDisposalProcess"}],"rdfs:comment":"A piece of written, printed or electronic matter that provides information or evidence that a process has met required criteria."},{"@id":"unece:usedMaterial","@type":["rdf:Property","owl:ObjectProperty"],"rdfs:label":"usedMaterial","schema:rangeIncludes":{"@id":"unece:SpecifiedMaterial"},"schema:domainIncludes":{"@id":"unece:CropProtectionTreatment"},"rdfs:comment":"A substance from which something is or could be made."},{"@id":"unece:appliedArea","@type":["rdf:Property","owl:ObjectProperty"],"rdfs:label":"appliedArea","schema:rangeIncludes":{"@id":"unece:Area"},"schema:domainIncludes":{"@id":"unece:AgriculturalApplication"},"rdfs:comment":"A specified agricultural application applied to this agricultural zone area."},{"@id":"unece:appliedCertificate","@type":["rdf:Property","owl:ObjectProperty"],"rdfs:label":"appliedCertificate","schema:rangeIncludes":{"@id":"unece:AgriculturalCertificate"},"schema:domainIncludes":{"@id":"unece:AgriculturalApplication"},"rdfs:comment":"An agricultural certificate applied to this specified agricultural application."},{"@id":"unece:appliedMaterial","@type":["rdf:Property","owl:ObjectProperty"],"rdfs:label":"appliedMaterial","schema:rangeIncludes":{"@id":"unece:SpecifiedMaterial"},"schema:domainIncludes":{"@id":"unece:AgriculturalApplication"},"rdfs:comment":"A substance from which something is or could be made."},{"@id":"unece:appliedTreatment","@type":["rdf:Property","owl:DatatypeProperty"],"rdfs:label":"appliedTreatment","schema:rangeIncludes":{"@id":"schema:Text"},"schema:domainIncludes":{"@id":"unece:CropProduceBatch"},"rdfs:comment":"A treatment, expressed as text, applied to this crop produce batch."},{"@id":"unece:breakUpDateTime","@type":["rdf:Property","owl:DatatypeProperty"],"rdfs:label":"breakUpDateTime","schema:rangeIncludes":{"@id":"schema:Text"},"schema:domainIncludes":[{"@id":"unece:CropProduceBatch"},{"@id":"unece:AnimalBatch"}],"rdfs:comment":"The break up date, time, date time, or other date time value for this experience event."},{"@id":"unece:creationDateTime","@type":["rdf:Property","owl:DatatypeProperty"],"rdfs:label":"creationDateTime","schema:rangeIncludes":{"@id":"schema:Text"},"schema:domainIncludes":[{"@id":"unece:CropProduceBatch"},{"@id":"unece:AnimalBatch"},{"@id":"unece:ExchangedDocument"},{"@id":"unece:SpecifiedNote"}],"rdfs:comment":"The creation date, time, date time, or other date time value for this payment trade settlement."},{"@id":"unece:nominalSizeNumeric","@type":["rdf:Property","owl:DatatypeProperty"],"rdfs:label":"nominalSizeNumeric","schema:rangeIncludes":{"@id":"schema:Text"},"schema:domainIncludes":{"@id":"unece:CropProduceBatch"},"rdfs:comment":"The value of the nominal size for this crop produce batch."},{"@id":"unece:productName","@type":["rdf:Property","owl:DatatypeProperty"],"rdfs:label":"productName","schema:rangeIncludes":{"@id":"schema:Text"},"schema:domainIncludes":{"@id":"unece:CropProduceBatch"},"rdfs:comment":"The product name, expressed as text, for this crop produce batch."},{"@id":"unece:sizeMeasure","@type":["rdf:Property","owl:ObjectProperty"],"rdfs:label":"sizeMeasure","schema:rangeIncludes":{"@id":"unece:MeasureType"},"schema:domainIncludes":[{"@id":"unece:CropProduceBatch"},{"@id":"unece:BinaryFile"}],"rdfs:comment":""},{"@id":"unece:specifiedProduce","@type":["rdf:Property","owl:ObjectProperty"],"rdfs:label":"specifiedProduce","schema:rangeIncludes":{"@id":"unece:Produce"},"schema:domainIncludes":{"@id":"unece:CropProduceBatch"},"rdfs:comment":"A crop produce specified for this crop produce batch."},{"@id":"unece:specifiedQuantity","@type":["rdf:Property","owl:ObjectProperty"],"rdfs:label":"specifiedQuantity","schema:rangeIncludes":{"@id":"unece:QuantityType"},"schema:domainIncludes":{"@id":"unece:CropProduceBatch"},"rdfs:comment":""},{"@id":"unece:unitQuantity","@type":["rdf:Property","owl:ObjectProperty"],"rdfs:label":"unitQuantity","schema:rangeIncludes":{"@id":"unece:QuantityType"},"schema:domainIncludes":[{"@id":"unece:CropProduceBatch"},{"@id":"unece:AnimalBatch"},{"@id":"unece:CommunicationEvent"},{"@id":"unece:EventElement"}],"rdfs:comment":""},{"@id":"unece:assertion","@type":["rdf:Property","owl:DatatypeProperty"],"rdfs:label":"assertion","schema:rangeIncludes":{"@id":"schema:Text"},"schema:domainIncludes":[{"@id":"unece:AnimalCertification"},{"@id":"unece:OrganizationalCertification"},{"@id":"unece:ProcessCertification"},{"@id":"unece:ProductBatchCertification"},{"@id":"unece:SpecifiedCertification"},{"@id":"unece:TradeProductCertification"}],"rdfs:comment":"An assertion, expressed as text, for this animal certification."},{"@id":"unece:assertionCode","@type":["rdf:Property","owl:DatatypeProperty"],"rdfs:label":"assertionCode","schema:rangeIncludes":{"@id":"schema:Text"},"schema:domainIncludes":[{"@id":"unece:AnimalCertification"},{"@id":"unece:OrganizationalCertification"},{"@id":"unece:ProcessCertification"},{"@id":"unece:ProductBatchCertification"},{"@id":"unece:SpecifiedCertification"},{"@id":"unece:TradeProductCertification"}],"rdfs:comment":"A code specifying an assertion for this specified certification, such as a claim that a product is free of hazardous chemicals."},{"@id":"unece:relatedLocation","@type":["rdf:Property","owl:ObjectProperty"],"rdfs:label":"relatedLocation","schema:rangeIncludes":{"@id":"unece:Location"},"schema:domainIncludes":[{"@id":"unece:AnimalCertification"},{"@id":"unece:OrganizationalCertification"},{"@id":"unece:ProcessCertification"},{"@id":"unece:ProductBatchCertification"},{"@id":"unece:SpecifiedCertification"},{"@id":"unece:TradeProductCertification"}],"rdfs:comment":"A reference to a physical location or place."},{"@id":"unece:responsibleAgency","@type":["rdf:Property","owl:DatatypeProperty"],"rdfs:label":"responsibleAgency","schema:rangeIncludes":{"@id":"schema:Text"},"schema:domainIncludes":[{"@id":"unece:AnimalCertification"},{"@id":"unece:OrganizationalCertification"},{"@id":"unece:ProcessCertification"},{"@id":"unece:ProductBatchCertification"},{"@id":"unece:SpecifiedCertification"},{"@id":"unece:TradeProductCertification"}],"rdfs:comment":"A responsible agency, expressed as text, for this specified certification."},{"@id":"unece:specifiedAssertion","@type":["rdf:Property","owl:ObjectProperty"],"rdfs:label":"specifiedAssertion","schema:rangeIncludes":{"@id":"unece:Assertion"},"schema:domainIncludes":[{"@id":"unece:AnimalCertification"},{"@id":"unece:Standard"},{"@id":"unece:OrganizationalCertification"},{"@id":"unece:ProcessCertification"},{"@id":"unece:ProductBatchCertification"},{"@id":"unece:SpecifiedCertification"},{"@id":"unece:TradeProductCertification"}],"rdfs:comment":"A statement that user needs of the present are met without compromising the needs of future generations."},{"@id":"unece:standard","@type":["rdf:Property","owl:DatatypeProperty"],"rdfs:label":"standard","schema:rangeIncludes":{"@id":"schema:Text"},"schema:domainIncludes":[{"@id":"unece:AnimalCertification"},{"@id":"unece:OrganizationalCertification"},{"@id":"unece:ProcessCertification"},{"@id":"unece:ProductBatchCertification"},{"@id":"unece:SpecifiedCertification"},{"@id":"unece:TradeProductCertification"}],"rdfs:comment":"A standard, expressed as text, for this specified certification."},{"@id":"unece:birthDateTime","@type":["rdf:Property","owl:DatatypeProperty"],"rdfs:label":"birthDateTime","schema:rangeIncludes":{"@id":"schema:Text"},"schema:domainIncludes":[{"@id":"unece:IndividualTTAnimal"},{"@id":"unece:Person"}],"rdfs:comment":"The birth date for this individual TT animal."},{"@id":"unece:deathDateTime","@type":["rdf:Property","owl:DatatypeProperty"],"rdfs:label":"deathDateTime","schema:rangeIncludes":{"@id":"schema:Text"},"schema:domainIncludes":{"@id":"unece:IndividualTTAnimal"},"rdfs:comment":"The death date for this individual TT animal."},{"@id":"unece:specifiedPeriod","@type":["rdf:Property","owl:ObjectProperty"],"rdfs:label":"specifiedPeriod","schema:rangeIncludes":{"@id":"unece:DelimitedPeriod"},"schema:domainIncludes":[{"@id":"unece:IndividualTTAnimal"},{"@id":"unece:AnimalBatch"},{"@id":"unece:CoordinateReferenceSystem"}],"rdfs:comment":"A period of time from a start date time onwards up to an end date time."},{"@id":"unece:botanicalGenusCode","@type":["rdf:Property","owl:DatatypeProperty"],"rdfs:label":"botanicalGenusCode","schema:rangeIncludes":{"@id":"schema:Text"},"schema:domainIncludes":{"@id":"unece:BotanicalCrop"},"rdfs:comment":"The code specifying the genus for this botanical crop."},{"@id":"unece:botanicalIdentificationId","@type":["rdf:Property","owl:DatatypeProperty"],"rdfs:label":"botanicalIdentificationId","schema:rangeIncludes":{"@id":"schema:Text"},"schema:domainIncludes":{"@id":"unece:BotanicalCrop"},"rdfs:comment":"The identifier for this botanical crop."},{"@id":"unece:botanicalName","@type":["rdf:Property","owl:DatatypeProperty"],"rdfs:label":"botanicalName","schema:rangeIncludes":{"@id":"schema:Text"},"schema:domainIncludes":{"@id":"unece:BotanicalCrop"},"rdfs:comment":"The botanical name, expressed as text, for this botanical crop."},{"@id":"unece:botanicalSpeciesCode","@type":["rdf:Property","owl:DatatypeProperty"],"rdfs:label":"botanicalSpeciesCode","schema:rangeIncludes":{"@id":"schema:Text"},"schema:domainIncludes":{"@id":"unece:BotanicalCrop"},"rdfs:comment":"The code specifying the species for this botanical crop."},{"@id":"unece:fLUXId","@type":["rdf:Property","owl:DatatypeProperty"],"rdfs:label":"fLUXId","schema:rangeIncludes":{"@id":"schema:Text"},"schema:domainIncludes":{"@id":"unece:AnimalBatch"},"rdfs:comment":"A Fisheries Language for Universal eXchange (FLUX) identifier for this animal batch."},{"@id":"unece:maximumSizeMeasure","@type":["rdf:Property","owl:ObjectProperty"],"rdfs:label":"maximumSizeMeasure","schema:rangeIncludes":{"@id":"unece:MeasureType"},"schema:domainIncludes":{"@id":"unece:AnimalBatch"},"rdfs:comment":""},{"@id":"unece:minimumSizeMeasure","@type":["rdf:Property","owl:ObjectProperty"],"rdfs:label":"minimumSizeMeasure","schema:rangeIncludes":{"@id":"unece:MeasureType"},"schema:domainIncludes":{"@id":"unece:AnimalBatch"},"rdfs:comment":""},{"@id":"unece:saleDateTime","@type":["rdf:Property","owl:DatatypeProperty"],"rdfs:label":"saleDateTime","schema:rangeIncludes":{"@id":"schema:Text"},"schema:domainIncludes":{"@id":"unece:AnimalBatch"},"rdfs:comment":"The date, time, date time, or other date time value of the sale for this animal batch."},{"@id":"unece:salesNoteId","@type":["rdf:Property","owl:DatatypeProperty"],"rdfs:label":"salesNoteId","schema:rangeIncludes":{"@id":"schema:Text"},"schema:domainIncludes":{"@id":"unece:AnimalBatch"},"rdfs:comment":"The identifier for the sales note for this animal batch."},{"@id":"unece:weightMeasure","@type":["rdf:Property","owl:ObjectProperty"],"rdfs:label":"weightMeasure","schema:rangeIncludes":{"@id":"unece:MeasureType"},"schema:domainIncludes":[{"@id":"unece:AnimalBatch"},{"@id":"unece:Chemical"},{"@id":"unece:SpecifiedMaterial"},{"@id":"unece:ProductionWasteMaterial"}],"rdfs:comment":""},{"@id":"unece:calculatedYieldMeasure","@type":["rdf:Property","owl:ObjectProperty"],"rdfs:label":"calculatedYieldMeasure","schema:rangeIncludes":{"@id":"unece:MeasureType"},"schema:domainIncludes":{"@id":"unece:Produce"},"rdfs:comment":""},{"@id":"unece:estimatedYieldMeasure","@type":["rdf:Property","owl:ObjectProperty"],"rdfs:label":"estimatedYieldMeasure","schema:rangeIncludes":{"@id":"unece:MeasureType"},"schema:domainIncludes":{"@id":"unece:Produce"},"rdfs:comment":""},{"@id":"unece:inputSpecifiedBatch","@type":["rdf:Property","owl:ObjectProperty"],"rdfs:label":"inputSpecifiedBatch","schema:rangeIncludes":{"@id":"unece:CropProduceBatch"},"schema:domainIncludes":{"@id":"unece:Produce"},"rdfs:comment":"An input batch crop produce, such as seed or fertilizer, specified for this crop produce."},{"@id":"unece:outputSpecifiedBatch","@type":["rdf:Property","owl:ObjectProperty"],"rdfs:label":"outputSpecifiedBatch","schema:rangeIncludes":{"@id":"unece:CropProduceBatch"},"schema:domainIncludes":{"@id":"unece:Produce"},"rdfs:comment":"An output batch crop produce, such as potatoes, grain, straw, specified for this crop produce."},{"@id":"unece:cropProportionPercent","@type":["rdf:Property","owl:DatatypeProperty"],"rdfs:label":"cropProportionPercent","schema:rangeIncludes":{"@id":"schema:Text"},"schema:domainIncludes":{"@id":"unece:CropMixtureConstituent"},"rdfs:comment":"The percent of the crop proportion of this field crop mixture constituent."},{"@id":"unece:specifiedBotanicalCrop","@type":["rdf:Property","owl:ObjectProperty"],"rdfs:label":"specifiedBotanicalCrop","schema:rangeIncludes":{"@id":"unece:BotanicalCrop"},"schema:domainIncludes":{"@id":"unece:CropMixtureConstituent"},"rdfs:comment":"The botanical crop specified for this field crop mixture constituent."},{"@id":"unece:value","@type":["rdf:Property","owl:DatatypeProperty"],"rdfs:label":"value","schema:rangeIncludes":{"@id":"schema:Text"},"schema:domainIncludes":[{"@id":"unece:AgriculturalCharacteristic"},{"@id":"unece:MetricCharacteristic"},{"@id":"unece:DocumentCharacteristic"},{"@id":"unece:SpecifiedParameter"},{"@id":"unece:Range"},{"@id":"unece:DocumentContextParameter"},{"@id":"unece:InspectionReference"},{"@id":"unece:LaboratoryObservationReference"},{"@id":"unece:ProductCharacteristic"},{"@id":"unece:ProductBatchCharacteristic"},{"@id":"unece:SustainabilityCharacteristic"},{"@id":"unece:ProcessCharacteristic"},{"@id":"unece:TechnicalCharacteristic"},{"@id":"unece:ControlSettingParameter"},{"@id":"unece:OperationalParameter"},{"@id":"unece:ObservationObjectiveParameter"},{"@id":"unece:OrganizationCharacteristic"}],"rdfs:comment":"A value, expressed as text, for this document characteristic."},{"@id":"unece:valueAmount","@type":["rdf:Property","owl:ObjectProperty"],"rdfs:label":"valueAmount","schema:rangeIncludes":{"@id":"unece:AmountType"},"schema:domainIncludes":[{"@id":"unece:AgriculturalCharacteristic"},{"@id":"unece:MetricCharacteristic"},{"@id":"unece:DocumentCharacteristic"},{"@id":"unece:ProductCharacteristic"},{"@id":"unece:ProductBatchCharacteristic"},{"@id":"unece:SustainabilityCharacteristic"},{"@id":"unece:ProcessCharacteristic"},{"@id":"unece:TechnicalCharacteristic"},{"@id":"unece:OrganizationCharacteristic"}],"rdfs:comment":""},{"@id":"unece:valueCode","@type":["rdf:Property","owl:DatatypeProperty"],"rdfs:label":"valueCode","schema:rangeIncludes":{"@id":"schema:Text"},"schema:domainIncludes":[{"@id":"unece:AgriculturalCharacteristic"},{"@id":"unece:MetricCharacteristic"},{"@id":"unece:DocumentCharacteristic"},{"@id":"unece:Range"},{"@id":"unece:InspectionReference"},{"@id":"unece:LaboratoryObservationReference"},{"@id":"unece:ProductBatchCharacteristic"},{"@id":"unece:SustainabilityCharacteristic"},{"@id":"unece:ProcessCharacteristic"},{"@id":"unece:TechnicalCharacteristic"},{"@id":"unece:CalibratedMeasurement"},{"@id":"unece:OrganizationCharacteristic"}],"rdfs:comment":"A code specifying a value for this specified range."},{"@id":"unece:valueDateTime","@type":["rdf:Property","owl:DatatypeProperty"],"rdfs:label":"valueDateTime","schema:rangeIncludes":{"@id":"schema:Text"},"schema:domainIncludes":[{"@id":"unece:AgriculturalCharacteristic"},{"@id":"unece:MetricCharacteristic"},{"@id":"unece:DocumentCharacteristic"},{"@id":"unece:ProductCharacteristic"},{"@id":"unece:ProductBatchCharacteristic"},{"@id":"unece:SustainabilityCharacteristic"},{"@id":"unece:ProcessCharacteristic"},{"@id":"unece:TechnicalCharacteristic"},{"@id":"unece:OrganizationCharacteristic"}],"rdfs:comment":"A date, time, date time or other date time value for this document characteristic."},{"@id":"unece:valueIndicator","@type":["rdf:Property","owl:DatatypeProperty"],"rdfs:label":"valueIndicator","schema:rangeIncludes":{"@id":"schema:Boolean"},"schema:domainIncludes":[{"@id":"unece:AgriculturalCharacteristic"},{"@id":"unece:MetricCharacteristic"},{"@id":"unece:ProductCharacteristic"},{"@id":"unece:ProductBatchCharacteristic"},{"@id":"unece:SustainabilityCharacteristic"},{"@id":"unece:ProcessCharacteristic"},{"@id":"unece:TechnicalCharacteristic"},{"@id":"unece:OrganizationCharacteristic"}],"rdfs:comment":"The value for this metric characteristic expressed as an indicator."},{"@id":"unece:valueMeasure","@type":["rdf:Property","owl:ObjectProperty"],"rdfs:label":"valueMeasure","schema:rangeIncludes":{"@id":"unece:MeasureType"},"schema:domainIncludes":[{"@id":"unece:AgriculturalCharacteristic"},{"@id":"unece:CommunicationEvent"},{"@id":"unece:WorkItemDimension"},{"@id":"unece:MetricCharacteristic"},{"@id":"unece:DocumentCharacteristic"},{"@id":"unece:SpatialDimension"},{"@id":"unece:SpecifiedParameter"},{"@id":"unece:ProductCharacteristic"},{"@id":"unece:ProductBatchCharacteristic"},{"@id":"unece:SustainabilityCharacteristic"},{"@id":"unece:ProcessCharacteristic"},{"@id":"unece:TechnicalCharacteristic"},{"@id":"unece:ControlSettingParameter"},{"@id":"unece:OperationalParameter"},{"@id":"unece:ObservationObjectiveParameter"},{"@id":"unece:CalibratedMeasurement"},{"@id":"unece:ProductCharacteristicCondition"},{"@id":"unece:OrganizationCharacteristic"}],"rdfs:comment":""},{"@id":"unece:valueMethod","@type":["rdf:Property","owl:ObjectProperty"],"rdfs:label":"valueMethod","schema:rangeIncludes":{"@id":"unece:SpecifiedMethod"},"schema:domainIncludes":[{"@id":"unece:AgriculturalCharacteristic"},{"@id":"unece:MetricCharacteristic"},{"@id":"unece:ProductCharacteristic"},{"@id":"unece:ProductBatchCharacteristic"},{"@id":"unece:ProcessCharacteristic"},{"@id":"unece:OrganizationCharacteristic"}],"rdfs:comment":"A defined way of performing something."},{"@id":"unece:valueNumeric","@type":["rdf:Property","owl:DatatypeProperty"],"rdfs:label":"valueNumeric","schema:rangeIncludes":{"@id":"schema:Text"},"schema:domainIncludes":[{"@id":"unece:AgriculturalCharacteristic"},{"@id":"unece:MetricCharacteristic"},{"@id":"unece:DocumentCharacteristic"},{"@id":"unece:ProductCharacteristic"},{"@id":"unece:ProductBatchCharacteristic"},{"@id":"unece:SustainabilityCharacteristic"},{"@id":"unece:ProcessCharacteristic"},{"@id":"unece:TechnicalCharacteristic"},{"@id":"unece:OrganizationCharacteristic"}],"rdfs:comment":"A value, expressed as a number, for this document characteristic."},{"@id":"unece:valueParameter","@type":["rdf:Property","owl:ObjectProperty"],"rdfs:label":"valueParameter","schema:rangeIncludes":{"@id":"unece:SpecifiedParameter"},"schema:domainIncludes":[{"@id":"unece:AgriculturalCharacteristic"},{"@id":"unece:MetricCharacteristic"},{"@id":"unece:ProductCharacteristic"},{"@id":"unece:ProductBatchCharacteristic"},{"@id":"unece:SustainabilityCharacteristic"},{"@id":"unece:ProcessCharacteristic"},{"@id":"unece:TechnicalCharacteristic"},{"@id":"unece:OrganizationCharacteristic"}],"rdfs:comment":"A specified feature that is fixed for the case in question but may be different in other cases."},{"@id":"unece:valueRange","@type":["rdf:Property","owl:ObjectProperty"],"rdfs:label":"valueRange","schema:rangeIncludes":{"@id":"unece:Range"},"schema:domainIncludes":[{"@id":"unece:AgriculturalCharacteristic"},{"@id":"unece:MetricCharacteristic"},{"@id":"unece:ProductCharacteristic"},{"@id":"unece:ProductBatchCharacteristic"},{"@id":"unece:SustainabilityCharacteristic"},{"@id":"unece:ProcessCharacteristic"},{"@id":"unece:TechnicalCharacteristic"},{"@id":"unece:OrganizationCharacteristic"}],"rdfs:comment":"A row, line or series, commonly used to express the difference between lowest and highest values."},{"@id":"unece:valueTolerance","@type":["rdf:Property","owl:ObjectProperty"],"rdfs:label":"valueTolerance","schema:rangeIncludes":{"@id":"unece:Tolerance"},"schema:domainIncludes":[{"@id":"unece:AgriculturalCharacteristic"},{"@id":"unece:MetricCharacteristic"},{"@id":"unece:SpecifiedParameter"},{"@id":"unece:ProductCharacteristic"},{"@id":"unece:ProductBatchCharacteristic"},{"@id":"unece:SustainabilityCharacteristic"},{"@id":"unece:ProcessCharacteristic"},{"@id":"unece:TechnicalCharacteristic"},{"@id":"unece:OrganizationCharacteristic"}],"rdfs:comment":"Permissible limit or limits of variation that is fixed for the case in question but may be different in other cases."},{"@id":"unece:identifierLengthNumeric","@type":["rdf:Property","owl:DatatypeProperty"],"rdfs:label":"identifierLengthNumeric","schema:rangeIncludes":{"@id":"schema:Text"},"schema:domainIncludes":{"@id":"unece:AnimalIdentity"},"rdfs:comment":"The length, expressed as the number of characters, of the identifier in this animal identity."},{"@id":"unece:issuerPartyName","@type":["rdf:Property","owl:DatatypeProperty"],"rdfs:label":"issuerPartyName","schema:rangeIncludes":{"@id":"schema:Text"},"schema:domainIncludes":{"@id":"unece:AnimalIdentity"},"rdfs:comment":"The name, expressed as text, of the party issuing this animal identity."},{"@id":"unece:legalBasis","@type":["rdf:Property","owl:DatatypeProperty"],"rdfs:label":"legalBasis","schema:rangeIncludes":{"@id":"schema:Text"},"schema:domainIncludes":{"@id":"unece:AnimalIdentity"},"rdfs:comment":"The legal basis, expressed as text, for this animal identity."},{"@id":"unece:locationId","@type":["rdf:Property","owl:DatatypeProperty"],"rdfs:label":"locationId","schema:rangeIncludes":{"@id":"schema:Text"},"schema:domainIncludes":{"@id":"unece:AnimalHoldingEvent"},"rdfs:comment":"An identifier of a location for this MDH health indication."},{"@id":"unece:occurrenceDateTime","@type":["rdf:Property","owl:DatatypeProperty"],"rdfs:label":"occurrenceDateTime","schema:rangeIncludes":{"@id":"schema:Text"},"schema:domainIncludes":[{"@id":"unece:AnimalHoldingEvent"},{"@id":"unece:CommunicationEvent"},{"@id":"unece:Schedule"},{"@id":"unece:AppliedChemicalTreatment"},{"@id":"unece:InspectionEvent"}],"rdfs:comment":"A date, time, date time, or other date time of an occurrence in this supply chain schedule."},{"@id":"unece:regulationSpeciesNameTypeCode","@type":["rdf:Property","owl:DatatypeProperty"],"rdfs:label":"regulationSpeciesNameTypeCode","schema:rangeIncludes":{"@id":"schema:Text"},"schema:domainIncludes":{"@id":"unece:SpeciesTTAnimal"},"rdfs:comment":"A code specifying the type of regulation species name for this TT animal."},{"@id":"unece:scientificSpeciesNameTypeCode","@type":["rdf:Property","owl:DatatypeProperty"],"rdfs:label":"scientificSpeciesNameTypeCode","schema:rangeIncludes":{"@id":"schema:Text"},"schema:domainIncludes":{"@id":"unece:SpeciesTTAnimal"},"rdfs:comment":"A code specifying the type of scientific species name for this TT animal."},{"@id":"unece:speciesTypeCode","@type":["rdf:Property","owl:DatatypeProperty"],"rdfs:label":"speciesTypeCode","schema:rangeIncludes":{"@id":"schema:Text"},"schema:domainIncludes":{"@id":"unece:SpeciesTTAnimal"},"rdfs:comment":"A code specifying the species type of this TT animal."},{"@id":"unece:tradeSpeciesNameTypeCode","@type":["rdf:Property","owl:DatatypeProperty"],"rdfs:label":"tradeSpeciesNameTypeCode","schema:rangeIncludes":{"@id":"schema:Text"},"schema:domainIncludes":{"@id":"unece:SpeciesTTAnimal"},"rdfs:comment":"A code specifying the type of trade species name for this TT animal."},{"@id":"unece:abstract","@type":["rdf:Property","owl:DatatypeProperty"],"rdfs:label":"abstract","schema:rangeIncludes":{"@id":"schema:Text"},"schema:domainIncludes":{"@id":"unece:ComplexDescription"},"rdfs:comment":"A textual abstract of the content of the work item complex description."},{"@id":"unece:content","@type":["rdf:Property","owl:DatatypeProperty"],"rdfs:label":"content","schema:rangeIncludes":{"@id":"schema:Text"},"schema:domainIncludes":[{"@id":"unece:ComplexDescription"},{"@id":"unece:InformationSource"},{"@id":"unece:Note"},{"@id":"unece:Response"},{"@id":"unece:SpecialQuery"},{"@id":"unece:SpecifiedNote"},{"@id":"unece:Clause"},{"@id":"unece:SpecificationQuery"},{"@id":"unece:InspectionNote"},{"@id":"unece:LaboratoryObservationNote"}],"rdfs:comment":"A content, expressed as text, of this note."},{"@id":"unece:contractualLanguageCode","@type":["rdf:Property","owl:DatatypeProperty"],"rdfs:label":"contractualLanguageCode","schema:rangeIncludes":{"@id":"schema:Text"},"schema:domainIncludes":[{"@id":"unece:ComplexDescription"},{"@id":"unece:QuantityAnalysis"},{"@id":"unece:WorkItemDimension"},{"@id":"unece:Response"},{"@id":"unece:SpecificationQuery"}],"rdfs:comment":"The code specifying the contractual language for this basic work item."},{"@id":"unece:requestingQuery","@type":["rdf:Property","owl:ObjectProperty"],"rdfs:label":"requestingQuery","schema:rangeIncludes":{"@id":"unece:SpecificationQuery"},"schema:domainIncludes":{"@id":"unece:ComplexDescription"},"rdfs:comment":"A requesting specification query for this work item complex description."},{"@id":"unece:respondingResponse","@type":["rdf:Property","owl:ObjectProperty"],"rdfs:label":"respondingResponse","schema:rangeIncludes":{"@id":"unece:Response"},"schema:domainIncludes":{"@id":"unece:ComplexDescription"},"rdfs:comment":"A responding specification response for this work item complex description."},{"@id":"unece:subsetComplexDescription","@type":["rdf:Property","owl:ObjectProperty"],"rdfs:label":"subsetComplexDescription","schema:rangeIncludes":{"@id":"unece:ComplexDescription"},"schema:domainIncludes":{"@id":"unece:ComplexDescription"},"rdfs:comment":"The complex description subset for this work item complex description."},{"@id":"unece:acceptablePeriod","@type":["rdf:Property","owl:ObjectProperty"],"rdfs:label":"acceptablePeriod","schema:rangeIncludes":{"@id":"unece:SpecifiedPeriod"},"schema:domainIncludes":{"@id":"unece:Document"},"rdfs:comment":"The specified period within which this referenced document may be accepted."},{"@id":"unece:acceptanceDateTime","@type":["rdf:Property","owl:DatatypeProperty"],"rdfs:label":"acceptanceDateTime","schema:rangeIncludes":{"@id":"schema:Text"},"schema:domainIncludes":[{"@id":"unece:Document"},{"@id":"unece:ExchangedDocument"}],"rdfs:comment":"The date, time, date time, or other date time value for the acceptance of this exchanged document."},{"@id":"unece:attachmentBinaryObject","@type":["rdf:Property","owl:DatatypeProperty"],"rdfs:label":"attachmentBinaryObject","schema:rangeIncludes":{"@id":"schema:Text"},"schema:domainIncludes":{"@id":"unece:Document"},"rdfs:comment":"A binary object that is attached or otherwise appended to this referenced document."},{"@id":"unece:authenticatedOriginalIndicator","@type":["rdf:Property","owl:DatatypeProperty"],"rdfs:label":"authenticatedOriginalIndicator","schema:rangeIncludes":{"@id":"schema:Boolean"},"schema:domainIncludes":{"@id":"unece:Document"},"rdfs:comment":"The indication of whether or not this referenced document is an authenticated original."},{"@id":"unece:categoryCode","@type":["rdf:Property","owl:DatatypeProperty"],"rdfs:label":"categoryCode","schema:rangeIncludes":{"@id":"schema:Text"},"schema:domainIncludes":[{"@id":"unece:Document"},{"@id":"unece:ExchangedDocument"},{"@id":"unece:SpecifiedFault"},{"@id":"unece:Object"},{"@id":"unece:CustomerClass"},{"@id":"unece:InformationSource"},{"@id":"unece:Authentication"},{"@id":"unece:ProtectionMeans"},{"@id":"unece:Accreditation"},{"@id":"unece:RegulatoryProcedure"},{"@id":"unece:SpecifiedCertificate"},{"@id":"unece:SustainabilityCharacteristic"},{"@id":"unece:Assessment"},{"@id":"unece:Source"},{"@id":"unece:GovernmentRegistration"},{"@id":"unece:RiskAnalysisResult"}],"rdfs:comment":"A code specifying a category for this cross-border regulatory procedure, such as the appendices of the CITES Convention."},{"@id":"unece:contractualClause","@type":["rdf:Property","owl:ObjectProperty"],"rdfs:label":"contractualClause","schema:rangeIncludes":{"@id":"unece:Clause"},"schema:domainIncludes":[{"@id":"unece:Document"},{"@id":"unece:ExchangedDocument"}],"rdfs:comment":"A contractual clause of this exchanged document."},{"@id":"unece:copyIndicator","@type":["rdf:Property","owl:DatatypeProperty"],"rdfs:label":"copyIndicator","schema:rangeIncludes":{"@id":"schema:Boolean"},"schema:domainIncludes":[{"@id":"unece:Document"},{"@id":"unece:ExchangedDocument"}],"rdfs:comment":"The indication of whether or not the referenced document is a copy."},{"@id":"unece:documentLanguageId","@type":["rdf:Property","owl:DatatypeProperty"],"rdfs:label":"documentLanguageId","schema:rangeIncludes":{"@id":"unece:LanguageId"},"schema:domainIncludes":{"@id":"unece:Document"},"rdfs:comment":"An identifier for a language used in this referenced document."},{"@id":"unece:documentStatusCode","@type":["rdf:Property","owl:DatatypeProperty"],"rdfs:label":"documentStatusCode","schema:rangeIncludes":{"@id":"unece:DocumentStatusCodeList"},"schema:domainIncludes":[{"@id":"unece:Document"},{"@id":"unece:ExchangedDocument"}],"rdfs:comment":"The code specifying the status for this referenced document."},{"@id":"unece:documentType","@type":["rdf:Property","owl:DatatypeProperty"],"rdfs:label":"documentType","schema:rangeIncludes":{"@id":"schema:Text"},"schema:domainIncludes":{"@id":"unece:Document"},"rdfs:comment":"A type, expressed as text, for this referenced document."},{"@id":"unece:documentTypeCode","@type":["rdf:Property","owl:DatatypeProperty"],"rdfs:label":"documentTypeCode","schema:rangeIncludes":{"@id":"unece:DocumentCodeList"},"schema:domainIncludes":[{"@id":"unece:Document"},{"@id":"unece:ExchangedDocument"}],"rdfs:comment":"A code specifying a type of acknowledgement document."},{"@id":"unece:effectiveSpecifiedPeriod","@type":["rdf:Property","owl:ObjectProperty"],"rdfs:label":"effectiveSpecifiedPeriod","schema:rangeIncludes":{"@id":"unece:SpecifiedPeriod"},"schema:domainIncludes":[{"@id":"unece:Document"},{"@id":"unece:ExchangedDocument"}],"rdfs:comment":"The period within which this document line is effective."},{"@id":"unece:electronicPresentationIndicator","@type":["rdf:Property","owl:DatatypeProperty"],"rdfs:label":"electronicPresentationIndicator","schema:rangeIncludes":{"@id":"schema:Boolean"},"schema:domainIncludes":[{"@id":"unece:Document"},{"@id":"unece:ExchangedDocument"}],"rdfs:comment":"The indication of whether or not this exchanged document is presented in an electronic format."},{"@id":"unece:globalId","@type":["rdf:Property","owl:DatatypeProperty"],"rdfs:label":"globalId","schema:rangeIncludes":{"@id":"schema:Text"},"schema:domainIncludes":[{"@id":"unece:Document"},{"@id":"unece:ExchangedDocument"},{"@id":"unece:Location"}],"rdfs:comment":"A global identifier for this supply chain consignment item."},{"@id":"unece:includedAmount","@type":["rdf:Property","owl:ObjectProperty"],"rdfs:label":"includedAmount","schema:rangeIncludes":{"@id":"unece:AmountType"},"schema:domainIncludes":{"@id":"unece:Document"},"rdfs:comment":"A monetary value included in this referenced document."},{"@id":"unece:includedNote","@type":["rdf:Property","owl:ObjectProperty"],"rdfs:label":"includedNote","schema:rangeIncludes":{"@id":"unece:Note"},"schema:domainIncludes":[{"@id":"unece:Document"},{"@id":"unece:ExchangedDocument"},{"@id":"unece:DocumentStatus"}],"rdfs:comment":"A note included for this document status."},{"@id":"unece:information","@type":["rdf:Property","owl:DatatypeProperty"],"rdfs:label":"information","schema:rangeIncludes":{"@id":"schema:Text"},"schema:domainIncludes":[{"@id":"unece:Document"},{"@id":"unece:ExchangedDocument"},{"@id":"unece:SpecifiedMethod"},{"@id":"unece:DocumentStatus"},{"@id":"unece:Segment"},{"@id":"unece:Tolerance"},{"@id":"unece:Authentication"},{"@id":"unece:LaboratoryObservationAnalysisMethod"},{"@id":"unece:SpecifiedMaterial"}],"rdfs:comment":"Information, expressed as text, concerning the transport of these dangerous goods."},{"@id":"unece:issueLocation","@type":["rdf:Property","owl:ObjectProperty"],"rdfs:label":"issueLocation","schema:rangeIncludes":{"@id":"unece:Location"},"schema:domainIncludes":[{"@id":"unece:Document"},{"@id":"unece:ExchangedDocument"},{"@id":"unece:Authentication"}],"rdfs:comment":"The issue location for this document authentication."},{"@id":"unece:issuerAssignedId","@type":["rdf:Property","owl:DatatypeProperty"],"rdfs:label":"issuerAssignedId","schema:rangeIncludes":{"@id":"schema:Text"},"schema:domainIncludes":{"@id":"unece:Document"},"rdfs:comment":"The unique issuer assigned identifier for this referenced document."},{"@id":"unece:issuerParty","@type":["rdf:Property","owl:ObjectProperty"],"rdfs:label":"issuerParty","schema:rangeIncludes":{"@id":"unece:Party"},"schema:domainIncludes":[{"@id":"unece:Document"},{"@id":"unece:ExchangedDocument"},{"@id":"unece:SpecifiedCertificate"},{"@id":"unece:Licence"},{"@id":"unece:SpecifiedDeclaration"}],"rdfs:comment":"A party that issues this specified declaration."},{"@id":"unece:issuerSpecifiedInstructions","@type":["rdf:Property","owl:ObjectProperty"],"rdfs:label":"issuerSpecifiedInstructions","schema:rangeIncludes":{"@id":"unece:DocumentHandlingInstructions"},"schema:domainIncludes":{"@id":"unece:Document"},"rdfs:comment":"Handling instructions specified by the issuer for this referenced document."},{"@id":"unece:lineId","@type":["rdf:Property","owl:DatatypeProperty"],"rdfs:label":"lineId","schema:rangeIncludes":{"@id":"schema:Text"},"schema:domainIncludes":{"@id":"unece:Document"},"rdfs:comment":"The unique identifier of a line in this referenced document."},{"@id":"unece:lodgementLocation","@type":["rdf:Property","owl:ObjectProperty"],"rdfs:label":"lodgementLocation","schema:rangeIncludes":{"@id":"unece:Location"},"schema:domainIncludes":[{"@id":"unece:Document"},{"@id":"unece:ExchangedDocument"}],"rdfs:comment":"The location where this exchanged document has been lodged."},{"@id":"unece:pageId","@type":["rdf:Property","owl:DatatypeProperty"],"rdfs:label":"pageId","schema:rangeIncludes":{"@id":"schema:Text"},"schema:domainIncludes":{"@id":"unece:Document"},"rdfs:comment":"The identifier of the page for this referenced document."},{"@id":"unece:previousRevisionId","@type":["rdf:Property","owl:DatatypeProperty"],"rdfs:label":"previousRevisionId","schema:rangeIncludes":{"@id":"schema:Text"},"schema:domainIncludes":[{"@id":"unece:Document"},{"@id":"unece:ExchangedDocument"}],"rdfs:comment":"An identifier for a previous revision of this referenced document."},{"@id":"unece:processCondition","@type":["rdf:Property","owl:DatatypeProperty"],"rdfs:label":"processCondition","schema:rangeIncludes":{"@id":"schema:Text"},"schema:domainIncludes":[{"@id":"unece:Document"},{"@id":"unece:DocumentStatus"}],"rdfs:comment":"A process condition, expressed as text, for this acknowledgement document."},{"@id":"unece:processConditionCode","@type":["rdf:Property","owl:DatatypeProperty"],"rdfs:label":"processConditionCode","schema:rangeIncludes":{"@id":"schema:Text"},"schema:domainIncludes":[{"@id":"unece:Document"},{"@id":"unece:DocumentStatus"}],"rdfs:comment":"The code specifying the process condition for this acknowledgement document."},{"@id":"unece:proprietaryType","@type":["rdf:Property","owl:DatatypeProperty"],"rdfs:label":"proprietaryType","schema:rangeIncludes":{"@id":"schema:Text"},"schema:domainIncludes":{"@id":"unece:Document"},"rdfs:comment":"A proprietary type, expressed as text, for this referenced document."},{"@id":"unece:receiptDateTime","@type":["rdf:Property","owl:DatatypeProperty"],"rdfs:label":"receiptDateTime","schema:rangeIncludes":{"@id":"schema:Text"},"schema:domainIncludes":{"@id":"unece:Document"},"rdfs:comment":"The date, time, date time, or other date time value for the formal receipt of this referenced document."},{"@id":"unece:recipientTradeParty","@type":["rdf:Property","owl:ObjectProperty"],"rdfs:label":"recipientTradeParty","schema:rangeIncludes":{"@id":"unece:Party"},"schema:domainIncludes":[{"@id":"unece:Document"},{"@id":"unece:ExchangedDocument"}],"rdfs:comment":"A trade party that receives this exchanged document."},{"@id":"unece:referenceDateTime","@type":["rdf:Property","owl:DatatypeProperty"],"rdfs:label":"referenceDateTime","schema:rangeIncludes":{"@id":"schema:Text"},"schema:domainIncludes":[{"@id":"unece:Document"},{"@id":"unece:DocumentStatus"}],"rdfs:comment":"The reference date or date time for this referenced document."},{"@id":"unece:referenceRelationshipTypeCode","@type":["rdf:Property","owl:DatatypeProperty"],"rdfs:label":"referenceRelationshipTypeCode","schema:rangeIncludes":{"@id":"unece:ReferenceCodeList"},"schema:domainIncludes":{"@id":"unece:Document"},"rdfs:comment":"The code specifying the type of relationship between this referenced document and another artefact, such as a replacement of an original document."},{"@id":"unece:referenceTypeCode","@type":["rdf:Property","owl:DatatypeProperty"],"rdfs:label":"referenceTypeCode","schema:rangeIncludes":{"@id":"unece:ReferenceCodeList"},"schema:domainIncludes":[{"@id":"unece:Document"},{"@id":"unece:Location"}],"rdfs:comment":"The code specifying the reference type of this referenced document."},{"@id":"unece:remarks","@type":["rdf:Property","owl:DatatypeProperty"],"rdfs:label":"remarks","schema:rangeIncludes":{"@id":"schema:Text"},"schema:domainIncludes":[{"@id":"unece:Document"},{"@id":"unece:ExchangedDocument"}],"rdfs:comment":"A remark, expressed as text, regarding this exchanged document."},{"@id":"unece:revisionId","@type":["rdf:Property","owl:DatatypeProperty"],"rdfs:label":"revisionId","schema:rangeIncludes":{"@id":"schema:Text"},"schema:domainIncludes":[{"@id":"unece:Document"},{"@id":"unece:ExchangedDocument"}],"rdfs:comment":"A unique identifier for a revision of this referenced document."},{"@id":"unece:sectionName","@type":["rdf:Property","owl:DatatypeProperty"],"rdfs:label":"sectionName","schema:rangeIncludes":{"@id":"schema:Text"},"schema:domainIncludes":{"@id":"unece:Document"},"rdfs:comment":"A section name, expressed as text, for this referenced document."},{"@id":"unece:senderTradeParty","@type":["rdf:Property","owl:ObjectProperty"],"rdfs:label":"senderTradeParty","schema:rangeIncludes":{"@id":"unece:Party"},"schema:domainIncludes":[{"@id":"unece:Document"},{"@id":"unece:ExchangedDocument"}],"rdfs:comment":"The party that sends this exchanged document."},{"@id":"unece:signatoryAuthentication","@type":["rdf:Property","owl:ObjectProperty"],"rdfs:label":"signatoryAuthentication","schema:rangeIncludes":{"@id":"unece:Authentication"},"schema:domainIncludes":[{"@id":"unece:Document"},{"@id":"unece:ExchangedDocument"}],"rdfs:comment":"A signatory authentication for this referenced document."},{"@id":"unece:specifiedDocumentStatus","@type":["rdf:Property","owl:ObjectProperty"],"rdfs:label":"specifiedDocumentStatus","schema:rangeIncludes":{"@id":"unece:DocumentStatus"},"schema:domainIncludes":{"@id":"unece:Document"},"rdfs:comment":"Status information specified for this referenced document."},{"@id":"unece:status","@type":["rdf:Property","owl:DatatypeProperty"],"rdfs:label":"status","schema:rangeIncludes":{"@id":"schema:Text"},"schema:domainIncludes":[{"@id":"unece:Document"},{"@id":"unece:InspectionReference"},{"@id":"unece:LaboratoryObservationReference"}],"rdfs:comment":"A status, expressed as text, for this acknowledgement document."},{"@id":"unece:subordinateLineId","@type":["rdf:Property","owl:DatatypeProperty"],"rdfs:label":"subordinateLineId","schema:rangeIncludes":{"@id":"schema:Text"},"schema:domainIncludes":{"@id":"unece:Document"},"rdfs:comment":"An identifier of a subordinate line of this document line."},{"@id":"unece:subtypeCode","@type":["rdf:Property","owl:DatatypeProperty"],"rdfs:label":"subtypeCode","schema:rangeIncludes":{"@id":"schema:Text"},"schema:domainIncludes":[{"@id":"unece:Document"},{"@id":"unece:ExchangedDocument"}],"rdfs:comment":"A code specifying a subtype of this referenced document."},{"@id":"unece:totalIssueCountNumeric","@type":["rdf:Property","owl:DatatypeProperty"],"rdfs:label":"totalIssueCountNumeric","schema:rangeIncludes":{"@id":"schema:Text"},"schema:domainIncludes":{"@id":"unece:Document"},"rdfs:comment":"The total issue count for this referenced document."},{"@id":"unece:uRIId","@type":["rdf:Property","owl:DatatypeProperty"],"rdfs:label":"uRIId","schema:rangeIncludes":{"@id":"schema:Text"},"schema:domainIncludes":[{"@id":"unece:Document"},{"@id":"unece:BinaryFile"},{"@id":"unece:Picture"},{"@id":"unece:Communication"},{"@id":"unece:Standard"},{"@id":"unece:SpecifiedCertification"}],"rdfs:comment":"A Uniform Resource Identifier (URI) for this specified certification."},{"@id":"unece:validityPeriod","@type":["rdf:Property","owl:ObjectProperty"],"rdfs:label":"validityPeriod","schema:rangeIncludes":{"@id":"unece:SpecifiedPeriod"},"schema:domainIncludes":[{"@id":"unece:Document"},{"@id":"unece:BinaryFile"},{"@id":"unece:DocumentStatus"},{"@id":"unece:GovernmentRegistration"}],"rdfs:comment":"A period of validity specified for this referenced document."},{"@id":"unece:versionId","@type":["rdf:Property","owl:DatatypeProperty"],"rdfs:label":"versionId","schema:rangeIncludes":{"@id":"schema:Text"},"schema:domainIncludes":[{"@id":"unece:Document"},{"@id":"unece:ExchangedDocument"},{"@id":"unece:BinaryFile"},{"@id":"unece:SpecialQuery"},{"@id":"unece:Standard"},{"@id":"unece:GovernmentRegistration"},{"@id":"unece:CalibratedMeasurement"}],"rdfs:comment":"The identifier for the version of this exchanged declaration."},{"@id":"unece:agentParty","@type":["rdf:Property","owl:ObjectProperty"],"rdfs:label":"agentParty","schema:rangeIncludes":{"@id":"unece:Party"},"schema:domainIncludes":{"@id":"unece:ExchangedDocument"},"rdfs:comment":"A party representing another party for this exchanged document."},{"@id":"unece:amendmentPurpose","@type":["rdf:Property","owl:DatatypeProperty"],"rdfs:label":"amendmentPurpose","schema:rangeIncludes":{"@id":"schema:Text"},"schema:domainIncludes":{"@id":"unece:ExchangedDocument"},"rdfs:comment":"An amendment purpose, expressed in text, for this exchanged document."},{"@id":"unece:approverSignatoryAuthentication","@type":["rdf:Property","owl:ObjectProperty"],"rdfs:label":"approverSignatoryAuthentication","schema:rangeIncludes":{"@id":"unece:Authentication"},"schema:domainIncludes":{"@id":"unece:ExchangedDocument"},"rdfs:comment":"The approver signature that authenticates this exchanged document."},{"@id":"unece:buyerSignatoryAuthentication","@type":["rdf:Property","owl:ObjectProperty"],"rdfs:label":"buyerSignatoryAuthentication","schema:rangeIncludes":{"@id":"unece:Authentication"},"schema:domainIncludes":{"@id":"unece:ExchangedDocument"},"rdfs:comment":"The buyer signature that authenticates this exchanged document."},{"@id":"unece:cancellationDateTime","@type":["rdf:Property","owl:DatatypeProperty"],"rdfs:label":"cancellationDateTime","schema:rangeIncludes":{"@id":"schema:Text"},"schema:domainIncludes":{"@id":"unece:ExchangedDocument"},"rdfs:comment":"The date, time, date time, or other date time value of a cancellation of the exchanged document."},{"@id":"unece:controlRequirementIndicator","@type":["rdf:Property","owl:DatatypeProperty"],"rdfs:label":"controlRequirementIndicator","schema:rangeIncludes":{"@id":"schema:Boolean"},"schema:domainIncludes":[{"@id":"unece:ExchangedDocument"},{"@id":"unece:RegulatoryProcedure"}],"rdfs:comment":"The indication of whether or not a control is required for this cross-border regulatory procedure."},{"@id":"unece:copyIssuedQuantity","@type":["rdf:Property","owl:ObjectProperty"],"rdfs:label":"copyIssuedQuantity","schema:rangeIncludes":{"@id":"unece:QuantityType"},"schema:domainIncludes":{"@id":"unece:ExchangedDocument"},"rdfs:comment":"The number of copies issued of this exchanged document."},{"@id":"unece:copyRequiredQuantity","@type":["rdf:Property","owl:ObjectProperty"],"rdfs:label":"copyRequiredQuantity","schema:rangeIncludes":{"@id":"unece:QuantityType"},"schema:domainIncludes":{"@id":"unece:ExchangedDocument"},"rdfs:comment":"The number of copies required of this exchanged document."},{"@id":"unece:customsId","@type":["rdf:Property","owl:DatatypeProperty"],"rdfs:label":"customsId","schema:rangeIncludes":{"@id":"schema:Text"},"schema:domainIncludes":{"@id":"unece:ExchangedDocument"},"rdfs:comment":"A unique identifier, for customs purposes, for this consignment."},{"@id":"unece:exchangedDocumentAmendmentPurposeCode","@type":["rdf:Property","owl:DatatypeProperty"],"rdfs:label":"exchangedDocumentAmendmentPurposeCode","schema:rangeIncludes":{"@id":"schema:Text"},"schema:domainIncludes":{"@id":"unece:ExchangedDocument"},"rdfs:comment":"A code specifying a purpose of an amendment to this exchanged document."},{"@id":"unece:exchangedDocumentResponseTypeCode","@type":["rdf:Property","owl:DatatypeProperty"],"rdfs:label":"exchangedDocumentResponseTypeCode","schema:rangeIncludes":{"@id":"unece:ResponseTypeCodeList"},"schema:domainIncludes":{"@id":"unece:ExchangedDocument"},"rdfs:comment":"A code specifying a type of response requested for this exchanged document."},{"@id":"unece:firstSignatoryAuthentication","@type":["rdf:Property","owl:ObjectProperty"],"rdfs:label":"firstSignatoryAuthentication","schema:rangeIncludes":{"@id":"unece:Authentication"},"schema:domainIncludes":{"@id":"unece:ExchangedDocument"},"rdfs:comment":"The first or primary signature that authenticates this exchanged document."},{"@id":"unece:firstVersionIssueDateTime","@type":["rdf:Property","owl:DatatypeProperty"],"rdfs:label":"firstVersionIssueDateTime","schema:rangeIncludes":{"@id":"schema:Text"},"schema:domainIncludes":{"@id":"unece:ExchangedDocument"},"rdfs:comment":"The date, time, date time or other date time value when the first version of this exchanged document was issued."},{"@id":"unece:fourthSignatoryAuthentication","@type":["rdf:Property","owl:ObjectProperty"],"rdfs:label":"fourthSignatoryAuthentication","schema:rangeIncludes":{"@id":"unece:Authentication"},"schema:domainIncludes":{"@id":"unece:ExchangedDocument"},"rdfs:comment":"The fourth signature, also known as the third counter signature, that has been authenticated on this exchanged document indicating where appropriate the authentication party."},{"@id":"unece:languageId","@type":["rdf:Property","owl:DatatypeProperty"],"rdfs:label":"languageId","schema:rangeIncludes":{"@id":"schema:Text"},"schema:domainIncludes":{"@id":"unece:ExchangedDocument"},"rdfs:comment":"A unique identifier for a language used in this exchanged document."},{"@id":"unece:lineCountNumeric","@type":["rdf:Property","owl:DatatypeProperty"],"rdfs:label":"lineCountNumeric","schema:rangeIncludes":{"@id":"schema:Text"},"schema:domainIncludes":{"@id":"unece:ExchangedDocument"},"rdfs:comment":"The count of the number of lines in this exchanged document."},{"@id":"unece:lineItemQuantity","@type":["rdf:Property","owl:ObjectProperty"],"rdfs:label":"lineItemQuantity","schema:rangeIncludes":{"@id":"unece:QuantityType"},"schema:domainIncludes":{"@id":"unece:ExchangedDocument"},"rdfs:comment":"The number of line items for this supply chain trade transaction."},{"@id":"unece:messageFunctionPurposeCode","@type":["rdf:Property","owl:DatatypeProperty"],"rdfs:label":"messageFunctionPurposeCode","schema:rangeIncludes":{"@id":"unece:MessageFunctionCodeList"},"schema:domainIncludes":{"@id":"unece:ExchangedDocument"},"rdfs:comment":"A code specifying the purpose of this exchanged document, such as request or reminder."},{"@id":"unece:offsetProcessingStatus","@type":["rdf:Property","owl:DatatypeProperty"],"rdfs:label":"offsetProcessingStatus","schema:rangeIncludes":{"@id":"schema:Text"},"schema:domainIncludes":{"@id":"unece:ExchangedDocument"},"rdfs:comment":"A status of an offset processing, expressed as text, for this exchanged document, such as the process offsetted by this document."},{"@id":"unece:originalIssuedQuantity","@type":["rdf:Property","owl:ObjectProperty"],"rdfs:label":"originalIssuedQuantity","schema:rangeIncludes":{"@id":"unece:QuantityType"},"schema:domainIncludes":{"@id":"unece:ExchangedDocument"},"rdfs:comment":"The number of originals issued of this exchanged document."},{"@id":"unece:originalRequiredQuantity","@type":["rdf:Property","owl:ObjectProperty"],"rdfs:label":"originalRequiredQuantity","schema:rangeIncludes":{"@id":"unece:QuantityType"},"schema:domainIncludes":{"@id":"unece:ExchangedDocument"},"rdfs:comment":"The number of originals required of this exchanged document."},{"@id":"unece:purpose","@type":["rdf:Property","owl:DatatypeProperty"],"rdfs:label":"purpose","schema:rangeIncludes":{"@id":"schema:Text"},"schema:domainIncludes":{"@id":"unece:ExchangedDocument"},"rdfs:comment":"The purpose, expressed as text, of this exchanged document."},{"@id":"unece:recipientAssignedId","@type":["rdf:Property","owl:DatatypeProperty"],"rdfs:label":"recipientAssignedId","schema:rangeIncludes":{"@id":"schema:Text"},"schema:domainIncludes":{"@id":"unece:ExchangedDocument"},"rdfs:comment":"A unique recipient assigned identifier for this exchanged document."},{"@id":"unece:referenceDocument","@type":["rdf:Property","owl:ObjectProperty"],"rdfs:label":"referenceDocument","schema:rangeIncludes":{"@id":"unece:Document"},"schema:domainIncludes":{"@id":"unece:ExchangedDocument"},"rdfs:comment":"A document referenced by this acknowledgement document."},{"@id":"unece:rejectionResponseDateTime","@type":["rdf:Property","owl:DatatypeProperty"],"rdfs:label":"rejectionResponseDateTime","schema:rangeIncludes":{"@id":"schema:Text"},"schema:domainIncludes":{"@id":"unece:ExchangedDocument"},"rdfs:comment":"A date, time, date time, or other date time value of a rejection response of the exchanged document."},{"@id":"unece:responseDateTime","@type":["rdf:Property","owl:DatatypeProperty"],"rdfs:label":"responseDateTime","schema:rangeIncludes":{"@id":"schema:Text"},"schema:domainIncludes":[{"@id":"unece:ExchangedDocument"},{"@id":"unece:SpecialQuery"}],"rdfs:comment":"A date, time, date time, or other date time value of a response of the exchanged document."},{"@id":"unece:responseReasonCode","@type":["rdf:Property","owl:DatatypeProperty"],"rdfs:label":"responseReasonCode","schema:rangeIncludes":{"@id":"schema:Text"},"schema:domainIncludes":{"@id":"unece:ExchangedDocument"},"rdfs:comment":"A code specifying a response reason for this exchanged document."},{"@id":"unece:revisionDateTime","@type":["rdf:Property","owl:DatatypeProperty"],"rdfs:label":"revisionDateTime","schema:rangeIncludes":{"@id":"schema:Text"},"schema:domainIncludes":{"@id":"unece:ExchangedDocument"},"rdfs:comment":"The date, time, date time or other date time value for the revision of this exchanged document."},{"@id":"unece:secondSignatoryAuthentication","@type":["rdf:Property","owl:ObjectProperty"],"rdfs:label":"secondSignatoryAuthentication","schema:rangeIncludes":{"@id":"unece:Authentication"},"schema:domainIncludes":{"@id":"unece:ExchangedDocument"},"rdfs:comment":"The second signature, also known as the first counter signature, that has been authenticated on this exchanged document indicating where appropriate the authentication party."},{"@id":"unece:senderAssignedId","@type":["rdf:Property","owl:DatatypeProperty"],"rdfs:label":"senderAssignedId","schema:rangeIncludes":{"@id":"schema:Text"},"schema:domainIncludes":{"@id":"unece:ExchangedDocument"},"rdfs:comment":"A unique sender assigned identifier for this exchanged document."},{"@id":"unece:submissionDateTime","@type":["rdf:Property","owl:DatatypeProperty"],"rdfs:label":"submissionDateTime","schema:rangeIncludes":{"@id":"schema:Text"},"schema:domainIncludes":{"@id":"unece:ExchangedDocument"},"rdfs:comment":"The date, time, date time or other date time value for the formal submission of this exchanged document to a receiver by a sender."},{"@id":"unece:thirdSignatoryAuthentication","@type":["rdf:Property","owl:ObjectProperty"],"rdfs:label":"thirdSignatoryAuthentication","schema:rangeIncludes":{"@id":"unece:Authentication"},"schema:domainIncludes":{"@id":"unece:ExchangedDocument"},"rdfs:comment":"The third signature, also known as the second counter signature, that has been authenticated on this exchanged document indicating where appropriate the authentication party."},{"@id":"unece:traderAssignedId","@type":["rdf:Property","owl:DatatypeProperty"],"rdfs:label":"traderAssignedId","schema:rangeIncludes":{"@id":"schema:Text"},"schema:domainIncludes":{"@id":"unece:ExchangedDocument"},"rdfs:comment":"A unique trader assigned identifier for this exchanged document."},{"@id":"unece:urgency","@type":["rdf:Property","owl:DatatypeProperty"],"rdfs:label":"urgency","schema:rangeIncludes":{"@id":"schema:Text"},"schema:domainIncludes":{"@id":"unece:ExchangedDocument"},"rdfs:comment":"An urgency, expressed as text, of this exchanged document."},{"@id":"unece:urgencyCode","@type":["rdf:Property","owl:DatatypeProperty"],"rdfs:label":"urgencyCode","schema:rangeIncludes":{"@id":"schema:Text"},"schema:domainIncludes":{"@id":"unece:ExchangedDocument"},"rdfs:comment":"The code specifying the urgency for this exchanged document."},{"@id":"unece:access","@type":["rdf:Property","owl:DatatypeProperty"],"rdfs:label":"access","schema:rangeIncludes":{"@id":"schema:Text"},"schema:domainIncludes":{"@id":"unece:BinaryFile"},"rdfs:comment":"Access information, expressed as text, for this specified binary file, such as security and download parameters."},{"@id":"unece:accessAvailabilityPeriod","@type":["rdf:Property","owl:ObjectProperty"],"rdfs:label":"accessAvailabilityPeriod","schema:rangeIncludes":{"@id":"unece:SpecifiedPeriod"},"schema:domainIncludes":{"@id":"unece:BinaryFile"},"rdfs:comment":"The specified period when access to this binary file is available."},{"@id":"unece:authorName","@type":["rdf:Property","owl:DatatypeProperty"],"rdfs:label":"authorName","schema:rangeIncludes":{"@id":"schema:Text"},"schema:domainIncludes":{"@id":"unece:BinaryFile"},"rdfs:comment":"A name of an author, expressed as text, of this specified binary file."},{"@id":"unece:characterSetCode","@type":["rdf:Property","owl:DatatypeProperty"],"rdfs:label":"characterSetCode","schema:rangeIncludes":{"@id":"schema:Text"},"schema:domainIncludes":{"@id":"unece:BinaryFile"},"rdfs:comment":"The code specifying the character set for this specified binary file."},{"@id":"unece:encodingCode","@type":["rdf:Property","owl:DatatypeProperty"],"rdfs:label":"encodingCode","schema:rangeIncludes":{"@id":"schema:Text"},"schema:domainIncludes":{"@id":"unece:BinaryFile"},"rdfs:comment":"The code specifying the encoding of this specified binary file."},{"@id":"unece:fileName","@type":["rdf:Property","owl:DatatypeProperty"],"rdfs:label":"fileName","schema:rangeIncludes":{"@id":"schema:Text"},"schema:domainIncludes":{"@id":"unece:BinaryFile"},"rdfs:comment":"The file name, expressed as text, of this specified binary file."},{"@id":"unece:includedBinaryObject","@type":["rdf:Property","owl:DatatypeProperty"],"rdfs:label":"includedBinaryObject","schema:rangeIncludes":{"@id":"schema:Text"},"schema:domainIncludes":{"@id":"unece:BinaryFile"},"rdfs:comment":"A binary object included in this specified binary file."},{"@id":"unece:mIMECode","@type":["rdf:Property","owl:DatatypeProperty"],"rdfs:label":"mIMECode","schema:rangeIncludes":{"@id":"unece:MimeCodeList"},"schema:domainIncludes":{"@id":"unece:BinaryFile"},"rdfs:comment":"The code specifying the Multipurpose Internet Mail Extensions (MIME) type for this specified binary file."},{"@id":"unece:title","@type":["rdf:Property","owl:DatatypeProperty"],"rdfs:label":"title","schema:rangeIncludes":{"@id":"schema:Text"},"schema:domainIncludes":{"@id":"unece:BinaryFile"},"rdfs:comment":"A title, expressed as text, for this specified binary file."},{"@id":"unece:acquisitionDateTime","@type":["rdf:Property","owl:DatatypeProperty"],"rdfs:label":"acquisitionDateTime","schema:rangeIncludes":{"@id":"schema:Text"},"schema:domainIncludes":[{"@id":"unece:GeographicalCoordinate"},{"@id":"unece:RegulatoryProcedure"}],"rdfs:comment":"The date, time, date time or other date time value of the acquisition of this geographical coordinate."},{"@id":"unece:alternativeSourceSystemId","@type":["rdf:Property","owl:DatatypeProperty"],"rdfs:label":"alternativeSourceSystemId","schema:rangeIncludes":{"@id":"schema:Text"},"schema:domainIncludes":{"@id":"unece:GeographicalCoordinate"},"rdfs:comment":"An alternative source system identifier for this geographical coordinate."},{"@id":"unece:altimetricSystemId","@type":["rdf:Property","owl:DatatypeProperty"],"rdfs:label":"altimetricSystemId","schema:rangeIncludes":{"@id":"schema:Text"},"schema:domainIncludes":{"@id":"unece:GeographicalCoordinate"},"rdfs:comment":"The unique identifier of the system used for measuring the altitude."},{"@id":"unece:altitudeMeasure","@type":["rdf:Property","owl:ObjectProperty"],"rdfs:label":"altitudeMeasure","schema:rangeIncludes":{"@id":"unece:MeasureType"},"schema:domainIncludes":{"@id":"unece:GeographicalCoordinate"},"rdfs:comment":"The measure of the altitude that reflects the vertical elevation of an object above a surface for this geographical coordinate (Reference ISO 6709)."},{"@id":"unece:latitudeDirectionIndicator","@type":["rdf:Property","owl:DatatypeProperty"],"rdfs:label":"latitudeDirectionIndicator","schema:rangeIncludes":{"@id":"schema:Boolean"},"schema:domainIncludes":{"@id":"unece:GeographicalCoordinate"},"rdfs:comment":"The indication of whether the latitude compass direction from the Equator meridian to the meridian of a specific place is North (+) or South (-)  (Reference ISO 6709)."},{"@id":"unece:latitudeMeasure","@type":["rdf:Property","owl:ObjectProperty"],"rdfs:label":"latitudeMeasure","schema:rangeIncludes":{"@id":"unece:MeasureType"},"schema:domainIncludes":{"@id":"unece:GeographicalCoordinate"},"rdfs:comment":"The measure of the latitude as an angular distance north or south from the Equator meridian to the meridian of a specific place for this geographical coordinate (Reference ISO 6709)."},{"@id":"unece:longitudeDirectionIndicator","@type":["rdf:Property","owl:DatatypeProperty"],"rdfs:label":"longitudeDirectionIndicator","schema:rangeIncludes":{"@id":"schema:Boolean"},"schema:domainIncludes":{"@id":"unece:GeographicalCoordinate"},"rdfs:comment":"The indication of whether the longitude as a compass direction from the Greenwich meridian to the meridian of a specific place is East (+) or West (-) for this geographical coordinate (Reference ISO 6709)."},{"@id":"unece:longitudeMeasure","@type":["rdf:Property","owl:ObjectProperty"],"rdfs:label":"longitudeMeasure","schema:rangeIncludes":{"@id":"unece:MeasureType"},"schema:domainIncludes":{"@id":"unece:GeographicalCoordinate"},"rdfs:comment":"The measure of the longitude as an angular distance east or west from the Greenwich meridian to the meridian of a specific place (Reference ISO 6709)."},{"@id":"unece:systemId","@type":["rdf:Property","owl:DatatypeProperty"],"rdfs:label":"systemId","schema:rangeIncludes":{"@id":"schema:Text"},"schema:domainIncludes":{"@id":"unece:GeographicalCoordinate"},"rdfs:comment":"The unique identifier of the classification system for this product classification."},{"@id":"unece:timeZone","@type":["rdf:Property","owl:DatatypeProperty"],"rdfs:label":"timeZone","schema:rangeIncludes":{"@id":"schema:Text"},"schema:domainIncludes":{"@id":"unece:GeographicalCoordinate"},"rdfs:comment":"The time zone, expressed as text, for this geographical coordinate."},{"@id":"unece:timeZoneCode","@type":["rdf:Property","owl:DatatypeProperty"],"rdfs:label":"timeZoneCode","schema:rangeIncludes":{"@id":"schema:Text"},"schema:domainIncludes":{"@id":"unece:GeographicalCoordinate"},"rdfs:comment":"The code specifying the time zone of this geographical coordinate."},{"@id":"unece:timeZoneDateTime","@type":["rdf:Property","owl:DatatypeProperty"],"rdfs:label":"timeZoneDateTime","schema:rangeIncludes":{"@id":"schema:DateTime"},"schema:domainIncludes":{"@id":"unece:GeographicalCoordinate"},"rdfs:comment":"The date, time, date time, or other date time value for the time zone of this geographical coordinate."},{"@id":"unece:usedCoordinateReferenceSystem","@type":["rdf:Property","owl:ObjectProperty"],"rdfs:label":"usedCoordinateReferenceSystem","schema:rangeIncludes":{"@id":"unece:CoordinateReferenceSystem"},"schema:domainIncludes":[{"@id":"unece:GeographicalCoordinate"},{"@id":"unece:GeographicalFeature"}],"rdfs:comment":"The CS (Coordinate System) engineering coordinate reference system used for this geographical coordinate."},{"@id":"unece:usedCoordinateSourceSystem","@type":["rdf:Property","owl:ObjectProperty"],"rdfs:label":"usedCoordinateSourceSystem","schema:rangeIncludes":{"@id":"unece:CoordinateSourceSystem"},"schema:domainIncludes":[{"@id":"unece:GeographicalCoordinate"},{"@id":"unece:GeographicalFeature"}],"rdfs:comment":"The geographical coordinate source system used for this geographical coordinate."},{"@id":"unece:actionType","@type":["rdf:Property","owl:DatatypeProperty"],"rdfs:label":"actionType","schema:rangeIncludes":{"@id":"schema:Text"},"schema:domainIncludes":[{"@id":"unece:SpecifiedAction"},{"@id":"unece:CorrectiveAction"},{"@id":"unece:PreventiveAction"}],"rdfs:comment":"A type, expressed as text, for this corrective action."},{"@id":"unece:activityAuthorizedParty","@type":["rdf:Property","owl:ObjectProperty"],"rdfs:label":"activityAuthorizedParty","schema:rangeIncludes":{"@id":"unece:Party"},"schema:domainIncludes":{"@id":"unece:CountrySubDivision"},"rdfs:comment":"A party that is authorized to perform an activity in this trade country sub-division."},{"@id":"unece:hierarchicalLevelCode","@type":["rdf:Property","owl:DatatypeProperty"],"rdfs:label":"hierarchicalLevelCode","schema:rangeIncludes":{"@id":"schema:Text"},"schema:domainIncludes":{"@id":"unece:CountrySubDivision"},"rdfs:comment":"The code specifying the hierarchical level of this trade country sub-division."},{"@id":"unece:locationFunctionTypeCode","@type":["rdf:Property","owl:DatatypeProperty"],"rdfs:label":"locationFunctionTypeCode","schema:rangeIncludes":{"@id":"unece:LocationFunctionCodeList"},"schema:domainIncludes":[{"@id":"unece:CountrySubDivision"},{"@id":"unece:SubordinateLocation"},{"@id":"unece:SubordinateSubordinateLocation"}],"rdfs:comment":"A code specifying the type of this logistics related location."},{"@id":"unece:subordinateCountrySubDivision","@type":["rdf:Property","owl:ObjectProperty"],"rdfs:label":"subordinateCountrySubDivision","schema:rangeIncludes":{"@id":"unece:CountrySubDivision"},"schema:domainIncludes":[{"@id":"unece:CountrySubDivision"},{"@id":"unece:Country"}],"rdfs:comment":"A subordinate country sub-division within this trade country sub-division."},{"@id":"unece:superordinateCountrySubDivision","@type":["rdf:Property","owl:ObjectProperty"],"rdfs:label":"superordinateCountrySubDivision","schema:rangeIncludes":{"@id":"unece:CountrySubDivision"},"schema:domainIncludes":{"@id":"unece:CountrySubDivision"},"rdfs:comment":"A superordinate country sub-division for this trade country sub-division."},{"@id":"unece:activityLevelMeasure","@type":["rdf:Property","owl:ObjectProperty"],"rdfs:label":"activityLevelMeasure","schema:rangeIncludes":{"@id":"unece:MeasureType"},"schema:domainIncludes":{"@id":"unece:RadioactiveIsotope"},"rdfs:comment":"A measure of the activity level of this specified radioactive isotope."},{"@id":"unece:note","@type":["rdf:Property","owl:DatatypeProperty"],"rdfs:label":"note","schema:rangeIncludes":{"@id":"schema:Text"},"schema:domainIncludes":{"@id":"unece:RadioactiveIsotope"},"rdfs:comment":"A note, expressed as text, for this specified radioactive isotope."},{"@id":"unece:specifiedRadionuclide","@type":["rdf:Property","owl:ObjectProperty"],"rdfs:label":"specifiedRadionuclide","schema:rangeIncludes":{"@id":"unece:Radionuclide"},"schema:domainIncludes":{"@id":"unece:RadioactiveIsotope"},"rdfs:comment":"The radionuclide details specified for this radioactive isotope."},{"@id":"unece:actualMeasure","@type":["rdf:Property","owl:ObjectProperty"],"rdfs:label":"actualMeasure","schema:rangeIncludes":{"@id":"unece:MeasureType"},"schema:domainIncludes":{"@id":"unece:Measurement"},"rdfs:comment":"An actual measure for this measurement."},{"@id":"unece:comparisonOperatorCode","@type":["rdf:Property","owl:DatatypeProperty"],"rdfs:label":"comparisonOperatorCode","schema:rangeIncludes":{"@id":"schema:Text"},"schema:domainIncludes":[{"@id":"unece:Measurement"},{"@id":"unece:InspectionResultCharacteristic"},{"@id":"unece:ObservationResultCharacteristic"}],"rdfs:comment":"A code specifying the operator, such as, less than, greater than or equal to, for comparing two actual measures."},{"@id":"unece:conditionMeasure","@type":["rdf:Property","owl:ObjectProperty"],"rdfs:label":"conditionMeasure","schema:rangeIncludes":{"@id":"unece:MeasureType"},"schema:domainIncludes":{"@id":"unece:Measurement"},"rdfs:comment":"A measure of a condition for this measurement."},{"@id":"unece:method","@type":["rdf:Property","owl:DatatypeProperty"],"rdfs:label":"method","schema:rangeIncludes":{"@id":"schema:Text"},"schema:domainIncludes":{"@id":"unece:Measurement"},"rdfs:comment":"A measurement method expressed as text."},{"@id":"unece:actualQuantity","@type":["rdf:Property","owl:ObjectProperty"],"rdfs:label":"actualQuantity","schema:rangeIncludes":{"@id":"unece:QuantityType"},"schema:domainIncludes":{"@id":"unece:QuantityAnalysis"},"rdfs:comment":"The actual quantity added or subtracted as a result of this delivery adjustment."},{"@id":"unece:actualQuantityDimension","@type":["rdf:Property","owl:ObjectProperty"],"rdfs:label":"actualQuantityDimension","schema:rangeIncludes":{"@id":"unece:WorkItemDimension"},"schema:domainIncludes":{"@id":"unece:QuantityAnalysis"},"rdfs:comment":"A work item dimension of the actual quantity in this work item quantity analysis."},{"@id":"unece:actualQuantityPercent","@type":["rdf:Property","owl:DatatypeProperty"],"rdfs:label":"actualQuantityPercent","schema:rangeIncludes":{"@id":"schema:Text"},"schema:domainIncludes":{"@id":"unece:QuantityAnalysis"},"rdfs:comment":"The percentage of a total quantity that the actual quantity of this work item quantity analysis represents."},{"@id":"unece:alternativeClassificationCode","@type":["rdf:Property","owl:DatatypeProperty"],"rdfs:label":"alternativeClassificationCode","schema:rangeIncludes":{"@id":"schema:Text"},"schema:domainIncludes":[{"@id":"unece:QuantityAnalysis"},{"@id":"unece:ProcessWorkItem"}],"rdfs:comment":"A code specifying an alternative classification for this basic work item."},{"@id":"unece:breakdownQuantityAnalysis","@type":["rdf:Property","owl:ObjectProperty"],"rdfs:label":"breakdownQuantityAnalysis","schema:rangeIncludes":{"@id":"unece:QuantityAnalysis"},"schema:domainIncludes":{"@id":"unece:QuantityAnalysis"},"rdfs:comment":"A quantity analysis breakdown of this work item quantity analysis."},{"@id":"unece:changedStatus","@type":["rdf:Property","owl:ObjectProperty"],"rdfs:label":"changedStatus","schema:rangeIncludes":{"@id":"unece:RecordedStatus"},"schema:domainIncludes":{"@id":"unece:QuantityAnalysis"},"rdfs:comment":"A changed recorded status for this basic work item."},{"@id":"unece:primaryClassificationCode","@type":["rdf:Property","owl:DatatypeProperty"],"rdfs:label":"primaryClassificationCode","schema:rangeIncludes":{"@id":"schema:Text"},"schema:domainIncludes":[{"@id":"unece:QuantityAnalysis"},{"@id":"unece:ProcessWorkItem"}],"rdfs:comment":"A code specifying a primary classification value for this work item quantity analysis."},{"@id":"unece:actualSpecifiedPercent","@type":["rdf:Property","owl:DatatypeProperty"],"rdfs:label":"actualSpecifiedPercent","schema:rangeIncludes":{"@id":"schema:Text"},"schema:domainIncludes":{"@id":"unece:SpecifiedFault"},"rdfs:comment":"The actual percentage of this specified fault."},{"@id":"unece:actualSpecifiedQuantity","@type":["rdf:Property","owl:ObjectProperty"],"rdfs:label":"actualSpecifiedQuantity","schema:rangeIncludes":{"@id":"unece:QuantityType"},"schema:domainIncludes":{"@id":"unece:SpecifiedFault"},"rdfs:comment":"The actual total quantity of this specified fault."},{"@id":"unece:estimatedSpecifiedPercent","@type":["rdf:Property","owl:DatatypeProperty"],"rdfs:label":"estimatedSpecifiedPercent","schema:rangeIncludes":{"@id":"schema:Text"},"schema:domainIncludes":{"@id":"unece:SpecifiedFault"},"rdfs:comment":"The estimated percentage of this specified fault."},{"@id":"unece:faultType","@type":["rdf:Property","owl:DatatypeProperty"],"rdfs:label":"faultType","schema:rangeIncludes":{"@id":"schema:Text"},"schema:domainIncludes":{"@id":"unece:SpecifiedFault"},"rdfs:comment":"A type, expressed as text, of this specified fault."},{"@id":"unece:operationalApplicableTolerance","@type":["rdf:Property","owl:ObjectProperty"],"rdfs:label":"operationalApplicableTolerance","schema:rangeIncludes":{"@id":"unece:Tolerance"},"schema:domainIncludes":{"@id":"unece:SpecifiedFault"},"rdfs:comment":"An applicable operational tolerance of this specified fault."},{"@id":"unece:additionalDescription","@type":["rdf:Property","owl:DatatypeProperty"],"rdfs:label":"additionalDescription","schema:rangeIncludes":{"@id":"schema:Text"},"schema:domainIncludes":{"@id":"unece:Picture"},"rdfs:comment":"An additional textual description for this trade product."},{"@id":"unece:areaIncluded","@type":["rdf:Property","owl:DatatypeProperty"],"rdfs:label":"areaIncluded","schema:rangeIncludes":{"@id":"schema:Text"},"schema:domainIncludes":{"@id":"unece:Picture"},"rdfs:comment":"The area or location, expressed as text, that is included in this photographic picture."},{"@id":"unece:copyrightOwnerName","@type":["rdf:Property","owl:DatatypeProperty"],"rdfs:label":"copyrightOwnerName","schema:rangeIncludes":{"@id":"schema:Text"},"schema:domainIncludes":{"@id":"unece:Picture"},"rdfs:comment":"The name of the copyright owner, expressed as text, for this photographic picture."},{"@id":"unece:digitalImageBinaryObject","@type":["rdf:Property","owl:DatatypeProperty"],"rdfs:label":"digitalImageBinaryObject","schema:rangeIncludes":{"@id":"schema:Text"},"schema:domainIncludes":{"@id":"unece:Picture"},"rdfs:comment":"Binary object data that is the actual digital image for this photographic picture."},{"@id":"unece:intendedUse","@type":["rdf:Property","owl:DatatypeProperty"],"rdfs:label":"intendedUse","schema:rangeIncludes":{"@id":"schema:Text"},"schema:domainIncludes":{"@id":"unece:Picture"},"rdfs:comment":"An intended use, expressed as text, for this photographic picture."},{"@id":"unece:intendedUseCode","@type":["rdf:Property","owl:DatatypeProperty"],"rdfs:label":"intendedUseCode","schema:rangeIncludes":{"@id":"schema:Text"},"schema:domainIncludes":{"@id":"unece:Picture"},"rdfs:comment":"The code specifying the intended use of this photographic picture."},{"@id":"unece:linearDimension","@type":["rdf:Property","owl:ObjectProperty"],"rdfs:label":"linearDimension","schema:rangeIncludes":{"@id":"unece:SpatialDimension"},"schema:domainIncludes":{"@id":"unece:Picture"},"rdfs:comment":"A linear dimension or a set of linear dimensions of this logistics packaging."},{"@id":"unece:pictureType","@type":["rdf:Property","owl:DatatypeProperty"],"rdfs:label":"pictureType","schema:rangeIncludes":{"@id":"schema:Text"},"schema:domainIncludes":{"@id":"unece:Picture"},"rdfs:comment":"The type, expressed as text, of this photographic picture."},{"@id":"unece:reference","@type":["rdf:Property","owl:DatatypeProperty"],"rdfs:label":"reference","schema:rangeIncludes":{"@id":"schema:Text"},"schema:domainIncludes":{"@id":"unece:Picture"},"rdfs:comment":"A reference, expressed as text, for this header trade agreement."},{"@id":"unece:renderingInformation","@type":["rdf:Property","owl:DatatypeProperty"],"rdfs:label":"renderingInformation","schema:rangeIncludes":{"@id":"schema:Text"},"schema:domainIncludes":{"@id":"unece:Picture"},"rdfs:comment":"Rendering information, expressed as text, for this photographic picture."},{"@id":"unece:resolutionTypeCode","@type":["rdf:Property","owl:DatatypeProperty"],"rdfs:label":"resolutionTypeCode","schema:rangeIncludes":{"@id":"schema:Text"},"schema:domainIncludes":{"@id":"unece:Picture"},"rdfs:comment":"The code specifying the type of resolution for this photographic picture."},{"@id":"unece:resolutionValueNumeric","@type":["rdf:Property","owl:DatatypeProperty"],"rdfs:label":"resolutionValueNumeric","schema:rangeIncludes":{"@id":"schema:Text"},"schema:domainIncludes":{"@id":"unece:Picture"},"rdfs:comment":"The value, expressed as a number, for the resolution of this photographic picture."},{"@id":"unece:specifiedNote","@type":["rdf:Property","owl:ObjectProperty"],"rdfs:label":"specifiedNote","schema:rangeIncludes":{"@id":"unece:Note"},"schema:domainIncludes":{"@id":"unece:Picture"},"rdfs:comment":"A note specified for this photographic picture."},{"@id":"unece:subject","@type":["rdf:Property","owl:DatatypeProperty"],"rdfs:label":"subject","schema:rangeIncludes":{"@id":"schema:Text"},"schema:domainIncludes":[{"@id":"unece:Picture"},{"@id":"unece:Note"},{"@id":"unece:SpecialQuery"},{"@id":"unece:SpecifiedNote"}],"rdfs:comment":"A subject, expressed as text, of this specified note."},{"@id":"unece:takenDateTime","@type":["rdf:Property","owl:DatatypeProperty"],"rdfs:label":"takenDateTime","schema:rangeIncludes":{"@id":"schema:Text"},"schema:domainIncludes":{"@id":"unece:Picture"},"rdfs:comment":"The date, time, date time, or other date value of when this photographic picture was created."},{"@id":"unece:titleName","@type":["rdf:Property","owl:DatatypeProperty"],"rdfs:label":"titleName","schema:rangeIncludes":{"@id":"schema:Text"},"schema:domainIncludes":{"@id":"unece:Picture"},"rdfs:comment":"The name, expressed as text, of the title for this photographic picture."},{"@id":"unece:additionalReason","@type":["rdf:Property","owl:DatatypeProperty"],"rdfs:label":"additionalReason","schema:rangeIncludes":{"@id":"schema:Text"},"schema:domainIncludes":{"@id":"unece:ValidationStatus"},"rdfs:comment":"Information, expressed as text, related to the reason for this validation status."},{"@id":"unece:reason","@type":["rdf:Property","owl:DatatypeProperty"],"rdfs:label":"reason","schema:rangeIncludes":{"@id":"schema:Text"},"schema:domainIncludes":[{"@id":"unece:ValidationStatus"},{"@id":"unece:CancellationStatus"},{"@id":"unece:DocumentStatus"}],"rdfs:comment":"A reason, expressed as text, for this cancellation status."},{"@id":"unece:reasonCode","@type":["rdf:Property","owl:DatatypeProperty"],"rdfs:label":"reasonCode","schema:rangeIncludes":{"@id":"schema:Text"},"schema:domainIncludes":[{"@id":"unece:ValidationStatus"},{"@id":"unece:Error"},{"@id":"unece:CommunicationEvent"},{"@id":"unece:CancellationStatus"}],"rdfs:comment":"A code specifying a reason for the declared error."},{"@id":"unece:validationDocumentStatusConditionCode","@type":["rdf:Property","owl:DatatypeProperty"],"rdfs:label":"validationDocumentStatusConditionCode","schema:rangeIncludes":{"@id":"unece:ValidationDocumentStatusCodeList"},"schema:domainIncludes":{"@id":"unece:ValidationStatus"},"rdfs:comment":"The code specifying the condition of this validation status."},{"@id":"unece:ageLimitation","@type":["rdf:Property","owl:DatatypeProperty"],"rdfs:label":"ageLimitation","schema:rangeIncludes":{"@id":"schema:Text"},"schema:domainIncludes":{"@id":"unece:UsageCondition"},"rdfs:comment":"An age limitation, expressed as text, for this specified usage condition."},{"@id":"unece:appropriateClothing","@type":["rdf:Property","owl:DatatypeProperty"],"rdfs:label":"appropriateClothing","schema:rangeIncludes":{"@id":"schema:Text"},"schema:domainIncludes":{"@id":"unece:UsageCondition"},"rdfs:comment":"Appropriate clothing, expressed as text, for this specified usage condition."},{"@id":"unece:duration","@type":["rdf:Property","owl:DatatypeProperty"],"rdfs:label":"duration","schema:rangeIncludes":{"@id":"schema:Text"},"schema:domainIncludes":[{"@id":"unece:UsageCondition"},{"@id":"unece:SpecifiedPeriod"}],"rdfs:comment":"A duration, expressed as text, for this specified period."},{"@id":"unece:genderLimitation","@type":["rdf:Property","owl:DatatypeProperty"],"rdfs:label":"genderLimitation","schema:rangeIncludes":{"@id":"schema:Text"},"schema:domainIncludes":{"@id":"unece:UsageCondition"},"rdfs:comment":"A gender limitation, expressed as text, for this specified usage condition."},{"@id":"unece:occupancy","@type":["rdf:Property","owl:DatatypeProperty"],"rdfs:label":"occupancy","schema:rangeIncludes":{"@id":"schema:Text"},"schema:domainIncludes":{"@id":"unece:UsageCondition"},"rdfs:comment":"Occupancy, expressed as text, for this specified usage condition."},{"@id":"unece:requiringParty","@type":["rdf:Property","owl:ObjectProperty"],"rdfs:label":"requiringParty","schema:rangeIncludes":{"@id":"unece:Party"},"schema:domainIncludes":{"@id":"unece:UsageCondition"},"rdfs:comment":"A party requiring this specified usage condition."},{"@id":"unece:alienRegistrationId","@type":["rdf:Property","owl:DatatypeProperty"],"rdfs:label":"alienRegistrationId","schema:rangeIncludes":{"@id":"schema:Text"},"schema:domainIncludes":{"@id":"unece:PersonIdentity"},"rdfs:comment":"The alien registration identifier for this person."},{"@id":"unece:driversLicenceId","@type":["rdf:Property","owl:DatatypeProperty"],"rdfs:label":"driversLicenceId","schema:rangeIncludes":{"@id":"schema:Text"},"schema:domainIncludes":{"@id":"unece:PersonIdentity"},"rdfs:comment":"The drivers licence identifier for this person."},{"@id":"unece:identityCardId","@type":["rdf:Property","owl:DatatypeProperty"],"rdfs:label":"identityCardId","schema:rangeIncludes":{"@id":"schema:Text"},"schema:domainIncludes":{"@id":"unece:PersonIdentity"},"rdfs:comment":"The identity card identifier for this person."},{"@id":"unece:passportId","@type":["rdf:Property","owl:DatatypeProperty"],"rdfs:label":"passportId","schema:rangeIncludes":{"@id":"schema:Text"},"schema:domainIncludes":{"@id":"unece:PersonIdentity"},"rdfs:comment":"The identifier of the passport of this guest."},{"@id":"unece:socialSecurityId","@type":["rdf:Property","owl:DatatypeProperty"],"rdfs:label":"socialSecurityId","schema:rangeIncludes":{"@id":"schema:Text"},"schema:domainIncludes":{"@id":"unece:PersonIdentity"},"rdfs:comment":"The social security identifier for this person."},{"@id":"unece:specifiedProprietaryIdentity","@type":["rdf:Property","owl:ObjectProperty"],"rdfs:label":"specifiedProprietaryIdentity","schema:rangeIncludes":{"@id":"unece:ProprietaryIdentity"},"schema:domainIncludes":{"@id":"unece:PersonIdentity"},"rdfs:comment":"A proprietary Identity specified for this person."},{"@id":"unece:applicableParameter","@type":["rdf:Property","owl:ObjectProperty"],"rdfs:label":"applicableParameter","schema:rangeIncludes":{"@id":"unece:SpecifiedParameter"},"schema:domainIncludes":{"@id":"unece:SpecifiedMethod"},"rdfs:comment":"A parameter applicable to this specified method."},{"@id":"unece:certificationId","@type":["rdf:Property","owl:DatatypeProperty"],"rdfs:label":"certificationId","schema:rangeIncludes":{"@id":"schema:Text"},"schema:domainIncludes":[{"@id":"unece:SpecifiedMethod"},{"@id":"unece:LaboratoryObservationAnalysisMethod"}],"rdfs:comment":"A certification identifier of this specified method."},{"@id":"unece:certificationTypeCode","@type":["rdf:Property","owl:DatatypeProperty"],"rdfs:label":"certificationTypeCode","schema:rangeIncludes":{"@id":"schema:Text"},"schema:domainIncludes":[{"@id":"unece:SpecifiedMethod"},{"@id":"unece:LaboratoryObservationAnalysisMethod"}],"rdfs:comment":"The code specifying the certification type of this method."},{"@id":"unece:externalReference","@type":["rdf:Property","owl:DatatypeProperty"],"rdfs:label":"externalReference","schema:rangeIncludes":{"@id":"schema:Text"},"schema:domainIncludes":[{"@id":"unece:SpecifiedMethod"},{"@id":"unece:LaboratoryObservationAnalysisMethod"}],"rdfs:comment":"An external reference, expressed as text, for this specified method."},{"@id":"unece:localTypeCode","@type":["rdf:Property","owl:DatatypeProperty"],"rdfs:label":"localTypeCode","schema:rangeIncludes":{"@id":"schema:Text"},"schema:domainIncludes":[{"@id":"unece:SpecifiedMethod"},{"@id":"unece:LaboratoryObservationAnalysisMethod"}],"rdfs:comment":"The code specifying the local type for this method."},{"@id":"unece:measurementCode","@type":["rdf:Property","owl:DatatypeProperty"],"rdfs:label":"measurementCode","schema:rangeIncludes":{"@id":"schema:Text"},"schema:domainIncludes":{"@id":"unece:SpecifiedMethod"},"rdfs:comment":"The code specifying the measurement for this method."},{"@id":"unece:obligatoryTypeCode","@type":["rdf:Property","owl:DatatypeProperty"],"rdfs:label":"obligatoryTypeCode","schema:rangeIncludes":{"@id":"schema:Text"},"schema:domainIncludes":[{"@id":"unece:SpecifiedMethod"},{"@id":"unece:LaboratoryObservationAnalysisMethod"}],"rdfs:comment":"The code specifying the obligatory type for this method."},{"@id":"unece:standardTypeCode","@type":["rdf:Property","owl:DatatypeProperty"],"rdfs:label":"standardTypeCode","schema:rangeIncludes":{"@id":"schema:Text"},"schema:domainIncludes":[{"@id":"unece:SpecifiedMethod"},{"@id":"unece:LaboratoryObservationAnalysisMethod"}],"rdfs:comment":"The code specifying the standard type for this method."},{"@id":"unece:usedTechnologyCode","@type":["rdf:Property","owl:DatatypeProperty"],"rdfs:label":"usedTechnologyCode","schema:rangeIncludes":{"@id":"schema:Text"},"schema:domainIncludes":{"@id":"unece:SpecifiedMethod"},"rdfs:comment":"The code specifying the technology used by this method."},{"@id":"unece:applicableRadioactiveIsotope","@type":["rdf:Property","owl:ObjectProperty"],"rdfs:label":"applicableRadioactiveIsotope","schema:rangeIncludes":{"@id":"unece:RadioactiveIsotope"},"schema:domainIncludes":{"@id":"unece:RadioactiveMaterial"},"rdfs:comment":"An isotope applicable to this radioactive material."},{"@id":"unece:compositionDescription","@type":["rdf:Property","owl:DatatypeProperty"],"rdfs:label":"compositionDescription","schema:rangeIncludes":{"@id":"schema:Text"},"schema:domainIncludes":{"@id":"unece:RadioactiveMaterial"},"rdfs:comment":"The textual description of the composition of this radioactive material."},{"@id":"unece:criticalitySafetyIndexNumeric","@type":["rdf:Property","owl:DatatypeProperty"],"rdfs:label":"criticalitySafetyIndexNumeric","schema:rangeIncludes":{"@id":"schema:Text"},"schema:domainIncludes":{"@id":"unece:RadioactiveMaterial"},"rdfs:comment":"The criticality safety index number of this radioactive material."},{"@id":"unece:fissileCriticalitySafetyIndexNumeric","@type":["rdf:Property","owl:DatatypeProperty"],"rdfs:label":"fissileCriticalitySafetyIndexNumeric","schema:rangeIncludes":{"@id":"schema:Text"},"schema:domainIncludes":{"@id":"unece:RadioactiveMaterial"},"rdfs:comment":"The number (rounded up to the next tenth) assigned to and placed on the label of a fissile radioactive material package, to designate the degree of control of accumulation of packages, overpacks or freight containers containing fissile material during transportation."},{"@id":"unece:fissileExceptionIndicator","@type":["rdf:Property","owl:DatatypeProperty"],"rdfs:label":"fissileExceptionIndicator","schema:rangeIncludes":{"@id":"schema:Boolean"},"schema:domainIncludes":{"@id":"unece:RadioactiveMaterial"},"rdfs:comment":"The indication of whether or not this radioactive material is a fissile exception."},{"@id":"unece:lowDispersibleInformation","@type":["rdf:Property","owl:DatatypeProperty"],"rdfs:label":"lowDispersibleInformation","schema:rangeIncludes":{"@id":"schema:Text"},"schema:domainIncludes":{"@id":"unece:RadioactiveMaterial"},"rdfs:comment":"Information, expressed as text, describing the low dispersion properties of this radioactive material."},{"@id":"unece:radioactivePackageTransportIndexCode","@type":["rdf:Property","owl:DatatypeProperty"],"rdfs:label":"radioactivePackageTransportIndexCode","schema:rangeIncludes":{"@id":"schema:Text"},"schema:domainIncludes":{"@id":"unece:RadioactiveMaterial"},"rdfs:comment":"A code specifying a package transport index for this radioactive material."},{"@id":"unece:radionuclideName","@type":["rdf:Property","owl:DatatypeProperty"],"rdfs:label":"radionuclideName","schema:rangeIncludes":{"@id":"schema:Text"},"schema:domainIncludes":{"@id":"unece:RadioactiveMaterial"},"rdfs:comment":"The name of the radionuclide, expressed as text, of this radioactive material."},{"@id":"unece:specialFormInformation","@type":["rdf:Property","owl:DatatypeProperty"],"rdfs:label":"specialFormInformation","schema:rangeIncludes":{"@id":"schema:Text"},"schema:domainIncludes":{"@id":"unece:RadioactiveMaterial"},"rdfs:comment":"Information, expressed as text, describing the special form for this radioactive material."},{"@id":"unece:transportIndexNumeric","@type":["rdf:Property","owl:DatatypeProperty"],"rdfs:label":"transportIndexNumeric","schema:rangeIncludes":{"@id":"schema:Text"},"schema:domainIncludes":{"@id":"unece:RadioactiveMaterial"},"rdfs:comment":"The transport index number of this radioactive material."},{"@id":"unece:associatedGeographicalFeature","@type":["rdf:Property","owl:ObjectProperty"],"rdfs:label":"associatedGeographicalFeature","schema:rangeIncludes":{"@id":"unece:GeographicalFeature"},"schema:domainIncludes":[{"@id":"unece:Location"},{"@id":"unece:CommunicationEvent"}],"rdfs:comment":"A geographical feature associated with this communication event."},{"@id":"unece:countryName","@type":["rdf:Property","owl:DatatypeProperty"],"rdfs:label":"countryName","schema:rangeIncludes":{"@id":"schema:Text"},"schema:domainIncludes":[{"@id":"unece:Location"},{"@id":"unece:Address"}],"rdfs:comment":"A name, expressed as text, of the country for this trade address."},{"@id":"unece:countrySubDivisionId","@type":["rdf:Property","owl:DatatypeProperty"],"rdfs:label":"countrySubDivisionId","schema:rangeIncludes":{"@id":"schema:Text"},"schema:domainIncludes":[{"@id":"unece:Location"},{"@id":"unece:Address"},{"@id":"unece:GovernmentRegistration"}],"rdfs:comment":"A unique identifier of the country sub-division for this trade address."},{"@id":"unece:locationCountryId","@type":["rdf:Property","owl:DatatypeProperty"],"rdfs:label":"locationCountryId","schema:rangeIncludes":{"@id":"unece:CountryId"},"schema:domainIncludes":{"@id":"unece:Location"},"rdfs:comment":"The identifier of the country for this referenced location."},{"@id":"unece:locationTypeCode","@type":["rdf:Property","owl:DatatypeProperty"],"rdfs:label":"locationTypeCode","schema:rangeIncludes":{"@id":"schema:Text"},"schema:domainIncludes":{"@id":"unece:Location"},"rdfs:comment":"The code specifying the type of referenced location."},{"@id":"unece:postalAddress","@type":["rdf:Property","owl:ObjectProperty"],"rdfs:label":"postalAddress","schema:rangeIncludes":{"@id":"unece:Address"},"schema:domainIncludes":[{"@id":"unece:Location"},{"@id":"unece:LegalOrganization"},{"@id":"unece:LaboratoryObservationParty"}],"rdfs:comment":"A postal address for this legally set up organization."},{"@id":"unece:specifiedSupplyChainEvent","@type":["rdf:Property","owl:ObjectProperty"],"rdfs:label":"specifiedSupplyChainEvent","schema:rangeIncludes":{"@id":"unece:Event"},"schema:domainIncludes":[{"@id":"unece:Location"},{"@id":"unece:SustainabilityCharacteristic"},{"@id":"unece:TechnicalCharacteristic"}],"rdfs:comment":"A supply chain event specified for this product batch."},{"@id":"unece:specifiedTradeParty","@type":["rdf:Property","owl:ObjectProperty"],"rdfs:label":"specifiedTradeParty","schema:rangeIncludes":{"@id":"unece:Party"},"schema:domainIncludes":{"@id":"unece:Location"},"rdfs:comment":"A party specified for this experience event."},{"@id":"unece:uTCOffsetNumeric","@type":["rdf:Property","owl:DatatypeProperty"],"rdfs:label":"uTCOffsetNumeric","schema:rangeIncludes":{"@id":"schema:Text"},"schema:domainIncludes":{"@id":"unece:Location"},"rdfs:comment":"The UTC (Universal Time Coordinate) time offset value for this referenced location."},{"@id":"unece:applicationSpecifiedParameter","@type":["rdf:Property","owl:ObjectProperty"],"rdfs:label":"applicationSpecifiedParameter","schema:rangeIncludes":{"@id":"unece:DocumentContextParameter"},"schema:domainIncludes":{"@id":"unece:ExchangedDocumentContext"},"rdfs:comment":"An application context parameter specified for this exchanged document context."},{"@id":"unece:bIMSpecifiedParameter","@type":["rdf:Property","owl:ObjectProperty"],"rdfs:label":"bIMSpecifiedParameter","schema:rangeIncludes":{"@id":"unece:DocumentContextParameter"},"schema:domainIncludes":{"@id":"unece:ExchangedDocumentContext"},"rdfs:comment":"A Business Information Master (BIM) context parameter specified for this exchanged document context."},{"@id":"unece:businessProcessSpecifiedParameter","@type":["rdf:Property","owl:ObjectProperty"],"rdfs:label":"businessProcessSpecifiedParameter","schema:rangeIncludes":{"@id":"unece:DocumentContextParameter"},"schema:domainIncludes":{"@id":"unece:ExchangedDocumentContext"},"rdfs:comment":"A business process context parameter specified for this exchanged document context."},{"@id":"unece:guidelineSpecifiedParameter","@type":["rdf:Property","owl:ObjectProperty"],"rdfs:label":"guidelineSpecifiedParameter","schema:rangeIncludes":{"@id":"unece:DocumentContextParameter"},"schema:domainIncludes":{"@id":"unece:ExchangedDocumentContext"},"rdfs:comment":"A guideline context parameter specified for this exchanged document context."},{"@id":"unece:messageStandardSpecifiedParameter","@type":["rdf:Property","owl:ObjectProperty"],"rdfs:label":"messageStandardSpecifiedParameter","schema:rangeIncludes":{"@id":"unece:DocumentContextParameter"},"schema:domainIncludes":{"@id":"unece:ExchangedDocumentContext"},"rdfs:comment":"The message standard document context parameter specified for this exchanged document context."},{"@id":"unece:processingTransactionDateTime","@type":["rdf:Property","owl:DatatypeProperty"],"rdfs:label":"processingTransactionDateTime","schema:rangeIncludes":{"@id":"schema:Text"},"schema:domainIncludes":{"@id":"unece:ExchangedDocumentContext"},"rdfs:comment":"The date, time, date time, or other date time value of the processing of a transaction for this exchanged document context."},{"@id":"unece:scenarioSpecifiedParameter","@type":["rdf:Property","owl:ObjectProperty"],"rdfs:label":"scenarioSpecifiedParameter","schema:rangeIncludes":{"@id":"unece:DocumentContextParameter"},"schema:domainIncludes":{"@id":"unece:ExchangedDocumentContext"},"rdfs:comment":"A scenario context parameter specified for this exchanged document context."},{"@id":"unece:specifiedTransactionId","@type":["rdf:Property","owl:DatatypeProperty"],"rdfs:label":"specifiedTransactionId","schema:rangeIncludes":{"@id":"schema:Text"},"schema:domainIncludes":{"@id":"unece:ExchangedDocumentContext"},"rdfs:comment":"The identifier of a specified transaction in this exchanged document context."},{"@id":"unece:subsetSpecifiedParameter","@type":["rdf:Property","owl:ObjectProperty"],"rdfs:label":"subsetSpecifiedParameter","schema:rangeIncludes":{"@id":"unece:DocumentContextParameter"},"schema:domainIncludes":{"@id":"unece:ExchangedDocumentContext"},"rdfs:comment":"A subset context parameter specified for this exchanged document context."},{"@id":"unece:testIndicator","@type":["rdf:Property","owl:DatatypeProperty"],"rdfs:label":"testIndicator","schema:rangeIncludes":{"@id":"schema:Boolean"},"schema:domainIncludes":{"@id":"unece:ExchangedDocumentContext"},"rdfs:comment":"The indication of whether or not this XHE document is a test ."},{"@id":"unece:userSpecifiedParameter","@type":["rdf:Property","owl:ObjectProperty"],"rdfs:label":"userSpecifiedParameter","schema:rangeIncludes":{"@id":"unece:DocumentContextParameter"},"schema:domainIncludes":{"@id":"unece:ExchangedDocumentContext"},"rdfs:comment":"A user specified document context parameter specified for this exchanged document context."},{"@id":"unece:associatedDirectPositionList","@type":["rdf:Property","owl:ObjectProperty"],"rdfs:label":"associatedDirectPositionList","schema:rangeIncludes":{"@id":"unece:DirectPositionList"},"schema:domainIncludes":[{"@id":"unece:GeographicalLine"},{"@id":"unece:GeographicalMultiCurve"},{"@id":"unece:GeographicalMultiPoint"},{"@id":"unece:GeographicalPoint"}],"rdfs:comment":"The direct position list associated with this geographical line."},{"@id":"unece:associatedGeographicalObjectCharacteristic","@type":["rdf:Property","owl:ObjectProperty"],"rdfs:label":"associatedGeographicalObjectCharacteristic","schema:rangeIncludes":{"@id":"unece:GeographicalObjectCharacteristic"},"schema:domainIncludes":[{"@id":"unece:GeographicalLine"},{"@id":"unece:GeographicalMultiCurve"},{"@id":"unece:GeographicalMultiPoint"},{"@id":"unece:GeographicalPoint"},{"@id":"unece:Circle"},{"@id":"unece:GeographicalGrid"},{"@id":"unece:GeographicalMultiSurface"},{"@id":"unece:GeographicalSurface"},{"@id":"unece:LinearRing"},{"@id":"unece:Polygon"}],"rdfs:comment":"The geographical object characteristic associated with this geographical grid."},{"@id":"unece:associatedLocation","@type":["rdf:Property","owl:ObjectProperty"],"rdfs:label":"associatedLocation","schema:rangeIncludes":{"@id":"unece:Location"},"schema:domainIncludes":[{"@id":"unece:GeographicalLine"},{"@id":"unece:GeographicalPoint"},{"@id":"unece:Circle"},{"@id":"unece:GeographicalGrid"},{"@id":"unece:Polygon"}],"rdfs:comment":"A logistics location associated with this specified circle."},{"@id":"unece:memberGeographicalLine","@type":["rdf:Property","owl:ObjectProperty"],"rdfs:label":"memberGeographicalLine","schema:rangeIncludes":{"@id":"unece:GeographicalLine"},"schema:domainIncludes":{"@id":"unece:GeographicalMultiCurve"},"rdfs:comment":"A geographical line member of this geographical multi-curve."},{"@id":"unece:memberGeographicalPoint","@type":["rdf:Property","owl:ObjectProperty"],"rdfs:label":"memberGeographicalPoint","schema:rangeIncludes":{"@id":"unece:GeographicalPoint"},"schema:domainIncludes":{"@id":"unece:GeographicalMultiPoint"},"rdfs:comment":"A geographical point member of this geographical multi-point feature."},{"@id":"unece:associatedEvent","@type":["rdf:Property","owl:ObjectProperty"],"rdfs:label":"associatedEvent","schema:rangeIncludes":{"@id":"unece:Event"},"schema:domainIncludes":{"@id":"unece:Error"},"rdfs:comment":"A corrective event associated with this declared error."},{"@id":"unece:occurrenceLogisticsLocation","@type":["rdf:Property","owl:ObjectProperty"],"rdfs:label":"occurrenceLogisticsLocation","schema:rangeIncludes":{"@id":"unece:Location"},"schema:domainIncludes":{"@id":"unece:CommunicationEvent"},"rdfs:comment":"A logistics location where this supply chain event occurs."},{"@id":"unece:operationalResponsibleParty","@type":["rdf:Property","owl:ObjectProperty"],"rdfs:label":"operationalResponsibleParty","schema:rangeIncludes":{"@id":"unece:Party"},"schema:domainIncludes":{"@id":"unece:CommunicationEvent"},"rdfs:comment":"The operational responsible party for this communication event."},{"@id":"unece:centreGeographicalPoint","@type":["rdf:Property","owl:ObjectProperty"],"rdfs:label":"centreGeographicalPoint","schema:rangeIncludes":{"@id":"unece:GeographicalPoint"},"schema:domainIncludes":{"@id":"unece:Circle"},"rdfs:comment":"The geographical point which defines the centre of this specified circle."},{"@id":"unece:radiusMeasure","@type":["rdf:Property","owl:ObjectProperty"],"rdfs:label":"radiusMeasure","schema:rangeIncludes":{"@id":"unece:MeasureType"},"schema:domainIncludes":{"@id":"unece:Circle"},"rdfs:comment":"The measure of the radius for this specified circle."},{"@id":"unece:axisName","@type":["rdf:Property","owl:DatatypeProperty"],"rdfs:label":"axisName","schema:rangeIncludes":{"@id":"schema:Text"},"schema:domainIncludes":{"@id":"unece:GeographicalGrid"},"rdfs:comment":"An axis name, expressed as text, for this geographical grid."},{"@id":"unece:cell","@type":["rdf:Property","owl:DatatypeProperty"],"rdfs:label":"cell","schema:rangeIncludes":{"@id":"schema:Text"},"schema:domainIncludes":{"@id":"unece:GeographicalGrid"},"rdfs:comment":"The cell value, expressed as text, for this geographical grid."},{"@id":"unece:dimensionNumeric","@type":["rdf:Property","owl:DatatypeProperty"],"rdfs:label":"dimensionNumeric","schema:rangeIncludes":{"@id":"schema:Text"},"schema:domainIncludes":{"@id":"unece:GeographicalGrid"},"rdfs:comment":"The dimension, expressed as a number, of this geographical grid."},{"@id":"unece:highLimit","@type":["rdf:Property","owl:DatatypeProperty"],"rdfs:label":"highLimit","schema:rangeIncludes":{"@id":"schema:Text"},"schema:domainIncludes":{"@id":"unece:GeographicalGrid"},"rdfs:comment":"The tuple of elements, expressed as text, indicating the high limit of this geographical grid specifying the diagonally opposing corner of each axis."},{"@id":"unece:lowLimit","@type":["rdf:Property","owl:DatatypeProperty"],"rdfs:label":"lowLimit","schema:rangeIncludes":{"@id":"schema:Text"},"schema:domainIncludes":{"@id":"unece:GeographicalGrid"},"rdfs:comment":"The tuple of elements, expressed as text, indicating the low limit of this geographical grid specifying the offset of each axis."},{"@id":"unece:offsetVectorNumeric","@type":["rdf:Property","owl:DatatypeProperty"],"rdfs:label":"offsetVectorNumeric","schema:rangeIncludes":{"@id":"schema:Text"},"schema:domainIncludes":{"@id":"unece:GeographicalGrid"},"rdfs:comment":"The offset vector, expressed as a number, which indicates the offset of cells along each axis for this geographical grid."},{"@id":"unece:originAssociatedDirectPositionList","@type":["rdf:Property","owl:ObjectProperty"],"rdfs:label":"originAssociatedDirectPositionList","schema:rangeIncludes":{"@id":"unece:DirectPositionList"},"schema:domainIncludes":{"@id":"unece:GeographicalGrid"},"rdfs:comment":"The direct position list associated with the origin of this geographical grid."},{"@id":"unece:includedPolygon","@type":["rdf:Property","owl:ObjectProperty"],"rdfs:label":"includedPolygon","schema:rangeIncludes":{"@id":"unece:Polygon"},"schema:domainIncludes":[{"@id":"unece:GeographicalMultiSurface"},{"@id":"unece:GeographicalSurface"},{"@id":"unece:GeographicalFeature"}],"rdfs:comment":"A polygon included in this geographical multi-surface."},{"@id":"unece:coordinate","@type":["rdf:Property","owl:DatatypeProperty"],"rdfs:label":"coordinate","schema:rangeIncludes":{"@id":"schema:Text"},"schema:domainIncludes":[{"@id":"unece:LinearRing"},{"@id":"unece:DirectPositionList"}],"rdfs:comment":"A coordinate, expressed as text, for this specified linear ring."},{"@id":"unece:coordinateDirectPosition","@type":["rdf:Property","owl:ObjectProperty"],"rdfs:label":"coordinateDirectPosition","schema:rangeIncludes":{"@id":"unece:DirectPosition"},"schema:domainIncludes":{"@id":"unece:LinearRing"},"rdfs:comment":"The specified direct position of a coordinate for this linear ring."},{"@id":"unece:exteriorLinearRing","@type":["rdf:Property","owl:ObjectProperty"],"rdfs:label":"exteriorLinearRing","schema:rangeIncludes":{"@id":"unece:LinearRing"},"schema:domainIncludes":{"@id":"unece:Polygon"},"rdfs:comment":"The exterior linear specified ring for this polygon."},{"@id":"unece:interiorLinearRing","@type":["rdf:Property","owl:ObjectProperty"],"rdfs:label":"interiorLinearRing","schema:rangeIncludes":{"@id":"unece:LinearRing"},"schema:domainIncludes":{"@id":"unece:Polygon"},"rdfs:comment":"An interior linear ring specified for this polygon."},{"@id":"unece:authorizedRegistration","@type":["rdf:Property","owl:ObjectProperty"],"rdfs:label":"authorizedRegistration","schema:rangeIncludes":{"@id":"unece:LegalRegistration"},"schema:domainIncludes":{"@id":"unece:LegalOrganization"},"rdfs:comment":"A legal registration authorized for this legally set up organization."},{"@id":"unece:businessTypeCode","@type":["rdf:Property","owl:DatatypeProperty"],"rdfs:label":"businessTypeCode","schema:rangeIncludes":{"@id":"schema:Text"},"schema:domainIncludes":{"@id":"unece:LegalOrganization"},"rdfs:comment":"A code specifying the type of business of this legally set up organization."},{"@id":"unece:establishedDateTime","@type":["rdf:Property","owl:DatatypeProperty"],"rdfs:label":"establishedDateTime","schema:rangeIncludes":{"@id":"schema:Text"},"schema:domainIncludes":{"@id":"unece:LegalOrganization"},"rdfs:comment":"The date, time, date time, or other date time value when this legally set up organization was established."},{"@id":"unece:legalClassificationCode","@type":["rdf:Property","owl:DatatypeProperty"],"rdfs:label":"legalClassificationCode","schema:rangeIncludes":{"@id":"schema:Text"},"schema:domainIncludes":{"@id":"unece:LegalOrganization"},"rdfs:comment":"The code specifying the legal classification of this organization, such as Incorporated (Inc), Limited Liability Corporation (LLC) or non-profit."},{"@id":"unece:tradingBusinessName","@type":["rdf:Property","owl:DatatypeProperty"],"rdfs:label":"tradingBusinessName","schema:rangeIncludes":{"@id":"schema:Text"},"schema:domainIncludes":{"@id":"unece:LegalOrganization"},"rdfs:comment":"The trading business name, expressed as text, of this legally set up organization."},{"@id":"unece:axisLabelList","@type":["rdf:Property","owl:DatatypeProperty"],"rdfs:label":"axisLabelList","schema:rangeIncludes":{"@id":"schema:Text"},"schema:domainIncludes":[{"@id":"unece:DirectPosition"},{"@id":"unece:DirectPositionList"}],"rdfs:comment":"An ordered list of axis labels, expressed as text, for this specified direct position list."},{"@id":"unece:coordinateReferenceDimension","@type":["rdf:Property","owl:DatatypeProperty"],"rdfs:label":"coordinateReferenceDimension","schema:rangeIncludes":{"@id":"schema:Text"},"schema:domainIncludes":[{"@id":"unece:DirectPosition"},{"@id":"unece:DirectPositionList"}],"rdfs:comment":"A coordinate reference dimension, expressed as text, for this specified direct position list."},{"@id":"unece:countNumeric","@type":["rdf:Property","owl:DatatypeProperty"],"rdfs:label":"countNumeric","schema:rangeIncludes":{"@id":"schema:Text"},"schema:domainIncludes":[{"@id":"unece:DirectPosition"},{"@id":"unece:DirectPositionList"}],"rdfs:comment":"A count for this specified direct position list."},{"@id":"unece:uOMLabelList","@type":["rdf:Property","owl:DatatypeProperty"],"rdfs:label":"uOMLabelList","schema:rangeIncludes":{"@id":"schema:Text"},"schema:domainIncludes":[{"@id":"unece:DirectPosition"},{"@id":"unece:DirectPositionList"}],"rdfs:comment":"An ordered list of Unit Of Measure (UOM) labels, expressed as text, for this specified direct position list."},{"@id":"unece:birthAddressCountryId","@type":["rdf:Property","owl:DatatypeProperty"],"rdfs:label":"birthAddressCountryId","schema:rangeIncludes":{"@id":"unece:CountryId"},"schema:domainIncludes":{"@id":"unece:BirthAddress"},"rdfs:comment":"The identifier of a country for this birth address."},{"@id":"unece:cityName","@type":["rdf:Property","owl:DatatypeProperty"],"rdfs:label":"cityName","schema:rangeIncludes":{"@id":"schema:Text"},"schema:domainIncludes":[{"@id":"unece:BirthAddress"},{"@id":"unece:Address"}],"rdfs:comment":"The name, expressed as text, of the city, town or village of this birth address."},{"@id":"unece:countrySubDivisionName","@type":["rdf:Property","owl:DatatypeProperty"],"rdfs:label":"countrySubDivisionName","schema:rangeIncludes":{"@id":"schema:Text"},"schema:domainIncludes":[{"@id":"unece:BirthAddress"},{"@id":"unece:Address"}],"rdfs:comment":"A name, expressed as text, of the sub-division of a country for this trade address."},{"@id":"unece:cancellationDocumentStatusConditionCode","@type":["rdf:Property","owl:DatatypeProperty"],"rdfs:label":"cancellationDocumentStatusConditionCode","schema:rangeIncludes":{"@id":"schema:Text"},"schema:domainIncludes":{"@id":"unece:CancellationStatus"},"rdfs:comment":"The code specifying the condition of this cancellation status."},{"@id":"unece:reasonInformation","@type":["rdf:Property","owl:DatatypeProperty"],"rdfs:label":"reasonInformation","schema:rangeIncludes":{"@id":"schema:Text"},"schema:domainIncludes":[{"@id":"unece:CancellationStatus"},{"@id":"unece:DocumentStatus"}],"rdfs:comment":"Information, expressed as text, related to the reason for this cancellation status."},{"@id":"unece:category","@type":["rdf:Property","owl:DatatypeProperty"],"rdfs:label":"category","schema:rangeIncludes":{"@id":"schema:Text"},"schema:domainIncludes":{"@id":"unece:Object"},"rdfs:comment":"A category, expressed as text, for this specified object."},{"@id":"unece:objectType","@type":["rdf:Property","owl:DatatypeProperty"],"rdfs:label":"objectType","schema:rangeIncludes":{"@id":"schema:Text"},"schema:domainIncludes":{"@id":"unece:Object"},"rdfs:comment":"A type, expressed as text, for this specified object."},{"@id":"unece:remark","@type":["rdf:Property","owl:DatatypeProperty"],"rdfs:label":"remark","schema:rangeIncludes":{"@id":"schema:Text"},"schema:domainIncludes":[{"@id":"unece:Object"},{"@id":"unece:RegulatoryProcedure"}],"rdfs:comment":"A remark, expressed as text, for this cross-border regulatory procedure."},{"@id":"unece:categoryName","@type":["rdf:Property","owl:DatatypeProperty"],"rdfs:label":"categoryName","schema:rangeIncludes":{"@id":"schema:Text"},"schema:domainIncludes":{"@id":"unece:CustomerClass"},"rdfs:comment":"A category name, expressed as text, of this specified customer class."},{"@id":"unece:genderCode","@type":["rdf:Property","owl:DatatypeProperty"],"rdfs:label":"genderCode","schema:rangeIncludes":{"@id":"schema:Text"},"schema:domainIncludes":[{"@id":"unece:CustomerClass"},{"@id":"unece:Person"}],"rdfs:comment":"A code specifying the gender of this transport person."},{"@id":"unece:lowerAgeLimitNumeric","@type":["rdf:Property","owl:DatatypeProperty"],"rdfs:label":"lowerAgeLimitNumeric","schema:rangeIncludes":{"@id":"schema:Text"},"schema:domainIncludes":{"@id":"unece:CustomerClass"},"rdfs:comment":"The value, expressed as a number of years, for the lower age limit for the category of this specified customer class."},{"@id":"unece:mealServiceCategoryCode","@type":["rdf:Property","owl:DatatypeProperty"],"rdfs:label":"mealServiceCategoryCode","schema:rangeIncludes":{"@id":"schema:Text"},"schema:domainIncludes":{"@id":"unece:CustomerClass"},"rdfs:comment":"The code specifying the meal service category for this specified customer class."},{"@id":"unece:specialBeddingServiceOfferedIndicator","@type":["rdf:Property","owl:DatatypeProperty"],"rdfs:label":"specialBeddingServiceOfferedIndicator","schema:rangeIncludes":{"@id":"schema:Boolean"},"schema:domainIncludes":{"@id":"unece:CustomerClass"},"rdfs:comment":"The indication of whether or not special bedding service is offered for this specified customer class."},{"@id":"unece:upperAgeLimitNumeric","@type":["rdf:Property","owl:DatatypeProperty"],"rdfs:label":"upperAgeLimitNumeric","schema:rangeIncludes":{"@id":"schema:Text"},"schema:domainIncludes":{"@id":"unece:CustomerClass"},"rdfs:comment":"The value, expressed as a number of years, for the upper age limit for the category of this specified customer class."},{"@id":"unece:securityInformation","@type":["rdf:Property","owl:DatatypeProperty"],"rdfs:label":"securityInformation","schema:rangeIncludes":{"@id":"schema:Text"},"schema:domainIncludes":{"@id":"unece:InformationSource"},"rdfs:comment":"Security information, expressed as text, of this specified information source."},{"@id":"unece:websiteURIId","@type":["rdf:Property","owl:DatatypeProperty"],"rdfs:label":"websiteURIId","schema:rangeIncludes":{"@id":"schema:Text"},"schema:domainIncludes":[{"@id":"unece:InformationSource"},{"@id":"unece:Communication"}],"rdfs:comment":"A website Uniform Resource Identifier (URI) for this specified marketplace."},{"@id":"unece:changedDateTime","@type":["rdf:Property","owl:DatatypeProperty"],"rdfs:label":"changedDateTime","schema:rangeIncludes":{"@id":"schema:Text"},"schema:domainIncludes":{"@id":"unece:RecordedStatus"},"rdfs:comment":"The date, time, date time, or other date time value when this recorded status changed."},{"@id":"unece:changerName","@type":["rdf:Property","owl:DatatypeProperty"],"rdfs:label":"changerName","schema:rangeIncludes":{"@id":"schema:Text"},"schema:domainIncludes":{"@id":"unece:RecordedStatus"},"rdfs:comment":"The name of the person or system, expressed as text, that changed this recorded status."},{"@id":"unece:recordedStatusConditionCode","@type":["rdf:Property","owl:DatatypeProperty"],"rdfs:label":"recordedStatusConditionCode","schema:rangeIncludes":{"@id":"schema:Text"},"schema:domainIncludes":{"@id":"unece:RecordedStatus"},"rdfs:comment":"The code specifying the condition for this recorded status."},{"@id":"unece:collectionIndicator","@type":["rdf:Property","owl:DatatypeProperty"],"rdfs:label":"collectionIndicator","schema:rangeIncludes":{"@id":"schema:Boolean"},"schema:domainIncludes":{"@id":"unece:GeographicalFeature"},"rdfs:comment":"The indication of whether or not this specified geographical feature is a collection of features."},{"@id":"unece:coordinateReferenceSystemId","@type":["rdf:Property","owl:DatatypeProperty"],"rdfs:label":"coordinateReferenceSystemId","schema:rangeIncludes":{"@id":"schema:Text"},"schema:domainIncludes":{"@id":"unece:GeographicalFeature"},"rdfs:comment":"The identifier of the coordinate reference system for this geographical feature."},{"@id":"unece:includedCircle","@type":["rdf:Property","owl:ObjectProperty"],"rdfs:label":"includedCircle","schema:rangeIncludes":{"@id":"unece:Circle"},"schema:domainIncludes":{"@id":"unece:GeographicalFeature"},"rdfs:comment":"A circle included in this specified geographical feature."},{"@id":"unece:includedGeographicalGrid","@type":["rdf:Property","owl:ObjectProperty"],"rdfs:label":"includedGeographicalGrid","schema:rangeIncludes":{"@id":"unece:GeographicalGrid"},"schema:domainIncludes":{"@id":"unece:GeographicalFeature"},"rdfs:comment":"The geographical grid included in this geographical feature."},{"@id":"unece:includedGeographicalLine","@type":["rdf:Property","owl:ObjectProperty"],"rdfs:label":"includedGeographicalLine","schema:rangeIncludes":{"@id":"unece:GeographicalLine"},"schema:domainIncludes":{"@id":"unece:GeographicalFeature"},"rdfs:comment":"The geographical line included in this geographical feature."},{"@id":"unece:includedGeographicalMultiCurve","@type":["rdf:Property","owl:ObjectProperty"],"rdfs:label":"includedGeographicalMultiCurve","schema:rangeIncludes":{"@id":"unece:GeographicalMultiCurve"},"schema:domainIncludes":{"@id":"unece:GeographicalFeature"},"rdfs:comment":"The geographical multi-curve included in this geographical feature."},{"@id":"unece:includedGeographicalMultiPoint","@type":["rdf:Property","owl:ObjectProperty"],"rdfs:label":"includedGeographicalMultiPoint","schema:rangeIncludes":{"@id":"unece:GeographicalMultiPoint"},"schema:domainIncludes":{"@id":"unece:GeographicalFeature"},"rdfs:comment":"The geographical multi-point included in this geographical feature."},{"@id":"unece:includedGeographicalMultiSurface","@type":["rdf:Property","owl:ObjectProperty"],"rdfs:label":"includedGeographicalMultiSurface","schema:rangeIncludes":{"@id":"unece:GeographicalMultiSurface"},"schema:domainIncludes":{"@id":"unece:GeographicalFeature"},"rdfs:comment":"The geographical multi-surface included in this geographical feature."},{"@id":"unece:includedGeographicalPoint","@type":["rdf:Property","owl:ObjectProperty"],"rdfs:label":"includedGeographicalPoint","schema:rangeIncludes":{"@id":"unece:GeographicalPoint"},"schema:domainIncludes":{"@id":"unece:GeographicalFeature"},"rdfs:comment":"The geographical point included in this geographical feature."},{"@id":"unece:includedGeographicalSurface","@type":["rdf:Property","owl:ObjectProperty"],"rdfs:label":"includedGeographicalSurface","schema:rangeIncludes":{"@id":"unece:GeographicalSurface"},"schema:domainIncludes":{"@id":"unece:GeographicalFeature"},"rdfs:comment":"The geographical surface included in this geographical feature."},{"@id":"unece:communicationChannelCode","@type":["rdf:Property","owl:DatatypeProperty"],"rdfs:label":"communicationChannelCode","schema:rangeIncludes":{"@id":"unece:CommunicationChannelCodeList"},"schema:domainIncludes":{"@id":"unece:Communication"},"rdfs:comment":"The code specifying the channel or manner in which a universal communication can be made, such as telephone or email."},{"@id":"unece:completeNumber","@type":["rdf:Property","owl:DatatypeProperty"],"rdfs:label":"completeNumber","schema:rangeIncludes":{"@id":"schema:Text"},"schema:domainIncludes":{"@id":"unece:Communication"},"rdfs:comment":"The text string of characters that make up the complete number for this universal communication."},{"@id":"unece:emailURIId","@type":["rdf:Property","owl:DatatypeProperty"],"rdfs:label":"emailURIId","schema:rangeIncludes":{"@id":"schema:Text"},"schema:domainIncludes":{"@id":"unece:Communication"},"rdfs:comment":"The Uniform Resource Identifier (URI) of the email for this universal communication."},{"@id":"unece:invalidIndicator","@type":["rdf:Property","owl:DatatypeProperty"],"rdfs:label":"invalidIndicator","schema:rangeIncludes":{"@id":"schema:Boolean"},"schema:domainIncludes":[{"@id":"unece:Communication"},{"@id":"unece:Address"}],"rdfs:comment":"The indication of whether or not this trade address is invalid."},{"@id":"unece:completeDateTime","@type":["rdf:Property","owl:DatatypeProperty"],"rdfs:label":"completeDateTime","schema:rangeIncludes":{"@id":"schema:Text"},"schema:domainIncludes":{"@id":"unece:SpecifiedPeriod"},"rdfs:comment":"The date, time, date time or other date time value for a complete specified period of time expressed as a specific month, a specific week, etc."},{"@id":"unece:continuousIndicator","@type":["rdf:Property","owl:DatatypeProperty"],"rdfs:label":"continuousIndicator","schema:rangeIncludes":{"@id":"schema:Boolean"},"schema:domainIncludes":{"@id":"unece:SpecifiedPeriod"},"rdfs:comment":"The indication of whether or not this specified period is continuous."},{"@id":"unece:dayQuantity","@type":["rdf:Property","owl:ObjectProperty"],"rdfs:label":"dayQuantity","schema:rangeIncludes":{"@id":"unece:QuantityType"},"schema:domainIncludes":{"@id":"unece:SpecifiedPeriod"},"rdfs:comment":"The number of days in this specified period."},{"@id":"unece:durationMeasure","@type":["rdf:Property","owl:ObjectProperty"],"rdfs:label":"durationMeasure","schema:rangeIncludes":{"@id":"unece:MeasureType"},"schema:domainIncludes":[{"@id":"unece:SpecifiedPeriod"},{"@id":"unece:DelimitedPeriod"}],"rdfs:comment":"A measure of the length of time for this specified time period such as hours, days, weeks, months, years."},{"@id":"unece:endDayOfWeekCode","@type":["rdf:Property","owl:DatatypeProperty"],"rdfs:label":"endDayOfWeekCode","schema:rangeIncludes":{"@id":"schema:Text"},"schema:domainIncludes":{"@id":"unece:SpecifiedPeriod"},"rdfs:comment":"The code specifying the end day of the week for this specified period."},{"@id":"unece:inclusiveIndicator","@type":["rdf:Property","owl:DatatypeProperty"],"rdfs:label":"inclusiveIndicator","schema:rangeIncludes":{"@id":"schema:Boolean"},"schema:domainIncludes":{"@id":"unece:SpecifiedPeriod"},"rdfs:comment":"The indication of whether or not the start and end dates are included in this specified period."},{"@id":"unece:maximumDurationMeasure","@type":["rdf:Property","owl:ObjectProperty"],"rdfs:label":"maximumDurationMeasure","schema:rangeIncludes":{"@id":"unece:DurationUnitMeasureType"},"schema:domainIncludes":{"@id":"unece:SpecifiedPeriod"},"rdfs:comment":"The measure of the maximum length of time for this specified period, such as hours, days, weeks, months, years."},{"@id":"unece:minimumDurationMeasure","@type":["rdf:Property","owl:ObjectProperty"],"rdfs:label":"minimumDurationMeasure","schema:rangeIncludes":{"@id":"unece:DurationUnitMeasureType"},"schema:domainIncludes":{"@id":"unece:SpecifiedPeriod"},"rdfs:comment":"The measure of the minimum length of time for this specified period, such as hours, days, weeks, months, years."},{"@id":"unece:nightQuantity","@type":["rdf:Property","owl:ObjectProperty"],"rdfs:label":"nightQuantity","schema:rangeIncludes":{"@id":"unece:QuantityType"},"schema:domainIncludes":{"@id":"unece:SpecifiedPeriod"},"rdfs:comment":"The number of nights in this specified period."},{"@id":"unece:openIndicator","@type":["rdf:Property","owl:DatatypeProperty"],"rdfs:label":"openIndicator","schema:rangeIncludes":{"@id":"schema:Boolean"},"schema:domainIncludes":{"@id":"unece:SpecifiedPeriod"},"rdfs:comment":"The indication of whether or not an entity is open during this specified period."},{"@id":"unece:seasonCode","@type":["rdf:Property","owl:DatatypeProperty"],"rdfs:label":"seasonCode","schema:rangeIncludes":{"@id":"schema:Text"},"schema:domainIncludes":{"@id":"unece:SpecifiedPeriod"},"rdfs:comment":"A code specifying a season for this trade product."},{"@id":"unece:sequenceNumeric","@type":["rdf:Property","owl:DatatypeProperty"],"rdfs:label":"sequenceNumeric","schema:rangeIncludes":{"@id":"schema:Text"},"schema:domainIncludes":[{"@id":"unece:SpecifiedPeriod"},{"@id":"unece:DocumentStatus"},{"@id":"unece:SpecifiedCertificate"},{"@id":"unece:InspectionInstructions"},{"@id":"unece:LaboratoryObservationInstructions"}],"rdfs:comment":"A sequence number for these specified personal effects."},{"@id":"unece:startDateFlexibilityCode","@type":["rdf:Property","owl:DatatypeProperty"],"rdfs:label":"startDateFlexibilityCode","schema:rangeIncludes":{"@id":"schema:Text"},"schema:domainIncludes":{"@id":"unece:SpecifiedPeriod"},"rdfs:comment":"The code specifying the flexibility of the start date of this specified period."},{"@id":"unece:startDayOfWeekCode","@type":["rdf:Property","owl:DatatypeProperty"],"rdfs:label":"startDayOfWeekCode","schema:rangeIncludes":{"@id":"schema:Text"},"schema:domainIncludes":{"@id":"unece:SpecifiedPeriod"},"rdfs:comment":"The code specifying the start day of the week for this specified period."},{"@id":"unece:componentDimension","@type":["rdf:Property","owl:ObjectProperty"],"rdfs:label":"componentDimension","schema:rangeIncludes":{"@id":"unece:WorkItemDimension"},"schema:domainIncludes":{"@id":"unece:WorkItemDimension"},"rdfs:comment":"A work item component dimension for this work item dimension."},{"@id":"unece:workItemDimensionTypeCode","@type":["rdf:Property","owl:DatatypeProperty"],"rdfs:label":"workItemDimensionTypeCode","schema:rangeIncludes":{"@id":"schema:Text"},"schema:domainIncludes":{"@id":"unece:WorkItemDimension"},"rdfs:comment":"The code specifying the type of this work item dimension."},{"@id":"unece:condition","@type":["rdf:Property","owl:DatatypeProperty"],"rdfs:label":"condition","schema:rangeIncludes":{"@id":"schema:Text"},"schema:domainIncludes":[{"@id":"unece:DocumentStatus"},{"@id":"unece:ProcessCharacteristic"},{"@id":"unece:OrganizationCharacteristic"}],"rdfs:comment":"A condition or status, expressed as text, for this process characteristic."},{"@id":"unece:documentStatusConditionCode","@type":["rdf:Property","owl:DatatypeProperty"],"rdfs:label":"documentStatusConditionCode","schema:rangeIncludes":{"@id":"unece:DocumentStatusCodeList"},"schema:domainIncludes":{"@id":"unece:DocumentStatus"},"rdfs:comment":"The code specifying the condition of this document status."},{"@id":"unece:documentStatusReasonCode","@type":["rdf:Property","owl:DatatypeProperty"],"rdfs:label":"documentStatusReasonCode","schema:rangeIncludes":{"@id":"schema:Text"},"schema:domainIncludes":{"@id":"unece:DocumentStatus"},"rdfs:comment":"A code specifying a reason for this document status."},{"@id":"unece:invalidInformation","@type":["rdf:Property","owl:DatatypeProperty"],"rdfs:label":"invalidInformation","schema:rangeIncludes":{"@id":"schema:Text"},"schema:domainIncludes":{"@id":"unece:DocumentStatus"},"rdfs:comment":"The invalid information, expressed as text, for this document status."},{"@id":"unece:reasonClassification","@type":["rdf:Property","owl:DatatypeProperty"],"rdfs:label":"reasonClassification","schema:rangeIncludes":{"@id":"schema:Text"},"schema:domainIncludes":{"@id":"unece:DocumentStatus"},"rdfs:comment":"A reason classification, expressed as text, for this document status."},{"@id":"unece:reasonClassificationCode","@type":["rdf:Property","owl:DatatypeProperty"],"rdfs:label":"reasonClassificationCode","schema:rangeIncludes":{"@id":"schema:Text"},"schema:domainIncludes":{"@id":"unece:DocumentStatus"},"rdfs:comment":"The code specifying the reason classification for this document status."},{"@id":"unece:reasonInformationCode","@type":["rdf:Property","owl:DatatypeProperty"],"rdfs:label":"reasonInformationCode","schema:rangeIncludes":{"@id":"schema:Text"},"schema:domainIncludes":{"@id":"unece:DocumentStatus"},"rdfs:comment":"The code specifying the reason for the information for this document status."},{"@id":"unece:requestedAction","@type":["rdf:Property","owl:DatatypeProperty"],"rdfs:label":"requestedAction","schema:rangeIncludes":{"@id":"schema:Text"},"schema:domainIncludes":{"@id":"unece:DocumentStatus"},"rdfs:comment":"A requested action, expressed as text, for this document status."},{"@id":"unece:requestedActionCode","@type":["rdf:Property","owl:DatatypeProperty"],"rdfs:label":"requestedActionCode","schema:rangeIncludes":{"@id":"schema:Text"},"schema:domainIncludes":{"@id":"unece:DocumentStatus"},"rdfs:comment":"A code specifying a requested action for this basic work item."},{"@id":"unece:specifiedDocumentCharacteristic","@type":["rdf:Property","owl:ObjectProperty"],"rdfs:label":"specifiedDocumentCharacteristic","schema:rangeIncludes":{"@id":"unece:DocumentCharacteristic"},"schema:domainIncludes":{"@id":"unece:DocumentStatus"},"rdfs:comment":"A document characteristic specified for this document status."},{"@id":"unece:validInformation","@type":["rdf:Property","owl:DatatypeProperty"],"rdfs:label":"validInformation","schema:rangeIncludes":{"@id":"schema:Text"},"schema:domainIncludes":{"@id":"unece:DocumentStatus"},"rdfs:comment":"The valid information, expressed as text, for this document status."},{"@id":"unece:constraintIndicator","@type":["rdf:Property","owl:DatatypeProperty"],"rdfs:label":"constraintIndicator","schema:rangeIncludes":{"@id":"schema:Boolean"},"schema:domainIncludes":{"@id":"unece:Project"},"rdfs:comment":"The indication of whether or not the project is constrained by an authority such as the World Trade Organization (WTO) for this procuring project."},{"@id":"unece:netBudgetAmount","@type":["rdf:Property","owl:ObjectProperty"],"rdfs:label":"netBudgetAmount","schema:rangeIncludes":{"@id":"unece:AmountType"},"schema:domainIncludes":{"@id":"unece:Project"},"rdfs:comment":"The monetary value of the net budget for this procuring project."},{"@id":"unece:subWorksTypeCode","@type":["rdf:Property","owl:DatatypeProperty"],"rdfs:label":"subWorksTypeCode","schema:rangeIncludes":{"@id":"schema:Text"},"schema:domainIncludes":{"@id":"unece:Project"},"rdfs:comment":"A code specifying the type of sub works, such as land surveying or information technology consulting, for this procuring project."},{"@id":"unece:totalBudgetAmount","@type":["rdf:Property","owl:ObjectProperty"],"rdfs:label":"totalBudgetAmount","schema:rangeIncludes":{"@id":"unece:AmountType"},"schema:domainIncludes":{"@id":"unece:Project"},"rdfs:comment":"The monetary value of the total budget which includes net amount, taxes, and material and instalment costs for this procuring project."},{"@id":"unece:worksTypeCode","@type":["rdf:Property","owl:DatatypeProperty"],"rdfs:label":"worksTypeCode","schema:rangeIncludes":{"@id":"schema:Text"},"schema:domainIncludes":{"@id":"unece:Project"},"rdfs:comment":"A code specifying the type of work, such as surveying or consulting, for this procuring project."},{"@id":"unece:contentCode","@type":["rdf:Property","owl:DatatypeProperty"],"rdfs:label":"contentCode","schema:rangeIncludes":{"@id":"schema:Text"},"schema:domainIncludes":{"@id":"unece:Note"},"rdfs:comment":"A code specifying the content of this note."},{"@id":"unece:noteSubjectCode","@type":["rdf:Property","owl:DatatypeProperty"],"rdfs:label":"noteSubjectCode","schema:rangeIncludes":{"@id":"schema:Text"},"schema:domainIncludes":{"@id":"unece:Note"},"rdfs:comment":"A code specifying the subject of this note."},{"@id":"unece:queryId","@type":["rdf:Property","owl:DatatypeProperty"],"rdfs:label":"queryId","schema:rangeIncludes":{"@id":"schema:Text"},"schema:domainIncludes":{"@id":"unece:Response"},"rdfs:comment":"The unique identifier for the query to which this response refers."},{"@id":"unece:responseTypeCode","@type":["rdf:Property","owl:DatatypeProperty"],"rdfs:label":"responseTypeCode","schema:rangeIncludes":{"@id":"unece:ResponseTypeCodeList"},"schema:domainIncludes":{"@id":"unece:Response"},"rdfs:comment":"The code specifying the type of this specification response."},{"@id":"unece:latestResponseDateTime","@type":["rdf:Property","owl:DatatypeProperty"],"rdfs:label":"latestResponseDateTime","schema:rangeIncludes":{"@id":"schema:DateTime"},"schema:domainIncludes":{"@id":"unece:SpecialQuery"},"rdfs:comment":"The date, time, date time, or other date time value for the latest response to this special query."},{"@id":"unece:responseStatusCode","@type":["rdf:Property","owl:DatatypeProperty"],"rdfs:label":"responseStatusCode","schema:rangeIncludes":{"@id":"schema:Text"},"schema:domainIncludes":{"@id":"unece:SpecialQuery"},"rdfs:comment":"The code specifying the response status for this special query."},{"@id":"unece:submittedDateTime","@type":["rdf:Property","owl:DatatypeProperty"],"rdfs:label":"submittedDateTime","schema:rangeIncludes":{"@id":"schema:DateTime"},"schema:domainIncludes":{"@id":"unece:SpecialQuery"},"rdfs:comment":"The date, time, date time, or other date time value when this special query was submitted."},{"@id":"unece:submittingPersonName","@type":["rdf:Property","owl:DatatypeProperty"],"rdfs:label":"submittingPersonName","schema:rangeIncludes":{"@id":"schema:Text"},"schema:domainIncludes":{"@id":"unece:SpecialQuery"},"rdfs:comment":"The name, expressed as text, of the person submitting this special query."},{"@id":"unece:subjectCode","@type":["rdf:Property","owl:DatatypeProperty"],"rdfs:label":"subjectCode","schema:rangeIncludes":{"@id":"schema:Text"},"schema:domainIncludes":{"@id":"unece:SpecifiedNote"},"rdfs:comment":"The code specifying the subject of this specified note."},{"@id":"unece:contentTypeCode","@type":["rdf:Property","owl:DatatypeProperty"],"rdfs:label":"contentTypeCode","schema:rangeIncludes":{"@id":"schema:Text"},"schema:domainIncludes":[{"@id":"unece:MetricCharacteristic"},{"@id":"unece:ProductCharacteristic"},{"@id":"unece:SustainabilityCharacteristic"}],"rdfs:comment":"A code specifying the content type of this product characteristic."},{"@id":"unece:valueQuantity","@type":["rdf:Property","owl:ObjectProperty"],"rdfs:label":"valueQuantity","schema:rangeIncludes":{"@id":"unece:QuantityType"},"schema:domainIncludes":[{"@id":"unece:MetricCharacteristic"},{"@id":"unece:DocumentCharacteristic"}],"rdfs:comment":"A value, expressed as a quantity, for this document characteristic."},{"@id":"unece:countryId","@type":["rdf:Property","owl:DatatypeProperty"],"rdfs:label":"countryId","schema:rangeIncludes":{"@id":"schema:Text"},"schema:domainIncludes":[{"@id":"unece:Country"},{"@id":"unece:LegalRegistration"},{"@id":"unece:GovernmentRegistration"}],"rdfs:comment":"A unique country identifier for this location party."},{"@id":"unece:lastRegisteredYearDateTime","@type":["rdf:Property","owl:DatatypeProperty"],"rdfs:label":"lastRegisteredYearDateTime","schema:rangeIncludes":{"@id":"schema:Text"},"schema:domainIncludes":[{"@id":"unece:LegalRegistration"},{"@id":"unece:GovernmentRegistration"}],"rdfs:comment":"The last registered year of this government registration."},{"@id":"unece:location","@type":["rdf:Property","owl:DatatypeProperty"],"rdfs:label":"location","schema:rangeIncludes":{"@id":"schema:Text"},"schema:domainIncludes":{"@id":"unece:DocumentCharacteristic"},"rdfs:comment":"A location, expressed as text, for this MDH sanitary measure."},{"@id":"unece:valueAdjustmentDirectionCode","@type":["rdf:Property","owl:DatatypeProperty"],"rdfs:label":"valueAdjustmentDirectionCode","schema:rangeIncludes":{"@id":"schema:Text"},"schema:domainIncludes":{"@id":"unece:DocumentCharacteristic"},"rdfs:comment":"The code specifying the adjustment direction for value of this document characteristic."},{"@id":"unece:valueChangedIndicator","@type":["rdf:Property","owl:DatatypeProperty"],"rdfs:label":"valueChangedIndicator","schema:rangeIncludes":{"@id":"schema:Boolean"},"schema:domainIncludes":{"@id":"unece:DocumentCharacteristic"},"rdfs:comment":"The indication of whether or not the value of this document characteristic is changed."},{"@id":"unece:valuePercent","@type":["rdf:Property","owl:DatatypeProperty"],"rdfs:label":"valuePercent","schema:rangeIncludes":{"@id":"schema:Text"},"schema:domainIncludes":{"@id":"unece:DocumentCharacteristic"},"rdfs:comment":"A value, expressed as a percentage, for this document characteristic."},{"@id":"unece:descriptionReference","@type":["rdf:Property","owl:DatatypeProperty"],"rdfs:label":"descriptionReference","schema:rangeIncludes":{"@id":"schema:Text"},"schema:domainIncludes":{"@id":"unece:GeographicalObjectCharacteristic"},"rdfs:comment":"The description reference, expressed as text, for this geographical object characteristic."},{"@id":"unece:geometryCollectionIndicator","@type":["rdf:Property","owl:DatatypeProperty"],"rdfs:label":"geometryCollectionIndicator","schema:rangeIncludes":{"@id":"schema:Boolean"},"schema:domainIncludes":{"@id":"unece:GeographicalObjectCharacteristic"},"rdfs:comment":"The indication of whether or not this geographical object can be characterized as a geometry collection."},{"@id":"unece:physicalIndicator","@type":["rdf:Property","owl:DatatypeProperty"],"rdfs:label":"physicalIndicator","schema:rangeIncludes":{"@id":"schema:Boolean"},"schema:domainIncludes":{"@id":"unece:GeographicalObjectCharacteristic"},"rdfs:comment":"The indication of whether or not this geographical object can be characterized as physical."},{"@id":"unece:relevantGeometryType","@type":["rdf:Property","owl:DatatypeProperty"],"rdfs:label":"relevantGeometryType","schema:rangeIncludes":{"@id":"schema:Text"},"schema:domainIncludes":{"@id":"unece:GeographicalObjectCharacteristic"},"rdfs:comment":"The type of geometry, expressed as text, relevant for this geographical object characteristic."},{"@id":"unece:shapeType","@type":["rdf:Property","owl:DatatypeProperty"],"rdfs:label":"shapeType","schema:rangeIncludes":{"@id":"schema:Text"},"schema:domainIncludes":{"@id":"unece:GeographicalObjectCharacteristic"},"rdfs:comment":"The type of shape, expressed as text, such as a semi-circle, for this geographical object characteristic."},{"@id":"unece:identificationCode","@type":["rdf:Property","owl:DatatypeProperty"],"rdfs:label":"identificationCode","schema:rangeIncludes":{"@id":"schema:Text"},"schema:domainIncludes":{"@id":"unece:IdentifiedFault"},"rdfs:comment":"A code specifying an identified fault."},{"@id":"unece:dimensionTypeCode","@type":["rdf:Property","owl:DatatypeProperty"],"rdfs:label":"dimensionTypeCode","schema:rangeIncludes":{"@id":"unece:DimensionTypeCodeList"},"schema:domainIncludes":{"@id":"unece:SpatialDimension"},"rdfs:comment":"The code specifying the type of spatial dimension, such as thickness, area, or volume."},{"@id":"unece:heightMeasure","@type":["rdf:Property","owl:ObjectProperty"],"rdfs:label":"heightMeasure","schema:rangeIncludes":{"@id":"unece:MeasureType"},"schema:domainIncludes":{"@id":"unece:SpatialDimension"},"rdfs:comment":"The measure of the height component of this spatial dimension."},{"@id":"unece:lengthMeasure","@type":["rdf:Property","owl:ObjectProperty"],"rdfs:label":"lengthMeasure","schema:rangeIncludes":{"@id":"unece:MeasureType"},"schema:domainIncludes":{"@id":"unece:SpatialDimension"},"rdfs:comment":"The measure of the length component of this spatial dimension."},{"@id":"unece:linearUnitDiameterMeasure","@type":["rdf:Property","owl:ObjectProperty"],"rdfs:label":"linearUnitDiameterMeasure","schema:rangeIncludes":{"@id":"unece:LinearUnitMeasureType"},"schema:domainIncludes":{"@id":"unece:SpatialDimension"},"rdfs:comment":"The measure of the diameter component for this spatial dimension."},{"@id":"unece:widthMeasure","@type":["rdf:Property","owl:ObjectProperty"],"rdfs:label":"widthMeasure","schema:rangeIncludes":{"@id":"unece:MeasureType"},"schema:domainIncludes":{"@id":"unece:SpatialDimension"},"rdfs:comment":"The measure of the width component of this spatial dimension."},{"@id":"unece:keywordMarketingPhrase","@type":["rdf:Property","owl:DatatypeProperty"],"rdfs:label":"keywordMarketingPhrase","schema:rangeIncludes":{"@id":"schema:Text"},"schema:domainIncludes":{"@id":"unece:SpecifiedFeature"},"rdfs:comment":"A keyword marketing phrase, expressed as text, for this feature."},{"@id":"unece:marketingPhrase","@type":["rdf:Property","owl:DatatypeProperty"],"rdfs:label":"marketingPhrase","schema:rangeIncludes":{"@id":"schema:Text"},"schema:domainIncludes":[{"@id":"unece:SpecifiedFeature"},{"@id":"unece:Source"}],"rdfs:comment":"A catch phrase, expressed as text, for marketing of this trade product feature."},{"@id":"unece:objective","@type":["rdf:Property","owl:DatatypeProperty"],"rdfs:label":"objective","schema:rangeIncludes":{"@id":"schema:Text"},"schema:domainIncludes":{"@id":"unece:SpecifiedFeature"},"rdfs:comment":"An objective, expressed as text, for this experience product."},{"@id":"unece:usageCode","@type":["rdf:Property","owl:DatatypeProperty"],"rdfs:label":"usageCode","schema:rangeIncludes":{"@id":"schema:Text"},"schema:domainIncludes":{"@id":"unece:SpecifiedFeature"},"rdfs:comment":"The code specifying the usage for this specified feature."},{"@id":"unece:directions","@type":["rdf:Property","owl:DatatypeProperty"],"rdfs:label":"directions","schema:rangeIncludes":{"@id":"schema:Text"},"schema:domainIncludes":{"@id":"unece:SpecifiedLocation"},"rdfs:comment":"Directions, expressed as text, for this specified location."},{"@id":"unece:geopoliticalRegionCode","@type":["rdf:Property","owl:DatatypeProperty"],"rdfs:label":"geopoliticalRegionCode","schema:rangeIncludes":{"@id":"schema:Text"},"schema:domainIncludes":{"@id":"unece:SpecifiedLocation"},"rdfs:comment":"The code specifying the geopolitical region for this specified location."},{"@id":"unece:geopoliticalRegionName","@type":["rdf:Property","owl:DatatypeProperty"],"rdfs:label":"geopoliticalRegionName","schema:rangeIncludes":{"@id":"schema:Text"},"schema:domainIncludes":{"@id":"unece:SpecifiedLocation"},"rdfs:comment":"The name, expressed as text, of the geopolitical region for this specified location."},{"@id":"unece:mapURIId","@type":["rdf:Property","owl:DatatypeProperty"],"rdfs:label":"mapURIId","schema:rangeIncludes":{"@id":"schema:Text"},"schema:domainIncludes":{"@id":"unece:SpecifiedLocation"},"rdfs:comment":"The Uniform Resource Identifier (URI) of the map of this specified route."},{"@id":"unece:specifiedLocationTypeCode","@type":["rdf:Property","owl:DatatypeProperty"],"rdfs:label":"specifiedLocationTypeCode","schema:rangeIncludes":{"@id":"schema:Text"},"schema:domainIncludes":{"@id":"unece:SpecifiedLocation"},"rdfs:comment":"The code specifying the type of this specified location."},{"@id":"unece:specifiedTradeAddress","@type":["rdf:Property","owl:ObjectProperty"],"rdfs:label":"specifiedTradeAddress","schema:rangeIncludes":{"@id":"unece:Address"},"schema:domainIncludes":{"@id":"unece:SpecifiedLocation"},"rdfs:comment":"A address specified for this location."},{"@id":"unece:parameterType","@type":["rdf:Property","owl:DatatypeProperty"],"rdfs:label":"parameterType","schema:rangeIncludes":{"@id":"schema:Text"},"schema:domainIncludes":[{"@id":"unece:SpecifiedParameter"},{"@id":"unece:ObservationObjectiveParameter"}],"rdfs:comment":"A type, expressed as text, for this observation objective parameter."},{"@id":"unece:statusValueMeasure","@type":["rdf:Property","owl:ObjectProperty"],"rdfs:label":"statusValueMeasure","schema:rangeIncludes":{"@id":"unece:MeasureType"},"schema:domainIncludes":[{"@id":"unece:SpecifiedParameter"},{"@id":"unece:ObservationObjectiveParameter"}],"rdfs:comment":"A measure of a value of the status for this specified parameter."},{"@id":"unece:valueAllowedIndicator","@type":["rdf:Property","owl:DatatypeProperty"],"rdfs:label":"valueAllowedIndicator","schema:rangeIncludes":{"@id":"schema:Boolean"},"schema:domainIncludes":[{"@id":"unece:SpecifiedParameter"},{"@id":"unece:ControlSettingParameter"},{"@id":"unece:OperationalParameter"},{"@id":"unece:ObservationObjectiveParameter"}],"rdfs:comment":"The indication of whether or not the value for this specified parameter is allowed."},{"@id":"unece:endId","@type":["rdf:Property","owl:DatatypeProperty"],"rdfs:label":"endId","schema:rangeIncludes":{"@id":"schema:Text"},"schema:domainIncludes":{"@id":"unece:Range"},"rdfs:comment":"The identifier of the end of this specified range."},{"@id":"unece:maximumValueMeasure","@type":["rdf:Property","owl:ObjectProperty"],"rdfs:label":"maximumValueMeasure","schema:rangeIncludes":{"@id":"unece:MeasureType"},"schema:domainIncludes":[{"@id":"unece:Range"},{"@id":"unece:SpecifiedTemperature"},{"@id":"unece:SustainabilityCharacteristic"},{"@id":"unece:ProcessCharacteristic"}],"rdfs:comment":"A measure of a maximum value for this sustainability characteristic."},{"@id":"unece:minimumValueMeasure","@type":["rdf:Property","owl:ObjectProperty"],"rdfs:label":"minimumValueMeasure","schema:rangeIncludes":{"@id":"unece:MeasureType"},"schema:domainIncludes":[{"@id":"unece:Range"},{"@id":"unece:SpecifiedTemperature"},{"@id":"unece:SustainabilityCharacteristic"},{"@id":"unece:ProcessCharacteristic"}],"rdfs:comment":"A measure of a minimum value for this sustainability characteristic."},{"@id":"unece:startId","@type":["rdf:Property","owl:DatatypeProperty"],"rdfs:label":"startId","schema:rangeIncludes":{"@id":"schema:Text"},"schema:domainIncludes":{"@id":"unece:Range"},"rdfs:comment":"The identifier of the start of this specified range."},{"@id":"unece:totalItemQuantity","@type":["rdf:Property","owl:ObjectProperty"],"rdfs:label":"totalItemQuantity","schema:rangeIncludes":{"@id":"unece:QuantityType"},"schema:domainIncludes":{"@id":"unece:Range"},"rdfs:comment":"The total number of items in this specified range."},{"@id":"unece:valueBaseSystemCode","@type":["rdf:Property","owl:DatatypeProperty"],"rdfs:label":"valueBaseSystemCode","schema:rangeIncludes":{"@id":"schema:Text"},"schema:domainIncludes":{"@id":"unece:Range"},"rdfs:comment":"The code specifying the value base system, such as Arabic numerals, for this specified range."},{"@id":"unece:identificationType","@type":["rdf:Property","owl:DatatypeProperty"],"rdfs:label":"identificationType","schema:rangeIncludes":{"@id":"schema:Text"},"schema:domainIncludes":{"@id":"unece:ProprietaryIdentity"},"rdfs:comment":"An identifier type, expressed as text, for this proprietary identity."},{"@id":"unece:level","@type":["rdf:Property","owl:DatatypeProperty"],"rdfs:label":"level","schema:rangeIncludes":{"@id":"schema:Text"},"schema:domainIncludes":{"@id":"unece:CoordinateReferenceSystem"},"rdfs:comment":"The level, expressed as text, of this CS engineering coordinate reference system."},{"@id":"unece:subordinateCoordinateReferenceSystem","@type":["rdf:Property","owl:ObjectProperty"],"rdfs:label":"subordinateCoordinateReferenceSystem","schema:rangeIncludes":{"@id":"unece:CoordinateReferenceSystem"},"schema:domainIncludes":{"@id":"unece:CoordinateReferenceSystem"},"rdfs:comment":"A CS engineering coordinate reference system subordinate to this CS engineering coordinate reference system."},{"@id":"unece:signalSourceAvailableQuantity","@type":["rdf:Property","owl:ObjectProperty"],"rdfs:label":"signalSourceAvailableQuantity","schema:rangeIncludes":{"@id":"unece:QuantityType"},"schema:domainIncludes":{"@id":"unece:CoordinateSourceSystem"},"rdfs:comment":"The quantity of signal source available for this geographical coordinate source system."},{"@id":"unece:sourceTypeCode","@type":["rdf:Property","owl:DatatypeProperty"],"rdfs:label":"sourceTypeCode","schema:rangeIncludes":{"@id":"schema:Text"},"schema:domainIncludes":{"@id":"unece:CoordinateSourceSystem"},"rdfs:comment":"The code specifying a type of source for this geographical coordinate source system."},{"@id":"unece:toleranceMeasure","@type":["rdf:Property","owl:ObjectProperty"],"rdfs:label":"toleranceMeasure","schema:rangeIncludes":{"@id":"unece:MeasureType"},"schema:domainIncludes":[{"@id":"unece:CoordinateSourceSystem"},{"@id":"unece:CalibratedMeasurement"}],"rdfs:comment":"The measure of the tolerance of this calibrated measurement."},{"@id":"unece:usedSignalSourceQuantity","@type":["rdf:Property","owl:ObjectProperty"],"rdfs:label":"usedSignalSourceQuantity","schema:rangeIncludes":{"@id":"unece:QuantityType"},"schema:domainIncludes":{"@id":"unece:CoordinateSourceSystem"},"rdfs:comment":"The quantity of the used signal source of this geographical coordinate source system."},{"@id":"unece:specifiedVersion","@type":["rdf:Property","owl:ObjectProperty"],"rdfs:label":"specifiedVersion","schema:rangeIncludes":{"@id":"unece:Version"},"schema:domainIncludes":{"@id":"unece:DocumentContextParameter"},"rdfs:comment":"The document version specified for this document context parameter."},{"@id":"unece:includedCountry","@type":["rdf:Property","owl:ObjectProperty"],"rdfs:label":"includedCountry","schema:rangeIncludes":{"@id":"unece:Country"},"schema:domainIncludes":{"@id":"unece:GeopoliticalRegion"},"rdfs:comment":"A country included in this trade geopolitical region."},{"@id":"unece:maximumSpecifiedCharacteristic","@type":["rdf:Property","owl:ObjectProperty"],"rdfs:label":"maximumSpecifiedCharacteristic","schema:rangeIncludes":{"@id":"unece:MetricCharacteristic"},"schema:domainIncludes":{"@id":"unece:Issue"},"rdfs:comment":"The maximum metric characteristic specified for this target issue."},{"@id":"unece:minimumSpecifiedCharacteristic","@type":["rdf:Property","owl:ObjectProperty"],"rdfs:label":"minimumSpecifiedCharacteristic","schema:rangeIncludes":{"@id":"unece:MetricCharacteristic"},"schema:domainIncludes":{"@id":"unece:Issue"},"rdfs:comment":"The minimum metric characteristic specified for this target issue."},{"@id":"unece:specifiedMetricCharacteristic","@type":["rdf:Property","owl:ObjectProperty"],"rdfs:label":"specifiedMetricCharacteristic","schema:rangeIncludes":{"@id":"unece:MetricCharacteristic"},"schema:domainIncludes":{"@id":"unece:Issue"},"rdfs:comment":"The metric characteristic specified for this target issue."},{"@id":"unece:lowDispersibleStatusIndicator","@type":["rdf:Property","owl:DatatypeProperty"],"rdfs:label":"lowDispersibleStatusIndicator","schema:rangeIncludes":{"@id":"schema:Boolean"},"schema:domainIncludes":{"@id":"unece:Radionuclide"},"rdfs:comment":"The indication of whether or not this radioactive radionuclide has a low dispersible status."},{"@id":"unece:specialFormIndicator","@type":["rdf:Property","owl:DatatypeProperty"],"rdfs:label":"specialFormIndicator","schema:rangeIncludes":{"@id":"schema:Boolean"},"schema:domainIncludes":{"@id":"unece:Radionuclide"},"rdfs:comment":"The indication of whether or not this radioactive radionuclide has a special form."},{"@id":"unece:includedSegment","@type":["rdf:Property","owl:ObjectProperty"],"rdfs:label":"includedSegment","schema:rangeIncludes":{"@id":"unece:Segment"},"schema:domainIncludes":{"@id":"unece:Section"},"rdfs:comment":"A segment included in this label section."},{"@id":"unece:patternCode","@type":["rdf:Property","owl:DatatypeProperty"],"rdfs:label":"patternCode","schema:rangeIncludes":{"@id":"schema:Text"},"schema:domainIncludes":{"@id":"unece:Section"},"rdfs:comment":"The code specifying the pattern of this label section."},{"@id":"unece:imageBinaryObject","@type":["rdf:Property","owl:DatatypeProperty"],"rdfs:label":"imageBinaryObject","schema:rangeIncludes":{"@id":"schema:Text"},"schema:domainIncludes":{"@id":"unece:Segment"},"rdfs:comment":"The image, expressed as a binary object, for this section segment."},{"@id":"unece:physicalGeographicalCoordinate","@type":["rdf:Property","owl:ObjectProperty"],"rdfs:label":"physicalGeographicalCoordinate","schema:rangeIncludes":{"@id":"unece:GeographicalCoordinate"},"schema:domainIncludes":[{"@id":"unece:SubordinateLocation"},{"@id":"unece:SubordinateSubordinateLocation"}],"rdfs:comment":"Geographical coordinate information for this logistics related location."},{"@id":"unece:subordinateSubordinateSubordinateLocation","@type":["rdf:Property","owl:ObjectProperty"],"rdfs:label":"subordinateSubordinateSubordinateLocation","schema:rangeIncludes":{"@id":"unece:SubordinateSubordinateLocation"},"schema:domainIncludes":{"@id":"unece:SubordinateLocation"},"rdfs:comment":"The location subordinate to this subordinate location."},{"@id":"unece:previousStatusCode","@type":["rdf:Property","owl:DatatypeProperty"],"rdfs:label":"previousStatusCode","schema:rangeIncludes":{"@id":"unece:WorkflowStatusCodeList"},"schema:domainIncludes":{"@id":"unece:WorkflowObject"},"rdfs:comment":"The code specifying the previous status of this trade workflow object."},{"@id":"unece:workflowStatusCode","@type":["rdf:Property","owl:DatatypeProperty"],"rdfs:label":"workflowStatusCode","schema:rangeIncludes":{"@id":"unece:WorkflowStatusCodeList"},"schema:domainIncludes":{"@id":"unece:WorkflowObject"},"rdfs:comment":"The code specifying the status of this trade workflow object."},{"@id":"unece:languageName","@type":["rdf:Property","owl:DatatypeProperty"],"rdfs:label":"languageName","schema:rangeIncludes":{"@id":"schema:Text"},"schema:domainIncludes":{"@id":"unece:LanguageProficiency"},"rdfs:comment":"A name, expressed as text, of the language for which this language proficiency is defined."},{"@id":"unece:personalLanguageProficiencyLanguageCode","@type":["rdf:Property","owl:DatatypeProperty"],"rdfs:label":"personalLanguageProficiencyLanguageCode","schema:rangeIncludes":{"@id":"unece:LanguageCodeList"},"schema:domainIncludes":{"@id":"unece:LanguageProficiency"},"rdfs:comment":"The code specifying the language for this personal language proficiency."},{"@id":"unece:personalLanguageProficiencyLanguageId","@type":["rdf:Property","owl:DatatypeProperty"],"rdfs:label":"personalLanguageProficiencyLanguageId","schema:rangeIncludes":{"@id":"unece:LanguageId"},"schema:domainIncludes":{"@id":"unece:LanguageProficiency"},"rdfs:comment":"The identifier of the language for which this personal language proficiency is defined."},{"@id":"unece:readingLevelCode","@type":["rdf:Property","owl:DatatypeProperty"],"rdfs:label":"readingLevelCode","schema:rangeIncludes":{"@id":"schema:Text"},"schema:domainIncludes":{"@id":"unece:LanguageProficiency"},"rdfs:comment":"The code specifying the personal reading proficiency level in this language."},{"@id":"unece:speakingLevelCode","@type":["rdf:Property","owl:DatatypeProperty"],"rdfs:label":"speakingLevelCode","schema:rangeIncludes":{"@id":"schema:Text"},"schema:domainIncludes":{"@id":"unece:LanguageProficiency"},"rdfs:comment":"The code specifying the personal speaking proficiency level in this language."},{"@id":"unece:writingLevelCode","@type":["rdf:Property","owl:DatatypeProperty"],"rdfs:label":"writingLevelCode","schema:rangeIncludes":{"@id":"schema:Text"},"schema:domainIncludes":{"@id":"unece:LanguageProficiency"},"rdfs:comment":"The code specifying the personal writing proficiency level in this language."},{"@id":"unece:locationCode","@type":["rdf:Property","owl:DatatypeProperty"],"rdfs:label":"locationCode","schema:rangeIncludes":{"@id":"schema:Text"},"schema:domainIncludes":{"@id":"unece:SecurityTag"},"rdfs:comment":"The code specifying the location of this product security tag."},{"@id":"unece:matchingEvent","@type":["rdf:Property","owl:ObjectProperty"],"rdfs:label":"matchingEvent","schema:rangeIncludes":{"@id":"unece:CommunicationEvent"},"schema:domainIncludes":{"@id":"unece:Pairing"},"rdfs:comment":"A matching event for this communication pairing."},{"@id":"unece:methodCode","@type":["rdf:Property","owl:DatatypeProperty"],"rdfs:label":"methodCode","schema:rangeIncludes":{"@id":"schema:Text"},"schema:domainIncludes":{"@id":"unece:Pairing"},"rdfs:comment":"The code specifying the method by which this cross-border customs valuation is determined."},{"@id":"unece:pairedIndicator","@type":["rdf:Property","owl:DatatypeProperty"],"rdfs:label":"pairedIndicator","schema:rangeIncludes":{"@id":"schema:Boolean"},"schema:domainIncludes":{"@id":"unece:Pairing"},"rdfs:comment":"The indication of whether or not the entity is paired in this communication pairing."},{"@id":"unece:targetEntityId","@type":["rdf:Property","owl:DatatypeProperty"],"rdfs:label":"targetEntityId","schema:rangeIncludes":{"@id":"schema:Text"},"schema:domainIncludes":{"@id":"unece:Pairing"},"rdfs:comment":"The identifier of the target entity for this communication pairing."},{"@id":"unece:temperatureUnitValueMeasure","@type":["rdf:Property","owl:ObjectProperty"],"rdfs:label":"temperatureUnitValueMeasure","schema:rangeIncludes":{"@id":"unece:TemperatureUnitMeasureType"},"schema:domainIncludes":{"@id":"unece:SpecifiedTemperature"},"rdfs:comment":"The measure of the value of this specified temperature, such as a temperature value of ten degrees Celsius."},{"@id":"unece:roleCode","@type":["rdf:Property","owl:DatatypeProperty"],"rdfs:label":"roleCode","schema:rangeIncludes":{"@id":"schema:Text"},"schema:domainIncludes":{"@id":"unece:CooperatingOrganization"},"rdfs:comment":"The code specifying the role for this cooperating organization."},{"@id":"unece:usedInformationSource","@type":["rdf:Property","owl:ObjectProperty"],"rdfs:label":"usedInformationSource","schema:rangeIncludes":{"@id":"unece:InformationSource"},"schema:domainIncludes":{"@id":"unece:CooperatingOrganization"},"rdfs:comment":"A specified cooperative information source used for or from this cooperating organization."},{"@id":"unece:objectClassId","@type":["rdf:Property","owl:DatatypeProperty"],"rdfs:label":"objectClassId","schema:rangeIncludes":{"@id":"schema:Text"},"schema:domainIncludes":{"@id":"unece:EventElement"},"rdfs:comment":"The identifier of the object class for this TT event element."},{"@id":"unece:procedure","@type":["rdf:Property","owl:DatatypeProperty"],"rdfs:label":"procedure","schema:rangeIncludes":{"@id":"schema:Text"},"schema:domainIncludes":[{"@id":"unece:DocumentHandlingInstructions"},{"@id":"unece:InspectionInstructions"},{"@id":"unece:LaboratoryObservationInstructions"},{"@id":"unece:TemperatureSettingInstructions"}],"rdfs:comment":"A procedure, expressed as text, for a set of inspection instructions."},{"@id":"unece:requirementIndicator","@type":["rdf:Property","owl:DatatypeProperty"],"rdfs:label":"requirementIndicator","schema:rangeIncludes":{"@id":"schema:Boolean"},"schema:domainIncludes":{"@id":"unece:DocumentHandlingInstructions"},"rdfs:comment":"The indication of whether or not a requirement exists for these document handling instructions."},{"@id":"unece:MeasureTypeValue","@type":["rdf:Property","owl:DatatypeProperty"],"rdfs:label":"MeasureTypeValue","schema:rangeIncludes":{"@id":"schema:Float"},"schema:domainIncludes":{"@id":"unece:MeasureType"},"rdfs:comment":"The numeric value."},{"@id":"unece:MeasureTypeCode","@type":["rdf:Property","owl:DatatypeProperty"],"rdfs:label":"MeasureTypeCode","schema:rangeIncludes":{"@id":"unece:MeasureCode"},"schema:domainIncludes":{"@id":"unece:MeasureType"},"rdfs:comment":"The unit code."},{"@id":"unece:TemperatureUnitMeasureTypeValue","@type":["rdf:Property","owl:DatatypeProperty"],"rdfs:label":"TemperatureUnitMeasureTypeValue","schema:rangeIncludes":{"@id":"schema:Float"},"schema:domainIncludes":{"@id":"unece:TemperatureUnitMeasureType"},"rdfs:comment":"The numeric value."},{"@id":"unece:TemperatureUnitMeasureTypeCode","@type":["rdf:Property","owl:DatatypeProperty"],"rdfs:label":"TemperatureUnitMeasureTypeCode","schema:rangeIncludes":{"@id":"unece:TemperatureUnitMeasureCode"},"schema:domainIncludes":{"@id":"unece:TemperatureUnitMeasureType"},"rdfs:comment":"The unit code."},{"@id":"unece:QuantityTypeValue","@type":["rdf:Property","owl:DatatypeProperty"],"rdfs:label":"QuantityTypeValue","schema:rangeIncludes":{"@id":"schema:Float"},"schema:domainIncludes":{"@id":"unece:QuantityType"},"rdfs:comment":"The numeric value."},{"@id":"unece:QuantityTypeCode","@type":["rdf:Property","owl:DatatypeProperty"],"rdfs:label":"QuantityTypeCode","schema:rangeIncludes":{"@id":"unece:QuantityCode"},"schema:domainIncludes":{"@id":"unece:QuantityType"},"rdfs:comment":"The unit code."},{"@id":"unece:AmountTypeValue","@type":["rdf:Property","owl:DatatypeProperty"],"rdfs:label":"AmountTypeValue","schema:rangeIncludes":{"@id":"schema:Float"},"schema:domainIncludes":{"@id":"unece:AmountType"},"rdfs:comment":"A number of monetary units."},{"@id":"unece:AmountTypeCurrency","@type":["rdf:Property","owl:DatatypeProperty"],"rdfs:label":"AmountTypeCurrency","schema:rangeIncludes":{"@id":"unece:AmountCurrency"},"schema:domainIncludes":{"@id":"unece:AmountType"},"rdfs:comment":"An amount currency code."},{"@id":"unece:DurationUnitMeasureTypeValue","@type":["rdf:Property","owl:DatatypeProperty"],"rdfs:label":"DurationUnitMeasureTypeValue","schema:rangeIncludes":{"@id":"schema:Float"},"schema:domainIncludes":{"@id":"unece:DurationUnitMeasureType"},"rdfs:comment":"The numeric value."},{"@id":"unece:DurationUnitMeasureTypeCode","@type":["rdf:Property","owl:DatatypeProperty"],"rdfs:label":"DurationUnitMeasureTypeCode","schema:rangeIncludes":{"@id":"unece:DurationUnitMeasureCode"},"schema:domainIncludes":{"@id":"unece:DurationUnitMeasureType"},"rdfs:comment":"The unit code."},{"@id":"unece:marginValueNumeric","@type":["rdf:Property","owl:DatatypeProperty"],"rdfs:label":"marginValueNumeric","schema:rangeIncludes":{"@id":"schema:Text"},"schema:domainIncludes":{"@id":"unece:Tolerance"},"rdfs:comment":"The margin numeric value of this specified tolerance."},{"@id":"unece:marginValuePercent","@type":["rdf:Property","owl:DatatypeProperty"],"rdfs:label":"marginValuePercent","schema:rangeIncludes":{"@id":"schema:Text"},"schema:domainIncludes":{"@id":"unece:Tolerance"},"rdfs:comment":"The margin percentage value of this specified tolerance."},{"@id":"unece:minusValuePercent","@type":["rdf:Property","owl:DatatypeProperty"],"rdfs:label":"minusValuePercent","schema:rangeIncludes":{"@id":"schema:Text"},"schema:domainIncludes":{"@id":"unece:Tolerance"},"rdfs:comment":"The minus percentage value of this specified tolerance."},{"@id":"unece:minusValueQuantity","@type":["rdf:Property","owl:ObjectProperty"],"rdfs:label":"minusValueQuantity","schema:rangeIncludes":{"@id":"unece:QuantityType"},"schema:domainIncludes":{"@id":"unece:Tolerance"},"rdfs:comment":"The minus quantity value of this specified tolerance."},{"@id":"unece:surplusValuePercent","@type":["rdf:Property","owl:DatatypeProperty"],"rdfs:label":"surplusValuePercent","schema:rangeIncludes":{"@id":"schema:Text"},"schema:domainIncludes":{"@id":"unece:Tolerance"},"rdfs:comment":"The surplus percentage value of this specified tolerance."},{"@id":"unece:surplusValueQuantity","@type":["rdf:Property","owl:ObjectProperty"],"rdfs:label":"surplusValueQuantity","schema:rangeIncludes":{"@id":"unece:QuantityType"},"schema:domainIncludes":{"@id":"unece:Tolerance"},"rdfs:comment":"The surplus quantity value of this specified tolerance."},{"@id":"unece:LinearUnitMeasureTypeValue","@type":["rdf:Property","owl:DatatypeProperty"],"rdfs:label":"LinearUnitMeasureTypeValue","schema:rangeIncludes":{"@id":"schema:Float"},"schema:domainIncludes":{"@id":"unece:LinearUnitMeasureType"},"rdfs:comment":"The numeric value."},{"@id":"unece:LinearUnitMeasureTypeCode","@type":["rdf:Property","owl:DatatypeProperty"],"rdfs:label":"LinearUnitMeasureTypeCode","schema:rangeIncludes":{"@id":"unece:LinearUnitMeasureCode"},"schema:domainIncludes":{"@id":"unece:LinearUnitMeasureType"},"rdfs:comment":"The unit code."},{"@id":"unece:actualDateTime","@type":["rdf:Property","owl:DatatypeProperty"],"rdfs:label":"actualDateTime","schema:rangeIncludes":{"@id":"schema:Text"},"schema:domainIncludes":{"@id":"unece:Authentication"},"rdfs:comment":"An actual date, time, date time, or other date time value of this financial booking."},{"@id":"unece:governmentActionTypeCode","@type":["rdf:Property","owl:DatatypeProperty"],"rdfs:label":"governmentActionTypeCode","schema:rangeIncludes":{"@id":"unece:GovernmentActionCodeList"},"schema:domainIncludes":{"@id":"unece:Authentication"},"rdfs:comment":"The code specifying the type of document authentication."},{"@id":"unece:includedClause","@type":["rdf:Property","owl:ObjectProperty"],"rdfs:label":"includedClause","schema:rangeIncludes":{"@id":"unece:Clause"},"schema:domainIncludes":{"@id":"unece:Authentication"},"rdfs:comment":"A document clause included in this document authentication."},{"@id":"unece:locationProviderParty","@type":["rdf:Property","owl:ObjectProperty"],"rdfs:label":"locationProviderParty","schema:rangeIncludes":{"@id":"unece:Party"},"schema:domainIncludes":{"@id":"unece:Authentication"},"rdfs:comment":"The trade party providing the location for this document authentication."},{"@id":"unece:providerParty","@type":["rdf:Property","owl:ObjectProperty"],"rdfs:label":"providerParty","schema:rangeIncludes":{"@id":"unece:Party"},"schema:domainIncludes":{"@id":"unece:Authentication"},"rdfs:comment":"The provider party for this monitoring IOT device."},{"@id":"unece:representationTypeCode","@type":["rdf:Property","owl:DatatypeProperty"],"rdfs:label":"representationTypeCode","schema:rangeIncludes":{"@id":"schema:Text"},"schema:domainIncludes":{"@id":"unece:Authentication"},"rdfs:comment":"The code specifying the type of representation of this document authentication, such as direct or indirect."},{"@id":"unece:signatory","@type":["rdf:Property","owl:DatatypeProperty"],"rdfs:label":"signatory","schema:rangeIncludes":{"@id":"schema:Text"},"schema:domainIncludes":{"@id":"unece:Authentication"},"rdfs:comment":"The signatory, expressed as text, for this document authentication."},{"@id":"unece:signatoryImageBinaryObject","@type":["rdf:Property","owl:DatatypeProperty"],"rdfs:label":"signatoryImageBinaryObject","schema:rangeIncludes":{"@id":"schema:Text"},"schema:domainIncludes":{"@id":"unece:Authentication"},"rdfs:comment":"The signatory image, expressed as a binary object, for this document authentication."},{"@id":"unece:statement","@type":["rdf:Property","owl:DatatypeProperty"],"rdfs:label":"statement","schema:rangeIncludes":{"@id":"schema:Text"},"schema:domainIncludes":[{"@id":"unece:Authentication"},{"@id":"unece:InspectionResult"}],"rdfs:comment":"A statement, expressed as text, for this specified inspection result."},{"@id":"unece:statementCode","@type":["rdf:Property","owl:DatatypeProperty"],"rdfs:label":"statementCode","schema:rangeIncludes":{"@id":"schema:Text"},"schema:domainIncludes":{"@id":"unece:Authentication"},"rdfs:comment":"The code specifying the statement for this document authentication."},{"@id":"unece:associatedMeasurement","@type":["rdf:Property","owl:ObjectProperty"],"rdfs:label":"associatedMeasurement","schema:rangeIncludes":{"@id":"unece:Measurement"},"schema:domainIncludes":{"@id":"unece:Clause"},"rdfs:comment":"A measurement associated with this document clause."},{"@id":"unece:associatedPeriod","@type":["rdf:Property","owl:ObjectProperty"],"rdfs:label":"associatedPeriod","schema:rangeIncludes":{"@id":"unece:SpecifiedPeriod"},"schema:domainIncludes":{"@id":"unece:Clause"},"rdfs:comment":"A period of time associated with this document clause."},{"@id":"unece:uRLId","@type":["rdf:Property","owl:DatatypeProperty"],"rdfs:label":"uRLId","schema:rangeIncludes":{"@id":"schema:Text"},"schema:domainIncludes":{"@id":"unece:Clause"},"rdfs:comment":"The Uniform Resource Locator (URL) for this document clause."},{"@id":"unece:additionalStreetName","@type":["rdf:Property","owl:DatatypeProperty"],"rdfs:label":"additionalStreetName","schema:rangeIncludes":{"@id":"schema:Text"},"schema:domainIncludes":{"@id":"unece:Address"},"rdfs:comment":"The additional name of a street, expressed as text, for this trade address."},{"@id":"unece:addressTypeCode","@type":["rdf:Property","owl:DatatypeProperty"],"rdfs:label":"addressTypeCode","schema:rangeIncludes":{"@id":"unece:AddressTypeCodeList"},"schema:domainIncludes":{"@id":"unece:Address"},"rdfs:comment":"A code specifying the type of this trade address, such as business address or home address."},{"@id":"unece:attentionOf","@type":["rdf:Property","owl:DatatypeProperty"],"rdfs:label":"attentionOf","schema:rangeIncludes":{"@id":"schema:Text"},"schema:domainIncludes":{"@id":"unece:Address"},"rdfs:comment":"The name, expressed as text, of a person or department in the organization to whom incoming mail is marked with words such as 'for the attention of' or 'FAO' or 'ATTN' for this trade address."},{"@id":"unece:buildingName","@type":["rdf:Property","owl:DatatypeProperty"],"rdfs:label":"buildingName","schema:rangeIncludes":{"@id":"schema:Text"},"schema:domainIncludes":{"@id":"unece:Address"},"rdfs:comment":"The name, expressed as text, of a building, a house or other structure on a street at this trade address."},{"@id":"unece:buildingNumber","@type":["rdf:Property","owl:DatatypeProperty"],"rdfs:label":"buildingNumber","schema:rangeIncludes":{"@id":"schema:Text"},"schema:domainIncludes":{"@id":"unece:Address"},"rdfs:comment":"The building number, expressed as text, in this trade address."},{"@id":"unece:careOf","@type":["rdf:Property","owl:DatatypeProperty"],"rdfs:label":"careOf","schema:rangeIncludes":{"@id":"schema:Text"},"schema:domainIncludes":{"@id":"unece:Address"},"rdfs:comment":"The name, expressed as text, of a person or organization at this trade address to whom incoming mail is marked with words such as 'care of' or 'C/O'."},{"@id":"unece:cityId","@type":["rdf:Property","owl:DatatypeProperty"],"rdfs:label":"cityId","schema:rangeIncludes":{"@id":"schema:Text"},"schema:domainIncludes":{"@id":"unece:Address"},"rdfs:comment":"The identifier of the city for this trade address, such as United Nations Location Code (UNLOCODE)."},{"@id":"unece:citySubDivisionName","@type":["rdf:Property","owl:DatatypeProperty"],"rdfs:label":"citySubDivisionName","schema:rangeIncludes":{"@id":"schema:Text"},"schema:domainIncludes":{"@id":"unece:Address"},"rdfs:comment":"A name, expressed as text, of a sub-division of a city for this trade address, for example a district or borough."},{"@id":"unece:departmentName","@type":["rdf:Property","owl:DatatypeProperty"],"rdfs:label":"departmentName","schema:rangeIncludes":{"@id":"schema:Text"},"schema:domainIncludes":[{"@id":"unece:Address"},{"@id":"unece:LaboratoryObservationContact"}],"rdfs:comment":"The name, expressed as text, of a department for this trade address."},{"@id":"unece:freeForm","@type":["rdf:Property","owl:DatatypeProperty"],"rdfs:label":"freeForm","schema:rangeIncludes":{"@id":"schema:Text"},"schema:domainIncludes":{"@id":"unece:Address"},"rdfs:comment":"A free form representation, expressed as text, of this trade address."},{"@id":"unece:geoCoordinateIdentificationGeographicalCoordinate","@type":["rdf:Property","owl:ObjectProperty"],"rdfs:label":"geoCoordinateIdentificationGeographicalCoordinate","schema:rangeIncludes":{"@id":"unece:GeographicalCoordinate"},"schema:domainIncludes":{"@id":"unece:Address"},"rdfs:comment":"An identification of a set of geographical coordinates for this trade address."},{"@id":"unece:lineFive","@type":["rdf:Property","owl:DatatypeProperty"],"rdfs:label":"lineFive","schema:rangeIncludes":{"@id":"schema:Text"},"schema:domainIncludes":{"@id":"unece:Address"},"rdfs:comment":"The fifth free form line, expressed as text, of this financial institution address."},{"@id":"unece:lineFour","@type":["rdf:Property","owl:DatatypeProperty"],"rdfs:label":"lineFour","schema:rangeIncludes":{"@id":"schema:Text"},"schema:domainIncludes":{"@id":"unece:Address"},"rdfs:comment":"The fourth free form line, expressed as text, of this financial institution address."},{"@id":"unece:lineOne","@type":["rdf:Property","owl:DatatypeProperty"],"rdfs:label":"lineOne","schema:rangeIncludes":{"@id":"schema:Text"},"schema:domainIncludes":{"@id":"unece:Address"},"rdfs:comment":"The first free form line, expressed as text, of this financial institution address."},{"@id":"unece:lineThree","@type":["rdf:Property","owl:DatatypeProperty"],"rdfs:label":"lineThree","schema:rangeIncludes":{"@id":"schema:Text"},"schema:domainIncludes":{"@id":"unece:Address"},"rdfs:comment":"The third free form line, expressed as text, of this financial institution address."},{"@id":"unece:lineTwo","@type":["rdf:Property","owl:DatatypeProperty"],"rdfs:label":"lineTwo","schema:rangeIncludes":{"@id":"schema:Text"},"schema:domainIncludes":{"@id":"unece:Address"},"rdfs:comment":"The second free form line, expressed as text, of this financial institution address."},{"@id":"unece:postOfficeBox","@type":["rdf:Property","owl:DatatypeProperty"],"rdfs:label":"postOfficeBox","schema:rangeIncludes":{"@id":"schema:Text"},"schema:domainIncludes":{"@id":"unece:Address"},"rdfs:comment":"The post office box, expressed as text, for this financial institution address."},{"@id":"unece:postcodeCode","@type":["rdf:Property","owl:DatatypeProperty"],"rdfs:label":"postcodeCode","schema:rangeIncludes":{"@id":"schema:Text"},"schema:domainIncludes":{"@id":"unece:Address"},"rdfs:comment":"A code specifying the postcode of this trade address."},{"@id":"unece:streetName","@type":["rdf:Property","owl:DatatypeProperty"],"rdfs:label":"streetName","schema:rangeIncludes":{"@id":"schema:Text"},"schema:domainIncludes":{"@id":"unece:Address"},"rdfs:comment":"A name, expressed as text, of a street or thoroughfare for this trade address."},{"@id":"unece:actualOccurrenceDateTime","@type":["rdf:Property","owl:DatatypeProperty"],"rdfs:label":"actualOccurrenceDateTime","schema:rangeIncludes":{"@id":"schema:Text"},"schema:domainIncludes":{"@id":"unece:Event"},"rdfs:comment":"The date, time, date time or other date time value of the actual arrival related to this transport event."},{"@id":"unece:actualOccurrencePeriod","@type":["rdf:Property","owl:ObjectProperty"],"rdfs:label":"actualOccurrencePeriod","schema:rangeIncludes":{"@id":"unece:SpecifiedPeriod"},"schema:domainIncludes":{"@id":"unece:Event"},"rdfs:comment":"The actual period of time during which this transport event occurred."},{"@id":"unece:estimatedOccurrenceDateTime","@type":["rdf:Property","owl:DatatypeProperty"],"rdfs:label":"estimatedOccurrenceDateTime","schema:rangeIncludes":{"@id":"schema:Text"},"schema:domainIncludes":{"@id":"unece:Event"},"rdfs:comment":"The estimated date, time, date time, or other date time value of the occurrence of this transport event."},{"@id":"unece:occurrencePeriod","@type":["rdf:Property","owl:ObjectProperty"],"rdfs:label":"occurrencePeriod","schema:rangeIncludes":{"@id":"unece:SpecifiedPeriod"},"schema:domainIncludes":{"@id":"unece:Event"},"rdfs:comment":"The specified period of laycan time during which this transport event occurs."},{"@id":"unece:scheduledOccurrenceDateTime","@type":["rdf:Property","owl:DatatypeProperty"],"rdfs:label":"scheduledOccurrenceDateTime","schema:rangeIncludes":{"@id":"schema:Text"},"schema:domainIncludes":{"@id":"unece:Event"},"rdfs:comment":"A pilot boarding place, expressed as text, for this transport event."},{"@id":"unece:scheduledOccurrencePeriod","@type":["rdf:Property","owl:ObjectProperty"],"rdfs:label":"scheduledOccurrencePeriod","schema:rangeIncludes":{"@id":"unece:SpecifiedPeriod"},"schema:domainIncludes":{"@id":"unece:Event"},"rdfs:comment":"The scheduled period of time specified for the occurrence of this transport event."},{"@id":"unece:WeightUnitMeasureTypeValue","@type":["rdf:Property","owl:DatatypeProperty"],"rdfs:label":"WeightUnitMeasureTypeValue","schema:rangeIncludes":{"@id":"schema:Float"},"schema:domainIncludes":{"@id":"unece:WeightUnitMeasureType"},"rdfs:comment":"The numeric value."},{"@id":"unece:WeightUnitMeasureTypeCode","@type":["rdf:Property","owl:DatatypeProperty"],"rdfs:label":"WeightUnitMeasureTypeCode","schema:rangeIncludes":{"@id":"unece:WeightUnitMeasureCode"},"schema:domainIncludes":{"@id":"unece:WeightUnitMeasureType"},"rdfs:comment":"The unit code."},{"@id":"unece:UnitMeasureTypeValue","@type":["rdf:Property","owl:DatatypeProperty"],"rdfs:label":"UnitMeasureTypeValue","schema:rangeIncludes":{"@id":"schema:Float"},"schema:domainIncludes":{"@id":"unece:UnitMeasureType"},"rdfs:comment":"The numeric value."},{"@id":"unece:UnitMeasureTypeCode","@type":["rdf:Property","owl:DatatypeProperty"],"rdfs:label":"UnitMeasureTypeCode","schema:rangeIncludes":{"@id":"unece:UnitMeasureCode"},"schema:domainIncludes":{"@id":"unece:UnitMeasureType"},"rdfs:comment":"The unit code."},{"@id":"unece:VolumeUnitMeasureTypeValue","@type":["rdf:Property","owl:DatatypeProperty"],"rdfs:label":"VolumeUnitMeasureTypeValue","schema:rangeIncludes":{"@id":"schema:Float"},"schema:domainIncludes":{"@id":"unece:VolumeUnitMeasureType"},"rdfs:comment":"The numeric value."},{"@id":"unece:VolumeUnitMeasureTypeCode","@type":["rdf:Property","owl:DatatypeProperty"],"rdfs:label":"VolumeUnitMeasureTypeCode","schema:rangeIncludes":{"@id":"unece:VolumeUnitMeasureCode"},"schema:domainIncludes":{"@id":"unece:VolumeUnitMeasureType"},"rdfs:comment":"The unit code."},{"@id":"unece:AirFlowUnitMeasureTypeValue","@type":["rdf:Property","owl:DatatypeProperty"],"rdfs:label":"AirFlowUnitMeasureTypeValue","schema:rangeIncludes":{"@id":"schema:Float"},"schema:domainIncludes":{"@id":"unece:AirFlowUnitMeasureType"},"rdfs:comment":"The numeric value."},{"@id":"unece:AirFlowUnitMeasureTypeCode","@type":["rdf:Property","owl:DatatypeProperty"],"rdfs:label":"AirFlowUnitMeasureTypeCode","schema:rangeIncludes":{"@id":"unece:AirFlowUnitMeasureCode"},"schema:domainIncludes":{"@id":"unece:AirFlowUnitMeasureType"},"rdfs:comment":"The unit code."},{"@id":"unece:birthCountryId","@type":["rdf:Property","owl:DatatypeProperty"],"rdfs:label":"birthCountryId","schema:rangeIncludes":{"@id":"schema:Text"},"schema:domainIncludes":{"@id":"unece:Person"},"rdfs:comment":"The identifier of the birth country of this transport person."},{"@id":"unece:birthplaceName","@type":["rdf:Property","owl:DatatypeProperty"],"rdfs:label":"birthplaceName","schema:rangeIncludes":{"@id":"schema:Text"},"schema:domainIncludes":{"@id":"unece:Person"},"rdfs:comment":"The name, expressed as text, of the place where this transport person was born."},{"@id":"unece:emailURICommunication","@type":["rdf:Property","owl:ObjectProperty"],"rdfs:label":"emailURICommunication","schema:rangeIncludes":{"@id":"unece:Communication"},"schema:domainIncludes":[{"@id":"unece:Person"},{"@id":"unece:Contact"}],"rdfs:comment":"A code specifying a category for this cross-border regulatory procedure, such as the appendices of the CITES Convention."},{"@id":"unece:familyName","@type":["rdf:Property","owl:DatatypeProperty"],"rdfs:label":"familyName","schema:rangeIncludes":{"@id":"schema:Text"},"schema:domainIncludes":[{"@id":"unece:Person"},{"@id":"unece:Chemical"}],"rdfs:comment":"A date, time, date time, or other date time value that this person embarked upon a means of transport."},{"@id":"unece:givenName","@type":["rdf:Property","owl:DatatypeProperty"],"rdfs:label":"givenName","schema:rangeIncludes":{"@id":"schema:Text"},"schema:domainIncludes":{"@id":"unece:Person"},"rdfs:comment":"A given name, expressed as text, for this transport person."},{"@id":"unece:landlineTelephoneCommunication","@type":["rdf:Property","owl:ObjectProperty"],"rdfs:label":"landlineTelephoneCommunication","schema:rangeIncludes":{"@id":"unece:Communication"},"schema:domainIncludes":{"@id":"unece:Person"},"rdfs:comment":"The indication of whether or not this transport person is in transit."},{"@id":"unece:mobileTelephoneCommunication","@type":["rdf:Property","owl:ObjectProperty"],"rdfs:label":"mobileTelephoneCommunication","schema:rangeIncludes":{"@id":"unece:Communication"},"schema:domainIncludes":[{"@id":"unece:Person"},{"@id":"unece:LaboratoryObservationContact"}],"rdfs:comment":"Mobile telephone communication information for this transport person."},{"@id":"unece:nationalityCountry","@type":["rdf:Property","owl:ObjectProperty"],"rdfs:label":"nationalityCountry","schema:rangeIncludes":{"@id":"unece:Country"},"schema:domainIncludes":{"@id":"unece:Person"},"rdfs:comment":"A country that constitutes a nationality by origin, birth, or naturalization for this transport person."},{"@id":"unece:contactPersonTitleCode","@type":["rdf:Property","owl:DatatypeProperty"],"rdfs:label":"contactPersonTitleCode","schema:rangeIncludes":{"@id":"unece:TitleCodeList"},"schema:domainIncludes":{"@id":"unece:Contact"},"rdfs:comment":"The code specifying the title of this contact person, such as Ms., Doctor, Mister."},{"@id":"unece:countryResidenceCountryId","@type":["rdf:Property","owl:DatatypeProperty"],"rdfs:label":"countryResidenceCountryId","schema:rangeIncludes":{"@id":"unece:CountryId"},"schema:domainIncludes":{"@id":"unece:Contact"},"rdfs:comment":"The identifier of the residence country of this contact person."},{"@id":"unece:faxCommunication","@type":["rdf:Property","owl:ObjectProperty"],"rdfs:label":"faxCommunication","schema:rangeIncludes":{"@id":"unece:Communication"},"schema:domainIncludes":[{"@id":"unece:Contact"},{"@id":"unece:LaboratoryObservationContact"}],"rdfs:comment":"Facsimile communication information for this contact person."},{"@id":"unece:instantMessagingCommunication","@type":["rdf:Property","owl:ObjectProperty"],"rdfs:label":"instantMessagingCommunication","schema:rangeIncludes":{"@id":"unece:Communication"},"schema:domainIncludes":{"@id":"unece:Contact"},"rdfs:comment":"An instant messaging communication for this contact person."},{"@id":"unece:role","@type":["rdf:Property","owl:DatatypeProperty"],"rdfs:label":"role","schema:rangeIncludes":{"@id":"schema:Text"},"schema:domainIncludes":{"@id":"unece:Contact"},"rdfs:comment":"A role, expressed as text, for this contact person."},{"@id":"unece:specifiedBirthAddress","@type":["rdf:Property","owl:ObjectProperty"],"rdfs:label":"specifiedBirthAddress","schema:rangeIncludes":{"@id":"unece:BirthAddress"},"schema:domainIncludes":{"@id":"unece:Contact"},"rdfs:comment":"The birth address specified for this contact person."},{"@id":"unece:specifiedEmployerIdentity","@type":["rdf:Property","owl:ObjectProperty"],"rdfs:label":"specifiedEmployerIdentity","schema:rangeIncludes":{"@id":"unece:EmployerIdentity"},"schema:domainIncludes":{"@id":"unece:Contact"},"rdfs:comment":"An employer identity specified for this contact person."},{"@id":"unece:specifiedPersonIdentity","@type":["rdf:Property","owl:ObjectProperty"],"rdfs:label":"specifiedPersonIdentity","schema:rangeIncludes":{"@id":"unece:PersonIdentity"},"schema:domainIncludes":{"@id":"unece:Contact"},"rdfs:comment":"The person identity specified for this contact person."},{"@id":"unece:telephoneCommunication","@type":["rdf:Property","owl:ObjectProperty"],"rdfs:label":"telephoneCommunication","schema:rangeIncludes":{"@id":"unece:Communication"},"schema:domainIncludes":[{"@id":"unece:Contact"},{"@id":"unece:LaboratoryObservationContact"}],"rdfs:comment":"A telephone communication for this trade party."},{"@id":"unece:websiteURICommunication","@type":["rdf:Property","owl:ObjectProperty"],"rdfs:label":"websiteURICommunication","schema:rangeIncludes":{"@id":"unece:Communication"},"schema:domainIncludes":[{"@id":"unece:Contact"},{"@id":"unece:LaboratoryObservationParty"}],"rdfs:comment":"A website Uniform Resource Identifier (URI) communication for this contact person."},{"@id":"unece:abbreviatedName","@type":["rdf:Property","owl:DatatypeProperty"],"rdfs:label":"abbreviatedName","schema:rangeIncludes":{"@id":"schema:Text"},"schema:domainIncludes":{"@id":"unece:AcademicQualification"},"rdfs:comment":"The abbreviated name, expressed as text, of this academic qualification."},{"@id":"unece:abbreviation","@type":["rdf:Property","owl:DatatypeProperty"],"rdfs:label":"abbreviation","schema:rangeIncludes":{"@id":"schema:Text"},"schema:domainIncludes":[{"@id":"unece:InspectionReference"},{"@id":"unece:LaboratoryObservationReference"}],"rdfs:comment":"An abbreviation, expressed as text, for this supply chain reference."},{"@id":"unece:comment","@type":["rdf:Property","owl:DatatypeProperty"],"rdfs:label":"comment","schema:rangeIncludes":{"@id":"schema:Text"},"schema:domainIncludes":[{"@id":"unece:InspectionReference"},{"@id":"unece:LaboratoryObservationReference"}],"rdfs:comment":"A comment, expressed as text for this MDH illness."},{"@id":"unece:propertyReferenceCode","@type":["rdf:Property","owl:DatatypeProperty"],"rdfs:label":"propertyReferenceCode","schema:rangeIncludes":{"@id":"schema:Text"},"schema:domainIncludes":[{"@id":"unece:InspectionReference"},{"@id":"unece:LaboratoryObservationReference"},{"@id":"unece:InspectionInstructions"},{"@id":"unece:LaboratoryObservationInstructions"}],"rdfs:comment":"A code specifying a property reference for this supply chain reference."},{"@id":"unece:acceptedIndicator","@type":["rdf:Property","owl:DatatypeProperty"],"rdfs:label":"acceptedIndicator","schema:rangeIncludes":{"@id":"schema:Boolean"},"schema:domainIncludes":{"@id":"unece:ProtectionMeans"},"rdfs:comment":"The indication of whether or not this disease protection means is accepted."},{"@id":"unece:item","@type":["rdf:Property","owl:DatatypeProperty"],"rdfs:label":"item","schema:rangeIncludes":{"@id":"schema:Text"},"schema:domainIncludes":{"@id":"unece:ProtectionMeans"},"rdfs:comment":"An item, expressed as text, for this disease protection means."},{"@id":"unece:restriction","@type":["rdf:Property","owl:DatatypeProperty"],"rdfs:label":"restriction","schema:rangeIncludes":{"@id":"schema:Text"},"schema:domainIncludes":{"@id":"unece:ProtectionMeans"},"rdfs:comment":"A restriction, expressed as text, for this disease protection means."},{"@id":"unece:accreditingBodyName","@type":["rdf:Property","owl:DatatypeProperty"],"rdfs:label":"accreditingBodyName","schema:rangeIncludes":{"@id":"schema:Text"},"schema:domainIncludes":{"@id":"unece:Accreditation"},"rdfs:comment":"The name of the accrediting body, expressed as text, for this certified accreditation."},{"@id":"unece:authenticationMethodCode","@type":["rdf:Property","owl:DatatypeProperty"],"rdfs:label":"authenticationMethodCode","schema:rangeIncludes":{"@id":"schema:Text"},"schema:domainIncludes":{"@id":"unece:Accreditation"},"rdfs:comment":"A code specifying an authentication method for this certified accreditation."},{"@id":"unece:obtainedDateTime","@type":["rdf:Property","owl:DatatypeProperty"],"rdfs:label":"obtainedDateTime","schema:rangeIncludes":{"@id":"schema:DateTime"},"schema:domainIncludes":{"@id":"unece:Accreditation"},"rdfs:comment":"The date, time, date time or other date time value when this certified accreditation was obtained."},{"@id":"unece:amendmentReasonCode","@type":["rdf:Property","owl:DatatypeProperty"],"rdfs:label":"amendmentReasonCode","schema:rangeIncludes":{"@id":"schema:Text"},"schema:domainIncludes":{"@id":"unece:RegulatoryProcedure"},"rdfs:comment":"A code specifying a reason for an amendment to this cross-border regulatory procedure."},{"@id":"unece:annualQuotaQuantity","@type":["rdf:Property","owl:ObjectProperty"],"rdfs:label":"annualQuotaQuantity","schema:rangeIncludes":{"@id":"unece:QuantityType"},"schema:domainIncludes":{"@id":"unece:RegulatoryProcedure"},"rdfs:comment":""},{"@id":"unece:applicableCurrencyExchange","@type":["rdf:Property","owl:ObjectProperty"],"rdfs:label":"applicableCurrencyExchange","schema:rangeIncludes":{"@id":"undefined:CurrencyExchange"},"schema:domainIncludes":{"@id":"unece:RegulatoryProcedure"},"owl:sameAs":{"@id":"undefined:applicableCurrencyExchange"},"rdfs:comment":"The conversion of one currency to another for trade purposes."},{"@id":"unece:applicablePeriod","@type":["rdf:Property","owl:ObjectProperty"],"rdfs:label":"applicablePeriod","schema:rangeIncludes":{"@id":"unece:SpecifiedPeriod"},"schema:domainIncludes":{"@id":"unece:RegulatoryProcedure"},"rdfs:comment":"A specified period of time."},{"@id":"unece:applicableTax","@type":["rdf:Property","owl:ObjectProperty"],"rdfs:label":"applicableTax","schema:rangeIncludes":{"@id":"undefined:Tax"},"schema:domainIncludes":{"@id":"unece:RegulatoryProcedure"},"owl:sameAs":{"@id":"undefined:applicableTax"},"rdfs:comment":"A trade related fiscal levy or duty."},{"@id":"unece:borderClearanceInstructions","@type":["rdf:Property","owl:ObjectProperty"],"rdfs:label":"borderClearanceInstructions","schema:rangeIncludes":{"@id":"unece:TransportInstructions"},"schema:domainIncludes":{"@id":"unece:RegulatoryProcedure"},"rdfs:comment":"Border clearance instructions for this cross-border regulatory procedure."},{"@id":"unece:certificationBasis","@type":["rdf:Property","owl:DatatypeProperty"],"rdfs:label":"certificationBasis","schema:rangeIncludes":{"@id":"schema:Text"},"schema:domainIncludes":{"@id":"unece:RegulatoryProcedure"},"rdfs:comment":"A basis for a certification, expressed as text, for this cross-border regulatory procedure."},{"@id":"unece:consignmentDestinationSpecifiedLocation","@type":["rdf:Property","owl:ObjectProperty"],"rdfs:label":"consignmentDestinationSpecifiedLocation","schema:rangeIncludes":{"@id":"unece:Location"},"schema:domainIncludes":{"@id":"unece:RegulatoryProcedure"},"rdfs:comment":"A reference to a physical location or place."},{"@id":"unece:controlResult","@type":["rdf:Property","owl:DatatypeProperty"],"rdfs:label":"controlResult","schema:rangeIncludes":{"@id":"schema:Text"},"schema:domainIncludes":{"@id":"unece:RegulatoryProcedure"},"rdfs:comment":"A control result, expressed as text, for this cross-border regulatory procedure."},{"@id":"unece:controlStartDateConfirmationIndicator","@type":["rdf:Property","owl:DatatypeProperty"],"rdfs:label":"controlStartDateConfirmationIndicator","schema:rangeIncludes":{"@id":"schema:Boolean"},"schema:domainIncludes":{"@id":"unece:RegulatoryProcedure"},"rdfs:comment":"The indication of whether or not the start date of a control has been confirmed for this cross-border regulatory procedure."},{"@id":"unece:crossBorderRegulatoryProcedurePaymentMethodCode","@type":["rdf:Property","owl:DatatypeProperty"],"rdfs:label":"crossBorderRegulatoryProcedurePaymentMethodCode","schema:rangeIncludes":{"@id":"undefined:PaymentMethodCodeList"},"schema:domainIncludes":{"@id":"unece:RegulatoryProcedure"},"rdfs:comment":"The code specifying the payment method for this cross-border regulatory procedure, such as by deferred payment method."},{"@id":"unece:crossBorderRegulatoryProcedureTypeCode","@type":["rdf:Property","owl:DatatypeProperty"],"rdfs:label":"crossBorderRegulatoryProcedureTypeCode","schema:rangeIncludes":{"@id":"schema:Text"},"schema:domainIncludes":{"@id":"unece:RegulatoryProcedure"},"rdfs:comment":"A code specifying a type of cross-border regulatory procedure."},{"@id":"unece:customsProcedureGuaranteeCode","@type":["rdf:Property","owl:DatatypeProperty"],"rdfs:label":"customsProcedureGuaranteeCode","schema:rangeIncludes":{"@id":"undefined:CustomsProcedureGuaranteeCodeList"},"schema:domainIncludes":{"@id":"unece:RegulatoryProcedure"},"rdfs:comment":"The code specifying an undertaking given in cash, bond or as a written guarantee to ensure that an obligation will be fulfilled for this cross-border regulatory procedure."},{"@id":"unece:declarantAssignedDeclarationId","@type":["rdf:Property","owl:DatatypeProperty"],"rdfs:label":"declarantAssignedDeclarationId","schema:rangeIncludes":{"@id":"schema:Text"},"schema:domainIncludes":{"@id":"unece:RegulatoryProcedure"},"rdfs:comment":"The declarant assigned identifier of a declaration for this cross-border regulatory procedure."},{"@id":"unece:declarationLodgementLocation","@type":["rdf:Property","owl:ObjectProperty"],"rdfs:label":"declarationLodgementLocation","schema:rangeIncludes":{"@id":"unece:Location"},"schema:domainIncludes":{"@id":"unece:RegulatoryProcedure"},"rdfs:comment":"A reference to a physical location or place."},{"@id":"unece:deferredPayableTotalChargeAmount","@type":["rdf:Property","owl:ObjectProperty"],"rdfs:label":"deferredPayableTotalChargeAmount","schema:rangeIncludes":{"@id":"unece:AmountType"},"schema:domainIncludes":{"@id":"unece:RegulatoryProcedure"},"rdfs:comment":""},{"@id":"unece:deferredPaymentMethodIndicator","@type":["rdf:Property","owl:DatatypeProperty"],"rdfs:label":"deferredPaymentMethodIndicator","schema:rangeIncludes":{"@id":"schema:Boolean"},"schema:domainIncludes":{"@id":"unece:RegulatoryProcedure"},"rdfs:comment":"The indication of whether or not the deferred payment method is applicable to this cross-border regulatory procedure."},{"@id":"unece:document","@type":["rdf:Property","owl:ObjectProperty"],"rdfs:label":"document","schema:rangeIncludes":{"@id":"unece:Document"},"schema:domainIncludes":{"@id":"unece:RegulatoryProcedure"},"rdfs:comment":"Written, printed or electronic matter that is referenced."},{"@id":"unece:entryCustomsOfficeSpecifiedLocation","@type":["rdf:Property","owl:ObjectProperty"],"rdfs:label":"entryCustomsOfficeSpecifiedLocation","schema:rangeIncludes":{"@id":"unece:Location"},"schema:domainIncludes":{"@id":"unece:RegulatoryProcedure"},"rdfs:comment":"A reference to a physical location or place."},{"@id":"unece:examinationEvent","@type":["rdf:Property","owl:ObjectProperty"],"rdfs:label":"examinationEvent","schema:rangeIncludes":{"@id":"unece:Event"},"schema:domainIncludes":{"@id":"unece:RegulatoryProcedure"},"rdfs:comment":"A significant occurrence or happening during transport.,A referenced significant occurrence or happening during transport."},{"@id":"unece:exemptionClaimantParty","@type":["rdf:Property","owl:ObjectProperty"],"rdfs:label":"exemptionClaimantParty","schema:rangeIncludes":{"@id":"unece:Party"},"schema:domainIncludes":{"@id":"unece:RegulatoryProcedure"},"rdfs:comment":""},{"@id":"unece:exitCustomsOfficeSpecifiedLocation","@type":["rdf:Property","owl:ObjectProperty"],"rdfs:label":"exitCustomsOfficeSpecifiedLocation","schema:rangeIncludes":{"@id":"unece:Location"},"schema:domainIncludes":{"@id":"unece:RegulatoryProcedure"},"rdfs:comment":"A reference to a physical location or place."},{"@id":"unece:exportCustomsOfficeSpecifiedLocation","@type":["rdf:Property","owl:ObjectProperty"],"rdfs:label":"exportCustomsOfficeSpecifiedLocation","schema:rangeIncludes":{"@id":"unece:Location"},"schema:domainIncludes":{"@id":"unece:RegulatoryProcedure"},"rdfs:comment":"A reference to a physical location or place."},{"@id":"unece:exportLicenceControlClassificationId","@type":["rdf:Property","owl:DatatypeProperty"],"rdfs:label":"exportLicenceControlClassificationId","schema:rangeIncludes":{"@id":"schema:Text"},"schema:domainIncludes":{"@id":"unece:RegulatoryProcedure"},"rdfs:comment":"The identifier of the export licence classification for control purposes relevant to this cross-border regulatory procedure, such as per the Wassenaar agreement concerning trade in weapons and dual-use goods and technologies."},{"@id":"unece:freeTradeAgreementName","@type":["rdf:Property","owl:DatatypeProperty"],"rdfs:label":"freeTradeAgreementName","schema:rangeIncludes":{"@id":"schema:Text"},"schema:domainIncludes":{"@id":"unece:RegulatoryProcedure"},"rdfs:comment":"The name of a free trade agreement, expressed as text, for this cross-border regulatory procedure."},{"@id":"unece:goodsStatusCode","@type":["rdf:Property","owl:DatatypeProperty"],"rdfs:label":"goodsStatusCode","schema:rangeIncludes":{"@id":"schema:Text"},"schema:domainIncludes":{"@id":"unece:RegulatoryProcedure"},"rdfs:comment":"The code specifying the goods status for this cross-border regulatory procedure."},{"@id":"unece:governmentActionResponsibleAgencyActionCode","@type":["rdf:Property","owl:DatatypeProperty"],"rdfs:label":"governmentActionResponsibleAgencyActionCode","schema:rangeIncludes":{"@id":"unece:GovernmentActionCodeList"},"schema:domainIncludes":{"@id":"unece:RegulatoryProcedure"},"rdfs:comment":"A code specifying an action for a responsible agency in this cross-border regulatory procedure."},{"@id":"unece:guarantee","@type":["rdf:Property","owl:DatatypeProperty"],"rdfs:label":"guarantee","schema:rangeIncludes":{"@id":"schema:Text"},"schema:domainIncludes":{"@id":"unece:RegulatoryProcedure"},"rdfs:comment":"The undertaking, expressed as text, given in cash, bond or as a written guarantee to ensure that an obligation will be fulfilled for this cross-border regulatory procedure."},{"@id":"unece:immediatePayableTotalChargeAmount","@type":["rdf:Property","owl:ObjectProperty"],"rdfs:label":"immediatePayableTotalChargeAmount","schema:rangeIncludes":{"@id":"unece:AmountType"},"schema:domainIncludes":{"@id":"unece:RegulatoryProcedure"},"rdfs:comment":""},{"@id":"unece:importCustomsOfficeSpecifiedLocation","@type":["rdf:Property","owl:ObjectProperty"],"rdfs:label":"importCustomsOfficeSpecifiedLocation","schema:rangeIncludes":{"@id":"unece:Location"},"schema:domainIncludes":{"@id":"unece:RegulatoryProcedure"},"rdfs:comment":"A reference to a physical location or place."},{"@id":"unece:nonTariffChargeAmount","@type":["rdf:Property","owl:ObjectProperty"],"rdfs:label":"nonTariffChargeAmount","schema:rangeIncludes":{"@id":"unece:AmountType"},"schema:domainIncludes":{"@id":"unece:RegulatoryProcedure"},"rdfs:comment":""},{"@id":"unece:originCriteria","@type":["rdf:Property","owl:DatatypeProperty"],"rdfs:label":"originCriteria","schema:rangeIncludes":{"@id":"schema:Text"},"schema:domainIncludes":{"@id":"unece:RegulatoryProcedure"},"rdfs:comment":"The origin criteria, expressed as text, for this cross-border regulatory procedure."},{"@id":"unece:paymentOfficeLocation","@type":["rdf:Property","owl:ObjectProperty"],"rdfs:label":"paymentOfficeLocation","schema:rangeIncludes":{"@id":"unece:Location"},"schema:domainIncludes":{"@id":"unece:RegulatoryProcedure"},"rdfs:comment":"A reference to a physical location or place."},{"@id":"unece:performanceDateTime","@type":["rdf:Property","owl:DatatypeProperty"],"rdfs:label":"performanceDateTime","schema:rangeIncludes":{"@id":"schema:Text"},"schema:domainIncludes":{"@id":"unece:RegulatoryProcedure"},"rdfs:comment":"A date, time, date time, or other date time value on which this cross-border regulatory procedure was, or will be, performed."},{"@id":"unece:previousDocument","@type":["rdf:Property","owl:ObjectProperty"],"rdfs:label":"previousDocument","schema:rangeIncludes":{"@id":"unece:Document"},"schema:domainIncludes":{"@id":"unece:RegulatoryProcedure"},"rdfs:comment":"Written, printed or electronic matter that is referenced."},{"@id":"unece:previousProcedureTypeCode","@type":["rdf:Property","owl:DatatypeProperty"],"rdfs:label":"previousProcedureTypeCode","schema:rangeIncludes":{"@id":"schema:Text"},"schema:domainIncludes":{"@id":"unece:RegulatoryProcedure"},"rdfs:comment":"A code specifying a type of previous procedure for this cross-border regulatory procedure."},{"@id":"unece:quotaId","@type":["rdf:Property","owl:DatatypeProperty"],"rdfs:label":"quotaId","schema:rangeIncludes":{"@id":"schema:Text"},"schema:domainIncludes":{"@id":"unece:RegulatoryProcedure"},"rdfs:comment":"A quota identifier for this cross-border regulatory procedure."},{"@id":"unece:registeredDeferredPaymentPayerId","@type":["rdf:Property","owl:DatatypeProperty"],"rdfs:label":"registeredDeferredPaymentPayerId","schema:rangeIncludes":{"@id":"schema:Text"},"schema:domainIncludes":{"@id":"unece:RegulatoryProcedure"},"rdfs:comment":"The identifier of the registered deferred payment payer for this cross-border regulatory procedure."},{"@id":"unece:requestOverrideCode","@type":["rdf:Property","owl:DatatypeProperty"],"rdfs:label":"requestOverrideCode","schema:rangeIncludes":{"@id":"schema:Text"},"schema:domainIncludes":{"@id":"unece:RegulatoryProcedure"},"rdfs:comment":"A code specifying a request, including a reason, to override previously submitted information for this cross-border regulatory procedure, such as due to an error condition."},{"@id":"unece:requiredChemicalTreatment","@type":["rdf:Property","owl:ObjectProperty"],"rdfs:label":"requiredChemicalTreatment","schema:rangeIncludes":{"@id":"unece:AppliedChemicalTreatment"},"schema:domainIncludes":{"@id":"unece:RegulatoryProcedure"},"rdfs:comment":"A chemical treatment applied as required by this cross-border regulatory procedure."},{"@id":"unece:requiredSeal","@type":["rdf:Property","owl:ObjectProperty"],"rdfs:label":"requiredSeal","schema:rangeIncludes":{"@id":"unece:Seal"},"schema:domainIncludes":{"@id":"unece:RegulatoryProcedure"},"rdfs:comment":"A seal required by this cross-border regulatory procedure."},{"@id":"unece:requiredTestSpecificationReport","@type":["rdf:Property","owl:ObjectProperty"],"rdfs:label":"requiredTestSpecificationReport","schema:rangeIncludes":{"@id":"unece:TestSpecificationReport"},"schema:domainIncludes":{"@id":"unece:RegulatoryProcedure"},"rdfs:comment":"A report of a certification test and its attributes that is required for this cross-border regulatory procedure."},{"@id":"unece:responsibleGovernmentAgencyInvolvementResponsibleAgencyInvolvementCode","@type":["rdf:Property","owl:DatatypeProperty"],"rdfs:label":"responsibleGovernmentAgencyInvolvementResponsibleAgencyInvolvementCode","schema:rangeIncludes":{"@id":"unece:ResponsibleGovernmentAgencyInvolvementCodeList"},"schema:domainIncludes":{"@id":"unece:RegulatoryProcedure"},"rdfs:comment":"A code specifying a responsible agency involved in this cross-border regulatory procedure."},{"@id":"unece:responsibleGovernmentAgencyResponsibleAgencyCode","@type":["rdf:Property","owl:DatatypeProperty"],"rdfs:label":"responsibleGovernmentAgencyResponsibleAgencyCode","schema:rangeIncludes":{"@id":"unece:ResponsibleGovernmentAgencyCodeList"},"schema:domainIncludes":{"@id":"unece:RegulatoryProcedure"},"rdfs:comment":"The code specifying the agency responsible for this cross-border regulatory procedure."},{"@id":"unece:specifiedDebtorFinancialAccount","@type":["rdf:Property","owl:ObjectProperty"],"rdfs:label":"specifiedDebtorFinancialAccount","schema:rangeIncludes":{"@id":"undefined:DebtorFinancialAccount"},"schema:domainIncludes":{"@id":"unece:RegulatoryProcedure"},"owl:sameAs":{"@id":"undefined:specifiedDebtorFinancialAccount"},"rdfs:comment":"A specific business arrangement whereby debits arising from transactions are recorded."},{"@id":"unece:statementNote","@type":["rdf:Property","owl:ObjectProperty"],"rdfs:label":"statementNote","schema:rangeIncludes":{"@id":"unece:Note"},"schema:domainIncludes":{"@id":"unece:RegulatoryProcedure"},"rdfs:comment":"A textual or coded description, such as a remark or additional information."},{"@id":"unece:tariffAmount","@type":["rdf:Property","owl:ObjectProperty"],"rdfs:label":"tariffAmount","schema:rangeIncludes":{"@id":"unece:AmountType"},"schema:domainIncludes":{"@id":"unece:RegulatoryProcedure"},"rdfs:comment":""},{"@id":"unece:tariffDeductionQuantity","@type":["rdf:Property","owl:ObjectProperty"],"rdfs:label":"tariffDeductionQuantity","schema:rangeIncludes":{"@id":"unece:QuantityType"},"schema:domainIncludes":{"@id":"unece:RegulatoryProcedure"},"rdfs:comment":""},{"@id":"unece:tariffQuantity","@type":["rdf:Property","owl:ObjectProperty"],"rdfs:label":"tariffQuantity","schema:rangeIncludes":{"@id":"unece:QuantityType"},"schema:domainIncludes":{"@id":"unece:RegulatoryProcedure"},"rdfs:comment":""},{"@id":"unece:totalChargeAmount","@type":["rdf:Property","owl:ObjectProperty"],"rdfs:label":"totalChargeAmount","schema:rangeIncludes":{"@id":"unece:AmountType"},"schema:domainIncludes":{"@id":"unece:RegulatoryProcedure"},"rdfs:comment":""},{"@id":"unece:totalConsignmentValueAmount","@type":["rdf:Property","owl:ObjectProperty"],"rdfs:label":"totalConsignmentValueAmount","schema:rangeIncludes":{"@id":"unece:AmountType"},"schema:domainIncludes":{"@id":"unece:RegulatoryProcedure"},"rdfs:comment":""},{"@id":"unece:transactionNatureCode","@type":["rdf:Property","owl:DatatypeProperty"],"rdfs:label":"transactionNatureCode","schema:rangeIncludes":{"@id":"schema:Text"},"schema:domainIncludes":{"@id":"unece:RegulatoryProcedure"},"rdfs:comment":"A code specifying the nature of a transaction for this cross-border regulatory procedure."},{"@id":"unece:transitCustomsOfficeSpecifiedLocation","@type":["rdf:Property","owl:ObjectProperty"],"rdfs:label":"transitCustomsOfficeSpecifiedLocation","schema:rangeIncludes":{"@id":"unece:Location"},"schema:domainIncludes":{"@id":"unece:RegulatoryProcedure"},"rdfs:comment":"A reference to a physical location or place."},{"@id":"unece:transitReleaseCustomsOfficeSpecifiedLocation","@type":["rdf:Property","owl:ObjectProperty"],"rdfs:label":"transitReleaseCustomsOfficeSpecifiedLocation","schema:rangeIncludes":{"@id":"unece:Location"},"schema:domainIncludes":{"@id":"unece:RegulatoryProcedure"},"rdfs:comment":"A reference to a physical location or place."},{"@id":"unece:transportMovementTypeCode","@type":["rdf:Property","owl:DatatypeProperty"],"rdfs:label":"transportMovementTypeCode","schema:rangeIncludes":{"@id":"unece:TransportMovementTypeCodeList"},"schema:domainIncludes":{"@id":"unece:RegulatoryProcedure"},"rdfs:comment":"A code specifying the transport movement type, such as import, export, transit, for this cross-border regulatory procedure."},{"@id":"unece:treatmentEvent","@type":["rdf:Property","owl:ObjectProperty"],"rdfs:label":"treatmentEvent","schema:rangeIncludes":{"@id":"unece:Event"},"schema:domainIncludes":{"@id":"unece:RegulatoryProcedure"},"rdfs:comment":"A significant occurrence or happening during transport.,A referenced significant occurrence or happening during transport."},{"@id":"unece:usedToDateQuotaQuantity","@type":["rdf:Property","owl:ObjectProperty"],"rdfs:label":"usedToDateQuotaQuantity","schema:rangeIncludes":{"@id":"unece:QuantityType"},"schema:domainIncludes":{"@id":"unece:RegulatoryProcedure"},"rdfs:comment":""},{"@id":"unece:valuationBasisAmount","@type":["rdf:Property","owl:ObjectProperty"],"rdfs:label":"valuationBasisAmount","schema:rangeIncludes":{"@id":"unece:AmountType"},"schema:domainIncludes":{"@id":"unece:RegulatoryProcedure"},"rdfs:comment":""},{"@id":"unece:applicableOrganizationCharacteristic","@type":["rdf:Property","owl:ObjectProperty"],"rdfs:label":"applicableOrganizationCharacteristic","schema:rangeIncludes":{"@id":"unece:OrganizationCharacteristic"},"schema:domainIncludes":{"@id":"unece:OrganizationalCertificate"},"rdfs:comment":"A characteristic applicable to this organization certificate."},{"@id":"unece:applicableOrganizationalCertification","@type":["rdf:Property","owl:ObjectProperty"],"rdfs:label":"applicableOrganizationalCertification","schema:rangeIncludes":{"@id":"unece:OrganizationalCertification"},"schema:domainIncludes":{"@id":"unece:OrganizationalCertificate"},"rdfs:comment":"An organizational certification applicable to this organizational certificate."},{"@id":"unece:applicableProcessCertification","@type":["rdf:Property","owl:ObjectProperty"],"rdfs:label":"applicableProcessCertification","schema:rangeIncludes":{"@id":"unece:ProcessCertification"},"schema:domainIncludes":{"@id":"unece:ProcessCertificate"},"rdfs:comment":"A process certification applicable to this process certificate."},{"@id":"unece:applicableProcessCharacteristic","@type":["rdf:Property","owl:ObjectProperty"],"rdfs:label":"applicableProcessCharacteristic","schema:rangeIncludes":{"@id":"unece:ProcessCharacteristic"},"schema:domainIncludes":{"@id":"unece:ProcessCertificate"},"rdfs:comment":"A process characteristic applicable to this process certificate."},{"@id":"unece:applicableProductCharacteristic","@type":["rdf:Property","owl:ObjectProperty"],"rdfs:label":"applicableProductCharacteristic","schema:rangeIncludes":{"@id":"unece:ProductCharacteristic"},"schema:domainIncludes":[{"@id":"unece:ProductBatchCertificate"},{"@id":"unece:ProductCertificate"},{"@id":"unece:Chemical"},{"@id":"unece:HazardousMaterial"},{"@id":"unece:SpecifiedMaterial"}],"rdfs:comment":"A characteristic applicable to this trade product."},{"@id":"unece:applicableTradeProductCertification","@type":["rdf:Property","owl:ObjectProperty"],"rdfs:label":"applicableTradeProductCertification","schema:rangeIncludes":{"@id":"unece:TradeProductCertification"},"schema:domainIncludes":[{"@id":"unece:ProductBatchCertificate"},{"@id":"unece:ProductCertificate"},{"@id":"unece:SpecifiedMaterial"}],"rdfs:comment":"A certification applicable to this trade product."},{"@id":"unece:aliasNameCode","@type":["rdf:Property","owl:DatatypeProperty"],"rdfs:label":"aliasNameCode","schema:rangeIncludes":{"@id":"schema:Text"},"schema:domainIncludes":{"@id":"unece:SpecifiedCertificate"},"rdfs:comment":"A code specifying an alias name of this specified certificate."},{"@id":"unece:applicableClause","@type":["rdf:Property","owl:ObjectProperty"],"rdfs:label":"applicableClause","schema:rangeIncludes":{"@id":"unece:Clause"},"schema:domainIncludes":{"@id":"unece:SpecifiedCertificate"},"rdfs:comment":"A distinct article or provision in a document, which requires compliance."},{"@id":"unece:applicableGeographicRegion","@type":["rdf:Property","owl:DatatypeProperty"],"rdfs:label":"applicableGeographicRegion","schema:rangeIncludes":{"@id":"schema:Text"},"schema:domainIncludes":{"@id":"unece:SpecifiedCertificate"},"rdfs:comment":"A geographic region, expressed as text, applicable for this specified certificate."},{"@id":"unece:assuranceLevelCode","@type":["rdf:Property","owl:DatatypeProperty"],"rdfs:label":"assuranceLevelCode","schema:rangeIncludes":{"@id":"schema:Text"},"schema:domainIncludes":[{"@id":"unece:SpecifiedCertificate"},{"@id":"unece:Assessment"},{"@id":"unece:Licence"},{"@id":"unece:SpecifiedDeclaration"}],"rdfs:comment":"A code specifying an assurance level of this specified declaration."},{"@id":"unece:availableLanguageCode","@type":["rdf:Property","owl:DatatypeProperty"],"rdfs:label":"availableLanguageCode","schema:rangeIncludes":{"@id":"unece:LanguageCodeList"},"schema:domainIncludes":{"@id":"unece:SpecifiedCertificate"},"rdfs:comment":"A code specifying an available language for this specified certificate."},{"@id":"unece:capabilityLevel","@type":["rdf:Property","owl:DatatypeProperty"],"rdfs:label":"capabilityLevel","schema:rangeIncludes":{"@id":"schema:Text"},"schema:domainIncludes":{"@id":"unece:SpecifiedCertificate"},"rdfs:comment":"A capability level, expressed as text, for this specified experience item."},{"@id":"unece:certifiedObject","@type":["rdf:Property","owl:ObjectProperty"],"rdfs:label":"certifiedObject","schema:rangeIncludes":{"@id":"unece:Object"},"schema:domainIncludes":{"@id":"unece:SpecifiedCertificate"},"rdfs:comment":"Anything that is visible or tangible, such as a product, process, or organization."},{"@id":"unece:certifiedParty","@type":["rdf:Property","owl:ObjectProperty"],"rdfs:label":"certifiedParty","schema:rangeIncludes":{"@id":"unece:Party"},"schema:domainIncludes":{"@id":"unece:SpecifiedCertificate"},"rdfs:comment":""},{"@id":"unece:certifiedPersonQuantity","@type":["rdf:Property","owl:ObjectProperty"],"rdfs:label":"certifiedPersonQuantity","schema:rangeIncludes":{"@id":"unece:QuantityType"},"schema:domainIncludes":{"@id":"unece:SpecifiedCertificate"},"rdfs:comment":""},{"@id":"unece:effectiveFromDateTime","@type":["rdf:Property","owl:DatatypeProperty"],"rdfs:label":"effectiveFromDateTime","schema:rangeIncludes":{"@id":"schema:DateTime"},"schema:domainIncludes":{"@id":"unece:SpecifiedCertificate"},"rdfs:comment":"The date, time, date time, or other date time value from which this specified certificate is effective."},{"@id":"unece:endorsementDateTime","@type":["rdf:Property","owl:DatatypeProperty"],"rdfs:label":"endorsementDateTime","schema:rangeIncludes":{"@id":"schema:DateTime"},"schema:domainIncludes":{"@id":"unece:SpecifiedCertificate"},"rdfs:comment":"An endorsement date, time, date time or other date time value for this specified certificate."},{"@id":"unece:issuanceLocation","@type":["rdf:Property","owl:ObjectProperty"],"rdfs:label":"issuanceLocation","schema:rangeIncludes":{"@id":"unece:Location"},"schema:domainIncludes":{"@id":"unece:SpecifiedCertificate"},"rdfs:comment":"A reference to a physical location or place."},{"@id":"unece:latestEndorsementDateTime","@type":["rdf:Property","owl:DatatypeProperty"],"rdfs:label":"latestEndorsementDateTime","schema:rangeIncludes":{"@id":"schema:DateTime"},"schema:domainIncludes":{"@id":"unece:SpecifiedCertificate"},"rdfs:comment":"A latest endorsement date, time, date time or other date time value for this specified certificate."},{"@id":"unece:partyId","@type":["rdf:Property","owl:DatatypeProperty"],"rdfs:label":"partyId","schema:rangeIncludes":{"@id":"schema:Text"},"schema:domainIncludes":{"@id":"unece:SpecifiedCertificate"},"rdfs:comment":"An identifier of a party for this specified certificate."},{"@id":"unece:providingParty","@type":["rdf:Property","owl:ObjectProperty"],"rdfs:label":"providingParty","schema:rangeIncludes":{"@id":"unece:Party"},"schema:domainIncludes":{"@id":"unece:SpecifiedCertificate"},"rdfs:comment":""},{"@id":"unece:reportedDocumentStatus","@type":["rdf:Property","owl:ObjectProperty"],"rdfs:label":"reportedDocumentStatus","schema:rangeIncludes":{"@id":"unece:DocumentStatus"},"schema:domainIncludes":{"@id":"unece:SpecifiedCertificate"},"rdfs:comment":"The information relevant to a condition related to a document."},{"@id":"unece:requiredIndicator","@type":["rdf:Property","owl:DatatypeProperty"],"rdfs:label":"requiredIndicator","schema:rangeIncludes":{"@id":"schema:Boolean"},"schema:domainIncludes":{"@id":"unece:SpecifiedCertificate"},"rdfs:comment":"The indication of whether or not this specified certificate is required."},{"@id":"unece:subjectTypeCode","@type":["rdf:Property","owl:DatatypeProperty"],"rdfs:label":"subjectTypeCode","schema:rangeIncludes":{"@id":"schema:Text"},"schema:domainIncludes":[{"@id":"unece:SpecifiedCertificate"},{"@id":"unece:Licence"},{"@id":"unece:SpecifiedDeclaration"}],"rdfs:comment":"A code specifying a subject type for this licence."},{"@id":"unece:validIndicator","@type":["rdf:Property","owl:DatatypeProperty"],"rdfs:label":"validIndicator","schema:rangeIncludes":{"@id":"schema:Boolean"},"schema:domainIncludes":[{"@id":"unece:SpecifiedCertificate"},{"@id":"unece:Licence"}],"rdfs:comment":"The indication of whether or not this specified certificate is valid."},{"@id":"unece:validityExtendedUntilDateTime","@type":["rdf:Property","owl:DatatypeProperty"],"rdfs:label":"validityExtendedUntilDateTime","schema:rangeIncludes":{"@id":"schema:DateTime"},"schema:domainIncludes":{"@id":"unece:SpecifiedCertificate"},"rdfs:comment":"A date, time, date time or other date time value until which this specified certificate will remain valid under the terms of an approved extension period."},{"@id":"unece:validityTypeCode","@type":["rdf:Property","owl:DatatypeProperty"],"rdfs:label":"validityTypeCode","schema:rangeIncludes":{"@id":"schema:Text"},"schema:domainIncludes":{"@id":"unece:SpecifiedCertificate"},"rdfs:comment":"A code specifying a type of validity for this specified certificate."},{"@id":"unece:actualObservationEndDateTime","@type":["rdf:Property","owl:DatatypeProperty"],"rdfs:label":"actualObservationEndDateTime","schema:rangeIncludes":{"@id":"schema:Text"},"schema:domainIncludes":{"@id":"unece:ObservationResult"},"rdfs:comment":"The date, time, date time, or other date time value for the end of the observation for this sample observation result."},{"@id":"unece:actualObservationStartDateTime","@type":["rdf:Property","owl:DatatypeProperty"],"rdfs:label":"actualObservationStartDateTime","schema:rangeIncludes":{"@id":"schema:Text"},"schema:domainIncludes":{"@id":"unece:ObservationResult"},"rdfs:comment":"The date, time, date time, or other date time value for the start of the observation for this sample observation result."},{"@id":"unece:applicableMethod","@type":["rdf:Property","owl:ObjectProperty"],"rdfs:label":"applicableMethod","schema:rangeIncludes":{"@id":"unece:SpecifiedMethod"},"schema:domainIncludes":[{"@id":"unece:ObservationResult"},{"@id":"unece:InspectionResult"},{"@id":"unece:InspectionResultCharacteristic"}],"rdfs:comment":"A defined way of performing something."},{"@id":"unece:attachedLaboratoryObservationNote","@type":["rdf:Property","owl:ObjectProperty"],"rdfs:label":"attachedLaboratoryObservationNote","schema:rangeIncludes":{"@id":"unece:LaboratoryObservationNote"},"schema:domainIncludes":{"@id":"unece:ObservationResult"},"rdfs:comment":"A note attached to the laboratory observation results with additional observations and or conclusions."},{"@id":"unece:authorizationParty","@type":["rdf:Property","owl:ObjectProperty"],"rdfs:label":"authorizationParty","schema:rangeIncludes":{"@id":"unece:LaboratoryObservationParty"},"schema:domainIncludes":{"@id":"unece:ObservationResult"},"rdfs:comment":"The laboratory observation party who authorized this sample observation result."},{"@id":"unece:emergencyObservationIndicator","@type":["rdf:Property","owl:DatatypeProperty"],"rdfs:label":"emergencyObservationIndicator","schema:rangeIncludes":{"@id":"schema:Boolean"},"schema:domainIncludes":{"@id":"unece:ObservationResult"},"rdfs:comment":"The indication of whether or not the observation was an emergency observation for this sample observation result."},{"@id":"unece:expectedValueSpecifiedObservationResultCharacteristic","@type":["rdf:Property","owl:ObjectProperty"],"rdfs:label":"expectedValueSpecifiedObservationResultCharacteristic","schema:rangeIncludes":{"@id":"unece:ObservationResultCharacteristic"},"schema:domainIncludes":{"@id":"unece:ObservationResult"},"rdfs:comment":"An expected value for the characteristic, to be observed or measured according to the specified type of observation for this sample observation result."},{"@id":"unece:generalCharacteristic","@type":["rdf:Property","owl:DatatypeProperty"],"rdfs:label":"generalCharacteristic","schema:rangeIncludes":{"@id":"schema:Text"},"schema:domainIncludes":[{"@id":"unece:ObservationResult"},{"@id":"unece:InspectionResult"}],"rdfs:comment":"A general characteristic, such as length, volume, density, sensitivity, conductivity, expressed as text, of this specified inspection result."},{"@id":"unece:interpretationResultApplicableParameter","@type":["rdf:Property","owl:ObjectProperty"],"rdfs:label":"interpretationResultApplicableParameter","schema:rangeIncludes":{"@id":"unece:ObservationObjectiveParameter"},"schema:domainIncludes":[{"@id":"unece:ObservationResult"},{"@id":"unece:InspectionResultCharacteristic"},{"@id":"unece:ObservationResultCharacteristic"}],"rdfs:comment":"An applicable objective observation parameter of the interpretation result for this inspection result characteristic."},{"@id":"unece:laboratoryAnalysisRequestSpecifiedReference","@type":["rdf:Property","owl:ObjectProperty"],"rdfs:label":"laboratoryAnalysisRequestSpecifiedReference","schema:rangeIncludes":{"@id":"unece:LaboratoryObservationReference"},"schema:domainIncludes":{"@id":"unece:ObservationResult"},"rdfs:comment":"A laboratory observation analysis request reference specified for this sample observation result."},{"@id":"unece:materialType","@type":["rdf:Property","owl:DatatypeProperty"],"rdfs:label":"materialType","schema:rangeIncludes":{"@id":"schema:Text"},"schema:domainIncludes":{"@id":"unece:ObservationResult"},"rdfs:comment":"The context material type of the observed sample, expressed as text, such as animal or blood."},{"@id":"unece:materialTypeCode","@type":["rdf:Property","owl:DatatypeProperty"],"rdfs:label":"materialTypeCode","schema:rangeIncludes":{"@id":"schema:Text"},"schema:domainIncludes":{"@id":"unece:ObservationResult"},"rdfs:comment":"The code specifying a material type for this sample observation result."},{"@id":"unece:maximumStandardValueSpecifiedObservationResultCharacteristic","@type":["rdf:Property","owl:ObjectProperty"],"rdfs:label":"maximumStandardValueSpecifiedObservationResultCharacteristic","schema:rangeIncludes":{"@id":"unece:ObservationResultCharacteristic"},"schema:domainIncludes":{"@id":"unece:ObservationResult"},"rdfs:comment":"A maximum standard value of the values for the characteristic observed or measured by using the specified type of observation for this sample observation result."},{"@id":"unece:minimumStandardValueSpecifiedObservationResultCharacteristic","@type":["rdf:Property","owl:ObjectProperty"],"rdfs:label":"minimumStandardValueSpecifiedObservationResultCharacteristic","schema:rangeIncludes":{"@id":"unece:ObservationResultCharacteristic"},"schema:domainIncludes":{"@id":"unece:ObservationResult"},"rdfs:comment":"A minimum standard value of the values for the characteristic observed or measured by using the specified type of observation for this sample observation result."},{"@id":"unece:observationDiscontinuationReason","@type":["rdf:Property","owl:DatatypeProperty"],"rdfs:label":"observationDiscontinuationReason","schema:rangeIncludes":{"@id":"schema:Text"},"schema:domainIncludes":{"@id":"unece:ObservationResult"},"rdfs:comment":"The observation discontinuation reason, expressed as text, for this sample observation result."},{"@id":"unece:observationDiscontinuationReasonCode","@type":["rdf:Property","owl:DatatypeProperty"],"rdfs:label":"observationDiscontinuationReasonCode","schema:rangeIncludes":{"@id":"schema:Text"},"schema:domainIncludes":{"@id":"unece:ObservationResult"},"rdfs:comment":"The code specifying the observation discontinuation reason for this sample observation result."},{"@id":"unece:observationTimeFrame","@type":["rdf:Property","owl:DatatypeProperty"],"rdfs:label":"observationTimeFrame","schema:rangeIncludes":{"@id":"schema:Text"},"schema:domainIncludes":{"@id":"unece:ObservationResult"},"rdfs:comment":"The observation time frame, expressed as text, for this sample observation result."},{"@id":"unece:observedValueSpecifiedObservationResultCharacteristic","@type":["rdf:Property","owl:ObjectProperty"],"rdfs:label":"observedValueSpecifiedObservationResultCharacteristic","schema:rangeIncludes":{"@id":"unece:ObservationResultCharacteristic"},"schema:domainIncludes":{"@id":"unece:ObservationResult"},"rdfs:comment":"An observed value for the characteristic, acquired by observing or measuring according to the specified type of observation for this sample observation result."},{"@id":"unece:outsourcedLaboratoryParty","@type":["rdf:Property","owl:ObjectProperty"],"rdfs:label":"outsourcedLaboratoryParty","schema:rangeIncludes":{"@id":"unece:LaboratoryObservationParty"},"schema:domainIncludes":{"@id":"unece:ObservationResult"},"rdfs:comment":"The outsourced laboratory party who performed this sample observation result."},{"@id":"unece:outsourcedObservationIndicator","@type":["rdf:Property","owl:DatatypeProperty"],"rdfs:label":"outsourcedObservationIndicator","schema:rangeIncludes":{"@id":"schema:Boolean"},"schema:domainIncludes":{"@id":"unece:ObservationResult"},"rdfs:comment":"The indication of whether or not the observation was an outsourced observation (performed by a third party)."},{"@id":"unece:shareableIndicator","@type":["rdf:Property","owl:DatatypeProperty"],"rdfs:label":"shareableIndicator","schema:rangeIncludes":{"@id":"schema:Boolean"},"schema:domainIncludes":[{"@id":"unece:ObservationResult"},{"@id":"unece:InspectionResult"},{"@id":"unece:SustainabilityCharacteristic"},{"@id":"unece:ObservationResultCharacteristic"}],"rdfs:comment":"The indication of whether or not this sample observation result characteristic is shareable."},{"@id":"unece:specifiedLaboratoryObservationInstructions","@type":["rdf:Property","owl:ObjectProperty"],"rdfs:label":"specifiedLaboratoryObservationInstructions","schema:rangeIncludes":{"@id":"unece:LaboratoryObservationInstructions"},"schema:domainIncludes":{"@id":"unece:ObservationResult"},"rdfs:comment":"A set of laboratory observation instructions specified for this sample observation result."},{"@id":"unece:specifiedLaboratoryObservationReference","@type":["rdf:Property","owl:ObjectProperty"],"rdfs:label":"specifiedLaboratoryObservationReference","schema:rangeIncludes":{"@id":"unece:LaboratoryObservationReference"},"schema:domainIncludes":{"@id":"unece:ObservationResult"},"rdfs:comment":"A laboratory observation reference specified for this sample observation result."},{"@id":"unece:usedMethod","@type":["rdf:Property","owl:ObjectProperty"],"rdfs:label":"usedMethod","schema:rangeIncludes":{"@id":"unece:LaboratoryObservationAnalysisMethod"},"schema:domainIncludes":{"@id":"unece:ObservationResult"},"rdfs:comment":"A laboratory observation analysis method used for this sample observation result."},{"@id":"unece:agencyId","@type":["rdf:Property","owl:DatatypeProperty"],"rdfs:label":"agencyId","schema:rangeIncludes":{"@id":"schema:Text"},"schema:domainIncludes":{"@id":"unece:Standard"},"rdfs:comment":"The identifier of the agency for this referenced standard."},{"@id":"unece:applicableAssessment","@type":["rdf:Property","owl:ObjectProperty"],"rdfs:label":"applicableAssessment","schema:rangeIncludes":{"@id":"unece:Assessment"},"schema:domainIncludes":[{"@id":"unece:Standard"},{"@id":"unece:SpecifiedMaterial"}],"rdfs:comment":"A specified assessment applicable to this referenced standard."},{"@id":"unece:applicableCountry","@type":["rdf:Property","owl:ObjectProperty"],"rdfs:label":"applicableCountry","schema:rangeIncludes":{"@id":"unece:Country"},"schema:domainIncludes":[{"@id":"unece:Standard"},{"@id":"unece:ProductCharacteristic"},{"@id":"unece:ProductBatchCharacteristic"}],"rdfs:comment":"The area of land that belongs to a nation together with its properties, such as population, political organization, etc., used or referenced for trade purposes."},{"@id":"unece:applicableDeclaration","@type":["rdf:Property","owl:ObjectProperty"],"rdfs:label":"applicableDeclaration","schema:rangeIncludes":{"@id":"unece:SpecifiedDeclaration"},"schema:domainIncludes":{"@id":"unece:Standard"},"rdfs:comment":"A specified declaration applicable to this production process."},{"@id":"unece:applicableLicence","@type":["rdf:Property","owl:ObjectProperty"],"rdfs:label":"applicableLicence","schema:rangeIncludes":{"@id":"unece:Licence"},"schema:domainIncludes":{"@id":"unece:Standard"},"rdfs:comment":"A specified licence applicable to this production process."},{"@id":"unece:applicableMetricCharacteristic","@type":["rdf:Property","owl:ObjectProperty"],"rdfs:label":"applicableMetricCharacteristic","schema:rangeIncludes":{"@id":"unece:MetricCharacteristic"},"schema:domainIncludes":{"@id":"unece:Standard"},"rdfs:comment":"A prominent attribute or aspect of a metric (a standard of measurement)."},{"@id":"unece:applicableSpecifiedCertificate","@type":["rdf:Property","owl:ObjectProperty"],"rdfs:label":"applicableSpecifiedCertificate","schema:rangeIncludes":{"@id":"unece:SpecifiedCertificate"},"schema:domainIncludes":[{"@id":"unece:Standard"},{"@id":"unece:SpecifiedMaterial"}],"rdfs:comment":"A certificate applicable to this product batch."},{"@id":"unece:elementVersionId","@type":["rdf:Property","owl:DatatypeProperty"],"rdfs:label":"elementVersionId","schema:rangeIncludes":{"@id":"schema:Text"},"schema:domainIncludes":{"@id":"unece:Standard"},"rdfs:comment":"The identifier of the version of a specific element within the referenced standard, such as the version of a data element."},{"@id":"unece:partId","@type":["rdf:Property","owl:DatatypeProperty"],"rdfs:label":"partId","schema:rangeIncludes":{"@id":"schema:Text"},"schema:domainIncludes":{"@id":"unece:Standard"},"rdfs:comment":"The identifier of a part of this referenced standard, such as a section or topic."},{"@id":"unece:specifiedDocument","@type":["rdf:Property","owl:ObjectProperty"],"rdfs:label":"specifiedDocument","schema:rangeIncludes":{"@id":"unece:Document"},"schema:domainIncludes":[{"@id":"unece:Standard"},{"@id":"unece:SustainabilityInspection"},{"@id":"unece:SpecifiedInspection"}],"rdfs:comment":"Written, printed or electronic matter that is referenced."},{"@id":"unece:totalQuantity","@type":["rdf:Property","owl:ObjectProperty"],"rdfs:label":"totalQuantity","schema:rangeIncludes":{"@id":"unece:QuantityType"},"schema:domainIncludes":{"@id":"unece:ProcessWorkItem"},"rdfs:comment":""},{"@id":"unece:applicableCondition","@type":["rdf:Property","owl:ObjectProperty"],"rdfs:label":"applicableCondition","schema:rangeIncludes":{"@id":"unece:ProductCharacteristicCondition"},"schema:domainIncludes":{"@id":"unece:ProductCharacteristic"},"rdfs:comment":"A condition applicable to this product characteristic."},{"@id":"unece:measurementMethodCode","@type":["rdf:Property","owl:DatatypeProperty"],"rdfs:label":"measurementMethodCode","schema:rangeIncludes":{"@id":"schema:Text"},"schema:domainIncludes":[{"@id":"unece:ProductCharacteristic"},{"@id":"unece:SustainabilityCharacteristic"},{"@id":"unece:TechnicalCharacteristic"}],"rdfs:comment":"A code specifying a measurement method for this product characteristic."},{"@id":"unece:productCharacteristicValueCode","@type":["rdf:Property","owl:DatatypeProperty"],"rdfs:label":"productCharacteristicValueCode","schema:rangeIncludes":{"@id":"schema:Text"},"schema:domainIncludes":{"@id":"unece:ProductCharacteristic"},"rdfs:comment":"The code specifying the value of this product characteristic."},{"@id":"unece:targetMarketDescription","@type":["rdf:Property","owl:DatatypeProperty"],"rdfs:label":"targetMarketDescription","schema:rangeIncludes":{"@id":"schema:Text"},"schema:domainIncludes":[{"@id":"unece:ProductCharacteristic"},{"@id":"unece:ProductBatchCharacteristic"}],"rdfs:comment":"A textual description of a target market for this product characteristic."},{"@id":"unece:valueBinaryFile","@type":["rdf:Property","owl:ObjectProperty"],"rdfs:label":"valueBinaryFile","schema:rangeIncludes":{"@id":"unece:BinaryFile"},"schema:domainIncludes":[{"@id":"unece:ProductCharacteristic"},{"@id":"unece:SustainabilityCharacteristic"}],"rdfs:comment":"A specified computer file or program stored in a binary format."},{"@id":"unece:applicableCorrectiveAction","@type":["rdf:Property","owl:ObjectProperty"],"rdfs:label":"applicableCorrectiveAction","schema:rangeIncludes":{"@id":"unece:CorrectiveAction"},"schema:domainIncludes":{"@id":"unece:InspectionResult"},"rdfs:comment":"A corrective action applicable to this specified inspection result."},{"@id":"unece:applicableInspectionResultCharacteristic","@type":["rdf:Property","owl:ObjectProperty"],"rdfs:label":"applicableInspectionResultCharacteristic","schema:rangeIncludes":{"@id":"unece:InspectionResultCharacteristic"},"schema:domainIncludes":{"@id":"unece:InspectionResult"},"rdfs:comment":"A characteristic applicable to this specified inspection result."},{"@id":"unece:applicablePreventiveAction","@type":["rdf:Property","owl:ObjectProperty"],"rdfs:label":"applicablePreventiveAction","schema:rangeIncludes":{"@id":"unece:PreventiveAction"},"schema:domainIncludes":{"@id":"unece:InspectionResult"},"rdfs:comment":"A preventive action applicable to this specified inspection result."},{"@id":"unece:applicableSpecifiedAction","@type":["rdf:Property","owl:ObjectProperty"],"rdfs:label":"applicableSpecifiedAction","schema:rangeIncludes":{"@id":"unece:SpecifiedAction"},"schema:domainIncludes":{"@id":"unece:InspectionResult"},"rdfs:comment":"The process of doing something in order to make something happen or to deal with a situation."},{"@id":"unece:approvalDateTime","@type":["rdf:Property","owl:DatatypeProperty"],"rdfs:label":"approvalDateTime","schema:rangeIncludes":{"@id":"schema:Text"},"schema:domainIncludes":{"@id":"unece:InspectionResult"},"rdfs:comment":"The date, time, date time, or other date time value for the approval of this specified inspection result."},{"@id":"unece:attachedInspectionNote","@type":["rdf:Property","owl:ObjectProperty"],"rdfs:label":"attachedInspectionNote","schema:rangeIncludes":{"@id":"unece:InspectionNote"},"schema:domainIncludes":{"@id":"unece:InspectionResult"},"rdfs:comment":"A note with additional information and or conclusions attached to this specified inspection result."},{"@id":"unece:expectedValueApplicableCharacteristic","@type":["rdf:Property","owl:ObjectProperty"],"rdfs:label":"expectedValueApplicableCharacteristic","schema:rangeIncludes":{"@id":"unece:InspectionResultCharacteristic"},"schema:domainIncludes":{"@id":"unece:InspectionResult"},"rdfs:comment":"An expected value for the inspection characteristic to be acquired by using the type of inspection applicable to this specified inspection result."},{"@id":"unece:inspectionDateTime","@type":["rdf:Property","owl:DatatypeProperty"],"rdfs:label":"inspectionDateTime","schema:rangeIncludes":{"@id":"schema:Text"},"schema:domainIncludes":{"@id":"unece:InspectionResult"},"rdfs:comment":"The date, time, date time, or other date time value of the inspection for this specified inspection result."},{"@id":"unece:inspectionParty","@type":["rdf:Property","owl:ObjectProperty"],"rdfs:label":"inspectionParty","schema:rangeIncludes":{"@id":"unece:Party"},"schema:domainIncludes":{"@id":"unece:InspectionResult"},"rdfs:comment":""},{"@id":"unece:inspectionStandard","@type":["rdf:Property","owl:ObjectProperty"],"rdfs:label":"inspectionStandard","schema:rangeIncludes":{"@id":"unece:Standard"},"schema:domainIncludes":{"@id":"unece:InspectionResult"},"rdfs:comment":"A referenced inspection standard for this specified inspection result."},{"@id":"unece:laboratoryObservationResult","@type":["rdf:Property","owl:ObjectProperty"],"rdfs:label":"laboratoryObservationResult","schema:rangeIncludes":{"@id":"unece:ObservationResult"},"schema:domainIncludes":{"@id":"unece:InspectionResult"},"rdfs:comment":"A laboratory sample observation result for this specified inspection result."},{"@id":"unece:maximumStandardValueApplicableCharacteristic","@type":["rdf:Property","owl:ObjectProperty"],"rdfs:label":"maximumStandardValueApplicableCharacteristic","schema:rangeIncludes":{"@id":"unece:InspectionResultCharacteristic"},"schema:domainIncludes":{"@id":"unece:InspectionResult"},"rdfs:comment":"A maximum standard value for the inspection characteristic observed or measured by using the type of inspection applicable to this specified inspection result."},{"@id":"unece:minimumStandardValueApplicableCharacteristic","@type":["rdf:Property","owl:ObjectProperty"],"rdfs:label":"minimumStandardValueApplicableCharacteristic","schema:rangeIncludes":{"@id":"unece:InspectionResultCharacteristic"},"schema:domainIncludes":{"@id":"unece:InspectionResult"},"rdfs:comment":"A minimum standard value for the inspection characteristic observed or measured by using the type of inspection applicable to this specified inspection result."},{"@id":"unece:observedValueApplicableCharacteristic","@type":["rdf:Property","owl:ObjectProperty"],"rdfs:label":"observedValueApplicableCharacteristic","schema:rangeIncludes":{"@id":"unece:InspectionResultCharacteristic"},"schema:domainIncludes":{"@id":"unece:InspectionResult"},"rdfs:comment":"An observed value for the inspection characteristic acquired by using the type of inspection applicable to this specified inspection result."},{"@id":"unece:obtainedAssertion","@type":["rdf:Property","owl:ObjectProperty"],"rdfs:label":"obtainedAssertion","schema:rangeIncludes":{"@id":"unece:Assertion"},"schema:domainIncludes":{"@id":"unece:InspectionResult"},"rdfs:comment":"A sustainability assertion obtained by means of this specified inspection result."},{"@id":"unece:obtainedConformanceCertificate","@type":["rdf:Property","owl:ObjectProperty"],"rdfs:label":"obtainedConformanceCertificate","schema:rangeIncludes":{"@id":"unece:ConformanceCertificate"},"schema:domainIncludes":{"@id":"unece:InspectionResult"},"rdfs:comment":"A conformance certificate obtained by means of this specified inspection result."},{"@id":"unece:obtainedOrganizationalCertificate","@type":["rdf:Property","owl:ObjectProperty"],"rdfs:label":"obtainedOrganizationalCertificate","schema:rangeIncludes":{"@id":"unece:OrganizationalCertificate"},"schema:domainIncludes":{"@id":"unece:InspectionResult"},"rdfs:comment":"An organizational certificate obtained by means of this specified inspection result."},{"@id":"unece:obtainedProcessCertificate","@type":["rdf:Property","owl:ObjectProperty"],"rdfs:label":"obtainedProcessCertificate","schema:rangeIncludes":{"@id":"unece:ProcessCertificate"},"schema:domainIncludes":{"@id":"unece:InspectionResult"},"rdfs:comment":"A process certificate obtained by means of this specified inspection result."},{"@id":"unece:obtainedProductCertificate","@type":["rdf:Property","owl:ObjectProperty"],"rdfs:label":"obtainedProductCertificate","schema:rangeIncludes":{"@id":"unece:ProductCertificate"},"schema:domainIncludes":{"@id":"unece:InspectionResult"},"rdfs:comment":"A product certificate obtained by means of this specified inspection result."},{"@id":"unece:obtainedSpecifiedCertificate","@type":["rdf:Property","owl:ObjectProperty"],"rdfs:label":"obtainedSpecifiedCertificate","schema:rangeIncludes":{"@id":"unece:SpecifiedCertificate"},"schema:domainIncludes":{"@id":"unece:InspectionResult"},"rdfs:comment":"A certificate obtained by means of this specified inspection result."},{"@id":"unece:outsourcedInspectionParty","@type":["rdf:Property","owl:ObjectProperty"],"rdfs:label":"outsourcedInspectionParty","schema:rangeIncludes":{"@id":"unece:Party"},"schema:domainIncludes":{"@id":"unece:InspectionResult"},"rdfs:comment":""},{"@id":"unece:relatedAssessment","@type":["rdf:Property","owl:ObjectProperty"],"rdfs:label":"relatedAssessment","schema:rangeIncludes":{"@id":"unece:Assessment"},"schema:domainIncludes":{"@id":"unece:InspectionResult"},"rdfs:comment":"An assessment related to this specified inspection result."},{"@id":"unece:relatedInstructions","@type":["rdf:Property","owl:ObjectProperty"],"rdfs:label":"relatedInstructions","schema:rangeIncludes":{"@id":"unece:InspectionInstructions"},"schema:domainIncludes":{"@id":"unece:InspectionResult"},"rdfs:comment":"Inspection instructions related to this specified inspection result."},{"@id":"unece:relatedMaterialType","@type":["rdf:Property","owl:DatatypeProperty"],"rdfs:label":"relatedMaterialType","schema:rangeIncludes":{"@id":"schema:Text"},"schema:domainIncludes":{"@id":"unece:InspectionResult"},"rdfs:comment":"A material type, expressed as text, related to this specified inspection result."},{"@id":"unece:relatedProductType","@type":["rdf:Property","owl:DatatypeProperty"],"rdfs:label":"relatedProductType","schema:rangeIncludes":{"@id":"schema:Text"},"schema:domainIncludes":{"@id":"unece:InspectionResult"},"rdfs:comment":"A product type, expressed as text, related to this specified inspection result."},{"@id":"unece:specifiedInspectionReference","@type":["rdf:Property","owl:ObjectProperty"],"rdfs:label":"specifiedInspectionReference","schema:rangeIncludes":{"@id":"unece:InspectionReference"},"schema:domainIncludes":{"@id":"unece:InspectionResult"},"rdfs:comment":"An inspection reference specified for this inspection result."},{"@id":"unece:applicableHazardousMaterial","@type":["rdf:Property","owl:ObjectProperty"],"rdfs:label":"applicableHazardousMaterial","schema:rangeIncludes":{"@id":"unece:HazardousMaterial"},"schema:domainIncludes":{"@id":"unece:Chemical"},"rdfs:comment":"An applicable toxicological hazardous material for this distinct chemical."},{"@id":"unece:commonName","@type":["rdf:Property","owl:DatatypeProperty"],"rdfs:label":"commonName","schema:rangeIncludes":{"@id":"schema:Text"},"schema:domainIncludes":{"@id":"unece:Chemical"},"rdfs:comment":"A common name, expressed as text, for this distinct chemical."},{"@id":"unece:formulaDescription","@type":["rdf:Property","owl:DatatypeProperty"],"rdfs:label":"formulaDescription","schema:rangeIncludes":{"@id":"schema:Text"},"schema:domainIncludes":{"@id":"unece:Chemical"},"rdfs:comment":"The textual description of the formula for this distinct chemical."},{"@id":"unece:massMeasure","@type":["rdf:Property","owl:ObjectProperty"],"rdfs:label":"massMeasure","schema:rangeIncludes":{"@id":"unece:MeasureType"},"schema:domainIncludes":[{"@id":"unece:Chemical"},{"@id":"unece:SpecifiedMaterial"}],"rdfs:comment":""},{"@id":"unece:massRatioMeasure","@type":["rdf:Property","owl:ObjectProperty"],"rdfs:label":"massRatioMeasure","schema:rangeIncludes":{"@id":"unece:MeasureType"},"schema:domainIncludes":[{"@id":"unece:Chemical"},{"@id":"unece:SpecifiedMaterial"}],"rdfs:comment":""},{"@id":"unece:molecularWeightMeasure","@type":["rdf:Property","owl:ObjectProperty"],"rdfs:label":"molecularWeightMeasure","schema:rangeIncludes":{"@id":"unece:MeasureType"},"schema:domainIncludes":{"@id":"unece:Chemical"},"rdfs:comment":""},{"@id":"unece:presenceMeasurement","@type":["rdf:Property","owl:ObjectProperty"],"rdfs:label":"presenceMeasurement","schema:rangeIncludes":{"@id":"unece:IngredientRangeMeasurement"},"schema:domainIncludes":{"@id":"unece:Chemical"},"rdfs:comment":"A measurement of the range of the presence of an ingredient in this distinct chemical."},{"@id":"unece:presencePercent","@type":["rdf:Property","owl:DatatypeProperty"],"rdfs:label":"presencePercent","schema:rangeIncludes":{"@id":"schema:Text"},"schema:domainIncludes":[{"@id":"unece:Chemical"},{"@id":"unece:SpecifiedMaterial"}],"rdfs:comment":"The percentage of the presence for this specified material."},{"@id":"unece:scientificName","@type":["rdf:Property","owl:DatatypeProperty"],"rdfs:label":"scientificName","schema:rangeIncludes":{"@id":"schema:Text"},"schema:domainIncludes":{"@id":"unece:Chemical"},"rdfs:comment":"A scientific name, expressed as text, for this trade product."},{"@id":"unece:specifiedProductCertificate","@type":["rdf:Property","owl:ObjectProperty"],"rdfs:label":"specifiedProductCertificate","schema:rangeIncludes":{"@id":"unece:ProductCertificate"},"schema:domainIncludes":{"@id":"unece:Chemical"},"rdfs:comment":"A product certificate specified for this distinct chemical."},{"@id":"unece:synonymName","@type":["rdf:Property","owl:DatatypeProperty"],"rdfs:label":"synonymName","schema:rangeIncludes":{"@id":"schema:Text"},"schema:domainIncludes":{"@id":"unece:Chemical"},"rdfs:comment":"A synonym name, expressed as text, for this distinct chemical."},{"@id":"unece:volumeMeasure","@type":["rdf:Property","owl:ObjectProperty"],"rdfs:label":"volumeMeasure","schema:rangeIncludes":{"@id":"unece:MeasureType"},"schema:domainIncludes":[{"@id":"unece:Chemical"},{"@id":"unece:SpecifiedMaterial"},{"@id":"unece:ProductionWasteMaterial"}],"rdfs:comment":""},{"@id":"unece:volumeRatioMeasure","@type":["rdf:Property","owl:ObjectProperty"],"rdfs:label":"volumeRatioMeasure","schema:rangeIncludes":{"@id":"unece:MeasureType"},"schema:domainIncludes":[{"@id":"unece:Chemical"},{"@id":"unece:SpecifiedMaterial"}],"rdfs:comment":""},{"@id":"unece:applicableInspectionResult","@type":["rdf:Property","owl:ObjectProperty"],"rdfs:label":"applicableInspectionResult","schema:rangeIncludes":{"@id":"unece:InspectionResult"},"schema:domainIncludes":[{"@id":"unece:SustainabilityCharacteristic"},{"@id":"unece:SustainabilityInspection"}],"rdfs:comment":"A specified inspection result applicable to this sustainability characteristic."},{"@id":"unece:subordinateCategoryCode","@type":["rdf:Property","owl:DatatypeProperty"],"rdfs:label":"subordinateCategoryCode","schema:rangeIncludes":{"@id":"schema:Text"},"schema:domainIncludes":{"@id":"unece:SustainabilityCharacteristic"},"rdfs:comment":"The subordinate category for this sustainability characteristic."},{"@id":"unece:valuePeriod","@type":["rdf:Property","owl:ObjectProperty"],"rdfs:label":"valuePeriod","schema:rangeIncludes":{"@id":"unece:SpecifiedPeriod"},"schema:domainIncludes":{"@id":"unece:SustainabilityCharacteristic"},"rdfs:comment":"A specified period of time."},{"@id":"unece:executionParty","@type":["rdf:Property","owl:ObjectProperty"],"rdfs:label":"executionParty","schema:rangeIncludes":{"@id":"unece:Party"},"schema:domainIncludes":[{"@id":"unece:SustainabilityInspection"},{"@id":"unece:SpecifiedInspection"}],"rdfs:comment":""},{"@id":"unece:executionPerson","@type":["rdf:Property","owl:ObjectProperty"],"rdfs:label":"executionPerson","schema:rangeIncludes":{"@id":"unece:InspectionPerson"},"schema:domainIncludes":[{"@id":"unece:SustainabilityInspection"},{"@id":"unece:SpecifiedInspection"}],"rdfs:comment":"The inspector executing this specified inspection."},{"@id":"unece:outsourcedIndicator","@type":["rdf:Property","owl:DatatypeProperty"],"rdfs:label":"outsourcedIndicator","schema:rangeIncludes":{"@id":"schema:Boolean"},"schema:domainIncludes":[{"@id":"unece:SustainabilityInspection"},{"@id":"unece:SpecifiedInspection"}],"rdfs:comment":"The indication of whether or not this specified inspection is outsourced."},{"@id":"unece:specifiedInspectionEvent","@type":["rdf:Property","owl:ObjectProperty"],"rdfs:label":"specifiedInspectionEvent","schema:rangeIncludes":{"@id":"unece:InspectionEvent"},"schema:domainIncludes":[{"@id":"unece:SustainabilityInspection"},{"@id":"unece:SpecifiedInspection"}],"rdfs:comment":"A specified inspection event for this sustainability inspection."},{"@id":"unece:specifiedInspectionStatus","@type":["rdf:Property","owl:ObjectProperty"],"rdfs:label":"specifiedInspectionStatus","schema:rangeIncludes":{"@id":"unece:InspectionStatus"},"schema:domainIncludes":[{"@id":"unece:SustainabilityInspection"},{"@id":"unece:SpecifiedInspection"}],"rdfs:comment":"The inspection status specified for this sustainability inspection."},{"@id":"unece:measuredAccuracyMeasure","@type":["rdf:Property","owl:ObjectProperty"],"rdfs:label":"measuredAccuracyMeasure","schema:rangeIncludes":{"@id":"unece:MeasureType"},"schema:domainIncludes":[{"@id":"unece:InspectionResultCharacteristic"},{"@id":"unece:ObservationResultCharacteristic"}],"rdfs:comment":""},{"@id":"unece:measuredValue","@type":["rdf:Property","owl:DatatypeProperty"],"rdfs:label":"measuredValue","schema:rangeIncludes":{"@id":"schema:Text"},"schema:domainIncludes":[{"@id":"unece:InspectionResultCharacteristic"},{"@id":"unece:ObservationResultCharacteristic"}],"rdfs:comment":"The measured value, expressed as text, for this inspection result characteristic."},{"@id":"unece:measuredValueMeasure","@type":["rdf:Property","owl:ObjectProperty"],"rdfs:label":"measuredValueMeasure","schema:rangeIncludes":{"@id":"unece:MeasureType"},"schema:domainIncludes":[{"@id":"unece:InspectionResultCharacteristic"},{"@id":"unece:ObservationResultCharacteristic"}],"rdfs:comment":""},{"@id":"unece:qualityResultCode","@type":["rdf:Property","owl:DatatypeProperty"],"rdfs:label":"qualityResultCode","schema:rangeIncludes":{"@id":"schema:Text"},"schema:domainIncludes":[{"@id":"unece:InspectionResultCharacteristic"},{"@id":"unece:ObservationResultCharacteristic"}],"rdfs:comment":"The code specifying the quality of the result for this inspection result characteristic."},{"@id":"unece:qualityResultDescription","@type":["rdf:Property","owl:DatatypeProperty"],"rdfs:label":"qualityResultDescription","schema:rangeIncludes":{"@id":"schema:Text"},"schema:domainIncludes":[{"@id":"unece:InspectionResultCharacteristic"},{"@id":"unece:ObservationResultCharacteristic"}],"rdfs:comment":"A textual description of the quality of the result for this inspection result characteristic."},{"@id":"unece:qualityResultReferenceLevelDescription","@type":["rdf:Property","owl:DatatypeProperty"],"rdfs:label":"qualityResultReferenceLevelDescription","schema:rangeIncludes":{"@id":"schema:Text"},"schema:domainIncludes":{"@id":"unece:InspectionResultCharacteristic"},"rdfs:comment":"A textual description of the reference level for the quality of the result for this inspection result characteristic."},{"@id":"unece:range","@type":["rdf:Property","owl:DatatypeProperty"],"rdfs:label":"range","schema:rangeIncludes":{"@id":"schema:Text"},"schema:domainIncludes":[{"@id":"unece:InspectionResultCharacteristic"},{"@id":"unece:ObservationResultCharacteristic"}],"rdfs:comment":"The range, expressed as text, of the values of the measurements performed for this inspection result characteristic."},{"@id":"unece:applicableNote","@type":["rdf:Property","owl:ObjectProperty"],"rdfs:label":"applicableNote","schema:rangeIncludes":{"@id":"unece:Note"},"schema:domainIncludes":{"@id":"unece:Observation"},"rdfs:comment":"A textual or coded description, such as a remark or additional information."},{"@id":"unece:relatedBinaryFile","@type":["rdf:Property","owl:ObjectProperty"],"rdfs:label":"relatedBinaryFile","schema:rangeIncludes":{"@id":"unece:BinaryFile"},"schema:domainIncludes":{"@id":"unece:Observation"},"rdfs:comment":"A specified computer file or program stored in a binary format."},{"@id":"unece:applicableProductCertificate","@type":["rdf:Property","owl:ObjectProperty"],"rdfs:label":"applicableProductCertificate","schema:rangeIncludes":{"@id":"unece:ProductCertificate"},"schema:domainIncludes":[{"@id":"unece:HazardousMaterial"},{"@id":"unece:SpecifiedMaterial"},{"@id":"unece:ProductionWasteMaterial"},{"@id":"unece:ProductionWasteMaterialComponent"}],"rdfs:comment":"A product certificate applicable to this production waste material component."},{"@id":"unece:biologicalSeverityDescription","@type":["rdf:Property","owl:DatatypeProperty"],"rdfs:label":"biologicalSeverityDescription","schema:rangeIncludes":{"@id":"schema:Text"},"schema:domainIncludes":{"@id":"unece:HazardousMaterial"},"rdfs:comment":"The textual description of the biological severity of this toxicological hazardous material."},{"@id":"unece:entryRouteDescription","@type":["rdf:Property","owl:DatatypeProperty"],"rdfs:label":"entryRouteDescription","schema:rangeIncludes":{"@id":"schema:Text"},"schema:domainIncludes":{"@id":"unece:HazardousMaterial"},"rdfs:comment":"A textual description of the entry route of this toxicological hazardous material."},{"@id":"unece:reproductiveToxinName","@type":["rdf:Property","owl:DatatypeProperty"],"rdfs:label":"reproductiveToxinName","schema:rangeIncludes":{"@id":"schema:Text"},"schema:domainIncludes":{"@id":"unece:HazardousMaterial"},"rdfs:comment":"The name, expressed as text, of the reproductive toxin in this toxicological hazardous material."},{"@id":"unece:applicableSpecifiedTemperature","@type":["rdf:Property","owl:ObjectProperty"],"rdfs:label":"applicableSpecifiedTemperature","schema:rangeIncludes":{"@id":"unece:SpecifiedTemperature"},"schema:domainIncludes":{"@id":"unece:AppliedChemicalTreatment"},"rdfs:comment":"A specified temperature value or range of values."},{"@id":"unece:appliedPeriod","@type":["rdf:Property","owl:ObjectProperty"],"rdfs:label":"appliedPeriod","schema:rangeIncludes":{"@id":"unece:SpecifiedPeriod"},"schema:domainIncludes":{"@id":"unece:AppliedChemicalTreatment"},"rdfs:comment":"A specified period of time."},{"@id":"unece:chemicalConcentrationMeasure","@type":["rdf:Property","owl:ObjectProperty"],"rdfs:label":"chemicalConcentrationMeasure","schema:rangeIncludes":{"@id":"unece:MeasureType"},"schema:domainIncludes":{"@id":"unece:AppliedChemicalTreatment"},"rdfs:comment":""},{"@id":"unece:methodName","@type":["rdf:Property","owl:DatatypeProperty"],"rdfs:label":"methodName","schema:rangeIncludes":{"@id":"schema:Text"},"schema:domainIncludes":{"@id":"unece:AppliedChemicalTreatment"},"rdfs:comment":"The name, expressed as text, of the method of this applied chemical treatment."},{"@id":"unece:resultAuthentication","@type":["rdf:Property","owl:ObjectProperty"],"rdfs:label":"resultAuthentication","schema:rangeIncludes":{"@id":"unece:Authentication"},"schema:domainIncludes":{"@id":"unece:AppliedChemicalTreatment"},"rdfs:comment":"A proof that a document is genuine."},{"@id":"unece:resultNote","@type":["rdf:Property","owl:ObjectProperty"],"rdfs:label":"resultNote","schema:rangeIncludes":{"@id":"unece:Note"},"schema:domainIncludes":{"@id":"unece:AppliedChemicalTreatment"},"rdfs:comment":"A textual or coded description, such as a remark or additional information."},{"@id":"unece:usedChemical","@type":["rdf:Property","owl:ObjectProperty"],"rdfs:label":"usedChemical","schema:rangeIncludes":{"@id":"unece:Chemical"},"schema:domainIncludes":[{"@id":"unece:AppliedChemicalTreatment"},{"@id":"unece:SpecifiedMaterial"}],"rdfs:comment":"A chemical used during this applied chemical treatment."},{"@id":"unece:descriptionCode","@type":["rdf:Property","owl:DatatypeProperty"],"rdfs:label":"descriptionCode","schema:rangeIncludes":{"@id":"schema:Text"},"schema:domainIncludes":[{"@id":"unece:Assertion"},{"@id":"unece:TechnicalCharacteristic"},{"@id":"unece:InspectionInstructions"},{"@id":"unece:SpecifiedMaterial"}],"rdfs:comment":"A code specifying a description of this technical characteristic."},{"@id":"unece:relatedPolicy","@type":["rdf:Property","owl:ObjectProperty"],"rdfs:label":"relatedPolicy","schema:rangeIncludes":{"@id":"unece:Policy"},"schema:domainIncludes":{"@id":"unece:Assertion"},"rdfs:comment":"A compliance policy related to this sustainability assertion."},{"@id":"unece:assessedObject","@type":["rdf:Property","owl:ObjectProperty"],"rdfs:label":"assessedObject","schema:rangeIncludes":{"@id":"unece:Object"},"schema:domainIncludes":{"@id":"unece:Assessment"},"rdfs:comment":"Anything that is visible or tangible, such as a product, process, or organization."},{"@id":"unece:assessorParty","@type":["rdf:Property","owl:ObjectProperty"],"rdfs:label":"assessorParty","schema:rangeIncludes":{"@id":"unece:Party"},"schema:domainIncludes":{"@id":"unece:Assessment"},"rdfs:comment":""},{"@id":"unece:associatedBinaryFile","@type":["rdf:Property","owl:ObjectProperty"],"rdfs:label":"associatedBinaryFile","schema:rangeIncludes":{"@id":"unece:BinaryFile"},"schema:domainIncludes":{"@id":"unece:Assessment"},"rdfs:comment":"A specified computer file or program stored in a binary format."},{"@id":"unece:reportDateTime","@type":["rdf:Property","owl:DatatypeProperty"],"rdfs:label":"reportDateTime","schema:rangeIncludes":{"@id":"schema:Text"},"schema:domainIncludes":{"@id":"unece:Assessment"},"rdfs:comment":"The date, time, date time or other date time value of the report of this specified assessment."},{"@id":"unece:reportId","@type":["rdf:Property","owl:DatatypeProperty"],"rdfs:label":"reportId","schema:rangeIncludes":{"@id":"schema:Text"},"schema:domainIncludes":{"@id":"unece:Assessment"},"rdfs:comment":"The report identifier for this specified assessment."},{"@id":"unece:selfAssessedIndicator","@type":["rdf:Property","owl:DatatypeProperty"],"rdfs:label":"selfAssessedIndicator","schema:rangeIncludes":{"@id":"schema:Boolean"},"schema:domainIncludes":{"@id":"unece:Assessment"},"rdfs:comment":"The indication of whether or not this specified assessment is self assessed."},{"@id":"unece:verifiedIndicator","@type":["rdf:Property","owl:DatatypeProperty"],"rdfs:label":"verifiedIndicator","schema:rangeIncludes":{"@id":"schema:Boolean"},"schema:domainIncludes":{"@id":"unece:Assessment"},"rdfs:comment":"The indication of whether or not this specified assessment is verified."},{"@id":"unece:verifierParty","@type":["rdf:Property","owl:ObjectProperty"],"rdfs:label":"verifierParty","schema:rangeIncludes":{"@id":"unece:Party"},"schema:domainIncludes":{"@id":"unece:Assessment"},"rdfs:comment":""},{"@id":"unece:measuredAttributeTypeCode","@type":["rdf:Property","owl:DatatypeProperty"],"rdfs:label":"measuredAttributeTypeCode","schema:rangeIncludes":{"@id":"unece:MeasuredAttributeCodeList"},"schema:domainIncludes":{"@id":"unece:ProcessCharacteristic"},"rdfs:comment":"The code specifying the type of this process characteristic."},{"@id":"unece:capacityValueMeasure","@type":["rdf:Property","owl:ObjectProperty"],"rdfs:label":"capacityValueMeasure","schema:rangeIncludes":{"@id":"unece:MeasureType"},"schema:domainIncludes":{"@id":"unece:TechnicalCharacteristic"},"rdfs:comment":""},{"@id":"unece:certificationCode","@type":["rdf:Property","owl:DatatypeProperty"],"rdfs:label":"certificationCode","schema:rangeIncludes":{"@id":"schema:Text"},"schema:domainIncludes":{"@id":"unece:TechnicalCharacteristic"},"rdfs:comment":"The code specifying the certification granted to this technical characteristic."},{"@id":"unece:componentMaterial","@type":["rdf:Property","owl:ObjectProperty"],"rdfs:label":"componentMaterial","schema:rangeIncludes":{"@id":"unece:SpecifiedMaterial"},"schema:domainIncludes":[{"@id":"unece:TechnicalCharacteristic"},{"@id":"unece:SpecifiedMaterial"}],"rdfs:comment":"A material component of this trade product."},{"@id":"unece:constructionDateTime","@type":["rdf:Property","owl:DatatypeProperty"],"rdfs:label":"constructionDateTime","schema:rangeIncludes":{"@id":"schema:Text"},"schema:domainIncludes":{"@id":"unece:TechnicalCharacteristic"},"rdfs:comment":"The date, time, date time, or other date time value of the construction of this technical characteristic."},{"@id":"unece:latestRenovationDateTime","@type":["rdf:Property","owl:DatatypeProperty"],"rdfs:label":"latestRenovationDateTime","schema:rangeIncludes":{"@id":"schema:Text"},"schema:domainIncludes":{"@id":"unece:TechnicalCharacteristic"},"rdfs:comment":"The date of the latest renovation of this experience facility."},{"@id":"unece:licence","@type":["rdf:Property","owl:DatatypeProperty"],"rdfs:label":"licence","schema:rangeIncludes":{"@id":"schema:Text"},"schema:domainIncludes":{"@id":"unece:TechnicalCharacteristic"},"rdfs:comment":"A licence, expressed as text, for this production facility."},{"@id":"unece:specifiedAnimalHoldingEvent","@type":["rdf:Property","owl:ObjectProperty"],"rdfs:label":"specifiedAnimalHoldingEvent","schema:rangeIncludes":{"@id":"unece:Event"},"schema:domainIncludes":{"@id":"unece:TechnicalCharacteristic"},"rdfs:comment":"A significant occurrence or happening during transport.,A referenced significant occurrence or happening during transport."},{"@id":"unece:appliedDilutionNumeric","@type":["rdf:Property","owl:DatatypeProperty"],"rdfs:label":"appliedDilutionNumeric","schema:rangeIncludes":{"@id":"schema:Text"},"schema:domainIncludes":{"@id":"unece:ObservationResultCharacteristic"},"rdfs:comment":"The rate of the applied dilution for this sample observation result characteristic."},{"@id":"unece:methodParameterId","@type":["rdf:Property","owl:DatatypeProperty"],"rdfs:label":"methodParameterId","schema:rangeIncludes":{"@id":"schema:Text"},"schema:domainIncludes":{"@id":"unece:ObservationResultCharacteristic"},"rdfs:comment":"The identifier of the method parameter for this sample observation result characteristic."},{"@id":"unece:parameterValue","@type":["rdf:Property","owl:DatatypeProperty"],"rdfs:label":"parameterValue","schema:rangeIncludes":{"@id":"schema:Text"},"schema:domainIncludes":{"@id":"unece:ObservationResultCharacteristic"},"rdfs:comment":"The parameter value, expressed as text, for this sample observation result characteristic."},{"@id":"unece:referenceLevelQualityResultDescription","@type":["rdf:Property","owl:DatatypeProperty"],"rdfs:label":"referenceLevelQualityResultDescription","schema:rangeIncludes":{"@id":"schema:Text"},"schema:domainIncludes":{"@id":"unece:ObservationResultCharacteristic"},"rdfs:comment":"The textual description of the reference level for the quality of the result for this sample observation result characteristic."},{"@id":"unece:auditDateTime","@type":["rdf:Property","owl:DatatypeProperty"],"rdfs:label":"auditDateTime","schema:rangeIncludes":{"@id":"schema:DateTime"},"schema:domainIncludes":{"@id":"unece:SpecifiedCertification"},"rdfs:comment":"An audit date, time, date time or other date time value for this specified certification."},{"@id":"unece:relatedStandard","@type":["rdf:Property","owl:ObjectProperty"],"rdfs:label":"relatedStandard","schema:rangeIncludes":{"@id":"unece:Standard"},"schema:domainIncludes":{"@id":"unece:SpecifiedCertification"},"rdfs:comment":"A referenced standard related to this specified certification."},{"@id":"unece:associatedStandard","@type":["rdf:Property","owl:ObjectProperty"],"rdfs:label":"associatedStandard","schema:rangeIncludes":{"@id":"unece:Standard"},"schema:domainIncludes":[{"@id":"unece:Licence"},{"@id":"unece:SpecifiedDeclaration"}],"rdfs:comment":"A referenced standard associated to this specified licence."},{"@id":"unece:grantedParty","@type":["rdf:Property","owl:ObjectProperty"],"rdfs:label":"grantedParty","schema:rangeIncludes":{"@id":"unece:Party"},"schema:domainIncludes":{"@id":"unece:Licence"},"rdfs:comment":""},{"@id":"unece:verifiedObject","@type":["rdf:Property","owl:ObjectProperty"],"rdfs:label":"verifiedObject","schema:rangeIncludes":{"@id":"unece:Object"},"schema:domainIncludes":[{"@id":"unece:Licence"},{"@id":"unece:SpecifiedDeclaration"}],"rdfs:comment":"Anything that is visible or tangible, such as a product, process, or organization."},{"@id":"unece:associatedTax","@type":["rdf:Property","owl:ObjectProperty"],"rdfs:label":"associatedTax","schema:rangeIncludes":{"@id":"undefined:RegisteredTax"},"schema:domainIncludes":{"@id":"unece:TaxRegistration"},"owl:sameAs":{"@id":"undefined:associatedTax"},"rdfs:comment":"A registered tax or duty system pertaining to an authority."},{"@id":"unece:iOSSId","@type":["rdf:Property","owl:DatatypeProperty"],"rdfs:label":"iOSSId","schema:rangeIncludes":{"@id":"schema:Text"},"schema:domainIncludes":{"@id":"unece:TaxRegistration"},"rdfs:comment":"The Import One Stop Shop (IOSS) identifier for this tax registration."},{"@id":"unece:reportedInspectionResult","@type":["rdf:Property","owl:ObjectProperty"],"rdfs:label":"reportedInspectionResult","schema:rangeIncludes":{"@id":"unece:InspectionResult"},"schema:domainIncludes":{"@id":"unece:SpecifiedInspection"},"rdfs:comment":"The result reported for this specified inspection."},{"@id":"unece:attainedAcademicQualification","@type":["rdf:Property","owl:ObjectProperty"],"rdfs:label":"attainedAcademicQualification","schema:rangeIncludes":{"@id":"unece:AcademicQualification"},"schema:domainIncludes":{"@id":"unece:AuthoritativeSignatoryPerson"},"rdfs:comment":"An academic qualification attained by this authoritative signatory person."},{"@id":"unece:attainedSpecifiedQualification","@type":["rdf:Property","owl:ObjectProperty"],"rdfs:label":"attainedSpecifiedQualification","schema:rangeIncludes":{"@id":"unece:SpecifiedQualification"},"schema:domainIncludes":{"@id":"unece:InspectionPerson"},"rdfs:comment":"The specified qualification attained by this inspection person."},{"@id":"unece:inspectionPersonName","@type":["rdf:Property","owl:DatatypeProperty"],"rdfs:label":"inspectionPersonName","schema:rangeIncludes":{"@id":"schema:Text"},"schema:domainIncludes":{"@id":"unece:InspectionPerson"},"rdfs:comment":"The name or set of names, expressed as text, by which this inspection person is known."},{"@id":"unece:bathingProhibitionCaution","@type":["rdf:Property","owl:DatatypeProperty"],"rdfs:label":"bathingProhibitionCaution","schema:rangeIncludes":{"@id":"schema:Text"},"schema:domainIncludes":{"@id":"unece:Source"},"rdfs:comment":"A caution, expressed as text, of a bathing prohibition for this water source."},{"@id":"unece:characteristicCode","@type":["rdf:Property","owl:DatatypeProperty"],"rdfs:label":"characteristicCode","schema:rangeIncludes":{"@id":"schema:Text"},"schema:domainIncludes":{"@id":"unece:Source"},"rdfs:comment":"The code specifying the characteristic of this water source."},{"@id":"unece:drinkingProhibitionCaution","@type":["rdf:Property","owl:DatatypeProperty"],"rdfs:label":"drinkingProhibitionCaution","schema:rangeIncludes":{"@id":"schema:Text"},"schema:domainIncludes":{"@id":"unece:Source"},"rdfs:comment":"A caution, expressed as text, of a drinking prohibition for this water source."},{"@id":"unece:healthBenefit","@type":["rdf:Property","owl:DatatypeProperty"],"rdfs:label":"healthBenefit","schema:rangeIncludes":{"@id":"schema:Text"},"schema:domainIncludes":{"@id":"unece:Source"},"rdfs:comment":"A health benefit, expressed as text, for this water source."},{"@id":"unece:licenceId","@type":["rdf:Property","owl:DatatypeProperty"],"rdfs:label":"licenceId","schema:rangeIncludes":{"@id":"schema:Text"},"schema:domainIncludes":{"@id":"unece:GovernmentRegistration"},"rdfs:comment":"The identifier of a licence for this government registration."},{"@id":"unece:recordedDate","@type":["rdf:Property","owl:DatatypeProperty"],"rdfs:label":"recordedDate","schema:rangeIncludes":{"@id":"schema:Text"},"schema:domainIncludes":{"@id":"unece:GovernmentRegistration"},"rdfs:comment":"The date that this government registration was recorded."},{"@id":"unece:consignmentRiskRelatedCode","@type":["rdf:Property","owl:DatatypeProperty"],"rdfs:label":"consignmentRiskRelatedCode","schema:rangeIncludes":{"@id":"schema:Text"},"schema:domainIncludes":{"@id":"unece:RiskAnalysisResult"},"rdfs:comment":"A code specifying a consignment related risk for this logistics risk analysis result."},{"@id":"unece:levelCode","@type":["rdf:Property","owl:DatatypeProperty"],"rdfs:label":"levelCode","schema:rangeIncludes":{"@id":"schema:Text"},"schema:domainIncludes":{"@id":"unece:RiskAnalysisResult"},"rdfs:comment":"The code specifying the level for this logistics risk analysis result."},{"@id":"unece:partyRiskRelatedCode","@type":["rdf:Property","owl:DatatypeProperty"],"rdfs:label":"partyRiskRelatedCode","schema:rangeIncludes":{"@id":"schema:Text"},"schema:domainIncludes":{"@id":"unece:RiskAnalysisResult"},"rdfs:comment":"A code specifying a party related risk for this logistics risk analysis result."},{"@id":"unece:screeningMethodCode","@type":["rdf:Property","owl:DatatypeProperty"],"rdfs:label":"screeningMethodCode","schema:rangeIncludes":{"@id":"schema:Text"},"schema:domainIncludes":{"@id":"unece:RiskAnalysisResult"},"rdfs:comment":"A code specifying a method of screening used in this logistics risk analysis result."},{"@id":"unece:securityExemptionCode","@type":["rdf:Property","owl:DatatypeProperty"],"rdfs:label":"securityExemptionCode","schema:rangeIncludes":{"@id":"schema:Text"},"schema:domainIncludes":{"@id":"unece:RiskAnalysisResult"},"rdfs:comment":"A code specifying a security exemption for this logistics risk analysis result."},{"@id":"unece:transportEquipmentRiskRelatedCode","@type":["rdf:Property","owl:DatatypeProperty"],"rdfs:label":"transportEquipmentRiskRelatedCode","schema:rangeIncludes":{"@id":"schema:Text"},"schema:domainIncludes":{"@id":"unece:RiskAnalysisResult"},"rdfs:comment":"A code specifying a transport equipment related risk for this logistics risk analysis result."},{"@id":"unece:transportMovementRiskRelatedCode","@type":["rdf:Property","owl:DatatypeProperty"],"rdfs:label":"transportMovementRiskRelatedCode","schema:rangeIncludes":{"@id":"schema:Text"},"schema:domainIncludes":{"@id":"unece:RiskAnalysisResult"},"rdfs:comment":"A code specifying a transport movement related risk for this logistics risk analysis result."},{"@id":"unece:softwareOperatingSystem","@type":["rdf:Property","owl:DatatypeProperty"],"rdfs:label":"softwareOperatingSystem","schema:rangeIncludes":{"@id":"schema:Text"},"schema:domainIncludes":{"@id":"unece:ConformanceCertificate"},"rdfs:comment":"The software operating system, expressed as text, for which this conformance certificate is produced."},{"@id":"unece:sampledObjectMinimumRequiredObjectSizeMeasure","@type":["rdf:Property","owl:ObjectProperty"],"rdfs:label":"sampledObjectMinimumRequiredObjectSizeMeasure","schema:rangeIncludes":{"@id":"unece:MeasureType"},"schema:domainIncludes":{"@id":"unece:LaboratoryObservationAnalysisMethod"},"rdfs:comment":""},{"@id":"unece:changeableIndicator","@type":["rdf:Property","owl:DatatypeProperty"],"rdfs:label":"changeableIndicator","schema:rangeIncludes":{"@id":"schema:Boolean"},"schema:domainIncludes":[{"@id":"unece:ControlSettingParameter"},{"@id":"unece:OperationalParameter"}],"rdfs:comment":"The indication whether or not this control setting parameter is changeable."},{"@id":"unece:requestedRange","@type":["rdf:Property","owl:ObjectProperty"],"rdfs:label":"requestedRange","schema:rangeIncludes":{"@id":"unece:Range"},"schema:domainIncludes":{"@id":"unece:ControlSettingParameter"},"rdfs:comment":"A row, line or series, commonly used to express the difference between lowest and highest values."},{"@id":"unece:definedRange","@type":["rdf:Property","owl:ObjectProperty"],"rdfs:label":"definedRange","schema:rangeIncludes":{"@id":"unece:Range"},"schema:domainIncludes":{"@id":"unece:OperationalParameter"},"rdfs:comment":"A row, line or series, commonly used to express the difference between lowest and highest values."},{"@id":"unece:conditionCode","@type":["rdf:Property","owl:DatatypeProperty"],"rdfs:label":"conditionCode","schema:rangeIncludes":{"@id":"schema:Text"},"schema:domainIncludes":{"@id":"unece:InspectionStatus"},"rdfs:comment":"A code specifying a condition of this logistics packaging."},{"@id":"unece:emailCommunication","@type":["rdf:Property","owl:ObjectProperty"],"rdfs:label":"emailCommunication","schema:rangeIncludes":{"@id":"unece:Communication"},"schema:domainIncludes":{"@id":"unece:LaboratoryObservationContact"},"rdfs:comment":"The exchange of thoughts, messages, or information, as universally exchanged by speech, signals, writing, or behaviour between persons and/or organizations."},{"@id":"unece:personName","@type":["rdf:Property","owl:DatatypeProperty"],"rdfs:label":"personName","schema:rangeIncludes":{"@id":"schema:Text"},"schema:domainIncludes":{"@id":"unece:LaboratoryObservationContact"},"rdfs:comment":"The name, expressed as text, of the person for this laboratory observation contact."},{"@id":"unece:disposalInstructionsRecyclingDescriptionCode","@type":["rdf:Property","owl:DatatypeProperty"],"rdfs:label":"disposalInstructionsRecyclingDescriptionCode","schema:rangeIncludes":{"@id":"schema:Text"},"schema:domainIncludes":{"@id":"unece:DisposalInstructions"},"rdfs:comment":"A code describing recycling in these disposal instructions."},{"@id":"unece:materialId","@type":["rdf:Property","owl:DatatypeProperty"],"rdfs:label":"materialId","schema:rangeIncludes":{"@id":"schema:Text"},"schema:domainIncludes":{"@id":"unece:DisposalInstructions"},"rdfs:comment":"An identifier of the material to which these returnable asset instructions apply."},{"@id":"unece:recyclingProcedure","@type":["rdf:Property","owl:DatatypeProperty"],"rdfs:label":"recyclingProcedure","schema:rangeIncludes":{"@id":"schema:Text"},"schema:domainIncludes":{"@id":"unece:DisposalInstructions"},"rdfs:comment":"A recycling procedure, expressed as text, for these disposal instructions."},{"@id":"unece:occurrenceLocation","@type":["rdf:Property","owl:ObjectProperty"],"rdfs:label":"occurrenceLocation","schema:rangeIncludes":{"@id":"unece:Location"},"schema:domainIncludes":{"@id":"unece:InspectionEvent"},"rdfs:comment":"A reference to a physical location or place."},{"@id":"unece:instructionsType","@type":["rdf:Property","owl:DatatypeProperty"],"rdfs:label":"instructionsType","schema:rangeIncludes":{"@id":"schema:Text"},"schema:domainIncludes":[{"@id":"unece:InspectionInstructions"},{"@id":"unece:LaboratoryObservationInstructions"}],"rdfs:comment":"A type, expressed as text, of these packaging instructions."},{"@id":"unece:interpretationCode","@type":["rdf:Property","owl:DatatypeProperty"],"rdfs:label":"interpretationCode","schema:rangeIncludes":{"@id":"schema:Text"},"schema:domainIncludes":[{"@id":"unece:InspectionInstructions"},{"@id":"unece:LaboratoryObservationInstructions"}],"rdfs:comment":"The code specifying the interpretation for this laboratory instruction."},{"@id":"unece:latestUpdateDateTime","@type":["rdf:Property","owl:DatatypeProperty"],"rdfs:label":"latestUpdateDateTime","schema:rangeIncludes":{"@id":"schema:Text"},"schema:domainIncludes":[{"@id":"unece:InspectionInstructions"},{"@id":"unece:LaboratoryObservationInstructions"}],"rdfs:comment":"The date, time, date time, or other date time value of the latest update of this set of inspection instructions."},{"@id":"unece:laboratoryObservationInstructionsDescriptionCode","@type":["rdf:Property","owl:DatatypeProperty"],"rdfs:label":"laboratoryObservationInstructionsDescriptionCode","schema:rangeIncludes":{"@id":"schema:Text"},"schema:domainIncludes":{"@id":"unece:LaboratoryObservationInstructions"},"rdfs:comment":"The code specifying a description of a laboratory observation instruction or a set of instructions."},{"@id":"unece:quarantineInstructionsDescriptionCode","@type":["rdf:Property","owl:DatatypeProperty"],"rdfs:label":"quarantineInstructionsDescriptionCode","schema:rangeIncludes":{"@id":"schema:Text"},"schema:domainIncludes":{"@id":"unece:QuarantineInstructions"},"rdfs:comment":"The code specifying the description of these quarantine instructions."},{"@id":"unece:rule","@type":["rdf:Property","owl:DatatypeProperty"],"rdfs:label":"rule","schema:rangeIncludes":{"@id":"schema:Text"},"schema:domainIncludes":{"@id":"unece:Requirement"},"rdfs:comment":"A rule, expressed as text, for this specified requirement."},{"@id":"unece:specifiedPaymentTradeSettlement","@type":["rdf:Property","owl:ObjectProperty"],"rdfs:label":"specifiedPaymentTradeSettlement","schema:rangeIncludes":{"@id":"undefined:PaymentTradeSettlement"},"schema:domainIncludes":{"@id":"unece:Requirement"},"owl:sameAs":{"@id":"undefined:specifiedPaymentTradeSettlement"},"rdfs:comment":"The information that enables the reconciliation of a payment with the item(s) that the payment is intended to settle, for example a commercial invoice."},{"@id":"unece:specifyingParty","@type":["rdf:Property","owl:ObjectProperty"],"rdfs:label":"specifyingParty","schema:rangeIncludes":{"@id":"unece:Party"},"schema:domainIncludes":{"@id":"unece:Requirement"},"rdfs:comment":""},{"@id":"unece:temperatureSettingInstructionsDescriptionCode","@type":["rdf:Property","owl:DatatypeProperty"],"rdfs:label":"temperatureSettingInstructionsDescriptionCode","schema:rangeIncludes":{"@id":"schema:Text"},"schema:domainIncludes":{"@id":"unece:TemperatureSettingInstructions"},"rdfs:comment":"The code specifying a description of these temperature setting instructions."},{"@id":"unece:quantificationTypeCode","@type":["rdf:Property","owl:DatatypeProperty"],"rdfs:label":"quantificationTypeCode","schema:rangeIncludes":{"@id":"schema:Text"},"schema:domainIncludes":{"@id":"unece:CalibratedMeasurement"},"rdfs:comment":"The code specifying a quantification type for this calibrated measurement, such as measured, calculated, or estimated."},{"@id":"unece:tolerancePercent","@type":["rdf:Property","owl:DatatypeProperty"],"rdfs:label":"tolerancePercent","schema:rangeIncludes":{"@id":"schema:Text"},"schema:domainIncludes":{"@id":"unece:CalibratedMeasurement"},"rdfs:comment":"The percent of tolerance of this calibrated measurement."},{"@id":"unece:officeAddress","@type":["rdf:Property","owl:ObjectProperty"],"rdfs:label":"officeAddress","schema:rangeIncludes":{"@id":"unece:Address"},"schema:domainIncludes":{"@id":"unece:LaboratoryObservationParty"},"rdfs:comment":"The location at which a particular trade related organization or person may be found or reached."},{"@id":"unece:personDefinedContact","@type":["rdf:Property","owl:ObjectProperty"],"rdfs:label":"personDefinedContact","schema:rangeIncludes":{"@id":"unece:LaboratoryObservationContact"},"schema:domainIncludes":{"@id":"unece:LaboratoryObservationParty"},"rdfs:comment":"The person defined as the contact for this laboratory observation party."},{"@id":"unece:thirdPartyIssuedIdentification","@type":["rdf:Property","owl:DatatypeProperty"],"rdfs:label":"thirdPartyIssuedIdentification","schema:rangeIncludes":{"@id":"schema:Text"},"schema:domainIncludes":{"@id":"unece:LaboratoryObservationParty"},"rdfs:comment":"A third party issued identifier, expressed as text, for this laboratory observation party."},{"@id":"unece:result","@type":["rdf:Property","owl:DatatypeProperty"],"rdfs:label":"result","schema:rangeIncludes":{"@id":"schema:Text"},"schema:domainIncludes":{"@id":"unece:TestSpecificationReport"},"rdfs:comment":"A result, expressed as text, reported in this certification test specification report."},{"@id":"unece:standardName","@type":["rdf:Property","owl:DatatypeProperty"],"rdfs:label":"standardName","schema:rangeIncludes":{"@id":"schema:Text"},"schema:domainIncludes":{"@id":"unece:TestSpecificationReport"},"rdfs:comment":"The name, expressed as text, of the standard applicable for this certification test specification report."},{"@id":"unece:testName","@type":["rdf:Property","owl:DatatypeProperty"],"rdfs:label":"testName","schema:rangeIncludes":{"@id":"schema:Text"},"schema:domainIncludes":{"@id":"unece:TestSpecificationReport"},"rdfs:comment":"A test name, expressed as text, for this certification test specification report."},{"@id":"unece:absolutePresenceVolumeMeasure","@type":["rdf:Property","owl:ObjectProperty"],"rdfs:label":"absolutePresenceVolumeMeasure","schema:rangeIncludes":{"@id":"unece:MeasureType"},"schema:domainIncludes":{"@id":"unece:GoodsCharacteristic"},"rdfs:comment":""},{"@id":"unece:absolutePresenceWeightMeasure","@type":["rdf:Property","owl:ObjectProperty"],"rdfs:label":"absolutePresenceWeightMeasure","schema:rangeIncludes":{"@id":"unece:MeasureType"},"schema:domainIncludes":{"@id":"unece:GoodsCharacteristic"},"rdfs:comment":""},{"@id":"unece:proportionalConstituentPercent","@type":["rdf:Property","owl:DatatypeProperty"],"rdfs:label":"proportionalConstituentPercent","schema:rangeIncludes":{"@id":"schema:Text"},"schema:domainIncludes":{"@id":"unece:GoodsCharacteristic"},"rdfs:comment":"The percentage presence of the material within the goods for this material goods characteristic."},{"@id":"unece:applicableGoodsCharacteristic","@type":["rdf:Property","owl:ObjectProperty"],"rdfs:label":"applicableGoodsCharacteristic","schema:rangeIncludes":{"@id":"unece:GoodsCharacteristic"},"schema:domainIncludes":{"@id":"unece:SpecifiedMaterial"},"rdfs:comment":"A distinguishing material feature applicable to this trade product instance."},{"@id":"unece:applicableQuantity","@type":["rdf:Property","owl:ObjectProperty"],"rdfs:label":"applicableQuantity","schema:rangeIncludes":{"@id":"unece:QuantityType"},"schema:domainIncludes":{"@id":"unece:SpecifiedMaterial"},"rdfs:comment":""},{"@id":"unece:applicableWasteMaterialRecoveryDisposalProcess","@type":["rdf:Property","owl:ObjectProperty"],"rdfs:label":"applicableWasteMaterialRecoveryDisposalProcess","schema:rangeIncludes":{"@id":"unece:WasteMaterialRecoveryDisposalProcess"},"schema:domainIncludes":{"@id":"unece:SpecifiedMaterial"},"rdfs:comment":"A waste material recovery disposal process applicable to this specified material."},{"@id":"unece:classificationId","@type":["rdf:Property","owl:DatatypeProperty"],"rdfs:label":"classificationId","schema:rangeIncludes":{"@id":"schema:Text"},"schema:domainIncludes":{"@id":"unece:SpecifiedMaterial"},"rdfs:comment":"An identifier of the classification of this specified material."},{"@id":"unece:manufacturerParty","@type":["rdf:Property","owl:ObjectProperty"],"rdfs:label":"manufacturerParty","schema:rangeIncludes":{"@id":"unece:Party"},"schema:domainIncludes":{"@id":"unece:SpecifiedMaterial"},"rdfs:comment":""},{"@id":"unece:transportInstructionsDescriptionCode","@type":["rdf:Property","owl:DatatypeProperty"],"rdfs:label":"transportInstructionsDescriptionCode","schema:rangeIncludes":{"@id":"schema:Text"},"schema:domainIncludes":{"@id":"unece:TransportInstructions"},"rdfs:comment":"The code specifying a description of these transport instructions."},{"@id":"unece:issuingParty","@type":["rdf:Property","owl:ObjectProperty"],"rdfs:label":"issuingParty","schema:rangeIncludes":{"@id":"unece:Party"},"schema:domainIncludes":{"@id":"unece:Seal"},"rdfs:comment":""},{"@id":"unece:logisticsSealTypeCode","@type":["rdf:Property","owl:DatatypeProperty"],"rdfs:label":"logisticsSealTypeCode","schema:rangeIncludes":{"@id":"schema:Text"},"schema:domainIncludes":{"@id":"unece:Seal"},"rdfs:comment":"The code specifying the type of logistics seal."},{"@id":"unece:logisticsSealingPartyRoleCode","@type":["rdf:Property","owl:DatatypeProperty"],"rdfs:label":"logisticsSealingPartyRoleCode","schema:rangeIncludes":{"@id":"unece:SealingPartyRoleCodeList"},"schema:domainIncludes":{"@id":"unece:Seal"},"rdfs:comment":"The code specifying the role of the party responsible for the sealing of this logistics seal."},{"@id":"unece:maximumId","@type":["rdf:Property","owl:DatatypeProperty"],"rdfs:label":"maximumId","schema:rangeIncludes":{"@id":"schema:Text"},"schema:domainIncludes":{"@id":"unece:Seal"},"rdfs:comment":"The maximum unique identifier used for these logistics seals."},{"@id":"unece:sealConditionCode","@type":["rdf:Property","owl:DatatypeProperty"],"rdfs:label":"sealConditionCode","schema:rangeIncludes":{"@id":"unece:SealConditionCodeList"},"schema:domainIncludes":{"@id":"unece:Seal"},"rdfs:comment":"A code specifying a condition of this logistics seal."},{"@id":"unece:lowerLimitActualMeasure","@type":["rdf:Property","owl:ObjectProperty"],"rdfs:label":"lowerLimitActualMeasure","schema:rangeIncludes":{"@id":"unece:MeasureType"},"schema:domainIncludes":{"@id":"unece:IngredientRangeMeasurement"},"rdfs:comment":""},{"@id":"unece:lowerLimitComparisonOperatorCode","@type":["rdf:Property","owl:DatatypeProperty"],"rdfs:label":"lowerLimitComparisonOperatorCode","schema:rangeIncludes":{"@id":"schema:Text"},"schema:domainIncludes":{"@id":"unece:IngredientRangeMeasurement"},"rdfs:comment":"The code specifying the comparison operator for the lower limit of this ingredient range measurement."},{"@id":"unece:lowerLimitPressureConditionMeasure","@type":["rdf:Property","owl:ObjectProperty"],"rdfs:label":"lowerLimitPressureConditionMeasure","schema:rangeIncludes":{"@id":"unece:MeasureType"},"schema:domainIncludes":{"@id":"unece:IngredientRangeMeasurement"},"rdfs:comment":""},{"@id":"unece:upperLimitActualMeasure","@type":["rdf:Property","owl:ObjectProperty"],"rdfs:label":"upperLimitActualMeasure","schema:rangeIncludes":{"@id":"unece:MeasureType"},"schema:domainIncludes":{"@id":"unece:IngredientRangeMeasurement"},"rdfs:comment":""},{"@id":"unece:upperLimitComparisonOperatorCode","@type":["rdf:Property","owl:DatatypeProperty"],"rdfs:label":"upperLimitComparisonOperatorCode","schema:rangeIncludes":{"@id":"schema:Text"},"schema:domainIncludes":{"@id":"unece:IngredientRangeMeasurement"},"rdfs:comment":"The code specifying the comparison operator for the upper limit of this ingredient range measurement."},{"@id":"unece:upperLimitPressureConditionMeasure","@type":["rdf:Property","owl:ObjectProperty"],"rdfs:label":"upperLimitPressureConditionMeasure","schema:rangeIncludes":{"@id":"unece:MeasureType"},"schema:domainIncludes":{"@id":"unece:IngredientRangeMeasurement"},"rdfs:comment":""},{"@id":"unece:applicableProductionWasteRecoveryDisposalProcess","@type":["rdf:Property","owl:ObjectProperty"],"rdfs:label":"applicableProductionWasteRecoveryDisposalProcess","schema:rangeIncludes":{"@id":"unece:ProductionWasteRecoveryDisposalProcess"},"schema:domainIncludes":{"@id":"unece:ProductionWasteMaterial"},"rdfs:comment":"A production waste recovery disposal process applicable to this production waste material."},{"@id":"unece:includedProductionWasteMaterialComponent","@type":["rdf:Property","owl:ObjectProperty"],"rdfs:label":"includedProductionWasteMaterialComponent","schema:rangeIncludes":{"@id":"unece:ProductionWasteMaterialComponent"},"schema:domainIncludes":{"@id":"unece:ProductionWasteMaterial"},"rdfs:comment":"A production waste material component included in this production waste material."},{"@id":"unece:specifiedProcessCertificate","@type":["rdf:Property","owl:ObjectProperty"],"rdfs:label":"specifiedProcessCertificate","schema:rangeIncludes":{"@id":"unece:ProcessCertificate"},"schema:domainIncludes":{"@id":"unece:ProductionWasteRecoveryDisposalProcess"},"rdfs:comment":"A process certificate for this specified chemical treatment."}]}