{"@context":{"rdf":"http://www.w3.org/1999/02/22-rdf-syntax-ns#","owl":"http://www.w3.org/2002/07/owl#","rdfs":"http://www.w3.org/2000/01/rdf-schema#","schema":"https://schema.org/","unece":"https://vocabulary.uncefact.org/"},"@graph":[{"@id":"unece:GuestPerson","@type":"rdfs:Class","rdfs:label":"GuestPerson","schema:source":{"@id":"https://vocabulary.uncefact.org/GuestPerson"},"rdfs:comment":"An individual guest."},{"@id":"unece:ExperienceProgramAction","@type":"rdfs:Class","rdfs:label":"ExperienceProgramAction","schema:source":{"@id":"https://vocabulary.uncefact.org/ExperienceProgramAction"},"rdfs:comment":"Any type of action, such as searching, reserving, or paying, necessary for an experience program, such as an adventure experience, a business experience, or a wellness experience."},{"@id":"unece:PetAnimal","@type":"rdfs:Class","rdfs:label":"PetAnimal","schema:source":{"@id":"https://vocabulary.uncefact.org/PetAnimal"},"rdfs:comment":"A domestic or tamed animal that is kept for companionship or pleasure."},{"@id":"unece:ExperienceItem","@type":"rdfs:Class","rdfs:label":"ExperienceItem","schema:source":{"@id":"https://vocabulary.uncefact.org/ExperienceItem"},"rdfs:comment":"A collection of information specific to the involvement of a person or persons in a happening, such as a theme park, a guided tour being used or reported on for trade purposes."},{"@id":"unece:ExperienceProduct","@type":"rdfs:Class","rdfs:label":"ExperienceProduct","schema:source":{"@id":"https://vocabulary.uncefact.org/ExperienceProduct"},"rdfs:comment":"Any service that provides an involvement, such as an adventure experience, wellness experience, social or business activity experience."},{"@id":"unece:ExperienceEvent","@type":"rdfs:Class","rdfs:label":"ExperienceEvent","schema:source":{"@id":"https://vocabulary.uncefact.org/ExperienceEvent"},"rdfs:comment":"An involvement in an experience program in which some thing happens, such as a nature watching, woodware manufacturing, meditation, holiday trip, dinner, theme park visit, could be experienced."},{"@id":"unece:ExperienceFacility","@type":"rdfs:Class","rdfs:label":"ExperienceFacility","schema:source":{"@id":"https://vocabulary.uncefact.org/ExperienceFacility"},"rdfs:comment":"A structure or place, such as a restaurant, hotel, theme park, hot spring bathing pool, parking lot, or meeting room, that provides a particular experience."},{"@id":"unece:GuestArrival","@type":"rdfs:Class","rdfs:label":"GuestArrival","schema:source":{"@id":"https://vocabulary.uncefact.org/GuestArrival"},"rdfs:comment":"The act of coming to or reaching a place by a specified guest."},{"@id":"unece:Allergy","@type":"rdfs:Class","rdfs:label":"Allergy","schema:source":{"@id":"https://vocabulary.uncefact.org/Allergy"},"rdfs:comment":"A guest condition of the abnormal reaction of the body to a previously encountered substance introduced by inhalation, ingestion, injection, or skin contact."},{"@id":"unece:CarriedEquipment","@type":"rdfs:Class","rdfs:label":"CarriedEquipment","schema:source":{"@id":"https://vocabulary.uncefact.org/CarriedEquipment"},"rdfs:comment":"A tool or device carried by a guest for an activity."},{"@id":"unece:Disability","@type":"rdfs:Class","rdfs:label":"Disability","schema:source":{"@id":"https://vocabulary.uncefact.org/Disability"},"rdfs:comment":"A physical or mental condition that limits a guest's movements, senses, or activities."},{"@id":"unece:FoodChoice","@type":"rdfs:Class","rdfs:label":"FoodChoice","schema:source":{"@id":"https://vocabulary.uncefact.org/FoodChoice"},"rdfs:comment":"A guest's decision which food to buy or eat."},{"@id":"unece:GuestHealthIndication","@type":"rdfs:Class","rdfs:label":"GuestHealthIndication","schema:source":{"@id":"https://vocabulary.uncefact.org/GuestHealthIndication"},"rdfs:comment":"A guest's physical or mental condition."},{"@id":"unece:PersonalEffects","@type":"rdfs:Class","rdfs:label":"PersonalEffects","schema:source":{"@id":"https://vocabulary.uncefact.org/PersonalEffects"},"rdfs:comment":"Specified privately owned articles for personal use by an individual."},{"@id":"unece:Preference","@type":"rdfs:Class","rdfs:label":"Preference","schema:source":{"@id":"https://vocabulary.uncefact.org/Preference"},"rdfs:comment":"An involvement in a happening, such as a theme park, a guided tour that is liked or wanted more than another item."},{"@id":"unece:accompanyingAnimal","@type":["rdf:Property","owl:ObjectProperty"],"rdfs:label":"accompanyingAnimal","schema:rangeIncludes":{"@id":"unece:PetAnimal"},"schema:domainIncludes":{"@id":"unece:GuestPerson"},"rdfs:comment":"A pet animal accompanying this guest person."},{"@id":"unece:applicableSpecifiedNote","@type":["rdf:Property","owl:ObjectProperty"],"rdfs:label":"applicableSpecifiedNote","schema:rangeIncludes":{"@id":"unece:SpecifiedNote"},"schema:domainIncludes":[{"@id":"unece:GuestPerson"},{"@id":"unece:ExperienceProduct"},{"@id":"unece:ExperienceEvent"}],"rdfs:comment":"A note applicable for this experience product."},{"@id":"unece:birthDateTime","@type":["rdf:Property","owl:DatatypeProperty"],"rdfs:label":"birthDateTime","schema:rangeIncludes":{"@id":"xsd:string"},"schema:domainIncludes":{"@id":"unece:GuestPerson"},"rdfs:comment":"The birth date for this individual TT animal."},{"@id":"unece:carriedCertificate","@type":["rdf:Property","owl:ObjectProperty"],"rdfs:label":"carriedCertificate","schema:rangeIncludes":{"@id":"unece:SpecifiedCertificate"},"schema:domainIncludes":{"@id":"unece:GuestPerson"},"rdfs:comment":"A certificate carried by this guest person."},{"@id":"unece:claimedLanguageProficiency","@type":["rdf:Property","owl:ObjectProperty"],"rdfs:label":"claimedLanguageProficiency","schema:rangeIncludes":{"@id":"unece:LanguageProficiency"},"schema:domainIncludes":{"@id":"unece:GuestPerson"},"rdfs:comment":"Personal language proficiency skills claimed by this found stowaway."},{"@id":"unece:description","@type":["rdf:Property","owl:DatatypeProperty"],"rdfs:label":"description","schema:rangeIncludes":{"@id":"xsd:string"},"schema:domainIncludes":[{"@id":"unece:GuestPerson"},{"@id":"unece:ExperienceProgramAction"},{"@id":"unece:PetAnimal"},{"@id":"unece:ExperienceItem"},{"@id":"unece:ExperienceProduct"},{"@id":"unece:ExperienceEvent"},{"@id":"unece:ExperienceFacility"},{"@id":"unece:Allergy"},{"@id":"unece:CarriedEquipment"},{"@id":"unece:Disability"},{"@id":"unece:FoodChoice"},{"@id":"unece:GuestHealthIndication"},{"@id":"unece:PersonalEffects"},{"@id":"unece:Preference"}],"rdfs:comment":"A textual description for the type of transportation waste recovery disposal process."},{"@id":"unece:durationUnitAgeMeasure","@type":["rdf:Property","owl:ObjectProperty"],"rdfs:label":"durationUnitAgeMeasure","schema:rangeIncludes":{"@id":"unece:DurationUnitMeasureType"},"schema:domainIncludes":{"@id":"unece:GuestPerson"},"rdfs:comment":"The measure of the age of this guest person."},{"@id":"unece:genderCode","@type":["rdf:Property","owl:DatatypeProperty"],"rdfs:label":"genderCode","schema:rangeIncludes":{"@id":"xsd:string"},"schema:domainIncludes":{"@id":"unece:GuestPerson"},"rdfs:comment":"A code specifying the gender of this transport person."},{"@id":"unece:identifier","@type":["rdf:Property","owl:DatatypeProperty"],"rdfs:label":"identifier","schema:rangeIncludes":{"@id":"xsd:string"},"schema:domainIncludes":[{"@id":"unece:GuestPerson"},{"@id":"unece:ExperienceItem"},{"@id":"unece:ExperienceProduct"},{"@id":"unece:ExperienceEvent"},{"@id":"unece:ExperienceFacility"}],"rdfs:comment":"A proprietary identifier."},{"@id":"unece:languageId","@type":["rdf:Property","owl:DatatypeProperty"],"rdfs:label":"languageId","schema:rangeIncludes":{"@id":"xsd:string"},"schema:domainIncludes":{"@id":"unece:GuestPerson"},"rdfs:comment":"A unique identifier for a language used in this exchanged document."},{"@id":"unece:name","@type":["rdf:Property","owl:DatatypeProperty"],"rdfs:label":"name","schema:rangeIncludes":{"@id":"xsd:string"},"schema:domainIncludes":[{"@id":"unece:GuestPerson"},{"@id":"unece:ExperienceItem"},{"@id":"unece:ExperienceProduct"},{"@id":"unece:ExperienceEvent"},{"@id":"unece:ExperienceFacility"},{"@id":"unece:Allergy"},{"@id":"unece:CarriedEquipment"},{"@id":"unece:Disability"},{"@id":"unece:FoodChoice"}],"owl:equivalentProperty":{"@id":"schema:name"},"rdfs:comment":"A name or symbol, expressed as text, of a radioactive radionuclide."},{"@id":"unece:notifiedAllergy","@type":["rdf:Property","owl:ObjectProperty"],"rdfs:label":"notifiedAllergy","schema:rangeIncludes":{"@id":"unece:Allergy"},"schema:domainIncludes":{"@id":"unece:GuestPerson"},"rdfs:comment":"An allergy notified for this guest person."},{"@id":"unece:notifiedDisability","@type":["rdf:Property","owl:ObjectProperty"],"rdfs:label":"notifiedDisability","schema:rangeIncludes":{"@id":"unece:Disability"},"schema:domainIncludes":{"@id":"unece:GuestPerson"},"rdfs:comment":"A disability notified for this guest person."},{"@id":"unece:notifiedFoodChoice","@type":["rdf:Property","owl:ObjectProperty"],"rdfs:label":"notifiedFoodChoice","schema:rangeIncludes":{"@id":"unece:FoodChoice"},"schema:domainIncludes":{"@id":"unece:GuestPerson"},"rdfs:comment":"A food choice notified for this guest person."},{"@id":"unece:notifiedGuestArrival","@type":["rdf:Property","owl:ObjectProperty"],"rdfs:label":"notifiedGuestArrival","schema:rangeIncludes":{"@id":"unece:GuestArrival"},"schema:domainIncludes":{"@id":"unece:GuestPerson"},"rdfs:comment":"An arrival notified for this guest person."},{"@id":"unece:notifiedHealthIndication","@type":["rdf:Property","owl:ObjectProperty"],"rdfs:label":"notifiedHealthIndication","schema:rangeIncludes":{"@id":"unece:GuestHealthIndication"},"schema:domainIncludes":{"@id":"unece:GuestPerson"},"rdfs:comment":"A health indication notified for this guest person."},{"@id":"unece:notifiedPreference","@type":["rdf:Property","owl:ObjectProperty"],"rdfs:label":"notifiedPreference","schema:rangeIncludes":{"@id":"unece:Preference"},"schema:domainIncludes":{"@id":"unece:GuestPerson"},"rdfs:comment":"An experience item preference notified for this guest person."},{"@id":"unece:notifiedProtectionMeans","@type":["rdf:Property","owl:ObjectProperty"],"rdfs:label":"notifiedProtectionMeans","schema:rangeIncludes":{"@id":"unece:ProtectionMeans"},"schema:domainIncludes":{"@id":"unece:GuestPerson"},"rdfs:comment":"A disease protection means notified for this guest person."},{"@id":"unece:passportId","@type":["rdf:Property","owl:DatatypeProperty"],"rdfs:label":"passportId","schema:rangeIncludes":{"@id":"xsd:string"},"schema:domainIncludes":{"@id":"unece:GuestPerson"},"rdfs:comment":"The identifier of the passport of this guest."},{"@id":"unece:raisedQuery","@type":["rdf:Property","owl:ObjectProperty"],"rdfs:label":"raisedQuery","schema:rangeIncludes":{"@id":"unece:SpecialQuery"},"schema:domainIncludes":{"@id":"unece:GuestPerson"},"rdfs:comment":"A special query raised for this guest person."},{"@id":"unece:residenceCountryId","@type":["rdf:Property","owl:DatatypeProperty"],"rdfs:label":"residenceCountryId","schema:rangeIncludes":{"@id":"xsd:string"},"schema:domainIncludes":{"@id":"unece:GuestPerson"},"rdfs:comment":"The identifier for the country of residence for this TT party, such as the country in which a person lives or in which a corporation has its place of incorporation."},{"@id":"unece:roleCode","@type":["rdf:Property","owl:DatatypeProperty"],"rdfs:label":"roleCode","schema:rangeIncludes":{"@id":"xsd:string"},"schema:domainIncludes":{"@id":"unece:GuestPerson"},"rdfs:comment":"The code specifying the role for this cooperating organization."},{"@id":"unece:specifiedCarriedEquipment","@type":["rdf:Property","owl:ObjectProperty"],"rdfs:label":"specifiedCarriedEquipment","schema:rangeIncludes":{"@id":"unece:CarriedEquipment"},"schema:domainIncludes":{"@id":"unece:GuestPerson"},"rdfs:comment":"Carried equipment specified for this guest person."},{"@id":"unece:specifiedPaymentMeans","@type":["rdf:Property","owl:ObjectProperty"],"rdfs:label":"specifiedPaymentMeans","schema:rangeIncludes":{"@id":"unece:PaymentMeans"},"schema:domainIncludes":{"@id":"unece:GuestPerson"},"rdfs:comment":"A payment means specified for this header trade settlement."},{"@id":"unece:title","@type":["rdf:Property","owl:DatatypeProperty"],"rdfs:label":"title","schema:rangeIncludes":{"@id":"xsd:string"},"schema:domainIncludes":{"@id":"unece:GuestPerson"},"rdfs:comment":"A title, expressed as text, for this specified binary file."},{"@id":"unece:titleCode","@type":["rdf:Property","owl:DatatypeProperty"],"rdfs:label":"titleCode","schema:rangeIncludes":{"@id":"xsd:string"},"schema:domainIncludes":{"@id":"unece:GuestPerson"},"rdfs:comment":"The code specifying the title of this guest person."},{"@id":"unece:travelInsuranceCertificate","@type":["rdf:Property","owl:ObjectProperty"],"rdfs:label":"travelInsuranceCertificate","schema:rangeIncludes":{"@id":"unece:SpecifiedCertificate"},"schema:domainIncludes":{"@id":"unece:GuestPerson"},"rdfs:comment":"A travel insurance certificate for this guest person."},{"@id":"unece:usedCommunication","@type":["rdf:Property","owl:ObjectProperty"],"rdfs:label":"usedCommunication","schema:rangeIncludes":{"@id":"unece:Communication"},"schema:domainIncludes":{"@id":"unece:GuestPerson"},"rdfs:comment":"A communication used by this trade contact."},{"@id":"unece:actionType","@type":["rdf:Property","owl:DatatypeProperty"],"rdfs:label":"actionType","schema:rangeIncludes":{"@id":"xsd:string"},"schema:domainIncludes":{"@id":"unece:ExperienceProgramAction"},"rdfs:comment":"A type, expressed as text, for this corrective action."},{"@id":"unece:specifiedTradeParty","@type":["rdf:Property","owl:ObjectProperty"],"rdfs:label":"specifiedTradeParty","schema:rangeIncludes":{"@id":"unece:Party"},"schema:domainIncludes":[{"@id":"unece:ExperienceProgramAction"},{"@id":"unece:ExperienceItem"},{"@id":"unece:ExperienceProduct"},{"@id":"unece:ExperienceEvent"}],"rdfs:comment":"A party specified for this experience event."},{"@id":"unece:statusCode","@type":["rdf:Property","owl:DatatypeProperty"],"rdfs:label":"statusCode","schema:rangeIncludes":{"@id":"xsd:string"},"schema:domainIncludes":[{"@id":"unece:ExperienceProgramAction"},{"@id":"unece:ExperienceItem"}],"rdfs:comment":"A code specifying a status for this trade product."},{"@id":"unece:typeCode","@type":["rdf:Property","owl:DatatypeProperty"],"rdfs:label":"typeCode","schema:rangeIncludes":{"@id":"xsd:string"},"schema:domainIncludes":[{"@id":"unece:ExperienceProgramAction"},{"@id":"unece:ExperienceFacility"},{"@id":"unece:Allergy"},{"@id":"unece:CarriedEquipment"},{"@id":"unece:Disability"},{"@id":"unece:FoodChoice"},{"@id":"unece:GuestHealthIndication"},{"@id":"unece:PersonalEffects"}],"rdfs:comment":"A code specifying a type of MDH health indication."},{"@id":"unece:allowedIndicator","@type":["rdf:Property","owl:DatatypeProperty"],"rdfs:label":"allowedIndicator","schema:rangeIncludes":{"@id":"xsd:boolean"},"schema:domainIncludes":{"@id":"unece:PetAnimal"},"rdfs:comment":"The indication of whether or not this pet animal is allowed."},{"@id":"unece:categoryCode","@type":["rdf:Property","owl:DatatypeProperty"],"rdfs:label":"categoryCode","schema:rangeIncludes":{"@id":"xsd:string"},"schema:domainIncludes":[{"@id":"unece:PetAnimal"},{"@id":"unece:ExperienceItem"},{"@id":"unece:ExperienceProduct"}],"rdfs:comment":"A code specifying a category for this cross-border regulatory procedure, such as the appendices of the CITES Convention."},{"@id":"unece:restriction","@type":["rdf:Property","owl:DatatypeProperty"],"rdfs:label":"restriction","schema:rangeIncludes":{"@id":"xsd:string"},"schema:domainIncludes":[{"@id":"unece:PetAnimal"},{"@id":"unece:Allergy"},{"@id":"unece:CarriedEquipment"},{"@id":"unece:Disability"},{"@id":"unece:FoodChoice"},{"@id":"unece:GuestHealthIndication"}],"rdfs:comment":"A restriction, expressed as text, for this disease protection means."},{"@id":"unece:applicablePeriod","@type":["rdf:Property","owl:ObjectProperty"],"rdfs:label":"applicablePeriod","schema:rangeIncludes":{"@id":"unece:SpecifiedPeriod"},"schema:domainIncludes":{"@id":"unece:ExperienceItem"},"rdfs:comment":"A period applicable to this cross-border regulatory procedure."},{"@id":"unece:applicableQuantityUnitTypeCode","@type":["rdf:Property","owl:DatatypeProperty"],"rdfs:label":"applicableQuantityUnitTypeCode","schema:rangeIncludes":{"@id":"xsd:string"},"schema:domainIncludes":[{"@id":"unece:ExperienceItem"},{"@id":"unece:ExperienceProduct"}],"rdfs:comment":"The code specifying the type of quantity unit applicable for this experience product."},{"@id":"unece:availablePeriod","@type":["rdf:Property","owl:ObjectProperty"],"rdfs:label":"availablePeriod","schema:rangeIncludes":{"@id":"unece:SpecifiedPeriod"},"schema:domainIncludes":{"@id":"unece:ExperienceItem"},"rdfs:comment":"An available period for this specified experience item."},{"@id":"unece:availableProduct","@type":["rdf:Property","owl:ObjectProperty"],"rdfs:label":"availableProduct","schema:rangeIncludes":{"@id":"unece:ExperienceProduct"},"schema:domainIncludes":{"@id":"unece:ExperienceItem"},"rdfs:comment":"An available product for this specified experience item."},{"@id":"unece:availableUnitQuantity","@type":["rdf:Property","owl:ObjectProperty"],"rdfs:label":"availableUnitQuantity","schema:rangeIncludes":{"@id":"unece:QuantityType"},"schema:domainIncludes":{"@id":"unece:ExperienceItem"},"rdfs:comment":"The number of units available for this specified experience item."},{"@id":"unece:brandName","@type":["rdf:Property","owl:DatatypeProperty"],"rdfs:label":"brandName","schema:rangeIncludes":{"@id":"xsd:string"},"schema:domainIncludes":[{"@id":"unece:ExperienceItem"},{"@id":"unece:ExperienceProduct"}],"rdfs:comment":"A brand name, expressed as text, for this experience product."},{"@id":"unece:calculatedPrice","@type":["rdf:Property","owl:ObjectProperty"],"rdfs:label":"calculatedPrice","schema:rangeIncludes":{"@id":"unece:TradePrice"},"schema:domainIncludes":[{"@id":"unece:ExperienceItem"},{"@id":"unece:ExperienceProduct"},{"@id":"unece:ExperienceEvent"}],"rdfs:comment":"A calculated price for this experience event."},{"@id":"unece:capabilityLevel","@type":["rdf:Property","owl:DatatypeProperty"],"rdfs:label":"capabilityLevel","schema:rangeIncludes":{"@id":"xsd:string"},"schema:domainIncludes":{"@id":"unece:ExperienceItem"},"rdfs:comment":"A capability level, expressed as text, for this specified experience item."},{"@id":"unece:destination","@type":["rdf:Property","owl:DatatypeProperty"],"rdfs:label":"destination","schema:rangeIncludes":{"@id":"xsd:string"},"schema:domainIncludes":{"@id":"unece:ExperienceItem"},"rdfs:comment":"A destination, expressed as text, for this specified experience item."},{"@id":"unece:guestSpecialCareIndicator","@type":["rdf:Property","owl:DatatypeProperty"],"rdfs:label":"guestSpecialCareIndicator","schema:rangeIncludes":{"@id":"xsd:boolean"},"schema:domainIncludes":{"@id":"unece:ExperienceItem"},"rdfs:comment":"The indication of whether or not guest special care is applicable for this specified experience item."},{"@id":"unece:indemnityClause","@type":["rdf:Property","owl:DatatypeProperty"],"rdfs:label":"indemnityClause","schema:rangeIncludes":{"@id":"xsd:string"},"schema:domainIncludes":[{"@id":"unece:ExperienceItem"},{"@id":"unece:ExperienceProduct"},{"@id":"unece:ExperienceEvent"}],"rdfs:comment":"An indemnity clause, expressed as text, for this experience event."},{"@id":"unece:instruction","@type":["rdf:Property","owl:DatatypeProperty"],"rdfs:label":"instruction","schema:rangeIncludes":{"@id":"xsd:string"},"schema:domainIncludes":[{"@id":"unece:ExperienceItem"},{"@id":"unece:ExperienceProduct"},{"@id":"unece:ExperienceEvent"}],"rdfs:comment":"An instruction, expressed as text, for this experience event."},{"@id":"unece:lowerPriceLimitAmount","@type":["rdf:Property","owl:ObjectProperty"],"rdfs:label":"lowerPriceLimitAmount","schema:rangeIncludes":{"@id":"unece:AmountType"},"schema:domainIncludes":{"@id":"unece:ExperienceItem"},"rdfs:comment":"A monetary value of a lower price limit of this specified experience item."},{"@id":"unece:maximumGuestQuantity","@type":["rdf:Property","owl:ObjectProperty"],"rdfs:label":"maximumGuestQuantity","schema:rangeIncludes":{"@id":"unece:QuantityType"},"schema:domainIncludes":{"@id":"unece:ExperienceItem"},"rdfs:comment":"The maximum number of guests for this specified experience item."},{"@id":"unece:minimumGuestQuantity","@type":["rdf:Property","owl:ObjectProperty"],"rdfs:label":"minimumGuestQuantity","schema:rangeIncludes":{"@id":"unece:QuantityType"},"schema:domainIncludes":{"@id":"unece:ExperienceItem"},"rdfs:comment":"The minimum number of guests for this specified experience item."},{"@id":"unece:reservationGuarantee","@type":["rdf:Property","owl:DatatypeProperty"],"rdfs:label":"reservationGuarantee","schema:rangeIncludes":{"@id":"xsd:string"},"schema:domainIncludes":[{"@id":"unece:ExperienceItem"},{"@id":"unece:ExperienceProduct"},{"@id":"unece:ExperienceEvent"}],"rdfs:comment":"A reservation guarantee, expressed as text, for this experience event."},{"@id":"unece:responseStatusCode","@type":["rdf:Property","owl:DatatypeProperty"],"rdfs:label":"responseStatusCode","schema:rangeIncludes":{"@id":"xsd:string"},"schema:domainIncludes":{"@id":"unece:ExperienceItem"},"rdfs:comment":"The code specifying the response status for this special query."},{"@id":"unece:theme","@type":["rdf:Property","owl:DatatypeProperty"],"rdfs:label":"theme","schema:rangeIncludes":{"@id":"xsd:string"},"schema:domainIncludes":[{"@id":"unece:ExperienceItem"},{"@id":"unece:ExperienceProduct"}],"rdfs:comment":"A theme, expressed as text, for this experience product."},{"@id":"unece:themeTypeCode","@type":["rdf:Property","owl:DatatypeProperty"],"rdfs:label":"themeTypeCode","schema:rangeIncludes":{"@id":"xsd:string"},"schema:domainIncludes":[{"@id":"unece:ExperienceItem"},{"@id":"unece:ExperienceProduct"}],"rdfs:comment":"The code specifying the type of theme for this experience product."},{"@id":"unece:unitQuantity","@type":["rdf:Property","owl:ObjectProperty"],"rdfs:label":"unitQuantity","schema:rangeIncludes":{"@id":"unece:QuantityType"},"schema:domainIncludes":{"@id":"unece:ExperienceItem"},"rdfs:comment":"A number of units for this supply chain event."},{"@id":"unece:upperPriceLimitAmount","@type":["rdf:Property","owl:ObjectProperty"],"rdfs:label":"upperPriceLimitAmount","schema:rangeIncludes":{"@id":"unece:AmountType"},"schema:domainIncludes":{"@id":"unece:ExperienceItem"},"rdfs:comment":"A monetary value of an upper price limit of this specified experience item."},{"@id":"unece:visitingPeriod","@type":["rdf:Property","owl:ObjectProperty"],"rdfs:label":"visitingPeriod","schema:rangeIncludes":{"@id":"unece:SpecifiedPeriod"},"schema:domainIncludes":{"@id":"unece:ExperienceItem"},"rdfs:comment":"A visiting period for this specified experience item."},{"@id":"unece:certifiedPersonArrangementIndicator","@type":["rdf:Property","owl:DatatypeProperty"],"rdfs:label":"certifiedPersonArrangementIndicator","schema:rangeIncludes":{"@id":"xsd:boolean"},"schema:domainIncludes":{"@id":"unece:ExperienceProduct"},"rdfs:comment":"The indication of whether or not a certified person arrangement is made for this experience product."},{"@id":"unece:distinctiveFeature","@type":["rdf:Property","owl:ObjectProperty"],"rdfs:label":"distinctiveFeature","schema:rangeIncludes":{"@id":"unece:SpecifiedFeature"},"schema:domainIncludes":[{"@id":"unece:ExperienceProduct"},{"@id":"unece:ExperienceEvent"}],"rdfs:comment":"A distinctive feature of this experience product."},{"@id":"unece:includedEvent","@type":["rdf:Property","owl:ObjectProperty"],"rdfs:label":"includedEvent","schema:rangeIncludes":{"@id":"unece:ExperienceEvent"},"schema:domainIncludes":{"@id":"unece:ExperienceProduct"},"rdfs:comment":"An event included within this experience product."},{"@id":"unece:location","@type":["rdf:Property","owl:DatatypeProperty"],"rdfs:label":"location","schema:rangeIncludes":{"@id":"xsd:string"},"schema:domainIncludes":[{"@id":"unece:ExperienceProduct"},{"@id":"unece:ExperienceEvent"}],"rdfs:comment":"A location, expressed as text, for this MDH sanitary measure."},{"@id":"unece:maximumUnitQuantity","@type":["rdf:Property","owl:ObjectProperty"],"rdfs:label":"maximumUnitQuantity","schema:rangeIncludes":{"@id":"unece:QuantityType"},"schema:domainIncludes":{"@id":"unece:ExperienceProduct"},"rdfs:comment":"The maximum number of units of this experience product."},{"@id":"unece:minimumUnitQuantity","@type":["rdf:Property","owl:ObjectProperty"],"rdfs:label":"minimumUnitQuantity","schema:rangeIncludes":{"@id":"unece:QuantityType"},"schema:domainIncludes":{"@id":"unece:ExperienceProduct"},"rdfs:comment":"The minimum number of units of this experience product."},{"@id":"unece:objective","@type":["rdf:Property","owl:DatatypeProperty"],"rdfs:label":"objective","schema:rangeIncludes":{"@id":"xsd:string"},"schema:domainIncludes":{"@id":"unece:ExperienceProduct"},"rdfs:comment":"An objective, expressed as text, for this experience product."},{"@id":"unece:operationalPeriod","@type":["rdf:Property","owl:ObjectProperty"],"rdfs:label":"operationalPeriod","schema:rangeIncludes":{"@id":"unece:SpecifiedPeriod"},"schema:domainIncludes":[{"@id":"unece:ExperienceProduct"},{"@id":"unece:ExperienceEvent"}],"rdfs:comment":"A operational period for this experience product."},{"@id":"unece:optionalProduct","@type":["rdf:Property","owl:ObjectProperty"],"rdfs:label":"optionalProduct","schema:rangeIncludes":{"@id":"unece:ExperienceProduct"},"schema:domainIncludes":{"@id":"unece:ExperienceProduct"},"rdfs:comment":"An optional product for this experience product."},{"@id":"unece:providedCertificate","@type":["rdf:Property","owl:ObjectProperty"],"rdfs:label":"providedCertificate","schema:rangeIncludes":{"@id":"unece:SpecifiedCertificate"},"schema:domainIncludes":[{"@id":"unece:ExperienceProduct"},{"@id":"unece:ExperienceEvent"}],"rdfs:comment":"A certificate provided for this experience product."},{"@id":"unece:providedRequirement","@type":["rdf:Property","owl:ObjectProperty"],"rdfs:label":"providedRequirement","schema:rangeIncludes":{"@id":"unece:Requirement"},"schema:domainIncludes":[{"@id":"unece:ExperienceProduct"},{"@id":"unece:ExperienceEvent"}],"rdfs:comment":"A requirement provided for this experience product."},{"@id":"unece:requiredReservationGuaranteeIndicator","@type":["rdf:Property","owl:DatatypeProperty"],"rdfs:label":"requiredReservationGuaranteeIndicator","schema:rangeIncludes":{"@id":"xsd:boolean"},"schema:domainIncludes":{"@id":"unece:ExperienceProduct"},"rdfs:comment":"The indication of whether or not this experience product requires a reservation guarantee."},{"@id":"unece:requiredUsageCondition","@type":["rdf:Property","owl:ObjectProperty"],"rdfs:label":"requiredUsageCondition","schema:rangeIncludes":{"@id":"unece:UsageCondition"},"schema:domainIncludes":[{"@id":"unece:ExperienceProduct"},{"@id":"unece:ExperienceEvent"}],"rdfs:comment":"A required usage condition for this experience product."},{"@id":"unece:basicObjective","@type":["rdf:Property","owl:DatatypeProperty"],"rdfs:label":"basicObjective","schema:rangeIncludes":{"@id":"xsd:string"},"schema:domainIncludes":{"@id":"unece:ExperienceEvent"},"rdfs:comment":"A basic objective, expressed as text, for this experience event."},{"@id":"unece:breakUpDateTime","@type":["rdf:Property","owl:DatatypeProperty"],"rdfs:label":"breakUpDateTime","schema:rangeIncludes":{"@id":"xsd:string"},"schema:domainIncludes":{"@id":"unece:ExperienceEvent"},"rdfs:comment":"The break up date, time, date time, or other date time value for this experience event."},{"@id":"unece:choiceAllowedIndicator","@type":["rdf:Property","owl:DatatypeProperty"],"rdfs:label":"choiceAllowedIndicator","schema:rangeIncludes":{"@id":"xsd:boolean"},"schema:domainIncludes":{"@id":"unece:ExperienceEvent"},"rdfs:comment":"The indication of whether or not a choice is allowed for this experience event."},{"@id":"unece:dateSequenceNumeric","@type":["rdf:Property","owl:DatatypeProperty"],"rdfs:label":"dateSequenceNumeric","schema:rangeIncludes":{"@id":"xsd:string"},"schema:domainIncludes":{"@id":"unece:ExperienceEvent"},"rdfs:comment":"The date sequence number for this experience event."},{"@id":"unece:meetingDateTime","@type":["rdf:Property","owl:DatatypeProperty"],"rdfs:label":"meetingDateTime","schema:rangeIncludes":{"@id":"xsd:datetime"},"schema:domainIncludes":{"@id":"unece:ExperienceEvent"},"rdfs:comment":"The meeting date, time, date time, or other date time value for this experience event."},{"@id":"unece:reservationRequiredIndicator","@type":["rdf:Property","owl:DatatypeProperty"],"rdfs:label":"reservationRequiredIndicator","schema:rangeIncludes":{"@id":"xsd:boolean"},"schema:domainIncludes":{"@id":"unece:ExperienceEvent"},"rdfs:comment":"The indication of whether or not a reservation is required for this experience event."},{"@id":"unece:architecturalStyle","@type":["rdf:Property","owl:DatatypeProperty"],"rdfs:label":"architecturalStyle","schema:rangeIncludes":{"@id":"xsd:string"},"schema:domainIncludes":{"@id":"unece:ExperienceFacility"},"rdfs:comment":"An architectural style, expressed as text, of this experience facility."},{"@id":"unece:completionDateTime","@type":["rdf:Property","owl:DatatypeProperty"],"rdfs:label":"completionDateTime","schema:rangeIncludes":{"@id":"xsd:string"},"schema:domainIncludes":{"@id":"unece:ExperienceFacility"},"rdfs:comment":"The date of the completion of this experience facility."},{"@id":"unece:facilityType","@type":["rdf:Property","owl:DatatypeProperty"],"rdfs:label":"facilityType","schema:rangeIncludes":{"@id":"xsd:string"},"schema:domainIncludes":{"@id":"unece:ExperienceFacility"},"rdfs:comment":"A type, expressed as text, of this experience facility."},{"@id":"unece:latestRenovationDateTime","@type":["rdf:Property","owl:DatatypeProperty"],"rdfs:label":"latestRenovationDateTime","schema:rangeIncludes":{"@id":"xsd:string"},"schema:domainIncludes":{"@id":"unece:ExperienceFacility"},"rdfs:comment":"The date of the latest renovation of this experience facility."},{"@id":"unece:physicalSpecifiedLocation","@type":["rdf:Property","owl:ObjectProperty"],"rdfs:label":"physicalSpecifiedLocation","schema:rangeIncludes":{"@id":"unece:SpecifiedLocation"},"schema:domainIncludes":{"@id":"unece:ExperienceFacility"},"rdfs:comment":"A physical location specified for this experience facility."},{"@id":"unece:specifiedCommunication","@type":["rdf:Property","owl:ObjectProperty"],"rdfs:label":"specifiedCommunication","schema:rangeIncludes":{"@id":"unece:Communication"},"schema:domainIncludes":{"@id":"unece:ExperienceFacility"},"rdfs:comment":"A communication specified for this payment financial institution."},{"@id":"unece:usedSource","@type":["rdf:Property","owl:ObjectProperty"],"rdfs:label":"usedSource","schema:rangeIncludes":{"@id":"unece:Source"},"schema:domainIncludes":{"@id":"unece:ExperienceFacility"},"rdfs:comment":"A water source used by this experience facility."},{"@id":"unece:carrierId","@type":["rdf:Property","owl:DatatypeProperty"],"rdfs:label":"carrierId","schema:rangeIncludes":{"@id":"xsd:string"},"schema:domainIncludes":{"@id":"unece:GuestArrival"},"rdfs:comment":"The identifier of the carrier for this specified guest arrival."},{"@id":"unece:carrierName","@type":["rdf:Property","owl:DatatypeProperty"],"rdfs:label":"carrierName","schema:rangeIncludes":{"@id":"xsd:string"},"schema:domainIncludes":{"@id":"unece:GuestArrival"},"rdfs:comment":"A carrier's name, expressed as text, related to this specified guest arrival."},{"@id":"unece:expectedDateTime","@type":["rdf:Property","owl:DatatypeProperty"],"rdfs:label":"expectedDateTime","schema:rangeIncludes":{"@id":"xsd:datetime"},"schema:domainIncludes":{"@id":"unece:GuestArrival"},"rdfs:comment":"The date, time, date time, or other date time value when this specified guest arrival is expected."},{"@id":"unece:transportModeCode","@type":["rdf:Property","owl:DatatypeProperty"],"rdfs:label":"transportModeCode","schema:rangeIncludes":{"@id":"xsd:string"},"schema:domainIncludes":{"@id":"unece:GuestArrival"},"rdfs:comment":"The code specifying the mode, such as by air, sea, rail, road or inland waterway, for this logistics transport movement."},{"@id":"unece:specificationNote","@type":["rdf:Property","owl:ObjectProperty"],"rdfs:label":"specificationNote","schema:rangeIncludes":{"@id":"unece:SpecifiedNote"},"schema:domainIncludes":{"@id":"unece:CarriedEquipment"},"rdfs:comment":"A specification note for this guest carried equipment."},{"@id":"unece:registeredDateTime","@type":["rdf:Property","owl:DatatypeProperty"],"rdfs:label":"registeredDateTime","schema:rangeIncludes":{"@id":"xsd:datetime"},"schema:domainIncludes":{"@id":"unece:Disability"},"rdfs:comment":"The date, time, date time, or other date time value when this guest disability has been registered."},{"@id":"unece:requiredSupportingDevice","@type":["rdf:Property","owl:DatatypeProperty"],"rdfs:label":"requiredSupportingDevice","schema:rangeIncludes":{"@id":"xsd:string"},"schema:domainIncludes":{"@id":"unece:Disability"},"rdfs:comment":"A supporting device, expressed as text, for this required guest disability."},{"@id":"unece:status","@type":["rdf:Property","owl:DatatypeProperty"],"rdfs:label":"status","schema:rangeIncludes":{"@id":"xsd:string"},"schema:domainIncludes":{"@id":"unece:GuestHealthIndication"},"rdfs:comment":"A status, expressed as text, for this acknowledgement document."},{"@id":"unece:onboardQuantity","@type":["rdf:Property","owl:ObjectProperty"],"rdfs:label":"onboardQuantity","schema:rangeIncludes":{"@id":"unece:QuantityType"},"schema:domainIncludes":{"@id":"unece:PersonalEffects"},"rdfs:comment":"An onboard number of these specified personal effects."},{"@id":"unece:sequenceNumeric","@type":["rdf:Property","owl:DatatypeProperty"],"rdfs:label":"sequenceNumeric","schema:rangeIncludes":{"@id":"xsd:string"},"schema:domainIncludes":{"@id":"unece:PersonalEffects"},"rdfs:comment":"A sequence number for these specified personal effects."},{"@id":"unece:dislikedItem","@type":["rdf:Property","owl:DatatypeProperty"],"rdfs:label":"dislikedItem","schema:rangeIncludes":{"@id":"xsd:string"},"schema:domainIncludes":{"@id":"unece:Preference"},"rdfs:comment":"A disliked item, expressed as text, for this experience item preference."},{"@id":"unece:preferredItem","@type":["rdf:Property","owl:DatatypeProperty"],"rdfs:label":"preferredItem","schema:rangeIncludes":{"@id":"xsd:string"},"schema:domainIncludes":{"@id":"unece:Preference"},"rdfs:comment":"A preferred item, expressed as text, for this experience item preference."},{"@id":"unece:priorityRankingNumeric","@type":["rdf:Property","owl:DatatypeProperty"],"rdfs:label":"priorityRankingNumeric","schema:rangeIncludes":{"@id":"xsd:string"},"schema:domainIncludes":{"@id":"unece:Preference"},"rdfs:comment":"The priority ranking number for this experience item preference."}]}