
{
    "@context": {
        "unece": "https://service.unece.org/trade/uncefact/vocabulary/unece#",
        "rdf": "http://www.w3.org/1999/02/22-rdf-syntax-ns#",
        "rdfs": "http://www.w3.org/2000/01/rdf-schema#",
        "schema": "http://schema.org/",
        "transport": "https://service.unece.org/trade/uncefact/vocabulary/unece/transport#",
        "cefact": "https://service.unece.org/trade/uncefact/vocabulary/cefact#",
        "xsd": "http://www.w3.org/2001/XMLSchema#"
    },
    "@graph": [
        {
            "@id": "transport:AssociatedTransportEquipment",
            "@type": "rdfs:Class",
            "rdfs:comment": "A piece of transport equipment that is associated with another piece of transport equipment, such as a maritime container placed on a rail wagon for transportation.",
            "rdfs:label": "AssociatedTransportEquipment",
            "unece:cefactElementMetadata": [
                {
                    "@id": "cefact:Associated_TransportEquipment.Details",
                    "@type": "unece:AggregateBIE",
                    "unece:cefactUNId": "UN01004883",
                    "rdfs:comment": "A piece of transport equipment that is associated with another piece of transport equipment, such as a maritime container placed on a rail wagon for transportation."
                }
            ]
        },
        {
            "@id": "transport:AttachedTransportEquipment",
            "@type": "rdfs:Class",
            "rdfs:comment": "A piece of attached transport equipment, such as a chain or a tarpaulin.",
            "rdfs:label": "AttachedTransportEquipment",
            "unece:cefactElementMetadata": [
                {
                    "@id": "cefact:Attached_TransportEquipment.Details",
                    "@type": "unece:AggregateBIE",
                    "unece:cefactUNId": "UN01003416",
                    "rdfs:comment": "A piece of attached transport equipment, such as a chain or a tarpaulin."
                }
            ]
        },
        {
            "@id": "transport:CalculatedEmission",
            "@type": "rdfs:Class",
            "rdfs:comment": "A calculation of the pollution (including noise, heat, and radiation etc.) discharged into the environment by a residential, commercial, or industrial facility or by a means of transport, such as a vessel, aircraft or truck.",
            "rdfs:label": "CalculatedEmission",
            "unece:cefactElementMetadata": [
                {
                    "@id": "cefact:Calculated_Emission.Details",
                    "@type": "unece:AggregateBIE",
                    "unece:cefactUNId": "UN01010051",
                    "rdfs:comment": "A calculation of the pollution (including noise, heat, and radiation etc.) discharged into the environment by a residential, commercial, or industrial facility or by a means of transport, such as a vessel, aircraft or truck."
                }
            ]
        },
        {
            "@id": "transport:ForecastDeliverySchedule",
            "@type": "rdfs:Class",
            "rdfs:comment": "Specification of the forecasted delivery quantities and date/time values for a delivery schedule.",
            "rdfs:label": "ForecastDeliverySchedule",
            "unece:cefactElementMetadata": [
                {
                    "@id": "cefact:Forecast_DeliverySchedule.Details",
                    "@type": "unece:AggregateBIE",
                    "unece:cefactUNId": "UN01014938",
                    "rdfs:comment": "Specification of the forecasted delivery quantities and date/time values for a delivery schedule."
                }
            ]
        },
        {
            "@id": "transport:IdentifiedFault",
            "@type": "rdfs:Class",
            "rdfs:comment": "An identified defect or fault.",
            "rdfs:label": "IdentifiedFault",
            "unece:cefactElementMetadata": [
                {
                    "@id": "cefact:Identified_Fault.Details",
                    "@type": "unece:AggregateBIE",
                    "unece:cefactUNId": "UN01010065",
                    "rdfs:comment": "An identified defect or fault."
                }
            ]
        },
        {
            "@id": "transport:LogisticsPackaging",
            "@type": "rdfs:Class",
            "rdfs:comment": "Any wrapping or containment, such as a box or a barrel, whether or not any goods are contained within.",
            "rdfs:label": "LogisticsPackaging",
            "unece:cefactElementMetadata": [
                {
                    "@id": "cefact:Logistics_Packaging.Details",
                    "@type": "unece:AggregateBIE",
                    "unece:cefactUNId": "UN01014945",
                    "rdfs:comment": "Any wrapping or containment, such as a box or a barrel, whether or not any goods are contained within."
                }
            ]
        },
        {
            "@id": "transport:LogisticsShippingMarks",
            "@type": "rdfs:Class",
            "rdfs:comment": "Physical markings or labels on individual packages or transport units for logistics purposes.",
            "rdfs:label": "LogisticsShippingMarks",
            "unece:cefactElementMetadata": [
                {
                    "@id": "cefact:Logistics_ShippingMarks.Details",
                    "@type": "unece:AggregateBIE",
                    "unece:cefactUNId": "UN01003741",
                    "rdfs:comment": "Physical markings or labels on individual packages or transport units for logistics purposes."
                }
            ]
        },
        {
            "@id": "transport:LogisticsTransportEquipment",
            "@type": "rdfs:Class",
            "rdfs:comment": "A piece of equipment used to hold, protect or secure cargo for logistics purposes.",
            "rdfs:label": "LogisticsTransportEquipment",
            "unece:cefactElementMetadata": [
                {
                    "@id": "cefact:Logistics_TransportEquipment.Details",
                    "@type": "unece:AggregateBIE",
                    "unece:cefactUNId": "UN01003757",
                    "rdfs:comment": "A piece of equipment used to hold, protect or secure cargo for logistics purposes."
                }
            ]
        },
        {
            "@id": "transport:LogisticsTransportMeans",
            "@type": "rdfs:Class",
            "rdfs:comment": "The devices used to convey goods or other objects from place to place during logistics cargo movements.",
            "rdfs:label": "LogisticsTransportMeans",
            "unece:cefactElementMetadata": [
                {
                    "@id": "cefact:Logistics_TransportMeans.Details",
                    "@type": "unece:AggregateBIE",
                    "unece:cefactUNId": "UN01003819",
                    "rdfs:comment": "The devices used to convey goods or other objects from place to place during logistics cargo movements."
                }
            ]
        },
        {
            "@id": "transport:LogisticsTransportMovement",
            "@type": "rdfs:Class",
            "rdfs:comment": "The conveyance (physical carriage) of goods or other objects used for logistics transport purposes.",
            "rdfs:label": "LogisticsTransportMovement",
            "unece:cefactElementMetadata": [
                {
                    "@id": "cefact:Logistics_TransportMovement.Details",
                    "@type": "unece:AggregateBIE",
                    "unece:cefactUNId": "UN01003837",
                    "rdfs:comment": "The conveyance (physical carriage) of goods or other objects used for logistics transport purposes."
                }
            ]
        },
        {
            "@id": "transport:Referenced_LogisticsTransportEquipment",
            "@type": "rdfs:Class",
            "rdfs:comment": "A referenced piece of equipment used to hold, protect or secure cargo for logistics purposes.",
            "rdfs:label": "Referenced_LogisticsTransportEquipment",
            "unece:cefactElementMetadata": [
                {
                    "@id": "cefact:Referenced_Logistics_TransportEquipment.Details",
                    "@type": "unece:AggregateBIE",
                    "unece:cefactUNId": "UN01004022",
                    "rdfs:comment": "A referenced piece of equipment used to hold, protect or secure cargo for logistics purposes."
                }
            ]
        },
        {
            "@id": "transport:Referenced_SupplyChainConsignment",
            "@type": "rdfs:Class",
            "rdfs:comment": "A referenced, separately identifiable collection of goods items to be transported or available to be transported from one consignor to one consignee via one or more modes of transport where each consignment is the subject of one single transport contract.",
            "rdfs:label": "Referenced_SupplyChainConsignment",
            "unece:cefactElementMetadata": [
                {
                    "@id": "cefact:Referenced_SupplyChain_Consignment.Details",
                    "@type": "unece:AggregateBIE",
                    "unece:cefactUNId": "UN01004040",
                    "rdfs:comment": "A referenced, separately identifiable collection of goods items to be transported or available to be transported from one consignor to one consignee via one or more modes of transport where each consignment is the subject of one single transport contract."
                }
            ]
        },
        {
            "@id": "transport:Referenced_SupplyChainConsignmentItem",
            "@type": "rdfs:Class",
            "rdfs:comment": "A reference to an item within a supply chain consignment of goods separately identified for transport and customs purposes.",
            "rdfs:label": "Referenced_SupplyChainConsignmentItem",
            "unece:cefactElementMetadata": [
                {
                    "@id": "cefact:Referenced_SupplyChain_ConsignmentItem.Details",
                    "@type": "unece:AggregateBIE",
                    "unece:cefactUNId": "UN01004035",
                    "rdfs:comment": "A reference to an item within a supply chain consignment of goods separately identified for transport and customs purposes."
                }
            ]
        },
        {
            "@id": "transport:SupplyChainConsignment",
            "@type": "rdfs:Class",
            "rdfs:comment": "A separately identifiable collection of goods items to be transported or available to be transported from one consignor to one consignee in a supply chain via one or more modes of transport where each consignment is the subject of one single transport contract.",
            "rdfs:label": "SupplyChainConsignment",
            "unece:cefactElementMetadata": [
                {
                    "@id": "cefact:SupplyChain_Consignment.Details",
                    "@type": "unece:AggregateBIE",
                    "unece:cefactUNId": "UN01004159",
                    "rdfs:comment": "A separately identifiable collection of goods items to be transported or available to be transported from one consignor to one consignee in a supply chain via one or more modes of transport where each consignment is the subject of one single transport contract."
                }
            ]
        },
        {
            "@id": "transport:SupplyChainConsignmentItem",
            "@type": "rdfs:Class",
            "rdfs:comment": "An item within a supply chain consignment of goods separately identified for transport and customs purposes.",
            "rdfs:label": "SupplyChainConsignmentItem",
            "unece:cefactElementMetadata": [
                {
                    "@id": "cefact:SupplyChain_ConsignmentItem.Details",
                    "@type": "unece:AggregateBIE",
                    "unece:cefactUNId": "UN01004103",
                    "rdfs:comment": "An item within a supply chain consignment of goods separately identified for transport and customs purposes."
                }
            ]
        },
        {
            "@id": "transport:SupplyChainPackaging",
            "@type": "rdfs:Class",
            "rdfs:comment": "Any material with which supply chain goods are packaged, such as a box or bubble wrap.",
            "rdfs:label": "SupplyChainPackaging",
            "unece:cefactElementMetadata": [
                {
                    "@id": "cefact:SupplyChain_Packaging.Details",
                    "@type": "unece:AggregateBIE",
                    "unece:cefactUNId": "UN01004312",
                    "rdfs:comment": "Any material with which supply chain goods are packaged, such as a box or bubble wrap."
                }
            ]
        },
        {
            "@id": "transport:TradeProduct_SupplyChainPackaging",
            "@type": "rdfs:Class",
            "rdfs:comment": "Any material with which supply chain products are packaged for trade purposes, such as a box or bubble wrap.",
            "rdfs:label": "TradeProduct_SupplyChainPackaging",
            "unece:cefactElementMetadata": [
                {
                    "@id": "cefact:TradeProduct_SupplyChain_Packaging.Details",
                    "@type": "unece:AggregateBIE",
                    "unece:cefactUNId": "UN01007477",
                    "rdfs:comment": "Any material with which supply chain products are packaged for trade purposes, such as a box or bubble wrap."
                }
            ]
        },
        {
            "@id": "transport:TransportationWasteRecoveryDisposalProcess",
            "@type": "rdfs:Class",
            "rdfs:comment": "A process of either regaining substances in usable form, or of getting rid of substances resulting from transportation.",
            "rdfs:label": "TransportationWasteRecoveryDisposalProcess",
            "unece:cefactElementMetadata": [
                {
                    "@id": "cefact:TransportationWasteRecoveryDisposal_Process.Details",
                    "@type": "unece:AggregateBIE",
                    "unece:cefactUNId": "UN01014616",
                    "rdfs:comment": "A process of either regaining substances in usable form, or of getting rid of substances resulting from transportation."
                }
            ]
        },
        {
            "@id": "transport:accompaniedIndicator",
            "@type": "rdf:Property",
            "schema:rangeIncludes": {
                "@id": "xsd:boolean"
            },
            "schema:domainIncludes": {
                "@id": "transport:LogisticsTransportEquipment"
            },
            "rdfs:comment": "The indication of whether or not this piece of logistics transport equipment is accompanied, such as by a transport means.",
            "rdfs:label": "accompaniedIndicator",
            "unece:cefactElementMetadata": [
                {
                    "@id": "cefact:Logistics_TransportEquipment.Accompanied.Indicator",
                    "@type": "unece:BasicBIE",
                    "unece:cefactUNId": "UN01003783",
                    "unece:cefactBieDomainClass": "cefact:Logistics_TransportEquipment.Details",
                    "rdfs:comment": "The indication of whether or not this piece of logistics transport equipment is accompanied, such as by a transport means."
                }
            ]
        },
        {
            "@id": "transport:actualRoute",
            "@type": "rdf:Property",
            "schema:rangeIncludes": {
                "@id": "transport:Route"
            },
            "schema:domainIncludes": {
                "@id": "transport:LogisticsTransportEquipment"
            },
            "rdfs:comment": "An actual route for this piece of logistics transport equipment.",
            "rdfs:label": "actualRoute",
            "unece:cefactElementMetadata": [
                {
                    "@id": "cefact:Logistics_TransportEquipment.Actual.Transport_Route",
                    "@type": "unece:AssociationBIE",
                    "unece:cefactUNId": "UN01013597",
                    "unece:cefactBieDomainClass": "cefact:Logistics_TransportEquipment.Details",
                    "rdfs:comment": "An actual route for this piece of logistics transport equipment."
                }
            ]
        },
        {
            "@id": "transport:additionalInstructionCode",
            "@type": "rdf:Property",
            "schema:rangeIncludes": {
                "@id": "xsd:token"
            },
            "schema:domainIncludes": {
                "@id": "transport:SupplyChainPackaging"
            },
            "rdfs:comment": "A code specifying an additional instruction for this supply chain packaging.",
            "rdfs:label": "additionalInstructionCode",
            "unece:cefactElementMetadata": [
                {
                    "@id": "cefact:SupplyChain_Packaging.Additional_Instruction.Code",
                    "@type": "unece:BasicBIE",
                    "unece:cefactUNId": "UN01012708",
                    "unece:cefactBieDomainClass": "cefact:SupplyChain_Packaging.Details",
                    "rdfs:comment": "A code specifying an additional instruction for this supply chain packaging."
                }
            ]
        },
        {
            "@id": "transport:additionalInstructionIndicator",
            "@type": "rdf:Property",
            "schema:rangeIncludes": {
                "@id": "xsd:boolean"
            },
            "schema:domainIncludes": {
                "@id": "transport:SupplyChainPackaging"
            },
            "rdfs:comment": "The indication of whether or not there is an additional instruction for this supply chain packaging.",
            "rdfs:label": "additionalInstructionIndicator",
            "unece:cefactElementMetadata": [
                {
                    "@id": "cefact:SupplyChain_Packaging.Additional_Instruction.Indicator",
                    "@type": "unece:BasicBIE",
                    "unece:cefactUNId": "UN01012709",
                    "unece:cefactBieDomainClass": "cefact:SupplyChain_Packaging.Details",
                    "rdfs:comment": "The indication of whether or not there is an additional instruction for this supply chain packaging."
                }
            ]
        },
        {
            "@id": "transport:additionalInstructions",
            "@type": "rdf:Property",
            "schema:rangeIncludes": {
                "@id": "transport:Instructions"
            },
            "schema:domainIncludes": {
                "@id": "transport:LogisticsTransportEquipment"
            },
            "rdfs:comment": "Additional instructions for this piece of logistics transport equipment.",
            "rdfs:label": "additionalInstructions",
            "unece:cefactElementMetadata": [
                {
                    "@id": "cefact:Logistics_TransportEquipment.Additional.Transport_Instructions",
                    "@type": "unece:AssociationBIE",
                    "unece:cefactUNId": "UN01003793",
                    "unece:cefactBieDomainClass": "cefact:Logistics_TransportEquipment.Details",
                    "rdfs:comment": "Additional instructions for this piece of logistics transport equipment."
                }
            ]
        },
        {
            "@id": "transport:administrativeMedicalPersonnelOnboardQuantity",
            "@type": "rdf:Property",
            "schema:rangeIncludes": {
                "@id": "xsd:decimal"
            },
            "schema:domainIncludes": {
                "@id": "transport:LogisticsTransportMovement"
            },
            "rdfs:comment": "The number of administrative medical personnel onboard this logistics transport movement.",
            "rdfs:label": "administrativeMedicalPersonnelOnboardQuantity",
            "unece:cefactElementMetadata": [
                {
                    "@id": "cefact:Logistics_TransportMovement.Administrative_MedicalPersonnelOnboard.Quantity",
                    "@type": "unece:BasicBIE",
                    "unece:cefactUNId": "UN01015087",
                    "unece:cefactBieDomainClass": "cefact:Logistics_TransportMovement.Details",
                    "rdfs:comment": "The number of administrative medical personnel onboard this logistics transport movement."
                }
            ]
        },
        {
            "@id": "transport:affectedDistanceMeasure",
            "@type": "rdf:Property",
            "schema:rangeIncludes": {
                "@id": "xsd:decimal"
            },
            "schema:domainIncludes": {
                "@id": "transport:CalculatedEmission"
            },
            "rdfs:comment": "The affected distance over which this calculated emission is measured.",
            "rdfs:label": "affectedDistanceMeasure",
            "unece:cefactElementMetadata": [
                {
                    "@id": "cefact:Calculated_Emission.Affected_Distance.Measure",
                    "@type": "unece:BasicBIE",
                    "unece:TDED": "6411",
                    "unece:cefactUNId": "UN01010053",
                    "unece:cefactBieDomainClass": "cefact:Calculated_Emission.Details",
                    "rdfs:comment": "The affected distance over which this calculated emission is measured."
                }
            ]
        },
        {
            "@id": "transport:affixedSeal",
            "@type": "rdf:Property",
            "schema:rangeIncludes": {
                "@id": "transport:Seal"
            },
            "schema:domainIncludes": [
                {
                    "@id": "transport:AssociatedTransportEquipment"
                },
                {
                    "@id": "transport:LogisticsTransportEquipment"
                },
                {
                    "@id": "transport:Referenced_LogisticsTransportEquipment"
                }
            ],
            "rdfs:comment": [
                "A logistics seal affixed to this piece of associated transport equipment.",
                "A seal affixed to this piece of logistics transport equipment.",
                "A seal affixed to this piece of referenced logistics transport equipment."
            ],
            "rdfs:label": "affixedSeal",
            "unece:cefactElementMetadata": [
                {
                    "@id": "cefact:Associated_TransportEquipment.Affixed.Logistics_Seal",
                    "@type": "unece:AssociationBIE",
                    "unece:cefactUNId": "UN01013662",
                    "unece:cefactBieDomainClass": "cefact:Associated_TransportEquipment.Details",
                    "rdfs:comment": "A logistics seal affixed to this piece of associated transport equipment."
                },
                {
                    "@id": "cefact:Referenced_Logistics_TransportEquipment.Affixed.Logistics_Seal",
                    "@type": "unece:AssociationBIE",
                    "unece:cefactUNId": "UN01013180",
                    "unece:cefactBieDomainClass": "cefact:Referenced_Logistics_TransportEquipment.Details",
                    "rdfs:comment": "A seal affixed to this piece of referenced logistics transport equipment."
                },
                {
                    "@id": "cefact:Logistics_TransportEquipment.Affixed.Logistics_Seal",
                    "@type": "unece:AssociationBIE",
                    "unece:cefactUNId": "UN01003795",
                    "unece:cefactBieDomainClass": "cefact:Logistics_TransportEquipment.Details",
                    "rdfs:comment": "A seal affixed to this piece of logistics transport equipment."
                }
            ]
        },
        {
            "@id": "transport:aftDraughtLevelMeasure",
            "@type": "rdf:Property",
            "schema:rangeIncludes": {
                "@id": "xsd:decimal"
            },
            "schema:domainIncludes": {
                "@id": "transport:LogisticsTransportMeans"
            },
            "rdfs:comment": "The draught level measured at the aft end of this transport means.",
            "rdfs:label": "aftDraughtLevelMeasure",
            "unece:cefactElementMetadata": [
                {
                    "@id": "cefact:Logistics_TransportMeans.Aft_DraughtLevel.Measure",
                    "@type": "unece:BasicBIE",
                    "unece:cefactUNId": "UN01010106",
                    "unece:cefactBieDomainClass": "cefact:Logistics_TransportMeans.Details",
                    "rdfs:comment": "The draught level measured at the aft end of this transport means."
                }
            ]
        },
        {
            "@id": "transport:airDraughtLevelMeasure",
            "@type": "rdf:Property",
            "schema:rangeIncludes": {
                "@id": "xsd:decimal"
            },
            "schema:domainIncludes": {
                "@id": "transport:LogisticsTransportMeans"
            },
            "rdfs:comment": "An air draught level measure for this logistics transport means.",
            "rdfs:label": "airDraughtLevelMeasure",
            "unece:cefactElementMetadata": [
                {
                    "@id": "cefact:Logistics_TransportMeans.Air_DraughtLevel.Measure",
                    "@type": "unece:BasicBIE",
                    "unece:cefactUNId": "UN01015083",
                    "unece:cefactBieDomainClass": "cefact:Logistics_TransportMeans.Details",
                    "rdfs:comment": "An air draught level measure for this logistics transport means."
                }
            ]
        },
        {
            "@id": "transport:airFlowMeasure",
            "@type": "rdf:Property",
            "schema:rangeIncludes": {
                "@id": "xsd:decimal"
            },
            "schema:domainIncludes": {
                "@id": "transport:LogisticsTransportEquipment"
            },
            "rdfs:comment": "The measure of the air flow for this piece of logistics transport equipment.",
            "rdfs:label": "airFlowMeasure",
            "unece:cefactElementMetadata": [
                {
                    "@id": "cefact:Logistics_TransportEquipment.AirFlow.Measure",
                    "@type": "unece:BasicBIE",
                    "unece:TDED": "6411",
                    "unece:cefactUNId": "UN01008982",
                    "unece:cefactBieDomainClass": "cefact:Logistics_TransportEquipment.Details",
                    "rdfs:comment": "The measure of the air flow for this piece of logistics transport equipment."
                }
            ]
        },
        {
            "@id": "transport:applicableAllowanceCharge",
            "@type": "rdf:Property",
            "schema:rangeIncludes": {
                "@id": "transport:AllowanceCharge"
            },
            "schema:domainIncludes": {
                "@id": "transport:SupplyChainConsignment"
            },
            "rdfs:comment": "An allowance or charge applicable to this supply chain consignment.",
            "rdfs:label": "applicableAllowanceCharge",
            "unece:cefactElementMetadata": [
                {
                    "@id": "cefact:SupplyChain_Consignment.Applicable.Trade_AllowanceCharge",
                    "@type": "unece:AssociationBIE",
                    "unece:cefactUNId": "UN01004287",
                    "unece:cefactBieDomainClass": "cefact:SupplyChain_Consignment.Details",
                    "rdfs:comment": "An allowance or charge applicable to this supply chain consignment."
                }
            ]
        },
        {
            "@id": "transport:applicableCargoInsurance",
            "@type": "rdf:Property",
            "schema:rangeIncludes": {
                "@id": "transport:CargoInsurance"
            },
            "schema:domainIncludes": {
                "@id": "transport:SupplyChainConsignment"
            },
            "rdfs:comment": "The cargo insurance applicable to this supply chain consignment.",
            "rdfs:label": "applicableCargoInsurance",
            "unece:cefactElementMetadata": [
                {
                    "@id": "cefact:SupplyChain_Consignment.Applicable.Transport_CargoInsurance",
                    "@type": "unece:AssociationBIE",
                    "unece:cefactUNId": "UN01004277",
                    "unece:cefactBieDomainClass": "cefact:SupplyChain_Consignment.Details",
                    "rdfs:comment": "The cargo insurance applicable to this supply chain consignment."
                }
            ]
        },
        {
            "@id": "transport:applicableCharacteristic",
            "@type": "rdf:Property",
            "schema:rangeIncludes": {
                "@id": "transport:Characteristic"
            },
            "schema:domainIncludes": [
                {
                    "@id": "transport:LogisticsTransportMeans"
                },
                {
                    "@id": "transport:LogisticsTransportMovement"
                }
            ],
            "rdfs:comment": [
                "A sustainability characteristic applicable to this logistics transport means.",
                "A sustainability characteristic applicable to this logistics transport movement."
            ],
            "rdfs:label": "applicableCharacteristic",
            "unece:cefactElementMetadata": [
                {
                    "@id": "cefact:Logistics_TransportMeans.Applicable.Sustainability_Characteristic",
                    "@type": "unece:AssociationBIE",
                    "unece:cefactUNId": "UN01013832",
                    "unece:cefactBieDomainClass": "cefact:Logistics_TransportMeans.Details",
                    "rdfs:comment": "A sustainability characteristic applicable to this logistics transport means."
                },
                {
                    "@id": "cefact:Logistics_TransportMovement.Applicable.Sustainability_Characteristic",
                    "@type": "unece:AssociationBIE",
                    "unece:cefactUNId": "UN01013838",
                    "unece:cefactBieDomainClass": "cefact:Logistics_TransportMovement.Details",
                    "rdfs:comment": "A sustainability characteristic applicable to this logistics transport movement."
                }
            ]
        },
        {
            "@id": "transport:applicableCurrencyExchange",
            "@type": "rdf:Property",
            "schema:rangeIncludes": {
                "@id": "transport:CurrencyExchange"
            },
            "schema:domainIncludes": {
                "@id": "transport:SupplyChainConsignment"
            },
            "rdfs:comment": "A currency exchange applicable to this supply chain consignment.",
            "rdfs:label": "applicableCurrencyExchange",
            "unece:cefactElementMetadata": [
                {
                    "@id": "cefact:SupplyChain_Consignment.Applicable.Trade_CurrencyExchange",
                    "@type": "unece:AssociationBIE",
                    "unece:cefactUNId": "UN01004279",
                    "unece:cefactBieDomainClass": "cefact:SupplyChain_Consignment.Details",
                    "rdfs:comment": "A currency exchange applicable to this supply chain consignment."
                }
            ]
        },
        {
            "@id": "transport:applicableCustomsProcedure",
            "@type": "rdf:Property",
            "schema:rangeIncludes": {
                "@id": "transport:CustomsProcedure"
            },
            "schema:domainIncludes": {
                "@id": "transport:SupplyChainConsignmentItem"
            },
            "rdfs:comment": "A customs procedure applicable to this supply chain consignment item.",
            "rdfs:label": "applicableCustomsProcedure",
            "unece:cefactElementMetadata": [
                {
                    "@id": "cefact:SupplyChain_ConsignmentItem.Applicable.Cross-Border_CustomsProcedure",
                    "@type": "unece:AssociationBIE",
                    "unece:cefactUNId": "UN01004151",
                    "unece:cefactBieDomainClass": "cefact:SupplyChain_ConsignmentItem.Details",
                    "rdfs:comment": "A customs procedure applicable to this supply chain consignment item."
                }
            ]
        },
        {
            "@id": "transport:applicableCustomsValuation",
            "@type": "rdf:Property",
            "schema:rangeIncludes": {
                "@id": "transport:CustomsValuation"
            },
            "schema:domainIncludes": {
                "@id": "transport:SupplyChainConsignmentItem"
            },
            "rdfs:comment": "A customs valuation applicable to this supply chain consignment item.",
            "rdfs:label": "applicableCustomsValuation",
            "unece:cefactElementMetadata": [
                {
                    "@id": "cefact:SupplyChain_ConsignmentItem.Applicable.Cross-Border_CustomsValuation",
                    "@type": "unece:AssociationBIE",
                    "unece:cefactUNId": "UN01008998",
                    "unece:cefactBieDomainClass": "cefact:SupplyChain_ConsignmentItem.Details",
                    "rdfs:comment": "A customs valuation applicable to this supply chain consignment item."
                }
            ]
        },
        {
            "@id": "transport:applicableDangerousGoods",
            "@type": "rdf:Property",
            "schema:rangeIncludes": {
                "@id": "transport:DangerousGoods"
            },
            "schema:domainIncludes": {
                "@id": "transport:SupplyChainConsignmentItem"
            },
            "rdfs:comment": "Dangerous goods transport details applicable to this supply chain consignment item.",
            "rdfs:label": "applicableDangerousGoods",
            "unece:cefactElementMetadata": [
                {
                    "@id": "cefact:SupplyChain_ConsignmentItem.Applicable.Transport_DangerousGoods",
                    "@type": "unece:AssociationBIE",
                    "unece:cefactUNId": "UN01004131",
                    "unece:cefactBieDomainClass": "cefact:SupplyChain_ConsignmentItem.Details",
                    "rdfs:comment": "Dangerous goods transport details applicable to this supply chain consignment item."
                }
            ]
        },
        {
            "@id": "transport:applicableInspection",
            "@type": "rdf:Property",
            "schema:rangeIncludes": {
                "@id": "transport:Inspection"
            },
            "schema:domainIncludes": {
                "@id": "transport:LogisticsTransportMovement"
            },
            "rdfs:comment": [
                "A specified inspection applicable to this logistics transport movement.",
                "A sustainability inspection applicable to this logistics transport movement."
            ],
            "rdfs:label": "applicableInspection",
            "unece:cefactElementMetadata": [
                {
                    "@id": "cefact:Logistics_TransportMovement.Applicable.Specified_Inspection",
                    "@type": "unece:AssociationBIE",
                    "unece:cefactUNId": "UN01013837",
                    "unece:cefactBieDomainClass": "cefact:Logistics_TransportMovement.Details",
                    "rdfs:comment": "A specified inspection applicable to this logistics transport movement."
                },
                {
                    "@id": "cefact:Logistics_TransportMovement.Applicable.Sustainability_Inspection",
                    "@type": "unece:AssociationBIE",
                    "unece:cefactUNId": "UN01013836",
                    "unece:cefactBieDomainClass": "cefact:Logistics_TransportMovement.Details",
                    "rdfs:comment": "A sustainability inspection applicable to this logistics transport movement."
                }
            ]
        },
        {
            "@id": "transport:applicableInstructions",
            "@type": "rdf:Property",
            "schema:rangeIncludes": {
                "@id": "transport:Instructions"
            },
            "schema:domainIncludes": [
                {
                    "@id": "transport:LogisticsPackaging"
                },
                {
                    "@id": "transport:SupplyChainPackaging"
                }
            ],
            "rdfs:comment": [
                "Instructions applicable to this logistics packaging.",
                "Packaging instructions applicable to this supply chain packaging."
            ],
            "rdfs:label": "applicableInstructions",
            "unece:cefactElementMetadata": [
                {
                    "@id": "cefact:Logistics_Packaging.Applicable.Packaging_Instructions",
                    "@type": "unece:AssociationBIE",
                    "unece:cefactUNId": "UN01014968",
                    "unece:cefactBieDomainClass": "cefact:Logistics_Packaging.Details",
                    "rdfs:comment": "Instructions applicable to this logistics packaging."
                },
                {
                    "@id": "cefact:SupplyChain_Packaging.Applicable.Packaging_Instructions",
                    "@type": "unece:AssociationBIE",
                    "unece:cefactUNId": "UN01014460",
                    "unece:cefactBieDomainClass": "cefact:SupplyChain_Packaging.Details",
                    "rdfs:comment": "Packaging instructions applicable to this supply chain packaging."
                }
            ]
        },
        {
            "@id": "transport:applicableNote",
            "@type": "rdf:Property",
            "schema:rangeIncludes": {
                "@id": "transport:Note"
            },
            "schema:domainIncludes": [
                {
                    "@id": "transport:LogisticsTransportEquipment"
                },
                {
                    "@id": "transport:SupplyChainConsignmentItem"
                }
            ],
            "rdfs:comment": [
                "A note providing information applicable to this piece of logistics transport equipment.",
                "A note providing information applicable to this supply chain consignment item."
            ],
            "rdfs:label": "applicableNote",
            "unece:cefactElementMetadata": [
                {
                    "@id": "cefact:Logistics_TransportEquipment.Applicable.Note",
                    "@type": "unece:AssociationBIE",
                    "unece:cefactUNId": "UN01012568",
                    "unece:cefactBieDomainClass": "cefact:Logistics_TransportEquipment.Details",
                    "rdfs:comment": "A note providing information applicable to this piece of logistics transport equipment."
                },
                {
                    "@id": "cefact:SupplyChain_ConsignmentItem.Applicable.Note",
                    "@type": "unece:AssociationBIE",
                    "unece:cefactUNId": "UN01012577",
                    "unece:cefactBieDomainClass": "cefact:SupplyChain_ConsignmentItem.Details",
                    "rdfs:comment": "A note providing information applicable to this supply chain consignment item."
                }
            ]
        },
        {
            "@id": "transport:applicableRegulatoryProcedure",
            "@type": "rdf:Property",
            "schema:rangeIncludes": {
                "@id": "transport:RegulatoryProcedure"
            },
            "schema:domainIncludes": [
                {
                    "@id": "transport:LogisticsTransportMovement"
                },
                {
                    "@id": "transport:Referenced_SupplyChainConsignment"
                },
                {
                    "@id": "transport:SupplyChainConsignment"
                },
                {
                    "@id": "transport:SupplyChainConsignmentItem"
                }
            ],
            "rdfs:comment": [
                "A cross-border regulatory procedure applicable to this logistics transport movement.",
                "A cross-border regulatory procedure applicable to this referenced supply chain consignment.",
                "A cross-border regulatory procedure applicable to this supply chain consignment item.",
                "A cross-border regulatory procedure applicable to this supply chain consignment."
            ],
            "rdfs:label": "applicableRegulatoryProcedure",
            "unece:cefactElementMetadata": [
                {
                    "@id": "cefact:SupplyChain_Consignment.Applicable.Cross-Border_RegulatoryProcedure",
                    "@type": "unece:AssociationBIE",
                    "unece:cefactUNId": "UN01006189",
                    "unece:cefactBieDomainClass": "cefact:SupplyChain_Consignment.Details",
                    "rdfs:comment": "A cross-border regulatory procedure applicable to this supply chain consignment."
                },
                {
                    "@id": "cefact:Logistics_TransportMovement.Applicable.Cross-Border_RegulatoryProcedure",
                    "@type": "unece:AssociationBIE",
                    "unece:cefactUNId": "UN01006187",
                    "unece:cefactBieDomainClass": "cefact:Logistics_TransportMovement.Details",
                    "rdfs:comment": "A cross-border regulatory procedure applicable to this logistics transport movement."
                },
                {
                    "@id": "cefact:Referenced_SupplyChain_Consignment.Applicable.Cross-Border_RegulatoryProcedure",
                    "@type": "unece:AssociationBIE",
                    "unece:cefactUNId": "UN01011064",
                    "unece:cefactBieDomainClass": "cefact:Referenced_SupplyChain_Consignment.Details",
                    "rdfs:comment": "A cross-border regulatory procedure applicable to this referenced supply chain consignment."
                },
                {
                    "@id": "cefact:SupplyChain_ConsignmentItem.Applicable.Cross-Border_RegulatoryProcedure",
                    "@type": "unece:AssociationBIE",
                    "unece:cefactUNId": "UN01006188",
                    "unece:cefactBieDomainClass": "cefact:SupplyChain_ConsignmentItem.Details",
                    "rdfs:comment": "A cross-border regulatory procedure applicable to this supply chain consignment item."
                }
            ]
        },
        {
            "@id": "transport:applicableServiceCharge",
            "@type": "rdf:Property",
            "schema:rangeIncludes": {
                "@id": "transport:ServiceCharge"
            },
            "schema:domainIncludes": [
                {
                    "@id": "transport:LogisticsTransportEquipment"
                },
                {
                    "@id": "transport:LogisticsTransportMeans"
                },
                {
                    "@id": "transport:LogisticsTransportMovement"
                },
                {
                    "@id": "transport:SupplyChainConsignment"
                },
                {
                    "@id": "transport:SupplyChainConsignmentItem"
                }
            ],
            "rdfs:comment": [
                "A logistics service charge applicable to this supply chain consignment item.",
                "A logistics service charge applicable to this supply chain consignment, such as freight or insurance charges.",
                "A service charge applicable to this piece of logistics transport equipment.",
                "A service charge, such as a freight charge, applicable to this logistics means of transport.",
                "A service charge, such as a freight charge, applicable to this logistics transport movement."
            ],
            "rdfs:label": "applicableServiceCharge",
            "unece:cefactElementMetadata": [
                {
                    "@id": "cefact:Logistics_TransportMovement.Applicable.Logistics_ServiceCharge",
                    "@type": "unece:AssociationBIE",
                    "unece:cefactUNId": "UN01003862",
                    "unece:cefactBieDomainClass": "cefact:Logistics_TransportMovement.Details",
                    "rdfs:comment": "A service charge, such as a freight charge, applicable to this logistics transport movement."
                },
                {
                    "@id": "cefact:SupplyChain_ConsignmentItem.Applicable.Logistics_ServiceCharge",
                    "@type": "unece:AssociationBIE",
                    "unece:cefactUNId": "UN01004154",
                    "unece:cefactBieDomainClass": "cefact:SupplyChain_ConsignmentItem.Details",
                    "rdfs:comment": "A logistics service charge applicable to this supply chain consignment item."
                },
                {
                    "@id": "cefact:Logistics_TransportEquipment.Applicable.Logistics_ServiceCharge",
                    "@type": "unece:AssociationBIE",
                    "unece:cefactUNId": "UN01003801",
                    "unece:cefactBieDomainClass": "cefact:Logistics_TransportEquipment.Details",
                    "rdfs:comment": "A service charge applicable to this piece of logistics transport equipment."
                },
                {
                    "@id": "cefact:Logistics_TransportMeans.Applicable.Logistics_ServiceCharge",
                    "@type": "unece:AssociationBIE",
                    "unece:cefactUNId": "UN01003832",
                    "unece:cefactBieDomainClass": "cefact:Logistics_TransportMeans.Details",
                    "rdfs:comment": "A service charge, such as a freight charge, applicable to this logistics means of transport."
                },
                {
                    "@id": "cefact:SupplyChain_Consignment.Applicable.Logistics_ServiceCharge",
                    "@type": "unece:AssociationBIE",
                    "unece:cefactUNId": "UN01004285",
                    "unece:cefactBieDomainClass": "cefact:SupplyChain_Consignment.Details",
                    "rdfs:comment": "A logistics service charge applicable to this supply chain consignment, such as freight or insurance charges."
                }
            ]
        },
        {
            "@id": "transport:applicableTransportMeans",
            "@type": "rdf:Property",
            "schema:rangeIncludes": {
                "@id": "transport:TransportMeans"
            },
            "schema:domainIncludes": {
                "@id": "transport:SupplyChainConsignmentItem"
            },
            "rdfs:comment": "The means of transport applicable to this supply chain consignment item.",
            "rdfs:label": "applicableTransportMeans",
            "unece:cefactElementMetadata": [
                {
                    "@id": "cefact:SupplyChain_ConsignmentItem.Applicable.Logistics_TransportMeans",
                    "@type": "unece:AssociationBIE",
                    "unece:cefactUNId": "UN01004150",
                    "unece:cefactBieDomainClass": "cefact:SupplyChain_ConsignmentItem.Details",
                    "rdfs:comment": "The means of transport applicable to this supply chain consignment item."
                }
            ]
        },
        {
            "@id": "transport:approvedSecurityPlanOnboardIndicator",
            "@type": "rdf:Property",
            "schema:rangeIncludes": {
                "@id": "xsd:boolean"
            },
            "schema:domainIncludes": {
                "@id": "transport:LogisticsTransportMeans"
            },
            "rdfs:comment": "The indication of whether or not there is an approved security plan onboard this logistics transport means.",
            "rdfs:label": "approvedSecurityPlanOnboardIndicator",
            "unece:cefactElementMetadata": [
                {
                    "@id": "cefact:Logistics_TransportMeans.ApprovedSecurityPlanOnboard.Indicator",
                    "@type": "unece:BasicBIE",
                    "unece:cefactUNId": "UN01013169",
                    "unece:cefactBieDomainClass": "cefact:Logistics_TransportMeans.Details",
                    "rdfs:comment": "The indication of whether or not there is an approved security plan onboard this logistics transport means."
                }
            ]
        },
        {
            "@id": "transport:arrivalEvent",
            "@type": "rdf:Property",
            "schema:rangeIncludes": {
                "@id": "transport:Event"
            },
            "schema:domainIncludes": {
                "@id": "transport:LogisticsTransportMovement"
            },
            "rdfs:comment": "An arrival event for this logistics transport movement.",
            "rdfs:label": "arrivalEvent",
            "unece:cefactElementMetadata": [
                {
                    "@id": "cefact:Logistics_TransportMovement.Arrival.Transport_Event",
                    "@type": "unece:AssociationBIE",
                    "unece:cefactUNId": "UN01003858",
                    "unece:cefactBieDomainClass": "cefact:Logistics_TransportMovement.Details",
                    "rdfs:comment": "An arrival event for this logistics transport movement."
                }
            ]
        },
        {
            "@id": "transport:arrivalReportedEvent",
            "@type": "rdf:Property",
            "schema:rangeIncludes": {
                "@id": "transport:Event"
            },
            "schema:domainIncludes": {
                "@id": "trade:LogisticsStatus"
            },
            "rdfs:comment": "A transport arrival event reported for this logistics status.",
            "rdfs:label": "arrivalReportedEvent",
            "unece:cefactElementMetadata": [
                {
                    "@id": "cefact:Logistics_Status.Arrival_Reported.Transport_Event",
                    "@type": "unece:AssociationBIE",
                    "unece:cefactUNId": "UN01010093",
                    "unece:cefactBieDomainClass": "cefact:Logistics_Status.Details",
                    "rdfs:comment": "A transport arrival event reported for this logistics status."
                }
            ]
        },
        {
            "@id": "transport:associatedConvoy",
            "@type": "rdf:Property",
            "schema:rangeIncludes": {
                "@id": "transport:Convoy"
            },
            "schema:domainIncludes": {
                "@id": "transport:LogisticsTransportMovement"
            },
            "rdfs:comment": "The convoy associated with this logistics transport movement.",
            "rdfs:label": "associatedConvoy",
            "unece:cefactElementMetadata": [
                {
                    "@id": "cefact:Logistics_TransportMovement.Associated.Logistics_Convoy",
                    "@type": "unece:AssociationBIE",
                    "unece:cefactUNId": "UN01010124",
                    "unece:cefactBieDomainClass": "cefact:Logistics_TransportMovement.Details",
                    "rdfs:comment": "The convoy associated with this logistics transport movement."
                }
            ]
        },
        {
            "@id": "transport:associatedCustomsProcedure",
            "@type": "rdf:Property",
            "schema:rangeIncludes": {
                "@id": "transport:CustomsProcedure"
            },
            "schema:domainIncludes": {
                "@id": "transport:SupplyChainConsignment"
            },
            "rdfs:comment": "A customs procedure associated with this supply chain consignment.",
            "rdfs:label": "associatedCustomsProcedure",
            "unece:cefactElementMetadata": [
                {
                    "@id": "cefact:SupplyChain_Consignment.Associated.Cross-Border_CustomsProcedure",
                    "@type": "unece:AssociationBIE",
                    "unece:cefactUNId": "UN01004278",
                    "unece:cefactBieDomainClass": "cefact:SupplyChain_Consignment.Details",
                    "rdfs:comment": "A customs procedure associated with this supply chain consignment."
                }
            ]
        },
        {
            "@id": "transport:associatedDocument",
            "@type": "rdf:Property",
            "schema:rangeIncludes": {
                "@id": "transport:Document"
            },
            "schema:domainIncludes": [
                {
                    "@id": "transport:LogisticsTransportEquipment"
                },
                {
                    "@id": "transport:Referenced_SupplyChainConsignmentItem"
                },
                {
                    "@id": "transport:SupplyChainConsignment"
                },
                {
                    "@id": "transport:SupplyChainConsignmentItem"
                }
            ],
            "rdfs:comment": [
                "A referenced document associated with this piece of logistics transport equipment.",
                "A referenced document associated with this referenced supply chain consignment item.",
                "A referenced document associated with this supply chain consignment item.",
                "A referenced document associated with this supply chain consignment, such as the certificate of origin or dangerous goods note."
            ],
            "rdfs:label": "associatedDocument",
            "unece:cefactElementMetadata": [
                {
                    "@id": "cefact:Referenced_SupplyChain_ConsignmentItem.Associated.Referenced_Document",
                    "@type": "unece:AssociationBIE",
                    "unece:cefactUNId": "UN01004039",
                    "unece:cefactBieDomainClass": "cefact:Referenced_SupplyChain_ConsignmentItem.Details",
                    "rdfs:comment": "A referenced document associated with this referenced supply chain consignment item."
                },
                {
                    "@id": "cefact:Logistics_TransportEquipment.Associated.Referenced_Document",
                    "@type": "unece:AssociationBIE",
                    "unece:cefactUNId": "UN01011040",
                    "unece:cefactBieDomainClass": "cefact:Logistics_TransportEquipment.Details",
                    "rdfs:comment": "A referenced document associated with this piece of logistics transport equipment."
                },
                {
                    "@id": "cefact:SupplyChain_ConsignmentItem.Associated.Referenced_Document",
                    "@type": "unece:AssociationBIE",
                    "unece:cefactUNId": "UN01004149",
                    "unece:cefactBieDomainClass": "cefact:SupplyChain_ConsignmentItem.Details",
                    "rdfs:comment": "A referenced document associated with this supply chain consignment item."
                },
                {
                    "@id": "cefact:SupplyChain_Consignment.Associated.Referenced_Document",
                    "@type": "unece:AssociationBIE",
                    "unece:cefactUNId": "UN01004245",
                    "unece:cefactBieDomainClass": "cefact:SupplyChain_Consignment.Details",
                    "rdfs:comment": "A referenced document associated with this supply chain consignment, such as the certificate of origin or dangerous goods note."
                }
            ]
        },
        {
            "@id": "transport:associatedInvoiceAmount",
            "@type": "rdf:Property",
            "schema:rangeIncludes": {
                "@id": "xsd:decimal"
            },
            "schema:domainIncludes": {
                "@id": "transport:SupplyChainConsignment"
            },
            "rdfs:comment": "A monetary value of an invoice associated with this supply chain consignment.",
            "rdfs:label": "associatedInvoiceAmount",
            "unece:cefactElementMetadata": [
                {
                    "@id": "cefact:SupplyChain_Consignment.AssociatedInvoice.Amount",
                    "@type": "unece:BasicBIE",
                    "unece:TDED": "5444",
                    "unece:cefactUNId": "UN01004181",
                    "unece:cefactBieDomainClass": "cefact:SupplyChain_Consignment.Details",
                    "rdfs:comment": "A monetary value of an invoice associated with this supply chain consignment."
                }
            ]
        },
        {
            "@id": "transport:associatedInvoiceDiscountAmount",
            "@type": "rdf:Property",
            "schema:rangeIncludes": {
                "@id": "xsd:decimal"
            },
            "schema:domainIncludes": {
                "@id": "transport:SupplyChainConsignment"
            },
            "rdfs:comment": "A monetary value of the discount on an invoice associated with this supply chain consignment.",
            "rdfs:label": "associatedInvoiceDiscountAmount",
            "unece:cefactElementMetadata": [
                {
                    "@id": "cefact:SupplyChain_Consignment.AssociatedInvoiceDiscount.Amount",
                    "@type": "unece:BasicBIE",
                    "unece:TDED": "5180",
                    "unece:cefactUNId": "UN01004190",
                    "unece:cefactBieDomainClass": "cefact:SupplyChain_Consignment.Details",
                    "rdfs:comment": "A monetary value of the discount on an invoice associated with this supply chain consignment."
                }
            ]
        },
        {
            "@id": "transport:associatedInvoiceDiscountPercent",
            "@type": "rdf:Property",
            "schema:rangeIncludes": {
                "@id": "xsd:decimal"
            },
            "schema:domainIncludes": {
                "@id": "transport:SupplyChainConsignment"
            },
            "rdfs:comment": "A percent that is a discount on an invoice amount associated with this supply chain consignment.",
            "rdfs:label": "associatedInvoiceDiscountPercent",
            "unece:cefactElementMetadata": [
                {
                    "@id": "cefact:SupplyChain_Consignment.AssociatedInvoiceDiscount.Percent",
                    "@type": "unece:BasicBIE",
                    "unece:cefactUNId": "UN01004191",
                    "unece:cefactBieDomainClass": "cefact:SupplyChain_Consignment.Details",
                    "rdfs:comment": "A percent that is a discount on an invoice amount associated with this supply chain consignment."
                }
            ]
        },
        {
            "@id": "transport:associatedTransportEquipment",
            "@type": "rdf:Property",
            "schema:rangeIncludes": {
                "@id": "transport:TransportEquipment"
            },
            "schema:domainIncludes": [
                {
                    "@id": "transport:Referenced_SupplyChainConsignmentItem"
                },
                {
                    "@id": "transport:SupplyChainConsignmentItem"
                }
            ],
            "rdfs:comment": [
                "A piece of transport equipment associated with this referenced supply chain consignment item.",
                "A referenced piece of transport equipment associated with this supply chain consignment item."
            ],
            "rdfs:label": "associatedTransportEquipment",
            "unece:cefactElementMetadata": [
                {
                    "@id": "cefact:Referenced_SupplyChain_ConsignmentItem.Associated.Referenced_Logistics_TransportEquipment",
                    "@type": "unece:AssociationBIE",
                    "unece:cefactUNId": "UN01011047",
                    "unece:cefactBieDomainClass": "cefact:Referenced_SupplyChain_ConsignmentItem.Details",
                    "rdfs:comment": "A piece of transport equipment associated with this referenced supply chain consignment item."
                },
                {
                    "@id": "cefact:SupplyChain_ConsignmentItem.Associated.Referenced_Logistics_TransportEquipment",
                    "@type": "unece:AssociationBIE",
                    "unece:cefactUNId": "UN01004145",
                    "unece:cefactBieDomainClass": "cefact:SupplyChain_ConsignmentItem.Details",
                    "rdfs:comment": "A referenced piece of transport equipment associated with this supply chain consignment item."
                }
            ]
        },
        {
            "@id": "transport:associatedTransportEquipmentUsedCapacityCode",
            "@type": "rdf:Property",
            "schema:rangeIncludes": {
                "@id": "unece:UNECECL8169Code"
            },
            "schema:domainIncludes": {
                "@id": "transport:AssociatedTransportEquipment"
            },
            "rdfs:comment": "The code specifying the used capacity, such as full or empty, of this associated piece of transport equipment.",
            "rdfs:label": "associatedTransportEquipmentUsedCapacityCode",
            "unece:cefactElementMetadata": [
                {
                    "@id": "cefact:Associated_TransportEquipment.UsedCapacity.Code",
                    "@type": "unece:BasicBIE",
                    "unece:TDED": "8169",
                    "unece:cefactUNId": "UN01014628",
                    "unece:cefactBieDomainClass": "cefact:Associated_TransportEquipment.Details",
                    "rdfs:comment": "The code specifying the used capacity, such as full or empty, of this associated piece of transport equipment."
                }
            ]
        },
        {
            "@id": "transport:atArrivalTransportMovement",
            "@type": "rdf:Property",
            "schema:rangeIncludes": {
                "@id": "transport:TransportMovement"
            },
            "schema:domainIncludes": {
                "@id": "transport:SupplyChainConsignment"
            },
            "rdfs:comment": "The logistics transport movement for this supply chain consignment at the point when the means of transport arrives in a country or at a regional border.",
            "rdfs:label": "atArrivalTransportMovement",
            "unece:cefactElementMetadata": [
                {
                    "@id": "cefact:SupplyChain_Consignment.AtArrival.Logistics_TransportMovement",
                    "@type": "unece:AssociationBIE",
                    "unece:cefactUNId": "UN01004265",
                    "unece:cefactBieDomainClass": "cefact:SupplyChain_Consignment.Details",
                    "rdfs:comment": "The logistics transport movement for this supply chain consignment at the point when the means of transport arrives in a country or at a regional border."
                }
            ]
        },
        {
            "@id": "transport:atDepartureTransportMovement",
            "@type": "rdf:Property",
            "schema:rangeIncludes": {
                "@id": "transport:TransportMovement"
            },
            "schema:domainIncludes": {
                "@id": "transport:SupplyChainConsignment"
            },
            "rdfs:comment": "The logistics transport movement for this supply chain consignment at the point when the means of transport departs a country or regional border.",
            "rdfs:label": "atDepartureTransportMovement",
            "unece:cefactElementMetadata": [
                {
                    "@id": "cefact:SupplyChain_Consignment.AtDeparture.Logistics_TransportMovement",
                    "@type": "unece:AssociationBIE",
                    "unece:cefactUNId": "UN01004266",
                    "unece:cefactBieDomainClass": "cefact:SupplyChain_Consignment.Details",
                    "rdfs:comment": "The logistics transport movement for this supply chain consignment at the point when the means of transport departs a country or regional border."
                }
            ]
        },
        {
            "@id": "transport:attachedIOTDevice",
            "@type": "rdf:Property",
            "schema:rangeIncludes": {
                "@id": "transport:IOTDevice"
            },
            "schema:domainIncludes": [
                {
                    "@id": "transport:LogisticsTransportEquipment"
                },
                {
                    "@id": "transport:LogisticsTransportMeans"
                }
            ],
            "rdfs:comment": [
                "An IOT device attached to this logistics transport means.",
                "An IOT device attached to this piece of logistics transport equipment."
            ],
            "rdfs:label": "attachedIOTDevice",
            "unece:cefactElementMetadata": [
                {
                    "@id": "cefact:Logistics_TransportEquipment.Attached.Monitoring_IOTDevice",
                    "@type": "unece:AssociationBIE",
                    "unece:cefactUNId": "UN01013598",
                    "unece:cefactBieDomainClass": "cefact:Logistics_TransportEquipment.Details",
                    "rdfs:comment": "An IOT device attached to this piece of logistics transport equipment."
                },
                {
                    "@id": "cefact:Logistics_TransportMeans.Attached.Monitoring_IOTDevice",
                    "@type": "unece:AssociationBIE",
                    "unece:cefactUNId": "UN01013602",
                    "unece:cefactBieDomainClass": "cefact:Logistics_TransportMeans.Details",
                    "rdfs:comment": "An IOT device attached to this logistics transport means."
                }
            ]
        },
        {
            "@id": "transport:attachedTransportEquipment",
            "@type": "rdf:Property",
            "schema:rangeIncludes": {
                "@id": "transport:TransportEquipment"
            },
            "schema:domainIncludes": [
                {
                    "@id": "transport:LogisticsTransportEquipment"
                },
                {
                    "@id": "transport:LogisticsTransportMeans"
                }
            ],
            "rdfs:comment": [
                "A piece of logistics transport equipment attached to this logistics means of transport.",
                "Transport equipment attached to this piece of logistics transport equipment, such as ropes or refrigeration units."
            ],
            "rdfs:label": "attachedTransportEquipment",
            "unece:cefactElementMetadata": [
                {
                    "@id": "cefact:Logistics_TransportMeans.Attached.Logistics_TransportEquipment",
                    "@type": "unece:AssociationBIE",
                    "unece:cefactUNId": "UN01003831",
                    "unece:cefactBieDomainClass": "cefact:Logistics_TransportMeans.Details",
                    "rdfs:comment": "A piece of logistics transport equipment attached to this logistics means of transport."
                },
                {
                    "@id": "cefact:Logistics_TransportEquipment.Attached.Attached_TransportEquipment",
                    "@type": "unece:AssociationBIE",
                    "unece:cefactUNId": "UN01003797",
                    "unece:cefactBieDomainClass": "cefact:Logistics_TransportEquipment.Details",
                    "rdfs:comment": "Transport equipment attached to this piece of logistics transport equipment, such as ropes or refrigeration units."
                }
            ]
        },
        {
            "@id": "transport:availabilityDueDateTime",
            "@type": "rdf:Property",
            "schema:rangeIncludes": {
                "@id": "xsd:dateTime"
            },
            "schema:domainIncludes": {
                "@id": "transport:SupplyChainConsignment"
            },
            "rdfs:comment": "The date, time, date time or other date time value when this supply chain consignment is due to be available.",
            "rdfs:label": "availabilityDueDateTime",
            "unece:cefactElementMetadata": [
                {
                    "@id": "cefact:SupplyChain_Consignment.AvailabilityDue.DateTime",
                    "@type": "unece:BasicBIE",
                    "unece:TDED": "2111",
                    "unece:cefactUNId": "UN01004169",
                    "unece:cefactBieDomainClass": "cefact:SupplyChain_Consignment.Details",
                    "rdfs:comment": "The date, time, date time or other date time value when this supply chain consignment is due to be available."
                }
            ]
        },
        {
            "@id": "transport:barcodeLabel",
            "@type": "rdf:Property",
            "schema:rangeIncludes": {
                "@id": "transport:Label"
            },
            "schema:domainIncludes": {
                "@id": "transport:LogisticsShippingMarks"
            },
            "rdfs:comment": "A barcode label that is a part of these logistics shipping marks.",
            "rdfs:label": "barcodeLabel",
            "unece:cefactElementMetadata": [
                {
                    "@id": "cefact:Logistics_ShippingMarks.Barcode.Logistics_Label",
                    "@type": "unece:AssociationBIE",
                    "unece:cefactUNId": "UN01003744",
                    "unece:cefactBieDomainClass": "cefact:Logistics_ShippingMarks.Details",
                    "rdfs:comment": "A barcode label that is a part of these logistics shipping marks."
                }
            ]
        },
        {
            "@id": "transport:bondedWarehouseStorageEvent",
            "@type": "rdf:Property",
            "schema:rangeIncludes": {
                "@id": "transport:Event"
            },
            "schema:domainIncludes": [
                {
                    "@id": "transport:LogisticsTransportEquipment"
                },
                {
                    "@id": "transport:SupplyChainConsignment"
                }
            ],
            "rdfs:comment": [
                "A bonded warehouse storage event for this supply chain consignment.",
                "A bonded warehouse storage event specifying when and where this piece of logistics transport equipment will be, or has been, stored."
            ],
            "rdfs:label": "bondedWarehouseStorageEvent",
            "unece:cefactElementMetadata": [
                {
                    "@id": "cefact:Logistics_TransportEquipment.BondedWarehouse_Storage.Transport_Event",
                    "@type": "unece:AssociationBIE",
                    "unece:cefactUNId": "UN01003805",
                    "unece:cefactBieDomainClass": "cefact:Logistics_TransportEquipment.Details",
                    "rdfs:comment": "A bonded warehouse storage event specifying when and where this piece of logistics transport equipment will be, or has been, stored."
                },
                {
                    "@id": "cefact:SupplyChain_Consignment.BondedWarehouse_Storage.Transport_Event",
                    "@type": "unece:AssociationBIE",
                    "unece:cefactUNId": "UN01004256",
                    "unece:cefactBieDomainClass": "cefact:SupplyChain_Consignment.Details",
                    "rdfs:comment": "A bonded warehouse storage event for this supply chain consignment."
                }
            ]
        },
        {
            "@id": "transport:borderClearanceInstructions",
            "@type": "rdf:Property",
            "schema:rangeIncludes": {
                "@id": "transport:Instructions"
            },
            "schema:domainIncludes": {
                "@id": "transport:SupplyChainConsignmentItem"
            },
            "rdfs:comment": "Border clearance instructions for this supply chain consignment item.",
            "rdfs:label": "borderClearanceInstructions",
            "unece:cefactElementMetadata": [
                {
                    "@id": "cefact:SupplyChain_ConsignmentItem.BorderClearance.Transport_Instructions",
                    "@type": "unece:AssociationBIE",
                    "unece:cefactUNId": "UN01009000",
                    "unece:cefactBieDomainClass": "cefact:SupplyChain_ConsignmentItem.Details",
                    "rdfs:comment": "Border clearance instructions for this supply chain consignment item."
                }
            ]
        },
        {
            "@id": "transport:borderCrossingDateTime",
            "@type": "rdf:Property",
            "schema:rangeIncludes": {
                "@id": "xsd:dateTime"
            },
            "schema:domainIncludes": {
                "@id": "transport:LogisticsTransportMovement"
            },
            "rdfs:comment": "A date, time, date time or other date time value when this logistics transport movement crosses a border.",
            "rdfs:label": "borderCrossingDateTime",
            "unece:cefactElementMetadata": [
                {
                    "@id": "cefact:Logistics_TransportMovement.BorderCrossing.DateTime",
                    "@type": "unece:BasicBIE",
                    "unece:cefactUNId": "UN01003847",
                    "unece:cefactBieDomainClass": "cefact:Logistics_TransportMovement.Details",
                    "rdfs:comment": "A date, time, date time or other date time value when this logistics transport movement crosses a border."
                }
            ]
        },
        {
            "@id": "transport:borderCrossingEvent",
            "@type": "rdf:Property",
            "schema:rangeIncludes": {
                "@id": "transport:Event"
            },
            "schema:domainIncludes": {
                "@id": "transport:LogisticsTransportMovement"
            },
            "rdfs:comment": "A border crossing event for this logistics transport movement.",
            "rdfs:label": "borderCrossingEvent",
            "unece:cefactElementMetadata": [
                {
                    "@id": "cefact:Logistics_TransportMovement.BorderCrossing.Transport_Event",
                    "@type": "unece:AssociationBIE",
                    "unece:cefactUNId": "UN01010125",
                    "unece:cefactBieDomainClass": "cefact:Logistics_TransportMovement.Details",
                    "rdfs:comment": "A border crossing event for this logistics transport movement."
                }
            ]
        },
        {
            "@id": "transport:borderCrossingTransportMovement",
            "@type": "rdf:Property",
            "schema:rangeIncludes": {
                "@id": "transport:TransportMovement"
            },
            "schema:domainIncludes": {
                "@id": "transport:SupplyChainConsignment"
            },
            "rdfs:comment": "A border crossing logistics transport movement for this supply chain consignment.",
            "rdfs:label": "borderCrossingTransportMovement",
            "unece:cefactElementMetadata": [
                {
                    "@id": "cefact:SupplyChain_Consignment.BorderCrossing.Logistics_TransportMovement",
                    "@type": "unece:AssociationBIE",
                    "unece:cefactUNId": "UN01004264",
                    "unece:cefactBieDomainClass": "cefact:SupplyChain_Consignment.Details",
                    "rdfs:comment": "A border crossing logistics transport movement for this supply chain consignment."
                }
            ]
        },
        {
            "@id": "transport:cODAmount",
            "@type": "rdf:Property",
            "schema:rangeIncludes": {
                "@id": "xsd:decimal"
            },
            "schema:domainIncludes": {
                "@id": "transport:SupplyChainConsignment"
            },
            "rdfs:comment": "The monetary value of the COD (Cash On Delivery) amount to be collected by the carrier upon delivery of this supply chain consignment.",
            "rdfs:label": "cODAmount",
            "unece:cefactElementMetadata": [
                {
                    "@id": "cefact:SupplyChain_Consignment.COD.Amount",
                    "@type": "unece:BasicBIE",
                    "unece:TDED": "5017",
                    "unece:cefactUNId": "UN01004189",
                    "unece:cefactBieDomainClass": "cefact:SupplyChain_Consignment.Details",
                    "rdfs:comment": "The monetary value of the COD (Cash On Delivery) amount to be collected by the carrier upon delivery of this supply chain consignment."
                }
            ]
        },
        {
            "@id": "transport:callEvent",
            "@type": "rdf:Property",
            "schema:rangeIncludes": {
                "@id": "transport:Event"
            },
            "schema:domainIncludes": {
                "@id": "transport:LogisticsTransportMovement"
            },
            "rdfs:comment": "A call event for this logistics transport movement.",
            "rdfs:label": "callEvent",
            "unece:cefactElementMetadata": [
                {
                    "@id": "cefact:Logistics_TransportMovement.Call.Transport_Event",
                    "@type": "unece:AssociationBIE",
                    "unece:cefactUNId": "UN01010123",
                    "unece:cefactBieDomainClass": "cefact:Logistics_TransportMovement.Details",
                    "rdfs:comment": "A call event for this logistics transport movement."
                }
            ]
        },
        {
            "@id": "transport:callPurposeCode",
            "@type": "rdf:Property",
            "schema:rangeIncludes": {
                "@id": "xsd:token"
            },
            "schema:domainIncludes": {
                "@id": "transport:LogisticsTransportMovement"
            },
            "rdfs:comment": "A code specifying a call purpose for this logistics transport movement.",
            "rdfs:label": "callPurposeCode",
            "unece:cefactElementMetadata": [
                {
                    "@id": "cefact:Logistics_TransportMovement.CallPurpose.Code",
                    "@type": "unece:BasicBIE",
                    "unece:cefactUNId": "UN01013173",
                    "unece:cefactBieDomainClass": "cefact:Logistics_TransportMovement.Details",
                    "rdfs:comment": "A code specifying a call purpose for this logistics transport movement."
                }
            ]
        },
        {
            "@id": "transport:capacityMeasure",
            "@type": "rdf:Property",
            "schema:rangeIncludes": {
                "@id": "xsd:decimal"
            },
            "schema:domainIncludes": [
                {
                    "@id": "transport:LogisticsPackaging"
                },
                {
                    "@id": "transport:SupplyChainPackaging"
                }
            ],
            "rdfs:comment": [
                "A measure of a capacity of this logistics packaging.",
                "The measure of the capacity of this supply chain packaging."
            ],
            "rdfs:label": "capacityMeasure",
            "unece:cefactElementMetadata": [
                {
                    "@id": "cefact:SupplyChain_Packaging.Capacity.Measure",
                    "@type": "unece:BasicBIE",
                    "unece:cefactUNId": "UN01004318",
                    "unece:cefactBieDomainClass": "cefact:SupplyChain_Packaging.Details",
                    "rdfs:comment": "The measure of the capacity of this supply chain packaging."
                },
                {
                    "@id": "cefact:Logistics_Packaging.Capacity.Measure",
                    "@type": "unece:BasicBIE",
                    "unece:cefactUNId": "UN01014955",
                    "unece:cefactBieDomainClass": "cefact:Logistics_Packaging.Details",
                    "rdfs:comment": "A measure of a capacity of this logistics packaging."
                }
            ]
        },
        {
            "@id": "transport:cargoDescription",
            "@type": "rdf:Property",
            "schema:rangeIncludes": {
                "@id": "xsd:string"
            },
            "schema:domainIncludes": {
                "@id": "transport:LogisticsTransportMovement"
            },
            "rdfs:comment": "The textual description of the cargo for this logistics transport movement.",
            "rdfs:label": "cargoDescription",
            "unece:cefactElementMetadata": [
                {
                    "@id": "cefact:Logistics_TransportMovement.CargoDescription.Text",
                    "@type": "unece:BasicBIE",
                    "unece:cefactUNId": "UN01010120",
                    "unece:cefactBieDomainClass": "cefact:Logistics_TransportMovement.Details",
                    "rdfs:comment": "The textual description of the cargo for this logistics transport movement."
                }
            ]
        },
        {
            "@id": "transport:cargoGrossWeightMeasure",
            "@type": "rdf:Property",
            "schema:rangeIncludes": {
                "@id": "xsd:decimal"
            },
            "schema:domainIncludes": {
                "@id": "transport:LogisticsTransportMeans"
            },
            "rdfs:comment": "The measure of the total gross weight (mass) of all cargo loaded onto this logistics means of transport, including packaging but excluding any associated transport equipment.",
            "rdfs:label": "cargoGrossWeightMeasure",
            "unece:cefactElementMetadata": [
                {
                    "@id": "cefact:Logistics_TransportMeans.CargoGrossWeight.Measure",
                    "@type": "unece:BasicBIE",
                    "unece:TDED": "6298",
                    "unece:cefactUNId": "UN01003828",
                    "unece:cefactBieDomainClass": "cefact:Logistics_TransportMeans.Details",
                    "rdfs:comment": "The measure of the total gross weight (mass) of all cargo loaded onto this logistics means of transport, including packaging but excluding any associated transport equipment."
                }
            ]
        },
        {
            "@id": "transport:cargoInsuranceInstructionsInformation",
            "@type": "rdf:Property",
            "schema:rangeIncludes": {
                "@id": "xsd:string"
            },
            "schema:domainIncludes": {
                "@id": "transport:SupplyChainConsignment"
            },
            "rdfs:comment": "Cargo insurance instructions, expressed as text, for this supply chain consignment.",
            "rdfs:label": "cargoInsuranceInstructionsInformation",
            "unece:cefactElementMetadata": [
                {
                    "@id": "cefact:SupplyChain_Consignment.CargoInsuranceInstructions_Information.Text",
                    "@type": "unece:BasicBIE",
                    "unece:cefactUNId": "UN01012578",
                    "unece:cefactBieDomainClass": "cefact:SupplyChain_Consignment.Details",
                    "rdfs:comment": "Cargo insurance instructions, expressed as text, for this supply chain consignment."
                }
            ]
        },
        {
            "@id": "transport:cargoToleranceInformation",
            "@type": "rdf:Property",
            "schema:rangeIncludes": {
                "@id": "xsd:string"
            },
            "schema:domainIncludes": [
                {
                    "@id": "transport:SupplyChainConsignment"
                },
                {
                    "@id": "transport:SupplyChainConsignmentItem"
                }
            ],
            "rdfs:comment": [
                "Cargo tolerance information, expressed as text, for this supply chain consignment item.",
                "Cargo tolerance information, expressed as text, for this supply chain consignment."
            ],
            "rdfs:label": "cargoToleranceInformation",
            "unece:cefactElementMetadata": [
                {
                    "@id": "cefact:SupplyChain_ConsignmentItem.CargoTolerance_Information.Text",
                    "@type": "unece:BasicBIE",
                    "unece:cefactUNId": "UN01004129",
                    "unece:cefactBieDomainClass": "cefact:SupplyChain_ConsignmentItem.Details",
                    "rdfs:comment": "Cargo tolerance information, expressed as text, for this supply chain consignment item."
                },
                {
                    "@id": "cefact:SupplyChain_Consignment.CargoTolerance_Information.Text",
                    "@type": "unece:BasicBIE",
                    "unece:TDED": "4070",
                    "unece:cefactUNId": "UN01004205",
                    "unece:cefactBieDomainClass": "cefact:SupplyChain_Consignment.Details",
                    "rdfs:comment": "Cargo tolerance information, expressed as text, for this supply chain consignment."
                }
            ]
        },
        {
            "@id": "transport:carriedGoodsCharacteristic",
            "@type": "rdf:Property",
            "schema:rangeIncludes": {
                "@id": "transport:GoodsCharacteristic"
            },
            "schema:domainIncludes": {
                "@id": "transport:LogisticsTransportMovement"
            },
            "rdfs:comment": "Material characteristics of goods carried during this logistics transport movement.",
            "rdfs:label": "carriedGoodsCharacteristic",
            "unece:cefactElementMetadata": [
                {
                    "@id": "cefact:Logistics_TransportMovement.Carried.Material_GoodsCharacteristic",
                    "@type": "unece:AssociationBIE",
                    "unece:cefactUNId": "UN01010131",
                    "unece:cefactBieDomainClass": "cefact:Logistics_TransportMovement.Details",
                    "rdfs:comment": "Material characteristics of goods carried during this logistics transport movement."
                }
            ]
        },
        {
            "@id": "transport:carriedInactiveTransportMeans",
            "@type": "rdf:Property",
            "schema:rangeIncludes": {
                "@id": "transport:TransportMeans"
            },
            "schema:domainIncludes": {
                "@id": "transport:LogisticsTransportMovement"
            },
            "rdfs:comment": "Details of transport means inactively carried during the transport movement, such as trucks on a Roll-On/Roll-Off (RORO) ferry.",
            "rdfs:label": "carriedInactiveTransportMeans",
            "unece:cefactElementMetadata": [
                {
                    "@id": "cefact:Logistics_TransportMovement.CarriedInactive.Referenced_TransportMeans",
                    "@type": "unece:AssociationBIE",
                    "unece:cefactUNId": "UN01010133",
                    "unece:cefactBieDomainClass": "cefact:Logistics_TransportMovement.Details",
                    "rdfs:comment": "Details of transport means inactively carried during the transport movement, such as trucks on a Roll-On/Roll-Off (RORO) ferry."
                }
            ]
        },
        {
            "@id": "transport:carriedTransportEquipment",
            "@type": "rdf:Property",
            "schema:rangeIncludes": {
                "@id": "transport:TransportEquipment"
            },
            "schema:domainIncludes": {
                "@id": "transport:LogisticsTransportEquipment"
            },
            "rdfs:comment": "A piece of transport equipment carried on this piece of logistics transport equipment, such as a container placed on a rail wagon.",
            "rdfs:label": "carriedTransportEquipment",
            "unece:cefactElementMetadata": [
                {
                    "@id": "cefact:Logistics_TransportEquipment.Carried.Associated_TransportEquipment",
                    "@type": "unece:AssociationBIE",
                    "unece:cefactUNId": "UN01003798",
                    "unece:cefactBieDomainClass": "cefact:Logistics_TransportEquipment.Details",
                    "rdfs:comment": "A piece of transport equipment carried on this piece of logistics transport equipment, such as a container placed on a rail wagon."
                }
            ]
        },
        {
            "@id": "transport:carrierAcceptanceDateTime",
            "@type": "rdf:Property",
            "schema:rangeIncludes": {
                "@id": "xsd:dateTime"
            },
            "schema:domainIncludes": [
                {
                    "@id": "transport:Referenced_SupplyChainConsignment"
                },
                {
                    "@id": "transport:SupplyChainConsignment"
                }
            ],
            "rdfs:comment": [
                "The date, time, date time or other date time value when this referenced supply chain consignment will be, or has been, accepted by the carrier.",
                "The date, time, date time or other date time value when this supply chain consignment will be, or has been, accepted by the carrier."
            ],
            "rdfs:label": "carrierAcceptanceDateTime",
            "unece:cefactElementMetadata": [
                {
                    "@id": "cefact:Referenced_SupplyChain_Consignment.CarrierAcceptance.DateTime",
                    "@type": "unece:BasicBIE",
                    "unece:TDED": "2127",
                    "unece:cefactUNId": "UN01011052",
                    "unece:cefactBieDomainClass": "cefact:Referenced_SupplyChain_Consignment.Details",
                    "rdfs:comment": "The date, time, date time or other date time value when this referenced supply chain consignment will be, or has been, accepted by the carrier."
                },
                {
                    "@id": "cefact:SupplyChain_Consignment.CarrierAcceptance.DateTime",
                    "@type": "unece:BasicBIE",
                    "unece:TDED": "2127",
                    "unece:cefactUNId": "UN01004170",
                    "unece:cefactBieDomainClass": "cefact:SupplyChain_Consignment.Details",
                    "rdfs:comment": "The date, time, date time or other date time value when this supply chain consignment will be, or has been, accepted by the carrier."
                }
            ]
        },
        {
            "@id": "transport:carrierAcceptanceLocation",
            "@type": "rdf:Property",
            "schema:rangeIncludes": {
                "@id": "transport:Location"
            },
            "schema:domainIncludes": [
                {
                    "@id": "transport:Referenced_SupplyChainConsignment"
                },
                {
                    "@id": "transport:SupplyChainConsignment"
                }
            ],
            "rdfs:comment": [
                "The location where this referenced supply chain consignment will be or has been accepted by the carrier.",
                "The location where this supply chain consignment will be, or has been, accepted by the carrier."
            ],
            "rdfs:label": "carrierAcceptanceLocation",
            "unece:cefactElementMetadata": [
                {
                    "@id": "cefact:Referenced_SupplyChain_Consignment.CarrierAcceptance.Logistics_Location",
                    "@type": "unece:AssociationBIE",
                    "unece:cefactUNId": "UN01011063",
                    "unece:cefactBieDomainClass": "cefact:Referenced_SupplyChain_Consignment.Details",
                    "rdfs:comment": "The location where this referenced supply chain consignment will be or has been accepted by the carrier."
                },
                {
                    "@id": "cefact:SupplyChain_Consignment.CarrierAcceptance.Logistics_Location",
                    "@type": "unece:AssociationBIE",
                    "unece:cefactUNId": "UN01004235",
                    "unece:cefactBieDomainClass": "cefact:SupplyChain_Consignment.Details",
                    "rdfs:comment": "The location where this supply chain consignment will be, or has been, accepted by the carrier."
                }
            ]
        },
        {
            "@id": "transport:carrierAgentParty",
            "@type": "rdf:Property",
            "schema:rangeIncludes": {
                "@id": "transport:Party"
            },
            "schema:domainIncludes": [
                {
                    "@id": "transport:LogisticsTransportMovement"
                },
                {
                    "@id": "transport:SupplyChainConsignment"
                }
            ],
            "rdfs:comment": [
                "The carrier agent trade party for this logistics transport movement.",
                "The party acting as the agent of the carrier for this supply chain consignment."
            ],
            "rdfs:label": "carrierAgentParty",
            "unece:cefactElementMetadata": [
                {
                    "@id": "cefact:SupplyChain_Consignment.CarrierAgent.Trade_Party",
                    "@type": "unece:AssociationBIE",
                    "unece:cefactUNId": "UN01004215",
                    "unece:cefactBieDomainClass": "cefact:SupplyChain_Consignment.Details",
                    "rdfs:comment": "The party acting as the agent of the carrier for this supply chain consignment."
                },
                {
                    "@id": "cefact:Logistics_TransportMovement.CarrierAgent.Trade_Party",
                    "@type": "unece:AssociationBIE",
                    "unece:cefactUNId": "UN01010130",
                    "unece:cefactBieDomainClass": "cefact:Logistics_TransportMovement.Details",
                    "rdfs:comment": "The carrier agent trade party for this logistics transport movement."
                }
            ]
        },
        {
            "@id": "transport:carrierAssignedBookingId",
            "@type": "rdf:Property",
            "schema:rangeIncludes": {
                "@id": "xsd:token"
            },
            "schema:domainIncludes": [
                {
                    "@id": "transport:LogisticsTransportEquipment"
                },
                {
                    "@id": "transport:Referenced_LogisticsTransportEquipment"
                }
            ],
            "rdfs:comment": [
                "A carrier assigned booking identifier for this piece of logistics transport equipment.",
                "A carrier assigned booking identifier for this piece of referenced logistics transport equipment."
            ],
            "rdfs:label": "carrierAssignedBookingId",
            "unece:cefactElementMetadata": [
                {
                    "@id": "cefact:Logistics_TransportEquipment.CarrierAssignedBooking_Identification.Identifier",
                    "@type": "unece:BasicBIE",
                    "unece:TDED": "8260",
                    "unece:cefactUNId": "UN01010099",
                    "unece:cefactBieDomainClass": "cefact:Logistics_TransportEquipment.Details",
                    "rdfs:comment": "A carrier assigned booking identifier for this piece of logistics transport equipment."
                },
                {
                    "@id": "cefact:Referenced_Logistics_TransportEquipment.CarrierAssignedBooking_Identification.Identifier",
                    "@type": "unece:BasicBIE",
                    "unece:TDED": "8260",
                    "unece:cefactUNId": "UN01010137",
                    "unece:cefactBieDomainClass": "cefact:Referenced_Logistics_TransportEquipment.Details",
                    "rdfs:comment": "A carrier assigned booking identifier for this piece of referenced logistics transport equipment."
                }
            ]
        },
        {
            "@id": "transport:carrierAssignedId",
            "@type": "rdf:Property",
            "schema:rangeIncludes": {
                "@id": "xsd:token"
            },
            "schema:domainIncludes": [
                {
                    "@id": "transport:Referenced_SupplyChainConsignment"
                },
                {
                    "@id": "transport:SupplyChainConsignment"
                }
            ],
            "rdfs:comment": [
                "The unique identifier assigned by the carrier to this referenced supply chain consignment, such as a booking reference number when cargo space is reserved prior to loading.",
                "The unique identifier assigned by the carrier to this supply chain consignment, such as a booking reference number when cargo space is reserved prior to loading."
            ],
            "rdfs:label": "carrierAssignedId",
            "unece:cefactElementMetadata": [
                {
                    "@id": "cefact:Referenced_SupplyChain_Consignment.CarrierAssigned.Identifier",
                    "@type": "unece:BasicBIE",
                    "unece:TDED": "1016",
                    "unece:cefactUNId": "UN01004044",
                    "unece:cefactBieDomainClass": "cefact:Referenced_SupplyChain_Consignment.Details",
                    "rdfs:comment": "The unique identifier assigned by the carrier to this referenced supply chain consignment, such as a booking reference number when cargo space is reserved prior to loading."
                },
                {
                    "@id": "cefact:SupplyChain_Consignment.CarrierAssigned.Identifier",
                    "@type": "unece:BasicBIE",
                    "unece:TDED": "1016",
                    "unece:cefactUNId": "UN01004164",
                    "unece:cefactBieDomainClass": "cefact:SupplyChain_Consignment.Details",
                    "rdfs:comment": "The unique identifier assigned by the carrier to this supply chain consignment, such as a booking reference number when cargo space is reserved prior to loading."
                }
            ]
        },
        {
            "@id": "transport:carrierParty",
            "@type": "rdf:Property",
            "schema:rangeIncludes": {
                "@id": "transport:Party"
            },
            "schema:domainIncludes": [
                {
                    "@id": "transport:LogisticsTransportEquipment"
                },
                {
                    "@id": "transport:LogisticsTransportMovement"
                },
                {
                    "@id": "transport:Referenced_SupplyChainConsignment"
                },
                {
                    "@id": "transport:SupplyChainConsignment"
                }
            ],
            "rdfs:comment": [
                "A carrier party for this logistics transport movement.",
                "A carrier party for this piece of logistics transport equipment.",
                "The carrier party for this referenced supply chain consignment.",
                "The carrier party for this supply chain consignment."
            ],
            "rdfs:label": "carrierParty",
            "unece:cefactElementMetadata": [
                {
                    "@id": "cefact:SupplyChain_Consignment.Carrier.Trade_Party",
                    "@type": "unece:AssociationBIE",
                    "unece:cefactUNId": "UN01004214",
                    "unece:cefactBieDomainClass": "cefact:SupplyChain_Consignment.Details",
                    "rdfs:comment": "The carrier party for this supply chain consignment."
                },
                {
                    "@id": "cefact:Logistics_TransportEquipment.Carrier.Trade_Party",
                    "@type": "unece:AssociationBIE",
                    "unece:cefactUNId": "UN01003812",
                    "unece:cefactBieDomainClass": "cefact:Logistics_TransportEquipment.Details",
                    "rdfs:comment": "A carrier party for this piece of logistics transport equipment."
                },
                {
                    "@id": "cefact:Logistics_TransportMovement.Carrier.Trade_Party",
                    "@type": "unece:AssociationBIE",
                    "unece:cefactUNId": "UN01003863",
                    "unece:cefactBieDomainClass": "cefact:Logistics_TransportMovement.Details",
                    "rdfs:comment": "A carrier party for this logistics transport movement."
                },
                {
                    "@id": "cefact:Referenced_SupplyChain_Consignment.Carrier.Trade_Party",
                    "@type": "unece:AssociationBIE",
                    "unece:cefactUNId": "UN01011059",
                    "unece:cefactBieDomainClass": "cefact:Referenced_SupplyChain_Consignment.Details",
                    "rdfs:comment": "The carrier party for this referenced supply chain consignment."
                }
            ]
        },
        {
            "@id": "transport:carrierProvidedInformation",
            "@type": "rdf:Property",
            "schema:rangeIncludes": {
                "@id": "xsd:string"
            },
            "schema:domainIncludes": {
                "@id": "transport:SupplyChainConsignment"
            },
            "rdfs:comment": "Information, expressed as text, provided by the carrier for this supply chain consignment.",
            "rdfs:label": "carrierProvidedInformation",
            "unece:cefactElementMetadata": [
                {
                    "@id": "cefact:SupplyChain_Consignment.CarrierProvided_Information.Text",
                    "@type": "unece:BasicBIE",
                    "unece:TDED": "4070",
                    "unece:cefactUNId": "UN01004204",
                    "unece:cefactBieDomainClass": "cefact:SupplyChain_Consignment.Details",
                    "rdfs:comment": "Information, expressed as text, provided by the carrier for this supply chain consignment."
                }
            ]
        },
        {
            "@id": "transport:certificationIndicator",
            "@type": "rdf:Property",
            "schema:rangeIncludes": {
                "@id": "xsd:boolean"
            },
            "schema:domainIncludes": {
                "@id": "transport:LogisticsPackaging"
            },
            "rdfs:comment": "The indication whether or not this logistics packaging has a certification.",
            "rdfs:label": "certificationIndicator",
            "unece:cefactElementMetadata": [
                {
                    "@id": "cefact:Logistics_Packaging.Certification.Indicator",
                    "@type": "unece:BasicBIE",
                    "unece:cefactUNId": "UN01014963",
                    "unece:cefactBieDomainClass": "cefact:Logistics_Packaging.Details",
                    "rdfs:comment": "The indication whether or not this logistics packaging has a certification."
                }
            ]
        },
        {
            "@id": "transport:certifiedEmission",
            "@type": "rdf:Property",
            "schema:rangeIncludes": {
                "@id": "transport:Emission"
            },
            "schema:domainIncludes": {
                "@id": "transport:LogisticsTransportMeans"
            },
            "rdfs:comment": "A certified level of pollution calculated for an emission from this logistics transport means.",
            "rdfs:label": "certifiedEmission",
            "unece:cefactElementMetadata": [
                {
                    "@id": "cefact:Logistics_TransportMeans.Certified.Calculated_Emission",
                    "@type": "unece:AssociationBIE",
                    "unece:cefactUNId": "UN01010115",
                    "unece:cefactBieDomainClass": "cefact:Logistics_TransportMeans.Details",
                    "rdfs:comment": "A certified level of pollution calculated for an emission from this logistics transport means."
                }
            ]
        },
        {
            "@id": "transport:characteristic",
            "@type": "rdf:Property",
            "schema:rangeIncludes": {
                "@id": "xsd:string"
            },
            "schema:domainIncludes": [
                {
                    "@id": "transport:AssociatedTransportEquipment"
                },
                {
                    "@id": "transport:AttachedTransportEquipment"
                },
                {
                    "@id": "transport:LogisticsTransportEquipment"
                },
                {
                    "@id": "transport:Referenced_LogisticsTransportEquipment"
                }
            ],
            "rdfs:comment": [
                "The characteristic or characteristics, expressed as text, of a piece of logistics transport equipment, such as its size and type.",
                "The characteristics, expressed as text, of a referenced piece of logistics transport equipment, such as size and type.",
                "The textual description of the characteristics, i.e. size and type, of this piece of associated transport equipment.",
                "The textual description of the characteristics, i.e. size and type, of this piece of attached transport equipment."
            ],
            "rdfs:label": "characteristic",
            "unece:cefactElementMetadata": [
                {
                    "@id": "cefact:Referenced_Logistics_TransportEquipment.Characteristic.Text",
                    "@type": "unece:BasicBIE",
                    "unece:TDED": "8154",
                    "unece:cefactUNId": "UN01004026",
                    "unece:cefactBieDomainClass": "cefact:Referenced_Logistics_TransportEquipment.Details",
                    "rdfs:comment": "The characteristics, expressed as text, of a referenced piece of logistics transport equipment, such as size and type."
                },
                {
                    "@id": "cefact:Associated_TransportEquipment.Characteristic.Text",
                    "@type": "unece:BasicBIE",
                    "unece:TDED": "8154",
                    "unece:cefactUNId": "UN01003415",
                    "unece:cefactBieDomainClass": "cefact:Associated_TransportEquipment.Details",
                    "rdfs:comment": "The textual description of the characteristics, i.e. size and type, of this piece of associated transport equipment."
                },
                {
                    "@id": "cefact:Logistics_TransportEquipment.Characteristic.Text",
                    "@type": "unece:BasicBIE",
                    "unece:TDED": "8154",
                    "unece:cefactUNId": "UN01003769",
                    "unece:cefactBieDomainClass": "cefact:Logistics_TransportEquipment.Details",
                    "rdfs:comment": "The characteristic or characteristics, expressed as text, of a piece of logistics transport equipment, such as its size and type."
                },
                {
                    "@id": "cefact:Attached_TransportEquipment.Characteristic.Text",
                    "@type": "unece:BasicBIE",
                    "unece:TDED": "8154",
                    "unece:cefactUNId": "UN01003420",
                    "unece:cefactBieDomainClass": "cefact:Attached_TransportEquipment.Details",
                    "rdfs:comment": "The textual description of the characteristics, i.e. size and type, of this piece of attached transport equipment."
                }
            ]
        },
        {
            "@id": "transport:chargeableTransportationStageQuantity",
            "@type": "rdf:Property",
            "schema:rangeIncludes": {
                "@id": "xsd:decimal"
            },
            "schema:domainIncludes": {
                "@id": "transport:SupplyChainConsignment"
            },
            "rdfs:comment": "The number of separately chargeable transportation stages to be covered by this supply chain consignment.",
            "rdfs:label": "chargeableTransportationStageQuantity",
            "unece:cefactElementMetadata": [
                {
                    "@id": "cefact:SupplyChain_Consignment.ChargeableTransportationStage.Quantity",
                    "@type": "unece:BasicBIE",
                    "unece:cefactUNId": "UN01004199",
                    "unece:cefactBieDomainClass": "cefact:SupplyChain_Consignment.Details",
                    "rdfs:comment": "The number of separately chargeable transportation stages to be covered by this supply chain consignment."
                }
            ]
        },
        {
            "@id": "transport:chargeableWeightMeasure",
            "@type": "rdf:Property",
            "schema:rangeIncludes": {
                "@id": "xsd:decimal"
            },
            "schema:domainIncludes": [
                {
                    "@id": "transport:SupplyChainConsignment"
                },
                {
                    "@id": "transport:SupplyChainConsignmentItem"
                }
            ],
            "rdfs:comment": [
                "A measure of a chargeable weight of this supply chain consignment.",
                "A measure of the supply chain consignment item weight on which charges are to be based."
            ],
            "rdfs:label": "chargeableWeightMeasure",
            "unece:cefactElementMetadata": [
                {
                    "@id": "cefact:SupplyChain_Consignment.ChargeableWeight.Measure",
                    "@type": "unece:BasicBIE",
                    "unece:cefactUNId": "UN01004177",
                    "unece:cefactBieDomainClass": "cefact:SupplyChain_Consignment.Details",
                    "rdfs:comment": "A measure of a chargeable weight of this supply chain consignment."
                },
                {
                    "@id": "cefact:SupplyChain_ConsignmentItem.ChargeableWeight.Measure",
                    "@type": "unece:BasicBIE",
                    "unece:cefactUNId": "UN01004123",
                    "unece:cefactBieDomainClass": "cefact:SupplyChain_ConsignmentItem.Details",
                    "rdfs:comment": "A measure of the supply chain consignment item weight on which charges are to be based."
                }
            ]
        },
        {
            "@id": "transport:classificationDocument",
            "@type": "rdf:Property",
            "schema:rangeIncludes": {
                "@id": "transport:Document"
            },
            "schema:domainIncludes": [
                {
                    "@id": "transport:SupplyChainConsignment"
                },
                {
                    "@id": "transport:SupplyChainConsignmentItem"
                }
            ],
            "rdfs:comment": [
                "The referenced classification document for this supply chain consignment item.",
                "The referenced classification document for this supply chain consignment."
            ],
            "rdfs:label": "classificationDocument",
            "unece:cefactElementMetadata": [
                {
                    "@id": "cefact:SupplyChain_Consignment.Classification.Referenced_Document",
                    "@type": "unece:AssociationBIE",
                    "unece:cefactUNId": "UN01014450",
                    "unece:cefactBieDomainClass": "cefact:SupplyChain_Consignment.Details",
                    "rdfs:comment": "The referenced classification document for this supply chain consignment."
                },
                {
                    "@id": "cefact:SupplyChain_ConsignmentItem.Classification.Referenced_Document",
                    "@type": "unece:AssociationBIE",
                    "unece:cefactUNId": "UN01014446",
                    "unece:cefactBieDomainClass": "cefact:SupplyChain_ConsignmentItem.Details",
                    "rdfs:comment": "The referenced classification document for this supply chain consignment item."
                }
            ]
        },
        {
            "@id": "transport:closingDateTime",
            "@type": "rdf:Property",
            "schema:rangeIncludes": {
                "@id": "xsd:dateTime"
            },
            "schema:domainIncludes": {
                "@id": "transport:LogisticsTransportMovement"
            },
            "rdfs:comment": "The date, time, date time, or other date time value by which cargo should be loaded onto the means of transport for the departure of this logistics transport movement.",
            "rdfs:label": "closingDateTime",
            "unece:cefactElementMetadata": [
                {
                    "@id": "cefact:Logistics_TransportMovement.Closing.DateTime",
                    "@type": "unece:BasicBIE",
                    "unece:cefactUNId": "UN01003846",
                    "unece:cefactBieDomainClass": "cefact:Logistics_TransportMovement.Details",
                    "rdfs:comment": "The date, time, date time, or other date time value by which cargo should be loaded onto the means of transport for the departure of this logistics transport movement."
                }
            ]
        },
        {
            "@id": "transport:commodityConsolidatorAgentParty",
            "@type": "rdf:Property",
            "schema:rangeIncludes": {
                "@id": "transport:Party"
            },
            "schema:domainIncludes": {
                "@id": "transport:LogisticsTransportMovement"
            },
            "rdfs:comment": "The commodity consolidator agent party for this logistics transport movement.",
            "rdfs:label": "commodityConsolidatorAgentParty",
            "unece:cefactElementMetadata": [
                {
                    "@id": "cefact:Logistics_TransportMovement.CommodityConsolidatorAgent.Trade_Party",
                    "@type": "unece:AssociationBIE",
                    "unece:cefactUNId": "UN01003868",
                    "unece:cefactBieDomainClass": "cefact:Logistics_TransportMovement.Details",
                    "rdfs:comment": "The commodity consolidator agent party for this logistics transport movement."
                }
            ]
        },
        {
            "@id": "transport:commodityConsolidatorParty",
            "@type": "rdf:Property",
            "schema:rangeIncludes": {
                "@id": "transport:Party"
            },
            "schema:domainIncludes": {
                "@id": "transport:LogisticsTransportMovement"
            },
            "rdfs:comment": "The commodity consolidator party for this logistics transport movement.",
            "rdfs:label": "commodityConsolidatorParty",
            "unece:cefactElementMetadata": [
                {
                    "@id": "cefact:Logistics_TransportMovement.CommodityConsolidator.Trade_Party",
                    "@type": "unece:AssociationBIE",
                    "unece:cefactUNId": "UN01003867",
                    "unece:cefactBieDomainClass": "cefact:Logistics_TransportMovement.Details",
                    "rdfs:comment": "The commodity consolidator party for this logistics transport movement."
                }
            ]
        },
        {
            "@id": "transport:companySecurityOfficerPerson",
            "@type": "rdf:Property",
            "schema:rangeIncludes": {
                "@id": "transport:Person"
            },
            "schema:domainIncludes": {
                "@id": "transport:LogisticsTransportMeans"
            },
            "rdfs:comment": "A person who is a company security officer for this logistics transport means.",
            "rdfs:label": "companySecurityOfficerPerson",
            "unece:cefactElementMetadata": [
                {
                    "@id": "cefact:Logistics_TransportMeans.CompanySecurityOfficer.Transport_Person",
                    "@type": "unece:AssociationBIE",
                    "unece:cefactUNId": "UN01013171",
                    "unece:cefactBieDomainClass": "cefact:Logistics_TransportMeans.Details",
                    "rdfs:comment": "A person who is a company security officer for this logistics transport means."
                }
            ]
        },
        {
            "@id": "transport:conditionCode",
            "@type": "rdf:Property",
            "schema:rangeIncludes": {
                "@id": "xsd:token"
            },
            "schema:domainIncludes": [
                {
                    "@id": "transport:LogisticsPackaging"
                },
                {
                    "@id": "transport:SupplyChainPackaging"
                }
            ],
            "rdfs:comment": [
                "A code specifying a condition of this logistics packaging.",
                "A code specifying the condition of this supply chain packaging."
            ],
            "rdfs:label": "conditionCode",
            "unece:cefactElementMetadata": [
                {
                    "@id": "cefact:Logistics_Packaging.Condition.Code",
                    "@type": "unece:BasicBIE",
                    "unece:cefactUNId": "UN01014953",
                    "unece:cefactBieDomainClass": "cefact:Logistics_Packaging.Details",
                    "rdfs:comment": "A code specifying a condition of this logistics packaging."
                },
                {
                    "@id": "cefact:SupplyChain_Packaging.Condition.Code",
                    "@type": "unece:BasicBIE",
                    "unece:cefactUNId": "UN01004316",
                    "unece:cefactBieDomainClass": "cefact:SupplyChain_Packaging.Details",
                    "rdfs:comment": "A code specifying the condition of this supply chain packaging."
                }
            ]
        },
        {
            "@id": "transport:conferenceCode",
            "@type": "rdf:Property",
            "schema:rangeIncludes": {
                "@id": "xsd:token"
            },
            "schema:domainIncludes": {
                "@id": "transport:LogisticsTransportMeans"
            },
            "rdfs:comment": "The code specifying the conference for this logistics means of transport.",
            "rdfs:label": "conferenceCode",
            "unece:cefactElementMetadata": [
                {
                    "@id": "cefact:Logistics_TransportMeans.Conference.Code",
                    "@type": "unece:BasicBIE",
                    "unece:cefactUNId": "UN01010103",
                    "unece:cefactBieDomainClass": "cefact:Logistics_TransportMeans.Details",
                    "rdfs:comment": "The code specifying the conference for this logistics means of transport."
                }
            ]
        },
        {
            "@id": "transport:connectingCarrierParty",
            "@type": "rdf:Property",
            "schema:rangeIncludes": {
                "@id": "transport:Party"
            },
            "schema:domainIncludes": {
                "@id": "transport:SupplyChainConsignment"
            },
            "rdfs:comment": "A connecting carrier party for this supply chain consignment.",
            "rdfs:label": "connectingCarrierParty",
            "unece:cefactElementMetadata": [
                {
                    "@id": "cefact:SupplyChain_Consignment.ConnectingCarrier.Trade_Party",
                    "@type": "unece:AssociationBIE",
                    "unece:cefactUNId": "UN01004227",
                    "unece:cefactBieDomainClass": "cefact:SupplyChain_Consignment.Details",
                    "rdfs:comment": "A connecting carrier party for this supply chain consignment."
                }
            ]
        },
        {
            "@id": "transport:consigneeAgentParty",
            "@type": "rdf:Property",
            "schema:rangeIncludes": {
                "@id": "transport:Party"
            },
            "schema:domainIncludes": {
                "@id": "transport:SupplyChainConsignment"
            },
            "rdfs:comment": "The party authorized to act for or on behalf of the consignee for this supply chain consignment.",
            "rdfs:label": "consigneeAgentParty",
            "unece:cefactElementMetadata": [
                {
                    "@id": "cefact:SupplyChain_Consignment.ConsigneeAgent.Trade_Party",
                    "@type": "unece:AssociationBIE",
                    "unece:cefactUNId": "UN01004233",
                    "unece:cefactBieDomainClass": "cefact:SupplyChain_Consignment.Details",
                    "rdfs:comment": "The party authorized to act for or on behalf of the consignee for this supply chain consignment."
                }
            ]
        },
        {
            "@id": "transport:consigneeAssignedConsignmentId",
            "@type": "rdf:Property",
            "schema:rangeIncludes": {
                "@id": "xsd:token"
            },
            "schema:domainIncludes": {
                "@id": "transport:LogisticsTransportEquipment"
            },
            "rdfs:comment": "The consignee assigned consignment identifier for this piece of logistics transport equipment.",
            "rdfs:label": "consigneeAssignedConsignmentId",
            "unece:cefactElementMetadata": [
                {
                    "@id": "cefact:Logistics_TransportEquipment.ConsigneeAssignedConsignment_Identification.Identifier",
                    "@type": "unece:BasicBIE",
                    "unece:TDED": "8260",
                    "unece:cefactUNId": "UN01011039",
                    "unece:cefactBieDomainClass": "cefact:Logistics_TransportEquipment.Details",
                    "rdfs:comment": "The consignee assigned consignment identifier for this piece of logistics transport equipment."
                }
            ]
        },
        {
            "@id": "transport:consigneeAssignedId",
            "@type": "rdf:Property",
            "schema:rangeIncludes": {
                "@id": "xsd:token"
            },
            "schema:domainIncludes": [
                {
                    "@id": "transport:Referenced_SupplyChainConsignment"
                },
                {
                    "@id": "transport:SupplyChainConsignment"
                }
            ],
            "rdfs:comment": [
                "The unique identifier assigned by the consignee to this referenced supply chain consignment.",
                "The unique identifier assigned by the consignee to this supply chain consignment."
            ],
            "rdfs:label": "consigneeAssignedId",
            "unece:cefactElementMetadata": [
                {
                    "@id": "cefact:SupplyChain_Consignment.ConsigneeAssigned.Identifier",
                    "@type": "unece:BasicBIE",
                    "unece:TDED": "1362",
                    "unece:cefactUNId": "UN01004162",
                    "unece:cefactBieDomainClass": "cefact:SupplyChain_Consignment.Details",
                    "rdfs:comment": "The unique identifier assigned by the consignee to this supply chain consignment."
                },
                {
                    "@id": "cefact:Referenced_SupplyChain_Consignment.ConsigneeAssigned.Identifier",
                    "@type": "unece:BasicBIE",
                    "unece:TDED": "1362",
                    "unece:cefactUNId": "UN01004043",
                    "unece:cefactBieDomainClass": "cefact:Referenced_SupplyChain_Consignment.Details",
                    "rdfs:comment": "The unique identifier assigned by the consignee to this referenced supply chain consignment."
                }
            ]
        },
        {
            "@id": "transport:consigneeParty",
            "@type": "rdf:Property",
            "schema:rangeIncludes": {
                "@id": "transport:Party"
            },
            "schema:domainIncludes": [
                {
                    "@id": "transport:Referenced_SupplyChainConsignment"
                },
                {
                    "@id": "transport:SupplyChainConsignment"
                }
            ],
            "rdfs:comment": [
                "The consignee party for this referenced supply chain consignment.",
                "The consignee party for this supply chain consignment."
            ],
            "rdfs:label": "consigneeParty",
            "unece:cefactElementMetadata": [
                {
                    "@id": "cefact:SupplyChain_Consignment.Consignee.Trade_Party",
                    "@type": "unece:AssociationBIE",
                    "unece:cefactUNId": "UN01004213",
                    "unece:cefactBieDomainClass": "cefact:SupplyChain_Consignment.Details",
                    "rdfs:comment": "The consignee party for this supply chain consignment."
                },
                {
                    "@id": "cefact:Referenced_SupplyChain_Consignment.Consignee.Trade_Party",
                    "@type": "unece:AssociationBIE",
                    "unece:cefactUNId": "UN01011055",
                    "unece:cefactBieDomainClass": "cefact:Referenced_SupplyChain_Consignment.Details",
                    "rdfs:comment": "The consignee party for this referenced supply chain consignment."
                }
            ]
        },
        {
            "@id": "transport:consigneeReceiptLocation",
            "@type": "rdf:Property",
            "schema:rangeIncludes": {
                "@id": "transport:Location"
            },
            "schema:domainIncludes": {
                "@id": "transport:SupplyChainConsignment"
            },
            "rdfs:comment": "The location at which this supply chain consignment will be or has been received by the consignee.",
            "rdfs:label": "consigneeReceiptLocation",
            "unece:cefactElementMetadata": [
                {
                    "@id": "cefact:SupplyChain_Consignment.ConsigneeReceipt.Logistics_Location",
                    "@type": "unece:AssociationBIE",
                    "unece:cefactUNId": "UN01004237",
                    "unece:cefactBieDomainClass": "cefact:SupplyChain_Consignment.Details",
                    "rdfs:comment": "The location at which this supply chain consignment will be or has been received by the consignee."
                }
            ]
        },
        {
            "@id": "transport:consignmentItemQuantity",
            "@type": "rdf:Property",
            "schema:rangeIncludes": {
                "@id": "xsd:decimal"
            },
            "schema:domainIncludes": [
                {
                    "@id": "transport:Referenced_SupplyChainConsignment"
                },
                {
                    "@id": "transport:SupplyChainConsignment"
                }
            ],
            "rdfs:comment": [
                "The number of consignment items separately defined for transport or customs purposes within this referenced supply chain consignment.",
                "The number of consignment items separately defined for transport or customs purposes within this supply chain consignment."
            ],
            "rdfs:label": "consignmentItemQuantity",
            "unece:cefactElementMetadata": [
                {
                    "@id": "cefact:SupplyChain_Consignment.ConsignmentItem.Quantity",
                    "@type": "unece:BasicBIE",
                    "unece:TDED": "7240",
                    "unece:cefactUNId": "UN01004196",
                    "unece:cefactBieDomainClass": "cefact:SupplyChain_Consignment.Details",
                    "rdfs:comment": "The number of consignment items separately defined for transport or customs purposes within this supply chain consignment."
                },
                {
                    "@id": "cefact:Referenced_SupplyChain_Consignment.ConsignmentItem.Quantity",
                    "@type": "unece:BasicBIE",
                    "unece:TDED": "7240",
                    "unece:cefactUNId": "UN01011051",
                    "unece:cefactBieDomainClass": "cefact:Referenced_SupplyChain_Consignment.Details",
                    "rdfs:comment": "The number of consignment items separately defined for transport or customs purposes within this referenced supply chain consignment."
                }
            ]
        },
        {
            "@id": "transport:consignmentQuantity",
            "@type": "rdf:Property",
            "schema:rangeIncludes": {
                "@id": "xsd:decimal"
            },
            "schema:domainIncludes": {
                "@id": "transport:LogisticsTransportMovement"
            },
            "rdfs:comment": "The number of consignments in this logistics transport movement.",
            "rdfs:label": "consignmentQuantity",
            "unece:cefactElementMetadata": [
                {
                    "@id": "cefact:Logistics_TransportMovement.Consignment.Quantity",
                    "@type": "unece:BasicBIE",
                    "unece:cefactUNId": "UN01006136",
                    "unece:cefactBieDomainClass": "cefact:Logistics_TransportMovement.Details",
                    "rdfs:comment": "The number of consignments in this logistics transport movement."
                }
            ]
        },
        {
            "@id": "transport:consignorAgentParty",
            "@type": "rdf:Property",
            "schema:rangeIncludes": {
                "@id": "transport:Party"
            },
            "schema:domainIncludes": {
                "@id": "transport:SupplyChainConsignment"
            },
            "rdfs:comment": "The party authorized to act for or on behalf of the consignor for this supply chain consignment.",
            "rdfs:label": "consignorAgentParty",
            "unece:cefactElementMetadata": [
                {
                    "@id": "cefact:SupplyChain_Consignment.ConsignorAgent.Trade_Party",
                    "@type": "unece:AssociationBIE",
                    "unece:cefactUNId": "UN01004232",
                    "unece:cefactBieDomainClass": "cefact:SupplyChain_Consignment.Details",
                    "rdfs:comment": "The party authorized to act for or on behalf of the consignor for this supply chain consignment."
                }
            ]
        },
        {
            "@id": "transport:consignorAssignedId",
            "@type": "rdf:Property",
            "schema:rangeIncludes": {
                "@id": "xsd:token"
            },
            "schema:domainIncludes": [
                {
                    "@id": "transport:Referenced_SupplyChainConsignment"
                },
                {
                    "@id": "transport:SupplyChainConsignment"
                }
            ],
            "rdfs:comment": [
                "The unique identifier assigned by the consignor to this referenced supply chain consignment.",
                "The unique identifier assigned by the consignor to this supply chain consignment."
            ],
            "rdfs:label": "consignorAssignedId",
            "unece:cefactElementMetadata": [
                {
                    "@id": "cefact:SupplyChain_Consignment.ConsignorAssigned.Identifier",
                    "@type": "unece:BasicBIE",
                    "unece:TDED": "1140",
                    "unece:cefactUNId": "UN01004161",
                    "unece:cefactBieDomainClass": "cefact:SupplyChain_Consignment.Details",
                    "rdfs:comment": "The unique identifier assigned by the consignor to this supply chain consignment."
                },
                {
                    "@id": "cefact:Referenced_SupplyChain_Consignment.ConsignorAssigned.Identifier",
                    "@type": "unece:BasicBIE",
                    "unece:TDED": "1140",
                    "unece:cefactUNId": "UN01004042",
                    "unece:cefactBieDomainClass": "cefact:Referenced_SupplyChain_Consignment.Details",
                    "rdfs:comment": "The unique identifier assigned by the consignor to this referenced supply chain consignment."
                }
            ]
        },
        {
            "@id": "transport:consignorParty",
            "@type": "rdf:Property",
            "schema:rangeIncludes": {
                "@id": "transport:Party"
            },
            "schema:domainIncludes": [
                {
                    "@id": "transport:Referenced_SupplyChainConsignment"
                },
                {
                    "@id": "transport:SupplyChainConsignment"
                }
            ],
            "rdfs:comment": [
                "The consignor party for this referenced supply chain consignment.",
                "The consignor party for this supply chain consignment."
            ],
            "rdfs:label": "consignorParty",
            "unece:cefactElementMetadata": [
                {
                    "@id": "cefact:SupplyChain_Consignment.Consignor.Trade_Party",
                    "@type": "unece:AssociationBIE",
                    "unece:cefactUNId": "UN01004212",
                    "unece:cefactBieDomainClass": "cefact:SupplyChain_Consignment.Details",
                    "rdfs:comment": "The consignor party for this supply chain consignment."
                },
                {
                    "@id": "cefact:Referenced_SupplyChain_Consignment.Consignor.Trade_Party",
                    "@type": "unece:AssociationBIE",
                    "unece:cefactUNId": "UN01011054",
                    "unece:cefactBieDomainClass": "cefact:Referenced_SupplyChain_Consignment.Details",
                    "rdfs:comment": "The consignor party for this referenced supply chain consignment."
                }
            ]
        },
        {
            "@id": "transport:consignorProvidedInformation",
            "@type": "rdf:Property",
            "schema:rangeIncludes": {
                "@id": "xsd:string"
            },
            "schema:domainIncludes": {
                "@id": "transport:SupplyChainConsignment"
            },
            "rdfs:comment": "Information, expressed as text, provided by the consignor for this supply chain consignment.",
            "rdfs:label": "consignorProvidedInformation",
            "unece:cefactElementMetadata": [
                {
                    "@id": "cefact:SupplyChain_Consignment.ConsignorProvided_Information.Text",
                    "@type": "unece:BasicBIE",
                    "unece:TDED": "4070",
                    "unece:cefactUNId": "UN01013607",
                    "unece:cefactBieDomainClass": "cefact:SupplyChain_Consignment.Details",
                    "rdfs:comment": "Information, expressed as text, provided by the consignor for this supply chain consignment."
                }
            ]
        },
        {
            "@id": "transport:consolidationEvent",
            "@type": "rdf:Property",
            "schema:rangeIncludes": {
                "@id": "transport:Event"
            },
            "schema:domainIncludes": {
                "@id": "transport:LogisticsTransportEquipment"
            },
            "rdfs:comment": "A consolidation event specifying when and where this piece of logistics transport equipment will be, or has been, stuffed.",
            "rdfs:label": "consolidationEvent",
            "unece:cefactElementMetadata": [
                {
                    "@id": "cefact:Logistics_TransportEquipment.Consolidation.Transport_Event",
                    "@type": "unece:AssociationBIE",
                    "unece:cefactUNId": "UN01008984",
                    "unece:cefactBieDomainClass": "cefact:Logistics_TransportEquipment.Details",
                    "rdfs:comment": "A consolidation event specifying when and where this piece of logistics transport equipment will be, or has been, stuffed."
                }
            ]
        },
        {
            "@id": "transport:consolidatorParty",
            "@type": "rdf:Property",
            "schema:rangeIncludes": {
                "@id": "transport:Party"
            },
            "schema:domainIncludes": {
                "@id": "transport:SupplyChainConsignment"
            },
            "rdfs:comment": "The party responsible for the consolidation of this supply chain consignment.",
            "rdfs:label": "consolidatorParty",
            "unece:cefactElementMetadata": [
                {
                    "@id": "cefact:SupplyChain_Consignment.Consolidator.Trade_Party",
                    "@type": "unece:AssociationBIE",
                    "unece:cefactUNId": "UN01004230",
                    "unece:cefactBieDomainClass": "cefact:SupplyChain_Consignment.Details",
                    "rdfs:comment": "The party responsible for the consolidation of this supply chain consignment."
                }
            ]
        },
        {
            "@id": "transport:consortiumCarrierParty",
            "@type": "rdf:Property",
            "schema:rangeIncludes": {
                "@id": "transport:Party"
            },
            "schema:domainIncludes": {
                "@id": "transport:LogisticsTransportMovement"
            },
            "rdfs:comment": "A consortium carrier party for this logistics transport movement.",
            "rdfs:label": "consortiumCarrierParty",
            "unece:cefactElementMetadata": [
                {
                    "@id": "cefact:Logistics_TransportMovement.Consortium_Carrier.Trade_Party",
                    "@type": "unece:AssociationBIE",
                    "unece:cefactUNId": "UN01003864",
                    "unece:cefactBieDomainClass": "cefact:Logistics_TransportMovement.Details",
                    "rdfs:comment": "A consortium carrier party for this logistics transport movement."
                }
            ]
        },
        {
            "@id": "transport:containedConsignment",
            "@type": "rdf:Property",
            "schema:rangeIncludes": {
                "@id": "transport:Consignment"
            },
            "schema:domainIncludes": [
                {
                    "@id": "transport:AssociatedTransportEquipment"
                },
                {
                    "@id": "transport:LogisticsTransportEquipment"
                }
            ],
            "rdfs:comment": [
                "A consignment contained in this piece of logistics transport equipment.",
                "A supply chain consignment contained in this piece of associated transport equipment."
            ],
            "rdfs:label": "containedConsignment",
            "unece:cefactElementMetadata": [
                {
                    "@id": "cefact:Logistics_TransportEquipment.Contained.SupplyChain_Consignment",
                    "@type": "unece:AssociationBIE",
                    "unece:cefactUNId": "UN01003786",
                    "unece:cefactBieDomainClass": "cefact:Logistics_TransportEquipment.Details",
                    "rdfs:comment": "A consignment contained in this piece of logistics transport equipment."
                },
                {
                    "@id": "cefact:Associated_TransportEquipment.Contained.SupplyChain_Consignment",
                    "@type": "unece:AssociationBIE",
                    "unece:cefactUNId": "UN01013660",
                    "unece:cefactBieDomainClass": "cefact:Associated_TransportEquipment.Details",
                    "rdfs:comment": "A supply chain consignment contained in this piece of associated transport equipment."
                }
            ]
        },
        {
            "@id": "transport:containedConsignmentQuantity",
            "@type": "rdf:Property",
            "schema:rangeIncludes": {
                "@id": "xsd:decimal"
            },
            "schema:domainIncludes": {
                "@id": "transport:LogisticsTransportEquipment"
            },
            "rdfs:comment": "The number of consignments contained in this piece of logistics transport equipment.",
            "rdfs:label": "containedConsignmentQuantity",
            "unece:cefactElementMetadata": [
                {
                    "@id": "cefact:Logistics_TransportEquipment.ContainedConsignment.Quantity",
                    "@type": "unece:BasicBIE",
                    "unece:cefactUNId": "UN01008983",
                    "unece:cefactBieDomainClass": "cefact:Logistics_TransportEquipment.Details",
                    "rdfs:comment": "The number of consignments contained in this piece of logistics transport equipment."
                }
            ]
        },
        {
            "@id": "transport:containedPackage",
            "@type": "rdf:Property",
            "schema:rangeIncludes": {
                "@id": "transport:Package"
            },
            "schema:domainIncludes": {
                "@id": "transport:LogisticsPackaging"
            },
            "rdfs:comment": "A package contained in this logistics packaging.",
            "rdfs:label": "containedPackage",
            "unece:cefactElementMetadata": [
                {
                    "@id": "cefact:Logistics_Packaging.Contained.Logistics_Package",
                    "@type": "unece:AssociationBIE",
                    "unece:cefactUNId": "UN01014966",
                    "unece:cefactBieDomainClass": "cefact:Logistics_Packaging.Details",
                    "rdfs:comment": "A package contained in this logistics packaging."
                }
            ]
        },
        {
            "@id": "transport:containedTransportEquipment",
            "@type": "rdf:Property",
            "schema:rangeIncludes": {
                "@id": "transport:TransportEquipment"
            },
            "schema:domainIncludes": {
                "@id": "transport:LogisticsTransportEquipment"
            },
            "rdfs:comment": "A piece of transport equipment contained within this piece of logistics transport equipment, such as a pallet.",
            "rdfs:label": "containedTransportEquipment",
            "unece:cefactElementMetadata": [
                {
                    "@id": "cefact:Logistics_TransportEquipment.Contained.Associated_TransportEquipment",
                    "@type": "unece:AssociationBIE",
                    "unece:cefactUNId": "UN01003799",
                    "unece:cefactBieDomainClass": "cefact:Logistics_TransportEquipment.Details",
                    "rdfs:comment": "A piece of transport equipment contained within this piece of logistics transport equipment, such as a pallet."
                }
            ]
        },
        {
            "@id": "transport:containerizationIndicator",
            "@type": "rdf:Property",
            "schema:rangeIncludes": {
                "@id": "xsd:boolean"
            },
            "schema:domainIncludes": {
                "@id": "transport:SupplyChainConsignment"
            },
            "rdfs:comment": "The indication of whether or not this supply chain consignment is to be transported in a container or containers.",
            "rdfs:label": "containerizationIndicator",
            "unece:cefactElementMetadata": [
                {
                    "@id": "cefact:SupplyChain_Consignment.Containerization.Indicator",
                    "@type": "unece:BasicBIE",
                    "unece:TDED": "4140",
                    "unece:cefactUNId": "UN01004195",
                    "unece:cefactBieDomainClass": "cefact:SupplyChain_Consignment.Details",
                    "rdfs:comment": "The indication of whether or not this supply chain consignment is to be transported in a container or containers."
                }
            ]
        },
        {
            "@id": "transport:contentLayerQuantity",
            "@type": "rdf:Property",
            "schema:rangeIncludes": {
                "@id": "xsd:decimal"
            },
            "schema:domainIncludes": {
                "@id": "transport:LogisticsPackaging"
            },
            "rdfs:comment": "A number of content layers in this logistics packaging.",
            "rdfs:label": "contentLayerQuantity",
            "unece:cefactElementMetadata": [
                {
                    "@id": "cefact:Logistics_Packaging.ContentLayer.Quantity",
                    "@type": "unece:BasicBIE",
                    "unece:cefactUNId": "UN01014961",
                    "unece:cefactBieDomainClass": "cefact:Logistics_Packaging.Details",
                    "rdfs:comment": "A number of content layers in this logistics packaging."
                }
            ]
        },
        {
            "@id": "transport:contractId",
            "@type": "rdf:Property",
            "schema:rangeIncludes": {
                "@id": "xsd:token"
            },
            "schema:domainIncludes": {
                "@id": "transport:SupplyChainConsignment"
            },
            "rdfs:comment": "A contract identifier for this supply chain consignment.",
            "rdfs:label": "contractId",
            "unece:cefactElementMetadata": [
                {
                    "@id": "cefact:SupplyChain_Consignment.Contract.Identifier",
                    "@type": "unece:BasicBIE",
                    "unece:TDED": "1296",
                    "unece:cefactUNId": "UN01015088",
                    "unece:cefactBieDomainClass": "cefact:SupplyChain_Consignment.Details",
                    "rdfs:comment": "A contract identifier for this supply chain consignment."
                }
            ]
        },
        {
            "@id": "transport:contractTermsInformation",
            "@type": "rdf:Property",
            "schema:rangeIncludes": {
                "@id": "xsd:string"
            },
            "schema:domainIncludes": {
                "@id": "transport:SupplyChainConsignment"
            },
            "rdfs:comment": "Information related to contract terms and conditions, expressed as text, for this supply chain consignment.",
            "rdfs:label": "contractTermsInformation",
            "unece:cefactElementMetadata": [
                {
                    "@id": "cefact:SupplyChain_Consignment.ContractTerms_Information.Text",
                    "@type": "unece:BasicBIE",
                    "unece:TDED": "4070",
                    "unece:cefactUNId": "UN01015090",
                    "unece:cefactBieDomainClass": "cefact:SupplyChain_Consignment.Details",
                    "rdfs:comment": "Information related to contract terms and conditions, expressed as text, for this supply chain consignment."
                }
            ]
        },
        {
            "@id": "transport:crewListRelatedDocument",
            "@type": "rdf:Property",
            "schema:rangeIncludes": {
                "@id": "transport:Document"
            },
            "schema:domainIncludes": {
                "@id": "transport:LogisticsTransportMovement"
            },
            "rdfs:comment": "The crew list document related to this logistics transport movement.",
            "rdfs:label": "crewListRelatedDocument",
            "unece:cefactElementMetadata": [
                {
                    "@id": "cefact:Logistics_TransportMovement.CrewList_Related.Referenced_Document",
                    "@type": "unece:AssociationBIE",
                    "unece:cefactUNId": "UN01010135",
                    "unece:cefactBieDomainClass": "cefact:Logistics_TransportMovement.Details",
                    "rdfs:comment": "The crew list document related to this logistics transport movement."
                }
            ]
        },
        {
            "@id": "transport:crewNationalityCountry",
            "@type": "rdf:Property",
            "schema:rangeIncludes": {
                "@id": "transport:Country"
            },
            "schema:domainIncludes": {
                "@id": "transport:LogisticsTransportMovement"
            },
            "rdfs:comment": "Crew nationality details for this logistics transport movement.",
            "rdfs:label": "crewNationalityCountry",
            "unece:cefactElementMetadata": [
                {
                    "@id": "cefact:Logistics_TransportMovement.CrewNationality.Trade_Country",
                    "@type": "unece:AssociationBIE",
                    "unece:cefactUNId": "UN01010127",
                    "unece:cefactBieDomainClass": "cefact:Logistics_TransportMovement.Details",
                    "rdfs:comment": "Crew nationality details for this logistics transport movement."
                }
            ]
        },
        {
            "@id": "transport:crewPerson",
            "@type": "rdf:Property",
            "schema:rangeIncludes": {
                "@id": "transport:Person"
            },
            "schema:domainIncludes": {
                "@id": "transport:LogisticsTransportMovement"
            },
            "rdfs:comment": "A person who is a member of the crew of the means of transport used for this logistics transport movement.",
            "rdfs:label": "crewPerson",
            "unece:cefactElementMetadata": [
                {
                    "@id": "cefact:Logistics_TransportMovement.Crew.Transport_Person",
                    "@type": "unece:AssociationBIE",
                    "unece:cefactUNId": "UN01003855",
                    "unece:cefactBieDomainClass": "cefact:Logistics_TransportMovement.Details",
                    "rdfs:comment": "A person who is a member of the crew of the means of transport used for this logistics transport movement."
                }
            ]
        },
        {
            "@id": "transport:crewPersonalEffects",
            "@type": "rdf:Property",
            "schema:rangeIncludes": {
                "@id": "transport:PersonalEffects"
            },
            "schema:domainIncludes": {
                "@id": "transport:LogisticsTransportMovement"
            },
            "rdfs:comment": "Personal effects of an individual member of the crew for this logistics transport movement.",
            "rdfs:label": "crewPersonalEffects",
            "unece:cefactElementMetadata": [
                {
                    "@id": "cefact:Logistics_TransportMovement.Crew.Specified_PersonalEffects",
                    "@type": "unece:AssociationBIE",
                    "unece:cefactUNId": "UN01013175",
                    "unece:cefactBieDomainClass": "cefact:Logistics_TransportMovement.Details",
                    "rdfs:comment": "Personal effects of an individual member of the crew for this logistics transport movement."
                }
            ]
        },
        {
            "@id": "transport:crewQuantity",
            "@type": "rdf:Property",
            "schema:rangeIncludes": {
                "@id": "xsd:decimal"
            },
            "schema:domainIncludes": {
                "@id": "transport:LogisticsTransportMovement"
            },
            "rdfs:comment": "The number of crew members for this logistics transport movement.",
            "rdfs:label": "crewQuantity",
            "unece:cefactElementMetadata": [
                {
                    "@id": "cefact:Logistics_TransportMovement.Crew.Quantity",
                    "@type": "unece:BasicBIE",
                    "unece:TDED": "6106",
                    "unece:cefactUNId": "UN01003850",
                    "unece:cefactBieDomainClass": "cefact:Logistics_TransportMovement.Details",
                    "rdfs:comment": "The number of crew members for this logistics transport movement."
                }
            ]
        },
        {
            "@id": "transport:currencyServiceChargeCurrencyCode",
            "@type": "rdf:Property",
            "schema:rangeIncludes": {
                "@id": "unece:UNECECL6343Code"
            },
            "schema:domainIncludes": {
                "@id": "transport:SupplyChainConsignment"
            },
            "rdfs:comment": "A code specifying a service charge currency for this supply chain consignment.",
            "rdfs:label": "currencyServiceChargeCurrencyCode",
            "unece:cefactElementMetadata": [
                {
                    "@id": "cefact:SupplyChain_Consignment.ServiceChargeCurrency.Code",
                    "@type": "unece:BasicBIE",
                    "unece:TDED": "6343",
                    "unece:cefactUNId": "UN01015091",
                    "unece:cefactBieDomainClass": "cefact:SupplyChain_Consignment.Details",
                    "rdfs:comment": "A code specifying a service charge currency for this supply chain consignment."
                }
            ]
        },
        {
            "@id": "transport:customerFacingTotalUnitQuantity",
            "@type": "rdf:Property",
            "schema:rangeIncludes": {
                "@id": "xsd:decimal"
            },
            "schema:domainIncludes": [
                {
                    "@id": "transport:SupplyChainPackaging"
                },
                {
                    "@id": "transport:TradeProduct_SupplyChainPackaging"
                }
            ],
            "rdfs:comment": [
                "The total number of units of this supply chain packaging facing the customer, such as would be seen when this packaging is placed on a retail shelf.",
                "The total number of units of this trade product supply chain packaging facing the customer, such as would be seen when this packaging is placed on a retail shelf."
            ],
            "rdfs:label": "customerFacingTotalUnitQuantity",
            "unece:cefactElementMetadata": [
                {
                    "@id": "cefact:SupplyChain_Packaging.CustomerFacing_TotalUnit.Quantity",
                    "@type": "unece:BasicBIE",
                    "unece:cefactUNId": "UN01007194",
                    "unece:cefactBieDomainClass": "cefact:SupplyChain_Packaging.Details",
                    "rdfs:comment": "The total number of units of this supply chain packaging facing the customer, such as would be seen when this packaging is placed on a retail shelf."
                },
                {
                    "@id": "cefact:TradeProduct_SupplyChain_Packaging.CustomerFacing_TotalUnit.Quantity",
                    "@type": "unece:BasicBIE",
                    "unece:cefactUNId": "UN01007478",
                    "unece:cefactBieDomainClass": "cefact:TradeProduct_SupplyChain_Packaging.Details",
                    "rdfs:comment": "The total number of units of this trade product supply chain packaging facing the customer, such as would be seen when this packaging is placed on a retail shelf."
                }
            ]
        },
        {
            "@id": "transport:customsExportAgentParty",
            "@type": "rdf:Property",
            "schema:rangeIncludes": {
                "@id": "transport:Party"
            },
            "schema:domainIncludes": {
                "@id": "transport:SupplyChainConsignment"
            },
            "rdfs:comment": "The party acting as an agent for, or on behalf of, the consignor with respect to the customs export procedures for this supply chain consignment.",
            "rdfs:label": "customsExportAgentParty",
            "unece:cefactElementMetadata": [
                {
                    "@id": "cefact:SupplyChain_Consignment.CustomsExportAgent.Trade_Party",
                    "@type": "unece:AssociationBIE",
                    "unece:cefactUNId": "UN01004225",
                    "unece:cefactBieDomainClass": "cefact:SupplyChain_Consignment.Details",
                    "rdfs:comment": "The party acting as an agent for, or on behalf of, the consignor with respect to the customs export procedures for this supply chain consignment."
                }
            ]
        },
        {
            "@id": "transport:customsId",
            "@type": "rdf:Property",
            "schema:rangeIncludes": {
                "@id": "xsd:token"
            },
            "schema:domainIncludes": [
                {
                    "@id": "transport:Referenced_SupplyChainConsignment"
                },
                {
                    "@id": "transport:SupplyChainConsignment"
                }
            ],
            "rdfs:comment": [
                "A unique identifier, for customs purposes, for this consignment.",
                "The identifier, for customs purposes, for this referenced supply chain consignment."
            ],
            "rdfs:label": "customsId",
            "unece:cefactElementMetadata": [
                {
                    "@id": "cefact:SupplyChain_Consignment.Customs_Identification.Identifier",
                    "@type": "unece:BasicBIE",
                    "unece:TDED": "1202",
                    "unece:cefactUNId": "UN01004163",
                    "unece:cefactBieDomainClass": "cefact:SupplyChain_Consignment.Details",
                    "rdfs:comment": "A unique identifier, for customs purposes, for this consignment."
                },
                {
                    "@id": "cefact:Referenced_SupplyChain_Consignment.Customs_Identification.Identifier",
                    "@type": "unece:BasicBIE",
                    "unece:TDED": "1202",
                    "unece:cefactUNId": "UN01011053",
                    "unece:cefactBieDomainClass": "cefact:Referenced_SupplyChain_Consignment.Details",
                    "rdfs:comment": "The identifier, for customs purposes, for this referenced supply chain consignment."
                }
            ]
        },
        {
            "@id": "transport:customsImportAgentParty",
            "@type": "rdf:Property",
            "schema:rangeIncludes": {
                "@id": "transport:Party"
            },
            "schema:domainIncludes": {
                "@id": "transport:SupplyChainConsignment"
            },
            "rdfs:comment": "The party acting as an agent for, or on behalf of, the consignee with respect to the customs import procedures for this supply chain consignment.",
            "rdfs:label": "customsImportAgentParty",
            "unece:cefactElementMetadata": [
                {
                    "@id": "cefact:SupplyChain_Consignment.CustomsImportAgent.Trade_Party",
                    "@type": "unece:AssociationBIE",
                    "unece:cefactUNId": "UN01004224",
                    "unece:cefactBieDomainClass": "cefact:SupplyChain_Consignment.Details",
                    "rdfs:comment": "The party acting as an agent for, or on behalf of, the consignee with respect to the customs import procedures for this supply chain consignment."
                }
            ]
        },
        {
            "@id": "transport:customsRequiredInvoiceDocument",
            "@type": "rdf:Property",
            "schema:rangeIncludes": {
                "@id": "transport:Document"
            },
            "schema:domainIncludes": {
                "@id": "transport:SupplyChainConsignment"
            },
            "rdfs:comment": "A referenced invoice document required by customs for this supply chain consignment.",
            "rdfs:label": "customsRequiredInvoiceDocument",
            "unece:cefactElementMetadata": [
                {
                    "@id": "cefact:SupplyChain_Consignment.CustomsRequiredInvoice.Referenced_Document",
                    "@type": "unece:AssociationBIE",
                    "unece:cefactUNId": "UN01004244",
                    "unece:cefactBieDomainClass": "cefact:SupplyChain_Consignment.Details",
                    "rdfs:comment": "A referenced invoice document required by customs for this supply chain consignment."
                }
            ]
        },
        {
            "@id": "transport:customsTransitAgentParty",
            "@type": "rdf:Property",
            "schema:rangeIncludes": {
                "@id": "transport:Party"
            },
            "schema:domainIncludes": {
                "@id": "transport:SupplyChainConsignment"
            },
            "rdfs:comment": "The party acting as an agent for, or on behalf of, the consignor with respect to customs transit procedures for this supply chain consignment.",
            "rdfs:label": "customsTransitAgentParty",
            "unece:cefactElementMetadata": [
                {
                    "@id": "cefact:SupplyChain_Consignment.CustomsTransitAgent.Trade_Party",
                    "@type": "unece:AssociationBIE",
                    "unece:cefactUNId": "UN01004226",
                    "unece:cefactBieDomainClass": "cefact:SupplyChain_Consignment.Details",
                    "rdfs:comment": "The party acting as an agent for, or on behalf of, the consignor with respect to customs transit procedures for this supply chain consignment."
                }
            ]
        },
        {
            "@id": "transport:cycle",
            "@type": "rdf:Property",
            "schema:rangeIncludes": {
                "@id": "xsd:string"
            },
            "schema:domainIncludes": {
                "@id": "transport:LogisticsTransportMovement"
            },
            "rdfs:comment": "The cycle, as expressed as text, of this logistics transport movement, such as twice a day.",
            "rdfs:label": "cycle",
            "unece:cefactElementMetadata": [
                {
                    "@id": "cefact:Logistics_TransportMovement.Cycle.Text",
                    "@type": "unece:BasicBIE",
                    "unece:cefactUNId": "UN01012754",
                    "unece:cefactBieDomainClass": "cefact:Logistics_TransportMovement.Details",
                    "rdfs:comment": "The cycle, as expressed as text, of this logistics transport movement, such as twice a day."
                }
            ]
        },
        {
            "@id": "transport:damageEvent",
            "@type": "rdf:Property",
            "schema:rangeIncludes": {
                "@id": "transport:Event"
            },
            "schema:domainIncludes": {
                "@id": "transport:LogisticsTransportMovement"
            },
            "rdfs:comment": "A damage event for this logistics transport movement.",
            "rdfs:label": "damageEvent",
            "unece:cefactElementMetadata": [
                {
                    "@id": "cefact:Logistics_TransportMovement.Damage.Transport_Event",
                    "@type": "unece:AssociationBIE",
                    "unece:cefactUNId": "UN01014632",
                    "unece:cefactBieDomainClass": "cefact:Logistics_TransportMovement.Details",
                    "rdfs:comment": "A damage event for this logistics transport movement."
                }
            ]
        },
        {
            "@id": "transport:damageRemark",
            "@type": "rdf:Property",
            "schema:rangeIncludes": {
                "@id": "xsd:string"
            },
            "schema:domainIncludes": {
                "@id": "transport:LogisticsTransportEquipment"
            },
            "rdfs:comment": "A damage remark, expressed as text, for this piece of logistics transport equipment.",
            "rdfs:label": "damageRemark",
            "unece:cefactElementMetadata": [
                {
                    "@id": "cefact:Logistics_TransportEquipment.DamageRemark.Text",
                    "@type": "unece:BasicBIE",
                    "unece:cefactUNId": "UN01003777",
                    "unece:cefactBieDomainClass": "cefact:Logistics_TransportEquipment.Details",
                    "rdfs:comment": "A damage remark, expressed as text, for this piece of logistics transport equipment."
                }
            ]
        },
        {
            "@id": "transport:damageRemarks",
            "@type": "rdf:Property",
            "schema:rangeIncludes": {
                "@id": "xsd:string"
            },
            "schema:domainIncludes": {
                "@id": "transport:SupplyChainConsignmentItem"
            },
            "rdfs:comment": "Damage remarks, expressed as text, for this supply chain consignment item.",
            "rdfs:label": "damageRemarks",
            "unece:cefactElementMetadata": [
                {
                    "@id": "cefact:SupplyChain_ConsignmentItem.DamageRemarks.Text",
                    "@type": "unece:BasicBIE",
                    "unece:cefactUNId": "UN01004127",
                    "unece:cefactBieDomainClass": "cefact:SupplyChain_ConsignmentItem.Details",
                    "rdfs:comment": "Damage remarks, expressed as text, for this supply chain consignment item."
                }
            ]
        },
        {
            "@id": "transport:dangerousGoodsIndicator",
            "@type": "rdf:Property",
            "schema:rangeIncludes": {
                "@id": "xsd:boolean"
            },
            "schema:domainIncludes": {
                "@id": "transport:LogisticsTransportMovement"
            },
            "rdfs:comment": "The indication of whether or not dangerous goods are carried for this logistics transport movement.",
            "rdfs:label": "dangerousGoodsIndicator",
            "unece:cefactElementMetadata": [
                {
                    "@id": "cefact:Logistics_TransportMovement.DangerousGoods.Indicator",
                    "@type": "unece:BasicBIE",
                    "unece:cefactUNId": "UN01010121",
                    "unece:cefactBieDomainClass": "cefact:Logistics_TransportMovement.Details",
                    "rdfs:comment": "The indication of whether or not dangerous goods are carried for this logistics transport movement."
                }
            ]
        },
        {
            "@id": "transport:dangerousGoodsNotifierParty",
            "@type": "rdf:Property",
            "schema:rangeIncludes": {
                "@id": "transport:Party"
            },
            "schema:domainIncludes": {
                "@id": "transport:SupplyChainConsignment"
            },
            "rdfs:comment": "The party responsible for providing the dangerous goods notification in accordance with the dangerous goods regulations relevant for this supply chain consignment.",
            "rdfs:label": "dangerousGoodsNotifierParty",
            "unece:cefactElementMetadata": [
                {
                    "@id": "cefact:SupplyChain_Consignment.DangerousGoodsNotifier.Trade_Party",
                    "@type": "unece:AssociationBIE",
                    "unece:cefactUNId": "UN01004228",
                    "unece:cefactBieDomainClass": "cefact:SupplyChain_Consignment.Details",
                    "rdfs:comment": "The party responsible for providing the dangerous goods notification in accordance with the dangerous goods regulations relevant for this supply chain consignment."
                }
            ]
        },
        {
            "@id": "transport:deadweightTonnageMeasure",
            "@type": "rdf:Property",
            "schema:rangeIncludes": {
                "@id": "xsd:decimal"
            },
            "schema:domainIncludes": {
                "@id": "transport:LogisticsTransportMeans"
            },
            "rdfs:comment": "The deadweight tonnage measure for this logistics transport means.",
            "rdfs:label": "deadweightTonnageMeasure",
            "unece:cefactElementMetadata": [
                {
                    "@id": "cefact:Logistics_TransportMeans.DeadweightTonnage.Measure",
                    "@type": "unece:BasicBIE",
                    "unece:cefactUNId": "UN01015082",
                    "unece:cefactBieDomainClass": "cefact:Logistics_TransportMeans.Details",
                    "rdfs:comment": "The deadweight tonnage measure for this logistics transport means."
                }
            ]
        },
        {
            "@id": "transport:declarationCountryRelationshipCode",
            "@type": "rdf:Property",
            "schema:rangeIncludes": {
                "@id": "xsd:token"
            },
            "schema:domainIncludes": {
                "@id": ":TradeDeliveryTerms"
            },
            "rdfs:comment": "The code specifying whether the place specified by these trade delivery terms is located in the country where a declaration is made, in another member country of the same economic or customs union, or in a third country.",
            "rdfs:label": "declarationCountryRelationshipCode",
            "unece:cefactElementMetadata": [
                {
                    "@id": "cefact:Trade_DeliveryTerms.DeclarationCountryRelationship.Code",
                    "@type": "unece:BasicBIE",
                    "unece:TDED": "4443",
                    "unece:cefactUNId": "UN01004585",
                    "unece:cefactBieDomainClass": "cefact:Trade_DeliveryTerms.Details",
                    "rdfs:comment": "The code specifying whether the place specified by these trade delivery terms is located in the country where a declaration is made, in another member country of the same economic or customs union, or in a third country."
                }
            ]
        },
        {
            "@id": "transport:declaredForCustomsLocation",
            "@type": "rdf:Property",
            "schema:rangeIncludes": {
                "@id": "transport:Location"
            },
            "schema:domainIncludes": [
                {
                    "@id": "transport:SupplyChainConsignment"
                },
                {
                    "@id": "transport:SupplyChainConsignmentItem"
                }
            ],
            "rdfs:comment": [
                "The location of this supply chain consignment as declared for customs.",
                "The location of this supply chain consignment item as declared for customs."
            ],
            "rdfs:label": "declaredForCustomsLocation",
            "unece:cefactElementMetadata": [
                {
                    "@id": "cefact:SupplyChain_Consignment.DeclaredForCustoms.Logistics_Location",
                    "@type": "unece:AssociationBIE",
                    "unece:cefactUNId": "UN01004241",
                    "unece:cefactBieDomainClass": "cefact:SupplyChain_Consignment.Details",
                    "rdfs:comment": "The location of this supply chain consignment as declared for customs."
                },
                {
                    "@id": "cefact:SupplyChain_ConsignmentItem.DeclaredForCustoms.Logistics_Location",
                    "@type": "unece:AssociationBIE",
                    "unece:cefactUNId": "UN01004144",
                    "unece:cefactBieDomainClass": "cefact:SupplyChain_ConsignmentItem.Details",
                    "rdfs:comment": "The location of this supply chain consignment item as declared for customs."
                }
            ]
        },
        {
            "@id": "transport:declaredValueForCarriageAmount",
            "@type": "rdf:Property",
            "schema:rangeIncludes": {
                "@id": "xsd:decimal"
            },
            "schema:domainIncludes": [
                {
                    "@id": "transport:SupplyChainConsignment"
                },
                {
                    "@id": "transport:SupplyChainConsignmentItem"
                }
            ],
            "rdfs:comment": [
                "The monetary value of this supply chain consignment as declared by the shipper or his agent for the purpose of varying the carrier's level of liability from that provided in the contract of carriage, in case of loss or damage to goods or delayed delivery.",
                "The monetary value of this supply chain consignment item as declared by the shipper or his agent for the purpose of varying the carrier's level of liability from that provided in the contract of carriage, in case of loss or damage to goods or delayed delivery."
            ],
            "rdfs:label": "declaredValueForCarriageAmount",
            "unece:cefactElementMetadata": [
                {
                    "@id": "cefact:SupplyChain_Consignment.DeclaredValueForCarriage.Amount",
                    "@type": "unece:BasicBIE",
                    "unece:TDED": "5036",
                    "unece:cefactUNId": "UN01006138",
                    "unece:cefactBieDomainClass": "cefact:SupplyChain_Consignment.Details",
                    "rdfs:comment": "The monetary value of this supply chain consignment as declared by the shipper or his agent for the purpose of varying the carrier's level of liability from that provided in the contract of carriage, in case of loss or damage to goods or delayed delivery."
                },
                {
                    "@id": "cefact:SupplyChain_ConsignmentItem.DeclaredValueForCarriage.Amount",
                    "@type": "unece:BasicBIE",
                    "unece:TDED": "5036",
                    "unece:cefactUNId": "UN01004114",
                    "unece:cefactBieDomainClass": "cefact:SupplyChain_ConsignmentItem.Details",
                    "rdfs:comment": "The monetary value of this supply chain consignment item as declared by the shipper or his agent for the purpose of varying the carrier's level of liability from that provided in the contract of carriage, in case of loss or damage to goods or delayed delivery."
                }
            ]
        },
        {
            "@id": "transport:declaredValueForCustomsAmount",
            "@type": "rdf:Property",
            "schema:rangeIncludes": {
                "@id": "xsd:decimal"
            },
            "schema:domainIncludes": [
                {
                    "@id": "transport:SupplyChainConsignment"
                },
                {
                    "@id": "transport:SupplyChainConsignmentItem"
                }
            ],
            "rdfs:comment": [
                "The monetary value declared for customs purposes for this supply chain consignment.",
                "The monetary value of this supply chain consignment item as declared for customs purposes."
            ],
            "rdfs:label": "declaredValueForCustomsAmount",
            "unece:cefactElementMetadata": [
                {
                    "@id": "cefact:SupplyChain_Consignment.DeclaredValueForCustoms.Amount",
                    "@type": "unece:BasicBIE",
                    "unece:TDED": "5032",
                    "unece:cefactUNId": "UN01004188",
                    "unece:cefactBieDomainClass": "cefact:SupplyChain_Consignment.Details",
                    "rdfs:comment": "The monetary value declared for customs purposes for this supply chain consignment."
                },
                {
                    "@id": "cefact:SupplyChain_ConsignmentItem.DeclaredValueForCustoms.Amount",
                    "@type": "unece:BasicBIE",
                    "unece:TDED": "5032",
                    "unece:cefactUNId": "UN01004113",
                    "unece:cefactBieDomainClass": "cefact:SupplyChain_ConsignmentItem.Details",
                    "rdfs:comment": "The monetary value of this supply chain consignment item as declared for customs purposes."
                }
            ]
        },
        {
            "@id": "transport:declaredValueForStatisticsAmount",
            "@type": "rdf:Property",
            "schema:rangeIncludes": {
                "@id": "xsd:decimal"
            },
            "schema:domainIncludes": {
                "@id": "transport:SupplyChainConsignmentItem"
            },
            "rdfs:comment": "The monetary value of this supply chain consignment item as declared for statistical purposes.",
            "rdfs:label": "declaredValueForStatisticsAmount",
            "unece:cefactElementMetadata": [
                {
                    "@id": "cefact:SupplyChain_ConsignmentItem.DeclaredValueForStatistics.Amount",
                    "@type": "unece:BasicBIE",
                    "unece:TDED": "5218",
                    "unece:cefactUNId": "UN01004115",
                    "unece:cefactBieDomainClass": "cefact:SupplyChain_ConsignmentItem.Details",
                    "rdfs:comment": "The monetary value of this supply chain consignment item as declared for statistical purposes."
                }
            ]
        },
        {
            "@id": "transport:deconsolidationEvent",
            "@type": "rdf:Property",
            "schema:rangeIncludes": {
                "@id": "transport:Event"
            },
            "schema:domainIncludes": {
                "@id": "transport:LogisticsTransportEquipment"
            },
            "rdfs:comment": "A deconsolidation event for this piece of logistics transport equipment.",
            "rdfs:label": "deconsolidationEvent",
            "unece:cefactElementMetadata": [
                {
                    "@id": "cefact:Logistics_TransportEquipment.Deconsolidation.Transport_Event",
                    "@type": "unece:AssociationBIE",
                    "unece:cefactUNId": "UN01015081",
                    "unece:cefactBieDomainClass": "cefact:Logistics_TransportEquipment.Details",
                    "rdfs:comment": "A deconsolidation event for this piece of logistics transport equipment."
                }
            ]
        },
        {
            "@id": "transport:deconsolidatorParty",
            "@type": "rdf:Property",
            "schema:rangeIncludes": {
                "@id": "transport:Party"
            },
            "schema:domainIncludes": {
                "@id": "transport:SupplyChainConsignment"
            },
            "rdfs:comment": "The party responsible for the deconsolidation of this supply chain consignment.",
            "rdfs:label": "deconsolidatorParty",
            "unece:cefactElementMetadata": [
                {
                    "@id": "cefact:SupplyChain_Consignment.Deconsolidator.Trade_Party",
                    "@type": "unece:AssociationBIE",
                    "unece:cefactUNId": "UN01004231",
                    "unece:cefactBieDomainClass": "cefact:SupplyChain_Consignment.Details",
                    "rdfs:comment": "The party responsible for the deconsolidation of this supply chain consignment."
                }
            ]
        },
        {
            "@id": "transport:deliveryDiscontinuationCode",
            "@type": "rdf:Property",
            "schema:rangeIncludes": {
                "@id": "xsd:token"
            },
            "schema:domainIncludes": {
                "@id": ":TradeDeliveryTerms"
            },
            "rdfs:comment": "The code specifying the delivery discontinuation for this trade delivery terms.",
            "rdfs:label": "deliveryDiscontinuationCode",
            "unece:cefactElementMetadata": [
                {
                    "@id": "cefact:Trade_DeliveryTerms.DeliveryDiscontinuation.Code",
                    "@type": "unece:BasicBIE",
                    "unece:cefactUNId": "UN01012762",
                    "unece:cefactBieDomainClass": "cefact:Trade_DeliveryTerms.Details",
                    "rdfs:comment": "The code specifying the delivery discontinuation for this trade delivery terms."
                }
            ]
        },
        {
            "@id": "transport:deliveryEvent",
            "@type": "rdf:Property",
            "schema:rangeIncludes": {
                "@id": "transport:Event"
            },
            "schema:domainIncludes": [
                {
                    "@id": "transport:LogisticsTransportEquipment"
                },
                {
                    "@id": "transport:SupplyChainConsignment"
                },
                {
                    "@id": "transport:SupplyChainConsignmentItem"
                }
            ],
            "rdfs:comment": [
                "A delivery event for this piece of logistics transport equipment.",
                "The delivery event for this supply chain consignment item.",
                "The delivery event for this supply chain consignment."
            ],
            "rdfs:label": "deliveryEvent",
            "unece:cefactElementMetadata": [
                {
                    "@id": "cefact:SupplyChain_ConsignmentItem.Delivery.Transport_Event",
                    "@type": "unece:AssociationBIE",
                    "unece:cefactUNId": "UN01004156",
                    "unece:cefactBieDomainClass": "cefact:SupplyChain_ConsignmentItem.Details",
                    "rdfs:comment": "The delivery event for this supply chain consignment item."
                },
                {
                    "@id": "cefact:Logistics_TransportEquipment.Delivery.Transport_Event",
                    "@type": "unece:AssociationBIE",
                    "unece:cefactUNId": "UN01010100",
                    "unece:cefactBieDomainClass": "cefact:Logistics_TransportEquipment.Details",
                    "rdfs:comment": "A delivery event for this piece of logistics transport equipment."
                },
                {
                    "@id": "cefact:SupplyChain_Consignment.Delivery.Transport_Event",
                    "@type": "unece:AssociationBIE",
                    "unece:cefactUNId": "UN01004251",
                    "unece:cefactBieDomainClass": "cefact:SupplyChain_Consignment.Details",
                    "rdfs:comment": "The delivery event for this supply chain consignment."
                }
            ]
        },
        {
            "@id": "transport:deliveryInstructions",
            "@type": "rdf:Property",
            "schema:rangeIncludes": {
                "@id": "transport:Instructions"
            },
            "schema:domainIncludes": {
                "@id": "transport:LogisticsTransportEquipment"
            },
            "rdfs:comment": "Delivery instructions for this piece of logistics transport equipment.",
            "rdfs:label": "deliveryInstructions",
            "unece:cefactElementMetadata": [
                {
                    "@id": "cefact:Logistics_TransportEquipment.Delivery.Delivery_Instructions",
                    "@type": "unece:AssociationBIE",
                    "unece:cefactUNId": "UN01003790",
                    "unece:cefactBieDomainClass": "cefact:Logistics_TransportEquipment.Details",
                    "rdfs:comment": "Delivery instructions for this piece of logistics transport equipment."
                }
            ]
        },
        {
            "@id": "transport:deliveryInstructionsText",
            "@type": "rdf:Property",
            "schema:rangeIncludes": {
                "@id": "xsd:string"
            },
            "schema:domainIncludes": {
                "@id": "transport:SupplyChainConsignmentItem"
            },
            "rdfs:comment": "Delivery instructions, expressed as text, for this supply chain consignment item.",
            "rdfs:label": "deliveryInstructionsText",
            "unece:cefactElementMetadata": [
                {
                    "@id": "cefact:SupplyChain_ConsignmentItem.DeliveryInstructions.Text",
                    "@type": "unece:BasicBIE",
                    "unece:cefactUNId": "UN01004126",
                    "unece:cefactBieDomainClass": "cefact:SupplyChain_ConsignmentItem.Details",
                    "rdfs:comment": "Delivery instructions, expressed as text, for this supply chain consignment item."
                }
            ]
        },
        {
            "@id": "transport:deliveryParty",
            "@type": "rdf:Property",
            "schema:rangeIncludes": {
                "@id": "transport:Party"
            },
            "schema:domainIncludes": [
                {
                    "@id": "transport:Referenced_SupplyChainConsignment"
                },
                {
                    "@id": "transport:SupplyChainConsignment"
                },
                {
                    "@id": "transport:SupplyChainConsignmentItem"
                }
            ],
            "rdfs:comment": [
                "The party to whom this referenced supply chain consignment will be or has been delivered.",
                "The party to whom this supply chain consignment item will be or has been delivered.",
                "The party to whom this supply chain consignment will be, or has been, delivered."
            ],
            "rdfs:label": "deliveryParty",
            "unece:cefactElementMetadata": [
                {
                    "@id": "cefact:SupplyChain_Consignment.Delivery.Trade_Party",
                    "@type": "unece:AssociationBIE",
                    "unece:cefactUNId": "UN01004220",
                    "unece:cefactBieDomainClass": "cefact:SupplyChain_Consignment.Details",
                    "rdfs:comment": "The party to whom this supply chain consignment will be, or has been, delivered."
                },
                {
                    "@id": "cefact:SupplyChain_ConsignmentItem.Delivery.Trade_Party",
                    "@type": "unece:AssociationBIE",
                    "unece:cefactUNId": "UN01004148",
                    "unece:cefactBieDomainClass": "cefact:SupplyChain_ConsignmentItem.Details",
                    "rdfs:comment": "The party to whom this supply chain consignment item will be or has been delivered."
                },
                {
                    "@id": "cefact:Referenced_SupplyChain_Consignment.Delivery.Trade_Party",
                    "@type": "unece:AssociationBIE",
                    "unece:cefactUNId": "UN01011057",
                    "unece:cefactBieDomainClass": "cefact:Referenced_SupplyChain_Consignment.Details",
                    "rdfs:comment": "The party to whom this referenced supply chain consignment will be or has been delivered."
                }
            ]
        },
        {
            "@id": "transport:deliveryTermsFunctionCode",
            "@type": "rdf:Property",
            "schema:rangeIncludes": {
                "@id": "unece:UNECECL4055Code"
            },
            "schema:domainIncludes": {
                "@id": ":TradeDeliveryTerms"
            },
            "rdfs:comment": "A code specifying a function of these trade delivery terms.",
            "rdfs:label": "deliveryTermsFunctionCode",
            "unece:cefactElementMetadata": [
                {
                    "@id": "cefact:Trade_DeliveryTerms.Function.Code",
                    "@type": "unece:BasicBIE",
                    "unece:TDED": "4055",
                    "unece:cefactUNId": "UN01009006",
                    "unece:cefactBieDomainClass": "cefact:Trade_DeliveryTerms.Details",
                    "rdfs:comment": "A code specifying a function of these trade delivery terms."
                }
            ]
        },
        {
            "@id": "transport:demurrageInformation",
            "@type": "rdf:Property",
            "schema:rangeIncludes": {
                "@id": "xsd:string"
            },
            "schema:domainIncludes": {
                "@id": "transport:SupplyChainConsignment"
            },
            "rdfs:comment": "Demurrage information, expressed as text, for this supply chain consignment.",
            "rdfs:label": "demurrageInformation",
            "unece:cefactElementMetadata": [
                {
                    "@id": "cefact:SupplyChain_Consignment.Demurrage_Information.Text",
                    "@type": "unece:BasicBIE",
                    "unece:TDED": "4070",
                    "unece:cefactUNId": "UN01004208",
                    "unece:cefactBieDomainClass": "cefact:SupplyChain_Consignment.Details",
                    "rdfs:comment": "Demurrage information, expressed as text, for this supply chain consignment."
                }
            ]
        },
        {
            "@id": "transport:departureEvent",
            "@type": "rdf:Property",
            "schema:rangeIncludes": {
                "@id": "transport:Event"
            },
            "schema:domainIncludes": {
                "@id": "transport:LogisticsTransportMovement"
            },
            "rdfs:comment": "A departure event during this logistics transport movement.",
            "rdfs:label": "departureEvent",
            "unece:cefactElementMetadata": [
                {
                    "@id": "cefact:Logistics_TransportMovement.Departure.Transport_Event",
                    "@type": "unece:AssociationBIE",
                    "unece:cefactUNId": "UN01003860",
                    "unece:cefactBieDomainClass": "cefact:Logistics_TransportMovement.Details",
                    "rdfs:comment": "A departure event during this logistics transport movement."
                }
            ]
        },
        {
            "@id": "transport:departureReportedEvent",
            "@type": "rdf:Property",
            "schema:rangeIncludes": {
                "@id": "transport:Event"
            },
            "schema:domainIncludes": {
                "@id": "trade:LogisticsStatus"
            },
            "rdfs:comment": "A transport departure event reported for this logistics status.",
            "rdfs:label": "departureReportedEvent",
            "unece:cefactElementMetadata": [
                {
                    "@id": "cefact:Logistics_Status.Departure_Reported.Transport_Event",
                    "@type": "unece:AssociationBIE",
                    "unece:cefactUNId": "UN01010094",
                    "unece:cefactBieDomainClass": "cefact:Logistics_Status.Details",
                    "rdfs:comment": "A transport departure event reported for this logistics status."
                }
            ]
        },
        {
            "@id": "transport:description",
            "@type": "rdf:Property",
            "schema:rangeIncludes": {
                "@id": "xsd:string"
            },
            "schema:domainIncludes": [
                {
                    "@id": "transport:IdentifiedFault"
                },
                {
                    "@id": "transport:LogisticsPackaging"
                },
                {
                    "@id": "transport:SupplyChainPackaging"
                },
                {
                    "@id": "transport:TransportationWasteRecoveryDisposalProcess"
                }
            ],
            "rdfs:comment": [
                "A textual description for the type of transportation waste recovery disposal process.",
                "A textual description of this identified fault.",
                "A textual description of this logistics packaging.",
                "A textual description of this supply chain packaging."
            ],
            "rdfs:label": "description",
            "unece:cefactElementMetadata": [
                {
                    "@id": "cefact:Identified_Fault.Description.Text",
                    "@type": "unece:BasicBIE",
                    "unece:cefactUNId": "UN01010066",
                    "unece:cefactBieDomainClass": "cefact:Identified_Fault.Details",
                    "rdfs:comment": "A textual description of this identified fault."
                },
                {
                    "@id": "cefact:Logistics_Packaging.Description.Text",
                    "@type": "unece:BasicBIE",
                    "unece:cefactUNId": "UN01014951",
                    "unece:cefactBieDomainClass": "cefact:Logistics_Packaging.Details",
                    "rdfs:comment": "A textual description of this logistics packaging."
                },
                {
                    "@id": "cefact:TransportationWasteRecoveryDisposal_Process.Description.Text",
                    "@type": "unece:BasicBIE",
                    "unece:TDED": "7190",
                    "unece:cefactUNId": "UN01014618",
                    "unece:cefactBieDomainClass": "cefact:TransportationWasteRecoveryDisposal_Process.Details",
                    "rdfs:comment": "A textual description for the type of transportation waste recovery disposal process."
                },
                {
                    "@id": "cefact:SupplyChain_Packaging.Description.Text",
                    "@type": "unece:BasicBIE",
                    "unece:cefactUNId": "UN01004315",
                    "unece:cefactBieDomainClass": "cefact:SupplyChain_Packaging.Details",
                    "rdfs:comment": "A textual description of this supply chain packaging."
                }
            ]
        },
        {
            "@id": "transport:despatchParty",
            "@type": "rdf:Property",
            "schema:rangeIncludes": {
                "@id": "transport:Party"
            },
            "schema:domainIncludes": [
                {
                    "@id": "transport:Referenced_SupplyChainConsignment"
                },
                {
                    "@id": "transport:SupplyChainConsignment"
                },
                {
                    "@id": "transport:SupplyChainConsignmentItem"
                }
            ],
            "rdfs:comment": [
                "The party from whom this referenced supply chain consignment will be or has been despatched.",
                "The party from whom this supply chain consignment item will be or has been despatched.",
                "The party from whom this supply chain consignment will be or has been despatched."
            ],
            "rdfs:label": "despatchParty",
            "unece:cefactElementMetadata": [
                {
                    "@id": "cefact:SupplyChain_ConsignmentItem.Despatch.Trade_Party",
                    "@type": "unece:AssociationBIE",
                    "unece:cefactUNId": "UN01004147",
                    "unece:cefactBieDomainClass": "cefact:SupplyChain_ConsignmentItem.Details",
                    "rdfs:comment": "The party from whom this supply chain consignment item will be or has been despatched."
                },
                {
                    "@id": "cefact:Referenced_SupplyChain_Consignment.Despatch.Trade_Party",
                    "@type": "unece:AssociationBIE",
                    "unece:cefactUNId": "UN01011056",
                    "unece:cefactBieDomainClass": "cefact:Referenced_SupplyChain_Consignment.Details",
                    "rdfs:comment": "The party from whom this referenced supply chain consignment will be or has been despatched."
                },
                {
                    "@id": "cefact:SupplyChain_Consignment.Despatch.Trade_Party",
                    "@type": "unece:AssociationBIE",
                    "unece:cefactUNId": "UN01004219",
                    "unece:cefactBieDomainClass": "cefact:SupplyChain_Consignment.Details",
                    "rdfs:comment": "The party from whom this supply chain consignment will be or has been despatched."
                }
            ]
        },
        {
            "@id": "transport:destinationCountry",
            "@type": "rdf:Property",
            "schema:rangeIncludes": {
                "@id": "transport:Country"
            },
            "schema:domainIncludes": [
                {
                    "@id": "transport:SupplyChainConsignment"
                },
                {
                    "@id": "transport:SupplyChainConsignmentItem"
                }
            ],
            "rdfs:comment": [
                "The destination country for this supply chain consignment item.",
                "The destination country for this supply chain consignment."
            ],
            "rdfs:label": "destinationCountry",
            "unece:cefactElementMetadata": [
                {
                    "@id": "cefact:SupplyChain_Consignment.Destination.Trade_Country",
                    "@type": "unece:AssociationBIE",
                    "unece:cefactUNId": "UN01004270",
                    "unece:cefactBieDomainClass": "cefact:SupplyChain_Consignment.Details",
                    "rdfs:comment": "The destination country for this supply chain consignment."
                },
                {
                    "@id": "cefact:SupplyChain_ConsignmentItem.Destination.Trade_Country",
                    "@type": "unece:AssociationBIE",
                    "unece:cefactUNId": "UN01004141",
                    "unece:cefactBieDomainClass": "cefact:SupplyChain_ConsignmentItem.Details",
                    "rdfs:comment": "The destination country for this supply chain consignment item."
                }
            ]
        },
        {
            "@id": "transport:devanningEvent",
            "@type": "rdf:Property",
            "schema:rangeIncludes": {
                "@id": "transport:Event"
            },
            "schema:domainIncludes": [
                {
                    "@id": "transport:Referenced_SupplyChainConsignment"
                },
                {
                    "@id": "transport:SupplyChainConsignment"
                }
            ],
            "rdfs:comment": [
                "A transport devanning event for this referenced supply chain consignment, i.e. the unloading of this consignment at the place of delivery.",
                "A transport devanning event for this supply chain consignment, i.e. the unloading of this consignment at the place of delivery."
            ],
            "rdfs:label": "devanningEvent",
            "unece:cefactElementMetadata": [
                {
                    "@id": "cefact:SupplyChain_Consignment.Devanning.Transport_Event",
                    "@type": "unece:AssociationBIE",
                    "unece:cefactUNId": "UN01013195",
                    "unece:cefactBieDomainClass": "cefact:SupplyChain_Consignment.Details",
                    "rdfs:comment": "A transport devanning event for this supply chain consignment, i.e. the unloading of this consignment at the place of delivery."
                },
                {
                    "@id": "cefact:Referenced_SupplyChain_Consignment.Devanning.Transport_Event",
                    "@type": "unece:AssociationBIE",
                    "unece:cefactUNId": "UN01013183",
                    "unece:cefactBieDomainClass": "cefact:Referenced_SupplyChain_Consignment.Details",
                    "rdfs:comment": "A transport devanning event for this referenced supply chain consignment, i.e. the unloading of this consignment at the place of delivery."
                }
            ]
        },
        {
            "@id": "transport:disposalMethodCode",
            "@type": "rdf:Property",
            "schema:rangeIncludes": {
                "@id": "xsd:token"
            },
            "schema:domainIncludes": [
                {
                    "@id": "transport:LogisticsPackaging"
                },
                {
                    "@id": "transport:SupplyChainPackaging"
                }
            ],
            "rdfs:comment": [
                "A code specifying a disposal method for this logistics packaging.",
                "A code specifying the disposal method of this supply chain packaging."
            ],
            "rdfs:label": "disposalMethodCode",
            "unece:cefactElementMetadata": [
                {
                    "@id": "cefact:Logistics_Packaging.DisposalMethod.Code",
                    "@type": "unece:BasicBIE",
                    "unece:cefactUNId": "UN01014954",
                    "unece:cefactBieDomainClass": "cefact:Logistics_Packaging.Details",
                    "rdfs:comment": "A code specifying a disposal method for this logistics packaging."
                },
                {
                    "@id": "cefact:SupplyChain_Packaging.DisposalMethod.Code",
                    "@type": "unece:BasicBIE",
                    "unece:cefactUNId": "UN01004317",
                    "unece:cefactBieDomainClass": "cefact:SupplyChain_Packaging.Details",
                    "rdfs:comment": "A code specifying the disposal method of this supply chain packaging."
                }
            ]
        },
        {
            "@id": "transport:documentaryInstructionsNotifiedParty",
            "@type": "rdf:Property",
            "schema:rangeIncludes": {
                "@id": "transport:Party"
            },
            "schema:domainIncludes": {
                "@id": "transport:LogisticsTransportMovement"
            },
            "rdfs:comment": "A party to be notified of the documentary instructions for this logistics transport movement.",
            "rdfs:label": "documentaryInstructionsNotifiedParty",
            "unece:cefactElementMetadata": [
                {
                    "@id": "cefact:Logistics_TransportMovement.DocumentaryInstructions_Notified.Trade_Party",
                    "@type": "unece:AssociationBIE",
                    "unece:cefactUNId": "UN01003874",
                    "unece:cefactBieDomainClass": "cefact:Logistics_TransportMovement.Details",
                    "rdfs:comment": "A party to be notified of the documentary instructions for this logistics transport movement."
                }
            ]
        },
        {
            "@id": "transport:draughtLevelMeasure",
            "@type": "rdf:Property",
            "schema:rangeIncludes": {
                "@id": "xsd:decimal"
            },
            "schema:domainIncludes": {
                "@id": "transport:LogisticsTransportMeans"
            },
            "rdfs:comment": "The measure of the draught level of this logistics means of transport.",
            "rdfs:label": "draughtLevelMeasure",
            "unece:cefactElementMetadata": [
                {
                    "@id": "cefact:Logistics_TransportMeans.DraughtLevel.Measure",
                    "@type": "unece:BasicBIE",
                    "unece:cefactUNId": "UN01003827",
                    "unece:cefactBieDomainClass": "cefact:Logistics_TransportMeans.Details",
                    "rdfs:comment": "The measure of the draught level of this logistics means of transport."
                }
            ]
        },
        {
            "@id": "transport:driverAccompaniedIndicator",
            "@type": "rdf:Property",
            "schema:rangeIncludes": {
                "@id": "xsd:boolean"
            },
            "schema:domainIncludes": [
                {
                    "@id": "transport:LogisticsTransportMeans"
                },
                {
                    "@id": ":ReferencedTransportMeans"
                }
            ],
            "rdfs:comment": [
                "The indication of whether or not this logistics means of transport is accompanied by a driver.",
                "The indication of whether or not this referenced means of transport is accompanied by a driver."
            ],
            "rdfs:label": "driverAccompaniedIndicator",
            "unece:cefactElementMetadata": [
                {
                    "@id": "cefact:Logistics_TransportMeans.DriverAccompanied.Indicator",
                    "@type": "unece:BasicBIE",
                    "unece:cefactUNId": "UN01010102",
                    "unece:cefactBieDomainClass": "cefact:Logistics_TransportMeans.Details",
                    "rdfs:comment": "The indication of whether or not this logistics means of transport is accompanied by a driver."
                },
                {
                    "@id": "cefact:Referenced_TransportMeans.DriverAccompanied.Indicator",
                    "@type": "unece:BasicBIE",
                    "unece:cefactUNId": "UN01010138",
                    "unece:cefactBieDomainClass": "cefact:Referenced_TransportMeans.Details",
                    "rdfs:comment": "The indication of whether or not this referenced means of transport is accompanied by a driver."
                }
            ]
        },
        {
            "@id": "transport:estimatedApplicableServiceCharge",
            "@type": "rdf:Property",
            "schema:rangeIncludes": {
                "@id": "transport:ServiceCharge"
            },
            "schema:domainIncludes": {
                "@id": "transport:SupplyChainConsignment"
            },
            "rdfs:comment": "An estimated logistics service charge applicable to this supply chain consignment, such as freight or insurance charges.",
            "rdfs:label": "estimatedApplicableServiceCharge",
            "unece:cefactElementMetadata": [
                {
                    "@id": "cefact:SupplyChain_Consignment.Estimated_Applicable.Logistics_ServiceCharge",
                    "@type": "unece:AssociationBIE",
                    "unece:cefactUNId": "UN01004286",
                    "unece:cefactBieDomainClass": "cefact:SupplyChain_Consignment.Details",
                    "rdfs:comment": "An estimated logistics service charge applicable to this supply chain consignment, such as freight or insurance charges."
                }
            ]
        },
        {
            "@id": "transport:examinationEvent",
            "@type": "rdf:Property",
            "schema:rangeIncludes": {
                "@id": "transport:Event"
            },
            "schema:domainIncludes": [
                {
                    "@id": "transport:SupplyChainConsignment"
                },
                {
                    "@id": "transport:SupplyChainConsignmentItem"
                }
            ],
            "rdfs:comment": [
                "An examination event for this supply chain consignment item.",
                "An examination event for this supply chain consignment."
            ],
            "rdfs:label": "examinationEvent",
            "unece:cefactElementMetadata": [
                {
                    "@id": "cefact:SupplyChain_ConsignmentItem.Examination.Transport_Event",
                    "@type": "unece:AssociationBIE",
                    "unece:cefactUNId": "UN01004157",
                    "unece:cefactBieDomainClass": "cefact:SupplyChain_ConsignmentItem.Details",
                    "rdfs:comment": "An examination event for this supply chain consignment item."
                },
                {
                    "@id": "cefact:SupplyChain_Consignment.Examination.Transport_Event",
                    "@type": "unece:AssociationBIE",
                    "unece:cefactUNId": "UN01004253",
                    "unece:cefactBieDomainClass": "cefact:SupplyChain_Consignment.Details",
                    "rdfs:comment": "An examination event for this supply chain consignment."
                }
            ]
        },
        {
            "@id": "transport:excessTransportService",
            "@type": "rdf:Property",
            "schema:rangeIncludes": {
                "@id": "transport:Service"
            },
            "schema:domainIncludes": {
                "@id": "transport:LogisticsTransportMovement"
            },
            "rdfs:comment": "An excess transport service for this logistics transport movement.",
            "rdfs:label": "excessTransportService",
            "unece:cefactElementMetadata": [
                {
                    "@id": "cefact:Logistics_TransportMovement.ExcessTransport.Transport_Service",
                    "@type": "unece:AssociationBIE",
                    "unece:cefactUNId": "UN01008988",
                    "unece:cefactBieDomainClass": "cefact:Logistics_TransportMovement.Details",
                    "rdfs:comment": "An excess transport service for this logistics transport movement."
                }
            ]
        },
        {
            "@id": "transport:exportCountry",
            "@type": "rdf:Property",
            "schema:rangeIncludes": {
                "@id": "transport:Country"
            },
            "schema:domainIncludes": [
                {
                    "@id": "transport:SupplyChainConsignment"
                },
                {
                    "@id": "transport:SupplyChainConsignmentItem"
                }
            ],
            "rdfs:comment": [
                "The export country for this supply chain consignment item.",
                "The export country for this supply chain consignment."
            ],
            "rdfs:label": "exportCountry",
            "unece:cefactElementMetadata": [
                {
                    "@id": "cefact:SupplyChain_ConsignmentItem.Export.Trade_Country",
                    "@type": "unece:AssociationBIE",
                    "unece:cefactUNId": "UN01004140",
                    "unece:cefactBieDomainClass": "cefact:SupplyChain_ConsignmentItem.Details",
                    "rdfs:comment": "The export country for this supply chain consignment item."
                },
                {
                    "@id": "cefact:SupplyChain_Consignment.Export.Trade_Country",
                    "@type": "unece:AssociationBIE",
                    "unece:cefactUNId": "UN01004273",
                    "unece:cefactBieDomainClass": "cefact:SupplyChain_Consignment.Details",
                    "rdfs:comment": "The export country for this supply chain consignment."
                }
            ]
        },
        {
            "@id": "transport:exportExitDateTime",
            "@type": "rdf:Property",
            "schema:rangeIncludes": {
                "@id": "xsd:dateTime"
            },
            "schema:domainIncludes": {
                "@id": "transport:SupplyChainConsignment"
            },
            "rdfs:comment": "The date, time, date time or other date time value when this supply chain consignment will exit, or has exited from the last port, airport, or border post of the country of export.",
            "rdfs:label": "exportExitDateTime",
            "unece:cefactElementMetadata": [
                {
                    "@id": "cefact:SupplyChain_Consignment.ExportExit.DateTime",
                    "@type": "unece:BasicBIE",
                    "unece:TDED": "2043",
                    "unece:cefactUNId": "UN01004171",
                    "unece:cefactBieDomainClass": "cefact:SupplyChain_Consignment.Details",
                    "rdfs:comment": "The date, time, date time or other date time value when this supply chain consignment will exit, or has exited from the last port, airport, or border post of the country of export."
                }
            ]
        },
        {
            "@id": "transport:exportGeopoliticalRegion",
            "@type": "rdf:Property",
            "schema:rangeIncludes": {
                "@id": "transport:GeopoliticalRegion"
            },
            "schema:domainIncludes": [
                {
                    "@id": "transport:SupplyChainConsignment"
                },
                {
                    "@id": "transport:SupplyChainConsignmentItem"
                }
            ],
            "rdfs:comment": [
                "The geopolitical region of export for this supply chain consignment item.",
                "The geopolitical region of export for this supply chain consignment."
            ],
            "rdfs:label": "exportGeopoliticalRegion",
            "unece:cefactElementMetadata": [
                {
                    "@id": "cefact:SupplyChain_ConsignmentItem.Export.Trade_GeopoliticalRegion",
                    "@type": "unece:AssociationBIE",
                    "unece:cefactUNId": "UN01004138",
                    "unece:cefactBieDomainClass": "cefact:SupplyChain_ConsignmentItem.Details",
                    "rdfs:comment": "The geopolitical region of export for this supply chain consignment item."
                },
                {
                    "@id": "cefact:SupplyChain_Consignment.Export.Trade_GeopoliticalRegion",
                    "@type": "unece:AssociationBIE",
                    "unece:cefactUNId": "UN01004276",
                    "unece:cefactBieDomainClass": "cefact:SupplyChain_Consignment.Details",
                    "rdfs:comment": "The geopolitical region of export for this supply chain consignment."
                }
            ]
        },
        {
            "@id": "transport:exportTypeCode",
            "@type": "rdf:Property",
            "schema:rangeIncludes": {
                "@id": "xsd:token"
            },
            "schema:domainIncludes": {
                "@id": "transport:SupplyChainConsignmentItem"
            },
            "rdfs:comment": "The code specifying the export type of supply chain consignment item.",
            "rdfs:label": "exportTypeCode",
            "unece:cefactElementMetadata": [
                {
                    "@id": "cefact:SupplyChain_ConsignmentItem.Export_Type.Code",
                    "@type": "unece:BasicBIE",
                    "unece:TDED": "7357",
                    "unece:cefactUNId": "UN01004111",
                    "unece:cefactBieDomainClass": "cefact:SupplyChain_ConsignmentItem.Details",
                    "rdfs:comment": "The code specifying the export type of supply chain consignment item."
                }
            ]
        },
        {
            "@id": "transport:exporterParty",
            "@type": "rdf:Property",
            "schema:rangeIncludes": {
                "@id": "transport:Party"
            },
            "schema:domainIncludes": {
                "@id": "transport:SupplyChainConsignment"
            },
            "rdfs:comment": "The party who exports this supply chain consignment.",
            "rdfs:label": "exporterParty",
            "unece:cefactElementMetadata": [
                {
                    "@id": "cefact:SupplyChain_Consignment.Exporter.Trade_Party",
                    "@type": "unece:AssociationBIE",
                    "unece:cefactUNId": "UN01004218",
                    "unece:cefactBieDomainClass": "cefact:SupplyChain_Consignment.Details",
                    "rdfs:comment": "The party who exports this supply chain consignment."
                }
            ]
        },
        {
            "@id": "transport:fOBAmount",
            "@type": "rdf:Property",
            "schema:rangeIncludes": {
                "@id": "xsd:decimal"
            },
            "schema:domainIncludes": [
                {
                    "@id": "transport:SupplyChainConsignment"
                },
                {
                    "@id": "transport:SupplyChainConsignmentItem"
                }
            ],
            "rdfs:comment": [
                "The monetary value for this supply chain consignment item as calculated under FOB (Free On Board) delivery terms.",
                "The monetary value that has to be, or has been, paid for this supply chain consignment as calculated under FOB (Free on Board) delivery terms."
            ],
            "rdfs:label": "fOBAmount",
            "unece:cefactElementMetadata": [
                {
                    "@id": "cefact:SupplyChain_Consignment.FOB.Amount",
                    "@type": "unece:BasicBIE",
                    "unece:TDED": "5054",
                    "unece:cefactUNId": "UN01004178",
                    "unece:cefactBieDomainClass": "cefact:SupplyChain_Consignment.Details",
                    "rdfs:comment": "The monetary value that has to be, or has been, paid for this supply chain consignment as calculated under FOB (Free on Board) delivery terms."
                },
                {
                    "@id": "cefact:SupplyChain_ConsignmentItem.FOB.Amount",
                    "@type": "unece:BasicBIE",
                    "unece:cefactUNId": "UN01004116",
                    "unece:cefactBieDomainClass": "cefact:SupplyChain_ConsignmentItem.Details",
                    "rdfs:comment": "The monetary value for this supply chain consignment item as calculated under FOB (Free On Board) delivery terms."
                }
            ]
        },
        {
            "@id": "transport:finalDestinationCountry",
            "@type": "rdf:Property",
            "schema:rangeIncludes": {
                "@id": "transport:Country"
            },
            "schema:domainIncludes": {
                "@id": "transport:SupplyChainConsignment"
            },
            "rdfs:comment": "The final destination country for this supply chain consignment.",
            "rdfs:label": "finalDestinationCountry",
            "unece:cefactElementMetadata": [
                {
                    "@id": "cefact:SupplyChain_Consignment.Final_Destination.Trade_Country",
                    "@type": "unece:AssociationBIE",
                    "unece:cefactUNId": "UN01004271",
                    "unece:cefactBieDomainClass": "cefact:SupplyChain_Consignment.Details",
                    "rdfs:comment": "The final destination country for this supply chain consignment."
                }
            ]
        },
        {
            "@id": "transport:finalDestinationLocation",
            "@type": "rdf:Property",
            "schema:rangeIncludes": {
                "@id": "transport:Location"
            },
            "schema:domainIncludes": {
                "@id": "transport:SupplyChainConsignment"
            },
            "rdfs:comment": "The final destination location for this supply chain consignment.",
            "rdfs:label": "finalDestinationLocation",
            "unece:cefactElementMetadata": [
                {
                    "@id": "cefact:SupplyChain_Consignment.FinalDestination.Logistics_Location",
                    "@type": "unece:AssociationBIE",
                    "unece:cefactUNId": "UN01004242",
                    "unece:cefactBieDomainClass": "cefact:SupplyChain_Consignment.Details",
                    "rdfs:comment": "The final destination location for this supply chain consignment."
                }
            ]
        },
        {
            "@id": "transport:firstArrivalEvent",
            "@type": "rdf:Property",
            "schema:rangeIncludes": {
                "@id": "transport:Event"
            },
            "schema:domainIncludes": {
                "@id": "transport:LogisticsTransportMovement"
            },
            "rdfs:comment": "The first arrival event for this logistics transport movement.",
            "rdfs:label": "firstArrivalEvent",
            "unece:cefactElementMetadata": [
                {
                    "@id": "cefact:Logistics_TransportMovement.First_Arrival.Transport_Event",
                    "@type": "unece:AssociationBIE",
                    "unece:cefactUNId": "UN01003859",
                    "unece:cefactBieDomainClass": "cefact:Logistics_TransportMovement.Details",
                    "rdfs:comment": "The first arrival event for this logistics transport movement."
                }
            ]
        },
        {
            "@id": "transport:firstTypeExtensionCode",
            "@type": "rdf:Property",
            "schema:rangeIncludes": {
                "@id": "xsd:token"
            },
            "schema:domainIncludes": {
                "@id": "transport:SupplyChainConsignmentItem"
            },
            "rdfs:comment": "The code used as a first extension to the type code for further specifying the type of supply chain consignment item.",
            "rdfs:label": "firstTypeExtensionCode",
            "unece:cefactElementMetadata": [
                {
                    "@id": "cefact:SupplyChain_ConsignmentItem.First_TypeExtension.Code",
                    "@type": "unece:BasicBIE",
                    "unece:TDED": "7361",
                    "unece:cefactUNId": "UN01004108",
                    "unece:cefactBieDomainClass": "cefact:SupplyChain_ConsignmentItem.Details",
                    "rdfs:comment": "The code used as a first extension to the type code for further specifying the type of supply chain consignment item."
                }
            ]
        },
        {
            "@id": "transport:forwardDraughtLevelMeasure",
            "@type": "rdf:Property",
            "schema:rangeIncludes": {
                "@id": "xsd:decimal"
            },
            "schema:domainIncludes": {
                "@id": "transport:LogisticsTransportMeans"
            },
            "rdfs:comment": "The draught level measured at the fore end of this transport means.",
            "rdfs:label": "forwardDraughtLevelMeasure",
            "unece:cefactElementMetadata": [
                {
                    "@id": "cefact:Logistics_TransportMeans.Forward_DraughtLevel.Measure",
                    "@type": "unece:BasicBIE",
                    "unece:cefactUNId": "UN01010105",
                    "unece:cefactBieDomainClass": "cefact:Logistics_TransportMeans.Details",
                    "rdfs:comment": "The draught level measured at the fore end of this transport means."
                }
            ]
        },
        {
            "@id": "transport:freightForwarderAssignedId",
            "@type": "rdf:Property",
            "schema:rangeIncludes": {
                "@id": "xsd:token"
            },
            "schema:domainIncludes": [
                {
                    "@id": "transport:Referenced_SupplyChainConsignment"
                },
                {
                    "@id": "transport:SupplyChainConsignment"
                }
            ],
            "rdfs:comment": [
                "The unique identifier assigned by the freight forwarder to this referenced supply chain consignment.",
                "The unique identifier assigned by the freight forwarder to this supply chain consignment."
            ],
            "rdfs:label": "freightForwarderAssignedId",
            "unece:cefactElementMetadata": [
                {
                    "@id": "cefact:Referenced_SupplyChain_Consignment.FreightForwarderAssigned.Identifier",
                    "@type": "unece:BasicBIE",
                    "unece:TDED": "1460",
                    "unece:cefactUNId": "UN01004045",
                    "unece:cefactBieDomainClass": "cefact:Referenced_SupplyChain_Consignment.Details",
                    "rdfs:comment": "The unique identifier assigned by the freight forwarder to this referenced supply chain consignment."
                },
                {
                    "@id": "cefact:SupplyChain_Consignment.FreightForwarderAssigned.Identifier",
                    "@type": "unece:BasicBIE",
                    "unece:TDED": "1460",
                    "unece:cefactUNId": "UN01004165",
                    "unece:cefactBieDomainClass": "cefact:SupplyChain_Consignment.Details",
                    "rdfs:comment": "The unique identifier assigned by the freight forwarder to this supply chain consignment."
                }
            ]
        },
        {
            "@id": "transport:freightForwarderParty",
            "@type": "rdf:Property",
            "schema:rangeIncludes": {
                "@id": "transport:Party"
            },
            "schema:domainIncludes": {
                "@id": "transport:SupplyChainConsignment"
            },
            "rdfs:comment": "The freight forwarder party for this supply chain consignment.",
            "rdfs:label": "freightForwarderParty",
            "unece:cefactElementMetadata": [
                {
                    "@id": "cefact:SupplyChain_Consignment.FreightForwarder.Trade_Party",
                    "@type": "unece:AssociationBIE",
                    "unece:cefactUNId": "UN01004216",
                    "unece:cefactBieDomainClass": "cefact:SupplyChain_Consignment.Details",
                    "rdfs:comment": "The freight forwarder party for this supply chain consignment."
                }
            ]
        },
        {
            "@id": "transport:globalId",
            "@type": "rdf:Property",
            "schema:rangeIncludes": {
                "@id": "xsd:token"
            },
            "schema:domainIncludes": [
                {
                    "@id": "transport:SupplyChainConsignment"
                },
                {
                    "@id": "transport:SupplyChainConsignmentItem"
                }
            ],
            "rdfs:comment": [
                "A global identifier for this supply chain consignment item.",
                "A global identifier of this supply chain consignment."
            ],
            "rdfs:label": "globalId",
            "unece:cefactElementMetadata": [
                {
                    "@id": "cefact:SupplyChain_Consignment.Global_Identification.Identifier",
                    "@type": "unece:BasicBIE",
                    "unece:TDED": "7014",
                    "unece:cefactUNId": "UN01014448",
                    "unece:cefactBieDomainClass": "cefact:SupplyChain_Consignment.Details",
                    "rdfs:comment": "A global identifier of this supply chain consignment."
                },
                {
                    "@id": "cefact:SupplyChain_ConsignmentItem.Global_Identification.Identifier",
                    "@type": "unece:BasicBIE",
                    "unece:cefactUNId": "UN01012575",
                    "unece:cefactBieDomainClass": "cefact:SupplyChain_ConsignmentItem.Details",
                    "rdfs:comment": "A global identifier for this supply chain consignment item."
                }
            ]
        },
        {
            "@id": "transport:goodsReleaseRestriction",
            "@type": "rdf:Property",
            "schema:rangeIncludes": {
                "@id": "xsd:string"
            },
            "schema:domainIncludes": {
                "@id": "transport:SupplyChainConsignment"
            },
            "rdfs:comment": "A goods release restriction, expressed as text, for this supply chain consignment.",
            "rdfs:label": "goodsReleaseRestriction",
            "unece:cefactElementMetadata": [
                {
                    "@id": "cefact:SupplyChain_Consignment.GoodsReleaseRestriction.Text",
                    "@type": "unece:BasicBIE",
                    "unece:TDED": "4248",
                    "unece:cefactUNId": "UN01004202",
                    "unece:cefactBieDomainClass": "cefact:SupplyChain_Consignment.Details",
                    "rdfs:comment": "A goods release restriction, expressed as text, for this supply chain consignment."
                }
            ]
        },
        {
            "@id": "transport:grossVolumeMeasure",
            "@type": "rdf:Property",
            "schema:rangeIncludes": {
                "@id": "xsd:decimal"
            },
            "schema:domainIncludes": [
                {
                    "@id": "transport:AssociatedTransportEquipment"
                },
                {
                    "@id": "transport:LogisticsTransportEquipment"
                },
                {
                    "@id": "transport:Referenced_LogisticsTransportEquipment"
                },
                {
                    "@id": "transport:Referenced_SupplyChainConsignment"
                },
                {
                    "@id": "transport:SupplyChainConsignment"
                },
                {
                    "@id": "transport:SupplyChainConsignmentItem"
                }
            ],
            "rdfs:comment": [
                "A measure of the gross volume, normally calculated by multiplying the maximum length, width and height of this supply chain consignment item.",
                "A measure of the gross volume, normally calculated by multiplying the maximum length, width and height of this supply chain consignment.",
                "A measure of the gross volume, normally calculated by multiplying the maximum length, width and height, of this referenced supply chain consignment.",
                "The measure of the gross volume of this piece of associated transport equipment.",
                "The measure of the gross volume of this piece of logistics transport equipment.",
                "The measure of the gross volume of this piece of referenced logistics transport equipment."
            ],
            "rdfs:label": "grossVolumeMeasure",
            "unece:cefactElementMetadata": [
                {
                    "@id": "cefact:SupplyChain_ConsignmentItem.GrossVolume.Measure",
                    "@type": "unece:BasicBIE",
                    "unece:TDED": "6322",
                    "unece:cefactUNId": "UN01004124",
                    "unece:cefactBieDomainClass": "cefact:SupplyChain_ConsignmentItem.Details",
                    "rdfs:comment": "A measure of the gross volume, normally calculated by multiplying the maximum length, width and height of this supply chain consignment item."
                },
                {
                    "@id": "cefact:SupplyChain_Consignment.GrossVolume.Measure",
                    "@type": "unece:BasicBIE",
                    "unece:TDED": "6422",
                    "unece:cefactUNId": "UN01004175",
                    "unece:cefactBieDomainClass": "cefact:SupplyChain_Consignment.Details",
                    "rdfs:comment": "A measure of the gross volume, normally calculated by multiplying the maximum length, width and height of this supply chain consignment."
                },
                {
                    "@id": "cefact:Referenced_SupplyChain_Consignment.GrossVolume.Measure",
                    "@type": "unece:BasicBIE",
                    "unece:TDED": "6422",
                    "unece:cefactUNId": "UN01011050",
                    "unece:cefactBieDomainClass": "cefact:Referenced_SupplyChain_Consignment.Details",
                    "rdfs:comment": "A measure of the gross volume, normally calculated by multiplying the maximum length, width and height, of this referenced supply chain consignment."
                },
                {
                    "@id": "cefact:Associated_TransportEquipment.GrossVolume.Measure",
                    "@type": "unece:BasicBIE",
                    "unece:cefactUNId": "UN01013657",
                    "unece:cefactBieDomainClass": "cefact:Associated_TransportEquipment.Details",
                    "rdfs:comment": "The measure of the gross volume of this piece of associated transport equipment."
                },
                {
                    "@id": "cefact:Referenced_Logistics_TransportEquipment.GrossVolume.Measure",
                    "@type": "unece:BasicBIE",
                    "unece:TDED": "6411",
                    "unece:cefactUNId": "UN01009016",
                    "unece:cefactBieDomainClass": "cefact:Referenced_Logistics_TransportEquipment.Details",
                    "rdfs:comment": "The measure of the gross volume of this piece of referenced logistics transport equipment."
                },
                {
                    "@id": "cefact:Logistics_TransportEquipment.GrossVolume.Measure",
                    "@type": "unece:BasicBIE",
                    "unece:TDED": "6411",
                    "unece:cefactUNId": "UN01003764",
                    "unece:cefactBieDomainClass": "cefact:Logistics_TransportEquipment.Details",
                    "rdfs:comment": "The measure of the gross volume of this piece of logistics transport equipment."
                }
            ]
        },
        {
            "@id": "transport:grossWeightMeasure",
            "@type": "rdf:Property",
            "schema:rangeIncludes": {
                "@id": "xsd:decimal"
            },
            "schema:domainIncludes": [
                {
                    "@id": "transport:AssociatedTransportEquipment"
                },
                {
                    "@id": "transport:LogisticsTransportEquipment"
                },
                {
                    "@id": "transport:LogisticsTransportMeans"
                },
                {
                    "@id": "transport:Referenced_LogisticsTransportEquipment"
                },
                {
                    "@id": "transport:Referenced_SupplyChainConsignment"
                },
                {
                    "@id": "transport:SupplyChainConsignment"
                },
                {
                    "@id": "transport:SupplyChainConsignmentItem"
                }
            ],
            "rdfs:comment": [
                "A measure of the gross weight (mass) of this referenced supply chain consignment which includes the weight of packaging but which excludes the weight of any transport equipment.",
                "A measure of the gross weight (mass) of this supply chain consignment item which includes packaging but excludes any transport equipment.",
                "A measure of the gross weight (mass) of this supply chain consignment which includes the weight of packaging but which excludes the weight of any transport equipment.",
                "The measure of the gross weight (mass) of this logistics means of transport including cargo, such as the measure of the overall size of a vessel determined in accordance with the provisions of the International Convention on Tonnage Measurement of Ships, 1969.",
                "The measure of the gross weight (mass) of this piece of associated transport equipment which is the weight (mass) including loaded goods, packing and transport equipment.",
                "The measure of the gross weight (mass) of this piece of logistics transport equipment which is the weight (mass) including loaded goods, packing and transport equipment.",
                "The measure of the gross weight (mass) of this piece of referenced logistics transport equipment which is the weight (mass) including loaded goods, packing and transport equipment."
            ],
            "rdfs:label": "grossWeightMeasure",
            "unece:cefactElementMetadata": [
                {
                    "@id": "cefact:SupplyChain_ConsignmentItem.GrossWeight.Measure",
                    "@type": "unece:BasicBIE",
                    "unece:TDED": "6292",
                    "unece:cefactUNId": "UN01004121",
                    "unece:cefactBieDomainClass": "cefact:SupplyChain_ConsignmentItem.Details",
                    "rdfs:comment": "A measure of the gross weight (mass) of this supply chain consignment item which includes packaging but excludes any transport equipment."
                },
                {
                    "@id": "cefact:Associated_TransportEquipment.GrossWeight.Measure",
                    "@type": "unece:BasicBIE",
                    "unece:TDED": "6294",
                    "unece:cefactUNId": "UN01013655",
                    "unece:cefactBieDomainClass": "cefact:Associated_TransportEquipment.Details",
                    "rdfs:comment": "The measure of the gross weight (mass) of this piece of associated transport equipment which is the weight (mass) including loaded goods, packing and transport equipment."
                },
                {
                    "@id": "cefact:Logistics_TransportMeans.GrossWeight.Measure",
                    "@type": "unece:BasicBIE",
                    "unece:TDED": "6411",
                    "unece:cefactUNId": "UN01003824",
                    "unece:cefactBieDomainClass": "cefact:Logistics_TransportMeans.Details",
                    "rdfs:comment": "The measure of the gross weight (mass) of this logistics means of transport including cargo, such as the measure of the overall size of a vessel determined in accordance with the provisions of the International Convention on Tonnage Measurement of Ships, 1969."
                },
                {
                    "@id": "cefact:SupplyChain_Consignment.GrossWeight.Measure",
                    "@type": "unece:BasicBIE",
                    "unece:TDED": "6012",
                    "unece:cefactUNId": "UN01004173",
                    "unece:cefactBieDomainClass": "cefact:SupplyChain_Consignment.Details",
                    "rdfs:comment": "A measure of the gross weight (mass) of this supply chain consignment which includes the weight of packaging but which excludes the weight of any transport equipment."
                },
                {
                    "@id": "cefact:Logistics_TransportEquipment.GrossWeight.Measure",
                    "@type": "unece:BasicBIE",
                    "unece:TDED": "6411",
                    "unece:cefactUNId": "UN01003759",
                    "unece:cefactBieDomainClass": "cefact:Logistics_TransportEquipment.Details",
                    "rdfs:comment": "The measure of the gross weight (mass) of this piece of logistics transport equipment which is the weight (mass) including loaded goods, packing and transport equipment."
                },
                {
                    "@id": "cefact:Referenced_Logistics_TransportEquipment.GrossWeight.Measure",
                    "@type": "unece:BasicBIE",
                    "unece:TDED": "6294",
                    "unece:cefactUNId": "UN01008993",
                    "unece:cefactBieDomainClass": "cefact:Referenced_Logistics_TransportEquipment.Details",
                    "rdfs:comment": "The measure of the gross weight (mass) of this piece of referenced logistics transport equipment which is the weight (mass) including loaded goods, packing and transport equipment."
                },
                {
                    "@id": "cefact:Referenced_SupplyChain_Consignment.GrossWeight.Measure",
                    "@type": "unece:BasicBIE",
                    "unece:TDED": "6012",
                    "unece:cefactUNId": "UN01011048",
                    "unece:cefactBieDomainClass": "cefact:Referenced_SupplyChain_Consignment.Details",
                    "rdfs:comment": "A measure of the gross weight (mass) of this referenced supply chain consignment which includes the weight of packaging but which excludes the weight of any transport equipment."
                }
            ]
        },
        {
            "@id": "transport:groupingCentreParty",
            "@type": "rdf:Property",
            "schema:rangeIncludes": {
                "@id": "transport:Party"
            },
            "schema:domainIncludes": {
                "@id": "transport:SupplyChainConsignment"
            },
            "rdfs:comment": "A grouping centre party for this supply chain consignment.",
            "rdfs:label": "groupingCentreParty",
            "unece:cefactElementMetadata": [
                {
                    "@id": "cefact:SupplyChain_Consignment.GroupingCentre.Trade_Party",
                    "@type": "unece:AssociationBIE",
                    "unece:cefactUNId": "UN01004234",
                    "unece:cefactBieDomainClass": "cefact:SupplyChain_Consignment.Details",
                    "rdfs:comment": "A grouping centre party for this supply chain consignment."
                }
            ]
        },
        {
            "@id": "transport:handlingInstructions",
            "@type": "rdf:Property",
            "schema:rangeIncludes": {
                "@id": "transport:Instructions"
            },
            "schema:domainIncludes": [
                {
                    "@id": "transport:LogisticsTransportEquipment"
                },
                {
                    "@id": "transport:SupplyChainConsignment"
                },
                {
                    "@id": "transport:SupplyChainConsignmentItem"
                }
            ],
            "rdfs:comment": [
                "Handling instructions for this piece of logistics transport equipment.",
                "Handling instructions for this supply chain consignment item.",
                "Handling instructions for this supply chain consignment, such as where or how specified packages or containers are to be loaded on a means of transport."
            ],
            "rdfs:label": "handlingInstructions",
            "unece:cefactElementMetadata": [
                {
                    "@id": "cefact:Logistics_TransportEquipment.Handling.Handling_Instructions",
                    "@type": "unece:AssociationBIE",
                    "unece:cefactUNId": "UN01003789",
                    "unece:cefactBieDomainClass": "cefact:Logistics_TransportEquipment.Details",
                    "rdfs:comment": "Handling instructions for this piece of logistics transport equipment."
                },
                {
                    "@id": "cefact:SupplyChain_Consignment.Handling.Handling_Instructions",
                    "@type": "unece:AssociationBIE",
                    "unece:cefactUNId": "UN01004248",
                    "unece:cefactBieDomainClass": "cefact:SupplyChain_Consignment.Details",
                    "rdfs:comment": "Handling instructions for this supply chain consignment, such as where or how specified packages or containers are to be loaded on a means of transport."
                },
                {
                    "@id": "cefact:SupplyChain_ConsignmentItem.Handling.Handling_Instructions",
                    "@type": "unece:AssociationBIE",
                    "unece:cefactUNId": "UN01004132",
                    "unece:cefactBieDomainClass": "cefact:SupplyChain_ConsignmentItem.Details",
                    "rdfs:comment": "Handling instructions for this supply chain consignment item."
                }
            ]
        },
        {
            "@id": "transport:haulageInstructions",
            "@type": "rdf:Property",
            "schema:rangeIncludes": {
                "@id": "transport:Instructions"
            },
            "schema:domainIncludes": {
                "@id": "transport:SupplyChainConsignment"
            },
            "rdfs:comment": "Haulage instructions for this supply chain consignment.",
            "rdfs:label": "haulageInstructions",
            "unece:cefactElementMetadata": [
                {
                    "@id": "cefact:SupplyChain_Consignment.Haulage.Haulage_Instructions",
                    "@type": "unece:AssociationBIE",
                    "unece:cefactUNId": "UN01004249",
                    "unece:cefactBieDomainClass": "cefact:SupplyChain_Consignment.Details",
                    "rdfs:comment": "Haulage instructions for this supply chain consignment."
                }
            ]
        },
        {
            "@id": "transport:helipadIndicator",
            "@type": "rdf:Property",
            "schema:rangeIncludes": {
                "@id": "xsd:boolean"
            },
            "schema:domainIncludes": {
                "@id": "transport:LogisticsTransportMeans"
            },
            "rdfs:comment": "The indication of whether or not there is a helipad on this logistics means of transport.",
            "rdfs:label": "helipadIndicator",
            "unece:cefactElementMetadata": [
                {
                    "@id": "cefact:Logistics_TransportMeans.Helipad.Indicator",
                    "@type": "unece:BasicBIE",
                    "unece:cefactUNId": "UN01010108",
                    "unece:cefactBieDomainClass": "cefact:Logistics_TransportMeans.Details",
                    "rdfs:comment": "The indication of whether or not there is a helipad on this logistics means of transport."
                }
            ]
        },
        {
            "@id": "transport:homeAddress",
            "@type": "rdf:Property",
            "schema:rangeIncludes": {
                "@id": "transport:Address"
            },
            "schema:domainIncludes": {
                "@id": ":FoundStowaway"
            },
            "rdfs:comment": "A home address for this found stowaway.",
            "rdfs:label": "homeAddress",
            "unece:cefactElementMetadata": [
                {
                    "@id": "cefact:Found_Stowaway.Home.Trade_Address",
                    "@type": "unece:AssociationBIE",
                    "unece:cefactUNId": "UN01014784",
                    "unece:cefactBieDomainClass": "cefact:Found_Stowaway.Details",
                    "rdfs:comment": "A home address for this found stowaway."
                }
            ]
        },
        {
            "@id": "transport:humidityPercent",
            "@type": "rdf:Property",
            "schema:rangeIncludes": {
                "@id": "xsd:decimal"
            },
            "schema:domainIncludes": {
                "@id": "transport:LogisticsTransportEquipment"
            },
            "rdfs:comment": "The percent of the humidity (moisture content) within this piece of logistics transport equipment.",
            "rdfs:label": "humidityPercent",
            "unece:cefactElementMetadata": [
                {
                    "@id": "cefact:Logistics_TransportEquipment.Humidity.Percent",
                    "@type": "unece:BasicBIE",
                    "unece:TDED": "6004",
                    "unece:cefactUNId": "UN01003766",
                    "unece:cefactBieDomainClass": "cefact:Logistics_TransportEquipment.Details",
                    "rdfs:comment": "The percent of the humidity (moisture content) within this piece of logistics transport equipment."
                }
            ]
        },
        {
            "@id": "transport:iSPSRelatedDocument",
            "@type": "rdf:Property",
            "schema:rangeIncludes": {
                "@id": "transport:Document"
            },
            "schema:domainIncludes": {
                "@id": "transport:LogisticsTransportMovement"
            },
            "rdfs:comment": "The International Ship and Port facility Security code (ISPS) document related to this transport movement.",
            "rdfs:label": "iSPSRelatedDocument",
            "unece:cefactElementMetadata": [
                {
                    "@id": "cefact:Logistics_TransportMovement.ISPS_Related.Referenced_Document",
                    "@type": "unece:AssociationBIE",
                    "unece:cefactUNId": "UN01010128",
                    "unece:cefactBieDomainClass": "cefact:Logistics_TransportMovement.Details",
                    "rdfs:comment": "The International Ship and Port facility Security code (ISPS) document related to this transport movement."
                }
            ]
        },
        {
            "@id": "transport:iSPSSecurityLevelCode",
            "@type": "rdf:Property",
            "schema:rangeIncludes": {
                "@id": "xsd:token"
            },
            "schema:domainIncludes": {
                "@id": "transport:LogisticsTransportMeans"
            },
            "rdfs:comment": "The code specifying the International Ship and Port facility Security (ISPS) level assigned to this logistics means of transport.",
            "rdfs:label": "iSPSSecurityLevelCode",
            "unece:cefactElementMetadata": [
                {
                    "@id": "cefact:Logistics_TransportMeans.ISPSSecurityLevel.Code",
                    "@type": "unece:BasicBIE",
                    "unece:cefactUNId": "UN01010109",
                    "unece:cefactBieDomainClass": "cefact:Logistics_TransportMeans.Details",
                    "rdfs:comment": "The code specifying the International Ship and Port facility Security (ISPS) level assigned to this logistics means of transport."
                }
            ]
        },
        {
            "@id": "transport:iSSCDocument",
            "@type": "rdf:Property",
            "schema:rangeIncludes": {
                "@id": "transport:Document"
            },
            "schema:domainIncludes": {
                "@id": "transport:LogisticsTransportMeans"
            },
            "rdfs:comment": "The referenced ISSC (International Ship Security Certificate) document for this logistics transport means.",
            "rdfs:label": "iSSCDocument",
            "unece:cefactElementMetadata": [
                {
                    "@id": "cefact:Logistics_TransportMeans.ISSC.Referenced_Document",
                    "@type": "unece:AssociationBIE",
                    "unece:cefactUNId": "UN01013170",
                    "unece:cefactBieDomainClass": "cefact:Logistics_TransportMeans.Details",
                    "rdfs:comment": "The referenced ISSC (International Ship Security Certificate) document for this logistics transport means."
                }
            ]
        },
        {
            "@id": "transport:iSSCIssuingAuthorityParty",
            "@type": "rdf:Property",
            "schema:rangeIncludes": {
                "@id": "transport:Party"
            },
            "schema:domainIncludes": {
                "@id": "transport:LogisticsTransportMeans"
            },
            "rdfs:comment": "The trade party authorized to issue the International Ship Security Certificate (ISSC) for this logistics means of transport.",
            "rdfs:label": "iSSCIssuingAuthorityParty",
            "unece:cefactElementMetadata": [
                {
                    "@id": "cefact:Logistics_TransportMeans.ISSCIssuingAuthority.Trade_Party",
                    "@type": "unece:AssociationBIE",
                    "unece:cefactUNId": "UN01010117",
                    "unece:cefactBieDomainClass": "cefact:Logistics_TransportMeans.Details",
                    "rdfs:comment": "The trade party authorized to issue the International Ship Security Certificate (ISSC) for this logistics means of transport."
                }
            ]
        },
        {
            "@id": "transport:id",
            "@type": "rdf:Property",
            "schema:rangeIncludes": {
                "@id": "xsd:token"
            },
            "schema:domainIncludes": [
                {
                    "@id": "transport:AssociatedTransportEquipment"
                },
                {
                    "@id": "transport:AttachedTransportEquipment"
                },
                {
                    "@id": "transport:LogisticsPackaging"
                },
                {
                    "@id": "transport:LogisticsTransportEquipment"
                },
                {
                    "@id": "transport:LogisticsTransportMeans"
                },
                {
                    "@id": "transport:LogisticsTransportMovement"
                },
                {
                    "@id": "transport:Referenced_LogisticsTransportEquipment"
                },
                {
                    "@id": "transport:Referenced_SupplyChainConsignment"
                },
                {
                    "@id": "transport:SupplyChainConsignment"
                },
                {
                    "@id": "transport:SupplyChainConsignmentItem"
                }
            ],
            "rdfs:comment": [
                "A unique identifier for this referenced supply chain consignment.",
                "A unique identifier for this supply chain consignment item.",
                "A unique identifier for this supply chain consignment.",
                "A unique identifier of this piece of attached transport equipment.",
                "A unique number, mark or name which identifies this associated piece of transport equipment.",
                "An identifier for this logistics packaging.",
                "An identifier of this logistics means of transport, such as the International Maritime Organization number of a vessel.",
                "The unique identifier for this logistics transport movement, such as a voyage number, flight number, or trip number.",
                "The unique identifier for this referenced piece of logistics transport equipment, such as a number, mark or name.",
                "The unique identifier of this piece of logistics transport equipment."
            ],
            "rdfs:label": "id",
            "unece:cefactElementMetadata": [
                {
                    "@id": "cefact:Logistics_TransportMeans.Identification.Identifier",
                    "@type": "unece:BasicBIE",
                    "unece:TDED": "8213",
                    "unece:cefactUNId": "UN01003822",
                    "unece:cefactBieDomainClass": "cefact:Logistics_TransportMeans.Details",
                    "rdfs:comment": "An identifier of this logistics means of transport, such as the International Maritime Organization number of a vessel."
                },
                {
                    "@id": "cefact:Referenced_Logistics_TransportEquipment.Identification.Identifier",
                    "@type": "unece:BasicBIE",
                    "unece:TDED": "8260",
                    "unece:cefactUNId": "UN01004023",
                    "unece:cefactBieDomainClass": "cefact:Referenced_Logistics_TransportEquipment.Details",
                    "rdfs:comment": "The unique identifier for this referenced piece of logistics transport equipment, such as a number, mark or name."
                },
                {
                    "@id": "cefact:Logistics_TransportEquipment.Identification.Identifier",
                    "@type": "unece:BasicBIE",
                    "unece:TDED": "8260",
                    "unece:cefactUNId": "UN01003758",
                    "unece:cefactBieDomainClass": "cefact:Logistics_TransportEquipment.Details",
                    "rdfs:comment": "The unique identifier of this piece of logistics transport equipment."
                },
                {
                    "@id": "cefact:SupplyChain_ConsignmentItem.Identification.Identifier",
                    "@type": "unece:BasicBIE",
                    "unece:cefactUNId": "UN01004104",
                    "unece:cefactBieDomainClass": "cefact:SupplyChain_ConsignmentItem.Details",
                    "rdfs:comment": "A unique identifier for this supply chain consignment item."
                },
                {
                    "@id": "cefact:Logistics_Packaging.Identification.Identifier",
                    "@type": "unece:BasicBIE",
                    "unece:cefactUNId": "UN01014946",
                    "unece:cefactBieDomainClass": "cefact:Logistics_Packaging.Details",
                    "rdfs:comment": "An identifier for this logistics packaging."
                },
                {
                    "@id": "cefact:Logistics_TransportMovement.Identification.Identifier",
                    "@type": "unece:BasicBIE",
                    "unece:TDED": "8028",
                    "unece:cefactUNId": "UN01003841",
                    "unece:cefactBieDomainClass": "cefact:Logistics_TransportMovement.Details",
                    "rdfs:comment": "The unique identifier for this logistics transport movement, such as a voyage number, flight number, or trip number."
                },
                {
                    "@id": "cefact:Attached_TransportEquipment.Identification.Identifier",
                    "@type": "unece:BasicBIE",
                    "unece:TDED": "8260",
                    "unece:cefactUNId": "UN01003417",
                    "unece:cefactBieDomainClass": "cefact:Attached_TransportEquipment.Details",
                    "rdfs:comment": "A unique identifier of this piece of attached transport equipment."
                },
                {
                    "@id": "cefact:SupplyChain_Consignment.Identification.Identifier",
                    "@type": "unece:BasicBIE",
                    "unece:TDED": "1202",
                    "unece:cefactUNId": "UN01004160",
                    "unece:cefactBieDomainClass": "cefact:SupplyChain_Consignment.Details",
                    "rdfs:comment": "A unique identifier for this supply chain consignment."
                },
                {
                    "@id": "cefact:Referenced_SupplyChain_Consignment.Identification.Identifier",
                    "@type": "unece:BasicBIE",
                    "unece:TDED": "1202",
                    "unece:cefactUNId": "UN01004041",
                    "unece:cefactBieDomainClass": "cefact:Referenced_SupplyChain_Consignment.Details",
                    "rdfs:comment": "A unique identifier for this referenced supply chain consignment."
                },
                {
                    "@id": "cefact:Associated_TransportEquipment.Identification.Identifier",
                    "@type": "unece:BasicBIE",
                    "unece:TDED": "8260",
                    "unece:cefactUNId": "UN01004884",
                    "unece:cefactBieDomainClass": "cefact:Associated_TransportEquipment.Details",
                    "rdfs:comment": "A unique number, mark or name which identifies this associated piece of transport equipment."
                }
            ]
        },
        {
            "@id": "transport:identificationCode",
            "@type": "rdf:Property",
            "schema:rangeIncludes": {
                "@id": "xsd:token"
            },
            "schema:domainIncludes": {
                "@id": "transport:IdentifiedFault"
            },
            "rdfs:comment": "A code specifying an identified fault.",
            "rdfs:label": "identificationCode",
            "unece:cefactElementMetadata": [
                {
                    "@id": "cefact:Identified_Fault.Identification.Code",
                    "@type": "unece:BasicBIE",
                    "unece:cefactUNId": "UN01010067",
                    "unece:cefactBieDomainClass": "cefact:Identified_Fault.Details",
                    "rdfs:comment": "A code specifying an identified fault."
                }
            ]
        },
        {
            "@id": "transport:importCountry",
            "@type": "rdf:Property",
            "schema:rangeIncludes": {
                "@id": "transport:Country"
            },
            "schema:domainIncludes": {
                "@id": "transport:SupplyChainConsignment"
            },
            "rdfs:comment": "The import country for this supply chain consignment.",
            "rdfs:label": "importCountry",
            "unece:cefactElementMetadata": [
                {
                    "@id": "cefact:SupplyChain_Consignment.Import.Trade_Country",
                    "@type": "unece:AssociationBIE",
                    "unece:cefactUNId": "UN01004272",
                    "unece:cefactBieDomainClass": "cefact:SupplyChain_Consignment.Details",
                    "rdfs:comment": "The import country for this supply chain consignment."
                }
            ]
        },
        {
            "@id": "transport:importTypeCode",
            "@type": "rdf:Property",
            "schema:rangeIncludes": {
                "@id": "xsd:token"
            },
            "schema:domainIncludes": {
                "@id": "transport:SupplyChainConsignmentItem"
            },
            "rdfs:comment": "The code specifying the import type of supply chain consignment item.",
            "rdfs:label": "importTypeCode",
            "unece:cefactElementMetadata": [
                {
                    "@id": "cefact:SupplyChain_ConsignmentItem.Import_Type.Code",
                    "@type": "unece:BasicBIE",
                    "unece:TDED": "7357",
                    "unece:cefactUNId": "UN01004112",
                    "unece:cefactBieDomainClass": "cefact:SupplyChain_ConsignmentItem.Details",
                    "rdfs:comment": "The code specifying the import type of supply chain consignment item."
                }
            ]
        },
        {
            "@id": "transport:importationCountry",
            "@type": "rdf:Property",
            "schema:rangeIncludes": {
                "@id": "transport:Country"
            },
            "schema:domainIncludes": {
                "@id": "transport:SupplyChainConsignmentItem"
            },
            "rdfs:comment": "The importation country for this supply chain consignment item.",
            "rdfs:label": "importationCountry",
            "unece:cefactElementMetadata": [
                {
                    "@id": "cefact:SupplyChain_ConsignmentItem.Importation.Trade_Country",
                    "@type": "unece:AssociationBIE",
                    "unece:cefactUNId": "UN01004142",
                    "unece:cefactBieDomainClass": "cefact:SupplyChain_ConsignmentItem.Details",
                    "rdfs:comment": "The importation country for this supply chain consignment item."
                }
            ]
        },
        {
            "@id": "transport:importerParty",
            "@type": "rdf:Property",
            "schema:rangeIncludes": {
                "@id": "transport:Party"
            },
            "schema:domainIncludes": {
                "@id": "transport:SupplyChainConsignment"
            },
            "rdfs:comment": "The party who imports this supply chain consignment.",
            "rdfs:label": "importerParty",
            "unece:cefactElementMetadata": [
                {
                    "@id": "cefact:SupplyChain_Consignment.Importer.Trade_Party",
                    "@type": "unece:AssociationBIE",
                    "unece:cefactUNId": "UN01004217",
                    "unece:cefactBieDomainClass": "cefact:SupplyChain_Consignment.Details",
                    "rdfs:comment": "The party who imports this supply chain consignment."
                }
            ]
        },
        {
            "@id": "transport:includedConsignment",
            "@type": "rdf:Property",
            "schema:rangeIncludes": {
                "@id": "transport:Consignment"
            },
            "schema:domainIncludes": {
                "@id": "transport:SupplyChainConsignment"
            },
            "rdfs:comment": "A referenced consignment included in this supply chain consignment.",
            "rdfs:label": "includedConsignment",
            "unece:cefactElementMetadata": [
                {
                    "@id": "cefact:SupplyChain_Consignment.Included.Referenced_SupplyChain_Consignment",
                    "@type": "unece:AssociationBIE",
                    "unece:cefactUNId": "UN01004259",
                    "unece:cefactBieDomainClass": "cefact:SupplyChain_Consignment.Details",
                    "rdfs:comment": "A referenced consignment included in this supply chain consignment."
                }
            ]
        },
        {
            "@id": "transport:includedConsignmentItem",
            "@type": "rdf:Property",
            "schema:rangeIncludes": {
                "@id": "transport:ConsignmentItem"
            },
            "schema:domainIncludes": [
                {
                    "@id": "transport:Referenced_SupplyChainConsignment"
                },
                {
                    "@id": "transport:SupplyChainConsignment"
                }
            ],
            "rdfs:comment": [
                "A consignment item included in this supply chain consignment.",
                "A referenced consignment item included in this referenced supply chain consignment."
            ],
            "rdfs:label": "includedConsignmentItem",
            "unece:cefactElementMetadata": [
                {
                    "@id": "cefact:Referenced_SupplyChain_Consignment.Included.Referenced_SupplyChain_ConsignmentItem",
                    "@type": "unece:AssociationBIE",
                    "unece:cefactUNId": "UN01004048",
                    "unece:cefactBieDomainClass": "cefact:Referenced_SupplyChain_Consignment.Details",
                    "rdfs:comment": "A referenced consignment item included in this referenced supply chain consignment."
                },
                {
                    "@id": "cefact:SupplyChain_Consignment.Included.SupplyChain_ConsignmentItem",
                    "@type": "unece:AssociationBIE",
                    "unece:cefactUNId": "UN01004258",
                    "unece:cefactBieDomainClass": "cefact:SupplyChain_Consignment.Details",
                    "rdfs:comment": "A consignment item included in this supply chain consignment."
                }
            ]
        },
        {
            "@id": "transport:includedTradeLineItem",
            "@type": "rdf:Property",
            "schema:rangeIncludes": {
                "@id": "transport:TradeLineItem"
            },
            "schema:domainIncludes": [
                {
                    "@id": "transport:Referenced_SupplyChainConsignmentItem"
                },
                {
                    "@id": "transport:SupplyChainConsignmentItem"
                }
            ],
            "rdfs:comment": [
                "A trade line item included in this referenced supply chain consignment item.",
                "A trade line item included in this supply chain consignment item."
            ],
            "rdfs:label": "includedTradeLineItem",
            "unece:cefactElementMetadata": [
                {
                    "@id": "cefact:Referenced_SupplyChain_ConsignmentItem.Included.SupplyChain_TradeLineItem",
                    "@type": "unece:AssociationBIE",
                    "unece:cefactUNId": "UN01011044",
                    "unece:cefactBieDomainClass": "cefact:Referenced_SupplyChain_ConsignmentItem.Details",
                    "rdfs:comment": "A trade line item included in this referenced supply chain consignment item."
                },
                {
                    "@id": "cefact:SupplyChain_ConsignmentItem.Included.SupplyChain_TradeLineItem",
                    "@type": "unece:AssociationBIE",
                    "unece:cefactUNId": "UN01004153",
                    "unece:cefactBieDomainClass": "cefact:SupplyChain_ConsignmentItem.Details",
                    "rdfs:comment": "A trade line item included in this supply chain consignment item."
                }
            ]
        },
        {
            "@id": "transport:information",
            "@type": "rdf:Property",
            "schema:rangeIncludes": {
                "@id": "xsd:string"
            },
            "schema:domainIncludes": [
                {
                    "@id": "transport:LogisticsPackaging"
                },
                {
                    "@id": "transport:LogisticsTransportEquipment"
                },
                {
                    "@id": "transport:SupplyChainConsignment"
                },
                {
                    "@id": "transport:SupplyChainConsignmentItem"
                }
            ],
            "rdfs:comment": [
                "Information, expressed as text, for this logistics packaging.",
                "Information, expressed as text, for this piece of logistics transport equipment.",
                "Information, expressed as text, for this supply chain consignment item.",
                "Information, expressed as text, for this supply chain consignment."
            ],
            "rdfs:label": "information",
            "unece:cefactElementMetadata": [
                {
                    "@id": "cefact:SupplyChain_ConsignmentItem.Information.Text",
                    "@type": "unece:BasicBIE",
                    "unece:cefactUNId": "UN01004128",
                    "unece:cefactBieDomainClass": "cefact:SupplyChain_ConsignmentItem.Details",
                    "rdfs:comment": "Information, expressed as text, for this supply chain consignment item."
                },
                {
                    "@id": "cefact:Logistics_Packaging.Information.Text",
                    "@type": "unece:BasicBIE",
                    "unece:TDED": "4150",
                    "unece:cefactUNId": "UN01014952",
                    "unece:cefactBieDomainClass": "cefact:Logistics_Packaging.Details",
                    "rdfs:comment": "Information, expressed as text, for this logistics packaging."
                },
                {
                    "@id": "cefact:Logistics_TransportEquipment.Information.Text",
                    "@type": "unece:BasicBIE",
                    "unece:TDED": "4014",
                    "unece:cefactUNId": "UN01003778",
                    "unece:cefactBieDomainClass": "cefact:Logistics_TransportEquipment.Details",
                    "rdfs:comment": "Information, expressed as text, for this piece of logistics transport equipment."
                },
                {
                    "@id": "cefact:SupplyChain_Consignment.Information.Text",
                    "@type": "unece:BasicBIE",
                    "unece:TDED": "4070",
                    "unece:cefactUNId": "UN01004203",
                    "unece:cefactBieDomainClass": "cefact:SupplyChain_Consignment.Details",
                    "rdfs:comment": "Information, expressed as text, for this supply chain consignment."
                }
            ]
        },
        {
            "@id": "transport:inspectionParty",
            "@type": "rdf:Property",
            "schema:rangeIncludes": {
                "@id": "transport:Party"
            },
            "schema:domainIncludes": {
                "@id": "transport:LogisticsTransportMovement"
            },
            "rdfs:comment": "An inspection party for this logistics transport movement.",
            "rdfs:label": "inspectionParty",
            "unece:cefactElementMetadata": [
                {
                    "@id": "cefact:Logistics_TransportMovement.Inspection.Trade_Party",
                    "@type": "unece:AssociationBIE",
                    "unece:cefactUNId": "UN01003869",
                    "unece:cefactBieDomainClass": "cefact:Logistics_TransportMovement.Details",
                    "rdfs:comment": "An inspection party for this logistics transport movement."
                }
            ]
        },
        {
            "@id": "transport:instructionCode",
            "@type": "rdf:Property",
            "schema:rangeIncludes": {
                "@id": "xsd:token"
            },
            "schema:domainIncludes": {
                "@id": "transport:LogisticsPackaging"
            },
            "rdfs:comment": "A code specifying an instruction for this logistics packaging.",
            "rdfs:label": "instructionCode",
            "unece:cefactElementMetadata": [
                {
                    "@id": "cefact:Logistics_Packaging.Instruction.Code",
                    "@type": "unece:BasicBIE",
                    "unece:cefactUNId": "UN01014958",
                    "unece:cefactBieDomainClass": "cefact:Logistics_Packaging.Details",
                    "rdfs:comment": "A code specifying an instruction for this logistics packaging."
                }
            ]
        },
        {
            "@id": "transport:instructionIndicator",
            "@type": "rdf:Property",
            "schema:rangeIncludes": {
                "@id": "xsd:boolean"
            },
            "schema:domainIncludes": {
                "@id": "transport:LogisticsPackaging"
            },
            "rdfs:comment": "The indication of whether or not this logistics packaging has an instruction.",
            "rdfs:label": "instructionIndicator",
            "unece:cefactElementMetadata": [
                {
                    "@id": "cefact:Logistics_Packaging.Instruction.Indicator",
                    "@type": "unece:BasicBIE",
                    "unece:cefactUNId": "UN01014964",
                    "unece:cefactBieDomainClass": "cefact:Logistics_Packaging.Details",
                    "rdfs:comment": "The indication of whether or not this logistics packaging has an instruction."
                }
            ]
        },
        {
            "@id": "transport:insuranceApplicableCurrencyExchange",
            "@type": "rdf:Property",
            "schema:rangeIncludes": {
                "@id": "transport:CurrencyExchange"
            },
            "schema:domainIncludes": {
                "@id": "transport:SupplyChainConsignment"
            },
            "rdfs:comment": "A currency exchange applicable to an insurance charge for this supply chain consignment.",
            "rdfs:label": "insuranceApplicableCurrencyExchange",
            "unece:cefactElementMetadata": [
                {
                    "@id": "cefact:SupplyChain_Consignment.Insurance_Applicable.Trade_CurrencyExchange",
                    "@type": "unece:AssociationBIE",
                    "unece:cefactUNId": "UN01004282",
                    "unece:cefactBieDomainClass": "cefact:SupplyChain_Consignment.Details",
                    "rdfs:comment": "A currency exchange applicable to an insurance charge for this supply chain consignment."
                }
            ]
        },
        {
            "@id": "transport:insurancePremiumAmount",
            "@type": "rdf:Property",
            "schema:rangeIncludes": {
                "@id": "xsd:decimal"
            },
            "schema:domainIncludes": {
                "@id": "transport:SupplyChainConsignment"
            },
            "rdfs:comment": "The monetary value of the insurance premium for this supply chain consignment.",
            "rdfs:label": "insurancePremiumAmount",
            "unece:cefactElementMetadata": [
                {
                    "@id": "cefact:SupplyChain_Consignment.InsurancePremium.Amount",
                    "@type": "unece:BasicBIE",
                    "unece:TDED": "5486",
                    "unece:cefactUNId": "UN01004180",
                    "unece:cefactBieDomainClass": "cefact:SupplyChain_Consignment.Details",
                    "rdfs:comment": "The monetary value of the insurance premium for this supply chain consignment."
                }
            ]
        },
        {
            "@id": "transport:insuranceValueAmount",
            "@type": "rdf:Property",
            "schema:rangeIncludes": {
                "@id": "xsd:decimal"
            },
            "schema:domainIncludes": [
                {
                    "@id": "transport:SupplyChainConsignment"
                },
                {
                    "@id": "transport:SupplyChainConsignmentItem"
                }
            ],
            "rdfs:comment": [
                "The monetary value of this supply chain consignment as covered by an insurance policy.",
                "The monetary value of this supply chain consignment item as covered by an insurance policy."
            ],
            "rdfs:label": "insuranceValueAmount",
            "unece:cefactElementMetadata": [
                {
                    "@id": "cefact:SupplyChain_Consignment.InsuranceValue.Amount",
                    "@type": "unece:BasicBIE",
                    "unece:TDED": "5011",
                    "unece:cefactUNId": "UN01004179",
                    "unece:cefactBieDomainClass": "cefact:SupplyChain_Consignment.Details",
                    "rdfs:comment": "The monetary value of this supply chain consignment as covered by an insurance policy."
                },
                {
                    "@id": "cefact:SupplyChain_ConsignmentItem.InsuranceValue.Amount",
                    "@type": "unece:BasicBIE",
                    "unece:cefactUNId": "UN01004117",
                    "unece:cefactBieDomainClass": "cefact:SupplyChain_ConsignmentItem.Details",
                    "rdfs:comment": "The monetary value of this supply chain consignment item as covered by an insurance policy."
                }
            ]
        },
        {
            "@id": "transport:intermediateConsigneeParty",
            "@type": "rdf:Property",
            "schema:rangeIncludes": {
                "@id": "transport:Party"
            },
            "schema:domainIncludes": {
                "@id": "transport:SupplyChainConsignment"
            },
            "rdfs:comment": "A party that is an intermediate consignee for this supply chain consignment.",
            "rdfs:label": "intermediateConsigneeParty",
            "unece:cefactElementMetadata": [
                {
                    "@id": "cefact:SupplyChain_Consignment.IntermediateConsignee.Trade_Party",
                    "@type": "unece:AssociationBIE",
                    "unece:cefactUNId": "UN01004229",
                    "unece:cefactBieDomainClass": "cefact:SupplyChain_Consignment.Details",
                    "rdfs:comment": "A party that is an intermediate consignee for this supply chain consignment."
                }
            ]
        },
        {
            "@id": "transport:invoiceAmount",
            "@type": "rdf:Property",
            "schema:rangeIncludes": {
                "@id": "xsd:decimal"
            },
            "schema:domainIncludes": {
                "@id": "transport:SupplyChainConsignmentItem"
            },
            "rdfs:comment": "A monetary value for an invoice for this supply chain consignment item.",
            "rdfs:label": "invoiceAmount",
            "unece:cefactElementMetadata": [
                {
                    "@id": "cefact:SupplyChain_ConsignmentItem.Invoice.Amount",
                    "@type": "unece:BasicBIE",
                    "unece:TDED": "5444",
                    "unece:cefactUNId": "UN01004118",
                    "unece:cefactBieDomainClass": "cefact:SupplyChain_ConsignmentItem.Details",
                    "rdfs:comment": "A monetary value for an invoice for this supply chain consignment item."
                }
            ]
        },
        {
            "@id": "transport:invoiceApplicableCurrencyExchange",
            "@type": "rdf:Property",
            "schema:rangeIncludes": {
                "@id": "transport:CurrencyExchange"
            },
            "schema:domainIncludes": {
                "@id": "transport:SupplyChainConsignment"
            },
            "rdfs:comment": "A currency exchange applicable to the invoice for this supply chain consignment.",
            "rdfs:label": "invoiceApplicableCurrencyExchange",
            "unece:cefactElementMetadata": [
                {
                    "@id": "cefact:SupplyChain_Consignment.Invoice_Applicable.Trade_CurrencyExchange",
                    "@type": "unece:AssociationBIE",
                    "unece:cefactUNId": "UN01004280",
                    "unece:cefactBieDomainClass": "cefact:SupplyChain_Consignment.Details",
                    "rdfs:comment": "A currency exchange applicable to the invoice for this supply chain consignment."
                }
            ]
        },
        {
            "@id": "transport:invoiceeAssociatedParty",
            "@type": "rdf:Property",
            "schema:rangeIncludes": {
                "@id": "transport:Party"
            },
            "schema:domainIncludes": {
                "@id": "transport:SupplyChainConsignment"
            },
            "rdfs:comment": "An invoicee trade party associated with this supply chain consignment.",
            "rdfs:label": "invoiceeAssociatedParty",
            "unece:cefactElementMetadata": [
                {
                    "@id": "cefact:SupplyChain_Consignment.Invoicee_Associated.Trade_Party",
                    "@type": "unece:AssociationBIE",
                    "unece:cefactUNId": "UN01010143",
                    "unece:cefactBieDomainClass": "cefact:SupplyChain_Consignment.Details",
                    "rdfs:comment": "An invoicee trade party associated with this supply chain consignment."
                }
            ]
        },
        {
            "@id": "transport:invoiceeParty",
            "@type": "rdf:Property",
            "schema:rangeIncludes": {
                "@id": "transport:Party"
            },
            "schema:domainIncludes": {
                "@id": "transport:LogisticsTransportEquipment"
            },
            "rdfs:comment": "The invoicee party for this piece of logistics transport equipment.",
            "rdfs:label": "invoiceeParty",
            "unece:cefactElementMetadata": [
                {
                    "@id": "cefact:Logistics_TransportEquipment.Invoicee.Trade_Party",
                    "@type": "unece:AssociationBIE",
                    "unece:cefactUNId": "UN01003811",
                    "unece:cefactBieDomainClass": "cefact:Logistics_TransportEquipment.Details",
                    "rdfs:comment": "The invoicee party for this piece of logistics transport equipment."
                }
            ]
        },
        {
            "@id": "transport:itineraryRoute",
            "@type": "rdf:Property",
            "schema:rangeIncludes": {
                "@id": "transport:Route"
            },
            "schema:domainIncludes": {
                "@id": "transport:LogisticsTransportMovement"
            },
            "rdfs:comment": "A route in the itinerary of this logistics transport movement.",
            "rdfs:label": "itineraryRoute",
            "unece:cefactElementMetadata": [
                {
                    "@id": "cefact:Logistics_TransportMovement.Itinerary.Transport_Route",
                    "@type": "unece:AssociationBIE",
                    "unece:cefactUNId": "UN01003877",
                    "unece:cefactBieDomainClass": "cefact:Logistics_TransportMovement.Details",
                    "rdfs:comment": "A route in the itinerary of this logistics transport movement."
                }
            ]
        },
        {
            "@id": "transport:layerTotalUnitQuantity",
            "@type": "rdf:Property",
            "schema:rangeIncludes": {
                "@id": "xsd:decimal"
            },
            "schema:domainIncludes": [
                {
                    "@id": "transport:SupplyChainPackaging"
                },
                {
                    "@id": "transport:TradeProduct_SupplyChainPackaging"
                }
            ],
            "rdfs:comment": [
                "The total number of units in a layer of this supply chain packaging.",
                "The total number of units in a layer of this supply chain trade product packaging."
            ],
            "rdfs:label": "layerTotalUnitQuantity",
            "unece:cefactElementMetadata": [
                {
                    "@id": "cefact:SupplyChain_Packaging.Layer_TotalUnit.Quantity",
                    "@type": "unece:BasicBIE",
                    "unece:cefactUNId": "UN01007196",
                    "unece:cefactBieDomainClass": "cefact:SupplyChain_Packaging.Details",
                    "rdfs:comment": "The total number of units in a layer of this supply chain packaging."
                },
                {
                    "@id": "cefact:TradeProduct_SupplyChain_Packaging.Layer_TotalUnit.Quantity",
                    "@type": "unece:BasicBIE",
                    "unece:cefactUNId": "UN01007480",
                    "unece:cefactBieDomainClass": "cefact:TradeProduct_SupplyChain_Packaging.Details",
                    "rdfs:comment": "The total number of units in a layer of this supply chain trade product packaging."
                }
            ]
        },
        {
            "@id": "transport:legalStatusCode",
            "@type": "rdf:Property",
            "schema:rangeIncludes": {
                "@id": "xsd:token"
            },
            "schema:domainIncludes": {
                "@id": "transport:LogisticsTransportEquipment"
            },
            "rdfs:comment": "The code specifying the legal status of this piece of logistics transport equipment with respect to a specific law such as the \"Container Convention Code\".",
            "rdfs:label": "legalStatusCode",
            "unece:cefactElementMetadata": [
                {
                    "@id": "cefact:Logistics_TransportEquipment.LegalStatus.Code",
                    "@type": "unece:BasicBIE",
                    "unece:TDED": "8193",
                    "unece:cefactUNId": "UN01003774",
                    "unece:cefactBieDomainClass": "cefact:Logistics_TransportEquipment.Details",
                    "rdfs:comment": "The code specifying the legal status of this piece of logistics transport equipment with respect to a specific law such as the \"Container Convention Code\"."
                }
            ]
        },
        {
            "@id": "transport:lengthMeasure",
            "@type": "rdf:Property",
            "schema:rangeIncludes": {
                "@id": "xsd:decimal"
            },
            "schema:domainIncludes": {
                "@id": "transport:LogisticsTransportMeans"
            },
            "rdfs:comment": "The measure of the length of this logistics means of transport.",
            "rdfs:label": "lengthMeasure",
            "unece:cefactElementMetadata": [
                {
                    "@id": "cefact:Logistics_TransportMeans.Length.Measure",
                    "@type": "unece:BasicBIE",
                    "unece:cefactUNId": "UN01003826",
                    "unece:cefactBieDomainClass": "cefact:Logistics_TransportMeans.Details",
                    "rdfs:comment": "The measure of the length of this logistics means of transport."
                }
            ]
        },
        {
            "@id": "transport:liftingInstructionsRelatedDocument",
            "@type": "rdf:Property",
            "schema:rangeIncludes": {
                "@id": "transport:Document"
            },
            "schema:domainIncludes": {
                "@id": "transport:LogisticsTransportMovement"
            },
            "rdfs:comment": "A referenced lifting instructions document related to this logistics transport movement.",
            "rdfs:label": "liftingInstructionsRelatedDocument",
            "unece:cefactElementMetadata": [
                {
                    "@id": "cefact:Logistics_TransportMovement.LiftingInstructions_Related.Referenced_Document",
                    "@type": "unece:AssociationBIE",
                    "unece:cefactUNId": "UN01003878",
                    "unece:cefactBieDomainClass": "cefact:Logistics_TransportMovement.Details",
                    "rdfs:comment": "A referenced lifting instructions document related to this logistics transport movement."
                }
            ]
        },
        {
            "@id": "transport:linearDimension",
            "@type": "rdf:Property",
            "schema:rangeIncludes": {
                "@id": "transport:Dimension"
            },
            "schema:domainIncludes": [
                {
                    "@id": "transport:LogisticsPackaging"
                },
                {
                    "@id": "transport:LogisticsTransportEquipment"
                },
                {
                    "@id": "transport:SupplyChainConsignmentItem"
                },
                {
                    "@id": "transport:SupplyChainPackaging"
                },
                {
                    "@id": "transport:TradeProduct_SupplyChainPackaging"
                }
            ],
            "rdfs:comment": [
                "A linear dimension or a set of linear dimensions of this logistics packaging.",
                "The Cross Industry (CI) linear spatial dimensions of this trade product supply chain packaging.",
                "The linear spatial dimensions of this piece of logistics transport equipment.",
                "The linear spatial dimensions of this supply chain consignment item.",
                "The linear spatial dimensions of this supply chain packaging."
            ],
            "rdfs:label": "linearDimension",
            "unece:cefactElementMetadata": [
                {
                    "@id": "cefact:SupplyChain_ConsignmentItem.Linear.Spatial_Dimension",
                    "@type": "unece:AssociationBIE",
                    "unece:cefactUNId": "UN01004136",
                    "unece:cefactBieDomainClass": "cefact:SupplyChain_ConsignmentItem.Details",
                    "rdfs:comment": "The linear spatial dimensions of this supply chain consignment item."
                },
                {
                    "@id": "cefact:SupplyChain_Packaging.Linear.Spatial_Dimension",
                    "@type": "unece:AssociationBIE",
                    "unece:cefactUNId": "UN01004320",
                    "unece:cefactBieDomainClass": "cefact:SupplyChain_Packaging.Details",
                    "rdfs:comment": "The linear spatial dimensions of this supply chain packaging."
                },
                {
                    "@id": "cefact:Logistics_Packaging.Linear.Spatial_Dimension",
                    "@type": "unece:AssociationBIE",
                    "unece:cefactUNId": "UN01014965",
                    "unece:cefactBieDomainClass": "cefact:Logistics_Packaging.Details",
                    "rdfs:comment": "A linear dimension or a set of linear dimensions of this logistics packaging."
                },
                {
                    "@id": "cefact:Logistics_TransportEquipment.Linear.Spatial_Dimension",
                    "@type": "unece:AssociationBIE",
                    "unece:cefactUNId": "UN01003796",
                    "unece:cefactBieDomainClass": "cefact:Logistics_TransportEquipment.Details",
                    "rdfs:comment": "The linear spatial dimensions of this piece of logistics transport equipment."
                },
                {
                    "@id": "cefact:TradeProduct_SupplyChain_Packaging.Linear.CI_Spatial_Dimension",
                    "@type": "unece:AssociationBIE",
                    "unece:cefactUNId": "UN01007482",
                    "unece:cefactBieDomainClass": "cefact:TradeProduct_SupplyChain_Packaging.Details",
                    "rdfs:comment": "The Cross Industry (CI) linear spatial dimensions of this trade product supply chain packaging."
                }
            ]
        },
        {
            "@id": "transport:loadedCargoMeasure",
            "@type": "rdf:Property",
            "schema:rangeIncludes": {
                "@id": "xsd:decimal"
            },
            "schema:domainIncludes": {
                "@id": "transport:LogisticsTransportMeans"
            },
            "rdfs:comment": "The measure of the cargo loaded onto this logistics means of transport, such as the number of barrels of oil or other quantity of breakbulk cargo.",
            "rdfs:label": "loadedCargoMeasure",
            "unece:cefactElementMetadata": [
                {
                    "@id": "cefact:Logistics_TransportMeans.LoadedCargo.Measure",
                    "@type": "unece:BasicBIE",
                    "unece:cefactUNId": "UN01003830",
                    "unece:cefactBieDomainClass": "cefact:Logistics_TransportMeans.Details",
                    "rdfs:comment": "The measure of the cargo loaded onto this logistics means of transport, such as the number of barrels of oil or other quantity of breakbulk cargo."
                }
            ]
        },
        {
            "@id": "transport:loadedConsignmentItem",
            "@type": "rdf:Property",
            "schema:rangeIncludes": {
                "@id": "transport:ConsignmentItem"
            },
            "schema:domainIncludes": {
                "@id": "transport:LogisticsTransportEquipment"
            },
            "rdfs:comment": "A consignment item loaded onto, or into, this piece of logistics transport equipment.",
            "rdfs:label": "loadedConsignmentItem",
            "unece:cefactElementMetadata": [
                {
                    "@id": "cefact:Logistics_TransportEquipment.Loaded.SupplyChain_ConsignmentItem",
                    "@type": "unece:AssociationBIE",
                    "unece:cefactUNId": "UN01003787",
                    "unece:cefactBieDomainClass": "cefact:Logistics_TransportEquipment.Details",
                    "rdfs:comment": "A consignment item loaded onto, or into, this piece of logistics transport equipment."
                }
            ]
        },
        {
            "@id": "transport:loadedDangerousGoods",
            "@type": "rdf:Property",
            "schema:rangeIncludes": {
                "@id": "transport:DangerousGoods"
            },
            "schema:domainIncludes": [
                {
                    "@id": "transport:AssociatedTransportEquipment"
                },
                {
                    "@id": "transport:LogisticsTransportEquipment"
                }
            ],
            "rdfs:comment": [
                "Dangerous goods loaded into or onto this piece of associated transport equipment.",
                "Dangerous goods loaded into this piece of logistics transport equipment."
            ],
            "rdfs:label": "loadedDangerousGoods",
            "unece:cefactElementMetadata": [
                {
                    "@id": "cefact:Logistics_TransportEquipment.Loaded.Transport_DangerousGoods",
                    "@type": "unece:AssociationBIE",
                    "unece:cefactUNId": "UN01003794",
                    "unece:cefactBieDomainClass": "cefact:Logistics_TransportEquipment.Details",
                    "rdfs:comment": "Dangerous goods loaded into this piece of logistics transport equipment."
                },
                {
                    "@id": "cefact:Associated_TransportEquipment.Loaded.Transport_DangerousGoods",
                    "@type": "unece:AssociationBIE",
                    "unece:cefactUNId": "UN01013661",
                    "unece:cefactBieDomainClass": "cefact:Associated_TransportEquipment.Details",
                    "rdfs:comment": "Dangerous goods loaded into or onto this piece of associated transport equipment."
                }
            ]
        },
        {
            "@id": "transport:loadedPackageQuantity",
            "@type": "rdf:Property",
            "schema:rangeIncludes": {
                "@id": "xsd:decimal"
            },
            "schema:domainIncludes": [
                {
                    "@id": "transport:AssociatedTransportEquipment"
                },
                {
                    "@id": "transport:LogisticsTransportEquipment"
                },
                {
                    "@id": "transport:Referenced_LogisticsTransportEquipment"
                }
            ],
            "rdfs:comment": [
                "The number of packages loaded into or onto this piece of associated transport equipment.",
                "The number of packages loaded into or onto this piece of logistics transport equipment.",
                "The number of packages loaded into or onto this piece of referenced logistics transport equipment."
            ],
            "rdfs:label": "loadedPackageQuantity",
            "unece:cefactElementMetadata": [
                {
                    "@id": "cefact:Logistics_TransportEquipment.LoadedPackage.Quantity",
                    "@type": "unece:BasicBIE",
                    "unece:TDED": "7228",
                    "unece:cefactUNId": "UN01003765",
                    "unece:cefactBieDomainClass": "cefact:Logistics_TransportEquipment.Details",
                    "rdfs:comment": "The number of packages loaded into or onto this piece of logistics transport equipment."
                },
                {
                    "@id": "cefact:Associated_TransportEquipment.LoadedPackage.Quantity",
                    "@type": "unece:BasicBIE",
                    "unece:TDED": "7228",
                    "unece:cefactUNId": "UN01013658",
                    "unece:cefactBieDomainClass": "cefact:Associated_TransportEquipment.Details",
                    "rdfs:comment": "The number of packages loaded into or onto this piece of associated transport equipment."
                },
                {
                    "@id": "cefact:Referenced_Logistics_TransportEquipment.LoadedPackage.Quantity",
                    "@type": "unece:BasicBIE",
                    "unece:TDED": "7228",
                    "unece:cefactUNId": "UN01008991",
                    "unece:cefactBieDomainClass": "cefact:Referenced_Logistics_TransportEquipment.Details",
                    "rdfs:comment": "The number of packages loaded into or onto this piece of referenced logistics transport equipment."
                }
            ]
        },
        {
            "@id": "transport:loadingBaseportLocation",
            "@type": "rdf:Property",
            "schema:rangeIncludes": {
                "@id": "transport:Location"
            },
            "schema:domainIncludes": {
                "@id": "transport:SupplyChainConsignment"
            },
            "rdfs:comment": "The baseport location at which this supply chain consignment is to be loaded on a means of transport according to the transport contract.",
            "rdfs:label": "loadingBaseportLocation",
            "unece:cefactElementMetadata": [
                {
                    "@id": "cefact:SupplyChain_Consignment.LoadingBaseport.Logistics_Location",
                    "@type": "unece:AssociationBIE",
                    "unece:cefactUNId": "UN01004238",
                    "unece:cefactBieDomainClass": "cefact:SupplyChain_Consignment.Details",
                    "rdfs:comment": "The baseport location at which this supply chain consignment is to be loaded on a means of transport according to the transport contract."
                }
            ]
        },
        {
            "@id": "transport:loadingEvent",
            "@type": "rdf:Property",
            "schema:rangeIncludes": {
                "@id": "transport:Event"
            },
            "schema:domainIncludes": [
                {
                    "@id": "transport:LogisticsTransportEquipment"
                },
                {
                    "@id": "transport:LogisticsTransportMovement"
                }
            ],
            "rdfs:comment": [
                "The loading event during which goods will be or have been loaded into or onto the means of transport used for this logistics transport movement.",
                "The loading event for this piece of logistics transport equipment."
            ],
            "rdfs:label": "loadingEvent",
            "unece:cefactElementMetadata": [
                {
                    "@id": "cefact:Logistics_TransportMovement.Loading.Transport_Event",
                    "@type": "unece:AssociationBIE",
                    "unece:cefactUNId": "UN01003856",
                    "unece:cefactBieDomainClass": "cefact:Logistics_TransportMovement.Details",
                    "rdfs:comment": "The loading event during which goods will be or have been loaded into or onto the means of transport used for this logistics transport movement."
                },
                {
                    "@id": "cefact:Logistics_TransportEquipment.Loading.Transport_Event",
                    "@type": "unece:AssociationBIE",
                    "unece:cefactUNId": "UN01003802",
                    "unece:cefactBieDomainClass": "cefact:Logistics_TransportEquipment.Details",
                    "rdfs:comment": "The loading event for this piece of logistics transport equipment."
                }
            ]
        },
        {
            "@id": "transport:loadingInformation",
            "@type": "rdf:Property",
            "schema:rangeIncludes": {
                "@id": "xsd:string"
            },
            "schema:domainIncludes": {
                "@id": "transport:SupplyChainConsignment"
            },
            "rdfs:comment": "Loading information, expressed as text, for this supply chain consignment, such as advice and instructions.",
            "rdfs:label": "loadingInformation",
            "unece:cefactElementMetadata": [
                {
                    "@id": "cefact:SupplyChain_Consignment.Loading_Information.Text",
                    "@type": "unece:BasicBIE",
                    "unece:TDED": "4070",
                    "unece:cefactUNId": "UN01004207",
                    "unece:cefactBieDomainClass": "cefact:SupplyChain_Consignment.Details",
                    "rdfs:comment": "Loading information, expressed as text, for this supply chain consignment, such as advice and instructions."
                }
            ]
        },
        {
            "@id": "transport:loadingInspectionParty",
            "@type": "rdf:Property",
            "schema:rangeIncludes": {
                "@id": "transport:Party"
            },
            "schema:domainIncludes": {
                "@id": "transport:LogisticsTransportMovement"
            },
            "rdfs:comment": "The loading inspection party for this logistics transport movement.",
            "rdfs:label": "loadingInspectionParty",
            "unece:cefactElementMetadata": [
                {
                    "@id": "cefact:Logistics_TransportMovement.Loading_Inspection.Trade_Party",
                    "@type": "unece:AssociationBIE",
                    "unece:cefactUNId": "UN01003870",
                    "unece:cefactBieDomainClass": "cefact:Logistics_TransportMovement.Details",
                    "rdfs:comment": "The loading inspection party for this logistics transport movement."
                }
            ]
        },
        {
            "@id": "transport:loadingInspectionSpecifiedInstructions",
            "@type": "rdf:Property",
            "schema:rangeIncludes": {
                "@id": "transport:Instructions"
            },
            "schema:domainIncludes": {
                "@id": "transport:LogisticsTransportMovement"
            },
            "rdfs:comment": "Loading inspection instructions specified for this logistics transport movement.",
            "rdfs:label": "loadingInspectionSpecifiedInstructions",
            "unece:cefactElementMetadata": [
                {
                    "@id": "cefact:Logistics_TransportMovement.LoadingInspection_Specified.Transport_Instructions",
                    "@type": "unece:AssociationBIE",
                    "unece:cefactUNId": "UN01003882",
                    "unece:cefactBieDomainClass": "cefact:Logistics_TransportMovement.Details",
                    "rdfs:comment": "Loading inspection instructions specified for this logistics transport movement."
                }
            ]
        },
        {
            "@id": "transport:loadingInstructions",
            "@type": "rdf:Property",
            "schema:rangeIncludes": {
                "@id": "transport:Instructions"
            },
            "schema:domainIncludes": [
                {
                    "@id": "transport:LogisticsTransportEquipment"
                },
                {
                    "@id": "transport:SupplyChainConsignment"
                }
            ],
            "rdfs:comment": [
                "Loading instructions for this piece of logistics transport equipment.",
                "Loading instructions for this supply chain consignment."
            ],
            "rdfs:label": "loadingInstructions",
            "unece:cefactElementMetadata": [
                {
                    "@id": "cefact:Logistics_TransportEquipment.Loading.Transport_Instructions",
                    "@type": "unece:AssociationBIE",
                    "unece:cefactUNId": "UN01003791",
                    "unece:cefactBieDomainClass": "cefact:Logistics_TransportEquipment.Details",
                    "rdfs:comment": "Loading instructions for this piece of logistics transport equipment."
                },
                {
                    "@id": "cefact:SupplyChain_Consignment.Loading.Transport_Instructions",
                    "@type": "unece:AssociationBIE",
                    "unece:cefactUNId": "UN01004250",
                    "unece:cefactBieDomainClass": "cefact:SupplyChain_Consignment.Details",
                    "rdfs:comment": "Loading instructions for this supply chain consignment."
                }
            ]
        },
        {
            "@id": "transport:loadingLengthMeasure",
            "@type": "rdf:Property",
            "schema:rangeIncludes": {
                "@id": "xsd:decimal"
            },
            "schema:domainIncludes": [
                {
                    "@id": "transport:LogisticsTransportEquipment"
                },
                {
                    "@id": "transport:SupplyChainConsignment"
                },
                {
                    "@id": "transport:SupplyChainConsignmentItem"
                }
            ],
            "rdfs:comment": [
                "A measure of the loading length which is the length along a means of transport over which the complete width and height is needed for loading all the goods items in this supply chain consignment.",
                "The measure of the loading length of this piece of logistics transport equipment.",
                "The measure of the loading length of this supply chain consignment item."
            ],
            "rdfs:label": "loadingLengthMeasure",
            "unece:cefactElementMetadata": [
                {
                    "@id": "cefact:SupplyChain_ConsignmentItem.LoadingLength.Measure",
                    "@type": "unece:BasicBIE",
                    "unece:TDED": "6411",
                    "unece:cefactUNId": "UN01008996",
                    "unece:cefactBieDomainClass": "cefact:SupplyChain_ConsignmentItem.Details",
                    "rdfs:comment": "The measure of the loading length of this supply chain consignment item."
                },
                {
                    "@id": "cefact:Logistics_TransportEquipment.LoadingLength.Measure",
                    "@type": "unece:BasicBIE",
                    "unece:TDED": "6411",
                    "unece:cefactUNId": "UN01003762",
                    "unece:cefactBieDomainClass": "cefact:Logistics_TransportEquipment.Details",
                    "rdfs:comment": "The measure of the loading length of this piece of logistics transport equipment."
                },
                {
                    "@id": "cefact:SupplyChain_Consignment.LoadingLength.Measure",
                    "@type": "unece:BasicBIE",
                    "unece:TDED": "6044",
                    "unece:cefactUNId": "UN01004176",
                    "unece:cefactBieDomainClass": "cefact:SupplyChain_Consignment.Details",
                    "rdfs:comment": "A measure of the loading length which is the length along a means of transport over which the complete width and height is needed for loading all the goods items in this supply chain consignment."
                }
            ]
        },
        {
            "@id": "transport:loadingListQuantity",
            "@type": "rdf:Property",
            "schema:rangeIncludes": {
                "@id": "xsd:decimal"
            },
            "schema:domainIncludes": {
                "@id": "transport:SupplyChainConsignment"
            },
            "rdfs:comment": "The number of loading lists, manifests or similar documents for this supply chain consignment.",
            "rdfs:label": "loadingListQuantity",
            "unece:cefactElementMetadata": [
                {
                    "@id": "cefact:SupplyChain_Consignment.LoadingList.Quantity",
                    "@type": "unece:BasicBIE",
                    "unece:TDED": "1166",
                    "unece:cefactUNId": "UN01004200",
                    "unece:cefactBieDomainClass": "cefact:SupplyChain_Consignment.Details",
                    "rdfs:comment": "The number of loading lists, manifests or similar documents for this supply chain consignment."
                }
            ]
        },
        {
            "@id": "transport:loadingLocation",
            "@type": "rdf:Property",
            "schema:rangeIncludes": {
                "@id": "transport:Location"
            },
            "schema:domainIncludes": {
                "@id": "transport:SupplyChainConsignment"
            },
            "rdfs:comment": "The logistics location where the supply chain consignment is loaded.",
            "rdfs:label": "loadingLocation",
            "unece:cefactElementMetadata": [
                {
                    "@id": "cefact:SupplyChain_Consignment.Loading.Logistics_Location",
                    "@type": "unece:AssociationBIE",
                    "unece:cefactUNId": "UN01013114",
                    "unece:cefactBieDomainClass": "cefact:SupplyChain_Consignment.Details",
                    "rdfs:comment": "The logistics location where the supply chain consignment is loaded."
                }
            ]
        },
        {
            "@id": "transport:loadingParty",
            "@type": "rdf:Property",
            "schema:rangeIncludes": {
                "@id": "transport:Party"
            },
            "schema:domainIncludes": {
                "@id": "transport:LogisticsTransportEquipment"
            },
            "rdfs:comment": "The party that loads this piece of logistics transport equipment.",
            "rdfs:label": "loadingParty",
            "unece:cefactElementMetadata": [
                {
                    "@id": "cefact:Logistics_TransportEquipment.Loading.Trade_Party",
                    "@type": "unece:AssociationBIE",
                    "unece:cefactUNId": "UN01003809",
                    "unece:cefactBieDomainClass": "cefact:Logistics_TransportEquipment.Details",
                    "rdfs:comment": "The party that loads this piece of logistics transport equipment."
                }
            ]
        },
        {
            "@id": "transport:loadingRemark",
            "@type": "rdf:Property",
            "schema:rangeIncludes": {
                "@id": "xsd:string"
            },
            "schema:domainIncludes": {
                "@id": "transport:LogisticsTransportEquipment"
            },
            "rdfs:comment": "A loading remark, expressed as text, for this piece of logistics transport equipment.",
            "rdfs:label": "loadingRemark",
            "unece:cefactElementMetadata": [
                {
                    "@id": "cefact:Logistics_TransportEquipment.LoadingRemark.Text",
                    "@type": "unece:BasicBIE",
                    "unece:cefactUNId": "UN01003776",
                    "unece:cefactBieDomainClass": "cefact:Logistics_TransportEquipment.Details",
                    "rdfs:comment": "A loading remark, expressed as text, for this piece of logistics transport equipment."
                }
            ]
        },
        {
            "@id": "transport:loadingReportedEvent",
            "@type": "rdf:Property",
            "schema:rangeIncludes": {
                "@id": "transport:Event"
            },
            "schema:domainIncludes": {
                "@id": "trade:LogisticsStatus"
            },
            "rdfs:comment": "A transport loading event reported for this logistics status.",
            "rdfs:label": "loadingReportedEvent",
            "unece:cefactElementMetadata": [
                {
                    "@id": "cefact:Logistics_Status.Loading_Reported.Transport_Event",
                    "@type": "unece:AssociationBIE",
                    "unece:cefactUNId": "UN01010095",
                    "unece:cefactBieDomainClass": "cefact:Logistics_Status.Details",
                    "rdfs:comment": "A transport loading event reported for this logistics status."
                }
            ]
        },
        {
            "@id": "transport:loadingSequenceNumeric",
            "@type": "rdf:Property",
            "schema:rangeIncludes": {
                "@id": "xsd:decimal"
            },
            "schema:domainIncludes": [
                {
                    "@id": "transport:LogisticsTransportEquipment"
                },
                {
                    "@id": "transport:SupplyChainConsignment"
                }
            ],
            "rdfs:comment": [
                "The loading sequence number for this supply chain consignment.",
                "The sequence number differentiating this piece of logistics transport equipment from others during loading."
            ],
            "rdfs:label": "loadingSequenceNumeric",
            "unece:cefactElementMetadata": [
                {
                    "@id": "cefact:SupplyChain_Consignment.LoadingSequence.Numeric",
                    "@type": "unece:BasicBIE",
                    "unece:TDED": "1312",
                    "unece:cefactUNId": "UN01004168",
                    "unece:cefactBieDomainClass": "cefact:SupplyChain_Consignment.Details",
                    "rdfs:comment": "The loading sequence number for this supply chain consignment."
                },
                {
                    "@id": "cefact:Logistics_TransportEquipment.LoadingSequence.Numeric",
                    "@type": "unece:BasicBIE",
                    "unece:cefactUNId": "UN01010098",
                    "unece:cefactBieDomainClass": "cefact:Logistics_TransportEquipment.Details",
                    "rdfs:comment": "The sequence number differentiating this piece of logistics transport equipment from others during loading."
                }
            ]
        },
        {
            "@id": "transport:logisticsPackagingLevelCode",
            "@type": "rdf:Property",
            "schema:rangeIncludes": {
                "@id": "unece:UNECECL7075Code"
            },
            "schema:domainIncludes": {
                "@id": "transport:LogisticsPackaging"
            },
            "rdfs:comment": "The code specifying the level of this logistics packaging.",
            "rdfs:label": "logisticsPackagingLevelCode",
            "unece:cefactElementMetadata": [
                {
                    "@id": "cefact:Logistics_Packaging.Level.Code",
                    "@type": "unece:BasicBIE",
                    "unece:TDED": "7075",
                    "unece:cefactUNId": "UN01014948",
                    "unece:cefactBieDomainClass": "cefact:Logistics_Packaging.Details",
                    "rdfs:comment": "The code specifying the level of this logistics packaging."
                }
            ]
        },
        {
            "@id": "transport:logisticsShippingMarksMarkingInstructionCode",
            "@type": "rdf:Property",
            "schema:rangeIncludes": {
                "@id": "unece:UNECECL4233Code"
            },
            "schema:domainIncludes": {
                "@id": "transport:LogisticsShippingMarks"
            },
            "rdfs:comment": "A code specifying a marking instruction for these logistics shipping marks.",
            "rdfs:label": "logisticsShippingMarksMarkingInstructionCode",
            "unece:cefactElementMetadata": [
                {
                    "@id": "cefact:Logistics_ShippingMarks.MarkingInstruction.Code",
                    "@type": "unece:BasicBIE",
                    "unece:TDED": "4233",
                    "unece:cefactUNId": "UN01003743",
                    "unece:cefactBieDomainClass": "cefact:Logistics_ShippingMarks.Details",
                    "rdfs:comment": "A code specifying a marking instruction for these logistics shipping marks."
                }
            ]
        },
        {
            "@id": "transport:logisticsTransportEquipmentCharacteristicCode",
            "@type": "rdf:Property",
            "schema:rangeIncludes": {
                "@id": "unece:UNECECL8155Code"
            },
            "schema:domainIncludes": {
                "@id": "transport:LogisticsTransportEquipment"
            },
            "rdfs:comment": "The code specifying the characteristic or characteristics of this piece of logistics transport equipment, such as the ISO 6346 transport equipment size and type code.",
            "rdfs:label": "logisticsTransportEquipmentCharacteristicCode",
            "unece:cefactElementMetadata": [
                {
                    "@id": "cefact:Logistics_TransportEquipment.Characteristic.Code",
                    "@type": "unece:BasicBIE",
                    "unece:TDED": "8155",
                    "unece:cefactUNId": "UN01003768",
                    "unece:cefactBieDomainClass": "cefact:Logistics_TransportEquipment.Details",
                    "rdfs:comment": "The code specifying the characteristic or characteristics of this piece of logistics transport equipment, such as the ISO 6346 transport equipment size and type code."
                }
            ]
        },
        {
            "@id": "transport:logisticsTransportMovementStatusCode",
            "@type": "rdf:Property",
            "schema:rangeIncludes": {
                "@id": "unece:UNECECL4405Code"
            },
            "schema:domainIncludes": {
                "@id": "transport:LogisticsTransportMovement"
            },
            "rdfs:comment": "The code specifying a status for the logistics transport movement, such as estimated or final.",
            "rdfs:label": "logisticsTransportMovementStatusCode",
            "unece:cefactElementMetadata": [
                {
                    "@id": "cefact:Logistics_TransportMovement.Status.Code",
                    "@type": "unece:BasicBIE",
                    "unece:TDED": "4405",
                    "unece:cefactUNId": "UN01011524",
                    "unece:cefactBieDomainClass": "cefact:Logistics_TransportMovement.Details",
                    "rdfs:comment": "The code specifying a status for the logistics transport movement, such as estimated or final."
                }
            ]
        },
        {
            "@id": "transport:mainCarriageTransportMovement",
            "@type": "rdf:Property",
            "schema:rangeIncludes": {
                "@id": "transport:TransportMovement"
            },
            "schema:domainIncludes": [
                {
                    "@id": "transport:LogisticsTransportEquipment"
                },
                {
                    "@id": "transport:SupplyChainConsignment"
                }
            ],
            "rdfs:comment": [
                "A main carriage logistics transport movement for this supply chain consignment.",
                "A main carriage transport movement for this piece of logistic transport equipment."
            ],
            "rdfs:label": "mainCarriageTransportMovement",
            "unece:cefactElementMetadata": [
                {
                    "@id": "cefact:SupplyChain_Consignment.MainCarriage.Logistics_TransportMovement",
                    "@type": "unece:AssociationBIE",
                    "unece:cefactUNId": "UN01004261",
                    "unece:cefactBieDomainClass": "cefact:SupplyChain_Consignment.Details",
                    "rdfs:comment": "A main carriage logistics transport movement for this supply chain consignment."
                },
                {
                    "@id": "cefact:Logistics_TransportEquipment.MainCarriage.Logistics_TransportMovement",
                    "@type": "unece:AssociationBIE",
                    "unece:cefactUNId": "UN01003816",
                    "unece:cefactBieDomainClass": "cefact:Logistics_TransportEquipment.Details",
                    "rdfs:comment": "A main carriage transport movement for this piece of logistic transport equipment."
                }
            ]
        },
        {
            "@id": "transport:manifestAssociatedDocument",
            "@type": "rdf:Property",
            "schema:rangeIncludes": {
                "@id": "transport:Document"
            },
            "schema:domainIncludes": {
                "@id": "transport:SupplyChainConsignment"
            },
            "rdfs:comment": "A referenced manifest document associated to this supply chain consignment.",
            "rdfs:label": "manifestAssociatedDocument",
            "unece:cefactElementMetadata": [
                {
                    "@id": "cefact:SupplyChain_Consignment.Manifest_Associated.Referenced_Document",
                    "@type": "unece:AssociationBIE",
                    "unece:cefactUNId": "UN01004246",
                    "unece:cefactBieDomainClass": "cefact:SupplyChain_Consignment.Details",
                    "rdfs:comment": "A referenced manifest document associated to this supply chain consignment."
                }
            ]
        },
        {
            "@id": "transport:manifestOnboardIndicator",
            "@type": "rdf:Property",
            "schema:rangeIncludes": {
                "@id": "xsd:boolean"
            },
            "schema:domainIncludes": {
                "@id": "transport:LogisticsTransportMovement"
            },
            "rdfs:comment": "The indication of whether or not the manifest for this logistics transport movement is onboard.",
            "rdfs:label": "manifestOnboardIndicator",
            "unece:cefactElementMetadata": [
                {
                    "@id": "cefact:Logistics_TransportMovement.ManifestOnboard.Indicator",
                    "@type": "unece:BasicBIE",
                    "unece:cefactUNId": "UN01010122",
                    "unece:cefactBieDomainClass": "cefact:Logistics_TransportMovement.Details",
                    "rdfs:comment": "The indication of whether or not the manifest for this logistics transport movement is onboard."
                }
            ]
        },
        {
            "@id": "transport:manifestRelatedDocument",
            "@type": "rdf:Property",
            "schema:rangeIncludes": {
                "@id": "transport:Document"
            },
            "schema:domainIncludes": {
                "@id": "transport:LogisticsTransportMovement"
            },
            "rdfs:comment": "A referenced manifest document related to this transport movement.",
            "rdfs:label": "manifestRelatedDocument",
            "unece:cefactElementMetadata": [
                {
                    "@id": "cefact:Logistics_TransportMovement.Manifest_Related.Referenced_Document",
                    "@type": "unece:AssociationBIE",
                    "unece:cefactUNId": "UN01003879",
                    "unece:cefactBieDomainClass": "cefact:Logistics_TransportMovement.Details",
                    "rdfs:comment": "A referenced manifest document related to this transport movement."
                }
            ]
        },
        {
            "@id": "transport:manoeuvringSpeedMeasure",
            "@type": "rdf:Property",
            "schema:rangeIncludes": {
                "@id": "xsd:decimal"
            },
            "schema:domainIncludes": {
                "@id": "transport:LogisticsTransportMeans"
            },
            "rdfs:comment": "The manoeuvring speed measured for this logistics means of transport.",
            "rdfs:label": "manoeuvringSpeedMeasure",
            "unece:cefactElementMetadata": [
                {
                    "@id": "cefact:Logistics_TransportMeans.Manoeuvring_Speed.Measure",
                    "@type": "unece:BasicBIE",
                    "unece:cefactUNId": "UN01010104",
                    "unece:cefactBieDomainClass": "cefact:Logistics_TransportMeans.Details",
                    "rdfs:comment": "The manoeuvring speed measured for this logistics means of transport."
                }
            ]
        },
        {
            "@id": "transport:manufacturerParty",
            "@type": "rdf:Property",
            "schema:rangeIncludes": {
                "@id": "transport:Party"
            },
            "schema:domainIncludes": [
                {
                    "@id": "transport:LogisticsTransportEquipment"
                },
                {
                    "@id": "transport:LogisticsTransportMeans"
                },
                {
                    "@id": "transport:SupplyChainConsignmentItem"
                }
            ],
            "rdfs:comment": [
                "The manufacturer party for this logistics means of transport.",
                "The manufacturer party specified for this piece of logistics transport equipment.",
                "The party which manufactured this supply chain consignment item."
            ],
            "rdfs:label": "manufacturerParty",
            "unece:cefactElementMetadata": [
                {
                    "@id": "cefact:Logistics_TransportEquipment.Manufacturer.Trade_Party",
                    "@type": "unece:AssociationBIE",
                    "unece:cefactUNId": "UN01013599",
                    "unece:cefactBieDomainClass": "cefact:Logistics_TransportEquipment.Details",
                    "rdfs:comment": "The manufacturer party specified for this piece of logistics transport equipment."
                },
                {
                    "@id": "cefact:Logistics_TransportMeans.Manufacturer.Trade_Party",
                    "@type": "unece:AssociationBIE",
                    "unece:cefactUNId": "UN01013603",
                    "unece:cefactBieDomainClass": "cefact:Logistics_TransportMeans.Details",
                    "rdfs:comment": "The manufacturer party for this logistics means of transport."
                },
                {
                    "@id": "cefact:SupplyChain_ConsignmentItem.Manufacturer.Trade_Party",
                    "@type": "unece:AssociationBIE",
                    "unece:cefactUNId": "UN01004146",
                    "unece:cefactBieDomainClass": "cefact:SupplyChain_ConsignmentItem.Details",
                    "rdfs:comment": "The party which manufactured this supply chain consignment item."
                }
            ]
        },
        {
            "@id": "transport:manufacturingDateTime",
            "@type": "rdf:Property",
            "schema:rangeIncludes": {
                "@id": "xsd:dateTime"
            },
            "schema:domainIncludes": [
                {
                    "@id": "transport:LogisticsTransportEquipment"
                },
                {
                    "@id": "transport:LogisticsTransportMeans"
                }
            ],
            "rdfs:comment": [
                "The manufacturing date, time, date time, or other date time value for this logistics means of transport.",
                "The manufacturing date, time, date time, or other date time value for this piece of logistics transport equipment."
            ],
            "rdfs:label": "manufacturingDateTime",
            "unece:cefactElementMetadata": [
                {
                    "@id": "cefact:Logistics_TransportMeans.Manufacturing.DateTime",
                    "@type": "unece:BasicBIE",
                    "unece:cefactUNId": "UN01013601",
                    "unece:cefactBieDomainClass": "cefact:Logistics_TransportMeans.Details",
                    "rdfs:comment": "The manufacturing date, time, date time, or other date time value for this logistics means of transport."
                },
                {
                    "@id": "cefact:Logistics_TransportEquipment.Manufacturing.DateTime",
                    "@type": "unece:BasicBIE",
                    "unece:cefactUNId": "UN01013591",
                    "unece:cefactBieDomainClass": "cefact:Logistics_TransportEquipment.Details",
                    "rdfs:comment": "The manufacturing date, time, date time, or other date time value for this piece of logistics transport equipment."
                }
            ]
        },
        {
            "@id": "transport:maritimeApplicableCertificate",
            "@type": "rdf:Property",
            "schema:rangeIncludes": {
                "@id": "transport:Certificate"
            },
            "schema:domainIncludes": {
                "@id": "transport:LogisticsTransportMeans"
            },
            "rdfs:comment": "A certificate applicable to a maritime logistics transport means.",
            "rdfs:label": "maritimeApplicableCertificate",
            "unece:cefactElementMetadata": [
                {
                    "@id": "cefact:Logistics_TransportMeans.Maritime_Applicable.Specified_Certificate",
                    "@type": "unece:AssociationBIE",
                    "unece:cefactUNId": "UN01014786",
                    "unece:cefactBieDomainClass": "cefact:Logistics_TransportMeans.Details",
                    "rdfs:comment": "A certificate applicable to a maritime logistics transport means."
                }
            ]
        },
        {
            "@id": "transport:maritimePollutantTypeCode",
            "@type": "rdf:Property",
            "schema:rangeIncludes": {
                "@id": "xsd:token"
            },
            "schema:domainIncludes": {
                "@id": ":TransportDangerousGoods"
            },
            "rdfs:comment": "A code specifying a type of maritime pollutant for the transported dangerous goods.",
            "rdfs:label": "maritimePollutantTypeCode",
            "unece:cefactElementMetadata": [
                {
                    "@id": "cefact:Transport_DangerousGoods.Maritime_PollutantType.Code",
                    "@type": "unece:BasicBIE",
                    "unece:cefactUNId": "UN01014802",
                    "unece:cefactBieDomainClass": "cefact:Transport_DangerousGoods.Details",
                    "rdfs:comment": "A code specifying a type of maritime pollutant for the transported dangerous goods."
                }
            ]
        },
        {
            "@id": "transport:marking",
            "@type": "rdf:Property",
            "schema:rangeIncludes": {
                "@id": "xsd:string"
            },
            "schema:domainIncludes": {
                "@id": "transport:LogisticsShippingMarks"
            },
            "rdfs:comment": "Marking, expressed as text, for these logistics shipping marks.",
            "rdfs:label": "marking",
            "unece:cefactElementMetadata": [
                {
                    "@id": "cefact:Logistics_ShippingMarks.Marking.Text",
                    "@type": "unece:BasicBIE",
                    "unece:TDED": "7102",
                    "unece:cefactUNId": "UN01003742",
                    "unece:cefactBieDomainClass": "cefact:Logistics_ShippingMarks.Details",
                    "rdfs:comment": "Marking, expressed as text, for these logistics shipping marks."
                }
            ]
        },
        {
            "@id": "transport:masterResponsiblePerson",
            "@type": "rdf:Property",
            "schema:rangeIncludes": {
                "@id": "transport:Person"
            },
            "schema:domainIncludes": {
                "@id": "transport:LogisticsTransportMovement"
            },
            "rdfs:comment": "The person legally responsible for the operation of the means of transport used for this logistics transport movement.",
            "rdfs:label": "masterResponsiblePerson",
            "unece:cefactElementMetadata": [
                {
                    "@id": "cefact:Logistics_TransportMovement.Master_Responsible.Transport_Person",
                    "@type": "unece:AssociationBIE",
                    "unece:cefactUNId": "UN01003854",
                    "unece:cefactBieDomainClass": "cefact:Logistics_TransportMovement.Details",
                    "rdfs:comment": "The person legally responsible for the operation of the means of transport used for this logistics transport movement."
                }
            ]
        },
        {
            "@id": "transport:maximumLinearDimension",
            "@type": "rdf:Property",
            "schema:rangeIncludes": {
                "@id": "transport:Dimension"
            },
            "schema:domainIncludes": {
                "@id": "transport:SupplyChainPackaging"
            },
            "rdfs:comment": "The maximum linear spatial dimensions of this supply chain packaging.",
            "rdfs:label": "maximumLinearDimension",
            "unece:cefactElementMetadata": [
                {
                    "@id": "cefact:SupplyChain_Packaging.Maximum_Linear.Spatial_Dimension",
                    "@type": "unece:AssociationBIE",
                    "unece:cefactUNId": "UN01004322",
                    "unece:cefactBieDomainClass": "cefact:SupplyChain_Packaging.Details",
                    "rdfs:comment": "The maximum linear spatial dimensions of this supply chain packaging."
                }
            ]
        },
        {
            "@id": "transport:maximumStackabilityQuantity",
            "@type": "rdf:Property",
            "schema:rangeIncludes": {
                "@id": "xsd:decimal"
            },
            "schema:domainIncludes": [
                {
                    "@id": "transport:LogisticsPackaging"
                },
                {
                    "@id": "transport:SupplyChainPackaging"
                }
            ],
            "rdfs:comment": [
                "The number of units of this type of logistics packaging which can be stacked on top of each other.",
                "The number of units of this type of supply chain packaging which can be stacked on top of each other."
            ],
            "rdfs:label": "maximumStackabilityQuantity",
            "unece:cefactElementMetadata": [
                {
                    "@id": "cefact:Logistics_Packaging.MaximumStackability.Quantity",
                    "@type": "unece:BasicBIE",
                    "unece:cefactUNId": "UN01014959",
                    "unece:cefactBieDomainClass": "cefact:Logistics_Packaging.Details",
                    "rdfs:comment": "The number of units of this type of logistics packaging which can be stacked on top of each other."
                },
                {
                    "@id": "cefact:SupplyChain_Packaging.MaximumStackability.Quantity",
                    "@type": "unece:BasicBIE",
                    "unece:cefactUNId": "UN01006749",
                    "unece:cefactBieDomainClass": "cefact:SupplyChain_Packaging.Details",
                    "rdfs:comment": "The number of units of this type of supply chain packaging which can be stacked on top of each other."
                }
            ]
        },
        {
            "@id": "transport:maximumStackabilityWeightMeasure",
            "@type": "rdf:Property",
            "schema:rangeIncludes": {
                "@id": "xsd:decimal"
            },
            "schema:domainIncludes": {
                "@id": "transport:SupplyChainPackaging"
            },
            "rdfs:comment": "The measure of the maximum stackability weight of this supply chain packaging.",
            "rdfs:label": "maximumStackabilityWeightMeasure",
            "unece:cefactElementMetadata": [
                {
                    "@id": "cefact:SupplyChain_Packaging.MaximumStackability_Weight.Measure",
                    "@type": "unece:BasicBIE",
                    "unece:cefactUNId": "UN01006750",
                    "unece:cefactBieDomainClass": "cefact:SupplyChain_Packaging.Details",
                    "rdfs:comment": "The measure of the maximum stackability weight of this supply chain packaging."
                }
            ]
        },
        {
            "@id": "transport:methodDescription",
            "@type": "rdf:Property",
            "schema:rangeIncludes": {
                "@id": "xsd:string"
            },
            "schema:domainIncludes": {
                "@id": "transport:LogisticsPackaging"
            },
            "rdfs:comment": "The textual description of the method of logistics packaging, such as hermetically sealed.",
            "rdfs:label": "methodDescription",
            "unece:cefactElementMetadata": [
                {
                    "@id": "cefact:Logistics_Packaging.MethodDescription.Text",
                    "@type": "unece:BasicBIE",
                    "unece:cefactUNId": "UN01014962",
                    "unece:cefactBieDomainClass": "cefact:Logistics_Packaging.Details",
                    "rdfs:comment": "The textual description of the method of logistics packaging, such as hermetically sealed."
                }
            ]
        },
        {
            "@id": "transport:minimumLinearDimension",
            "@type": "rdf:Property",
            "schema:rangeIncludes": {
                "@id": "transport:Dimension"
            },
            "schema:domainIncludes": {
                "@id": "transport:SupplyChainPackaging"
            },
            "rdfs:comment": "The minimum linear spatial dimensions of this supply chain packaging.",
            "rdfs:label": "minimumLinearDimension",
            "unece:cefactElementMetadata": [
                {
                    "@id": "cefact:SupplyChain_Packaging.Minimum_Linear.Spatial_Dimension",
                    "@type": "unece:AssociationBIE",
                    "unece:cefactUNId": "UN01004321",
                    "unece:cefactBieDomainClass": "cefact:SupplyChain_Packaging.Details",
                    "rdfs:comment": "The minimum linear spatial dimensions of this supply chain packaging."
                }
            ]
        },
        {
            "@id": "transport:mode",
            "@type": "rdf:Property",
            "schema:rangeIncludes": {
                "@id": "xsd:string"
            },
            "schema:domainIncludes": {
                "@id": "transport:LogisticsTransportMovement"
            },
            "rdfs:comment": "The mode, expressed as text, of this logistics transport movement.",
            "rdfs:label": "mode",
            "unece:cefactElementMetadata": [
                {
                    "@id": "cefact:Logistics_TransportMovement.Mode.Text",
                    "@type": "unece:BasicBIE",
                    "unece:TDED": "8066",
                    "unece:cefactUNId": "UN01003840",
                    "unece:cefactBieDomainClass": "cefact:Logistics_TransportMovement.Details",
                    "rdfs:comment": "The mode, expressed as text, of this logistics transport movement."
                }
            ]
        },
        {
            "@id": "transport:modeCode",
            "@type": "rdf:Property",
            "schema:rangeIncludes": {
                "@id": "xsd:token"
            },
            "schema:domainIncludes": {
                "@id": "transport:LogisticsTransportMovement"
            },
            "rdfs:comment": "The code specifying the mode, such as by air, sea, rail, road or inland waterway, for this logistics transport movement.",
            "rdfs:label": "modeCode",
            "unece:cefactElementMetadata": [
                {
                    "@id": "cefact:Logistics_TransportMovement.Mode.Code",
                    "@type": "unece:BasicBIE",
                    "unece:TDED": "8067",
                    "unece:cefactUNId": "UN01003839",
                    "unece:cefactBieDomainClass": "cefact:Logistics_TransportMovement.Details",
                    "rdfs:comment": "The code specifying the mode, such as by air, sea, rail, road or inland waterway, for this logistics transport movement."
                }
            ]
        },
        {
            "@id": "transport:nVOCCCarrierParty",
            "@type": "rdf:Property",
            "schema:rangeIncludes": {
                "@id": "transport:Party"
            },
            "schema:domainIncludes": {
                "@id": "transport:LogisticsTransportMovement"
            },
            "rdfs:comment": "A Non-Vessel Operating Common Carrier (NVOCC) carrier party for this logistics transport movement.",
            "rdfs:label": "nVOCCCarrierParty",
            "unece:cefactElementMetadata": [
                {
                    "@id": "cefact:Logistics_TransportMovement.NVOCC_Carrier.Trade_Party",
                    "@type": "unece:AssociationBIE",
                    "unece:cefactUNId": "UN01003865",
                    "unece:cefactBieDomainClass": "cefact:Logistics_TransportMovement.Details",
                    "rdfs:comment": "A Non-Vessel Operating Common Carrier (NVOCC) carrier party for this logistics transport movement."
                }
            ]
        },
        {
            "@id": "transport:name",
            "@type": "rdf:Property",
            "schema:rangeIncludes": {
                "@id": "xsd:string"
            },
            "schema:domainIncludes": [
                {
                    "@id": "transport:LogisticsTransportMeans"
                },
                {
                    "@id": "transport:LogisticsTransportMovement"
                }
            ],
            "rdfs:comment": [
                "The name, expressed as text, for this logistics transport movement.",
                "The name, expressed as text, of this logistics means of transport."
            ],
            "rdfs:label": "name",
            "unece:cefactElementMetadata": [
                {
                    "@id": "cefact:Logistics_TransportMovement.Name.Text",
                    "@type": "unece:BasicBIE",
                    "unece:cefactUNId": "UN01013604",
                    "unece:cefactBieDomainClass": "cefact:Logistics_TransportMovement.Details",
                    "rdfs:comment": "The name, expressed as text, for this logistics transport movement."
                },
                {
                    "@id": "cefact:Logistics_TransportMeans.Name.Text",
                    "@type": "unece:BasicBIE",
                    "unece:TDED": "8212",
                    "unece:cefactUNId": "UN01003823",
                    "unece:cefactBieDomainClass": "cefact:Logistics_TransportMeans.Details",
                    "rdfs:comment": "The name, expressed as text, of this logistics means of transport."
                }
            ]
        },
        {
            "@id": "transport:nationalTypeExtensionCode",
            "@type": "rdf:Property",
            "schema:rangeIncludes": {
                "@id": "xsd:token"
            },
            "schema:domainIncludes": {
                "@id": "transport:SupplyChainConsignmentItem"
            },
            "rdfs:comment": "The code used as a national extension to the type code for further specifying the type of supply chain consignment item.",
            "rdfs:label": "nationalTypeExtensionCode",
            "unece:cefactElementMetadata": [
                {
                    "@id": "cefact:SupplyChain_ConsignmentItem.National_TypeExtension.Code",
                    "@type": "unece:BasicBIE",
                    "unece:TDED": "7361",
                    "unece:cefactUNId": "UN01004110",
                    "unece:cefactBieDomainClass": "cefact:SupplyChain_ConsignmentItem.Details",
                    "rdfs:comment": "The code used as a national extension to the type code for further specifying the type of supply chain consignment item."
                }
            ]
        },
        {
            "@id": "transport:natureIdentificationCargo",
            "@type": "rdf:Property",
            "schema:rangeIncludes": {
                "@id": "transport:Cargo"
            },
            "schema:domainIncludes": [
                {
                    "@id": "transport:Referenced_SupplyChainConsignmentItem"
                },
                {
                    "@id": "transport:SupplyChainConsignment"
                },
                {
                    "@id": "transport:SupplyChainConsignmentItem"
                }
            ],
            "rdfs:comment": [
                "Transport cargo details of this referenced supply chain consignment item sufficient to identify its nature for customs, statistical or transport purposes.",
                "Transport cargo details of this supply chain consignment item sufficient to identify its nature for customs, statistical or transport purposes.",
                "Transport cargo details of this supply chain consignment sufficient to identify its nature for customs, statistical or transport purposes."
            ],
            "rdfs:label": "natureIdentificationCargo",
            "unece:cefactElementMetadata": [
                {
                    "@id": "cefact:Referenced_SupplyChain_ConsignmentItem.NatureIdentification.Transport_Cargo",
                    "@type": "unece:AssociationBIE",
                    "unece:cefactUNId": "UN01011045",
                    "unece:cefactBieDomainClass": "cefact:Referenced_SupplyChain_ConsignmentItem.Details",
                    "rdfs:comment": "Transport cargo details of this referenced supply chain consignment item sufficient to identify its nature for customs, statistical or transport purposes."
                },
                {
                    "@id": "cefact:SupplyChain_Consignment.NatureIdentification.Transport_Cargo",
                    "@type": "unece:AssociationBIE",
                    "unece:cefactUNId": "UN01006140",
                    "unece:cefactBieDomainClass": "cefact:SupplyChain_Consignment.Details",
                    "rdfs:comment": "Transport cargo details of this supply chain consignment sufficient to identify its nature for customs, statistical or transport purposes."
                },
                {
                    "@id": "cefact:SupplyChain_ConsignmentItem.NatureIdentification.Transport_Cargo",
                    "@type": "unece:AssociationBIE",
                    "unece:cefactUNId": "UN01004130",
                    "unece:cefactBieDomainClass": "cefact:SupplyChain_ConsignmentItem.Details",
                    "rdfs:comment": "Transport cargo details of this supply chain consignment item sufficient to identify its nature for customs, statistical or transport purposes."
                }
            ]
        },
        {
            "@id": "transport:netVolumeMeasure",
            "@type": "rdf:Property",
            "schema:rangeIncludes": {
                "@id": "xsd:decimal"
            },
            "schema:domainIncludes": {
                "@id": "transport:SupplyChainConsignment"
            },
            "rdfs:comment": "A measure of the net volume of this supply chain consignment item which excludes all packaging.",
            "rdfs:label": "netVolumeMeasure",
            "unece:cefactElementMetadata": [
                {
                    "@id": "cefact:SupplyChain_Consignment.NetVolume.Measure",
                    "@type": "unece:BasicBIE",
                    "unece:cefactUNId": "UN01012710",
                    "unece:cefactBieDomainClass": "cefact:SupplyChain_Consignment.Details",
                    "rdfs:comment": "A measure of the net volume of this supply chain consignment item which excludes all packaging."
                }
            ]
        },
        {
            "@id": "transport:netWeightMeasure",
            "@type": "rdf:Property",
            "schema:rangeIncludes": {
                "@id": "xsd:decimal"
            },
            "schema:domainIncludes": [
                {
                    "@id": "transport:LogisticsTransportEquipment"
                },
                {
                    "@id": "transport:LogisticsTransportMeans"
                },
                {
                    "@id": "transport:Referenced_LogisticsTransportEquipment"
                },
                {
                    "@id": "transport:Referenced_SupplyChainConsignment"
                },
                {
                    "@id": "transport:SupplyChainConsignment"
                },
                {
                    "@id": "transport:SupplyChainConsignmentItem"
                }
            ],
            "rdfs:comment": [
                "A measure of the net weight (mass) of this consignment which excludes the weight of packaging of this supply chain consignment and that of any transport equipment.",
                "A measure of the net weight (mass) of this referenced consignment which excludes the weight of packaging and the weight of any transport equipment.",
                "A measure of the net weight (mass) of this supply chain consignment item which excludes all packaging.",
                "The measure of the net weight (mass) of this logistics means of transport, such as the net tonnage of a vessel determined in accordance with the provisions of the International Convention on Tonnage Measurement of Ships, 1969.",
                "The measure of the net weight (mass) of this piece of logistics transport equipment.",
                "The measure of the net weight (mass) of this piece of referenced logistics transport equipment."
            ],
            "rdfs:label": "netWeightMeasure",
            "unece:cefactElementMetadata": [
                {
                    "@id": "cefact:Referenced_SupplyChain_Consignment.NetWeight.Measure",
                    "@type": "unece:BasicBIE",
                    "unece:TDED": "6014",
                    "unece:cefactUNId": "UN01011049",
                    "unece:cefactBieDomainClass": "cefact:Referenced_SupplyChain_Consignment.Details",
                    "rdfs:comment": "A measure of the net weight (mass) of this referenced consignment which excludes the weight of packaging and the weight of any transport equipment."
                },
                {
                    "@id": "cefact:SupplyChain_Consignment.NetWeight.Measure",
                    "@type": "unece:BasicBIE",
                    "unece:TDED": "6014",
                    "unece:cefactUNId": "UN01004174",
                    "unece:cefactBieDomainClass": "cefact:SupplyChain_Consignment.Details",
                    "rdfs:comment": "A measure of the net weight (mass) of this consignment which excludes the weight of packaging of this supply chain consignment and that of any transport equipment."
                },
                {
                    "@id": "cefact:Logistics_TransportMeans.NetWeight.Measure",
                    "@type": "unece:BasicBIE",
                    "unece:TDED": "6302",
                    "unece:cefactUNId": "UN01003825",
                    "unece:cefactBieDomainClass": "cefact:Logistics_TransportMeans.Details",
                    "rdfs:comment": "The measure of the net weight (mass) of this logistics means of transport, such as the net tonnage of a vessel determined in accordance with the provisions of the International Convention on Tonnage Measurement of Ships, 1969."
                },
                {
                    "@id": "cefact:SupplyChain_ConsignmentItem.NetWeight.Measure",
                    "@type": "unece:BasicBIE",
                    "unece:TDED": "6016",
                    "unece:cefactUNId": "UN01004122",
                    "unece:cefactBieDomainClass": "cefact:SupplyChain_ConsignmentItem.Details",
                    "rdfs:comment": "A measure of the net weight (mass) of this supply chain consignment item which excludes all packaging."
                },
                {
                    "@id": "cefact:Logistics_TransportEquipment.NetWeight.Measure",
                    "@type": "unece:BasicBIE",
                    "unece:TDED": "6160",
                    "unece:cefactUNId": "UN01003760",
                    "unece:cefactBieDomainClass": "cefact:Logistics_TransportEquipment.Details",
                    "rdfs:comment": "The measure of the net weight (mass) of this piece of logistics transport equipment."
                },
                {
                    "@id": "cefact:Referenced_Logistics_TransportEquipment.NetWeight.Measure",
                    "@type": "unece:BasicBIE",
                    "unece:TDED": "6160",
                    "unece:cefactUNId": "UN01008994",
                    "unece:cefactBieDomainClass": "cefact:Referenced_Logistics_TransportEquipment.Details",
                    "rdfs:comment": "The measure of the net weight (mass) of this piece of referenced logistics transport equipment."
                }
            ]
        },
        {
            "@id": "transport:nilCarriageValueIndicator",
            "@type": "rdf:Property",
            "schema:rangeIncludes": {
                "@id": "xsd:boolean"
            },
            "schema:domainIncludes": {
                "@id": "transport:SupplyChainConsignment"
            },
            "rdfs:comment": "The indication of whether or not this supply chain consignment has a nil value for carriage.",
            "rdfs:label": "nilCarriageValueIndicator",
            "unece:cefactElementMetadata": [
                {
                    "@id": "cefact:SupplyChain_Consignment.NilCarriageValue.Indicator",
                    "@type": "unece:BasicBIE",
                    "unece:TDED": "5168",
                    "unece:cefactUNId": "UN01004193",
                    "unece:cefactBieDomainClass": "cefact:SupplyChain_Consignment.Details",
                    "rdfs:comment": "The indication of whether or not this supply chain consignment has a nil value for carriage."
                }
            ]
        },
        {
            "@id": "transport:nilCustomsValueIndicator",
            "@type": "rdf:Property",
            "schema:rangeIncludes": {
                "@id": "xsd:boolean"
            },
            "schema:domainIncludes": {
                "@id": "transport:SupplyChainConsignment"
            },
            "rdfs:comment": "The indication of whether or not this supply chain consignment has a nil value for customs.",
            "rdfs:label": "nilCustomsValueIndicator",
            "unece:cefactElementMetadata": [
                {
                    "@id": "cefact:SupplyChain_Consignment.NilCustomsValue.Indicator",
                    "@type": "unece:BasicBIE",
                    "unece:TDED": "5170",
                    "unece:cefactUNId": "UN01004192",
                    "unece:cefactBieDomainClass": "cefact:SupplyChain_Consignment.Details",
                    "rdfs:comment": "The indication of whether or not this supply chain consignment has a nil value for customs."
                }
            ]
        },
        {
            "@id": "transport:nilInsuranceValueIndicator",
            "@type": "rdf:Property",
            "schema:rangeIncludes": {
                "@id": "xsd:boolean"
            },
            "schema:domainIncludes": {
                "@id": "transport:SupplyChainConsignment"
            },
            "rdfs:comment": "The indication of whether or not this supply chain consignment has a nil value for insurance.",
            "rdfs:label": "nilInsuranceValueIndicator",
            "unece:cefactElementMetadata": [
                {
                    "@id": "cefact:SupplyChain_Consignment.NilInsuranceValue.Indicator",
                    "@type": "unece:BasicBIE",
                    "unece:TDED": "5166",
                    "unece:cefactUNId": "UN01004194",
                    "unece:cefactBieDomainClass": "cefact:SupplyChain_Consignment.Details",
                    "rdfs:comment": "The indication of whether or not this supply chain consignment has a nil value for insurance."
                }
            ]
        },
        {
            "@id": "transport:notifiedParty",
            "@type": "rdf:Property",
            "schema:rangeIncludes": {
                "@id": "transport:Party"
            },
            "schema:domainIncludes": [
                {
                    "@id": "transport:LogisticsTransportEquipment"
                },
                {
                    "@id": "transport:LogisticsTransportMovement"
                },
                {
                    "@id": "transport:Referenced_SupplyChainConsignment"
                },
                {
                    "@id": "transport:SupplyChainConsignment"
                }
            ],
            "rdfs:comment": [
                "A party to be notified about this logistics transport movement.",
                "A party who has been or will be notified about this piece of logistics transport equipment.",
                "A party who has been or will be notified about this referenced supply chain consignment.",
                "A party who has been or will be notified about this supply chain consignment."
            ],
            "rdfs:label": "notifiedParty",
            "unece:cefactElementMetadata": [
                {
                    "@id": "cefact:Referenced_SupplyChain_Consignment.Notified.Trade_Party",
                    "@type": "unece:AssociationBIE",
                    "unece:cefactUNId": "UN01011058",
                    "unece:cefactBieDomainClass": "cefact:Referenced_SupplyChain_Consignment.Details",
                    "rdfs:comment": "A party who has been or will be notified about this referenced supply chain consignment."
                },
                {
                    "@id": "cefact:SupplyChain_Consignment.Notified.Trade_Party",
                    "@type": "unece:AssociationBIE",
                    "unece:cefactUNId": "UN01004223",
                    "unece:cefactBieDomainClass": "cefact:SupplyChain_Consignment.Details",
                    "rdfs:comment": "A party who has been or will be notified about this supply chain consignment."
                },
                {
                    "@id": "cefact:Logistics_TransportMovement.Notified.Trade_Party",
                    "@type": "unece:AssociationBIE",
                    "unece:cefactUNId": "UN01003873",
                    "unece:cefactBieDomainClass": "cefact:Logistics_TransportMovement.Details",
                    "rdfs:comment": "A party to be notified about this logistics transport movement."
                },
                {
                    "@id": "cefact:Logistics_TransportEquipment.Notified.Trade_Party",
                    "@type": "unece:AssociationBIE",
                    "unece:cefactUNId": "UN01003813",
                    "unece:cefactBieDomainClass": "cefact:Logistics_TransportEquipment.Details",
                    "rdfs:comment": "A party who has been or will be notified about this piece of logistics transport equipment."
                }
            ]
        },
        {
            "@id": "transport:onCarriageTransportMovement",
            "@type": "rdf:Property",
            "schema:rangeIncludes": {
                "@id": "transport:TransportMovement"
            },
            "schema:domainIncludes": [
                {
                    "@id": "transport:LogisticsTransportEquipment"
                },
                {
                    "@id": "transport:SupplyChainConsignment"
                }
            ],
            "rdfs:comment": [
                "An on-carriage logistics transport movement for this supply chain consignment.",
                "An on-carriage transport movement for this piece of logistics transport equipment."
            ],
            "rdfs:label": "onCarriageTransportMovement",
            "unece:cefactElementMetadata": [
                {
                    "@id": "cefact:SupplyChain_Consignment.On-Carriage.Logistics_TransportMovement",
                    "@type": "unece:AssociationBIE",
                    "unece:cefactUNId": "UN01004263",
                    "unece:cefactBieDomainClass": "cefact:SupplyChain_Consignment.Details",
                    "rdfs:comment": "An on-carriage logistics transport movement for this supply chain consignment."
                },
                {
                    "@id": "cefact:Logistics_TransportEquipment.On-Carriage.Logistics_TransportMovement",
                    "@type": "unece:AssociationBIE",
                    "unece:cefactUNId": "UN01003817",
                    "unece:cefactBieDomainClass": "cefact:Logistics_TransportEquipment.Details",
                    "rdfs:comment": "An on-carriage transport movement for this piece of logistics transport equipment."
                }
            ]
        },
        {
            "@id": "transport:onboardInventory",
            "@type": "rdf:Property",
            "schema:rangeIncludes": {
                "@id": "transport:Inventory"
            },
            "schema:domainIncludes": {
                "@id": "transport:LogisticsTransportMovement"
            },
            "rdfs:comment": "A stores inventory item held onboard for this logistics transport movement.",
            "rdfs:label": "onboardInventory",
            "unece:cefactElementMetadata": [
                {
                    "@id": "cefact:Logistics_TransportMovement.Onboard.StoresItem_Inventory",
                    "@type": "unece:AssociationBIE",
                    "unece:cefactUNId": "UN01013176",
                    "unece:cefactBieDomainClass": "cefact:Logistics_TransportMovement.Details",
                    "rdfs:comment": "A stores inventory item held onboard for this logistics transport movement."
                }
            ]
        },
        {
            "@id": "transport:onboardPerson",
            "@type": "rdf:Property",
            "schema:rangeIncludes": {
                "@id": "transport:Person"
            },
            "schema:domainIncludes": {
                "@id": "transport:LogisticsTransportMovement"
            },
            "rdfs:comment": "A person onboard this logistics transport movement.",
            "rdfs:label": "onboardPerson",
            "unece:cefactElementMetadata": [
                {
                    "@id": "cefact:Logistics_TransportMovement.Onboard.Transport_Person",
                    "@type": "unece:AssociationBIE",
                    "unece:cefactUNId": "UN01013174",
                    "unece:cefactBieDomainClass": "cefact:Logistics_TransportMovement.Details",
                    "rdfs:comment": "A person onboard this logistics transport movement."
                }
            ]
        },
        {
            "@id": "transport:onboardPersonQuantity",
            "@type": "rdf:Property",
            "schema:rangeIncludes": {
                "@id": "xsd:decimal"
            },
            "schema:domainIncludes": {
                "@id": "transport:LogisticsTransportMovement"
            },
            "rdfs:comment": "The number of onboard persons for this logistics transport movement.",
            "rdfs:label": "onboardPersonQuantity",
            "unece:cefactElementMetadata": [
                {
                    "@id": "cefact:Logistics_TransportMovement.OnboardPerson.Quantity",
                    "@type": "unece:BasicBIE",
                    "unece:cefactUNId": "UN01015084",
                    "unece:cefactBieDomainClass": "cefact:Logistics_TransportMovement.Details",
                    "rdfs:comment": "The number of onboard persons for this logistics transport movement."
                }
            ]
        },
        {
            "@id": "transport:onwardRoutingLocation",
            "@type": "rdf:Property",
            "schema:rangeIncludes": {
                "@id": "transport:Location"
            },
            "schema:domainIncludes": {
                "@id": "transport:SupplyChainConsignment"
            },
            "rdfs:comment": "An onward routing location for this supply chain consignment.",
            "rdfs:label": "onwardRoutingLocation",
            "unece:cefactElementMetadata": [
                {
                    "@id": "cefact:SupplyChain_Consignment.OnwardRouting.Logistics_Location",
                    "@type": "unece:AssociationBIE",
                    "unece:cefactUNId": "UN01015092",
                    "unece:cefactBieDomainClass": "cefact:SupplyChain_Consignment.Details",
                    "rdfs:comment": "An onward routing location for this supply chain consignment."
                }
            ]
        },
        {
            "@id": "transport:operatingParty",
            "@type": "rdf:Property",
            "schema:rangeIncludes": {
                "@id": "transport:Party"
            },
            "schema:domainIncludes": {
                "@id": "transport:LogisticsTransportEquipment"
            },
            "rdfs:comment": "The party that operates this piece of logistics transport equipment.",
            "rdfs:label": "operatingParty",
            "unece:cefactElementMetadata": [
                {
                    "@id": "cefact:Logistics_TransportEquipment.Operating.Trade_Party",
                    "@type": "unece:AssociationBIE",
                    "unece:cefactUNId": "UN01003808",
                    "unece:cefactBieDomainClass": "cefact:Logistics_TransportEquipment.Details",
                    "rdfs:comment": "The party that operates this piece of logistics transport equipment."
                }
            ]
        },
        {
            "@id": "transport:operatorNationalityCountry",
            "@type": "rdf:Property",
            "schema:rangeIncludes": {
                "@id": "transport:Country"
            },
            "schema:domainIncludes": {
                "@id": "transport:LogisticsTransportMeans"
            },
            "rdfs:comment": "The country of nationality of the operator of this logistics means of transport.",
            "rdfs:label": "operatorNationalityCountry",
            "unece:cefactElementMetadata": [
                {
                    "@id": "cefact:Logistics_TransportMeans.OperatorNationality.Trade_Country",
                    "@type": "unece:AssociationBIE",
                    "unece:cefactUNId": "UN01003833",
                    "unece:cefactBieDomainClass": "cefact:Logistics_TransportMeans.Details",
                    "rdfs:comment": "The country of nationality of the operator of this logistics means of transport."
                }
            ]
        },
        {
            "@id": "transport:operatorParty",
            "@type": "rdf:Property",
            "schema:rangeIncludes": {
                "@id": "transport:Party"
            },
            "schema:domainIncludes": {
                "@id": "transport:LogisticsTransportMeans"
            },
            "rdfs:comment": "The party operating this logistics means of transport.",
            "rdfs:label": "operatorParty",
            "unece:cefactElementMetadata": [
                {
                    "@id": "cefact:Logistics_TransportMeans.Operator.Trade_Party",
                    "@type": "unece:AssociationBIE",
                    "unece:cefactUNId": "UN01003835",
                    "unece:cefactBieDomainClass": "cefact:Logistics_TransportMeans.Details",
                    "rdfs:comment": "The party operating this logistics means of transport."
                }
            ]
        },
        {
            "@id": "transport:originCountry",
            "@type": "rdf:Property",
            "schema:rangeIncludes": {
                "@id": "transport:Country"
            },
            "schema:domainIncludes": [
                {
                    "@id": "transport:SupplyChainConsignment"
                },
                {
                    "@id": "transport:SupplyChainConsignmentItem"
                }
            ],
            "rdfs:comment": [
                "A country of origin for this supply chain consignment.",
                "The country of origin where this supply chain consignment item has been produced."
            ],
            "rdfs:label": "originCountry",
            "unece:cefactElementMetadata": [
                {
                    "@id": "cefact:SupplyChain_ConsignmentItem.Origin.Trade_Country",
                    "@type": "unece:AssociationBIE",
                    "unece:cefactUNId": "UN01004139",
                    "unece:cefactBieDomainClass": "cefact:SupplyChain_ConsignmentItem.Details",
                    "rdfs:comment": "The country of origin where this supply chain consignment item has been produced."
                },
                {
                    "@id": "cefact:SupplyChain_Consignment.Origin.Trade_Country",
                    "@type": "unece:AssociationBIE",
                    "unece:cefactUNId": "UN01004268",
                    "unece:cefactBieDomainClass": "cefact:SupplyChain_Consignment.Details",
                    "rdfs:comment": "A country of origin for this supply chain consignment."
                }
            ]
        },
        {
            "@id": "transport:originGeopoliticalRegion",
            "@type": "rdf:Property",
            "schema:rangeIncludes": {
                "@id": "transport:GeopoliticalRegion"
            },
            "schema:domainIncludes": [
                {
                    "@id": "transport:SupplyChainConsignment"
                },
                {
                    "@id": "transport:SupplyChainConsignmentItem"
                }
            ],
            "rdfs:comment": [
                "The geopolitical region of origin for this supply chain consignment item.",
                "The geopolitical region of origin for this supply chain consignment."
            ],
            "rdfs:label": "originGeopoliticalRegion",
            "unece:cefactElementMetadata": [
                {
                    "@id": "cefact:SupplyChain_ConsignmentItem.Origin.Trade_GeopoliticalRegion",
                    "@type": "unece:AssociationBIE",
                    "unece:cefactUNId": "UN01004137",
                    "unece:cefactBieDomainClass": "cefact:SupplyChain_ConsignmentItem.Details",
                    "rdfs:comment": "The geopolitical region of origin for this supply chain consignment item."
                },
                {
                    "@id": "cefact:SupplyChain_Consignment.Origin.Trade_GeopoliticalRegion",
                    "@type": "unece:AssociationBIE",
                    "unece:cefactUNId": "UN01004275",
                    "unece:cefactBieDomainClass": "cefact:SupplyChain_Consignment.Details",
                    "rdfs:comment": "The geopolitical region of origin for this supply chain consignment."
                }
            ]
        },
        {
            "@id": "transport:originalDespatchLocation",
            "@type": "rdf:Property",
            "schema:rangeIncludes": {
                "@id": "transport:Location"
            },
            "schema:domainIncludes": {
                "@id": "transport:SupplyChainConsignment"
            },
            "rdfs:comment": "The location from which this supply chain consignment was originally despatched.",
            "rdfs:label": "originalDespatchLocation",
            "unece:cefactElementMetadata": [
                {
                    "@id": "cefact:SupplyChain_Consignment.OriginalDespatch.Logistics_Location",
                    "@type": "unece:AssociationBIE",
                    "unece:cefactUNId": "UN01015093",
                    "unece:cefactBieDomainClass": "cefact:SupplyChain_Consignment.Details",
                    "rdfs:comment": "The location from which this supply chain consignment was originally despatched."
                }
            ]
        },
        {
            "@id": "transport:ownerAgentParty",
            "@type": "rdf:Property",
            "schema:rangeIncludes": {
                "@id": "transport:Party"
            },
            "schema:domainIncludes": {
                "@id": "transport:LogisticsTransportMeans"
            },
            "rdfs:comment": "The owner agent trade party for this logistics means of transport.",
            "rdfs:label": "ownerAgentParty",
            "unece:cefactElementMetadata": [
                {
                    "@id": "cefact:Logistics_TransportMeans.OwnerAgent.Trade_Party",
                    "@type": "unece:AssociationBIE",
                    "unece:cefactUNId": "UN01010116",
                    "unece:cefactBieDomainClass": "cefact:Logistics_TransportMeans.Details",
                    "rdfs:comment": "The owner agent trade party for this logistics means of transport."
                }
            ]
        },
        {
            "@id": "transport:ownerParty",
            "@type": "rdf:Property",
            "schema:rangeIncludes": {
                "@id": "transport:Party"
            },
            "schema:domainIncludes": [
                {
                    "@id": "transport:LogisticsTransportEquipment"
                },
                {
                    "@id": "transport:LogisticsTransportMeans"
                }
            ],
            "rdfs:comment": [
                "A party who owns this piece of logistics transport equipment.",
                "The party owning this logistics means of transport."
            ],
            "rdfs:label": "ownerParty",
            "unece:cefactElementMetadata": [
                {
                    "@id": "cefact:Logistics_TransportMeans.Owner.Trade_Party",
                    "@type": "unece:AssociationBIE",
                    "unece:cefactUNId": "UN01003836",
                    "unece:cefactBieDomainClass": "cefact:Logistics_TransportMeans.Details",
                    "rdfs:comment": "The party owning this logistics means of transport."
                },
                {
                    "@id": "cefact:Logistics_TransportEquipment.Owner.Trade_Party",
                    "@type": "unece:AssociationBIE",
                    "unece:cefactUNId": "UN01014631",
                    "unece:cefactBieDomainClass": "cefact:Logistics_TransportEquipment.Details",
                    "rdfs:comment": "A party who owns this piece of logistics transport equipment."
                }
            ]
        },
        {
            "@id": "transport:packageQuantity",
            "@type": "rdf:Property",
            "schema:rangeIncludes": {
                "@id": "xsd:decimal"
            },
            "schema:domainIncludes": [
                {
                    "@id": "transport:LogisticsTransportMovement"
                },
                {
                    "@id": "transport:SupplyChainConsignment"
                },
                {
                    "@id": "transport:SupplyChainConsignmentItem"
                }
            ],
            "rdfs:comment": [
                "The number of packages in this logistics transport movement.",
                "The number of packages within this supply chain consignment.",
                "The package quantity for this supply chain consignment item."
            ],
            "rdfs:label": "packageQuantity",
            "unece:cefactElementMetadata": [
                {
                    "@id": "cefact:Logistics_TransportMovement.Package.Quantity",
                    "@type": "unece:BasicBIE",
                    "unece:cefactUNId": "UN01006137",
                    "unece:cefactBieDomainClass": "cefact:Logistics_TransportMovement.Details",
                    "rdfs:comment": "The number of packages in this logistics transport movement."
                },
                {
                    "@id": "cefact:SupplyChain_ConsignmentItem.Package.Quantity",
                    "@type": "unece:BasicBIE",
                    "unece:TDED": "7012",
                    "unece:cefactUNId": "UN01010139",
                    "unece:cefactBieDomainClass": "cefact:SupplyChain_ConsignmentItem.Details",
                    "rdfs:comment": "The package quantity for this supply chain consignment item."
                },
                {
                    "@id": "cefact:SupplyChain_Consignment.Package.Quantity",
                    "@type": "unece:BasicBIE",
                    "unece:TDED": "7370",
                    "unece:cefactUNId": "UN01004197",
                    "unece:cefactBieDomainClass": "cefact:SupplyChain_Consignment.Details",
                    "rdfs:comment": "The number of packages within this supply chain consignment."
                }
            ]
        },
        {
            "@id": "transport:packageType",
            "@type": "rdf:Property",
            "schema:rangeIncludes": {
                "@id": "xsd:string"
            },
            "schema:domainIncludes": [
                {
                    "@id": "transport:SupplyChainConsignment"
                },
                {
                    "@id": "transport:SupplyChainConsignmentItem"
                }
            ],
            "rdfs:comment": [
                "A package type, expressed as text, for this supply chain consignment item.",
                "A type of package, expressed as text, for this supply chain consignment."
            ],
            "rdfs:label": "packageType",
            "unece:cefactElementMetadata": [
                {
                    "@id": "cefact:SupplyChain_Consignment.PackageType.Text",
                    "@type": "unece:BasicBIE",
                    "unece:TDED": "7014",
                    "unece:cefactUNId": "UN01010142",
                    "unece:cefactBieDomainClass": "cefact:SupplyChain_Consignment.Details",
                    "rdfs:comment": "A type of package, expressed as text, for this supply chain consignment."
                },
                {
                    "@id": "cefact:SupplyChain_ConsignmentItem.PackageType.Text",
                    "@type": "unece:BasicBIE",
                    "unece:TDED": "7064",
                    "unece:cefactUNId": "UN01010140",
                    "unece:cefactBieDomainClass": "cefact:SupplyChain_ConsignmentItem.Details",
                    "rdfs:comment": "A package type, expressed as text, for this supply chain consignment item."
                }
            ]
        },
        {
            "@id": "transport:partialDeliveryAllowedIndicator",
            "@type": "rdf:Property",
            "schema:rangeIncludes": {
                "@id": "xsd:boolean"
            },
            "schema:domainIncludes": {
                "@id": ":TradeDeliveryTerms"
            },
            "rdfs:comment": "The indication of whether or not these trade delivery terms allow a partial delivery.",
            "rdfs:label": "partialDeliveryAllowedIndicator",
            "unece:cefactElementMetadata": [
                {
                    "@id": "cefact:Trade_DeliveryTerms.PartialDeliveryAllowed.Indicator",
                    "@type": "unece:BasicBIE",
                    "unece:cefactUNId": "UN01012763",
                    "unece:cefactBieDomainClass": "cefact:Trade_DeliveryTerms.Details",
                    "rdfs:comment": "The indication of whether or not these trade delivery terms allow a partial delivery."
                }
            ]
        },
        {
            "@id": "transport:passengerListRelatedDocument",
            "@type": "rdf:Property",
            "schema:rangeIncludes": {
                "@id": "transport:Document"
            },
            "schema:domainIncludes": {
                "@id": "transport:LogisticsTransportMovement"
            },
            "rdfs:comment": "The passenger list document related to this logistics transport movement.",
            "rdfs:label": "passengerListRelatedDocument",
            "unece:cefactElementMetadata": [
                {
                    "@id": "cefact:Logistics_TransportMovement.PassengerList_Related.Referenced_Document",
                    "@type": "unece:AssociationBIE",
                    "unece:cefactUNId": "UN01010136",
                    "unece:cefactBieDomainClass": "cefact:Logistics_TransportMovement.Details",
                    "rdfs:comment": "The passenger list document related to this logistics transport movement."
                }
            ]
        },
        {
            "@id": "transport:passengerNationalityCountry",
            "@type": "rdf:Property",
            "schema:rangeIncludes": {
                "@id": "transport:Country"
            },
            "schema:domainIncludes": {
                "@id": "transport:LogisticsTransportMovement"
            },
            "rdfs:comment": "Passenger nationality details for this logistics transport movement.",
            "rdfs:label": "passengerNationalityCountry",
            "unece:cefactElementMetadata": [
                {
                    "@id": "cefact:Logistics_TransportMovement.PassengerNationality.Trade_Country",
                    "@type": "unece:AssociationBIE",
                    "unece:cefactUNId": "UN01010126",
                    "unece:cefactBieDomainClass": "cefact:Logistics_TransportMovement.Details",
                    "rdfs:comment": "Passenger nationality details for this logistics transport movement."
                }
            ]
        },
        {
            "@id": "transport:passengerQuantity",
            "@type": "rdf:Property",
            "schema:rangeIncludes": {
                "@id": "xsd:decimal"
            },
            "schema:domainIncludes": {
                "@id": "transport:LogisticsTransportMovement"
            },
            "rdfs:comment": "The number of passengers for this logistics transport movement.",
            "rdfs:label": "passengerQuantity",
            "unece:cefactElementMetadata": [
                {
                    "@id": "cefact:Logistics_TransportMovement.Passenger.Quantity",
                    "@type": "unece:BasicBIE",
                    "unece:TDED": "7056",
                    "unece:cefactUNId": "UN01003849",
                    "unece:cefactBieDomainClass": "cefact:Logistics_TransportMovement.Details",
                    "rdfs:comment": "The number of passengers for this logistics transport movement."
                }
            ]
        },
        {
            "@id": "transport:physicalShippingMarks",
            "@type": "rdf:Property",
            "schema:rangeIncludes": {
                "@id": "transport:ShippingMarks"
            },
            "schema:domainIncludes": [
                {
                    "@id": "transport:Referenced_SupplyChainConsignmentItem"
                },
                {
                    "@id": "transport:SupplyChainConsignment"
                },
                {
                    "@id": "transport:SupplyChainConsignmentItem"
                }
            ],
            "rdfs:comment": [
                "Physical logistics shipping marks and barcode information for this referenced supply chain consignment item.",
                "Physical logistics shipping marks and barcode information for this supply chain consignment item.",
                "Physical logistics shipping marks and barcoding information related to this supply chain consignment."
            ],
            "rdfs:label": "physicalShippingMarks",
            "unece:cefactElementMetadata": [
                {
                    "@id": "cefact:Referenced_SupplyChain_ConsignmentItem.Physical.Logistics_ShippingMarks",
                    "@type": "unece:AssociationBIE",
                    "unece:cefactUNId": "UN01011046",
                    "unece:cefactBieDomainClass": "cefact:Referenced_SupplyChain_ConsignmentItem.Details",
                    "rdfs:comment": "Physical logistics shipping marks and barcode information for this referenced supply chain consignment item."
                },
                {
                    "@id": "cefact:SupplyChain_Consignment.Physical.Logistics_ShippingMarks",
                    "@type": "unece:AssociationBIE",
                    "unece:cefactUNId": "UN01004247",
                    "unece:cefactBieDomainClass": "cefact:SupplyChain_Consignment.Details",
                    "rdfs:comment": "Physical logistics shipping marks and barcoding information related to this supply chain consignment."
                },
                {
                    "@id": "cefact:SupplyChain_ConsignmentItem.Physical.Logistics_ShippingMarks",
                    "@type": "unece:AssociationBIE",
                    "unece:cefactUNId": "UN01004135",
                    "unece:cefactBieDomainClass": "cefact:SupplyChain_ConsignmentItem.Details",
                    "rdfs:comment": "Physical logistics shipping marks and barcode information for this supply chain consignment item."
                }
            ]
        },
        {
            "@id": "transport:pickUpEvent",
            "@type": "rdf:Property",
            "schema:rangeIncludes": {
                "@id": "transport:Event"
            },
            "schema:domainIncludes": [
                {
                    "@id": "transport:LogisticsTransportEquipment"
                },
                {
                    "@id": "transport:SupplyChainConsignment"
                },
                {
                    "@id": "transport:SupplyChainConsignmentItem"
                }
            ],
            "rdfs:comment": [
                "A pick-up event specifying when and where this piece of logistics transport equipment will be, or has been, collected, i.e. picked-up by the carrier.",
                "A pick-up transport event for this supply chain consignment item.",
                "The pick-up event for this supply chain consignment."
            ],
            "rdfs:label": "pickUpEvent",
            "unece:cefactElementMetadata": [
                {
                    "@id": "cefact:SupplyChain_Consignment.Pick-Up.Transport_Event",
                    "@type": "unece:AssociationBIE",
                    "unece:cefactUNId": "UN01004254",
                    "unece:cefactBieDomainClass": "cefact:SupplyChain_Consignment.Details",
                    "rdfs:comment": "The pick-up event for this supply chain consignment."
                },
                {
                    "@id": "cefact:SupplyChain_ConsignmentItem.Pick-Up.Transport_Event",
                    "@type": "unece:AssociationBIE",
                    "unece:cefactUNId": "UN01008999",
                    "unece:cefactBieDomainClass": "cefact:SupplyChain_ConsignmentItem.Details",
                    "rdfs:comment": "A pick-up transport event for this supply chain consignment item."
                },
                {
                    "@id": "cefact:Logistics_TransportEquipment.Pick-Up.Transport_Event",
                    "@type": "unece:AssociationBIE",
                    "unece:cefactUNId": "UN01003807",
                    "unece:cefactBieDomainClass": "cefact:Logistics_TransportEquipment.Details",
                    "rdfs:comment": "A pick-up event specifying when and where this piece of logistics transport equipment will be, or has been, collected, i.e. picked-up by the carrier."
                }
            ]
        },
        {
            "@id": "transport:pilotageExemptionId",
            "@type": "rdf:Property",
            "schema:rangeIncludes": {
                "@id": "xsd:token"
            },
            "schema:domainIncludes": {
                "@id": "transport:LogisticsTransportMovement"
            },
            "rdfs:comment": "The identifier of a pilotage exemption for this logistics transport movement.",
            "rdfs:label": "pilotageExemptionId",
            "unece:cefactElementMetadata": [
                {
                    "@id": "cefact:Logistics_TransportMovement.PilotageExemption.Identifier",
                    "@type": "unece:BasicBIE",
                    "unece:cefactUNId": "UN01010119",
                    "unece:cefactBieDomainClass": "cefact:Logistics_TransportMovement.Details",
                    "rdfs:comment": "The identifier of a pilotage exemption for this logistics transport movement."
                }
            ]
        },
        {
            "@id": "transport:pollutionMeasure",
            "@type": "rdf:Property",
            "schema:rangeIncludes": {
                "@id": "xsd:decimal"
            },
            "schema:domainIncludes": {
                "@id": "transport:CalculatedEmission"
            },
            "rdfs:comment": "A measure of the pollution calculated for this emission.",
            "rdfs:label": "pollutionMeasure",
            "unece:cefactElementMetadata": [
                {
                    "@id": "cefact:Calculated_Emission.Pollution.Measure",
                    "@type": "unece:BasicBIE",
                    "unece:cefactUNId": "UN01010055",
                    "unece:cefactBieDomainClass": "cefact:Calculated_Emission.Details",
                    "rdfs:comment": "A measure of the pollution calculated for this emission."
                }
            ]
        },
        {
            "@id": "transport:positioningEvent",
            "@type": "rdf:Property",
            "schema:rangeIncludes": {
                "@id": "transport:Event"
            },
            "schema:domainIncludes": {
                "@id": "transport:LogisticsTransportEquipment"
            },
            "rdfs:comment": "A positioning event specifying when and where this piece of logistics transport equipment will be, or has been, positioned, i.e. delivered and available for pick-up.",
            "rdfs:label": "positioningEvent",
            "unece:cefactElementMetadata": [
                {
                    "@id": "cefact:Logistics_TransportEquipment.Positioning.Transport_Event",
                    "@type": "unece:AssociationBIE",
                    "unece:cefactUNId": "UN01003806",
                    "unece:cefactBieDomainClass": "cefact:Logistics_TransportEquipment.Details",
                    "rdfs:comment": "A positioning event specifying when and where this piece of logistics transport equipment will be, or has been, positioned, i.e. delivered and available for pick-up."
                }
            ]
        },
        {
            "@id": "transport:powerSupplyConnectorQuantity",
            "@type": "rdf:Property",
            "schema:rangeIncludes": {
                "@id": "xsd:decimal"
            },
            "schema:domainIncludes": {
                "@id": "transport:LogisticsTransportEquipment"
            },
            "rdfs:comment": "The number of power supply connectors for this piece of logistics transport equipment.",
            "rdfs:label": "powerSupplyConnectorQuantity",
            "unece:cefactElementMetadata": [
                {
                    "@id": "cefact:Logistics_TransportEquipment.PowerSupplyConnector.Quantity",
                    "@type": "unece:BasicBIE",
                    "unece:cefactUNId": "UN01003782",
                    "unece:cefactBieDomainClass": "cefact:Logistics_TransportEquipment.Details",
                    "rdfs:comment": "The number of power supply connectors for this piece of logistics transport equipment."
                }
            ]
        },
        {
            "@id": "transport:powerSupplyType",
            "@type": "rdf:Property",
            "schema:rangeIncludes": {
                "@id": "xsd:string"
            },
            "schema:domainIncludes": {
                "@id": "transport:LogisticsTransportEquipment"
            },
            "rdfs:comment": "The type of power supply, expressed as text, for this piece of logistics transport equipment, such as diesel fuel or electricity.",
            "rdfs:label": "powerSupplyType",
            "unece:cefactElementMetadata": [
                {
                    "@id": "cefact:Logistics_TransportEquipment.PowerSupplyType.Text",
                    "@type": "unece:BasicBIE",
                    "unece:cefactUNId": "UN01003781",
                    "unece:cefactBieDomainClass": "cefact:Logistics_TransportEquipment.Details",
                    "rdfs:comment": "The type of power supply, expressed as text, for this piece of logistics transport equipment, such as diesel fuel or electricity."
                }
            ]
        },
        {
            "@id": "transport:powerSupplyTypeCode",
            "@type": "rdf:Property",
            "schema:rangeIncludes": {
                "@id": "xsd:token"
            },
            "schema:domainIncludes": {
                "@id": "transport:LogisticsTransportEquipment"
            },
            "rdfs:comment": "The code specifying the type of power supply for this piece of logistics transport equipment, such as diesel fuel or electricity.",
            "rdfs:label": "powerSupplyTypeCode",
            "unece:cefactElementMetadata": [
                {
                    "@id": "cefact:Logistics_TransportEquipment.PowerSupplyType.Code",
                    "@type": "unece:BasicBIE",
                    "unece:cefactUNId": "UN01003780",
                    "unece:cefactBieDomainClass": "cefact:Logistics_TransportEquipment.Details",
                    "rdfs:comment": "The code specifying the type of power supply for this piece of logistics transport equipment, such as diesel fuel or electricity."
                }
            ]
        },
        {
            "@id": "transport:preCarriageTransportMovement",
            "@type": "rdf:Property",
            "schema:rangeIncludes": {
                "@id": "transport:TransportMovement"
            },
            "schema:domainIncludes": [
                {
                    "@id": "transport:LogisticsTransportEquipment"
                },
                {
                    "@id": "transport:Referenced_SupplyChainConsignment"
                },
                {
                    "@id": "transport:SupplyChainConsignment"
                }
            ],
            "rdfs:comment": [
                "A pre-carriage logistics transport movement for this referenced supply chain consignment.",
                "A pre-carriage logistics transport movement for this supply chain consignment.",
                "A pre-carriage transport movement for this piece of logistics transport equipment."
            ],
            "rdfs:label": "preCarriageTransportMovement",
            "unece:cefactElementMetadata": [
                {
                    "@id": "cefact:Logistics_TransportEquipment.Pre-Carriage.Logistics_TransportMovement",
                    "@type": "unece:AssociationBIE",
                    "unece:cefactUNId": "UN01003815",
                    "unece:cefactBieDomainClass": "cefact:Logistics_TransportEquipment.Details",
                    "rdfs:comment": "A pre-carriage transport movement for this piece of logistics transport equipment."
                },
                {
                    "@id": "cefact:Referenced_SupplyChain_Consignment.Pre-Carriage.Logistics_TransportMovement",
                    "@type": "unece:AssociationBIE",
                    "unece:cefactUNId": "UN01011066",
                    "unece:cefactBieDomainClass": "cefact:Referenced_SupplyChain_Consignment.Details",
                    "rdfs:comment": "A pre-carriage logistics transport movement for this referenced supply chain consignment."
                },
                {
                    "@id": "cefact:SupplyChain_Consignment.Pre-Carriage.Logistics_TransportMovement",
                    "@type": "unece:AssociationBIE",
                    "unece:cefactUNId": "UN01004262",
                    "unece:cefactBieDomainClass": "cefact:SupplyChain_Consignment.Details",
                    "rdfs:comment": "A pre-carriage logistics transport movement for this supply chain consignment."
                }
            ]
        },
        {
            "@id": "transport:previousAdministrativeDocument",
            "@type": "rdf:Property",
            "schema:rangeIncludes": {
                "@id": "transport:Document"
            },
            "schema:domainIncludes": [
                {
                    "@id": "transport:SupplyChainConsignment"
                },
                {
                    "@id": "transport:SupplyChainConsignmentItem"
                }
            ],
            "rdfs:comment": [
                "A previous administrative referenced document for this supply chain consignment item.",
                "A previous administrative referenced document for this supply chain consignment."
            ],
            "rdfs:label": "previousAdministrativeDocument",
            "unece:cefactElementMetadata": [
                {
                    "@id": "cefact:SupplyChain_ConsignmentItem.PreviousAdministrative.Referenced_Document",
                    "@type": "unece:AssociationBIE",
                    "unece:cefactUNId": "UN01012576",
                    "unece:cefactBieDomainClass": "cefact:SupplyChain_ConsignmentItem.Details",
                    "rdfs:comment": "A previous administrative referenced document for this supply chain consignment item."
                },
                {
                    "@id": "cefact:SupplyChain_Consignment.PreviousAdministrative.Referenced_Document",
                    "@type": "unece:AssociationBIE",
                    "unece:cefactUNId": "UN01012580",
                    "unece:cefactBieDomainClass": "cefact:SupplyChain_Consignment.Details",
                    "rdfs:comment": "A previous administrative referenced document for this supply chain consignment."
                }
            ]
        },
        {
            "@id": "transport:professionalMedicalPersonnelOnboardQuantity",
            "@type": "rdf:Property",
            "schema:rangeIncludes": {
                "@id": "xsd:decimal"
            },
            "schema:domainIncludes": {
                "@id": "transport:LogisticsTransportMovement"
            },
            "rdfs:comment": "The number of professional medical personnel onboard this logistics transport movement.",
            "rdfs:label": "professionalMedicalPersonnelOnboardQuantity",
            "unece:cefactElementMetadata": [
                {
                    "@id": "cefact:Logistics_TransportMovement.Professional_MedicalPersonnelOnboard.Quantity",
                    "@type": "unece:BasicBIE",
                    "unece:cefactUNId": "UN01015085",
                    "unece:cefactBieDomainClass": "cefact:Logistics_TransportMovement.Details",
                    "rdfs:comment": "The number of professional medical personnel onboard this logistics transport movement."
                }
            ]
        },
        {
            "@id": "transport:quarantineInstructions",
            "@type": "rdf:Property",
            "schema:rangeIncludes": {
                "@id": "transport:Instructions"
            },
            "schema:domainIncludes": [
                {
                    "@id": "transport:LogisticsTransportEquipment"
                },
                {
                    "@id": "transport:SupplyChainConsignmentItem"
                }
            ],
            "rdfs:comment": [
                "Quarantine instructions for this piece of logistics transport equipment.",
                "Quarantine instructions for this supply chain consignment item."
            ],
            "rdfs:label": "quarantineInstructions",
            "unece:cefactElementMetadata": [
                {
                    "@id": "cefact:Logistics_TransportEquipment.Quarantine.Quarantine_Instructions",
                    "@type": "unece:AssociationBIE",
                    "unece:cefactUNId": "UN01003788",
                    "unece:cefactBieDomainClass": "cefact:Logistics_TransportEquipment.Details",
                    "rdfs:comment": "Quarantine instructions for this piece of logistics transport equipment."
                },
                {
                    "@id": "cefact:SupplyChain_ConsignmentItem.Quarantine.Quarantine_Instructions",
                    "@type": "unece:AssociationBIE",
                    "unece:cefactUNId": "UN01004133",
                    "unece:cefactBieDomainClass": "cefact:SupplyChain_ConsignmentItem.Details",
                    "rdfs:comment": "Quarantine instructions for this supply chain consignment item."
                }
            ]
        },
        {
            "@id": "transport:rFIDLabel",
            "@type": "rdf:Property",
            "schema:rangeIncludes": {
                "@id": "transport:Label"
            },
            "schema:domainIncludes": {
                "@id": "transport:LogisticsShippingMarks"
            },
            "rdfs:comment": "A Radio Frequency Identification (RFID) label that is a part of these logistics shipping marks.",
            "rdfs:label": "rFIDLabel",
            "unece:cefactElementMetadata": [
                {
                    "@id": "cefact:Logistics_ShippingMarks.RFID.Logistics_Label",
                    "@type": "unece:AssociationBIE",
                    "unece:cefactUNId": "UN01003745",
                    "unece:cefactBieDomainClass": "cefact:Logistics_ShippingMarks.Details",
                    "rdfs:comment": "A Radio Frequency Identification (RFID) label that is a part of these logistics shipping marks."
                }
            ]
        },
        {
            "@id": "transport:radioactiveIndicator",
            "@type": "rdf:Property",
            "schema:rangeIncludes": {
                "@id": "xsd:boolean"
            },
            "schema:domainIncludes": {
                "@id": ":TransportDangerousGoods"
            },
            "rdfs:comment": "The indicator of whether or not these transported dangerous goods are radioactive.",
            "rdfs:label": "radioactiveIndicator",
            "unece:cefactElementMetadata": [
                {
                    "@id": "cefact:Transport_DangerousGoods.Radioactive.Indicator",
                    "@type": "unece:BasicBIE",
                    "unece:cefactUNId": "UN01014760",
                    "unece:cefactBieDomainClass": "cefact:Transport_DangerousGoods.Details",
                    "rdfs:comment": "The indicator of whether or not these transported dangerous goods are radioactive."
                }
            ]
        },
        {
            "@id": "transport:radioactiveLabel",
            "@type": "rdf:Property",
            "schema:rangeIncludes": {
                "@id": "transport:Label"
            },
            "schema:domainIncludes": {
                "@id": "transport:LogisticsShippingMarks"
            },
            "rdfs:comment": "Radioactive labelling that is a part of these logistics shipping marks.",
            "rdfs:label": "radioactiveLabel",
            "unece:cefactElementMetadata": [
                {
                    "@id": "cefact:Logistics_ShippingMarks.Radioactive.Logistics_Label",
                    "@type": "unece:AssociationBIE",
                    "unece:cefactUNId": "UN01014744",
                    "unece:cefactBieDomainClass": "cefact:Logistics_ShippingMarks.Details",
                    "rdfs:comment": "Radioactive labelling that is a part of these logistics shipping marks."
                }
            ]
        },
        {
            "@id": "transport:reExportCountry",
            "@type": "rdf:Property",
            "schema:rangeIncludes": {
                "@id": "transport:Country"
            },
            "schema:domainIncludes": {
                "@id": "transport:SupplyChainConsignment"
            },
            "rdfs:comment": "A re-export country for this supply chain consignment.",
            "rdfs:label": "reExportCountry",
            "unece:cefactElementMetadata": [
                {
                    "@id": "cefact:SupplyChain_Consignment.Re-Export.Trade_Country",
                    "@type": "unece:AssociationBIE",
                    "unece:cefactUNId": "UN01004274",
                    "unece:cefactBieDomainClass": "cefact:SupplyChain_Consignment.Details",
                    "rdfs:comment": "A re-export country for this supply chain consignment."
                }
            ]
        },
        {
            "@id": "transport:reasonCode",
            "@type": "rdf:Property",
            "schema:rangeIncludes": {
                "@id": "xsd:token"
            },
            "schema:domainIncludes": {
                "@id": "transport:LogisticsTransportMovement"
            },
            "rdfs:comment": "The code specifying the reason for this logistics transport movement.",
            "rdfs:label": "reasonCode",
            "unece:cefactElementMetadata": [
                {
                    "@id": "cefact:Logistics_TransportMovement.Reason.Code",
                    "@type": "unece:BasicBIE",
                    "unece:cefactUNId": "UN01013835",
                    "unece:cefactBieDomainClass": "cefact:Logistics_TransportMovement.Details",
                    "rdfs:comment": "The code specifying the reason for this logistics transport movement."
                }
            ]
        },
        {
            "@id": "transport:recyclableIndicator",
            "@type": "rdf:Property",
            "schema:rangeIncludes": {
                "@id": "xsd:boolean"
            },
            "schema:domainIncludes": {
                "@id": "transport:SupplyChainPackaging"
            },
            "rdfs:comment": "The indication of whether or not this supply chain packaging is recyclable.",
            "rdfs:label": "recyclableIndicator",
            "unece:cefactElementMetadata": [
                {
                    "@id": "cefact:SupplyChain_Packaging.Recyclable.Indicator",
                    "@type": "unece:BasicBIE",
                    "unece:cefactUNId": "UN01014458",
                    "unece:cefactBieDomainClass": "cefact:SupplyChain_Packaging.Details",
                    "rdfs:comment": "The indication of whether or not this supply chain packaging is recyclable."
                }
            ]
        },
        {
            "@id": "transport:recycledMaterialIndicator",
            "@type": "rdf:Property",
            "schema:rangeIncludes": {
                "@id": "xsd:boolean"
            },
            "schema:domainIncludes": {
                "@id": "transport:SupplyChainPackaging"
            },
            "rdfs:comment": "The indication of whether or not this supply chain packaging is made of recycled material.",
            "rdfs:label": "recycledMaterialIndicator",
            "unece:cefactElementMetadata": [
                {
                    "@id": "cefact:SupplyChain_Packaging.RecycledMaterial.Indicator",
                    "@type": "unece:BasicBIE",
                    "unece:cefactUNId": "UN01014457",
                    "unece:cefactBieDomainClass": "cefact:SupplyChain_Packaging.Details",
                    "rdfs:comment": "The indication of whether or not this supply chain packaging is made of recycled material."
                }
            ]
        },
        {
            "@id": "transport:recycledMaterialPercent",
            "@type": "rdf:Property",
            "schema:rangeIncludes": {
                "@id": "xsd:decimal"
            },
            "schema:domainIncludes": {
                "@id": "transport:SupplyChainPackaging"
            },
            "rdfs:comment": "The percentage of recycled material in this supply chain packaging.",
            "rdfs:label": "recycledMaterialPercent",
            "unece:cefactElementMetadata": [
                {
                    "@id": "cefact:SupplyChain_Packaging.RecycledMaterial.Percent",
                    "@type": "unece:BasicBIE",
                    "unece:cefactUNId": "UN01014459",
                    "unece:cefactBieDomainClass": "cefact:SupplyChain_Packaging.Details",
                    "rdfs:comment": "The percentage of recycled material in this supply chain packaging."
                }
            ]
        },
        {
            "@id": "transport:registrationCountry",
            "@type": "rdf:Property",
            "schema:rangeIncludes": {
                "@id": "transport:Country"
            },
            "schema:domainIncludes": {
                "@id": "transport:LogisticsTransportMeans"
            },
            "rdfs:comment": "The country of registration of this logistics means of transport.",
            "rdfs:label": "registrationCountry",
            "unece:cefactElementMetadata": [
                {
                    "@id": "cefact:Logistics_TransportMeans.Registration.Trade_Country",
                    "@type": "unece:AssociationBIE",
                    "unece:cefactUNId": "UN01003834",
                    "unece:cefactBieDomainClass": "cefact:Logistics_TransportMeans.Details",
                    "rdfs:comment": "The country of registration of this logistics means of transport."
                }
            ]
        },
        {
            "@id": "transport:registrationEvent",
            "@type": "rdf:Property",
            "schema:rangeIncludes": {
                "@id": "transport:Event"
            },
            "schema:domainIncludes": {
                "@id": "transport:LogisticsTransportMeans"
            },
            "rdfs:comment": "A registration event of this logistics transport means.",
            "rdfs:label": "registrationEvent",
            "unece:cefactElementMetadata": [
                {
                    "@id": "cefact:Logistics_TransportMeans.Registration.Transport_Event",
                    "@type": "unece:AssociationBIE",
                    "unece:cefactUNId": "UN01010114",
                    "unece:cefactBieDomainClass": "cefact:Logistics_TransportMeans.Details",
                    "rdfs:comment": "A registration event of this logistics transport means."
                }
            ]
        },
        {
            "@id": "transport:relatedBookingType",
            "@type": "rdf:Property",
            "schema:rangeIncludes": {
                "@id": "xsd:string"
            },
            "schema:domainIncludes": {
                "@id": "transport:SupplyChainConsignment"
            },
            "rdfs:comment": "The type of booking, expressed as text, related to this supply chain consignment.",
            "rdfs:label": "relatedBookingType",
            "unece:cefactElementMetadata": [
                {
                    "@id": "cefact:SupplyChain_Consignment.RelatedBookingType.Text",
                    "@type": "unece:BasicBIE",
                    "unece:cefactUNId": "UN01013606",
                    "unece:cefactBieDomainClass": "cefact:SupplyChain_Consignment.Details",
                    "rdfs:comment": "The type of booking, expressed as text, related to this supply chain consignment."
                }
            ]
        },
        {
            "@id": "transport:relatedCustomsProcedure",
            "@type": "rdf:Property",
            "schema:rangeIncludes": {
                "@id": "transport:CustomsProcedure"
            },
            "schema:domainIncludes": {
                "@id": "transport:LogisticsTransportMovement"
            },
            "rdfs:comment": "A cross-border customs procedure related to this logistics transport movement, such as any procedure based on the World Customs Organization Data Model.",
            "rdfs:label": "relatedCustomsProcedure",
            "unece:cefactElementMetadata": [
                {
                    "@id": "cefact:Logistics_TransportMovement.Related.Cross-Border_CustomsProcedure",
                    "@type": "unece:AssociationBIE",
                    "unece:cefactUNId": "UN01003876",
                    "unece:cefactBieDomainClass": "cefact:Logistics_TransportMovement.Details",
                    "rdfs:comment": "A cross-border customs procedure related to this logistics transport movement, such as any procedure based on the World Customs Organization Data Model."
                }
            ]
        },
        {
            "@id": "transport:relatedEvent",
            "@type": "rdf:Property",
            "schema:rangeIncludes": {
                "@id": "transport:Event"
            },
            "schema:domainIncludes": {
                "@id": "transport:LogisticsTransportEquipment"
            },
            "rdfs:comment": "A communication event related to this piece of logistics transport equipment.",
            "rdfs:label": "relatedEvent",
            "unece:cefactElementMetadata": [
                {
                    "@id": "cefact:Logistics_TransportEquipment.Related.Communication_Event",
                    "@type": "unece:AssociationBIE",
                    "unece:cefactUNId": "UN01013594",
                    "unece:cefactBieDomainClass": "cefact:Logistics_TransportEquipment.Details",
                    "rdfs:comment": "A communication event related to this piece of logistics transport equipment."
                }
            ]
        },
        {
            "@id": "transport:relatedTradeTransaction",
            "@type": "rdf:Property",
            "schema:rangeIncludes": {
                "@id": "transport:TradeTransaction"
            },
            "schema:domainIncludes": [
                {
                    "@id": "transport:Referenced_SupplyChainConsignment"
                },
                {
                    "@id": "transport:SupplyChainConsignment"
                }
            ],
            "rdfs:comment": [
                "A trade transaction related to this referenced supply chain consignment.",
                "A trade transaction related to this supply chain consignment."
            ],
            "rdfs:label": "relatedTradeTransaction",
            "unece:cefactElementMetadata": [
                {
                    "@id": "cefact:SupplyChain_Consignment.Related.SupplyChain_TradeTransaction",
                    "@type": "unece:AssociationBIE",
                    "unece:cefactUNId": "UN01004289",
                    "unece:cefactBieDomainClass": "cefact:SupplyChain_Consignment.Details",
                    "rdfs:comment": "A trade transaction related to this supply chain consignment."
                },
                {
                    "@id": "cefact:Referenced_SupplyChain_Consignment.Related.SupplyChain_TradeTransaction",
                    "@type": "unece:AssociationBIE",
                    "unece:cefactUNId": "UN01011060",
                    "unece:cefactBieDomainClass": "cefact:Referenced_SupplyChain_Consignment.Details",
                    "rdfs:comment": "A trade transaction related to this referenced supply chain consignment."
                }
            ]
        },
        {
            "@id": "transport:releaseId",
            "@type": "rdf:Property",
            "schema:rangeIncludes": {
                "@id": "xsd:token"
            },
            "schema:domainIncludes": {
                "@id": "transport:LogisticsTransportEquipment"
            },
            "rdfs:comment": "The release identifier for this piece of logistics transport equipment.",
            "rdfs:label": "releaseId",
            "unece:cefactElementMetadata": [
                {
                    "@id": "cefact:Logistics_TransportEquipment.Release.Identifier",
                    "@type": "unece:BasicBIE",
                    "unece:cefactUNId": "UN01003784",
                    "unece:cefactBieDomainClass": "cefact:Logistics_TransportEquipment.Details",
                    "rdfs:comment": "The release identifier for this piece of logistics transport equipment."
                }
            ]
        },
        {
            "@id": "transport:releaseRestriction",
            "@type": "rdf:Property",
            "schema:rangeIncludes": {
                "@id": "xsd:string"
            },
            "schema:domainIncludes": {
                "@id": "transport:LogisticsTransportEquipment"
            },
            "rdfs:comment": "The release restriction, expressed as text, for this piece of logistics transport equipment.",
            "rdfs:label": "releaseRestriction",
            "unece:cefactElementMetadata": [
                {
                    "@id": "cefact:Logistics_TransportEquipment.ReleaseRestriction.Text",
                    "@type": "unece:BasicBIE",
                    "unece:cefactUNId": "UN01003785",
                    "unece:cefactBieDomainClass": "cefact:Logistics_TransportEquipment.Details",
                    "rdfs:comment": "The release restriction, expressed as text, for this piece of logistics transport equipment."
                }
            ]
        },
        {
            "@id": "transport:reportedMaterial",
            "@type": "rdf:Property",
            "schema:rangeIncludes": {
                "@id": "transport:Material"
            },
            "schema:domainIncludes": {
                "@id": "transport:LogisticsTransportMovement"
            },
            "rdfs:comment": "Transportation waste material reported for this logistics transport movement.",
            "rdfs:label": "reportedMaterial",
            "unece:cefactElementMetadata": [
                {
                    "@id": "cefact:Logistics_TransportMovement.Reported.TransportationWaste_Material",
                    "@type": "unece:AssociationBIE",
                    "unece:cefactUNId": "UN01013177",
                    "unece:cefactBieDomainClass": "cefact:Logistics_TransportMovement.Details",
                    "rdfs:comment": "Transportation waste material reported for this logistics transport movement."
                }
            ]
        },
        {
            "@id": "transport:reportedSecurityInformation",
            "@type": "rdf:Property",
            "schema:rangeIncludes": {
                "@id": "xsd:string"
            },
            "schema:domainIncludes": {
                "@id": "transport:LogisticsTransportMovement"
            },
            "rdfs:comment": "Reported security information, expressed as text, for this logistics transport movement.",
            "rdfs:label": "reportedSecurityInformation",
            "unece:cefactElementMetadata": [
                {
                    "@id": "cefact:Logistics_TransportMovement.ReportedSecurity_Information.Text",
                    "@type": "unece:BasicBIE",
                    "unece:TDED": "4032",
                    "unece:cefactUNId": "UN01013172",
                    "unece:cefactBieDomainClass": "cefact:Logistics_TransportMovement.Details",
                    "rdfs:comment": "Reported security information, expressed as text, for this logistics transport movement."
                }
            ]
        },
        {
            "@id": "transport:reportedStatus",
            "@type": "rdf:Property",
            "schema:rangeIncludes": {
                "@id": "transport:Status"
            },
            "schema:domainIncludes": [
                {
                    "@id": "transport:LogisticsTransportEquipment"
                },
                {
                    "@id": "transport:SupplyChainConsignment"
                },
                {
                    "@id": "transport:SupplyChainConsignmentItem"
                }
            ],
            "rdfs:comment": [
                "A logistics status reported for this supply chain consignment item.",
                "A logistics status reported for this supply chain consignment.",
                "A status reported for this piece of logistics transport equipment."
            ],
            "rdfs:label": "reportedStatus",
            "unece:cefactElementMetadata": [
                {
                    "@id": "cefact:Logistics_TransportEquipment.Reported.Logistics_Status",
                    "@type": "unece:AssociationBIE",
                    "unece:cefactUNId": "UN01003818",
                    "unece:cefactBieDomainClass": "cefact:Logistics_TransportEquipment.Details",
                    "rdfs:comment": "A status reported for this piece of logistics transport equipment."
                },
                {
                    "@id": "cefact:SupplyChain_ConsignmentItem.Reported.Logistics_Status",
                    "@type": "unece:AssociationBIE",
                    "unece:cefactUNId": "UN01004155",
                    "unece:cefactBieDomainClass": "cefact:SupplyChain_ConsignmentItem.Details",
                    "rdfs:comment": "A logistics status reported for this supply chain consignment item."
                },
                {
                    "@id": "cefact:SupplyChain_Consignment.Reported.Logistics_Status",
                    "@type": "unece:AssociationBIE",
                    "unece:cefactUNId": "UN01004288",
                    "unece:cefactBieDomainClass": "cefact:SupplyChain_Consignment.Details",
                    "rdfs:comment": "A logistics status reported for this supply chain consignment."
                }
            ]
        },
        {
            "@id": "transport:reportingIOTDeviceEvent",
            "@type": "rdf:Property",
            "schema:rangeIncludes": {
                "@id": "transport:Event"
            },
            "schema:domainIncludes": {
                "@id": "transport:LogisticsTransportEquipment"
            },
            "rdfs:comment": "An IOT device reported transport event for this piece of logistics transport equipment.",
            "rdfs:label": "reportingIOTDeviceEvent",
            "unece:cefactElementMetadata": [
                {
                    "@id": "cefact:Logistics_TransportEquipment.Reporting_IOTDevice.Transport_Event",
                    "@type": "unece:AssociationBIE",
                    "unece:cefactUNId": "UN01013593",
                    "unece:cefactBieDomainClass": "cefact:Logistics_TransportEquipment.Details",
                    "rdfs:comment": "An IOT device reported transport event for this piece of logistics transport equipment."
                }
            ]
        },
        {
            "@id": "transport:reportingIOTDevicePairing",
            "@type": "rdf:Property",
            "schema:rangeIncludes": {
                "@id": "transport:Pairing"
            },
            "schema:domainIncludes": {
                "@id": "transport:LogisticsTransportEquipment"
            },
            "rdfs:comment": "An IOT device reported communication pairing for this piece of logistics transport equipment.",
            "rdfs:label": "reportingIOTDevicePairing",
            "unece:cefactElementMetadata": [
                {
                    "@id": "cefact:Logistics_TransportEquipment.Reporting_IOTDevice.Communication_Pairing",
                    "@type": "unece:AssociationBIE",
                    "unece:cefactUNId": "UN01013592",
                    "unece:cefactBieDomainClass": "cefact:Logistics_TransportEquipment.Details",
                    "rdfs:comment": "An IOT device reported communication pairing for this piece of logistics transport equipment."
                }
            ]
        },
        {
            "@id": "transport:requestedRoute",
            "@type": "rdf:Property",
            "schema:rangeIncludes": {
                "@id": "transport:Route"
            },
            "schema:domainIncludes": {
                "@id": "transport:LogisticsTransportEquipment"
            },
            "rdfs:comment": "A requested route for this piece of logistics transport equipment.",
            "rdfs:label": "requestedRoute",
            "unece:cefactElementMetadata": [
                {
                    "@id": "cefact:Logistics_TransportEquipment.Requested.Transport_Route",
                    "@type": "unece:AssociationBIE",
                    "unece:cefactUNId": "UN01013596",
                    "unece:cefactBieDomainClass": "cefact:Logistics_TransportEquipment.Details",
                    "rdfs:comment": "A requested route for this piece of logistics transport equipment."
                }
            ]
        },
        {
            "@id": "transport:requiredLaneLengthMeasure",
            "@type": "rdf:Property",
            "schema:rangeIncludes": {
                "@id": "xsd:decimal"
            },
            "schema:domainIncludes": [
                {
                    "@id": "transport:LogisticsTransportEquipment"
                },
                {
                    "@id": "transport:LogisticsTransportMeans"
                }
            ],
            "rdfs:comment": [
                "The measure of the external length required in a lane for this logistics transport means.",
                "The measure of the length required in a lane for this piece of logistics transport equipment."
            ],
            "rdfs:label": "requiredLaneLengthMeasure",
            "unece:cefactElementMetadata": [
                {
                    "@id": "cefact:Logistics_TransportEquipment.RequiredLaneLength.Measure",
                    "@type": "unece:BasicBIE",
                    "unece:TDED": "6046",
                    "unece:cefactUNId": "UN01003763",
                    "unece:cefactBieDomainClass": "cefact:Logistics_TransportEquipment.Details",
                    "rdfs:comment": "The measure of the length required in a lane for this piece of logistics transport equipment."
                },
                {
                    "@id": "cefact:Logistics_TransportMeans.RequiredLaneLength.Measure",
                    "@type": "unece:BasicBIE",
                    "unece:cefactUNId": "UN01003829",
                    "unece:cefactBieDomainClass": "cefact:Logistics_TransportMeans.Details",
                    "rdfs:comment": "The measure of the external length required in a lane for this logistics transport means."
                }
            ]
        },
        {
            "@id": "transport:requiredService",
            "@type": "rdf:Property",
            "schema:rangeIncludes": {
                "@id": "transport:Service"
            },
            "schema:domainIncludes": {
                "@id": "transport:LogisticsTransportMeans"
            },
            "rdfs:comment": "A transport service required for this logistics means of transport.",
            "rdfs:label": "requiredService",
            "unece:cefactElementMetadata": [
                {
                    "@id": "cefact:Logistics_TransportMeans.Required.Transport_Service",
                    "@type": "unece:AssociationBIE",
                    "unece:cefactUNId": "UN01010113",
                    "unece:cefactBieDomainClass": "cefact:Logistics_TransportMeans.Details",
                    "rdfs:comment": "A transport service required for this logistics means of transport."
                }
            ]
        },
        {
            "@id": "transport:returnableIndicator",
            "@type": "rdf:Property",
            "schema:rangeIncludes": {
                "@id": "xsd:boolean"
            },
            "schema:domainIncludes": [
                {
                    "@id": "transport:LogisticsPackaging"
                },
                {
                    "@id": "transport:LogisticsTransportEquipment"
                },
                {
                    "@id": "transport:SupplyChainPackaging"
                },
                {
                    "@id": "transport:TradeProduct_SupplyChainPackaging"
                }
            ],
            "rdfs:comment": [
                "The indication of whether or not this logistics packaging is returnable.",
                "The indication of whether or not this piece of logistics transport equipment is returnable.",
                "The indication of whether or not this supply chain packaging is returnable.",
                "The indication of whether or not this trade product supply chain packaging is returnable."
            ],
            "rdfs:label": "returnableIndicator",
            "unece:cefactElementMetadata": [
                {
                    "@id": "cefact:TradeProduct_SupplyChain_Packaging.Returnable.Indicator",
                    "@type": "unece:BasicBIE",
                    "unece:cefactUNId": "UN01007481",
                    "unece:cefactBieDomainClass": "cefact:TradeProduct_SupplyChain_Packaging.Details",
                    "rdfs:comment": "The indication of whether or not this trade product supply chain packaging is returnable."
                },
                {
                    "@id": "cefact:SupplyChain_Packaging.Returnable.Indicator",
                    "@type": "unece:BasicBIE",
                    "unece:cefactUNId": "UN01006751",
                    "unece:cefactBieDomainClass": "cefact:SupplyChain_Packaging.Details",
                    "rdfs:comment": "The indication of whether or not this supply chain packaging is returnable."
                },
                {
                    "@id": "cefact:Logistics_Packaging.Returnable.Indicator",
                    "@type": "unece:BasicBIE",
                    "unece:cefactUNId": "UN01014960",
                    "unece:cefactBieDomainClass": "cefact:Logistics_Packaging.Details",
                    "rdfs:comment": "The indication of whether or not this logistics packaging is returnable."
                },
                {
                    "@id": "cefact:Logistics_TransportEquipment.Returnable.Indicator",
                    "@type": "unece:BasicBIE",
                    "unece:cefactUNId": "UN01012583",
                    "unece:cefactBieDomainClass": "cefact:Logistics_TransportEquipment.Details",
                    "rdfs:comment": "The indication of whether or not this piece of logistics transport equipment is returnable."
                }
            ]
        },
        {
            "@id": "transport:riskFactorCode",
            "@type": "rdf:Property",
            "schema:rangeIncludes": {
                "@id": "xsd:token"
            },
            "schema:domainIncludes": {
                "@id": "transport:SupplyChainConsignment"
            },
            "rdfs:comment": "The code specifying a risk factor for this supply chain consignment.",
            "rdfs:label": "riskFactorCode",
            "unece:cefactElementMetadata": [
                {
                    "@id": "cefact:SupplyChain_Consignment.RiskFactor.Code",
                    "@type": "unece:BasicBIE",
                    "unece:cefactUNId": "UN01004211",
                    "unece:cefactBieDomainClass": "cefact:SupplyChain_Consignment.Details",
                    "rdfs:comment": "The code specifying a risk factor for this supply chain consignment."
                }
            ]
        },
        {
            "@id": "transport:riskResponsibilityCode",
            "@type": "rdf:Property",
            "schema:rangeIncludes": {
                "@id": "xsd:token"
            },
            "schema:domainIncludes": {
                "@id": ":TradeDeliveryTerms"
            },
            "rdfs:comment": "A code specifying the risk responsibility for these trade delivery terms.",
            "rdfs:label": "riskResponsibilityCode",
            "unece:cefactElementMetadata": [
                {
                    "@id": "cefact:Trade_DeliveryTerms.RiskResponsibility.Code",
                    "@type": "unece:BasicBIE",
                    "unece:cefactUNId": "UN01004586",
                    "unece:cefactBieDomainClass": "cefact:Trade_DeliveryTerms.Details",
                    "rdfs:comment": "A code specifying the risk responsibility for these trade delivery terms."
                }
            ]
        },
        {
            "@id": "transport:sailingAdviceNotificationInformation",
            "@type": "rdf:Property",
            "schema:rangeIncludes": {
                "@id": "xsd:string"
            },
            "schema:domainIncludes": {
                "@id": "transport:LogisticsTransportMovement"
            },
            "rdfs:comment": "Sailing advice notification information, expressed as text, for this logistics transport movement.",
            "rdfs:label": "sailingAdviceNotificationInformation",
            "unece:cefactElementMetadata": [
                {
                    "@id": "cefact:Logistics_TransportMovement.SailingAdviceNotification_Information.Text",
                    "@type": "unece:BasicBIE",
                    "unece:TDED": "4032",
                    "unece:cefactUNId": "UN01003853",
                    "unece:cefactBieDomainClass": "cefact:Logistics_TransportMovement.Details",
                    "rdfs:comment": "Sailing advice notification information, expressed as text, for this logistics transport movement."
                }
            ]
        },
        {
            "@id": "transport:sailingAdviceNotifiedParty",
            "@type": "rdf:Property",
            "schema:rangeIncludes": {
                "@id": "transport:Party"
            },
            "schema:domainIncludes": {
                "@id": "transport:LogisticsTransportMovement"
            },
            "rdfs:comment": "A party to be notified of the sailing advice for this logistics transport movement.",
            "rdfs:label": "sailingAdviceNotifiedParty",
            "unece:cefactElementMetadata": [
                {
                    "@id": "cefact:Logistics_TransportMovement.SailingAdvice_Notified.Trade_Party",
                    "@type": "unece:AssociationBIE",
                    "unece:cefactUNId": "UN01003875",
                    "unece:cefactBieDomainClass": "cefact:Logistics_TransportMovement.Details",
                    "rdfs:comment": "A party to be notified of the sailing advice for this logistics transport movement."
                }
            ]
        },
        {
            "@id": "transport:scheduledId",
            "@type": "rdf:Property",
            "schema:rangeIncludes": {
                "@id": "xsd:token"
            },
            "schema:domainIncludes": {
                "@id": "transport:LogisticsTransportMovement"
            },
            "rdfs:comment": "A unique identifier for this logistics transport movement, such as a voyage number, flight number, or trip number, as stated in a schedule.",
            "rdfs:label": "scheduledId",
            "unece:cefactElementMetadata": [
                {
                    "@id": "cefact:Logistics_TransportMovement.Scheduled_Identification.Identifier",
                    "@type": "unece:BasicBIE",
                    "unece:TDED": "8028",
                    "unece:cefactUNId": "UN01003842",
                    "unece:cefactBieDomainClass": "cefact:Logistics_TransportMovement.Details",
                    "rdfs:comment": "A unique identifier for this logistics transport movement, such as a voyage number, flight number, or trip number, as stated in a schedule."
                }
            ]
        },
        {
            "@id": "transport:scheduledRoute",
            "@type": "rdf:Property",
            "schema:rangeIncludes": {
                "@id": "transport:Route"
            },
            "schema:domainIncludes": {
                "@id": "transport:LogisticsTransportEquipment"
            },
            "rdfs:comment": "A scheduled or planned route for this piece of logistics transport equipment.",
            "rdfs:label": "scheduledRoute",
            "unece:cefactElementMetadata": [
                {
                    "@id": "cefact:Logistics_TransportEquipment.Scheduled.Transport_Route",
                    "@type": "unece:AssociationBIE",
                    "unece:cefactUNId": "UN01013595",
                    "unece:cefactBieDomainClass": "cefact:Logistics_TransportEquipment.Details",
                    "rdfs:comment": "A scheduled or planned route for this piece of logistics transport equipment."
                }
            ]
        },
        {
            "@id": "transport:scopeCode",
            "@type": "rdf:Property",
            "schema:rangeIncludes": {
                "@id": "xsd:token"
            },
            "schema:domainIncludes": {
                "@id": "transport:ForecastDeliverySchedule"
            },
            "rdfs:comment": "The code indicating the scope of a forecast delivery schedule.",
            "rdfs:label": "scopeCode",
            "unece:cefactElementMetadata": [
                {
                    "@id": "cefact:Forecast_DeliverySchedule.Scope.Code",
                    "@type": "unece:BasicBIE",
                    "unece:cefactUNId": "UN01014939",
                    "unece:cefactBieDomainClass": "cefact:Forecast_DeliverySchedule.Details",
                    "rdfs:comment": "The code indicating the scope of a forecast delivery schedule."
                }
            ]
        },
        {
            "@id": "transport:sealQuantity",
            "@type": "rdf:Property",
            "schema:rangeIncludes": {
                "@id": "xsd:decimal"
            },
            "schema:domainIncludes": [
                {
                    "@id": "transport:AssociatedTransportEquipment"
                },
                {
                    "@id": "transport:LogisticsTransportEquipment"
                }
            ],
            "rdfs:comment": [
                "A quantity of seals for this associated piece of transport equipment.",
                "The quantity of seals for this piece of logistics transport equipment."
            ],
            "rdfs:label": "sealQuantity",
            "unece:cefactElementMetadata": [
                {
                    "@id": "cefact:Logistics_TransportEquipment.Seal.Quantity",
                    "@type": "unece:BasicBIE",
                    "unece:cefactUNId": "UN01006135",
                    "unece:cefactBieDomainClass": "cefact:Logistics_TransportEquipment.Details",
                    "rdfs:comment": "The quantity of seals for this piece of logistics transport equipment."
                },
                {
                    "@id": "cefact:Associated_TransportEquipment.Seal.Quantity",
                    "@type": "unece:BasicBIE",
                    "unece:cefactUNId": "UN01014630",
                    "unece:cefactBieDomainClass": "cefact:Associated_TransportEquipment.Details",
                    "rdfs:comment": "A quantity of seals for this associated piece of transport equipment."
                }
            ]
        },
        {
            "@id": "transport:sealedIndicator",
            "@type": "rdf:Property",
            "schema:rangeIncludes": {
                "@id": "xsd:boolean"
            },
            "schema:domainIncludes": [
                {
                    "@id": "transport:AssociatedTransportEquipment"
                },
                {
                    "@id": "transport:LogisticsTransportEquipment"
                }
            ],
            "rdfs:comment": [
                "The indication of whether or not this associated piece of transport equipment is sealed.",
                "The indication of whether or not this piece of logistics transport equipment is sealed."
            ],
            "rdfs:label": "sealedIndicator",
            "unece:cefactElementMetadata": [
                {
                    "@id": "cefact:Logistics_TransportEquipment.Sealed.Indicator",
                    "@type": "unece:BasicBIE",
                    "unece:cefactUNId": "UN01012567",
                    "unece:cefactBieDomainClass": "cefact:Logistics_TransportEquipment.Details",
                    "rdfs:comment": "The indication of whether or not this piece of logistics transport equipment is sealed."
                },
                {
                    "@id": "cefact:Associated_TransportEquipment.Sealed.Indicator",
                    "@type": "unece:BasicBIE",
                    "unece:cefactUNId": "UN01014629",
                    "unece:cefactBieDomainClass": "cefact:Associated_TransportEquipment.Details",
                    "rdfs:comment": "The indication of whether or not this associated piece of transport equipment is sealed."
                }
            ]
        },
        {
            "@id": "transport:secondTypeExtensionCode",
            "@type": "rdf:Property",
            "schema:rangeIncludes": {
                "@id": "xsd:token"
            },
            "schema:domainIncludes": {
                "@id": "transport:SupplyChainConsignmentItem"
            },
            "rdfs:comment": "The code used as a second extension to the type code for further specifying the type of supply chain consignment item.",
            "rdfs:label": "secondTypeExtensionCode",
            "unece:cefactElementMetadata": [
                {
                    "@id": "cefact:SupplyChain_ConsignmentItem.Second_TypeExtension.Code",
                    "@type": "unece:BasicBIE",
                    "unece:TDED": "7361",
                    "unece:cefactUNId": "UN01004109",
                    "unece:cefactBieDomainClass": "cefact:SupplyChain_ConsignmentItem.Details",
                    "rdfs:comment": "The code used as a second extension to the type code for further specifying the type of supply chain consignment item."
                }
            ]
        },
        {
            "@id": "transport:sequenceNumeric",
            "@type": "rdf:Property",
            "schema:rangeIncludes": {
                "@id": "xsd:decimal"
            },
            "schema:domainIncludes": [
                {
                    "@id": "transport:LogisticsPackaging"
                },
                {
                    "@id": "transport:LogisticsTransportEquipment"
                },
                {
                    "@id": "transport:LogisticsTransportMeans"
                },
                {
                    "@id": "transport:Referenced_SupplyChainConsignment"
                },
                {
                    "@id": "transport:Referenced_SupplyChainConsignmentItem"
                },
                {
                    "@id": "transport:SupplyChainConsignment"
                },
                {
                    "@id": "transport:SupplyChainConsignmentItem"
                }
            ],
            "rdfs:comment": [
                "A sequence number for this supply chain consignment.",
                "The sequence number differentiating this logistics transport means from others.",
                "The sequence number differentiating this piece of logistics transport equipment from others in a set of transport equipment.",
                "The sequence number for this logistics packaging.",
                "The sequence number for this referenced supply chain consignment item.",
                "The sequence number for this referenced supply chain consignment.",
                "The sequence number for this supply chain consignment item."
            ],
            "rdfs:label": "sequenceNumeric",
            "unece:cefactElementMetadata": [
                {
                    "@id": "cefact:Referenced_SupplyChain_ConsignmentItem.Sequence.Numeric",
                    "@type": "unece:BasicBIE",
                    "unece:TDED": "1496",
                    "unece:cefactUNId": "UN01004036",
                    "unece:cefactBieDomainClass": "cefact:Referenced_SupplyChain_ConsignmentItem.Details",
                    "rdfs:comment": "The sequence number for this referenced supply chain consignment item."
                },
                {
                    "@id": "cefact:Logistics_Packaging.Sequence.Numeric",
                    "@type": "unece:BasicBIE",
                    "unece:cefactUNId": "UN01014947",
                    "unece:cefactBieDomainClass": "cefact:Logistics_Packaging.Details",
                    "rdfs:comment": "The sequence number for this logistics packaging."
                },
                {
                    "@id": "cefact:Referenced_SupplyChain_Consignment.Sequence.Numeric",
                    "@type": "unece:BasicBIE",
                    "unece:TDED": "1490",
                    "unece:cefactUNId": "UN01004046",
                    "unece:cefactBieDomainClass": "cefact:Referenced_SupplyChain_Consignment.Details",
                    "rdfs:comment": "The sequence number for this referenced supply chain consignment."
                },
                {
                    "@id": "cefact:Logistics_TransportEquipment.Sequence.Numeric",
                    "@type": "unece:BasicBIE",
                    "unece:TDED": "1492",
                    "unece:cefactUNId": "UN01003779",
                    "unece:cefactBieDomainClass": "cefact:Logistics_TransportEquipment.Details",
                    "rdfs:comment": "The sequence number differentiating this piece of logistics transport equipment from others in a set of transport equipment."
                },
                {
                    "@id": "cefact:SupplyChain_ConsignmentItem.Sequence.Numeric",
                    "@type": "unece:BasicBIE",
                    "unece:TDED": "1496",
                    "unece:cefactUNId": "UN01004105",
                    "unece:cefactBieDomainClass": "cefact:SupplyChain_ConsignmentItem.Details",
                    "rdfs:comment": "The sequence number for this supply chain consignment item."
                },
                {
                    "@id": "cefact:Logistics_TransportMeans.Sequence.Numeric",
                    "@type": "unece:BasicBIE",
                    "unece:cefactUNId": "UN01010101",
                    "unece:cefactBieDomainClass": "cefact:Logistics_TransportMeans.Details",
                    "rdfs:comment": "The sequence number differentiating this logistics transport means from others."
                },
                {
                    "@id": "cefact:SupplyChain_Consignment.Sequence.Numeric",
                    "@type": "unece:BasicBIE",
                    "unece:TDED": "1490",
                    "unece:cefactUNId": "UN01004167",
                    "unece:cefactBieDomainClass": "cefact:SupplyChain_Consignment.Details",
                    "rdfs:comment": "A sequence number for this supply chain consignment."
                }
            ]
        },
        {
            "@id": "transport:service",
            "@type": "rdf:Property",
            "schema:rangeIncludes": {
                "@id": "xsd:string"
            },
            "schema:domainIncludes": {
                "@id": "transport:LogisticsTransportMovement"
            },
            "rdfs:comment": "The service, expressed as text, of this logistics transport movement.",
            "rdfs:label": "service",
            "unece:cefactElementMetadata": [
                {
                    "@id": "cefact:Logistics_TransportMovement.Service.Text",
                    "@type": "unece:BasicBIE",
                    "unece:cefactUNId": "UN01012752",
                    "unece:cefactBieDomainClass": "cefact:Logistics_TransportMovement.Details",
                    "rdfs:comment": "The service, expressed as text, of this logistics transport movement."
                }
            ]
        },
        {
            "@id": "transport:serviceChargeApplicableCurrencyExchange",
            "@type": "rdf:Property",
            "schema:rangeIncludes": {
                "@id": "transport:CurrencyExchange"
            },
            "schema:domainIncludes": {
                "@id": "transport:SupplyChainConsignment"
            },
            "rdfs:comment": "A currency exchange applicable to a service charge for this supply chain consignment.",
            "rdfs:label": "serviceChargeApplicableCurrencyExchange",
            "unece:cefactElementMetadata": [
                {
                    "@id": "cefact:SupplyChain_Consignment.ServiceCharge_Applicable.Trade_CurrencyExchange",
                    "@type": "unece:AssociationBIE",
                    "unece:cefactUNId": "UN01004281",
                    "unece:cefactBieDomainClass": "cefact:SupplyChain_Consignment.Details",
                    "rdfs:comment": "A currency exchange applicable to a service charge for this supply chain consignment."
                }
            ]
        },
        {
            "@id": "transport:serviceCode",
            "@type": "rdf:Property",
            "schema:rangeIncludes": {
                "@id": "xsd:token"
            },
            "schema:domainIncludes": {
                "@id": "transport:LogisticsTransportMovement"
            },
            "rdfs:comment": "The code specifying the service of this logistics transport movement, such as regular, milk run or spot service.",
            "rdfs:label": "serviceCode",
            "unece:cefactElementMetadata": [
                {
                    "@id": "cefact:Logistics_TransportMovement.Service.Code",
                    "@type": "unece:BasicBIE",
                    "unece:cefactUNId": "UN01012751",
                    "unece:cefactBieDomainClass": "cefact:Logistics_TransportMovement.Details",
                    "rdfs:comment": "The code specifying the service of this logistics transport movement, such as regular, milk run or spot service."
                }
            ]
        },
        {
            "@id": "transport:serviceProviderParty",
            "@type": "rdf:Property",
            "schema:rangeIncludes": {
                "@id": "transport:Party"
            },
            "schema:domainIncludes": {
                "@id": "transport:LogisticsTransportMeans"
            },
            "rdfs:comment": "A trade party providing services for this logistics means of transport.",
            "rdfs:label": "serviceProviderParty",
            "unece:cefactElementMetadata": [
                {
                    "@id": "cefact:Logistics_TransportMeans.ServiceProvider.Trade_Party",
                    "@type": "unece:AssociationBIE",
                    "unece:cefactUNId": "UN01010111",
                    "unece:cefactBieDomainClass": "cefact:Logistics_TransportMeans.Details",
                    "rdfs:comment": "A trade party providing services for this logistics means of transport."
                }
            ]
        },
        {
            "@id": "transport:settingTemperature",
            "@type": "rdf:Property",
            "schema:rangeIncludes": {
                "@id": "transport:Temperature"
            },
            "schema:domainIncludes": [
                {
                    "@id": "transport:AssociatedTransportEquipment"
                },
                {
                    "@id": "transport:LogisticsTransportEquipment"
                },
                {
                    "@id": "transport:Referenced_LogisticsTransportEquipment"
                }
            ],
            "rdfs:comment": [
                "A temperature setting for this piece of associated transport equipment, such as storage temperature or operational temperature.",
                "A temperature setting for this piece of logistics transport equipment, such as storage temperature or operational temperature.",
                "A temperature setting for this piece of referenced logistics transport equipment, such as storage temperature or operational temperature."
            ],
            "rdfs:label": "settingTemperature",
            "unece:cefactElementMetadata": [
                {
                    "@id": "cefact:Associated_TransportEquipment.Setting.TransportSetting_Temperature",
                    "@type": "unece:AssociationBIE",
                    "unece:cefactUNId": "UN01013663",
                    "unece:cefactBieDomainClass": "cefact:Associated_TransportEquipment.Details",
                    "rdfs:comment": "A temperature setting for this piece of associated transport equipment, such as storage temperature or operational temperature."
                },
                {
                    "@id": "cefact:Logistics_TransportEquipment.Setting.TransportSetting_Temperature",
                    "@type": "unece:AssociationBIE",
                    "unece:cefactUNId": "UN01003800",
                    "unece:cefactBieDomainClass": "cefact:Logistics_TransportEquipment.Details",
                    "rdfs:comment": "A temperature setting for this piece of logistics transport equipment, such as storage temperature or operational temperature."
                },
                {
                    "@id": "cefact:Referenced_Logistics_TransportEquipment.Setting.TransportSetting_Temperature",
                    "@type": "unece:AssociationBIE",
                    "unece:cefactUNId": "UN01013181",
                    "unece:cefactBieDomainClass": "cefact:Referenced_Logistics_TransportEquipment.Details",
                    "rdfs:comment": "A temperature setting for this piece of referenced logistics transport equipment, such as storage temperature or operational temperature."
                }
            ]
        },
        {
            "@id": "transport:shipFromParty",
            "@type": "rdf:Property",
            "schema:rangeIncludes": {
                "@id": "transport:Party"
            },
            "schema:domainIncludes": {
                "@id": "transport:SupplyChainConsignment"
            },
            "rdfs:comment": "The ship from party for this supply chain consignment.",
            "rdfs:label": "shipFromParty",
            "unece:cefactElementMetadata": [
                {
                    "@id": "cefact:SupplyChain_Consignment.ShipFrom.Trade_Party",
                    "@type": "unece:AssociationBIE",
                    "unece:cefactUNId": "UN01004221",
                    "unece:cefactBieDomainClass": "cefact:SupplyChain_Consignment.Details",
                    "rdfs:comment": "The ship from party for this supply chain consignment."
                }
            ]
        },
        {
            "@id": "transport:shipStoresIndicator",
            "@type": "rdf:Property",
            "schema:rangeIncludes": {
                "@id": "xsd:boolean"
            },
            "schema:domainIncludes": {
                "@id": "transport:SupplyChainConsignment"
            },
            "rdfs:comment": "The indication of whether or not this supply chain consignment is for ship stores, such as for consumption on the means of transport.",
            "rdfs:label": "shipStoresIndicator",
            "unece:cefactElementMetadata": [
                {
                    "@id": "cefact:SupplyChain_Consignment.ShipStores.Indicator",
                    "@type": "unece:BasicBIE",
                    "unece:cefactUNId": "UN01004209",
                    "unece:cefactBieDomainClass": "cefact:SupplyChain_Consignment.Details",
                    "rdfs:comment": "The indication of whether or not this supply chain consignment is for ship stores, such as for consumption on the means of transport."
                }
            ]
        },
        {
            "@id": "transport:shipToParty",
            "@type": "rdf:Property",
            "schema:rangeIncludes": {
                "@id": "transport:Party"
            },
            "schema:domainIncludes": [
                {
                    "@id": "transport:ForecastDeliverySchedule"
                },
                {
                    "@id": "transport:SupplyChainConsignment"
                }
            ],
            "rdfs:comment": [
                "A ship to party for this forecast delivery schedule.",
                "The ship to party for this supply chain consignment."
            ],
            "rdfs:label": "shipToParty",
            "unece:cefactElementMetadata": [
                {
                    "@id": "cefact:SupplyChain_Consignment.ShipTo.Trade_Party",
                    "@type": "unece:AssociationBIE",
                    "unece:cefactUNId": "UN01004222",
                    "unece:cefactBieDomainClass": "cefact:SupplyChain_Consignment.Details",
                    "rdfs:comment": "The ship to party for this supply chain consignment."
                },
                {
                    "@id": "cefact:Forecast_DeliverySchedule.ShipTo.Trade_Party",
                    "@type": "unece:AssociationBIE",
                    "unece:cefactUNId": "UN01014940",
                    "unece:cefactBieDomainClass": "cefact:Forecast_DeliverySchedule.Details",
                    "rdfs:comment": "A ship to party for this forecast delivery schedule."
                }
            ]
        },
        {
            "@id": "transport:shipToShipEvent",
            "@type": "rdf:Property",
            "schema:rangeIncludes": {
                "@id": "transport:Event"
            },
            "schema:domainIncludes": {
                "@id": "transport:LogisticsTransportMovement"
            },
            "rdfs:comment": "A ship to ship event for this logistics transport movement.",
            "rdfs:label": "shipToShipEvent",
            "unece:cefactElementMetadata": [
                {
                    "@id": "cefact:Logistics_TransportMovement.ShipToShip.Transport_Event",
                    "@type": "unece:AssociationBIE",
                    "unece:cefactUNId": "UN01013178",
                    "unece:cefactBieDomainClass": "cefact:Logistics_TransportMovement.Details",
                    "rdfs:comment": "A ship to ship event for this logistics transport movement."
                }
            ]
        },
        {
            "@id": "transport:shippedOnboardDateTime",
            "@type": "rdf:Property",
            "schema:rangeIncludes": {
                "@id": "xsd:dateTime"
            },
            "schema:domainIncludes": {
                "@id": "transport:SupplyChainConsignment"
            },
            "rdfs:comment": "A date, time, date time, or other date time value when this supply chain consignment is shipped onboard.",
            "rdfs:label": "shippedOnboardDateTime",
            "unece:cefactElementMetadata": [
                {
                    "@id": "cefact:SupplyChain_Consignment.ShippedOnboard.DateTime",
                    "@type": "unece:BasicBIE",
                    "unece:cefactUNId": "UN01015089",
                    "unece:cefactBieDomainClass": "cefact:SupplyChain_Consignment.Details",
                    "rdfs:comment": "A date, time, date time, or other date time value when this supply chain consignment is shipped onboard."
                }
            ]
        },
        {
            "@id": "transport:shipperReferenceInformation",
            "@type": "rdf:Property",
            "schema:rangeIncludes": {
                "@id": "xsd:string"
            },
            "schema:domainIncludes": {
                "@id": "transport:LogisticsTransportEquipment"
            },
            "rdfs:comment": "Shipper reference information, expressed as text, for this piece of logistics transport equipment.",
            "rdfs:label": "shipperReferenceInformation",
            "unece:cefactElementMetadata": [
                {
                    "@id": "cefact:Logistics_TransportEquipment.ShipperReference_Information.Text",
                    "@type": "unece:BasicBIE",
                    "unece:TDED": "4014",
                    "unece:cefactUNId": "UN01013167",
                    "unece:cefactBieDomainClass": "cefact:Logistics_TransportEquipment.Details",
                    "rdfs:comment": "Shipper reference information, expressed as text, for this piece of logistics transport equipment."
                }
            ]
        },
        {
            "@id": "transport:specialInstructions",
            "@type": "rdf:Property",
            "schema:rangeIncludes": {
                "@id": "xsd:string"
            },
            "schema:domainIncludes": {
                "@id": "transport:SupplyChainConsignmentItem"
            },
            "rdfs:comment": "Special instructions, expressed as text, for this supply chain consignment item.",
            "rdfs:label": "specialInstructions",
            "unece:cefactElementMetadata": [
                {
                    "@id": "cefact:SupplyChain_ConsignmentItem.SpecialInstructions.Text",
                    "@type": "unece:BasicBIE",
                    "unece:cefactUNId": "UN01004125",
                    "unece:cefactBieDomainClass": "cefact:SupplyChain_ConsignmentItem.Details",
                    "rdfs:comment": "Special instructions, expressed as text, for this supply chain consignment item."
                }
            ]
        },
        {
            "@id": "transport:specialSpecifiedInstructions",
            "@type": "rdf:Property",
            "schema:rangeIncludes": {
                "@id": "transport:Instructions"
            },
            "schema:domainIncludes": {
                "@id": "transport:LogisticsTransportMovement"
            },
            "rdfs:comment": "Special transport instructions specified for this logistics transport movement.",
            "rdfs:label": "specialSpecifiedInstructions",
            "unece:cefactElementMetadata": [
                {
                    "@id": "cefact:Logistics_TransportMovement.Special_Specified.Transport_Instructions",
                    "@type": "unece:AssociationBIE",
                    "unece:cefactUNId": "UN01003880",
                    "unece:cefactBieDomainClass": "cefact:Logistics_TransportMovement.Details",
                    "rdfs:comment": "Special transport instructions specified for this logistics transport movement."
                }
            ]
        },
        {
            "@id": "transport:specifiedCertificate",
            "@type": "rdf:Property",
            "schema:rangeIncludes": {
                "@id": "transport:Certificate"
            },
            "schema:domainIncludes": [
                {
                    "@id": "transport:LogisticsTransportMovement"
                },
                {
                    "@id": "transport:TransportationWasteRecoveryDisposalProcess"
                }
            ],
            "rdfs:comment": [
                "A process certificate specified for this logistics transport movement.",
                "A process certificate specified for this transportation waste recovery disposal process.",
                "An organizational certificate specified for this logistics transport movement."
            ],
            "rdfs:label": "specifiedCertificate",
            "unece:cefactElementMetadata": [
                {
                    "@id": "cefact:Logistics_TransportMovement.Specified.Process_Certificate",
                    "@type": "unece:AssociationBIE",
                    "unece:cefactUNId": "UN01013839",
                    "unece:cefactBieDomainClass": "cefact:Logistics_TransportMovement.Details",
                    "rdfs:comment": "A process certificate specified for this logistics transport movement."
                },
                {
                    "@id": "cefact:Logistics_TransportMovement.Specified.Organizational_Certificate",
                    "@type": "unece:AssociationBIE",
                    "unece:cefactUNId": "UN01013840",
                    "unece:cefactBieDomainClass": "cefact:Logistics_TransportMovement.Details",
                    "rdfs:comment": "An organizational certificate specified for this logistics transport movement."
                },
                {
                    "@id": "cefact:TransportationWasteRecoveryDisposal_Process.Specified.Process_Certificate",
                    "@type": "unece:AssociationBIE",
                    "unece:cefactUNId": "UN01014619",
                    "unece:cefactBieDomainClass": "cefact:TransportationWasteRecoveryDisposal_Process.Details",
                    "rdfs:comment": "A process certificate specified for this transportation waste recovery disposal process."
                }
            ]
        },
        {
            "@id": "transport:specifiedDeliveryTerms",
            "@type": "rdf:Property",
            "schema:rangeIncludes": {
                "@id": "transport:DeliveryTerms"
            },
            "schema:domainIncludes": {
                "@id": "transport:SupplyChainConsignment"
            },
            "rdfs:comment": "Delivery terms specified for this supply chain consignment.",
            "rdfs:label": "specifiedDeliveryTerms",
            "unece:cefactElementMetadata": [
                {
                    "@id": "cefact:SupplyChain_Consignment.Specified.Trade_DeliveryTerms",
                    "@type": "unece:AssociationBIE",
                    "unece:cefactUNId": "UN01004283",
                    "unece:cefactBieDomainClass": "cefact:SupplyChain_Consignment.Details",
                    "rdfs:comment": "Delivery terms specified for this supply chain consignment."
                }
            ]
        },
        {
            "@id": "transport:specifiedDimension",
            "@type": "rdf:Property",
            "schema:rangeIncludes": {
                "@id": "transport:Dimension"
            },
            "schema:domainIncludes": {
                "@id": "transport:LogisticsTransportMeans"
            },
            "rdfs:comment": "Spatial dimensions specified for this logistics means of transport.",
            "rdfs:label": "specifiedDimension",
            "unece:cefactElementMetadata": [
                {
                    "@id": "cefact:Logistics_TransportMeans.Specified.Spatial_Dimension",
                    "@type": "unece:AssociationBIE",
                    "unece:cefactUNId": "UN01010110",
                    "unece:cefactBieDomainClass": "cefact:Logistics_TransportMeans.Details",
                    "rdfs:comment": "Spatial dimensions specified for this logistics means of transport."
                }
            ]
        },
        {
            "@id": "transport:specifiedEmission",
            "@type": "rdf:Property",
            "schema:rangeIncludes": {
                "@id": "transport:Emission"
            },
            "schema:domainIncludes": [
                {
                    "@id": "transport:LogisticsTransportMeans"
                },
                {
                    "@id": "transport:LogisticsTransportMovement"
                }
            ],
            "rdfs:comment": [
                "A calculated emission specified for this logistics transport means.",
                "A calculated emission specified for this logistics transport movement."
            ],
            "rdfs:label": "specifiedEmission",
            "unece:cefactElementMetadata": [
                {
                    "@id": "cefact:Logistics_TransportMeans.Specified.Calculated_Emission",
                    "@type": "unece:AssociationBIE",
                    "unece:cefactUNId": "UN01013833",
                    "unece:cefactBieDomainClass": "cefact:Logistics_TransportMeans.Details",
                    "rdfs:comment": "A calculated emission specified for this logistics transport means."
                },
                {
                    "@id": "cefact:Logistics_TransportMovement.Specified.Calculated_Emission",
                    "@type": "unece:AssociationBIE",
                    "unece:cefactUNId": "UN01010129",
                    "unece:cefactBieDomainClass": "cefact:Logistics_TransportMovement.Details",
                    "rdfs:comment": "A calculated emission specified for this logistics transport movement."
                }
            ]
        },
        {
            "@id": "transport:specifiedEvent",
            "@type": "rdf:Property",
            "schema:rangeIncludes": {
                "@id": "transport:Event"
            },
            "schema:domainIncludes": [
                {
                    "@id": "transport:LogisticsTransportMovement"
                },
                {
                    "@id": "transport:SupplyChainConsignment"
                },
                {
                    "@id": "transport:SupplyChainConsignmentItem"
                }
            ],
            "rdfs:comment": [
                "A transport event specified for this logistics transport movement.",
                "An inspection event specified for this supply chain consignment item.",
                "An inspection event specified for this supply chain consignment."
            ],
            "rdfs:label": "specifiedEvent",
            "unece:cefactElementMetadata": [
                {
                    "@id": "cefact:Logistics_TransportMovement.Specified.Transport_Event",
                    "@type": "unece:AssociationBIE",
                    "unece:cefactUNId": "UN01012569",
                    "unece:cefactBieDomainClass": "cefact:Logistics_TransportMovement.Details",
                    "rdfs:comment": "A transport event specified for this logistics transport movement."
                },
                {
                    "@id": "cefact:SupplyChain_ConsignmentItem.Specified.Inspection_Event",
                    "@type": "unece:AssociationBIE",
                    "unece:cefactUNId": "UN01014447",
                    "unece:cefactBieDomainClass": "cefact:SupplyChain_ConsignmentItem.Details",
                    "rdfs:comment": "An inspection event specified for this supply chain consignment item."
                },
                {
                    "@id": "cefact:SupplyChain_Consignment.Specified.Inspection_Event",
                    "@type": "unece:AssociationBIE",
                    "unece:cefactUNId": "UN01014449",
                    "unece:cefactBieDomainClass": "cefact:SupplyChain_Consignment.Details",
                    "rdfs:comment": "An inspection event specified for this supply chain consignment."
                }
            ]
        },
        {
            "@id": "transport:specifiedFault",
            "@type": "rdf:Property",
            "schema:rangeIncludes": {
                "@id": "transport:Fault"
            },
            "schema:domainIncludes": {
                "@id": "transport:LogisticsTransportMeans"
            },
            "rdfs:comment": "An identified defect specified for this logistics means of transport.",
            "rdfs:label": "specifiedFault",
            "unece:cefactElementMetadata": [
                {
                    "@id": "cefact:Logistics_TransportMeans.Specified.Identified_Fault",
                    "@type": "unece:AssociationBIE",
                    "unece:cefactUNId": "UN01010118",
                    "unece:cefactBieDomainClass": "cefact:Logistics_TransportMeans.Details",
                    "rdfs:comment": "An identified defect specified for this logistics means of transport."
                }
            ]
        },
        {
            "@id": "transport:specifiedInstructions",
            "@type": "rdf:Property",
            "schema:rangeIncludes": {
                "@id": "transport:Instructions"
            },
            "schema:domainIncludes": [
                {
                    "@id": "transport:LogisticsTransportMeans"
                },
                {
                    "@id": "transport:LogisticsTransportMovement"
                }
            ],
            "rdfs:comment": [
                "Handling instructions specified for this logistics means of transport.",
                "Handling instructions specified for this logistics transport movement."
            ],
            "rdfs:label": "specifiedInstructions",
            "unece:cefactElementMetadata": [
                {
                    "@id": "cefact:Logistics_TransportMeans.Specified.Handling_Instructions",
                    "@type": "unece:AssociationBIE",
                    "unece:cefactUNId": "UN01010112",
                    "unece:cefactBieDomainClass": "cefact:Logistics_TransportMeans.Details",
                    "rdfs:comment": "Handling instructions specified for this logistics means of transport."
                },
                {
                    "@id": "cefact:Logistics_TransportMovement.Specified.Handling_Instructions",
                    "@type": "unece:AssociationBIE",
                    "unece:cefactUNId": "UN01010132",
                    "unece:cefactBieDomainClass": "cefact:Logistics_TransportMovement.Details",
                    "rdfs:comment": "Handling instructions specified for this logistics transport movement."
                }
            ]
        },
        {
            "@id": "transport:specifiedMarking",
            "@type": "rdf:Property",
            "schema:rangeIncludes": {
                "@id": "transport:Marking"
            },
            "schema:domainIncludes": [
                {
                    "@id": "transport:LogisticsPackaging"
                },
                {
                    "@id": "transport:SupplyChainPackaging"
                },
                {
                    "@id": "transport:TradeProduct_SupplyChainPackaging"
                }
            ],
            "rdfs:comment": [
                "A Cross Industry (CI) packaging marking specified for this trade product supply chain packaging, such as an inscription, stamp or label to indicate date, ownership, quality, manufacture or origin.",
                "A marking specified for this logistics packaging.",
                "A marking specified for this supply chain packaging, such as an inscription, stamp or label to indicate date, ownership, quality, manufacture or origin."
            ],
            "rdfs:label": "specifiedMarking",
            "unece:cefactElementMetadata": [
                {
                    "@id": "cefact:SupplyChain_Packaging.Specified.Packaging_Marking",
                    "@type": "unece:AssociationBIE",
                    "unece:cefactUNId": "UN01004323",
                    "unece:cefactBieDomainClass": "cefact:SupplyChain_Packaging.Details",
                    "rdfs:comment": "A marking specified for this supply chain packaging, such as an inscription, stamp or label to indicate date, ownership, quality, manufacture or origin."
                },
                {
                    "@id": "cefact:TradeProduct_SupplyChain_Packaging.Specified.CI_Packaging_Marking",
                    "@type": "unece:AssociationBIE",
                    "unece:cefactUNId": "UN01007483",
                    "unece:cefactBieDomainClass": "cefact:TradeProduct_SupplyChain_Packaging.Details",
                    "rdfs:comment": "A Cross Industry (CI) packaging marking specified for this trade product supply chain packaging, such as an inscription, stamp or label to indicate date, ownership, quality, manufacture or origin."
                },
                {
                    "@id": "cefact:Logistics_Packaging.Specified.Packaging_Marking",
                    "@type": "unece:AssociationBIE",
                    "unece:cefactUNId": "UN01014967",
                    "unece:cefactBieDomainClass": "cefact:Logistics_Packaging.Details",
                    "rdfs:comment": "A marking specified for this logistics packaging."
                }
            ]
        },
        {
            "@id": "transport:specifiedReference",
            "@type": "rdf:Property",
            "schema:rangeIncludes": {
                "@id": "transport:Reference"
            },
            "schema:domainIncludes": {
                "@id": "transport:SupplyChainConsignment"
            },
            "rdfs:comment": "A reference specified for this supply chain consignment.",
            "rdfs:label": "specifiedReference",
            "unece:cefactElementMetadata": [
                {
                    "@id": "cefact:SupplyChain_Consignment.Specified.SupplyChain_Reference",
                    "@type": "unece:AssociationBIE",
                    "unece:cefactUNId": "UN01014970",
                    "unece:cefactBieDomainClass": "cefact:SupplyChain_Consignment.Details",
                    "rdfs:comment": "A reference specified for this supply chain consignment."
                }
            ]
        },
        {
            "@id": "transport:specifiedRiskAnalysisResult",
            "@type": "rdf:Property",
            "schema:rangeIncludes": {
                "@id": "transport:RiskAnalysisResult"
            },
            "schema:domainIncludes": [
                {
                    "@id": "transport:LogisticsTransportEquipment"
                },
                {
                    "@id": "transport:LogisticsTransportMovement"
                },
                {
                    "@id": "transport:Referenced_SupplyChainConsignment"
                },
                {
                    "@id": "transport:SupplyChainConsignment"
                },
                {
                    "@id": "transport:SupplyChainConsignmentItem"
                }
            ],
            "rdfs:comment": [
                "A result of a logistics risk analysis calculation specified for this supply chain consignment.",
                "A result of a logistics risk analysis calculation specified for this transport equipment.",
                "A result of a logistics risk analysis calculation specified for this transport movement.",
                "A result of a logistics risk analysis specified for this referenced supply chain consignment.",
                "Results of a logistics risk analysis specified for this supply chain consignment item."
            ],
            "rdfs:label": "specifiedRiskAnalysisResult",
            "unece:cefactElementMetadata": [
                {
                    "@id": "cefact:Logistics_TransportEquipment.Specified.Logistics_RiskAnalysisResult",
                    "@type": "unece:AssociationBIE",
                    "unece:cefactUNId": "UN01013051",
                    "unece:cefactBieDomainClass": "cefact:Logistics_TransportEquipment.Details",
                    "rdfs:comment": "A result of a logistics risk analysis calculation specified for this transport equipment."
                },
                {
                    "@id": "cefact:Logistics_TransportMovement.Specified.Logistics_RiskAnalysisResult",
                    "@type": "unece:AssociationBIE",
                    "unece:cefactUNId": "UN01013052",
                    "unece:cefactBieDomainClass": "cefact:Logistics_TransportMovement.Details",
                    "rdfs:comment": "A result of a logistics risk analysis calculation specified for this transport movement."
                },
                {
                    "@id": "cefact:SupplyChain_Consignment.Specified.Logistics_RiskAnalysisResult",
                    "@type": "unece:AssociationBIE",
                    "unece:cefactUNId": "UN01013053",
                    "unece:cefactBieDomainClass": "cefact:SupplyChain_Consignment.Details",
                    "rdfs:comment": "A result of a logistics risk analysis calculation specified for this supply chain consignment."
                },
                {
                    "@id": "cefact:Referenced_SupplyChain_Consignment.Specified.Logistics_RiskAnalysisResult",
                    "@type": "unece:AssociationBIE",
                    "unece:cefactUNId": "UN01013182",
                    "unece:cefactBieDomainClass": "cefact:Referenced_SupplyChain_Consignment.Details",
                    "rdfs:comment": "A result of a logistics risk analysis specified for this referenced supply chain consignment."
                },
                {
                    "@id": "cefact:SupplyChain_ConsignmentItem.Specified.Logistics_RiskAnalysisResult",
                    "@type": "unece:AssociationBIE",
                    "unece:cefactUNId": "UN01014758",
                    "unece:cefactBieDomainClass": "cefact:SupplyChain_ConsignmentItem.Details",
                    "rdfs:comment": "Results of a logistics risk analysis specified for this supply chain consignment item."
                }
            ]
        },
        {
            "@id": "transport:specifiedStatus",
            "@type": "rdf:Property",
            "schema:rangeIncludes": {
                "@id": "transport:Status"
            },
            "schema:domainIncludes": [
                {
                    "@id": "transport:LogisticsTransportMovement"
                },
                {
                    "@id": "transport:SupplyChainConsignment"
                }
            ],
            "rdfs:comment": [
                "A status specified for this logistics transport movement.",
                "Logistics status information specified for this supply chain consignment."
            ],
            "rdfs:label": "specifiedStatus",
            "unece:cefactElementMetadata": [
                {
                    "@id": "cefact:Logistics_TransportMovement.Specified.Logistics_Status",
                    "@type": "unece:AssociationBIE",
                    "unece:cefactUNId": "UN01014988",
                    "unece:cefactBieDomainClass": "cefact:Logistics_TransportMovement.Details",
                    "rdfs:comment": "A status specified for this logistics transport movement."
                },
                {
                    "@id": "cefact:SupplyChain_Consignment.Specified.Logistics_Status",
                    "@type": "unece:AssociationBIE",
                    "unece:cefactUNId": "UN01014985",
                    "unece:cefactBieDomainClass": "cefact:SupplyChain_Consignment.Details",
                    "rdfs:comment": "Logistics status information specified for this supply chain consignment."
                }
            ]
        },
        {
            "@id": "transport:specifiedTradeLineItem",
            "@type": "rdf:Property",
            "schema:rangeIncludes": {
                "@id": "transport:TradeLineItem"
            },
            "schema:domainIncludes": {
                "@id": "transport:ForecastDeliverySchedule"
            },
            "rdfs:comment": "A trade line item specified for this forecast delivery schedule.",
            "rdfs:label": "specifiedTradeLineItem",
            "unece:cefactElementMetadata": [
                {
                    "@id": "cefact:Forecast_DeliverySchedule.Specified.SupplyChain_TradeLineItem",
                    "@type": "unece:AssociationBIE",
                    "unece:cefactUNId": "UN01014941",
                    "unece:cefactBieDomainClass": "cefact:Forecast_DeliverySchedule.Details",
                    "rdfs:comment": "A trade line item specified for this forecast delivery schedule."
                }
            ]
        },
        {
            "@id": "transport:specifiedTransportMeans",
            "@type": "rdf:Property",
            "schema:rangeIncludes": {
                "@id": "transport:TransportMeans"
            },
            "schema:domainIncludes": {
                "@id": "transport:LogisticsTransportEquipment"
            },
            "rdfs:comment": "A transport means specified for this piece of logistics transport equipment.",
            "rdfs:label": "specifiedTransportMeans",
            "unece:cefactElementMetadata": [
                {
                    "@id": "cefact:Logistics_TransportEquipment.Specified.Logistics_TransportMeans",
                    "@type": "unece:AssociationBIE",
                    "unece:cefactUNId": "UN01003814",
                    "unece:cefactBieDomainClass": "cefact:Logistics_TransportEquipment.Details",
                    "rdfs:comment": "A transport means specified for this piece of logistics transport equipment."
                }
            ]
        },
        {
            "@id": "transport:specifiedTransportMovement",
            "@type": "rdf:Property",
            "schema:rangeIncludes": {
                "@id": "transport:TransportMovement"
            },
            "schema:domainIncludes": {
                "@id": "transport:SupplyChainConsignment"
            },
            "rdfs:comment": "A logistics transport movement specified for this supply chain consignment.",
            "rdfs:label": "specifiedTransportMovement",
            "unece:cefactElementMetadata": [
                {
                    "@id": "cefact:SupplyChain_Consignment.Specified.Logistics_TransportMovement",
                    "@type": "unece:AssociationBIE",
                    "unece:cefactUNId": "UN01004267",
                    "unece:cefactBieDomainClass": "cefact:SupplyChain_Consignment.Details",
                    "rdfs:comment": "A logistics transport movement specified for this supply chain consignment."
                }
            ]
        },
        {
            "@id": "transport:stage",
            "@type": "rdf:Property",
            "schema:rangeIncludes": {
                "@id": "xsd:string"
            },
            "schema:domainIncludes": {
                "@id": "transport:LogisticsTransportMovement"
            },
            "rdfs:comment": "A stage, expressed as text, of this logistics transport movement.",
            "rdfs:label": "stage",
            "unece:cefactElementMetadata": [
                {
                    "@id": "cefact:Logistics_TransportMovement.Stage.Text",
                    "@type": "unece:BasicBIE",
                    "unece:cefactUNId": "UN01013834",
                    "unece:cefactBieDomainClass": "cefact:Logistics_TransportMovement.Details",
                    "rdfs:comment": "A stage, expressed as text, of this logistics transport movement."
                }
            ]
        },
        {
            "@id": "transport:statedCondition",
            "@type": "rdf:Property",
            "schema:rangeIncludes": {
                "@id": "transport:Condition"
            },
            "schema:domainIncludes": {
                "@id": ":TransportDangerousGoods"
            },
            "rdfs:comment": "A stated condition of these transported dangerous goods.",
            "rdfs:label": "statedCondition",
            "unece:cefactElementMetadata": [
                {
                    "@id": "cefact:Transport_DangerousGoods.Stated.Specified_Condition",
                    "@type": "unece:AssociationBIE",
                    "unece:cefactUNId": "UN01014761",
                    "unece:cefactBieDomainClass": "cefact:Transport_DangerousGoods.Details",
                    "rdfs:comment": "A stated condition of these transported dangerous goods."
                }
            ]
        },
        {
            "@id": "transport:stayId",
            "@type": "rdf:Property",
            "schema:rangeIncludes": {
                "@id": "xsd:token"
            },
            "schema:domainIncludes": {
                "@id": "transport:LogisticsTransportMovement"
            },
            "rdfs:comment": "The unique identifier of a stay in a port, airport or other place of service for this logistics transport movement.",
            "rdfs:label": "stayId",
            "unece:cefactElementMetadata": [
                {
                    "@id": "cefact:Logistics_TransportMovement.Stay.Identifier",
                    "@type": "unece:BasicBIE",
                    "unece:TDED": "1099",
                    "unece:cefactUNId": "UN01003845",
                    "unece:cefactBieDomainClass": "cefact:Logistics_TransportMovement.Details",
                    "rdfs:comment": "The unique identifier of a stay in a port, airport or other place of service for this logistics transport movement."
                }
            ]
        },
        {
            "@id": "transport:stevedoreParty",
            "@type": "rdf:Property",
            "schema:rangeIncludes": {
                "@id": "transport:Party"
            },
            "schema:domainIncludes": {
                "@id": "transport:LogisticsTransportMovement"
            },
            "rdfs:comment": "A stevedore party for this logistics transport movement.",
            "rdfs:label": "stevedoreParty",
            "unece:cefactElementMetadata": [
                {
                    "@id": "cefact:Logistics_TransportMovement.Stevedore.Trade_Party",
                    "@type": "unece:AssociationBIE",
                    "unece:cefactUNId": "UN01003872",
                    "unece:cefactBieDomainClass": "cefact:Logistics_TransportMovement.Details",
                    "rdfs:comment": "A stevedore party for this logistics transport movement."
                }
            ]
        },
        {
            "@id": "transport:storageEvent",
            "@type": "rdf:Property",
            "schema:rangeIncludes": {
                "@id": "transport:Event"
            },
            "schema:domainIncludes": [
                {
                    "@id": "transport:LogisticsTransportEquipment"
                },
                {
                    "@id": "transport:SupplyChainConsignment"
                }
            ],
            "rdfs:comment": [
                "A storage event for this supply chain consignment.",
                "A storage event specifying when and where this piece of logistics transport equipment will be, or has been, stored."
            ],
            "rdfs:label": "storageEvent",
            "unece:cefactElementMetadata": [
                {
                    "@id": "cefact:Logistics_TransportEquipment.Storage.Transport_Event",
                    "@type": "unece:AssociationBIE",
                    "unece:cefactUNId": "UN01003804",
                    "unece:cefactBieDomainClass": "cefact:Logistics_TransportEquipment.Details",
                    "rdfs:comment": "A storage event specifying when and where this piece of logistics transport equipment will be, or has been, stored."
                },
                {
                    "@id": "cefact:SupplyChain_Consignment.Storage.Transport_Event",
                    "@type": "unece:AssociationBIE",
                    "unece:cefactUNId": "UN01004255",
                    "unece:cefactBieDomainClass": "cefact:SupplyChain_Consignment.Details",
                    "rdfs:comment": "A storage event for this supply chain consignment."
                }
            ]
        },
        {
            "@id": "transport:stowagePositionId",
            "@type": "rdf:Property",
            "schema:rangeIncludes": {
                "@id": "xsd:token"
            },
            "schema:domainIncludes": {
                "@id": "transport:LogisticsTransportEquipment"
            },
            "rdfs:comment": "The stowage position identifier for this piece of logistics transport equipment.",
            "rdfs:label": "stowagePositionId",
            "unece:cefactElementMetadata": [
                {
                    "@id": "cefact:Logistics_TransportEquipment.StowagePosition.Identifier",
                    "@type": "unece:BasicBIE",
                    "unece:cefactUNId": "UN01013168",
                    "unece:cefactBieDomainClass": "cefact:Logistics_TransportEquipment.Details",
                    "rdfs:comment": "The stowage position identifier for this piece of logistics transport equipment."
                }
            ]
        },
        {
            "@id": "transport:summaryDescription",
            "@type": "rdf:Property",
            "schema:rangeIncludes": {
                "@id": "xsd:string"
            },
            "schema:domainIncludes": {
                "@id": "transport:SupplyChainConsignment"
            },
            "rdfs:comment": "A textual summary description of this supply chain consignment.",
            "rdfs:label": "summaryDescription",
            "unece:cefactElementMetadata": [
                {
                    "@id": "cefact:SupplyChain_Consignment.SummaryDescription.Text",
                    "@type": "unece:BasicBIE",
                    "unece:TDED": "7004",
                    "unece:cefactUNId": "UN01004201",
                    "unece:cefactBieDomainClass": "cefact:SupplyChain_Consignment.Details",
                    "rdfs:comment": "A textual summary description of this supply chain consignment."
                }
            ]
        },
        {
            "@id": "transport:tareWeightMeasure",
            "@type": "rdf:Property",
            "schema:rangeIncludes": {
                "@id": "xsd:decimal"
            },
            "schema:domainIncludes": [
                {
                    "@id": "transport:AssociatedTransportEquipment"
                },
                {
                    "@id": "transport:LogisticsTransportEquipment"
                },
                {
                    "@id": "transport:LogisticsTransportMeans"
                }
            ],
            "rdfs:comment": [
                "The measure of the tare weight (mass) of this logistics means of transport which is the weight (mass) including permanent equipment but excluding goods and loose accessories.",
                "The measure of the tare weight (mass) of this piece of associated transport equipment which is the weight (mass) including permanent equipment but excluding goods and loose accessories.",
                "The measure of the tare weight (mass) of this piece of logistics transport equipment which is the weight (mass) including permanent equipment but excluding goods and loose accessories."
            ],
            "rdfs:label": "tareWeightMeasure",
            "unece:cefactElementMetadata": [
                {
                    "@id": "cefact:Logistics_TransportMeans.TareWeight.Measure",
                    "@type": "unece:BasicBIE",
                    "unece:cefactUNId": "UN01013600",
                    "unece:cefactBieDomainClass": "cefact:Logistics_TransportMeans.Details",
                    "rdfs:comment": "The measure of the tare weight (mass) of this logistics means of transport which is the weight (mass) including permanent equipment but excluding goods and loose accessories."
                },
                {
                    "@id": "cefact:Logistics_TransportEquipment.TareWeight.Measure",
                    "@type": "unece:BasicBIE",
                    "unece:TDED": "6411",
                    "unece:cefactUNId": "UN01003761",
                    "unece:cefactBieDomainClass": "cefact:Logistics_TransportEquipment.Details",
                    "rdfs:comment": "The measure of the tare weight (mass) of this piece of logistics transport equipment which is the weight (mass) including permanent equipment but excluding goods and loose accessories."
                },
                {
                    "@id": "cefact:Associated_TransportEquipment.TareWeight.Measure",
                    "@type": "unece:BasicBIE",
                    "unece:TDED": "6156",
                    "unece:cefactUNId": "UN01013656",
                    "unece:cefactBieDomainClass": "cefact:Associated_TransportEquipment.Details",
                    "rdfs:comment": "The measure of the tare weight (mass) of this piece of associated transport equipment which is the weight (mass) including permanent equipment but excluding goods and loose accessories."
                }
            ]
        },
        {
            "@id": "transport:terminalOperatorAssignedId",
            "@type": "rdf:Property",
            "schema:rangeIncludes": {
                "@id": "xsd:token"
            },
            "schema:domainIncludes": {
                "@id": "transport:LogisticsTransportMovement"
            },
            "rdfs:comment": "A unique identifier for this logistics transport movement as assigned by a terminal operator.",
            "rdfs:label": "terminalOperatorAssignedId",
            "unece:cefactElementMetadata": [
                {
                    "@id": "cefact:Logistics_TransportMovement.TerminalOperatorAssigned_Identification.Identifier",
                    "@type": "unece:BasicBIE",
                    "unece:TDED": "8028",
                    "unece:cefactUNId": "UN01003844",
                    "unece:cefactBieDomainClass": "cefact:Logistics_TransportMovement.Details",
                    "rdfs:comment": "A unique identifier for this logistics transport movement as assigned by a terminal operator."
                }
            ]
        },
        {
            "@id": "transport:terminalOperatorParty",
            "@type": "rdf:Property",
            "schema:rangeIncludes": {
                "@id": "transport:Party"
            },
            "schema:domainIncludes": {
                "@id": "transport:LogisticsTransportMovement"
            },
            "rdfs:comment": "A terminal operator party for this logistics transport movement.",
            "rdfs:label": "terminalOperatorParty",
            "unece:cefactElementMetadata": [
                {
                    "@id": "cefact:Logistics_TransportMovement.TerminalOperator.Trade_Party",
                    "@type": "unece:AssociationBIE",
                    "unece:cefactUNId": "UN01003866",
                    "unece:cefactBieDomainClass": "cefact:Logistics_TransportMovement.Details",
                    "rdfs:comment": "A terminal operator party for this logistics transport movement."
                }
            ]
        },
        {
            "@id": "transport:totalAllowanceChargeAmount",
            "@type": "rdf:Property",
            "schema:rangeIncludes": {
                "@id": "xsd:decimal"
            },
            "schema:domainIncludes": {
                "@id": "transport:SupplyChainConsignment"
            },
            "rdfs:comment": "The total monetary value of all allowances and charges for this supply chain consignment.",
            "rdfs:label": "totalAllowanceChargeAmount",
            "unece:cefactElementMetadata": [
                {
                    "@id": "cefact:SupplyChain_Consignment.TotalAllowanceCharge.Amount",
                    "@type": "unece:BasicBIE",
                    "unece:cefactUNId": "UN01004185",
                    "unece:cefactBieDomainClass": "cefact:SupplyChain_Consignment.Details",
                    "rdfs:comment": "The total monetary value of all allowances and charges for this supply chain consignment."
                }
            ]
        },
        {
            "@id": "transport:totalChargeAmount",
            "@type": "rdf:Property",
            "schema:rangeIncludes": {
                "@id": "xsd:decimal"
            },
            "schema:domainIncludes": [
                {
                    "@id": "transport:SupplyChainConsignment"
                },
                {
                    "@id": "transport:SupplyChainConsignmentItem"
                }
            ],
            "rdfs:comment": [
                "The monetary value of all freight and other service charges for this supply chain consignment item.",
                "The total monetary value of all freight and other service charges for this supply chain consignment."
            ],
            "rdfs:label": "totalChargeAmount",
            "unece:cefactElementMetadata": [
                {
                    "@id": "cefact:SupplyChain_Consignment.TotalCharge.Amount",
                    "@type": "unece:BasicBIE",
                    "unece:TDED": "5290",
                    "unece:cefactUNId": "UN01004182",
                    "unece:cefactBieDomainClass": "cefact:SupplyChain_Consignment.Details",
                    "rdfs:comment": "The total monetary value of all freight and other service charges for this supply chain consignment."
                },
                {
                    "@id": "cefact:SupplyChain_ConsignmentItem.TotalCharge.Amount",
                    "@type": "unece:BasicBIE",
                    "unece:cefactUNId": "UN01004119",
                    "unece:cefactBieDomainClass": "cefact:SupplyChain_ConsignmentItem.Details",
                    "rdfs:comment": "The monetary value of all freight and other service charges for this supply chain consignment item."
                }
            ]
        },
        {
            "@id": "transport:totalCollectChargeAmount",
            "@type": "rdf:Property",
            "schema:rangeIncludes": {
                "@id": "xsd:decimal"
            },
            "schema:domainIncludes": {
                "@id": "transport:SupplyChainConsignment"
            },
            "rdfs:comment": "The total monetary value of all freight and other service charges which are to be collected from the consignee at or after delivery for this supply chain consignment.",
            "rdfs:label": "totalCollectChargeAmount",
            "unece:cefactElementMetadata": [
                {
                    "@id": "cefact:SupplyChain_Consignment.TotalCollectCharge.Amount",
                    "@type": "unece:BasicBIE",
                    "unece:TDED": "5398",
                    "unece:cefactUNId": "UN01004183",
                    "unece:cefactBieDomainClass": "cefact:SupplyChain_Consignment.Details",
                    "rdfs:comment": "The total monetary value of all freight and other service charges which are to be collected from the consignee at or after delivery for this supply chain consignment."
                }
            ]
        },
        {
            "@id": "transport:totalDisbursementAmount",
            "@type": "rdf:Property",
            "schema:rangeIncludes": {
                "@id": "xsd:decimal"
            },
            "schema:domainIncludes": {
                "@id": "transport:SupplyChainConsignment"
            },
            "rdfs:comment": "The monetary value of total disbursement for this supply chain consignment, such as the amount to be collected by the carrier according to the order given by the consignor.",
            "rdfs:label": "totalDisbursementAmount",
            "unece:cefactElementMetadata": [
                {
                    "@id": "cefact:SupplyChain_Consignment.TotalDisbursement.Amount",
                    "@type": "unece:BasicBIE",
                    "unece:TDED": "5416",
                    "unece:cefactUNId": "UN01004186",
                    "unece:cefactBieDomainClass": "cefact:SupplyChain_Consignment.Details",
                    "rdfs:comment": "The monetary value of total disbursement for this supply chain consignment, such as the amount to be collected by the carrier according to the order given by the consignor."
                }
            ]
        },
        {
            "@id": "transport:totalExportExitToImportEntryChargeAmount",
            "@type": "rdf:Property",
            "schema:rangeIncludes": {
                "@id": "xsd:decimal"
            },
            "schema:domainIncludes": [
                {
                    "@id": "transport:SupplyChainConsignment"
                },
                {
                    "@id": "transport:SupplyChainConsignmentItem"
                }
            ],
            "rdfs:comment": [
                "The monetary value of the total charge or charges of freight, insurance and other services for this supply chain consignment calculated from the export exit location to the import entry location.",
                "The monetary value of the total charge or charges of freight, insurance and other services for this supply chain consignment item calculated from the export exit location to the import entry location."
            ],
            "rdfs:label": "totalExportExitToImportEntryChargeAmount",
            "unece:cefactElementMetadata": [
                {
                    "@id": "cefact:SupplyChain_ConsignmentItem.TotalExportExitToImportEntryCharge.Amount",
                    "@type": "unece:BasicBIE",
                    "unece:cefactUNId": "UN01004120",
                    "unece:cefactBieDomainClass": "cefact:SupplyChain_ConsignmentItem.Details",
                    "rdfs:comment": "The monetary value of the total charge or charges of freight, insurance and other services for this supply chain consignment item calculated from the export exit location to the import entry location."
                },
                {
                    "@id": "cefact:SupplyChain_Consignment.TotalExportExitToImportEntryCharge.Amount",
                    "@type": "unece:BasicBIE",
                    "unece:TDED": "5506",
                    "unece:cefactUNId": "UN01004187",
                    "unece:cefactBieDomainClass": "cefact:SupplyChain_Consignment.Details",
                    "rdfs:comment": "The monetary value of the total charge or charges of freight, insurance and other services for this supply chain consignment calculated from the export exit location to the import entry location."
                }
            ]
        },
        {
            "@id": "transport:totalPrepaidChargeAmount",
            "@type": "rdf:Property",
            "schema:rangeIncludes": {
                "@id": "xsd:decimal"
            },
            "schema:domainIncludes": {
                "@id": "transport:SupplyChainConsignment"
            },
            "rdfs:comment": "The total monetary value of all freight and other service charges which have been paid in advance for this supply chain consignment.",
            "rdfs:label": "totalPrepaidChargeAmount",
            "unece:cefactElementMetadata": [
                {
                    "@id": "cefact:SupplyChain_Consignment.TotalPrepaidCharge.Amount",
                    "@type": "unece:BasicBIE",
                    "unece:TDED": "5302",
                    "unece:cefactUNId": "UN01004184",
                    "unece:cefactBieDomainClass": "cefact:SupplyChain_Consignment.Details",
                    "rdfs:comment": "The total monetary value of all freight and other service charges which have been paid in advance for this supply chain consignment."
                }
            ]
        },
        {
            "@id": "transport:totalUnitQuantity",
            "@type": "rdf:Property",
            "schema:rangeIncludes": {
                "@id": "xsd:decimal"
            },
            "schema:domainIncludes": [
                {
                    "@id": "transport:LogisticsPackaging"
                },
                {
                    "@id": "transport:SupplyChainPackaging"
                },
                {
                    "@id": "transport:TradeProduct_SupplyChainPackaging"
                }
            ],
            "rdfs:comment": [
                "A total number of units contained in this logistics packaging.",
                "A total number of units contained in this supply chain packaging.",
                "A total number of units contained in this trade product supply chain packaging."
            ],
            "rdfs:label": "totalUnitQuantity",
            "unece:cefactElementMetadata": [
                {
                    "@id": "cefact:Logistics_Packaging.TotalUnit.Quantity",
                    "@type": "unece:BasicBIE",
                    "unece:cefactUNId": "UN01014956",
                    "unece:cefactBieDomainClass": "cefact:Logistics_Packaging.Details",
                    "rdfs:comment": "A total number of units contained in this logistics packaging."
                },
                {
                    "@id": "cefact:TradeProduct_SupplyChain_Packaging.TotalUnit.Quantity",
                    "@type": "unece:BasicBIE",
                    "unece:cefactUNId": "UN01007479",
                    "unece:cefactBieDomainClass": "cefact:TradeProduct_SupplyChain_Packaging.Details",
                    "rdfs:comment": "A total number of units contained in this trade product supply chain packaging."
                },
                {
                    "@id": "cefact:SupplyChain_Packaging.TotalUnit.Quantity",
                    "@type": "unece:BasicBIE",
                    "unece:cefactUNId": "UN01007195",
                    "unece:cefactBieDomainClass": "cefact:SupplyChain_Packaging.Details",
                    "rdfs:comment": "A total number of units contained in this supply chain packaging."
                }
            ]
        },
        {
            "@id": "transport:towingVesselRelatedTransportMovement",
            "@type": "rdf:Property",
            "schema:rangeIncludes": {
                "@id": "transport:TransportMovement"
            },
            "schema:domainIncludes": {
                "@id": "transport:LogisticsTransportMovement"
            },
            "rdfs:comment": "A towing vessel transport movement related to this logistics transport movement.",
            "rdfs:label": "towingVesselRelatedTransportMovement",
            "unece:cefactElementMetadata": [
                {
                    "@id": "cefact:Logistics_TransportMovement.TowingVessel_Related.Logistics_TransportMovement",
                    "@type": "unece:AssociationBIE",
                    "unece:cefactUNId": "UN01003883",
                    "unece:cefactBieDomainClass": "cefact:Logistics_TransportMovement.Details",
                    "rdfs:comment": "A towing vessel transport movement related to this logistics transport movement."
                }
            ]
        },
        {
            "@id": "transport:tradeLineItemQuantity",
            "@type": "rdf:Property",
            "schema:rangeIncludes": {
                "@id": "xsd:decimal"
            },
            "schema:domainIncludes": [
                {
                    "@id": "transport:Referenced_SupplyChainConsignmentItem"
                },
                {
                    "@id": "transport:SupplyChainConsignmentItem"
                }
            ],
            "rdfs:comment": [
                "The number of trade line items in this referenced supply chain consignment item.",
                "The number of trade line items in this supply chain consignment item."
            ],
            "rdfs:label": "tradeLineItemQuantity",
            "unece:cefactElementMetadata": [
                {
                    "@id": "cefact:SupplyChain_ConsignmentItem.TradeLineItem.Quantity",
                    "@type": "unece:BasicBIE",
                    "unece:cefactUNId": "UN01011069",
                    "unece:cefactBieDomainClass": "cefact:SupplyChain_ConsignmentItem.Details",
                    "rdfs:comment": "The number of trade line items in this supply chain consignment item."
                },
                {
                    "@id": "cefact:Referenced_SupplyChain_ConsignmentItem.TradeLineItem.Quantity",
                    "@type": "unece:BasicBIE",
                    "unece:cefactUNId": "UN01011042",
                    "unece:cefactBieDomainClass": "cefact:Referenced_SupplyChain_ConsignmentItem.Details",
                    "rdfs:comment": "The number of trade line items in this referenced supply chain consignment item."
                }
            ]
        },
        {
            "@id": "transport:tradedParcelId",
            "@type": "rdf:Property",
            "schema:rangeIncludes": {
                "@id": "xsd:token"
            },
            "schema:domainIncludes": {
                "@id": "transport:SupplyChainConsignment"
            },
            "rdfs:comment": "A traded parcel identifier for this supply chain consignment.",
            "rdfs:label": "tradedParcelId",
            "unece:cefactElementMetadata": [
                {
                    "@id": "cefact:SupplyChain_Consignment.TradedParcel.Identifier",
                    "@type": "unece:BasicBIE",
                    "unece:cefactUNId": "UN01004166",
                    "unece:cefactBieDomainClass": "cefact:SupplyChain_Consignment.Details",
                    "rdfs:comment": "A traded parcel identifier for this supply chain consignment."
                }
            ]
        },
        {
            "@id": "transport:tradedParcelQuantity",
            "@type": "rdf:Property",
            "schema:rangeIncludes": {
                "@id": "xsd:decimal"
            },
            "schema:domainIncludes": {
                "@id": "transport:LogisticsTransportMovement"
            },
            "rdfs:comment": "The number of traded parcels of cargo being transported in this logistics transport movement.",
            "rdfs:label": "tradedParcelQuantity",
            "unece:cefactElementMetadata": [
                {
                    "@id": "cefact:Logistics_TransportMovement.TradedParcel.Quantity",
                    "@type": "unece:BasicBIE",
                    "unece:cefactUNId": "UN01003852",
                    "unece:cefactBieDomainClass": "cefact:Logistics_TransportMovement.Details",
                    "rdfs:comment": "The number of traded parcels of cargo being transported in this logistics transport movement."
                }
            ]
        },
        {
            "@id": "transport:tradingConsolidatorAssignedId",
            "@type": "rdf:Property",
            "schema:rangeIncludes": {
                "@id": "xsd:token"
            },
            "schema:domainIncludes": {
                "@id": "transport:LogisticsTransportMovement"
            },
            "rdfs:comment": "The unique identifier for this logistics transport movement as assigned by the trading consolidator.",
            "rdfs:label": "tradingConsolidatorAssignedId",
            "unece:cefactElementMetadata": [
                {
                    "@id": "cefact:Logistics_TransportMovement.TradingConsolidatorAssigned_Identification.Identifier",
                    "@type": "unece:BasicBIE",
                    "unece:TDED": "8028",
                    "unece:cefactUNId": "UN01003843",
                    "unece:cefactBieDomainClass": "cefact:Logistics_TransportMovement.Details",
                    "rdfs:comment": "The unique identifier for this logistics transport movement as assigned by the trading consolidator."
                }
            ]
        },
        {
            "@id": "transport:trainedMedicalPersonnelOnboardQuantity",
            "@type": "rdf:Property",
            "schema:rangeIncludes": {
                "@id": "xsd:decimal"
            },
            "schema:domainIncludes": {
                "@id": "transport:LogisticsTransportMovement"
            },
            "rdfs:comment": "The number of trained medical personnel onboard this logistics transport movement.",
            "rdfs:label": "trainedMedicalPersonnelOnboardQuantity",
            "unece:cefactElementMetadata": [
                {
                    "@id": "cefact:Logistics_TransportMovement.Trained_MedicalPersonnelOnboard.Quantity",
                    "@type": "unece:BasicBIE",
                    "unece:cefactUNId": "UN01015086",
                    "unece:cefactBieDomainClass": "cefact:Logistics_TransportMovement.Details",
                    "rdfs:comment": "The number of trained medical personnel onboard this logistics transport movement."
                }
            ]
        },
        {
            "@id": "transport:transitCountry",
            "@type": "rdf:Property",
            "schema:rangeIncludes": {
                "@id": "transport:Country"
            },
            "schema:domainIncludes": [
                {
                    "@id": "transport:SupplyChainConsignment"
                },
                {
                    "@id": "transport:SupplyChainConsignmentItem"
                }
            ],
            "rdfs:comment": [
                "A transit country for this supply chain consignment item.",
                "A transit country for this supply chain consignment."
            ],
            "rdfs:label": "transitCountry",
            "unece:cefactElementMetadata": [
                {
                    "@id": "cefact:SupplyChain_Consignment.Transit.Trade_Country",
                    "@type": "unece:AssociationBIE",
                    "unece:cefactUNId": "UN01004269",
                    "unece:cefactBieDomainClass": "cefact:SupplyChain_Consignment.Details",
                    "rdfs:comment": "A transit country for this supply chain consignment."
                },
                {
                    "@id": "cefact:SupplyChain_ConsignmentItem.Transit.Trade_Country",
                    "@type": "unece:AssociationBIE",
                    "unece:cefactUNId": "UN01004143",
                    "unece:cefactBieDomainClass": "cefact:SupplyChain_ConsignmentItem.Details",
                    "rdfs:comment": "A transit country for this supply chain consignment item."
                }
            ]
        },
        {
            "@id": "transport:transitLocation",
            "@type": "rdf:Property",
            "schema:rangeIncludes": {
                "@id": "transport:Location"
            },
            "schema:domainIncludes": {
                "@id": "transport:SupplyChainConsignment"
            },
            "rdfs:comment": "A location of transit for this supply chain consignment.",
            "rdfs:label": "transitLocation",
            "unece:cefactElementMetadata": [
                {
                    "@id": "cefact:SupplyChain_Consignment.Transit.Logistics_Location",
                    "@type": "unece:AssociationBIE",
                    "unece:cefactUNId": "UN01004240",
                    "unece:cefactBieDomainClass": "cefact:SupplyChain_Consignment.Details",
                    "rdfs:comment": "A location of transit for this supply chain consignment."
                }
            ]
        },
        {
            "@id": "transport:transportContractDocument",
            "@type": "rdf:Property",
            "schema:rangeIncludes": {
                "@id": "transport:Document"
            },
            "schema:domainIncludes": [
                {
                    "@id": "transport:Referenced_SupplyChainConsignment"
                },
                {
                    "@id": "transport:SupplyChainConsignment"
                },
                {
                    "@id": "transport:SupplyChainConsignmentItem"
                }
            ],
            "rdfs:comment": [
                "A transport contract document for this supply chain consignment item.",
                "The referenced transport contract document for this supply chain consignment, such as an airwaybill or a seawaybill.",
                "The transport contract document for this referenced supply chain consignment, such as an airwaybill or a seawaybill."
            ],
            "rdfs:label": "transportContractDocument",
            "unece:cefactElementMetadata": [
                {
                    "@id": "cefact:Referenced_SupplyChain_Consignment.TransportContract.Referenced_Document",
                    "@type": "unece:AssociationBIE",
                    "unece:cefactUNId": "UN01011065",
                    "unece:cefactBieDomainClass": "cefact:Referenced_SupplyChain_Consignment.Details",
                    "rdfs:comment": "The transport contract document for this referenced supply chain consignment, such as an airwaybill or a seawaybill."
                },
                {
                    "@id": "cefact:SupplyChain_Consignment.TransportContract.Referenced_Document",
                    "@type": "unece:AssociationBIE",
                    "unece:cefactUNId": "UN01004243",
                    "unece:cefactBieDomainClass": "cefact:SupplyChain_Consignment.Details",
                    "rdfs:comment": "The referenced transport contract document for this supply chain consignment, such as an airwaybill or a seawaybill."
                },
                {
                    "@id": "cefact:SupplyChain_ConsignmentItem.TransportContract.Referenced_Document",
                    "@type": "unece:AssociationBIE",
                    "unece:cefactUNId": "UN01008997",
                    "unece:cefactBieDomainClass": "cefact:SupplyChain_ConsignmentItem.Details",
                    "rdfs:comment": "A transport contract document for this supply chain consignment item."
                }
            ]
        },
        {
            "@id": "transport:transportContractRelatedDocument",
            "@type": "rdf:Property",
            "schema:rangeIncludes": {
                "@id": "transport:Document"
            },
            "schema:domainIncludes": {
                "@id": "transport:LogisticsTransportMovement"
            },
            "rdfs:comment": "A transport contract document related to this logistics transport movement.",
            "rdfs:label": "transportContractRelatedDocument",
            "unece:cefactElementMetadata": [
                {
                    "@id": "cefact:Logistics_TransportMovement.TransportContract_Related.Referenced_Document",
                    "@type": "unece:AssociationBIE",
                    "unece:cefactUNId": "UN01008986",
                    "unece:cefactBieDomainClass": "cefact:Logistics_TransportMovement.Details",
                    "rdfs:comment": "A transport contract document related to this logistics transport movement."
                }
            ]
        },
        {
            "@id": "transport:transportEquipmentCategoryCode",
            "@type": "rdf:Property",
            "schema:rangeIncludes": {
                "@id": "unece:UNECECL8053Code"
            },
            "schema:domainIncludes": [
                {
                    "@id": "transport:AssociatedTransportEquipment"
                },
                {
                    "@id": "transport:AttachedTransportEquipment"
                },
                {
                    "@id": "transport:LogisticsTransportEquipment"
                },
                {
                    "@id": "transport:Referenced_LogisticsTransportEquipment"
                }
            ],
            "rdfs:comment": [
                "A code specifying a category of this piece of associated transport equipment.",
                "A code specifying a category of this piece of attached transport equipment.",
                "The code specifying the category for this piece of logistics transport equipment, such as container or trailer.",
                "The code specifying the category of this referenced piece of logistics transport equipment."
            ],
            "rdfs:label": "transportEquipmentCategoryCode",
            "unece:cefactElementMetadata": [
                {
                    "@id": "cefact:Associated_TransportEquipment.Category.Code",
                    "@type": "unece:BasicBIE",
                    "unece:TDED": "8053",
                    "unece:cefactUNId": "UN01003413",
                    "unece:cefactBieDomainClass": "cefact:Associated_TransportEquipment.Details",
                    "rdfs:comment": "A code specifying a category of this piece of associated transport equipment."
                },
                {
                    "@id": "cefact:Referenced_Logistics_TransportEquipment.Category.Code",
                    "@type": "unece:BasicBIE",
                    "unece:TDED": "8053",
                    "unece:cefactUNId": "UN01004024",
                    "unece:cefactBieDomainClass": "cefact:Referenced_Logistics_TransportEquipment.Details",
                    "rdfs:comment": "The code specifying the category of this referenced piece of logistics transport equipment."
                },
                {
                    "@id": "cefact:Attached_TransportEquipment.Category.Code",
                    "@type": "unece:BasicBIE",
                    "unece:TDED": "8053",
                    "unece:cefactUNId": "UN01003418",
                    "unece:cefactBieDomainClass": "cefact:Attached_TransportEquipment.Details",
                    "rdfs:comment": "A code specifying a category of this piece of attached transport equipment."
                },
                {
                    "@id": "cefact:Logistics_TransportEquipment.Category.Code",
                    "@type": "unece:BasicBIE",
                    "unece:TDED": "8053",
                    "unece:cefactUNId": "UN01003767",
                    "unece:cefactBieDomainClass": "cefact:Logistics_TransportEquipment.Details",
                    "rdfs:comment": "The code specifying the category for this piece of logistics transport equipment, such as container or trailer."
                }
            ]
        },
        {
            "@id": "transport:transportEquipmentFullnessUsedCapacityCode",
            "@type": "rdf:Property",
            "schema:rangeIncludes": {
                "@id": "unece:UNECECL8169Code"
            },
            "schema:domainIncludes": {
                "@id": "transport:LogisticsTransportEquipment"
            },
            "rdfs:comment": "The code specifying the used capacity of this piece of logistics transport equipment, such as full or empty.",
            "rdfs:label": "transportEquipmentFullnessUsedCapacityCode",
            "unece:cefactElementMetadata": [
                {
                    "@id": "cefact:Logistics_TransportEquipment.UsedCapacity.Code",
                    "@type": "unece:BasicBIE",
                    "unece:TDED": "8169",
                    "unece:cefactUNId": "UN01003771",
                    "unece:cefactBieDomainClass": "cefact:Logistics_TransportEquipment.Details",
                    "rdfs:comment": "The code specifying the used capacity of this piece of logistics transport equipment, such as full or empty."
                }
            ]
        },
        {
            "@id": "transport:transportEquipmentHaulageArrangementsCode",
            "@type": "rdf:Property",
            "schema:rangeIncludes": {
                "@id": "unece:UNECECL8341Code"
            },
            "schema:domainIncludes": {
                "@id": "transport:LogisticsTransportEquipment"
            },
            "rdfs:comment": "The code specifying the arrangement for the haulage of this piece of logistics transport equipment.",
            "rdfs:label": "transportEquipmentHaulageArrangementsCode",
            "unece:cefactElementMetadata": [
                {
                    "@id": "cefact:Logistics_TransportEquipment.HaulageArrangement.Code",
                    "@type": "unece:BasicBIE",
                    "unece:TDED": "8341",
                    "unece:cefactUNId": "UN01003775",
                    "unece:cefactBieDomainClass": "cefact:Logistics_TransportEquipment.Details",
                    "rdfs:comment": "The code specifying the arrangement for the haulage of this piece of logistics transport equipment."
                }
            ]
        },
        {
            "@id": "transport:transportEquipmentMovementStatusTransportMovementStatusCode",
            "@type": "rdf:Property",
            "schema:rangeIncludes": {
                "@id": "unece:UNECECL8249Code"
            },
            "schema:domainIncludes": {
                "@id": "transport:LogisticsTransportEquipment"
            },
            "rdfs:comment": "The code specifying the transport movement status for this piece of logistics transport equipment, such as for export, for import, or for transhipment.",
            "rdfs:label": "transportEquipmentMovementStatusTransportMovementStatusCode",
            "unece:cefactElementMetadata": [
                {
                    "@id": "cefact:Logistics_TransportEquipment.TransportMovementStatus.Code",
                    "@type": "unece:BasicBIE",
                    "unece:TDED": "8249",
                    "unece:cefactUNId": "UN01003773",
                    "unece:cefactBieDomainClass": "cefact:Logistics_TransportEquipment.Details",
                    "rdfs:comment": "The code specifying the transport movement status for this piece of logistics transport equipment, such as for export, for import, or for transhipment."
                }
            ]
        },
        {
            "@id": "transport:transportEquipmentOperationalStatusCode",
            "@type": "rdf:Property",
            "schema:rangeIncludes": {
                "@id": "unece:UNECECL8249Code"
            },
            "schema:domainIncludes": {
                "@id": "transport:LogisticsTransportEquipment"
            },
            "rdfs:comment": "The code specifying the operational status for this piece of logistics transport equipment, such as to be repaired or to be shifted.",
            "rdfs:label": "transportEquipmentOperationalStatusCode",
            "unece:cefactElementMetadata": [
                {
                    "@id": "cefact:Logistics_TransportEquipment.OperationalStatus.Code",
                    "@type": "unece:BasicBIE",
                    "unece:TDED": "8249",
                    "unece:cefactUNId": "UN01003772",
                    "unece:cefactBieDomainClass": "cefact:Logistics_TransportEquipment.Details",
                    "rdfs:comment": "The code specifying the operational status for this piece of logistics transport equipment, such as to be repaired or to be shifted."
                }
            ]
        },
        {
            "@id": "transport:transportEquipmentQuantity",
            "@type": "rdf:Property",
            "schema:rangeIncludes": {
                "@id": "xsd:decimal"
            },
            "schema:domainIncludes": [
                {
                    "@id": "transport:LogisticsTransportMovement"
                },
                {
                    "@id": "transport:SupplyChainConsignment"
                }
            ],
            "rdfs:comment": [
                "A number of pieces of transport equipment, such as containers or similar unit load devices, in this supply chain consignment.",
                "The number of pieces of transport equipment for this logistics transport movement."
            ],
            "rdfs:label": "transportEquipmentQuantity",
            "unece:cefactElementMetadata": [
                {
                    "@id": "cefact:SupplyChain_Consignment.TransportEquipment.Quantity",
                    "@type": "unece:BasicBIE",
                    "unece:TDED": "8046",
                    "unece:cefactUNId": "UN01004198",
                    "unece:cefactBieDomainClass": "cefact:SupplyChain_Consignment.Details",
                    "rdfs:comment": "A number of pieces of transport equipment, such as containers or similar unit load devices, in this supply chain consignment."
                },
                {
                    "@id": "cefact:Logistics_TransportMovement.TransportEquipment.Quantity",
                    "@type": "unece:BasicBIE",
                    "unece:cefactUNId": "UN01003851",
                    "unece:cefactBieDomainClass": "cefact:Logistics_TransportMovement.Details",
                    "rdfs:comment": "The number of pieces of transport equipment for this logistics transport movement."
                }
            ]
        },
        {
            "@id": "transport:transportEquipmentSizeTypeCharacteristicCode",
            "@type": "rdf:Property",
            "schema:rangeIncludes": {
                "@id": "unece:UNECECL8155Code"
            },
            "schema:domainIncludes": [
                {
                    "@id": "transport:AssociatedTransportEquipment"
                },
                {
                    "@id": "transport:AttachedTransportEquipment"
                },
                {
                    "@id": "transport:Referenced_LogisticsTransportEquipment"
                }
            ],
            "rdfs:comment": [
                "The code specifying the characteristics, i.e. size and type, of this piece of associated transport equipment.",
                "The code specifying the characteristics, i.e. size and type, of this piece of attached transport equipment.",
                "The code specifying the characteristics, such as size and type, of this referenced piece of logistics transport equipment."
            ],
            "rdfs:label": "transportEquipmentSizeTypeCharacteristicCode",
            "unece:cefactElementMetadata": [
                {
                    "@id": "cefact:Attached_TransportEquipment.Characteristic.Code",
                    "@type": "unece:BasicBIE",
                    "unece:TDED": "8155",
                    "unece:cefactUNId": "UN01003419",
                    "unece:cefactBieDomainClass": "cefact:Attached_TransportEquipment.Details",
                    "rdfs:comment": "The code specifying the characteristics, i.e. size and type, of this piece of attached transport equipment."
                },
                {
                    "@id": "cefact:Referenced_Logistics_TransportEquipment.Characteristic.Code",
                    "@type": "unece:BasicBIE",
                    "unece:TDED": "8155",
                    "unece:cefactUNId": "UN01004025",
                    "unece:cefactBieDomainClass": "cefact:Referenced_Logistics_TransportEquipment.Details",
                    "rdfs:comment": "The code specifying the characteristics, such as size and type, of this referenced piece of logistics transport equipment."
                },
                {
                    "@id": "cefact:Associated_TransportEquipment.Characteristic.Code",
                    "@type": "unece:BasicBIE",
                    "unece:TDED": "8155",
                    "unece:cefactUNId": "UN01003414",
                    "unece:cefactBieDomainClass": "cefact:Associated_TransportEquipment.Details",
                    "rdfs:comment": "The code specifying the characteristics, i.e. size and type, of this piece of associated transport equipment."
                }
            ]
        },
        {
            "@id": "transport:transportEquipmentSplitGoodsIndicator",
            "@type": "rdf:Property",
            "schema:rangeIncludes": {
                "@id": "xsd:boolean"
            },
            "schema:domainIncludes": {
                "@id": "transport:SupplyChainConsignment"
            },
            "rdfs:comment": "The indication of whether or not the goods in this supply chain consignment are split across more than one piece of transport equipment.",
            "rdfs:label": "transportEquipmentSplitGoodsIndicator",
            "unece:cefactElementMetadata": [
                {
                    "@id": "cefact:SupplyChain_Consignment.TransportEquipmentSplitGoods.Indicator",
                    "@type": "unece:BasicBIE",
                    "unece:cefactUNId": "UN01004210",
                    "unece:cefactBieDomainClass": "cefact:SupplyChain_Consignment.Details",
                    "rdfs:comment": "The indication of whether or not the goods in this supply chain consignment are split across more than one piece of transport equipment."
                }
            ]
        },
        {
            "@id": "transport:transportEquipmentSupplierPartyRoleCode",
            "@type": "rdf:Property",
            "schema:rangeIncludes": {
                "@id": "unece:UNECECL8077Code"
            },
            "schema:domainIncludes": {
                "@id": "transport:LogisticsTransportEquipment"
            },
            "rdfs:comment": "The code specifying the role of the party responsible for supplying this piece of logistics transport equipment, such as the carrier or the buyer.",
            "rdfs:label": "transportEquipmentSupplierPartyRoleCode",
            "unece:cefactElementMetadata": [
                {
                    "@id": "cefact:Logistics_TransportEquipment.SupplierPartyRole.Code",
                    "@type": "unece:BasicBIE",
                    "unece:TDED": "8077",
                    "unece:cefactUNId": "UN01003770",
                    "unece:cefactBieDomainClass": "cefact:Logistics_TransportEquipment.Details",
                    "rdfs:comment": "The code specifying the role of the party responsible for supplying this piece of logistics transport equipment, such as the carrier or the buyer."
                }
            ]
        },
        {
            "@id": "transport:transportEvent",
            "@type": "rdf:Property",
            "schema:rangeIncludes": {
                "@id": "transport:Event"
            },
            "schema:domainIncludes": {
                "@id": "transport:SupplyChainConsignment"
            },
            "rdfs:comment": "An event occurring during the transport of this supply chain consignment.",
            "rdfs:label": "transportEvent",
            "unece:cefactElementMetadata": [
                {
                    "@id": "cefact:SupplyChain_Consignment.Transport.Transport_Event",
                    "@type": "unece:AssociationBIE",
                    "unece:cefactUNId": "UN01004252",
                    "unece:cefactBieDomainClass": "cefact:SupplyChain_Consignment.Details",
                    "rdfs:comment": "An event occurring during the transport of this supply chain consignment."
                }
            ]
        },
        {
            "@id": "transport:transportMeansDirectionTransitDirectionCode",
            "@type": "rdf:Property",
            "schema:rangeIncludes": {
                "@id": "unece:UNECECL8101Code"
            },
            "schema:domainIncludes": {
                "@id": "transport:LogisticsTransportMovement"
            },
            "rdfs:comment": "The code specifying the transit direction of this logistics transport movement.",
            "rdfs:label": "transportMeansDirectionTransitDirectionCode",
            "unece:cefactElementMetadata": [
                {
                    "@id": "cefact:Logistics_TransportMovement.TransitDirection.Code",
                    "@type": "unece:BasicBIE",
                    "unece:TDED": "8101",
                    "unece:cefactUNId": "UN01003848",
                    "unece:cefactBieDomainClass": "cefact:Logistics_TransportMovement.Details",
                    "rdfs:comment": "The code specifying the transit direction of this logistics transport movement."
                }
            ]
        },
        {
            "@id": "transport:transportMeansSecurityOfficerPerson",
            "@type": "rdf:Property",
            "schema:rangeIncludes": {
                "@id": "transport:Person"
            },
            "schema:domainIncludes": {
                "@id": "transport:LogisticsTransportMovement"
            },
            "rdfs:comment": "The officer responsible for the security of the means of transport used for this logistics transport movement.",
            "rdfs:label": "transportMeansSecurityOfficerPerson",
            "unece:cefactElementMetadata": [
                {
                    "@id": "cefact:Logistics_TransportMovement.TransportMeansSecurityOfficer.Transport_Person",
                    "@type": "unece:AssociationBIE",
                    "unece:cefactUNId": "UN01010134",
                    "unece:cefactBieDomainClass": "cefact:Logistics_TransportMovement.Details",
                    "rdfs:comment": "The officer responsible for the security of the means of transport used for this logistics transport movement."
                }
            ]
        },
        {
            "@id": "transport:transportMeansTypeCode",
            "@type": "rdf:Property",
            "schema:rangeIncludes": {
                "@id": "unece:UNECECL8179Code"
            },
            "schema:domainIncludes": {
                "@id": "transport:LogisticsTransportMeans"
            },
            "rdfs:comment": "The code specifying the type of logistics means of transport (Reference UNECE Recommendation 28).",
            "rdfs:label": "transportMeansTypeCode",
            "unece:cefactElementMetadata": [
                {
                    "@id": "cefact:Logistics_TransportMeans.Type.Code",
                    "@type": "unece:BasicBIE",
                    "unece:TDED": "8179",
                    "unece:cefactUNId": "UN01003820",
                    "unece:cefactBieDomainClass": "cefact:Logistics_TransportMeans.Details",
                    "rdfs:comment": "The code specifying the type of logistics means of transport (Reference UNECE Recommendation 28)."
                }
            ]
        },
        {
            "@id": "transport:transportMovementStageCode",
            "@type": "rdf:Property",
            "schema:rangeIncludes": {
                "@id": "unece:UNECECL8051Code"
            },
            "schema:domainIncludes": {
                "@id": "transport:LogisticsTransportMovement"
            },
            "rdfs:comment": "The code specifying the stage of this logistics transport movement.",
            "rdfs:label": "transportMovementStageCode",
            "unece:cefactElementMetadata": [
                {
                    "@id": "cefact:Logistics_TransportMovement.Stage.Code",
                    "@type": "unece:BasicBIE",
                    "unece:TDED": "8051",
                    "unece:cefactUNId": "UN01003838",
                    "unece:cefactBieDomainClass": "cefact:Logistics_TransportMovement.Details",
                    "rdfs:comment": "The code specifying the stage of this logistics transport movement."
                }
            ]
        },
        {
            "@id": "transport:transportPackage",
            "@type": "rdf:Property",
            "schema:rangeIncludes": {
                "@id": "transport:Package"
            },
            "schema:domainIncludes": [
                {
                    "@id": "transport:Referenced_SupplyChainConsignment"
                },
                {
                    "@id": "transport:Referenced_SupplyChainConsignmentItem"
                },
                {
                    "@id": "transport:SupplyChainConsignment"
                },
                {
                    "@id": "transport:SupplyChainConsignmentItem"
                }
            ],
            "rdfs:comment": [
                "A transport package for this referenced supply chain consignment item.",
                "A transport package for this supply chain consignment item.",
                "Transport packages for this referenced supply chain consignment.",
                "Transport packages for this supply chain consignment."
            ],
            "rdfs:label": "transportPackage",
            "unece:cefactElementMetadata": [
                {
                    "@id": "cefact:SupplyChain_Consignment.Transport.Logistics_Package",
                    "@type": "unece:AssociationBIE",
                    "unece:cefactUNId": "UN01004290",
                    "unece:cefactBieDomainClass": "cefact:SupplyChain_Consignment.Details",
                    "rdfs:comment": "Transport packages for this supply chain consignment."
                },
                {
                    "@id": "cefact:SupplyChain_ConsignmentItem.Transport.Logistics_Package",
                    "@type": "unece:AssociationBIE",
                    "unece:cefactUNId": "UN01004152",
                    "unece:cefactBieDomainClass": "cefact:SupplyChain_ConsignmentItem.Details",
                    "rdfs:comment": "A transport package for this supply chain consignment item."
                },
                {
                    "@id": "cefact:Referenced_SupplyChain_ConsignmentItem.Transport.Logistics_Package",
                    "@type": "unece:AssociationBIE",
                    "unece:cefactUNId": "UN01011043",
                    "unece:cefactBieDomainClass": "cefact:Referenced_SupplyChain_ConsignmentItem.Details",
                    "rdfs:comment": "A transport package for this referenced supply chain consignment item."
                },
                {
                    "@id": "cefact:Referenced_SupplyChain_Consignment.Transport.Logistics_Package",
                    "@type": "unece:AssociationBIE",
                    "unece:cefactUNId": "UN01011061",
                    "unece:cefactBieDomainClass": "cefact:Referenced_SupplyChain_Consignment.Details",
                    "rdfs:comment": "Transport packages for this referenced supply chain consignment."
                }
            ]
        },
        {
            "@id": "transport:transportService",
            "@type": "rdf:Property",
            "schema:rangeIncludes": {
                "@id": "transport:Service"
            },
            "schema:domainIncludes": [
                {
                    "@id": "transport:LogisticsTransportEquipment"
                },
                {
                    "@id": "transport:SupplyChainConsignment"
                }
            ],
            "rdfs:comment": [
                "A transport service for this piece of logistics transport equipment.",
                "A transport service for this supply chain consignment."
            ],
            "rdfs:label": "transportService",
            "unece:cefactElementMetadata": [
                {
                    "@id": "cefact:Logistics_TransportEquipment.Transport.Transport_Service",
                    "@type": "unece:AssociationBIE",
                    "unece:cefactUNId": "UN01008985",
                    "unece:cefactBieDomainClass": "cefact:Logistics_TransportEquipment.Details",
                    "rdfs:comment": "A transport service for this piece of logistics transport equipment."
                },
                {
                    "@id": "cefact:SupplyChain_Consignment.Transport.Transport_Service",
                    "@type": "unece:AssociationBIE",
                    "unece:cefactUNId": "UN01004284",
                    "unece:cefactBieDomainClass": "cefact:SupplyChain_Consignment.Details",
                    "rdfs:comment": "A transport service for this supply chain consignment."
                }
            ]
        },
        {
            "@id": "transport:transportServicePaymentArrangementCode",
            "@type": "rdf:Property",
            "schema:rangeIncludes": {
                "@id": "unece:UNECECL4237Code"
            },
            "schema:domainIncludes": {
                "@id": "transport:SupplyChainConsignment"
            },
            "rdfs:comment": "The code specifying the payment arrangements for this supply chain consignment.",
            "rdfs:label": "transportServicePaymentArrangementCode",
            "unece:cefactElementMetadata": [
                {
                    "@id": "cefact:SupplyChain_Consignment.PaymentArrangement.Code",
                    "@type": "unece:BasicBIE",
                    "unece:TDED": "4237",
                    "unece:cefactUNId": "UN01006139",
                    "unece:cefactBieDomainClass": "cefact:SupplyChain_Consignment.Details",
                    "rdfs:comment": "The code specifying the payment arrangements for this supply chain consignment."
                }
            ]
        },
        {
            "@id": "transport:transportServicesBuyerParty",
            "@type": "rdf:Property",
            "schema:rangeIncludes": {
                "@id": "transport:Party"
            },
            "schema:domainIncludes": [
                {
                    "@id": "transport:LogisticsTransportEquipment"
                },
                {
                    "@id": "transport:SupplyChainConsignment"
                }
            ],
            "rdfs:comment": [
                "The party which is the buyer of the transport services for this supply chain consignment.",
                "The transport services buyer party for this piece of logistics transport equipment."
            ],
            "rdfs:label": "transportServicesBuyerParty",
            "unece:cefactElementMetadata": [
                {
                    "@id": "cefact:SupplyChain_Consignment.TransportServicesBuyer.Trade_Party",
                    "@type": "unece:AssociationBIE",
                    "unece:cefactUNId": "UN01012665",
                    "unece:cefactBieDomainClass": "cefact:SupplyChain_Consignment.Details",
                    "rdfs:comment": "The party which is the buyer of the transport services for this supply chain consignment."
                },
                {
                    "@id": "cefact:Logistics_TransportEquipment.TransportServicesBuyer.Trade_Party",
                    "@type": "unece:AssociationBIE",
                    "unece:cefactUNId": "UN01003810",
                    "unece:cefactBieDomainClass": "cefact:Logistics_TransportEquipment.Details",
                    "rdfs:comment": "The transport services buyer party for this piece of logistics transport equipment."
                }
            ]
        },
        {
            "@id": "transport:transportSplitDescription",
            "@type": "rdf:Property",
            "schema:rangeIncludes": {
                "@id": "xsd:string"
            },
            "schema:domainIncludes": [
                {
                    "@id": "transport:Referenced_SupplyChainConsignment"
                },
                {
                    "@id": "transport:SupplyChainConsignment"
                }
            ],
            "rdfs:comment": [
                "The textual description of the transport split of this referenced supply chain consignment across different transport means or transport equipment.",
                "The textual description of the transport split of this supply chain consignment across different transport means or transport equipment."
            ],
            "rdfs:label": "transportSplitDescription",
            "unece:cefactElementMetadata": [
                {
                    "@id": "cefact:SupplyChain_Consignment.TransportSplitDescription.Text",
                    "@type": "unece:BasicBIE",
                    "unece:cefactUNId": "UN01004206",
                    "unece:cefactBieDomainClass": "cefact:SupplyChain_Consignment.Details",
                    "rdfs:comment": "The textual description of the transport split of this supply chain consignment across different transport means or transport equipment."
                },
                {
                    "@id": "cefact:Referenced_SupplyChain_Consignment.TransportSplitDescription.Text",
                    "@type": "unece:BasicBIE",
                    "unece:cefactUNId": "UN01004047",
                    "unece:cefactBieDomainClass": "cefact:Referenced_SupplyChain_Consignment.Details",
                    "rdfs:comment": "The textual description of the transport split of this referenced supply chain consignment across different transport means or transport equipment."
                }
            ]
        },
        {
            "@id": "transport:transportTemperature",
            "@type": "rdf:Property",
            "schema:rangeIncludes": {
                "@id": "transport:Temperature"
            },
            "schema:domainIncludes": {
                "@id": "transport:SupplyChainConsignmentItem"
            },
            "rdfs:comment": "The transport temperature setting for this supply chain consignment item.",
            "rdfs:label": "transportTemperature",
            "unece:cefactElementMetadata": [
                {
                    "@id": "cefact:SupplyChain_ConsignmentItem.Transport.TransportSetting_Temperature",
                    "@type": "unece:AssociationBIE",
                    "unece:cefactUNId": "UN01004134",
                    "unece:cefactBieDomainClass": "cefact:SupplyChain_ConsignmentItem.Details",
                    "rdfs:comment": "The transport temperature setting for this supply chain consignment item."
                }
            ]
        },
        {
            "@id": "transport:transportWasteSpecifiedInstructions",
            "@type": "rdf:Property",
            "schema:rangeIncludes": {
                "@id": "transport:Instructions"
            },
            "schema:domainIncludes": {
                "@id": "transport:LogisticsTransportMovement"
            },
            "rdfs:comment": "Transport waste disposal instructions specified for this logistics transport movement.",
            "rdfs:label": "transportWasteSpecifiedInstructions",
            "unece:cefactElementMetadata": [
                {
                    "@id": "cefact:Logistics_TransportMovement.TransportWaste_Specified.Disposal_Instructions",
                    "@type": "unece:AssociationBIE",
                    "unece:cefactUNId": "UN01013841",
                    "unece:cefactBieDomainClass": "cefact:Logistics_TransportMovement.Details",
                    "rdfs:comment": "Transport waste disposal instructions specified for this logistics transport movement."
                }
            ]
        },
        {
            "@id": "transport:transportationWasteRecoveryDisposalProcessTypeCode",
            "@type": "rdf:Property",
            "schema:rangeIncludes": {
                "@id": "unece:UNECECL7187Code"
            },
            "schema:domainIncludes": {
                "@id": "transport:TransportationWasteRecoveryDisposalProcess"
            },
            "rdfs:comment": "The code specifying the type of transportation waste recovery disposal process.",
            "rdfs:label": "transportationWasteRecoveryDisposalProcessTypeCode",
            "unece:cefactElementMetadata": [
                {
                    "@id": "cefact:TransportationWasteRecoveryDisposal_Process.Type.Code",
                    "@type": "unece:BasicBIE",
                    "unece:TDED": "7187",
                    "unece:cefactUNId": "UN01014617",
                    "unece:cefactBieDomainClass": "cefact:TransportationWasteRecoveryDisposal_Process.Details",
                    "rdfs:comment": "The code specifying the type of transportation waste recovery disposal process."
                }
            ]
        },
        {
            "@id": "transport:transshipmentIntermediateEvent",
            "@type": "rdf:Property",
            "schema:rangeIncludes": {
                "@id": "transport:Event"
            },
            "schema:domainIncludes": {
                "@id": "transport:LogisticsTransportMovement"
            },
            "rdfs:comment": "A transshipment intermediate event during this logistics transport movement.",
            "rdfs:label": "transshipmentIntermediateEvent",
            "unece:cefactElementMetadata": [
                {
                    "@id": "cefact:Logistics_TransportMovement.Transshipment_Intermediate.Transport_Event",
                    "@type": "unece:AssociationBIE",
                    "unece:cefactUNId": "UN01008987",
                    "unece:cefactBieDomainClass": "cefact:Logistics_TransportMovement.Details",
                    "rdfs:comment": "A transshipment intermediate event during this logistics transport movement."
                }
            ]
        },
        {
            "@id": "transport:transshipmentLocation",
            "@type": "rdf:Property",
            "schema:rangeIncludes": {
                "@id": "transport:Location"
            },
            "schema:domainIncludes": {
                "@id": "transport:SupplyChainConsignment"
            },
            "rdfs:comment": "A transshipment location for this supply chain consignment.",
            "rdfs:label": "transshipmentLocation",
            "unece:cefactElementMetadata": [
                {
                    "@id": "cefact:SupplyChain_Consignment.Transshipment.Logistics_Location",
                    "@type": "unece:AssociationBIE",
                    "unece:cefactUNId": "UN01004236",
                    "unece:cefactBieDomainClass": "cefact:SupplyChain_Consignment.Details",
                    "rdfs:comment": "A transshipment location for this supply chain consignment."
                }
            ]
        },
        {
            "@id": "transport:transshipmentPermissionIndicator",
            "@type": "rdf:Property",
            "schema:rangeIncludes": {
                "@id": "xsd:boolean"
            },
            "schema:domainIncludes": {
                "@id": "transport:SupplyChainConsignment"
            },
            "rdfs:comment": "The indication of whether or not transshipment is permitted for this supply chain consignment.",
            "rdfs:label": "transshipmentPermissionIndicator",
            "unece:cefactElementMetadata": [
                {
                    "@id": "cefact:SupplyChain_Consignment.TransshipmentPermission.Indicator",
                    "@type": "unece:BasicBIE",
                    "unece:cefactUNId": "UN01012579",
                    "unece:cefactBieDomainClass": "cefact:SupplyChain_Consignment.Details",
                    "rdfs:comment": "The indication of whether or not transshipment is permitted for this supply chain consignment."
                }
            ]
        },
        {
            "@id": "transport:type",
            "@type": "rdf:Property",
            "schema:rangeIncludes": {
                "@id": "xsd:string"
            },
            "schema:domainIncludes": [
                {
                    "@id": "transport:LogisticsPackaging"
                },
                {
                    "@id": "transport:LogisticsTransportMeans"
                },
                {
                    "@id": "transport:LogisticsTransportMovement"
                },
                {
                    "@id": "transport:SupplyChainPackaging"
                }
            ],
            "rdfs:comment": [
                "The type, as expressed as text, of the logistics transport movement.",
                "The type, expressed as text, of supply chain packaging.",
                "The type, expressed as text, of this logistics means of transport.",
                "The type, expressed as text, of this logistics packaging."
            ],
            "rdfs:label": "type",
            "unece:cefactElementMetadata": [
                {
                    "@id": "cefact:Logistics_Packaging.Type.Text",
                    "@type": "unece:BasicBIE",
                    "unece:TDED": "7064",
                    "unece:cefactUNId": "UN01014950",
                    "unece:cefactBieDomainClass": "cefact:Logistics_Packaging.Details",
                    "rdfs:comment": "The type, expressed as text, of this logistics packaging."
                },
                {
                    "@id": "cefact:SupplyChain_Packaging.Type.Text",
                    "@type": "unece:BasicBIE",
                    "unece:TDED": "7064",
                    "unece:cefactUNId": "UN01004314",
                    "unece:cefactBieDomainClass": "cefact:SupplyChain_Packaging.Details",
                    "rdfs:comment": "The type, expressed as text, of supply chain packaging."
                },
                {
                    "@id": "cefact:Logistics_TransportMovement.Type.Text",
                    "@type": "unece:BasicBIE",
                    "unece:cefactUNId": "UN01012753",
                    "unece:cefactBieDomainClass": "cefact:Logistics_TransportMovement.Details",
                    "rdfs:comment": "The type, as expressed as text, of the logistics transport movement."
                },
                {
                    "@id": "cefact:Logistics_TransportMeans.Type.Text",
                    "@type": "unece:BasicBIE",
                    "unece:TDED": "8178",
                    "unece:cefactUNId": "UN01003821",
                    "unece:cefactBieDomainClass": "cefact:Logistics_TransportMeans.Details",
                    "rdfs:comment": "The type, expressed as text, of this logistics means of transport."
                }
            ]
        },
        {
            "@id": "transport:typeCode",
            "@type": "rdf:Property",
            "schema:rangeIncludes": {
                "@id": "xsd:token"
            },
            "schema:domainIncludes": [
                {
                    "@id": "transport:CalculatedEmission"
                },
                {
                    "@id": "transport:LogisticsPackaging"
                },
                {
                    "@id": "transport:Referenced_SupplyChainConsignmentItem"
                },
                {
                    "@id": "transport:SupplyChainConsignmentItem"
                },
                {
                    "@id": "transport:SupplyChainPackaging"
                }
            ],
            "rdfs:comment": [
                "A code specifying a type of logistics packaging.",
                "The code specifying the type of referenced supply chain consignment item.",
                "The code specifying the type of supply chain consignment item.",
                "The code specifying the type of supply chain packaging.",
                "The code specifying the type of this calculated emission."
            ],
            "rdfs:label": "typeCode",
            "unece:cefactElementMetadata": [
                {
                    "@id": "cefact:Logistics_Packaging.Type.Code",
                    "@type": "unece:BasicBIE",
                    "unece:TDED": "7065",
                    "unece:cefactUNId": "UN01014949",
                    "unece:cefactBieDomainClass": "cefact:Logistics_Packaging.Details",
                    "rdfs:comment": "A code specifying a type of logistics packaging."
                },
                {
                    "@id": "cefact:SupplyChain_Packaging.Type.Code",
                    "@type": "unece:BasicBIE",
                    "unece:TDED": "7065",
                    "unece:cefactUNId": "UN01004313",
                    "unece:cefactBieDomainClass": "cefact:SupplyChain_Packaging.Details",
                    "rdfs:comment": "The code specifying the type of supply chain packaging."
                },
                {
                    "@id": "cefact:SupplyChain_ConsignmentItem.Type.Code",
                    "@type": "unece:BasicBIE",
                    "unece:TDED": "7357",
                    "unece:cefactUNId": "UN01004106",
                    "unece:cefactBieDomainClass": "cefact:SupplyChain_ConsignmentItem.Details",
                    "rdfs:comment": "The code specifying the type of supply chain consignment item."
                },
                {
                    "@id": "cefact:Referenced_SupplyChain_ConsignmentItem.Type.Code",
                    "@type": "unece:BasicBIE",
                    "unece:TDED": "7357",
                    "unece:cefactUNId": "UN01004037",
                    "unece:cefactBieDomainClass": "cefact:Referenced_SupplyChain_ConsignmentItem.Details",
                    "rdfs:comment": "The code specifying the type of referenced supply chain consignment item."
                },
                {
                    "@id": "cefact:Calculated_Emission.Type.Code",
                    "@type": "unece:BasicBIE",
                    "unece:cefactUNId": "UN01010052",
                    "unece:cefactBieDomainClass": "cefact:Calculated_Emission.Details",
                    "rdfs:comment": "The code specifying the type of this calculated emission."
                }
            ]
        },
        {
            "@id": "transport:typeExtensionCode",
            "@type": "rdf:Property",
            "schema:rangeIncludes": {
                "@id": "xsd:token"
            },
            "schema:domainIncludes": [
                {
                    "@id": "transport:Referenced_SupplyChainConsignmentItem"
                },
                {
                    "@id": "transport:SupplyChainConsignmentItem"
                }
            ],
            "rdfs:comment": [
                "The code used as an extension to the type code for further specifying the type of referenced supply chain consignment item.",
                "The code used as an extension to the type code for further specifying the type of supply chain consignment item."
            ],
            "rdfs:label": "typeExtensionCode",
            "unece:cefactElementMetadata": [
                {
                    "@id": "cefact:Referenced_SupplyChain_ConsignmentItem.TypeExtension.Code",
                    "@type": "unece:BasicBIE",
                    "unece:TDED": "7361",
                    "unece:cefactUNId": "UN01004038",
                    "unece:cefactBieDomainClass": "cefact:Referenced_SupplyChain_ConsignmentItem.Details",
                    "rdfs:comment": "The code used as an extension to the type code for further specifying the type of referenced supply chain consignment item."
                },
                {
                    "@id": "cefact:SupplyChain_ConsignmentItem.TypeExtension.Code",
                    "@type": "unece:BasicBIE",
                    "unece:TDED": "7361",
                    "unece:cefactUNId": "UN01004107",
                    "unece:cefactBieDomainClass": "cefact:SupplyChain_ConsignmentItem.Details",
                    "rdfs:comment": "The code used as an extension to the type code for further specifying the type of supply chain consignment item."
                }
            ]
        },
        {
            "@id": "transport:unitQuantity",
            "@type": "rdf:Property",
            "schema:rangeIncludes": {
                "@id": "xsd:decimal"
            },
            "schema:domainIncludes": [
                {
                    "@id": "transport:AssociatedTransportEquipment"
                },
                {
                    "@id": "transport:AttachedTransportEquipment"
                },
                {
                    "@id": "transport:LogisticsTransportEquipment"
                },
                {
                    "@id": "transport:Referenced_LogisticsTransportEquipment"
                }
            ],
            "rdfs:comment": [
                "The number of units of attached transport equipment.",
                "The number of units of this type of associated transport equipment.",
                "The number of units of this type of logistics transport equipment.",
                "The number of units of this type of referenced logistics transport equipment."
            ],
            "rdfs:label": "unitQuantity",
            "unece:cefactElementMetadata": [
                {
                    "@id": "cefact:Associated_TransportEquipment.Unit.Quantity",
                    "@type": "unece:BasicBIE",
                    "unece:TDED": "6350",
                    "unece:cefactUNId": "UN01013659",
                    "unece:cefactBieDomainClass": "cefact:Associated_TransportEquipment.Details",
                    "rdfs:comment": "The number of units of this type of associated transport equipment."
                },
                {
                    "@id": "cefact:Attached_TransportEquipment.Unit.Quantity",
                    "@type": "unece:BasicBIE",
                    "unece:TDED": "6350",
                    "unece:cefactUNId": "UN01008955",
                    "unece:cefactBieDomainClass": "cefact:Attached_TransportEquipment.Details",
                    "rdfs:comment": "The number of units of attached transport equipment."
                },
                {
                    "@id": "cefact:Logistics_TransportEquipment.Unit.Quantity",
                    "@type": "unece:BasicBIE",
                    "unece:TDED": "6350",
                    "unece:cefactUNId": "UN01008981",
                    "unece:cefactBieDomainClass": "cefact:Logistics_TransportEquipment.Details",
                    "rdfs:comment": "The number of units of this type of logistics transport equipment."
                },
                {
                    "@id": "cefact:Referenced_Logistics_TransportEquipment.Unit.Quantity",
                    "@type": "unece:BasicBIE",
                    "unece:TDED": "6350",
                    "unece:cefactUNId": "UN01008992",
                    "unece:cefactBieDomainClass": "cefact:Referenced_Logistics_TransportEquipment.Details",
                    "rdfs:comment": "The number of units of this type of referenced logistics transport equipment."
                }
            ]
        },
        {
            "@id": "transport:unloadingBaseportLocation",
            "@type": "rdf:Property",
            "schema:rangeIncludes": {
                "@id": "transport:Location"
            },
            "schema:domainIncludes": {
                "@id": "transport:SupplyChainConsignment"
            },
            "rdfs:comment": "The baseport location at which this supply chain consignment is to be unloaded from a means of transport according to the transport contract.",
            "rdfs:label": "unloadingBaseportLocation",
            "unece:cefactElementMetadata": [
                {
                    "@id": "cefact:SupplyChain_Consignment.UnloadingBaseport.Logistics_Location",
                    "@type": "unece:AssociationBIE",
                    "unece:cefactUNId": "UN01004239",
                    "unece:cefactBieDomainClass": "cefact:SupplyChain_Consignment.Details",
                    "rdfs:comment": "The baseport location at which this supply chain consignment is to be unloaded from a means of transport according to the transport contract."
                }
            ]
        },
        {
            "@id": "transport:unloadingEvent",
            "@type": "rdf:Property",
            "schema:rangeIncludes": {
                "@id": "transport:Event"
            },
            "schema:domainIncludes": [
                {
                    "@id": "transport:LogisticsTransportEquipment"
                },
                {
                    "@id": "transport:LogisticsTransportMovement"
                }
            ],
            "rdfs:comment": [
                "The unloading event during which goods will be or have been unloaded from the means of transport used for this logistics transport movement.",
                "The unloading event for this piece of logistics transport equipment."
            ],
            "rdfs:label": "unloadingEvent",
            "unece:cefactElementMetadata": [
                {
                    "@id": "cefact:Logistics_TransportMovement.Unloading.Transport_Event",
                    "@type": "unece:AssociationBIE",
                    "unece:cefactUNId": "UN01003857",
                    "unece:cefactBieDomainClass": "cefact:Logistics_TransportMovement.Details",
                    "rdfs:comment": "The unloading event during which goods will be or have been unloaded from the means of transport used for this logistics transport movement."
                },
                {
                    "@id": "cefact:Logistics_TransportEquipment.Unloading.Transport_Event",
                    "@type": "unece:AssociationBIE",
                    "unece:cefactUNId": "UN01003803",
                    "unece:cefactBieDomainClass": "cefact:Logistics_TransportEquipment.Details",
                    "rdfs:comment": "The unloading event for this piece of logistics transport equipment."
                }
            ]
        },
        {
            "@id": "transport:unloadingInspectionParty",
            "@type": "rdf:Property",
            "schema:rangeIncludes": {
                "@id": "transport:Party"
            },
            "schema:domainIncludes": {
                "@id": "transport:LogisticsTransportMovement"
            },
            "rdfs:comment": "The inspection party for the unloading of this logistics transport movement.",
            "rdfs:label": "unloadingInspectionParty",
            "unece:cefactElementMetadata": [
                {
                    "@id": "cefact:Logistics_TransportMovement.Unloading_Inspection.Trade_Party",
                    "@type": "unece:AssociationBIE",
                    "unece:cefactUNId": "UN01003871",
                    "unece:cefactBieDomainClass": "cefact:Logistics_TransportMovement.Details",
                    "rdfs:comment": "The inspection party for the unloading of this logistics transport movement."
                }
            ]
        },
        {
            "@id": "transport:unloadingInspectionSpecifiedInstructions",
            "@type": "rdf:Property",
            "schema:rangeIncludes": {
                "@id": "transport:Instructions"
            },
            "schema:domainIncludes": {
                "@id": "transport:LogisticsTransportMovement"
            },
            "rdfs:comment": "Unloading inspection instructions specified for this logistics transport movement.",
            "rdfs:label": "unloadingInspectionSpecifiedInstructions",
            "unece:cefactElementMetadata": [
                {
                    "@id": "cefact:Logistics_TransportMovement.UnloadingInspection_Specified.Transport_Instructions",
                    "@type": "unece:AssociationBIE",
                    "unece:cefactUNId": "UN01003881",
                    "unece:cefactBieDomainClass": "cefact:Logistics_TransportMovement.Details",
                    "rdfs:comment": "Unloading inspection instructions specified for this logistics transport movement."
                }
            ]
        },
        {
            "@id": "transport:unloadingInstructions",
            "@type": "rdf:Property",
            "schema:rangeIncludes": {
                "@id": "transport:Instructions"
            },
            "schema:domainIncludes": {
                "@id": "transport:LogisticsTransportEquipment"
            },
            "rdfs:comment": "Unloading instructions for this piece of logistics transport equipment.",
            "rdfs:label": "unloadingInstructions",
            "unece:cefactElementMetadata": [
                {
                    "@id": "cefact:Logistics_TransportEquipment.Unloading.Transport_Instructions",
                    "@type": "unece:AssociationBIE",
                    "unece:cefactUNId": "UN01003792",
                    "unece:cefactBieDomainClass": "cefact:Logistics_TransportEquipment.Details",
                    "rdfs:comment": "Unloading instructions for this piece of logistics transport equipment."
                }
            ]
        },
        {
            "@id": "transport:unloadingLocation",
            "@type": "rdf:Property",
            "schema:rangeIncludes": {
                "@id": "transport:Location"
            },
            "schema:domainIncludes": {
                "@id": "transport:SupplyChainConsignment"
            },
            "rdfs:comment": "The logistics location where the supply chain consignment is unloaded.",
            "rdfs:label": "unloadingLocation",
            "unece:cefactElementMetadata": [
                {
                    "@id": "cefact:SupplyChain_Consignment.Unloading.Logistics_Location",
                    "@type": "unece:AssociationBIE",
                    "unece:cefactUNId": "UN01013113",
                    "unece:cefactBieDomainClass": "cefact:SupplyChain_Consignment.Details",
                    "rdfs:comment": "The logistics location where the supply chain consignment is unloaded."
                }
            ]
        },
        {
            "@id": "transport:unloadingReportedEvent",
            "@type": "rdf:Property",
            "schema:rangeIncludes": {
                "@id": "transport:Event"
            },
            "schema:domainIncludes": {
                "@id": "trade:LogisticsStatus"
            },
            "rdfs:comment": "A transport unloading event reported for this logistics status.",
            "rdfs:label": "unloadingReportedEvent",
            "unece:cefactElementMetadata": [
                {
                    "@id": "cefact:Logistics_Status.Unloading_Reported.Transport_Event",
                    "@type": "unece:AssociationBIE",
                    "unece:cefactUNId": "UN01010096",
                    "unece:cefactBieDomainClass": "cefact:Logistics_Status.Details",
                    "rdfs:comment": "A transport unloading event reported for this logistics status."
                }
            ]
        },
        {
            "@id": "transport:unloadingSequenceNumeric",
            "@type": "rdf:Property",
            "schema:rangeIncludes": {
                "@id": "xsd:decimal"
            },
            "schema:domainIncludes": [
                {
                    "@id": "transport:LogisticsTransportEquipment"
                },
                {
                    "@id": "transport:SupplyChainConsignment"
                }
            ],
            "rdfs:comment": [
                "The sequence number differentiating this piece of logistics transport equipment from others during unloading.",
                "The unloading sequence number for this supply chain consignment."
            ],
            "rdfs:label": "unloadingSequenceNumeric",
            "unece:cefactElementMetadata": [
                {
                    "@id": "cefact:Logistics_TransportEquipment.UnloadingSequence.Numeric",
                    "@type": "unece:BasicBIE",
                    "unece:cefactUNId": "UN01010097",
                    "unece:cefactBieDomainClass": "cefact:Logistics_TransportEquipment.Details",
                    "rdfs:comment": "The sequence number differentiating this piece of logistics transport equipment from others during unloading."
                },
                {
                    "@id": "cefact:SupplyChain_Consignment.UnloadingSequence.Numeric",
                    "@type": "unece:BasicBIE",
                    "unece:cefactUNId": "UN01010141",
                    "unece:cefactBieDomainClass": "cefact:SupplyChain_Consignment.Details",
                    "rdfs:comment": "The unloading sequence number for this supply chain consignment."
                }
            ]
        },
        {
            "@id": "transport:usedTransportMeans",
            "@type": "rdf:Property",
            "schema:rangeIncludes": {
                "@id": "transport:TransportMeans"
            },
            "schema:domainIncludes": {
                "@id": "transport:LogisticsTransportMovement"
            },
            "rdfs:comment": "The means of transport used for this logistics transport movement.",
            "rdfs:label": "usedTransportMeans",
            "unece:cefactElementMetadata": [
                {
                    "@id": "cefact:Logistics_TransportMovement.Used.Logistics_TransportMeans",
                    "@type": "unece:AssociationBIE",
                    "unece:cefactUNId": "UN01003861",
                    "unece:cefactBieDomainClass": "cefact:Logistics_TransportMovement.Details",
                    "rdfs:comment": "The means of transport used for this logistics transport movement."
                }
            ]
        },
        {
            "@id": "transport:utilizedTransportEquipment",
            "@type": "rdf:Property",
            "schema:rangeIncludes": {
                "@id": "transport:TransportEquipment"
            },
            "schema:domainIncludes": [
                {
                    "@id": "transport:Referenced_SupplyChainConsignment"
                },
                {
                    "@id": "transport:SupplyChainConsignment"
                }
            ],
            "rdfs:comment": [
                "Logistics transport equipment utilized for this referenced supply chain consignment.",
                "Logistics transport equipment utilized for this supply chain consignment."
            ],
            "rdfs:label": "utilizedTransportEquipment",
            "unece:cefactElementMetadata": [
                {
                    "@id": "cefact:Referenced_SupplyChain_Consignment.Utilized.Logistics_TransportEquipment",
                    "@type": "unece:AssociationBIE",
                    "unece:cefactUNId": "UN01011067",
                    "unece:cefactBieDomainClass": "cefact:Referenced_SupplyChain_Consignment.Details",
                    "rdfs:comment": "Logistics transport equipment utilized for this referenced supply chain consignment."
                },
                {
                    "@id": "cefact:SupplyChain_Consignment.Utilized.Logistics_TransportEquipment",
                    "@type": "unece:AssociationBIE",
                    "unece:cefactUNId": "UN01004260",
                    "unece:cefactBieDomainClass": "cefact:SupplyChain_Consignment.Details",
                    "rdfs:comment": "Logistics transport equipment utilized for this supply chain consignment."
                }
            ]
        },
        {
            "@id": "transport:vINLabel",
            "@type": "rdf:Property",
            "schema:rangeIncludes": {
                "@id": "transport:Label"
            },
            "schema:domainIncludes": {
                "@id": "transport:LogisticsShippingMarks"
            },
            "rdfs:comment": "A Vehicle Identification Number (VIN) label that is a part of these logistics shipping marks.",
            "rdfs:label": "vINLabel",
            "unece:cefactElementMetadata": [
                {
                    "@id": "cefact:Logistics_ShippingMarks.VIN.Logistics_Label",
                    "@type": "unece:AssociationBIE",
                    "unece:cefactUNId": "UN01003746",
                    "unece:cefactBieDomainClass": "cefact:Logistics_ShippingMarks.Details",
                    "rdfs:comment": "A Vehicle Identification Number (VIN) label that is a part of these logistics shipping marks."
                }
            ]
        },
        {
            "@id": "transport:validityPeriod",
            "@type": "rdf:Property",
            "schema:rangeIncludes": {
                "@id": "transport:Period"
            },
            "schema:domainIncludes": {
                "@id": "trade:LogisticsStatus"
            },
            "rdfs:comment": "A specific validity period for this logistics status.",
            "rdfs:label": "validityPeriod",
            "unece:cefactElementMetadata": [
                {
                    "@id": "cefact:Logistics_Status.Validity.Specified_Period",
                    "@type": "unece:AssociationBIE",
                    "unece:cefactUNId": "UN01010092",
                    "unece:cefactBieDomainClass": "cefact:Logistics_Status.Details",
                    "rdfs:comment": "A specific validity period for this logistics status."
                }
            ]
        },
        {
            "@id": "transport:vanningEvent",
            "@type": "rdf:Property",
            "schema:rangeIncludes": {
                "@id": "transport:Event"
            },
            "schema:domainIncludes": [
                {
                    "@id": "transport:Referenced_SupplyChainConsignment"
                },
                {
                    "@id": "transport:SupplyChainConsignment"
                },
                {
                    "@id": "transport:SupplyChainConsignmentItem"
                }
            ],
            "rdfs:comment": [
                "The vanning event (the loading of this consignment at the place of its original despatch) for this referenced supply chain consignment.",
                "The vanning event for this supply chain consignment item, i.e. the loading of this consignment item at the place of original despatch.",
                "The vanning event for this supply chain consignment, i.e. the loading of this consignment at the place of original despatch."
            ],
            "rdfs:label": "vanningEvent",
            "unece:cefactElementMetadata": [
                {
                    "@id": "cefact:SupplyChain_ConsignmentItem.Vanning.Transport_Event",
                    "@type": "unece:AssociationBIE",
                    "unece:cefactUNId": "UN01004158",
                    "unece:cefactBieDomainClass": "cefact:SupplyChain_ConsignmentItem.Details",
                    "rdfs:comment": "The vanning event for this supply chain consignment item, i.e. the loading of this consignment item at the place of original despatch."
                },
                {
                    "@id": "cefact:SupplyChain_Consignment.Vanning.Transport_Event",
                    "@type": "unece:AssociationBIE",
                    "unece:cefactUNId": "UN01004257",
                    "unece:cefactBieDomainClass": "cefact:SupplyChain_Consignment.Details",
                    "rdfs:comment": "The vanning event for this supply chain consignment, i.e. the loading of this consignment at the place of original despatch."
                },
                {
                    "@id": "cefact:Referenced_SupplyChain_Consignment.Vanning.Transport_Event",
                    "@type": "unece:AssociationBIE",
                    "unece:cefactUNId": "UN01011062",
                    "unece:cefactBieDomainClass": "cefact:Referenced_SupplyChain_Consignment.Details",
                    "rdfs:comment": "The vanning event (the loading of this consignment at the place of its original despatch) for this referenced supply chain consignment."
                }
            ]
        },
        {
            "@id": "transport:warehouseArrivalDateTime",
            "@type": "rdf:Property",
            "schema:rangeIncludes": {
                "@id": "xsd:dateTime"
            },
            "schema:domainIncludes": {
                "@id": "transport:SupplyChainConsignment"
            },
            "rdfs:comment": "The date, time, date time or other date time value of the arrival of this supply chain consignment at a warehouse.",
            "rdfs:label": "warehouseArrivalDateTime",
            "unece:cefactElementMetadata": [
                {
                    "@id": "cefact:SupplyChain_Consignment.WarehouseArrival.DateTime",
                    "@type": "unece:BasicBIE",
                    "unece:cefactUNId": "UN01004172",
                    "unece:cefactBieDomainClass": "cefact:SupplyChain_Consignment.Details",
                    "rdfs:comment": "The date, time, date time or other date time value of the arrival of this supply chain consignment at a warehouse."
                }
            ]
        },
        {
            "@id": "transport:warehouseDepositorParty",
            "@type": "rdf:Property",
            "schema:rangeIncludes": {
                "@id": "transport:Party"
            },
            "schema:domainIncludes": {
                "@id": "transport:SupplyChainConsignment"
            },
            "rdfs:comment": "A party depositing goods in a warehouse for this supply chain consignment.",
            "rdfs:label": "warehouseDepositorParty",
            "unece:cefactElementMetadata": [
                {
                    "@id": "cefact:SupplyChain_Consignment.WarehouseDepositor.Trade_Party",
                    "@type": "unece:AssociationBIE",
                    "unece:cefactUNId": "UN01014892",
                    "unece:cefactBieDomainClass": "cefact:SupplyChain_Consignment.Details",
                    "rdfs:comment": "A party depositing goods in a warehouse for this supply chain consignment."
                }
            ]
        },
        {
            "@id": "transport:warehouseKeeperParty",
            "@type": "rdf:Property",
            "schema:rangeIncludes": {
                "@id": "transport:Party"
            },
            "schema:domainIncludes": {
                "@id": "transport:SupplyChainConsignment"
            },
            "rdfs:comment": "A party taking responsibility for goods stored in a warehouse for this supply chain consignment.",
            "rdfs:label": "warehouseKeeperParty",
            "unece:cefactElementMetadata": [
                {
                    "@id": "cefact:SupplyChain_Consignment.WarehouseKeeper.Trade_Party",
                    "@type": "unece:AssociationBIE",
                    "unece:cefactUNId": "UN01014891",
                    "unece:cefactBieDomainClass": "cefact:SupplyChain_Consignment.Details",
                    "rdfs:comment": "A party taking responsibility for goods stored in a warehouse for this supply chain consignment."
                }
            ]
        },
        {
            "@id": "transport:warehouseOperatorParty",
            "@type": "rdf:Property",
            "schema:rangeIncludes": {
                "@id": "transport:Party"
            },
            "schema:domainIncludes": {
                "@id": "transport:SupplyChainConsignment"
            },
            "rdfs:comment": "A party that operates a warehouse in which goods are stored for this supply chain consignment.",
            "rdfs:label": "warehouseOperatorParty",
            "unece:cefactElementMetadata": [
                {
                    "@id": "cefact:SupplyChain_Consignment.WarehouseOperator.Trade_Party",
                    "@type": "unece:AssociationBIE",
                    "unece:cefactUNId": "UN01014890",
                    "unece:cefactBieDomainClass": "cefact:SupplyChain_Consignment.Details",
                    "rdfs:comment": "A party that operates a warehouse in which goods are stored for this supply chain consignment."
                }
            ]
        },
        {
            "@id": "transport:warehouseStorageEvent",
            "@type": "rdf:Property",
            "schema:rangeIncludes": {
                "@id": "transport:Event"
            },
            "schema:domainIncludes": {
                "@id": "transport:Referenced_SupplyChainConsignment"
            },
            "rdfs:comment": "A warehouse storage event for this referenced supply chain consignment.",
            "rdfs:label": "warehouseStorageEvent",
            "unece:cefactElementMetadata": [
                {
                    "@id": "cefact:Referenced_SupplyChain_Consignment.Warehouse_Storage.Transport_Event",
                    "@type": "unece:AssociationBIE",
                    "unece:cefactUNId": "UN01011068",
                    "unece:cefactBieDomainClass": "cefact:Referenced_SupplyChain_Consignment.Details",
                    "rdfs:comment": "A warehouse storage event for this referenced supply chain consignment."
                }
            ]
        },
        {
            "@id": "transport:wasteReportingExemptionIndicator",
            "@type": "rdf:Property",
            "schema:rangeIncludes": {
                "@id": "xsd:boolean"
            },
            "schema:domainIncludes": {
                "@id": "transport:LogisticsTransportMeans"
            },
            "rdfs:comment": "The indication of whether or not there is a waste reporting exemption for this logistics means of transport.",
            "rdfs:label": "wasteReportingExemptionIndicator",
            "unece:cefactElementMetadata": [
                {
                    "@id": "cefact:Logistics_TransportMeans.WasteReportingExemption.Indicator",
                    "@type": "unece:BasicBIE",
                    "unece:cefactUNId": "UN01010107",
                    "unece:cefactBieDomainClass": "cefact:Logistics_TransportMeans.Details",
                    "rdfs:comment": "The indication of whether or not there is a waste reporting exemption for this logistics means of transport."
                }
            ]
        },
        {
            "@id": "transport:weightMeasure",
            "@type": "rdf:Property",
            "schema:rangeIncludes": {
                "@id": "xsd:decimal"
            },
            "schema:domainIncludes": [
                {
                    "@id": "transport:CalculatedEmission"
                },
                {
                    "@id": "transport:LogisticsPackaging"
                },
                {
                    "@id": "transport:SupplyChainPackaging"
                }
            ],
            "rdfs:comment": [
                "A measure of a weight (mass) of this logistics packaging.",
                "A measure of the weight of this supply chain packaging.",
                "A weight for which this calculated emission is measured."
            ],
            "rdfs:label": "weightMeasure",
            "unece:cefactElementMetadata": [
                {
                    "@id": "cefact:Logistics_Packaging.Weight.Measure",
                    "@type": "unece:BasicBIE",
                    "unece:cefactUNId": "UN01014957",
                    "unece:cefactBieDomainClass": "cefact:Logistics_Packaging.Details",
                    "rdfs:comment": "A measure of a weight (mass) of this logistics packaging."
                },
                {
                    "@id": "cefact:Calculated_Emission.Weight.Measure",
                    "@type": "unece:BasicBIE",
                    "unece:TDED": "6411",
                    "unece:cefactUNId": "UN01010054",
                    "unece:cefactBieDomainClass": "cefact:Calculated_Emission.Details",
                    "rdfs:comment": "A weight for which this calculated emission is measured."
                },
                {
                    "@id": "cefact:SupplyChain_Packaging.Weight.Measure",
                    "@type": "unece:BasicBIE",
                    "unece:cefactUNId": "UN01004319",
                    "unece:cefactBieDomainClass": "cefact:SupplyChain_Packaging.Details",
                    "rdfs:comment": "A measure of the weight of this supply chain packaging."
                }
            ]
        }
    ]
}